@prefix piirrite: <http://piirrite.univ-lyon1.fr/ontology/core#> .
@prefix piirritev: <http://piirrite.univ-lyon1.fr/vocabulary#> .
@prefix rdfs: <http://www.w3.org/2000/01/rdf-schema#> .
@prefix skos: <http://www.w3.org/2004/02/skos/core#> .

piirritev:OsmAbandoned a skos:ConceptScheme ;
    piirrite:osmId "abandoned" ;
    skos:definition "A man-made feature abandoned and no longer maintained. Also see key:abandoned:*."@en ;
    skos:prefLabel "Abandoned, types"@en .

piirritev:OsmAccessAgricultural a skos:Concept ;
    piirrite:osmId "agricultural" ;
    rdfs:subClassOf piirrite:OsmEntity ;
    skos:definition "Restricted to usage of the road for agricultural purposes (for any type of transportation mode)"@en ;
    skos:inScheme piirritev:OsmAccess ;
    skos:prefLabel "Agricultural"@en .

piirritev:OsmAccessCustomers a skos:Concept ;
    piirrite:osmId "customers" ;
    rdfs:subClassOf piirrite:OsmEntity ;
    skos:definition "Restricted to customers at the destination."@en ;
    skos:inScheme piirritev:OsmAccess ;
    skos:prefLabel "Customers"@en .

piirritev:OsmAccessDelivery a skos:Concept ;
    piirrite:hasRelatedOsmTag piirrite:hasOsmDeliveryHighway ;
    piirrite:osmId "delivery" ;
    rdfs:subClassOf piirrite:OsmEntity ;
    skos:definition "Access only when delivering"@en ;
    skos:inScheme piirritev:OsmAccess ;
    skos:prefLabel "Delivery"@en .

piirritev:OsmAccessDesignated a skos:Concept ;
    piirrite:osmId "designated" ;
    rdfs:subClassOf piirrite:OsmEntity ;
    skos:definition "A way marked for a particular use. Only used with a specific mode of transport!"@en ;
    skos:inScheme piirritev:OsmAccess ;
    skos:prefLabel "Designated"@en .

piirritev:OsmAccessDestination a skos:Concept ;
    piirrite:hasRelatedOsmTag piirrite:hasOsmDestinationHighway,
        piirrite:hasOsmDestinationWaterway ;
    piirrite:osmId "destination" ;
    rdfs:subClassOf piirrite:OsmEntity ;
    skos:definition "Through traffic of all modes of transportation forbidden, non-through traffic users allowed"@en ;
    skos:inScheme piirritev:OsmAccess ;
    skos:prefLabel "Destination"@en .

piirritev:OsmAccessForestry a skos:Concept ;
    piirrite:osmId "forestry" ;
    rdfs:subClassOf piirrite:OsmEntity ;
    skos:definition "Value that restricts access to the road to usage for forestry purposes (not restricted to a technical class of vehicles)."@en ;
    skos:inScheme piirritev:OsmAccess ;
    skos:prefLabel "Forestry"@en .

piirritev:OsmAccessMilitary a skos:Concept ;
    piirrite:osmId "military" ;
    rdfs:subClassOf piirrite:OsmEntity ;
    skos:definition "Only for military vehicles and vehicles on military business."@en ;
    skos:inScheme piirritev:OsmAccess ;
    skos:prefLabel "Military"@en .

piirritev:OsmAccessPermissive a skos:Concept ;
    piirrite:hasRelatedOsmTag piirrite:hasOsmPermissiveAmenity,
        piirrite:hasOsmPermissiveHighway,
        piirrite:hasOsmPermissiveRailway,
        piirrite:hasOsmPermissiveWaterway ;
    piirrite:osmId "permissive" ;
    rdfs:subClassOf piirrite:OsmEntity ;
    skos:definition "The object is open to general public use, but access is not protected by legislation and can be revoked."@en ;
    skos:inScheme piirritev:OsmAccess ;
    skos:prefLabel "Permissive"@en .

piirritev:OsmAccessPermit a skos:Concept ;
    piirrite:hasRelatedOsmTag piirrite:hasOsmPermitHighway,
        piirrite:hasOsmPermitRailway,
        piirrite:hasOsmPermitWaterway ;
    piirrite:osmId "permit" ;
    rdfs:subClassOf piirrite:OsmEntity ;
    skos:definition "Access requires a permit, ordinarily granted."@en ;
    skos:inScheme piirritev:OsmAccess ;
    skos:prefLabel "Permit"@en .

piirritev:OsmAccessPrivate a skos:Concept ;
    piirrite:hasRelatedOsmTag piirrite:hasOsmPrivateHighway,
        piirrite:hasOsmPrivateRailway,
        piirrite:hasOsmPrivateWaterway ;
    piirrite:osmId "private" ;
    rdfs:subClassOf piirrite:OsmEntity ;
    skos:definition "The feature is not to be used by the public."@en ;
    skos:inScheme piirritev:OsmAccess ;
    skos:prefLabel "Private"@en .

piirritev:OsmAdminLevel a skos:ConceptScheme ;
    piirrite:osmId "admin_level" ;
    skos:definition "Indicates the level of an administrative boundary."@en ;
    skos:prefLabel "Admin level, types"@en .

piirritev:OsmAerialwayPylon a skos:Concept ;
    piirrite:hasRelatedOsmTag piirrite:hasOsmPylonRef ;
    piirrite:osmId "pylon" ;
    rdfs:subClassOf piirrite:OsmEntity ;
    skos:definition "A pylon supporting the aerialway cable."@en ;
    skos:inScheme piirritev:OsmAerialway ;
    skos:prefLabel "Pylon"@en .

piirritev:OsmAerialwayStation a skos:Concept ;
    piirrite:hasRelatedOsmTag piirrite:hasOsmStationEle,
        piirrite:hasOsmStationName,
        piirrite:hasOsmStationOperator ;
    piirrite:osmId "station" ;
    rdfs:subClassOf piirrite:OsmEntity ;
    skos:definition "A station where passengers and/or goods can enter and/or leave the aerialway  osmcarto-rendering = File:Rendering-railway-tram stop-mapnik.png.png  osmcarto-rendering-size = 14px"@en ;
    skos:inScheme piirritev:OsmAerialway ;
    skos:prefLabel "Station"@en .

piirritev:OsmAerowayAerodrome a skos:Concept ;
    piirrite:hasRelatedOsmTag piirrite:hasOsmAerodromeDescription,
        piirrite:hasOsmAerodromeIata,
        piirrite:hasOsmAerodromeIcao,
        piirrite:hasOsmAerodromeName,
        piirrite:hasOsmAerodromeOperator,
        piirrite:hasOsmAerodromeWebsite,
        piirrite:hasOsmAerodromeWikipedia ;
    piirrite:osmId "aerodrome" ;
    rdfs:subClassOf piirrite:OsmEntity ;
    skos:definition "An aerodrome, airport or airfield  osmcarto-rendering = File:Aerodrome.svg  osmcarto-rendering-size = 28px  osmcarto-rendering-area = File:Area transportation.png  osmcarto-rendering-area-size = 100px"@en ;
    skos:inScheme piirritev:OsmAeroway ;
    skos:prefLabel "Aerodrome"@en .

piirritev:OsmAerowayApron a skos:Concept ;
    piirrite:hasRelatedOsmTag piirrite:hasOsmApronAeroway,
        piirrite:hasOsmApronName,
        piirrite:hasOsmApronRef,
        piirrite:hasOsmApronSurface ;
    piirrite:osmId "apron" ;
    rdfs:subClassOf piirrite:OsmEntity ;
    skos:definition "An area of an airport where planes are parked, unloaded, loaded, refueled, or boarded.  osmcarto-rendering = File:Osmarender-apron.png  osmcarto-rendering-size = 100px"@en ;
    skos:inScheme piirritev:OsmAeroway ;
    skos:prefLabel "Apron"@en .

piirritev:OsmAerowayGate a skos:Concept ;
    piirrite:hasRelatedOsmTag piirrite:hasOsmGateRef ;
    piirrite:osmId "gate" ;
    rdfs:subClassOf piirrite:OsmEntity ;
    skos:definition "The bounded space, inside the airport terminal, where passengers wait before boarding their flight"@en ;
    skos:inScheme piirritev:OsmAeroway ;
    skos:prefLabel "Gate"@en .

piirritev:OsmAerowayHangar a skos:Concept ;
    piirrite:hasRelatedOsmTag piirrite:hasOsmHangarBuilding,
        piirrite:hasOsmHangarName,
        piirrite:hasOsmHangarRef ;
    piirrite:osmId "hangar" ;
    rdfs:subClassOf piirrite:OsmEntity ;
    skos:definition "A large airport building with extensive floor area that is used for housing aircraft or spacecraft."@en ;
    skos:inScheme piirritev:OsmAeroway ;
    skos:prefLabel "Hangar"@en .

piirritev:OsmAerowayHelipad a skos:Concept ;
    piirrite:hasRelatedOsmTag piirrite:hasOsmHelipadIcao,
        piirrite:hasOsmHelipadMaxrotordiameter,
        piirrite:hasOsmHelipadMaxweight,
        piirrite:hasOsmHelipadName,
        piirrite:hasOsmHelipadRef ;
    piirrite:osmId "helipad" ;
    rdfs:subClassOf piirrite:OsmEntity ;
    skos:definition "A landing area or platform designed for helicopters. It might be part of an aerodrome, heliport, hospital, hotel etc.  osmcarto-rendering = File:Helipad.16.svg  osmcarto-rendering-size = 28px  osmcarto-rendering-area = File:Rendering-aeroway area.png  osmcarto-rendering-area-size = 100px"@en ;
    skos:inScheme piirritev:OsmAeroway ;
    skos:prefLabel "Helipad"@en .

piirritev:OsmAerowayHoldingPosition a skos:Concept ;
    piirrite:osmId "holding_position" ;
    rdfs:subClassOf piirrite:OsmEntity ;
    skos:definition "A point behind which aircraft are considered clear of a crossing way"@en ;
    skos:inScheme piirritev:OsmAeroway ;
    skos:prefLabel "Holding position"@en .

piirritev:OsmAerowayJetBridge a skos:Concept ;
    piirrite:hasRelatedOsmTag piirrite:hasOsmJetBridgeHighway,
        piirrite:hasOsmJetBridgeRef ;
    piirrite:osmId "jet_bridge" ;
    rdfs:subClassOf piirrite:OsmEntity ;
    skos:definition "An enclosed, movable connector that extends from an airport terminal to an airplane"@en ;
    skos:inScheme piirritev:OsmAeroway ;
    skos:prefLabel "Jet bridge"@en .

piirritev:OsmAerowayNavigationaid a skos:Concept ;
    piirrite:hasRelatedOsmTag piirrite:hasOsmNavigationaidType ;
    piirrite:osmId "navigationaid" ;
    rdfs:subClassOf piirrite:OsmEntity ;
    skos:definition "A facility that supports visual navigation for aircraft"@en ;
    skos:inScheme piirritev:OsmAeroway ;
    skos:prefLabel "Navigationaid"@en .

piirritev:OsmAerowayParkingPosition a skos:Concept ;
    piirrite:hasRelatedOsmTag piirrite:hasOsmParkingPositionEle,
        piirrite:hasOsmParkingPositionRef,
        piirrite:hasOsmParkingPositionSurface ;
    piirrite:osmId "parking_position" ;
    rdfs:subClassOf piirrite:OsmEntity ;
    skos:definition "A location where an airplane can park."@en ;
    skos:inScheme piirritev:OsmAeroway ;
    skos:prefLabel "Parking position"@en .

piirritev:OsmAerowayRunway a skos:Concept ;
    piirrite:hasRelatedOsmTag piirrite:hasOsmRunwayCenterline,
        piirrite:hasOsmRunwayEle,
        piirrite:hasOsmRunwayLength,
        piirrite:hasOsmRunwayRef,
        piirrite:hasOsmRunwaySurface,
        piirrite:hasOsmRunwayWidth ;
    piirrite:osmId "runway" ;
    rdfs:subClassOf piirrite:OsmEntity ;
    skos:definition "A designated strip of surface on which aircrafts can take off and land.  osmcarto-rendering = File:Rendering-aeroway runway.png  osmcarto-rendering-size = 100px"@en ;
    skos:inScheme piirritev:OsmAeroway ;
    skos:prefLabel "Runway"@en .

piirritev:OsmAerowayTaxilane a skos:Concept ;
    piirrite:osmId "taxilane" ;
    rdfs:subClassOf piirrite:OsmEntity ;
    skos:definition "A path for aircraft in an airport that is part of the aircraft parking area or apron"@en ;
    skos:inScheme piirritev:OsmAeroway ;
    skos:prefLabel "Taxilane"@en .

piirritev:OsmAerowayTaxiway a skos:Concept ;
    piirrite:hasRelatedOsmTag piirrite:hasOsmTaxiwayRef,
        piirrite:hasOsmTaxiwaySurface ;
    piirrite:osmId "taxiway" ;
    rdfs:subClassOf piirrite:OsmEntity ;
    skos:definition "A route where airplanes manouevre between runways and parking areas within an aerodrome  osmcarto-rendering = File:Rendering-aeroway taxiway.png  osmcarto-rendering-size = 100px"@en ;
    skos:inScheme piirritev:OsmAeroway ;
    skos:prefLabel "Taxiway"@en .

piirritev:OsmAerowayTerminal a skos:Concept ;
    piirrite:hasRelatedOsmTag piirrite:hasOsmTerminalBuilding,
        piirrite:hasOsmTerminalEntrance,
        piirrite:hasOsmTerminalName,
        piirrite:hasOsmTerminalRef ;
    piirrite:osmId "terminal" ;
    rdfs:subClassOf piirrite:OsmEntity ;
    skos:definition "An airport passenger building  osmcarto-rendering = File:Area amenity=place of worship.png"@en ;
    skos:inScheme piirritev:OsmAeroway ;
    skos:prefLabel "Terminal"@en .

piirritev:OsmAerowayWindsock a skos:Concept ;
    piirrite:hasRelatedOsmTag piirrite:hasOsmWindsockLit ;
    piirrite:osmId "windsock" ;
    rdfs:subClassOf piirrite:OsmEntity ;
    skos:definition "An object that shows wind direction and speed."@en ;
    skos:inScheme piirritev:OsmAeroway ;
    skos:prefLabel "Windsock"@en .

piirritev:OsmAgeMature a skos:Concept ;
    piirrite:osmId "mature" ;
    rdfs:subClassOf piirrite:OsmEntity ;
    skos:definition ""@en ;
    skos:inScheme piirritev:OsmAge ;
    skos:prefLabel "Mature"@en .

piirritev:OsmAgeSemi-Mature a skos:Concept ;
    piirrite:osmId "semi-mature" ;
    rdfs:subClassOf piirrite:OsmEntity ;
    skos:definition ""@en ;
    skos:inScheme piirritev:OsmAge ;
    skos:prefLabel "Semi-mature"@en .

piirritev:OsmAgeYoung a skos:Concept ;
    piirrite:osmId "young" ;
    rdfs:subClassOf piirrite:OsmEntity ;
    skos:definition ""@en ;
    skos:inScheme piirritev:OsmAge ;
    skos:prefLabel "Young"@en .

piirritev:OsmAirConditioning a skos:ConceptScheme ;
    piirrite:osmId "air_conditioning" ;
    skos:definition "Indication whether a feature has air-conditioning"@en ;
    skos:prefLabel "Air conditioning, types"@en .

piirritev:OsmAltName a skos:ConceptScheme ;
    piirrite:osmId "alt_name" ;
    skos:definition "Alternative name or names by which the feature is known in the local language; for names in other languages, use name:xy where xy is the ISO 639 language code; not to be confused with name:alt, which is for the name in the Altai language"@en ;
    skos:prefLabel "Alt name, types"@en .

piirritev:OsmAmenityAnimalBreeding a skos:Concept ;
    piirrite:hasRelatedOsmTag piirrite:hasOsmAnimalBreedingName,
        piirrite:hasOsmAnimalBreedingOperator ;
    piirrite:osmId "animal_breeding" ;
    rdfs:subClassOf piirrite:OsmEntity ;
    skos:definition "A facility where animals are bred, usually to sell them."@en ;
    skos:inScheme piirritev:OsmAmenity ;
    skos:prefLabel "Animal breeding"@en .

piirritev:OsmAmenityArtsCentre a skos:Concept ;
    piirrite:hasRelatedOsmTag piirrite:hasOsmArtsCentreDescription,
        piirrite:hasOsmArtsCentreName,
        piirrite:hasOsmArtsCentreOperator ;
    piirrite:osmId "arts_centre" ;
    rdfs:subClassOf piirrite:OsmEntity ;
    skos:definition "An arts centre. A venue where a variety of arts are performed or conducted  osmcarto-rendering = File:Arts centre.svg  osmcarto-rendering-size = 28px  osmcarto-rendering-area = File:Rendering-area-amenity-school.png  osmcarto-rendering-area-size = 100px"@en ;
    skos:inScheme piirritev:OsmAmenity ;
    skos:prefLabel "Arts centre"@en .

piirritev:OsmAmenityAtm a skos:Concept ;
    piirrite:hasRelatedOsmTag piirrite:hasOsmAtmDriveThrough,
        piirrite:hasOsmAtmOperator ;
    piirrite:osmId "atm" ;
    rdfs:subClassOf piirrite:OsmEntity ;
    skos:definition "A device that provides the clients of a financial institution with access to financial transactions."@en ;
    skos:inScheme piirritev:OsmAmenity ;
    skos:prefLabel "Atm"@en .

piirritev:OsmAmenityBank a skos:Concept ;
    piirrite:hasRelatedOsmTag piirrite:hasOsmBankAtm,
        piirrite:hasOsmBankBic,
        piirrite:hasOsmBankBranch,
        piirrite:hasOsmBankBrand,
        piirrite:hasOsmBankDriveThrough,
        piirrite:hasOsmBankName,
        piirrite:hasOsmBankOpeningHours,
        piirrite:hasOsmBankOperator,
        piirrite:hasOsmBankWheelchair ;
    piirrite:osmId "bank" ;
    rdfs:subClassOf piirrite:OsmEntity ;
    skos:definition "A financial establishment where customers can, among other services, deposit money and take loans.  osmcarto-rendering = File:Bank-16.svg  osmcarto-rendering-size = 28px"@en ;
    skos:inScheme piirritev:OsmAmenity ;
    skos:prefLabel "Bank"@en .

piirritev:OsmAmenityBar a skos:Concept ;
    piirrite:hasRelatedOsmTag piirrite:hasOsmBarBrewery,
        piirrite:hasOsmBarDistillery,
        piirrite:hasOsmBarLiveMusic,
        piirrite:hasOsmBarMicrobrewery,
        piirrite:hasOsmBarName,
        piirrite:hasOsmBarOpeningHours,
        piirrite:hasOsmBarOperator,
        piirrite:hasOsmBarWebsite,
        piirrite:hasOsmBarWheelchair,
        piirrite:hasOsmBarWinery ;
    piirrite:osmId "bar" ;
    rdfs:subClassOf piirrite:OsmEntity ;
    skos:definition " osmcarto-rendering = File:Bar-16.svg  osmcarto-rendering-size = 28px"@en ;
    skos:inScheme piirritev:OsmAmenity ;
    skos:prefLabel "Bar"@en .

piirritev:OsmAmenityBbq a skos:Concept ;
    piirrite:hasRelatedOsmTag piirrite:hasOsmBbqCovered,
        piirrite:hasOsmBbqFuel ;
    piirrite:osmId "bbq" ;
    rdfs:subClassOf piirrite:OsmEntity ;
    skos:definition "A permanently built place for having a BBQ.  osmcarto-rendering = File:Bbq-14.svg  osmcarto-rendering-size = 28px"@en ;
    skos:inScheme piirritev:OsmAmenity ;
    skos:prefLabel "Bbq"@en .

piirritev:OsmAmenityBench a skos:Concept ;
    piirrite:hasRelatedOsmTag piirrite:hasOsmBenchArmrest,
        piirrite:hasOsmBenchBackrest,
        piirrite:hasOsmBenchColour,
        piirrite:hasOsmBenchCovered,
        piirrite:hasOsmBenchDirection,
        piirrite:hasOsmBenchHistoric,
        piirrite:hasOsmBenchInscription,
        piirrite:hasOsmBenchLength,
        piirrite:hasOsmBenchMaterial,
        piirrite:hasOsmBenchMemorial,
        piirrite:hasOsmBenchOperator,
        piirrite:hasOsmBenchSeats,
        piirrite:hasOsmBenchSide,
        piirrite:hasOsmBenchStartDate,
        piirrite:hasOsmBenchTwoSided,
        piirrite:hasOsmBenchWheelchair ;
    piirrite:osmId "bench" ;
    rdfs:subClassOf piirrite:OsmEntity ;
    skos:definition "A place for people to sit, allowing room for one or more people.  osmcarto-rendering = File:Bench-16.svg  osmcarto-rendering-size = 28px"@en ;
    skos:inScheme piirritev:OsmAmenity ;
    skos:prefLabel "Bench"@en .

piirritev:OsmAmenityBicycleParking a skos:Concept ;
    piirrite:hasRelatedOsmTag piirrite:hasOsmBicycleParkingAccess,
        piirrite:hasOsmBicycleParkingCapacity,
        piirrite:hasOsmBicycleParkingCargoBike,
        piirrite:hasOsmBicycleParkingCovered,
        piirrite:hasOsmBicycleParkingCyclestreetsId,
        piirrite:hasOsmBicycleParkingFee,
        piirrite:hasOsmBicycleParkingIndoor,
        piirrite:hasOsmBicycleParkingMaxstay,
        piirrite:hasOsmBicycleParkingName,
        piirrite:hasOsmBicycleParkingOperator,
        piirrite:hasOsmBicycleParkingSurveillance,
        piirrite:hasOsmBicycleParkingType ;
    piirrite:osmId "bicycle_parking" ;
    rdfs:subClassOf piirrite:OsmEntity ;
    skos:definition "A parking space designed for bicycles.  osmcarto-rendering = File:Parking-bicycle-16.svg  osmcarto-rendering-size = 28px  osmcarto-rendering-area = File:Area parking.png  osmcarto-rendering-area-size = 100px"@en ;
    skos:inScheme piirritev:OsmAmenity ;
    skos:prefLabel "Bicycle parking"@en .

piirritev:OsmAmenityBicycleRental a skos:Concept ;
    piirrite:hasRelatedOsmTag piirrite:hasOsmBicycleRentalCapacity,
        piirrite:hasOsmBicycleRentalName,
        piirrite:hasOsmBicycleRentalNetwork,
        piirrite:hasOsmBicycleRentalOperator,
        piirrite:hasOsmBicycleRentalRef ;
    piirrite:osmId "bicycle_rental" ;
    rdfs:subClassOf piirrite:OsmEntity ;
    skos:definition "A place, often unattended, where you can pick up and drop off rented bikes.  osmcarto-rendering = File:Rental-bicycle-16.svg  osmcarto-rendering-size = 28px"@en ;
    skos:inScheme piirritev:OsmAmenity ;
    skos:prefLabel "Bicycle rental"@en .

piirritev:OsmAmenityBiergarten a skos:Concept ;
    piirrite:hasRelatedOsmTag piirrite:hasOsmBiergartenName ;
    piirrite:osmId "biergarten" ;
    rdfs:subClassOf piirrite:OsmEntity ;
    skos:definition "An open-air seating area where beer is served.  osmcarto-rendering = File:Biergarten-16.svg  osmcarto-rendering-size = 28px"@en ;
    skos:inScheme piirritev:OsmAmenity ;
    skos:prefLabel "Biergarten"@en .

piirritev:OsmAmenityBusStation a skos:Concept ;
    piirrite:hasRelatedOsmTag piirrite:hasOsmBusStationName,
        piirrite:hasOsmBusStationOperator ;
    piirrite:osmId "bus_station" ;
    rdfs:subClassOf piirrite:OsmEntity ;
    skos:definition "A bus station would usually be a terminus where many routes stop / start, and where you can change between routes, etc.  osmcarto-rendering = File:Amenity bus station.svg  osmcarto-rendering-size = 28px  osmcarto-rendering-area = File:Area transportation.png  osmcarto-rendering-area-size = 100px"@en ;
    skos:inScheme piirritev:OsmAmenity ;
    skos:prefLabel "Bus station"@en .

piirritev:OsmAmenityCafe a skos:Concept ;
    piirrite:hasRelatedOsmTag piirrite:hasOsmCafeAirConditioning,
        piirrite:hasOsmCafeAmenity,
        piirrite:hasOsmCafeBakery,
        piirrite:hasOsmCafeBrand,
        piirrite:hasOsmCafeCapacity,
        piirrite:hasOsmCafeChangingTable,
        piirrite:hasOsmCafeCuisine,
        piirrite:hasOsmCafeDog,
        piirrite:hasOsmCafeDrinkingStraw,
        piirrite:hasOsmCafeIceCream,
        piirrite:hasOsmCafeIndoorSeating,
        piirrite:hasOsmCafeInternetAccess,
        piirrite:hasOsmCafeLaptop,
        piirrite:hasOsmCafeName,
        piirrite:hasOsmCafeOpeningHours,
        piirrite:hasOsmCafeOperator,
        piirrite:hasOsmCafeOutdoorSeating,
        piirrite:hasOsmCafePastry,
        piirrite:hasOsmCafePhone,
        piirrite:hasOsmCafeSelfService,
        piirrite:hasOsmCafeSmoking,
        piirrite:hasOsmCafeTakeaway,
        piirrite:hasOsmCafeTelevision,
        piirrite:hasOsmCafeToilets,
        piirrite:hasOsmCafeWebsite,
        piirrite:hasOsmCafeWheelchair ;
    piirrite:osmId "cafe" ;
    rdfs:subClassOf piirrite:OsmEntity ;
    skos:definition "A generally informal place with sit-down facilities selling beverages and light meals and/or snacks.  osmcarto-rendering = File:Cafe-16.svg  osmcarto-rendering-size = 28px"@en ;
    skos:inScheme piirritev:OsmAmenity ;
    skos:prefLabel "Cafe"@en .

piirritev:OsmAmenityCarRental a skos:Concept ;
    piirrite:hasRelatedOsmTag piirrite:hasOsmCarRentalName,
        piirrite:hasOsmCarRentalOpeningHours,
        piirrite:hasOsmCarRentalOperator,
        piirrite:hasOsmCarRentalPhone,
        piirrite:hasOsmCarRentalWebsite ;
    piirrite:osmId "car_rental" ;
    rdfs:subClassOf piirrite:OsmEntity ;
    skos:definition "A place from which cars can be rented.  osmcarto-rendering = File:Rental-car-16.svg  osmcarto-rendering-size = 28px"@en ;
    skos:inScheme piirritev:OsmAmenity ;
    skos:prefLabel "Car rental"@en .

piirritev:OsmAmenityCarSharing a skos:Concept ;
    piirrite:hasRelatedOsmTag piirrite:hasOsmCarSharingName,
        piirrite:hasOsmCarSharingNetwork,
        piirrite:hasOsmCarSharingOperator ;
    piirrite:osmId "car_sharing" ;
    rdfs:subClassOf piirrite:OsmEntity ;
    skos:definition "Carsharing station, where you get your booked car, often separate areas on parking places."@en ;
    skos:inScheme piirritev:OsmAmenity ;
    skos:prefLabel "Car sharing"@en .

piirritev:OsmAmenityCarWash a skos:Concept ;
    piirrite:hasRelatedOsmTag piirrite:hasOsmCarWashAccess,
        piirrite:hasOsmCarWashAmenity,
        piirrite:hasOsmCarWashAutomated,
        piirrite:hasOsmCarWashBrand,
        piirrite:hasOsmCarWashBus,
        piirrite:hasOsmCarWashDogWashing,
        piirrite:hasOsmCarWashMaxheight,
        piirrite:hasOsmCarWashMaxwidth,
        piirrite:hasOsmCarWashName,
        piirrite:hasOsmCarWashOpeningHours,
        piirrite:hasOsmCarWashOperator,
        piirrite:hasOsmCarWashPhone,
        piirrite:hasOsmCarWashSelfService,
        piirrite:hasOsmCarWashTouchlessWash,
        piirrite:hasOsmCarWashTruckWash,
        piirrite:hasOsmCarWashVacuumCleaner,
        piirrite:hasOsmCarWashWebsite ;
    piirrite:osmId "car_wash" ;
    rdfs:subClassOf piirrite:OsmEntity ;
    skos:definition "A facility used to clean the exterior of motor vehicles  osmcarto-rendering = File:Car wash-14.svg  osmcarto-rendering-size = 28px"@en ;
    skos:inScheme piirritev:OsmAmenity ;
    skos:prefLabel "Car wash"@en .

piirritev:OsmAmenityChargingStation a skos:Concept ;
    piirrite:hasRelatedOsmTag piirrite:hasOsmChargingStationAccess,
        piirrite:hasOsmChargingStationBrand,
        piirrite:hasOsmChargingStationCapacity ;
    piirrite:osmId "charging_station" ;
    rdfs:subClassOf piirrite:OsmEntity ;
    skos:definition "A location where battery electric vehicles can be charged.  osmcarto-rendering = File:Charging station.16.svg  osmcarto-rendering-size = 28px"@en ;
    skos:inScheme piirritev:OsmAmenity ;
    skos:prefLabel "Charging station"@en .

piirritev:OsmAmenityChildcare a skos:Concept ;
    piirrite:osmId "childcare" ;
    rdfs:subClassOf piirrite:OsmEntity ;
    skos:definition "A place where children are looked after which is not an tag:amenity=kindergarten.  osmcarto-rendering = File:Social amenity darken 80-16.svg  osmcarto-rendering-size = 28px"@en ;
    skos:inScheme piirritev:OsmAmenity ;
    skos:prefLabel "Childcare"@en .

piirritev:OsmAmenityCinema a skos:Concept ;
    piirrite:hasRelatedOsmTag piirrite:hasOsmCinemaName ;
    piirrite:osmId "cinema" ;
    rdfs:subClassOf piirrite:OsmEntity ;
    skos:definition "A movie theater, a place showing movies.  osmcarto-rendering = File:Cinema-16.svg  osmcarto-rendering-size = 28px"@en ;
    skos:inScheme piirritev:OsmAmenity ;
    skos:prefLabel "Cinema"@en .

piirritev:OsmAmenityClinic a skos:Concept ;
    piirrite:hasRelatedOsmTag piirrite:hasOsmClinicName,
        piirrite:hasOsmClinicOpeningHours ;
    piirrite:osmId "clinic" ;
    rdfs:subClassOf piirrite:OsmEntity ;
    skos:definition "A clinic is a medical centre, with more staff than a doctor's office, that does not admit inpatients.  osmcarto-rendering = File:Doctors-14.svg  osmcarto-rendering-size = 28px  osmcarto-rendering-area = File:Rendering-area-amenity-school.png  osmcarto-rendering-area-size = 100px"@en ;
    skos:inScheme piirritev:OsmAmenity ;
    skos:prefLabel "Clinic"@en .

piirritev:OsmAmenityClock a skos:Concept ;
    piirrite:osmId "clock" ;
    rdfs:subClassOf piirrite:OsmEntity ;
    skos:definition "A publicly visible clock"@en ;
    skos:inScheme piirritev:OsmAmenity ;
    skos:prefLabel "Clock"@en .

piirritev:OsmAmenityCollege a skos:Concept ;
    piirrite:hasRelatedOsmTag piirrite:hasOsmCollegeName,
        piirrite:hasOsmCollegeOperator,
        piirrite:hasOsmCollegePhone,
        piirrite:hasOsmCollegeWebsite ;
    piirrite:osmId "college" ;
    rdfs:subClassOf piirrite:OsmEntity ;
    skos:definition "A place for further education, a post-secondary education institution which is not a University  osmcarto-rendering-area = File:Rendering-area-amenity-school.png  osmcarto-rendering-area-size = 125px"@en ;
    skos:inScheme piirritev:OsmAmenity ;
    skos:prefLabel "College"@en .

piirritev:OsmAmenityCommunityCentre a skos:Concept ;
    piirrite:hasRelatedOsmTag piirrite:hasOsmCommunityCentreType ;
    piirrite:osmId "community_centre" ;
    rdfs:subClassOf piirrite:OsmEntity ;
    skos:definition "A place mostly used for local events, festivities and group activities.  osmcarto-rendering = File:Community centre-14.svg  osmcarto-rendering-size = 28px  osmcarto-rendering-area = File:Rendering-area-amenity-school.png  osmcarto-rendering-area-size = 100px"@en ;
    skos:inScheme piirritev:OsmAmenity ;
    skos:prefLabel "Community centre"@en .

piirritev:OsmAmenityCompressedAir a skos:Concept ;
    piirrite:hasRelatedOsmTag piirrite:hasOsmCompressedAirAccess,
        piirrite:hasOsmCompressedAirFee,
        piirrite:hasOsmCompressedAirOpeningHours,
        piirrite:hasOsmCompressedAirPressure,
        piirrite:hasOsmCompressedAirValves ;
    piirrite:osmId "compressed_air" ;
    rdfs:subClassOf piirrite:OsmEntity ;
    skos:definition "A device to inflate tyres, mostly of motor vehicles."@en ;
    skos:inScheme piirritev:OsmAmenity ;
    skos:prefLabel "Compressed air"@en .

piirritev:OsmAmenityCourthouse a skos:Concept ;
    piirrite:hasRelatedOsmTag piirrite:hasOsmCourthouseAdminLevel,
        piirrite:hasOsmCourthouseName,
        piirrite:hasOsmCourthouseOpeningHours,
        piirrite:hasOsmCourthouseOperator,
        piirrite:hasOsmCourthousePhone,
        piirrite:hasOsmCourthouseWebsite,
        piirrite:hasOsmCourthouseWheelchair ;
    piirrite:osmId "courthouse" ;
    rdfs:subClassOf piirrite:OsmEntity ;
    skos:definition "A building which is home to a court of law, which administers justice according to the rule of law.  osmcarto-rendering = File:Courthouse-16.svg  osmcarto-rendering-size = 28px"@en ;
    skos:inScheme piirritev:OsmAmenity ;
    skos:prefLabel "Courthouse"@en .

piirritev:OsmAmenityDentist a skos:Concept ;
    piirrite:hasRelatedOsmTag piirrite:hasOsmDentistName ;
    piirrite:osmId "dentist" ;
    rdfs:subClassOf piirrite:OsmEntity ;
    skos:definition "A dentist practice / surgery.  osmcarto-rendering = File:Dentist-14.svg  osmcarto-rendering-size = 28px"@en ;
    skos:inScheme piirritev:OsmAmenity ;
    skos:prefLabel "Dentist"@en .

piirritev:OsmAmenityDoctors a skos:Concept ;
    piirrite:hasRelatedOsmTag piirrite:hasOsmDoctorsHealthcare,
        piirrite:hasOsmDoctorsName ;
    piirrite:osmId "doctors" ;
    rdfs:subClassOf piirrite:OsmEntity ;
    skos:definition "A doctor's office, a place to get medical attention or a check up from a physician.  osmcarto-rendering = File:Doctors-14.svg  osmcarto-rendering-size = 28px"@en ;
    skos:inScheme piirritev:OsmAmenity ;
    skos:prefLabel "Doctors"@en .

piirritev:OsmAmenityDrinkingWater a skos:Concept ;
    piirrite:hasRelatedOsmTag piirrite:hasOsmDrinkingWaterAccess,
        piirrite:hasOsmDrinkingWaterBottle,
        piirrite:hasOsmDrinkingWaterCapacity,
        piirrite:hasOsmDrinkingWaterDescription,
        piirrite:hasOsmDrinkingWaterFountain,
        piirrite:hasOsmDrinkingWaterIndoor,
        piirrite:hasOsmDrinkingWaterName,
        piirrite:hasOsmDrinkingWaterOperator ;
    piirrite:osmId "drinking_water" ;
    rdfs:subClassOf piirrite:OsmEntity ;
    skos:definition "A drinking water source which provides potable water for consumption.  osmcarto-rendering = File:Drinking-water-16.svg  osmcarto-rendering-size = 28px"@en ;
    skos:inScheme piirritev:OsmAmenity ;
    skos:prefLabel "Drinking water"@en .

piirritev:OsmAmenityDrivingSchool a skos:Concept ;
    piirrite:hasRelatedOsmTag piirrite:hasOsmDrivingSchoolLicenseClasses,
        piirrite:hasOsmDrivingSchoolName ;
    piirrite:osmId "driving_school" ;
    rdfs:subClassOf piirrite:OsmEntity ;
    skos:definition "A school to learn to drive a motor vehicle. osmcarto-rendering=File:Shop-other-16.svg osmcarto-rendering-size=28px"@en ;
    skos:inScheme piirritev:OsmAmenity ;
    skos:prefLabel "Driving school"@en .

piirritev:OsmAmenityEventsVenue a skos:Concept ;
    piirrite:hasRelatedOsmTag piirrite:hasOsmEventsVenueAmenity,
        piirrite:hasOsmEventsVenueOpeningHours,
        piirrite:hasOsmEventsVenueOperator,
        piirrite:hasOsmEventsVenuePhone,
        piirrite:hasOsmEventsVenueWebsite,
        piirrite:hasOsmEventsVenueWheelchair ;
    piirrite:osmId "events_venue" ;
    rdfs:subClassOf piirrite:OsmEntity ;
    skos:definition "A place that provides facilities for events such as banquets, weddings etc."@en ;
    skos:inScheme piirritev:OsmAmenity ;
    skos:prefLabel "Events venue"@en .

piirritev:OsmAmenityFastFood a skos:Concept ;
    piirrite:hasRelatedOsmTag piirrite:hasOsmFastFoodCuisine,
        piirrite:hasOsmFastFoodDelivery,
        piirrite:hasOsmFastFoodName,
        piirrite:hasOsmFastFoodTakeaway ;
    piirrite:osmId "fast_food" ;
    rdfs:subClassOf piirrite:OsmEntity ;
    skos:definition "A place which offers self-service and take-away food. osmcarto-rendering=File:Fast-food-16.svg osmcarto-rendering-size=28px"@en ;
    skos:inScheme piirritev:OsmAmenity ;
    skos:prefLabel "Fast food"@en .

piirritev:OsmAmenityFerryTerminal a skos:Concept ;
    piirrite:hasRelatedOsmTag piirrite:hasOsmFerryTerminalCargo,
        piirrite:hasOsmFerryTerminalName,
        piirrite:hasOsmFerryTerminalOperator ;
    piirrite:osmId "ferry_terminal" ;
    rdfs:subClassOf piirrite:OsmEntity ;
    skos:definition "A place where people, cars etc. can board and leave a ferry. osmcarto-rendering = File:Ferry-icon.svg osmcarto-rendering-size = 28px osmcarto-rendering-area = File:Area transportation.png osmcarto-rendering-area-size = 100px"@en ;
    skos:inScheme piirritev:OsmAmenity ;
    skos:prefLabel "Ferry terminal"@en .

piirritev:OsmAmenityFireStation a skos:Concept ;
    piirrite:hasRelatedOsmTag piirrite:hasOsmFireStationBranch,
        piirrite:hasOsmFireStationBuilding,
        piirrite:hasOsmFireStationName,
        piirrite:hasOsmFireStationOperator,
        piirrite:hasOsmFireStationPhone,
        piirrite:hasOsmFireStationWebsite ;
    piirrite:osmId "fire_station" ;
    rdfs:subClassOf piirrite:OsmEntity ;
    skos:definition "A station from which a fire brigade operates."@en ;
    skos:inScheme piirritev:OsmAmenity ;
    skos:prefLabel "Fire station"@en .

piirritev:OsmAmenityFoodCourt a skos:Concept ;
    piirrite:hasRelatedOsmTag piirrite:hasOsmFoodCourtCuisine,
        piirrite:hasOsmFoodCourtName,
        piirrite:hasOsmFoodCourtOpeningHours,
        piirrite:hasOsmFoodCourtOperator,
        piirrite:hasOsmFoodCourtPhone,
        piirrite:hasOsmFoodCourtSeasonal,
        piirrite:hasOsmFoodCourtSmoking,
        piirrite:hasOsmFoodCourtWheelchair ;
    piirrite:osmId "food_court" ;
    rdfs:subClassOf piirrite:OsmEntity ;
    skos:definition "A place with sit-down facilities shared by multiple self-service food vendors. osmcarto-rendering=File:Restaurant-14.svg osmcarto-rendering-size=28px"@en ;
    skos:inScheme piirritev:OsmAmenity ;
    skos:prefLabel "Food court"@en .

piirritev:OsmAmenityFountain a skos:Concept ;
    piirrite:hasRelatedOsmTag piirrite:hasOsmFountainDrinkingWater,
        piirrite:hasOsmFountainName ;
    piirrite:osmId "fountain" ;
    rdfs:subClassOf piirrite:OsmEntity ;
    skos:definition "A fountain with cultural, decorational or historical significance or which serves a recreational purpose. osmcarto-rendering=File:Fountain-14.svg osmcarto-rendering-size=28px"@en ;
    skos:inScheme piirritev:OsmAmenity ;
    skos:prefLabel "Fountain"@en .

piirritev:OsmAmenityFuel a skos:Concept ;
    piirrite:hasRelatedOsmTag piirrite:hasOsmFuelBrand,
        piirrite:hasOsmFuelCapacity,
        piirrite:hasOsmFuelMaxheight,
        piirrite:hasOsmFuelName,
        piirrite:hasOsmFuelOpeningHours,
        piirrite:hasOsmFuelOperator,
        piirrite:hasOsmFuelPhone,
        piirrite:hasOsmFuelSelfService,
        piirrite:hasOsmFuelWebsite ;
    piirrite:osmId "fuel" ;
    rdfs:subClassOf piirrite:OsmEntity ;
    skos:definition "A retail facility for refueling motor vehicles osmcarto-rendering=File:Fuel-16.svg osmcarto-rendering-size=28px"@en ;
    skos:inScheme piirritev:OsmAmenity ;
    skos:prefLabel "Fuel"@en .

piirritev:OsmAmenityGraveYard a skos:Concept ;
    piirrite:hasRelatedOsmTag piirrite:hasOsmGraveYardName,
        piirrite:hasOsmGraveYardReligion ;
    piirrite:osmId "grave_yard" ;
    rdfs:subClassOf piirrite:OsmEntity ;
    skos:definition "A place where people (or sometimes animals) are buried, usually close to a place of worship. osmcarto-rendering=File:Landuse-cemetery.png osmcarto-rendering-size=125px"@en ;
    skos:inScheme piirritev:OsmAmenity ;
    skos:prefLabel "Grave yard"@en .

piirritev:OsmAmenityGritBin a skos:Concept ;
    piirrite:hasRelatedOsmTag piirrite:hasOsmGritBinAccess ;
    piirrite:osmId "grit_bin" ;
    rdfs:subClassOf piirrite:OsmEntity ;
    skos:definition "A container that holds sand, salt and gravel to spread on roads for winter safety."@en ;
    skos:inScheme piirritev:OsmAmenity ;
    skos:prefLabel "Grit bin"@en .

piirritev:OsmAmenityHospital a skos:Concept ;
    piirrite:hasRelatedOsmTag piirrite:hasOsmHospitalBeds,
        piirrite:hasOsmHospitalEmergency,
        piirrite:hasOsmHospitalHealthcare,
        piirrite:hasOsmHospitalName,
        piirrite:hasOsmHospitalOperator,
        piirrite:hasOsmHospitalPhone,
        piirrite:hasOsmHospitalWebsite ;
    piirrite:osmId "hospital" ;
    rdfs:subClassOf piirrite:OsmEntity ;
    skos:definition "A hospital providing in-patient medical treatment. osmcarto-rendering=File:Hospital-14.svg osmcarto-rendering-size=28px osmcarto-rendering-area = File:Rendering-area-amenity-school.png osmcarto-rendering-area-size = 100px"@en ;
    skos:inScheme piirritev:OsmAmenity ;
    skos:prefLabel "Hospital"@en .

piirritev:OsmAmenityHuntingStand a skos:Concept ;
    piirrite:hasRelatedOsmTag piirrite:hasOsmHuntingStandAmenity,
        piirrite:hasOsmHuntingStandDirection,
        piirrite:hasOsmHuntingStandHeight,
        piirrite:hasOsmHuntingStandHide,
        piirrite:hasOsmHuntingStandLadder,
        piirrite:hasOsmHuntingStandLock,
        piirrite:hasOsmHuntingStandLockable,
        piirrite:hasOsmHuntingStandRaised,
        piirrite:hasOsmHuntingStandShelter,
        piirrite:hasOsmHuntingStandTree,
        piirrite:hasOsmHuntingStandType ;
    piirrite:osmId "hunting_stand" ;
    rdfs:subClassOf piirrite:OsmEntity ;
    skos:definition "An open or enclosed platform used by hunters to place themselves, usually at an elevated height above the terrain."@en ;
    skos:inScheme piirritev:OsmAmenity ;
    skos:prefLabel "Hunting stand"@en .

piirritev:OsmAmenityIceCream a skos:Concept ;
    piirrite:hasRelatedOsmTag piirrite:hasOsmIceCreamName,
        piirrite:hasOsmIceCreamOpeningHours ;
    piirrite:osmId "ice_cream" ;
    rdfs:subClassOf piirrite:OsmEntity ;
    skos:definition "A place that sells ice cream and/or frozen yoghurt over the counter. osmcarto-rendering=File:Ice-cream-14.svg osmcarto-rendering-size=28px"@en ;
    skos:inScheme piirritev:OsmAmenity ;
    skos:prefLabel "Ice cream"@en .

piirritev:OsmAmenityInternetCafe a skos:Concept ;
    piirrite:hasRelatedOsmTag piirrite:hasOsmInternetCafeAddr,
        piirrite:hasOsmInternetCafeName,
        piirrite:hasOsmInternetCafeOpeningHours,
        piirrite:hasOsmInternetCafeOperator,
        piirrite:hasOsmInternetCafeOutdoorSeating,
        piirrite:hasOsmInternetCafeSmoking ;
    piirrite:osmId "internet_cafe" ;
    rdfs:subClassOf piirrite:OsmEntity ;
    skos:definition "A place whose principal role is providing internet services. osmcarto-rendering = File:Internet cafe-14.svg osmcarto-rendering-size = 28px"@en ;
    skos:inScheme piirritev:OsmAmenity ;
    skos:prefLabel "Internet cafe"@en .

piirritev:OsmAmenityKindergarten a skos:Concept ;
    piirrite:hasRelatedOsmTag piirrite:hasOsmKindergartenName,
        piirrite:hasOsmKindergartenOperator ;
    piirrite:osmId "kindergarten" ;
    rdfs:subClassOf piirrite:OsmEntity ;
    skos:definition "A place for looking after preschool children and (typically) giving early education. osmcarto-rendering-node=File:Rendering-amenity-kindergarten.png osmcarto-rendering-node-size=125px osmcarto-rendering-area=File:Rendering-area-amenity-school.png osmcarto-rendering-area-size=125px"@en ;
    skos:inScheme piirritev:OsmAmenity ;
    skos:prefLabel "Kindergarten"@en .

piirritev:OsmAmenityLavoir a skos:Concept ;
    piirrite:hasRelatedOsmTag piirrite:hasOsmLavoirAccess,
        piirrite:hasOsmLavoirCovered ;
    piirrite:osmId "lavoir" ;
    rdfs:subClassOf piirrite:OsmEntity ;
    skos:definition "A public place where people come to wash their clothes manually"@en ;
    skos:inScheme piirritev:OsmAmenity ;
    skos:prefLabel "Lavoir"@en .

piirritev:OsmAmenityLetterBox a skos:Concept ;
    piirrite:osmId "letter_box" ;
    rdfs:subClassOf piirrite:OsmEntity ;
    skos:definition "Private mailboxes where mailmen or other people deposit letters to specific addresses."@en ;
    skos:inScheme piirritev:OsmAmenity ;
    skos:prefLabel "Letter box"@en .

piirritev:OsmAmenityLibrary a skos:Concept ;
    piirrite:hasRelatedOsmTag piirrite:hasOsmLibraryBooks,
        piirrite:hasOsmLibraryName,
        piirrite:hasOsmLibraryPhone,
        piirrite:hasOsmLibraryWebsite ;
    piirrite:osmId "library" ;
    rdfs:subClassOf piirrite:OsmEntity ;
    skos:definition "A place to read and/or borrow books. osmcarto-rendering=File:Library-16.svg osmcarto-rendering-size=28px"@en ;
    skos:inScheme piirritev:OsmAmenity ;
    skos:prefLabel "Library"@en .

piirritev:OsmAmenityLoadingDock a skos:Concept ;
    piirrite:hasRelatedOsmTag piirrite:hasOsmLoadingDockDoor,
        piirrite:hasOsmLoadingDockMaxheight,
        piirrite:hasOsmLoadingDockMaxlength,
        piirrite:hasOsmLoadingDockMaxwidth,
        piirrite:hasOsmLoadingDockRef ;
    piirrite:osmId "loading_dock" ;
    rdfs:subClassOf piirrite:OsmEntity ;
    skos:definition "A loading dock is an entrance to a building used for loading and unloading goods vehicles."@en ;
    skos:inScheme piirritev:OsmAmenity ;
    skos:prefLabel "Loading dock"@en .

piirritev:OsmAmenityLounger a skos:Concept ;
    piirrite:hasRelatedOsmTag piirrite:hasOsmLoungerColour,
        piirrite:hasOsmLoungerDirection,
        piirrite:hasOsmLoungerMaterial,
        piirrite:hasOsmLoungerOperator,
        piirrite:hasOsmLoungerSeasonal ;
    piirrite:osmId "lounger" ;
    rdfs:subClassOf piirrite:OsmEntity ;
    skos:definition "An object for people to lie down."@en ;
    skos:inScheme piirritev:OsmAmenity ;
    skos:prefLabel "Lounger"@en .

piirritev:OsmAmenityMarketplace a skos:Concept ;
    piirrite:hasRelatedOsmTag piirrite:hasOsmMarketplaceBuilding,
        piirrite:hasOsmMarketplaceName,
        piirrite:hasOsmMarketplaceOpeningHours,
        piirrite:hasOsmMarketplaceOperator,
        piirrite:hasOsmMarketplaceOrganic ;
    piirrite:osmId "marketplace" ;
    rdfs:subClassOf piirrite:OsmEntity ;
    skos:definition "A marketplace where goods and services are traded daily or weekly. osmcarto-rendering=File:Marketplace-14.svg osmcarto-rendering-size=28px osmcarto-rendering-area=File:Landuse-retail.png osmcarto-rendering-area-size=100px"@en ;
    skos:inScheme piirritev:OsmAmenity ;
    skos:prefLabel "Marketplace"@en .

piirritev:OsmAmenityMonastery a skos:Concept ;
    piirrite:hasRelatedOsmTag piirrite:hasOsmMonasteryCommunity,
        piirrite:hasOsmMonasteryName,
        piirrite:hasOsmMonasteryReligion ;
    piirrite:osmId "monastery" ;
    rdfs:subClassOf piirrite:OsmEntity ;
    skos:definition "An active monastery or convent, occupied by a community of monks or nuns living under religious vows."@en ;
    skos:inScheme piirritev:OsmAmenity ;
    skos:prefLabel "Monastery"@en .

piirritev:OsmAmenityMotorcycleParking a skos:Concept ;
    piirrite:hasRelatedOsmTag piirrite:hasOsmMotorcycleParkingAccess,
        piirrite:hasOsmMotorcycleParkingBuilding,
        piirrite:hasOsmMotorcycleParkingCapacity,
        piirrite:hasOsmMotorcycleParkingCovered,
        piirrite:hasOsmMotorcycleParkingFee,
        piirrite:hasOsmMotorcycleParkingMaxstay,
        piirrite:hasOsmMotorcycleParkingName,
        piirrite:hasOsmMotorcycleParkingOperator,
        piirrite:hasOsmMotorcycleParkingParking,
        piirrite:hasOsmMotorcycleParkingRef ;
    piirrite:osmId "motorcycle_parking" ;
    rdfs:subClassOf piirrite:OsmEntity ;
    skos:definition "A place which is designated for parking motorcycles."@en ;
    skos:inScheme piirritev:OsmAmenity ;
    skos:prefLabel "Motorcycle parking"@en .

piirritev:OsmAmenityMusicSchool a skos:Concept ;
    piirrite:hasRelatedOsmTag piirrite:hasOsmMusicSchoolName,
        piirrite:hasOsmMusicSchoolOperator,
        piirrite:hasOsmMusicSchoolPhone,
        piirrite:hasOsmMusicSchoolWebsite,
        piirrite:hasOsmMusicSchoolWheelchair ;
    piirrite:osmId "music_school" ;
    rdfs:subClassOf piirrite:OsmEntity ;
    skos:definition "Music school, an educational institution specialized in the study, training, and research of music"@en ;
    skos:inScheme piirritev:OsmAmenity ;
    skos:prefLabel "Music school"@en .

piirritev:OsmAmenityNightclub a skos:Concept ;
    piirrite:hasRelatedOsmTag piirrite:hasOsmNightclubLiveMusic,
        piirrite:hasOsmNightclubMusic,
        piirrite:hasOsmNightclubName,
        piirrite:hasOsmNightclubOpeningHours,
        piirrite:hasOsmNightclubOperator,
        piirrite:hasOsmNightclubPhone,
        piirrite:hasOsmNightclubWebsite,
        piirrite:hasOsmNightclubWheelchair ;
    piirrite:osmId "nightclub" ;
    rdfs:subClassOf piirrite:OsmEntity ;
    skos:definition "A place to dance and drink at night. Also known as a disco. osmcarto-rendering=File:Nightclub-16.svg osmcarto-rendering-size=28px"@en ;
    skos:inScheme piirritev:OsmAmenity ;
    skos:prefLabel "Nightclub"@en .

piirritev:OsmAmenityNursingHome a skos:Concept ;
    piirrite:hasRelatedOsmTag piirrite:hasOsmNursingHomeBuilding,
        piirrite:hasOsmNursingHomePhone,
        piirrite:hasOsmNursingHomeWebsite ;
    piirrite:osmId "nursing_home" ;
    rdfs:subClassOf piirrite:OsmEntity ;
    skos:definition "A home for disabled/elderly persons who need permanent care. osmcarto-rendering=File:Social amenity darken 80-16.svg osmcarto-rendering-size=28px"@en ;
    skos:inScheme piirritev:OsmAmenity ;
    skos:prefLabel "Nursing home"@en .

piirritev:OsmAmenityParcelLocker a skos:Concept ;
    piirrite:osmId "parcel_locker" ;
    rdfs:subClassOf piirrite:OsmEntity ;
    skos:definition "Machine for picking up and sending parcels.  osmcarto-rendering = File:Parcel locker.svg  osmcarto-rendering-size = 28px"@en ;
    skos:inScheme piirritev:OsmAmenity ;
    skos:prefLabel "Parcel locker"@en .

piirritev:OsmAmenityParking a skos:Concept ;
    piirrite:hasRelatedOsmTag piirrite:hasOsmParkingAccess,
        piirrite:hasOsmParkingCapacity,
        piirrite:hasOsmParkingFee,
        piirrite:hasOsmParkingMaxstay,
        piirrite:hasOsmParkingName,
        piirrite:hasOsmParkingOperator,
        piirrite:hasOsmParkingType ;
    piirrite:osmId "parking" ;
    rdfs:subClassOf piirrite:OsmEntity ;
    skos:definition "A place for parking cars."@en ;
    skos:inScheme piirritev:OsmAmenity ;
    skos:prefLabel "Parking"@en .

piirritev:OsmAmenityParkingEntrance a skos:Concept ;
    piirrite:hasRelatedOsmTag piirrite:hasOsmParkingEntranceParking ;
    piirrite:osmId "parking_entrance" ;
    rdfs:subClassOf piirrite:OsmEntity ;
    skos:definition "An entrance to an underground or multi storey parking facility."@en ;
    skos:inScheme piirritev:OsmAmenity ;
    skos:prefLabel "Parking entrance"@en .

piirritev:OsmAmenityParkingSpace a skos:Concept ;
    piirrite:hasRelatedOsmTag piirrite:hasOsmParkingSpaceSite,
        piirrite:hasOsmParkingSpaceType ;
    piirrite:osmId "parking_space" ;
    rdfs:subClassOf piirrite:OsmEntity ;
    skos:definition "A single parking space on a parking lot. osmcarto-rendering=File:Rendering-parking space.png osmcarto-rendering-size=125px"@en ;
    skos:inScheme piirritev:OsmAmenity ;
    skos:prefLabel "Parking space"@en .

piirritev:OsmAmenityPaymentTerminal a skos:Concept ;
    piirrite:hasRelatedOsmTag piirrite:hasOsmPaymentTerminalBrand,
        piirrite:hasOsmPaymentTerminalOperator ;
    piirrite:osmId "payment_terminal" ;
    rdfs:subClassOf piirrite:OsmEntity ;
    skos:definition "Self-service payment kiosk/terminal."@en ;
    skos:inScheme piirritev:OsmAmenity ;
    skos:prefLabel "Payment terminal"@en .

piirritev:OsmAmenityPharmacy a skos:Concept ;
    piirrite:hasRelatedOsmTag piirrite:hasOsmPharmacyDispensing,
        piirrite:hasOsmPharmacyDriveThrough,
        piirrite:hasOsmPharmacyHealthcare,
        piirrite:hasOsmPharmacyMedicalSupply,
        piirrite:hasOsmPharmacyName,
        piirrite:hasOsmPharmacyOperator,
        piirrite:hasOsmPharmacyWebsite ;
    piirrite:osmId "pharmacy" ;
    rdfs:subClassOf piirrite:OsmEntity ;
    skos:definition "A shop where a pharmacist sells medications."@en ;
    skos:inScheme piirritev:OsmAmenity ;
    skos:prefLabel "Pharmacy"@en .

piirritev:OsmAmenityPolice a skos:Concept ;
    piirrite:hasRelatedOsmTag piirrite:hasOsmPoliceDetention,
        piirrite:hasOsmPoliceName,
        piirrite:hasOsmPoliceOpeningHours,
        piirrite:hasOsmPoliceOperator,
        piirrite:hasOsmPoliceType,
        piirrite:hasOsmPoliceWheelchair ;
    piirrite:osmId "police" ;
    rdfs:subClassOf piirrite:OsmEntity ;
    skos:definition "A police station is a facility where police officers patrol from and that is a first point of contact for civilians. osmcarto-rendering=File:Police-16.svg osmcarto-rendering-size=24px osmcarto-rendering-area=File:Police fire station 100.png osmcarto-rendering-area-size=100px"@en ;
    skos:inScheme piirritev:OsmAmenity ;
    skos:prefLabel "Police"@en .

piirritev:OsmAmenityPostBox a skos:Concept ;
    piirrite:hasRelatedOsmTag piirrite:hasOsmPostBoxCheckDate,
        piirrite:hasOsmPostBoxCollectionTimes,
        piirrite:hasOsmPostBoxDriveThrough,
        piirrite:hasOsmPostBoxOperator,
        piirrite:hasOsmPostBoxRef ;
    piirrite:osmId "post_box" ;
    rdfs:subClassOf piirrite:OsmEntity ;
    skos:definition "A box to deposit outgoing postal items."@en ;
    skos:inScheme piirritev:OsmAmenity ;
    skos:prefLabel "Post box"@en .

piirritev:OsmAmenityPostOffice a skos:Concept ;
    piirrite:hasRelatedOsmTag piirrite:hasOsmPostOfficeAmenity,
        piirrite:hasOsmPostOfficeAtm,
        piirrite:hasOsmPostOfficeBrand,
        piirrite:hasOsmPostOfficeChangeMachine,
        piirrite:hasOsmPostOfficeName,
        piirrite:hasOsmPostOfficeOperator,
        piirrite:hasOsmPostOfficeRef,
        piirrite:hasOsmPostOfficeType,
        piirrite:hasOsmPostOfficeVending ;
    piirrite:osmId "post_office" ;
    rdfs:subClassOf piirrite:OsmEntity ;
    skos:definition "A place where letters and parcels may be sent or collected. osmcarto-rendering=File:Post office-14.svg osmcarto-rendering-size=28px"@en ;
    skos:inScheme piirritev:OsmAmenity ;
    skos:prefLabel "Post office"@en .

piirritev:OsmAmenityPrepSchool a skos:Concept ;
    piirrite:hasRelatedOsmTag piirrite:hasOsmPrepSchoolName,
        piirrite:hasOsmPrepSchoolOpeningHours ;
    piirrite:osmId "prep_school" ;
    rdfs:subClassOf piirrite:OsmEntity ;
    skos:definition "Tutor or test prep centre."@en ;
    skos:inScheme piirritev:OsmAmenity ;
    skos:prefLabel "Prep school"@en .

piirritev:OsmAmenityPrison a skos:Concept ;
    piirrite:hasRelatedOsmTag piirrite:hasOsmPrisonAccess,
        piirrite:hasOsmPrisonBarrier,
        piirrite:hasOsmPrisonName,
        piirrite:hasOsmPrisonOperator,
        piirrite:hasOsmPrisonType ;
    piirrite:osmId "prison" ;
    rdfs:subClassOf piirrite:OsmEntity ;
    skos:definition "A prison or jail where people are incarcerated before trial or after conviction osmcarto-rendering=File:Prison-16.svg osmcarto-rendering-size=28px osmcarto-rendering-area=File:Area_amenity%3Dprison.png osmcarto-rendering-area-size=100px"@en ;
    skos:inScheme piirritev:OsmAmenity ;
    skos:prefLabel "Prison"@en .

piirritev:OsmAmenityPub a skos:Concept ;
    piirrite:hasRelatedOsmTag piirrite:hasOsmPubBrewery,
        piirrite:hasOsmPubContact,
        piirrite:hasOsmPubCuisine,
        piirrite:hasOsmPubDistillery,
        piirrite:hasOsmPubDrink,
        piirrite:hasOsmPubInternetAccess,
        piirrite:hasOsmPubLiveMusic,
        piirrite:hasOsmPubMicrobrewery,
        piirrite:hasOsmPubName,
        piirrite:hasOsmPubOpeningHours,
        piirrite:hasOsmPubOperator,
        piirrite:hasOsmPubOutdoorSeating,
        piirrite:hasOsmPubWinery ;
    piirrite:osmId "pub" ;
    rdfs:subClassOf piirrite:OsmEntity ;
    skos:definition "osmcarto-rendering=File:Pub-16.svg osmcarto-rendering-size=28px"@en ;
    skos:inScheme piirritev:OsmAmenity ;
    skos:prefLabel "Pub"@en .

piirritev:OsmAmenityPublicBath a skos:Concept ;
    piirrite:hasRelatedOsmTag piirrite:hasOsmPublicBathFee,
        piirrite:hasOsmPublicBathFemale,
        piirrite:hasOsmPublicBathGenderSegregated,
        piirrite:hasOsmPublicBathMale,
        piirrite:hasOsmPublicBathName,
        piirrite:hasOsmPublicBathNudism,
        piirrite:hasOsmPublicBathOutdoor,
        piirrite:hasOsmPublicBathShower,
        piirrite:hasOsmPublicBathUnisex ;
    piirrite:osmId "public_bath" ;
    rdfs:subClassOf piirrite:OsmEntity ;
    skos:definition "A facility for communal bathing that is open to the public."@en ;
    skos:inScheme piirritev:OsmAmenity ;
    skos:prefLabel "Public bath"@en .

piirritev:OsmAmenityPublicBookcase a skos:Concept ;
    piirrite:hasRelatedOsmTag piirrite:hasOsmPublicBookcaseBrand,
        piirrite:hasOsmPublicBookcaseCapacity,
        piirrite:hasOsmPublicBookcaseDescription,
        piirrite:hasOsmPublicBookcaseLocation,
        piirrite:hasOsmPublicBookcaseName,
        piirrite:hasOsmPublicBookcaseOpeningHours,
        piirrite:hasOsmPublicBookcaseOperator,
        piirrite:hasOsmPublicBookcaseWebsite ;
    piirrite:osmId "public_bookcase" ;
    rdfs:subClassOf piirrite:OsmEntity ;
    skos:definition "A street furniture containing books. Take one, leave one."@en ;
    skos:inScheme piirritev:OsmAmenity ;
    skos:prefLabel "Public bookcase"@en .

piirritev:OsmAmenityPublicBuilding a skos:Concept ;
    piirrite:osmId "public_building" ;
    rdfs:subClassOf piirrite:OsmEntity ;
    skos:definition "Using this tag is discouraged, use tag:building=public or tag:building=civic or a feature tag like tag:office=government, tag:amenity=townhall instead."@en ;
    skos:inScheme piirritev:OsmAmenity ;
    skos:prefLabel "Public building"@en .

piirritev:OsmAmenityRecycling a skos:Concept ;
    piirrite:hasRelatedOsmTag piirrite:hasOsmRecyclingCapacity,
        piirrite:hasOsmRecyclingFee,
        piirrite:hasOsmRecyclingOpeningHours,
        piirrite:hasOsmRecyclingOperator,
        piirrite:hasOsmRecyclingRef ;
    piirrite:osmId "recycling" ;
    rdfs:subClassOf piirrite:OsmEntity ;
    skos:definition "A container or centre that accepts waste material for reuse or recycling. osmcarto-rendering=File:Recycling-16.svg osmcarto-rendering-size=28px"@en ;
    skos:inScheme piirritev:OsmAmenity ;
    skos:prefLabel "Recycling"@en .

piirritev:OsmAmenityRestaurant a skos:Concept ;
    piirrite:hasRelatedOsmTag piirrite:hasOsmRestaurantAirConditioning,
        piirrite:hasOsmRestaurantAmenity,
        piirrite:hasOsmRestaurantBar,
        piirrite:hasOsmRestaurantBrand,
        piirrite:hasOsmRestaurantBreakfast,
        piirrite:hasOsmRestaurantCapacity,
        piirrite:hasOsmRestaurantChangingTable,
        piirrite:hasOsmRestaurantCuisine,
        piirrite:hasOsmRestaurantDelivery,
        piirrite:hasOsmRestaurantDinner,
        piirrite:hasOsmRestaurantDog,
        piirrite:hasOsmRestaurantDriveThrough,
        piirrite:hasOsmRestaurantHighchair,
        piirrite:hasOsmRestaurantImage,
        piirrite:hasOsmRestaurantInternetAccess,
        piirrite:hasOsmRestaurantKidsArea,
        piirrite:hasOsmRestaurantLevel,
        piirrite:hasOsmRestaurantLunch,
        piirrite:hasOsmRestaurantMicrobrewery,
        piirrite:hasOsmRestaurantName,
        piirrite:hasOsmRestaurantOpeningHours,
        piirrite:hasOsmRestaurantOperator,
        piirrite:hasOsmRestaurantOutdoorSeating,
        piirrite:hasOsmRestaurantPhone,
        piirrite:hasOsmRestaurantReservation,
        piirrite:hasOsmRestaurantSmoking,
        piirrite:hasOsmRestaurantStars,
        piirrite:hasOsmRestaurantStartDate,
        piirrite:hasOsmRestaurantTakeaway,
        piirrite:hasOsmRestaurantTelevision,
        piirrite:hasOsmRestaurantToilets,
        piirrite:hasOsmRestaurantWebsite,
        piirrite:hasOsmRestaurantWheelchair,
        piirrite:hasOsmRestaurantWikimediaCommons ;
    piirrite:osmId "restaurant" ;
    rdfs:subClassOf piirrite:OsmEntity ;
    skos:definition "A restaurant sells full sit-down meals with servers, and may sell alcohol.  osmcarto-rendering = File:Restaurant-14.svg  osmcarto-rendering-size = 28px"@en ;
    skos:inScheme piirritev:OsmAmenity ;
    skos:prefLabel "Restaurant"@en .

piirritev:OsmAmenitySchool a skos:Concept ;
    piirrite:hasRelatedOsmTag piirrite:hasOsmSchoolName,
        piirrite:hasOsmSchoolOperator ;
    piirrite:osmId "school" ;
    rdfs:subClassOf piirrite:OsmEntity ;
    skos:definition "A primary or secondary school (pupils typically aged 6 to 18). osmcarto-rendering-node = File:Rendering-amenity-school.png osmcarto-rendering-node-size = 125px osmcarto-rendering-area = File:Rendering-area-amenity-school.png osmcarto-rendering-area-size = 125px"@en ;
    skos:inScheme piirritev:OsmAmenity ;
    skos:prefLabel "School"@en .

piirritev:OsmAmenityShelter a skos:Concept ;
    piirrite:hasRelatedOsmTag piirrite:hasOsmShelterAccess,
        piirrite:hasOsmShelterBench,
        piirrite:hasOsmShelterBin,
        piirrite:hasOsmShelterBuilding,
        piirrite:hasOsmShelterDrinkingWater,
        piirrite:hasOsmShelterHighway,
        piirrite:hasOsmShelterLockable,
        piirrite:hasOsmShelterLocked,
        piirrite:hasOsmShelterPicnicTable,
        piirrite:hasOsmShelterPublicTransport,
        piirrite:hasOsmShelterShelterType,
        piirrite:hasOsmShelterSurface,
        piirrite:hasOsmShelterTable,
        piirrite:hasOsmShelterTourism,
        piirrite:hasOsmShelterType ;
    piirrite:osmId "shelter" ;
    rdfs:subClassOf piirrite:OsmEntity ;
    skos:definition "A small structure for protection against bad weather conditions osmcarto-rendering=File:Shelter-14.svg osmcarto-rendering-size=28px"@en ;
    skos:inScheme piirritev:OsmAmenity ;
    skos:prefLabel "Shelter"@en .

piirritev:OsmAmenityShower a skos:Concept ;
    piirrite:hasRelatedOsmTag piirrite:hasOsmShowerAccess,
        piirrite:hasOsmShowerCapacity,
        piirrite:hasOsmShowerCentralkey,
        piirrite:hasOsmShowerFee,
        piirrite:hasOsmShowerFemale,
        piirrite:hasOsmShowerHotWater,
        piirrite:hasOsmShowerIndoor,
        piirrite:hasOsmShowerMale,
        piirrite:hasOsmShowerName,
        piirrite:hasOsmShowerOpeningHours,
        piirrite:hasOsmShowerOperator,
        piirrite:hasOsmShowerOutdoor,
        piirrite:hasOsmShowerSupervised,
        piirrite:hasOsmShowerUnisex,
        piirrite:hasOsmShowerWheelchair ;
    piirrite:osmId "shower" ;
    rdfs:subClassOf piirrite:OsmEntity ;
    skos:definition "Public showers, where people can bathe under water sprays"@en ;
    skos:inScheme piirritev:OsmAmenity ;
    skos:prefLabel "Shower"@en .

piirritev:OsmAmenitySocialCentre a skos:Concept ;
    piirrite:hasRelatedOsmTag piirrite:hasOsmSocialCentreBuilding,
        piirrite:hasOsmSocialCentreName ;
    piirrite:osmId "social_centre" ;
    rdfs:subClassOf piirrite:OsmEntity ;
    skos:definition "A centre of fraternities, sororities, professional societies, union halls and other nonprofit organizations."@en ;
    skos:inScheme piirritev:OsmAmenity ;
    skos:prefLabel "Social centre"@en .

piirritev:OsmAmenitySocialFacility a skos:Concept ;
    piirrite:hasRelatedOsmTag piirrite:hasOsmSocialFacilityName,
        piirrite:hasOsmSocialFacilityType ;
    piirrite:osmId "social_facility" ;
    rdfs:subClassOf piirrite:OsmEntity ;
    skos:definition "A facility that provides social services."@en ;
    skos:inScheme piirritev:OsmAmenity ;
    skos:prefLabel "Social facility"@en .

piirritev:OsmAmenityStudio a skos:Concept ;
    piirrite:hasRelatedOsmTag piirrite:hasOsmStudioName,
        piirrite:hasOsmStudioPhone,
        piirrite:hasOsmStudioType,
        piirrite:hasOsmStudioWebsite ;
    piirrite:osmId "studio" ;
    rdfs:subClassOf piirrite:OsmEntity ;
    skos:definition "A studio used for creating radio or television programmes and broadcasting them. It can also be used to mark a music recording studio."@en ;
    skos:inScheme piirritev:OsmAmenity ;
    skos:prefLabel "Studio"@en .

piirritev:OsmAmenityTaxi a skos:Concept ;
    piirrite:hasRelatedOsmTag piirrite:hasOsmTaxiName,
        piirrite:hasOsmTaxiOperator,
        piirrite:hasOsmTaxiPhone,
        piirrite:hasOsmTaxiTaxiVehicle ;
    piirrite:osmId "taxi" ;
    rdfs:subClassOf piirrite:OsmEntity ;
    skos:definition "A place where taxis wait for passengers. Often near where many people congregate. osmcarto-rendering=File:Taxi.16.svg osmcarto-rendering-size=28px osmcarto-rendering-area=File:Area parking.png osmcarto-rendering-area-size=100px"@en ;
    skos:inScheme piirritev:OsmAmenity ;
    skos:prefLabel "Taxi"@en .

piirritev:OsmAmenityTelephone a skos:Concept ;
    piirrite:hasRelatedOsmTag piirrite:hasOsmTelephoneIndoor,
        piirrite:hasOsmTelephoneOperator,
        piirrite:hasOsmTelephonePhone,
        piirrite:hasOsmTelephoneRef ;
    piirrite:osmId "telephone" ;
    rdfs:subClassOf piirrite:OsmEntity ;
    skos:definition "A public telephone. osmcarto-rendering=File:Telephone.16.svg osmcarto-rendering-size=28px"@en ;
    skos:inScheme piirritev:OsmAmenity ;
    skos:prefLabel "Telephone"@en .

piirritev:OsmAmenityTheatre a skos:Concept ;
    piirrite:hasRelatedOsmTag piirrite:hasOsmTheatreName,
        piirrite:hasOsmTheatreOpeningHours,
        piirrite:hasOsmTheatreOperator,
        piirrite:hasOsmTheatrePhone,
        piirrite:hasOsmTheatreWebsite,
        piirrite:hasOsmTheatreWheelchair ;
    piirrite:osmId "theatre" ;
    rdfs:subClassOf piirrite:OsmEntity ;
    skos:definition "A place where live performances occur, such as plays, musicals and formal concerts.  osmcarto-rendering = File:Theatre-16.svg  osmcarto-rendering-size = 28px"@en ;
    skos:inScheme piirritev:OsmAmenity ;
    skos:prefLabel "Theatre"@en .

piirritev:OsmAmenityTicketValidator a skos:Concept ;
    piirrite:hasRelatedOsmTag piirrite:hasOsmTicketValidatorBarrier,
        piirrite:hasOsmTicketValidatorNetwork,
        piirrite:hasOsmTicketValidatorOperator ;
    piirrite:osmId "ticket_validator" ;
    rdfs:subClassOf piirrite:OsmEntity ;
    skos:definition "An analog device which validates public transport tickets, or devices which are integrated in systems to gain access to an area or service like public transport or parking garages."@en ;
    skos:inScheme piirritev:OsmAmenity ;
    skos:prefLabel "Ticket validator"@en .

piirritev:OsmAmenityToilets a skos:Concept ;
    piirrite:hasRelatedOsmTag piirrite:hasOsmToiletsChangingTable,
        piirrite:hasOsmToiletsComposting,
        piirrite:hasOsmToiletsDrinkingWater,
        piirrite:hasOsmToiletsFee,
        piirrite:hasOsmToiletsHotWater,
        piirrite:hasOsmToiletsIndoor,
        piirrite:hasOsmToiletsOpeningHours,
        piirrite:hasOsmToiletsOperator,
        piirrite:hasOsmToiletsSupervised,
        piirrite:hasOsmToiletsType,
        piirrite:hasOsmToiletsWheelchair ;
    piirrite:osmId "toilets" ;
    rdfs:subClassOf piirrite:OsmEntity ;
    skos:definition "Indicates publicly accessible toilets.  osmcarto-rendering = File:Toilets-16.svg  osmcarto-rendering-size = 28px"@en ;
    skos:inScheme piirritev:OsmAmenity ;
    skos:prefLabel "Toilets"@en .

piirritev:OsmAmenityTownhall a skos:Concept ;
    piirrite:hasRelatedOsmTag piirrite:hasOsmTownhallBuilding,
        piirrite:hasOsmTownhallName,
        piirrite:hasOsmTownhallOperator ;
    piirrite:osmId "townhall" ;
    rdfs:subClassOf piirrite:OsmEntity ;
    skos:definition "A townhall serves as a community administrative center or meeting place. osmcarto-rendering=File:Town-hall-16.svg osmcarto-rendering-size=28px"@en ;
    skos:inScheme piirritev:OsmAmenity ;
    skos:prefLabel "Townhall"@en .

piirritev:OsmAmenityTrolleyBay a skos:Concept ;
    piirrite:osmId "trolley_bay" ;
    rdfs:subClassOf piirrite:OsmEntity ;
    skos:definition "A trolley bay (aka cart corral) is the place where trolleys are \"parked\"."@en ;
    skos:inScheme piirritev:OsmAmenity ;
    skos:prefLabel "Trolley bay"@en .

piirritev:OsmAmenityUniversity a skos:Concept ;
    piirrite:hasRelatedOsmTag piirrite:hasOsmUniversityName,
        piirrite:hasOsmUniversityOperator,
        piirrite:hasOsmUniversityType ;
    piirrite:osmId "university" ;
    rdfs:subClassOf piirrite:OsmEntity ;
    skos:definition "An educational institution designed for instruction, examination, or both, of students in many branches of advanced learning."@en ;
    skos:inScheme piirritev:OsmAmenity ;
    skos:prefLabel "University"@en .

piirritev:OsmAmenityVehicleInspection a skos:Concept ;
    piirrite:hasRelatedOsmTag piirrite:hasOsmVehicleInspectionName,
        piirrite:hasOsmVehicleInspectionOpeningHours,
        piirrite:hasOsmVehicleInspectionOperator,
        piirrite:hasOsmVehicleInspectionPhone,
        piirrite:hasOsmVehicleInspectionWebsite ;
    piirrite:osmId "vehicle_inspection" ;
    rdfs:subClassOf piirrite:OsmEntity ;
    skos:definition "A place where legally-required vehicle inspection may be performed osmcarto-rendering = File:Vehicle inspection-14.svg osmcarto-rendering-size = 28px"@en ;
    skos:inScheme piirritev:OsmAmenity ;
    skos:prefLabel "Vehicle inspection"@en .

piirritev:OsmAmenityVendingMachine a skos:Concept ;
    piirrite:hasRelatedOsmTag piirrite:hasOsmVendingMachineOperator,
        piirrite:hasOsmVendingMachineRef,
        piirrite:hasOsmVendingMachineVending ;
    piirrite:osmId "vending_machine" ;
    rdfs:subClassOf piirrite:OsmEntity ;
    skos:definition "A vending machine sells food, drinks, tickets or other goods automatically."@en ;
    skos:inScheme piirritev:OsmAmenity ;
    skos:prefLabel "Vending machine"@en .

piirritev:OsmAmenityVeterinary a skos:Concept ;
    piirrite:hasRelatedOsmTag piirrite:hasOsmVeterinaryName ;
    piirrite:osmId "veterinary" ;
    rdfs:subClassOf piirrite:OsmEntity ;
    skos:definition "A place that deals with the prevention, diagnosis and treatment of disease in animals. osmcarto-rendering=File:Veterinary-14.svg osmcarto-rendering-size=28px"@en ;
    skos:inScheme piirritev:OsmAmenity ;
    skos:prefLabel "Veterinary"@en .

piirritev:OsmAmenityWasteBasket a skos:Concept ;
    piirrite:hasRelatedOsmTag piirrite:hasOsmWasteBasketWaste ;
    piirrite:osmId "waste_basket" ;
    rdfs:subClassOf piirrite:OsmEntity ;
    skos:definition "A single small container for depositing garbage that is easily accessible for pedestrians. osmcarto-rendering=File:Waste-basket-12.svg osmcarto-rendering-size=24px"@en ;
    skos:inScheme piirritev:OsmAmenity ;
    skos:prefLabel "Waste basket"@en .

piirritev:OsmAmenityWasteDisposal a skos:Concept ;
    piirrite:hasRelatedOsmTag piirrite:hasOsmWasteDisposalAccess,
        piirrite:hasOsmWasteDisposalFee,
        piirrite:hasOsmWasteDisposalOperator,
        piirrite:hasOsmWasteDisposalWaste ;
    piirrite:osmId "waste_disposal" ;
    rdfs:subClassOf piirrite:OsmEntity ;
    skos:definition "A medium or large disposal bin, typically for bagged up household or industrial waste."@en ;
    skos:inScheme piirritev:OsmAmenity ;
    skos:prefLabel "Waste disposal"@en .

piirritev:OsmAmenityWaterPoint a skos:Concept ;
    piirrite:osmId "water_point" ;
    rdfs:subClassOf piirrite:OsmEntity ;
    skos:definition "A place where you can get large amounts of drinking water for refilling fresh water holding tanks."@en ;
    skos:inScheme piirritev:OsmAmenity ;
    skos:prefLabel "Water point"@en .

piirritev:OsmAmenityWateringPlace a skos:Concept ;
    piirrite:hasRelatedOsmTag piirrite:hasOsmWateringPlaceName ;
    piirrite:osmId "watering_place" ;
    rdfs:subClassOf piirrite:OsmEntity ;
    skos:definition "A place where water is contained and animals such as horses can drink."@en ;
    skos:inScheme piirritev:OsmAmenity ;
    skos:prefLabel "Watering place"@en .

piirritev:OsmAmenityWeighbridge a skos:Concept ;
    piirrite:hasRelatedOsmTag piirrite:hasOsmWeighbridgeHighway,
        piirrite:hasOsmWeighbridgeOperator ;
    piirrite:osmId "weighbridge" ;
    rdfs:subClassOf piirrite:OsmEntity ;
    skos:definition "A large weight scale to weigh vehicles and goods."@en ;
    skos:inScheme piirritev:OsmAmenity ;
    skos:prefLabel "Weighbridge"@en .

piirritev:OsmArea a skos:ConceptScheme ;
    piirrite:osmId "area" ;
    skos:definition "Indicates whether a closed way represents an area or just a circular way."@en ;
    skos:prefLabel "Area, types"@en .

piirritev:OsmArmrest a skos:ConceptScheme ;
    piirrite:osmId "armrest" ;
    skos:definition "Whether a bench has any armrests."@en ;
    skos:prefLabel "Armrest, types"@en .

piirritev:OsmArtistName a skos:ConceptScheme ;
    piirrite:osmId "artist_name" ;
    skos:definition "A name of an artist who created the piece of art."@en ;
    skos:prefLabel "Artist name, types"@en .

piirritev:OsmArtworkTypeInstallation a skos:Concept ;
    piirrite:hasRelatedOsmTag piirrite:hasOsmInstallationName ;
    piirrite:osmId "installation" ;
    rdfs:subClassOf piirrite:OsmEntity ;
    skos:definition "Installation art"@en ;
    skos:inScheme piirritev:OsmArtworkType ;
    skos:prefLabel "Installation"@en .

piirritev:OsmArtworkTypeMural a skos:Concept ;
    piirrite:hasRelatedOsmTag piirrite:hasOsmMuralArtistName,
        piirrite:hasOsmMuralArtworkSubject,
        piirrite:hasOsmMuralHistoric,
        piirrite:hasOsmMuralImage,
        piirrite:hasOsmMuralStartDate,
        piirrite:hasOsmMuralWikimediaCommons ;
    piirrite:osmId "mural" ;
    rdfs:subClassOf piirrite:OsmEntity ;
    skos:definition "A piece of artwork painted directly on a wall."@en ;
    skos:inScheme piirritev:OsmArtworkType ;
    skos:prefLabel "Mural"@en .

piirritev:OsmArtworkTypeSculpture a skos:Concept ;
    piirrite:hasRelatedOsmTag piirrite:hasOsmSculptureName ;
    piirrite:osmId "sculpture" ;
    rdfs:subClassOf piirrite:OsmEntity ;
    skos:definition "Sculpture osmcarto-rendering= osmcarto-rendering-size="@en ;
    skos:inScheme piirritev:OsmArtworkType ;
    skos:prefLabel "Sculpture"@en .

piirritev:OsmArtworkTypeStatue a skos:Concept ;
    piirrite:hasRelatedOsmTag piirrite:hasOsmStatueArtistName,
        piirrite:hasOsmStatueMaterial,
        piirrite:hasOsmStatueName,
        piirrite:hasOsmStatueStartDate,
        piirrite:hasOsmStatueType ;
    piirrite:osmId "statue" ;
    rdfs:subClassOf piirrite:OsmEntity ;
    skos:definition "Figurative sculpture of people, animals or gods in a durable material. osmcarto-rendering=File:Statue-14.svg osmcarto-rendering-size=28px"@en ;
    skos:inScheme piirritev:OsmArtworkType ;
    skos:prefLabel "Statue"@en .

piirritev:OsmAtm a skos:ConceptScheme ;
    piirrite:osmId "atm" ;
    skos:definition ""@en ;
    skos:prefLabel "Atm, types"@en .

piirritev:OsmAttributionBakersfieldGis a skos:Concept ;
    piirrite:osmId "Bakersfield_GIS" ;
    rdfs:subClassOf piirrite:OsmEntity ;
    skos:definition ""@en ;
    skos:inScheme piirritev:OsmAttribution ;
    skos:prefLabel "Bakersfield gis"@en .

piirritev:OsmAttributionMassdot a skos:Concept ;
    piirrite:osmId "massDOT" ;
    rdfs:subClassOf piirrite:OsmEntity ;
    skos:definition ""@en ;
    skos:inScheme piirritev:OsmAttribution ;
    skos:prefLabel "Massdot"@en .

piirritev:OsmAttributionNhd a skos:Concept ;
    piirrite:osmId "NHD" ;
    rdfs:subClassOf piirrite:OsmEntity ;
    skos:definition ""@en ;
    skos:inScheme piirritev:OsmAttribution ;
    skos:prefLabel "Nhd"@en .

piirritev:OsmAttributionTiger a skos:Concept ;
    piirrite:osmId "tiger" ;
    rdfs:subClassOf piirrite:OsmEntity ;
    skos:definition ""@en ;
    skos:inScheme piirritev:OsmAttribution ;
    skos:prefLabel "Tiger"@en .

piirritev:OsmAttributionUs-Nfs a skos:Concept ;
    piirrite:osmId "US-NFS" ;
    rdfs:subClassOf piirrite:OsmEntity ;
    skos:definition ""@en ;
    skos:inScheme piirritev:OsmAttribution ;
    skos:prefLabel "Us-nfs"@en .

piirritev:OsmAttributionUs-Nps a skos:Concept ;
    piirrite:osmId "US-NPS" ;
    rdfs:subClassOf piirrite:OsmEntity ;
    skos:definition ""@en ;
    skos:inScheme piirritev:OsmAttribution ;
    skos:prefLabel "Us-nps"@en .

piirritev:OsmAttributionUsgs-Nhd a skos:Concept ;
    piirrite:osmId "USGS-NHD" ;
    rdfs:subClassOf piirrite:OsmEntity ;
    skos:definition ""@en ;
    skos:inScheme piirritev:OsmAttribution ;
    skos:prefLabel "Usgs-nhd"@en .

piirritev:OsmBackrest a skos:ConceptScheme ;
    piirrite:osmId "backrest" ;
    skos:definition "Whether a bench has a backrest (or backrests)."@en ;
    skos:prefLabel "Backrest, types"@en .

piirritev:OsmBarrierBlock a skos:Concept ;
    piirrite:osmId "block" ;
    rdfs:subClassOf piirrite:OsmEntity ;
    skos:definition "One or more large immobile block(s) usually barring free access along a way. osmcarto-rendering=File:Barrier.svg osmcarto-rendering-size=28px"@en ;
    skos:inScheme piirritev:OsmBarrier ;
    skos:prefLabel "Block"@en .

piirritev:OsmBarrierBollard a skos:Concept ;
    piirrite:hasRelatedOsmTag piirrite:hasOsmBollardType ;
    piirrite:osmId "bollard" ;
    rdfs:subClassOf piirrite:OsmEntity ;
    skos:definition "One or more solid (usually concrete or metal) pillar(s) used to control traffic.  osmcarto-rendering = File:Barrier.svg  osmcarto-rendering-size = 28px"@en ;
    skos:inScheme piirritev:OsmBarrier ;
    skos:prefLabel "Bollard"@en .

piirritev:OsmBarrierCattleGrid a skos:Concept ;
    piirrite:osmId "cattle_grid" ;
    rdfs:subClassOf piirrite:OsmEntity ;
    skos:definition "A hole in the road surface covered in a series of bars that allow wheeled vehicles but not animals to cross.  osmcarto-rendering = File:Barrier cattle grid-14.svg  osmcarto-rendering-size = 28px"@en ;
    skos:inScheme piirritev:OsmBarrier ;
    skos:prefLabel "Cattle grid"@en .

piirritev:OsmBarrierChain a skos:Concept ;
    piirrite:hasRelatedOsmTag piirrite:hasOsmChainAccess,
        piirrite:hasOsmChainLocked,
        piirrite:hasOsmChainWheelchair ;
    piirrite:osmId "chain" ;
    rdfs:subClassOf piirrite:OsmEntity ;
    skos:definition "A chain used to prevent motorised vehicles. osmcarto-rendering=File:Barrier fence mapnik.png osmcarto-rendering-size=125px"@en ;
    skos:inScheme piirritev:OsmBarrier ;
    skos:prefLabel "Chain"@en .

piirritev:OsmBarrierCityWall a skos:Concept ;
    piirrite:hasRelatedOsmTag piirrite:hasOsmCityWallHistoric,
        piirrite:hasOsmCityWallTwoSided ;
    piirrite:osmId "city_wall" ;
    rdfs:subClassOf piirrite:OsmEntity ;
    skos:definition "A fortification used to defend settlements in ancient to modern times.  osmcarto-rendering = File:City-wall-render-eg1.png  osmcarto-rendering-size = 125px"@en ;
    skos:inScheme piirritev:OsmBarrier ;
    skos:prefLabel "City wall"@en .

piirritev:OsmBarrierCycleBarrier a skos:Concept ;
    piirrite:hasRelatedOsmTag piirrite:hasOsmCycleBarrierAccess,
        piirrite:hasOsmCycleBarrierOpening,
        piirrite:hasOsmCycleBarrierOverlap,
        piirrite:hasOsmCycleBarrierSpacing,
        piirrite:hasOsmCycleBarrierType,
        piirrite:hasOsmCycleBarrierWheelchair ;
    piirrite:osmId "cycle_barrier" ;
    rdfs:subClassOf piirrite:OsmEntity ;
    skos:definition "A barrier along a path that slows or prevents access for bicycle users. osmcarto-rendering=File:Cycle barrier-14.svg osmcarto-rendering-size=28px"@en ;
    skos:inScheme piirritev:OsmBarrier ;
    skos:prefLabel "Cycle barrier"@en .

piirritev:OsmBarrierDitch a skos:Concept ;
    piirrite:hasRelatedOsmTag piirrite:hasOsmDitchIntermittent,
        piirrite:hasOsmDitchType,
        piirrite:hasOsmDitchWidth ;
    piirrite:osmId "ditch" ;
    rdfs:subClassOf piirrite:OsmEntity ;
    skos:definition "A ditch or a trench is a long and narrow man-made barrier dug in the ground to prevent access to the other side.  osmcarto-rendering = File:Barrier fence mapnik.png  osmcarto-rendering-size = 125px"@en ;
    skos:inScheme piirritev:OsmBarrier ;
    skos:prefLabel "Ditch"@en .

piirritev:OsmBarrierEntrance a skos:Concept ;
    piirrite:hasRelatedOsmTag piirrite:hasOsmEntranceWidth ;
    piirrite:osmId "entrance" ;
    rdfs:subClassOf piirrite:OsmEntity ;
    skos:definition "An opening or gap in a barrier."@en ;
    skos:inScheme piirritev:OsmBarrier ;
    skos:prefLabel "Entrance"@en .

piirritev:OsmBarrierFence a skos:Concept ;
    piirrite:hasRelatedOsmTag piirrite:hasOsmFenceFenceType,
        piirrite:hasOsmFenceHeight ;
    piirrite:osmId "fence" ;
    rdfs:subClassOf piirrite:OsmEntity ;
    skos:definition "A freestanding structure designed to restrict or prevent movement across a boundary, generally distinguished from a wall by the lightness of its construction. osmcarto-rendering=File:Barrier fence mapnik.png osmcarto-rendering-size=125px"@en ;
    skos:inScheme piirritev:OsmBarrier ;
    skos:prefLabel "Fence"@en .

piirritev:OsmBarrierGate a skos:Concept ;
    piirrite:hasRelatedOsmTag piirrite:hasOsmGateAccess,
        piirrite:hasOsmGateAmenity,
        piirrite:hasOsmGateBarrier,
        piirrite:hasOsmGateBicycle,
        piirrite:hasOsmGateFoot,
        piirrite:hasOsmGateHeight,
        piirrite:hasOsmGateLocked,
        piirrite:hasOsmGateMaxwidth,
        piirrite:hasOsmGateWidth ;
    piirrite:osmId "gate" ;
    rdfs:subClassOf piirrite:OsmEntity ;
    skos:definition "A section in a wall or fence which can be opened to allow access. osmcarto-rendering=File:Barrier gate.svg osmcarto-rendering-size=24px"@en ;
    skos:inScheme piirritev:OsmBarrier ;
    skos:prefLabel "Gate"@en .

piirritev:OsmBarrierGuardRail a skos:Concept ;
    piirrite:hasRelatedOsmTag piirrite:hasOsmGuardRailBarrier,
        piirrite:hasOsmGuardRailFenceType ;
    piirrite:osmId "guard_rail" ;
    rdfs:subClassOf piirrite:OsmEntity ;
    skos:definition "A rail, typically metal, designed to keep vehicles within their roadway and prevent collisions or runaways. Right side is the smooth side facing the roadway. In most editors, the side with arrows points towards the road."@en ;
    skos:inScheme piirritev:OsmBarrier ;
    skos:prefLabel "Guard rail"@en .

piirritev:OsmBarrierHandrail a skos:Concept ;
    piirrite:hasRelatedOsmTag piirrite:hasOsmHandrailType ;
    piirrite:osmId "handrail" ;
    rdfs:subClassOf piirrite:OsmEntity ;
    skos:definition "A rail designed to be grasped by the hand so as to provide stability or support."@en ;
    skos:inScheme piirritev:OsmBarrier ;
    skos:prefLabel "Handrail"@en .

piirritev:OsmBarrierHedge a skos:Concept ;
    piirrite:hasRelatedOsmTag piirrite:hasOsmHedgeGenus,
        piirrite:hasOsmHedgeHeight,
        piirrite:hasOsmHedgeLeafCycle,
        piirrite:hasOsmHedgeLeafType,
        piirrite:hasOsmHedgeSpecies,
        piirrite:hasOsmHedgeTaxon,
        piirrite:hasOsmHedgeWidth ;
    piirrite:osmId "hedge" ;
    rdfs:subClassOf piirrite:OsmEntity ;
    skos:definition "A line of closely spaced shrubs and tree species, which form a barrier or mark the boundary of an area. osmcarto-rendering=File:Barrier hedge.png osmcarto-rendering-size=125px"@en ;
    skos:inScheme piirritev:OsmBarrier ;
    skos:prefLabel "Hedge"@en .

piirritev:OsmBarrierHeightRestrictor a skos:Concept ;
    piirrite:hasRelatedOsmTag piirrite:hasOsmHeightRestrictorMaxheight ;
    piirrite:osmId "height_restrictor" ;
    rdfs:subClassOf piirrite:OsmEntity ;
    skos:definition "A height restrictor which prevents access of vehicles higher than a set limit."@en ;
    skos:inScheme piirritev:OsmBarrier ;
    skos:prefLabel "Height restrictor"@en .

piirritev:OsmBarrierJerseyBarrier a skos:Concept ;
    piirrite:hasRelatedOsmTag piirrite:hasOsmJerseyBarrierAccess ;
    piirrite:osmId "jersey_barrier" ;
    rdfs:subClassOf piirrite:OsmEntity ;
    skos:definition "A barrier made of heavy prefabricated blocks. osmcarto-rendering=File:Barrier fence mapnik.png osmcarto-rendering-size=125px"@en ;
    skos:inScheme piirritev:OsmBarrier ;
    skos:prefLabel "Jersey barrier"@en .

piirritev:OsmBarrierKerb a skos:Concept ;
    piirrite:hasRelatedOsmTag piirrite:hasOsmKerbHeight,
        piirrite:hasOsmKerbTactilePaving,
        piirrite:hasOsmKerbWheelchair ;
    piirrite:osmId "kerb" ;
    rdfs:subClassOf piirrite:OsmEntity ;
    skos:definition "A stone edging to a pavement or raised path. osmcarto-rendering= osmcarto-rendering-size="@en ;
    skos:inScheme piirritev:OsmBarrier ;
    skos:prefLabel "Kerb"@en .

piirritev:OsmBarrierKissingGate a skos:Concept ;
    piirrite:hasRelatedOsmTag piirrite:hasOsmKissingGateMaxwidth ;
    piirrite:osmId "kissing_gate" ;
    rdfs:subClassOf piirrite:OsmEntity ;
    skos:definition "A type of gate where you have to go into an enclosure and open a gate to get through. osmcarto-rendering = File:Kissing gate-14.svg osmcarto-rendering-size = 28px"@en ;
    skos:inScheme piirritev:OsmBarrier ;
    skos:prefLabel "Kissing gate"@en .

piirritev:OsmBarrierLiftGate a skos:Concept ;
    piirrite:hasRelatedOsmTag piirrite:hasOsmLiftGateAccess,
        piirrite:hasOsmLiftGateLocked ;
    piirrite:osmId "lift_gate" ;
    rdfs:subClassOf piirrite:OsmEntity ;
    skos:definition "A bar or pole pivoted (rotates upwards to open) in such a way as to allow the boom to block vehicular access through a controlled point. osmcarto-rendering=File:Liftgate-7.svg osmcarto-rendering-size=28px"@en ;
    skos:inScheme piirritev:OsmBarrier ;
    skos:prefLabel "Lift gate"@en .

piirritev:OsmBarrierLog a skos:Concept ;
    piirrite:hasRelatedOsmTag piirrite:hasOsmLogAccess ;
    piirrite:osmId "log" ;
    rdfs:subClassOf piirrite:OsmEntity ;
    skos:definition "A log blocking access. osmcarto-rendering=File:Barrier.svg osmcarto-rendering-size=28px"@en ;
    skos:inScheme piirritev:OsmBarrier ;
    skos:prefLabel "Log"@en .

piirritev:OsmBarrierRetainingWall a skos:Concept ;
    piirrite:hasRelatedOsmTag piirrite:hasOsmRetainingWallHeight,
        piirrite:hasOsmRetainingWallMaterial ;
    piirrite:osmId "retaining_wall" ;
    rdfs:subClassOf piirrite:OsmEntity ;
    skos:definition "A linear structure that holds back soil or rock. (Lower side to right.)"@en ;
    skos:inScheme piirritev:OsmBarrier ;
    skos:prefLabel "Retaining wall"@en .

piirritev:OsmBarrierSlidingGate a skos:Concept ;
    piirrite:hasRelatedOsmTag piirrite:hasOsmSlidingGateAccess,
        piirrite:hasOsmSlidingGateBicycle,
        piirrite:hasOsmSlidingGateFoot,
        piirrite:hasOsmSlidingGateMaxwidth ;
    piirrite:osmId "sliding_gate" ;
    rdfs:subClassOf piirrite:OsmEntity ;
    skos:definition "A section in a wall or fence which slides or rolls to the side to allow access (note: barrier=gate is the standard tagging for such objects, this tag is used primarily by Grab employees)."@en ;
    skos:inScheme piirritev:OsmBarrier ;
    skos:prefLabel "Sliding gate"@en .

piirritev:OsmBarrierStile a skos:Concept ;
    piirrite:osmId "stile" ;
    rdfs:subClassOf piirrite:OsmEntity ;
    skos:definition "A structure which provides people a passage through or over a boundary via steps, ladders or narrow gaps. osmcarto-rendering=File:Barrier stile-14.svg osmcarto-rendering-size=28px"@en ;
    skos:inScheme piirritev:OsmBarrier ;
    skos:prefLabel "Stile"@en .

piirritev:OsmBarrierSwingGate a skos:Concept ;
    piirrite:hasRelatedOsmTag piirrite:hasOsmSwingGateAccess,
        piirrite:hasOsmSwingGateLocked ;
    piirrite:osmId "swing_gate" ;
    rdfs:subClassOf piirrite:OsmEntity ;
    skos:definition "A gate consisting of a bar or pole pivoted (rotates sidewards to open) in such a way as to allow the boom to block vehicular access through a controlled point. osmcarto-rendering=File:Liftgate-7.svg osmcarto-rendering-size=28px"@en ;
    skos:inScheme piirritev:OsmBarrier ;
    skos:prefLabel "Swing gate"@en .

piirritev:OsmBarrierTollBooth a skos:Concept ;
    piirrite:osmId "toll_booth" ;
    rdfs:subClassOf piirrite:OsmEntity ;
    skos:definition "A place where a road usage toll or fee is collected."@en ;
    skos:inScheme piirritev:OsmBarrier ;
    skos:prefLabel "Toll booth"@en .

piirritev:OsmBarrierTurnstile a skos:Concept ;
    piirrite:osmId "turnstile" ;
    rdfs:subClassOf piirrite:OsmEntity ;
    skos:definition "A turnstile, a passage on foot designed to allow one person at a time to pass osmcarto-rendering=File:Barrier.svg osmcarto-rendering-size=28px"@en ;
    skos:inScheme piirritev:OsmBarrier ;
    skos:prefLabel "Turnstile"@en .

piirritev:OsmBarrierWall a skos:Concept ;
    piirrite:hasRelatedOsmTag piirrite:hasOsmWallHeight,
        piirrite:hasOsmWallMaterial,
        piirrite:hasOsmWallType,
        piirrite:hasOsmWallWidth ;
    piirrite:osmId "wall" ;
    rdfs:subClassOf piirrite:OsmEntity ;
    skos:definition "A freestanding structure, designed to restrict or prevent movement across a boundary, typically made from solid brick, concrete or rocks, and almost always built so that it is opaque to vision. osmcarto-rendering=File:Barrier fence mapnik.png osmcarto-rendering-size=125px"@en ;
    skos:inScheme piirritev:OsmBarrier ;
    skos:prefLabel "Wall"@en .

piirritev:OsmBarrierWicketGate a skos:Concept ;
    piirrite:hasRelatedOsmTag piirrite:hasOsmWicketGateAccess,
        piirrite:hasOsmWicketGateEntrance,
        piirrite:hasOsmWicketGateMaterial,
        piirrite:hasOsmWicketGateOpeningHours,
        piirrite:hasOsmWicketGateWidth ;
    piirrite:osmId "wicket_gate" ;
    rdfs:subClassOf piirrite:OsmEntity ;
    skos:definition "A pedestrian door or gate built into a wall or fence near or within a larger gate."@en ;
    skos:inScheme piirritev:OsmBarrier ;
    skos:prefLabel "Wicket gate"@en .

piirritev:OsmBench a skos:ConceptScheme ;
    piirrite:osmId "bench" ;
    skos:definition "Indicates the presence of an associated bench."@en ;
    skos:prefLabel "Bench, types"@en .

piirritev:OsmBicycleCustomers a skos:Concept ;
    piirrite:osmId "customers" ;
    rdfs:subClassOf piirrite:OsmEntity ;
    skos:definition "Indicates that riding bicycle is allowed for customers of some object."@en ;
    skos:inScheme piirritev:OsmBicycle ;
    skos:prefLabel "Customers"@en .

piirritev:OsmBicycleDesignated a skos:Concept ;
    piirrite:hasRelatedOsmTag piirrite:hasOsmDesignatedHighway ;
    piirrite:osmId "designated" ;
    rdfs:subClassOf piirrite:OsmEntity ;
    skos:definition "Roads and other objects designated/signed to use for cyclists."@en ;
    skos:inScheme piirritev:OsmBicycle ;
    skos:prefLabel "Designated"@en .

piirritev:OsmBicycleDestination a skos:Concept ;
    piirrite:osmId "destination" ;
    rdfs:subClassOf piirrite:OsmEntity ;
    skos:definition ""@en ;
    skos:inScheme piirritev:OsmBicycle ;
    skos:prefLabel "Destination"@en .

piirritev:OsmBicycleDismount a skos:Concept ;
    piirrite:osmId "dismount" ;
    rdfs:subClassOf piirrite:OsmEntity ;
    skos:definition "Indicates that riding bicycle is not allowed, but pushing a bicycle is allowed."@en ;
    skos:inScheme piirritev:OsmBicycle ;
    skos:prefLabel "Dismount"@en .

piirritev:OsmBicycleParkingBollard a skos:Concept ;
    piirrite:hasRelatedOsmTag piirrite:hasOsmBollardCapacity,
        piirrite:hasOsmBollardCovered,
        piirrite:hasOsmBollardSupervised ;
    piirrite:osmId "bollard" ;
    rdfs:subClassOf piirrite:OsmEntity ;
    skos:definition "Bollard with a unique central pole and arms allowing to securely lock a bike."@en ;
    skos:inScheme piirritev:OsmBicycleParking ;
    skos:prefLabel "Bollard"@en .

piirritev:OsmBicycleParkingRack a skos:Concept ;
    piirrite:hasRelatedOsmTag piirrite:hasOsmRackCapacity,
        piirrite:hasOsmRackCovered,
        piirrite:hasOsmRackSupervised ;
    piirrite:osmId "rack" ;
    rdfs:subClassOf piirrite:OsmEntity ;
    skos:definition "Coathanger or ring types of metal brackets to hang bike front wheel only."@en ;
    skos:inScheme piirritev:OsmBicycleParking ;
    skos:prefLabel "Rack"@en .

piirritev:OsmBicycleParkingShed a skos:Concept ;
    piirrite:osmId "shed" ;
    rdfs:subClassOf piirrite:OsmEntity ;
    skos:definition ""@en ;
    skos:inScheme piirritev:OsmBicycleParking ;
    skos:prefLabel "Shed"@en .

piirritev:OsmBicycleParkingStands a skos:Concept ;
    piirrite:hasRelatedOsmTag piirrite:hasOsmStandsCapacity,
        piirrite:hasOsmStandsCovered,
        piirrite:hasOsmStandsSupervised ;
    piirrite:osmId "stands" ;
    rdfs:subClassOf piirrite:OsmEntity ;
    skos:definition "Metal bracket to park bicycles."@en ;
    skos:inScheme piirritev:OsmBicycleParking ;
    skos:prefLabel "Stands"@en .

piirritev:OsmBicycleParkingWallLoops a skos:Concept ;
    piirrite:hasRelatedOsmTag piirrite:hasOsmWallLoopsCapacity,
        piirrite:hasOsmWallLoopsCovered,
        piirrite:hasOsmWallLoopsSupervised ;
    piirrite:osmId "wall_loops" ;
    rdfs:subClassOf piirrite:OsmEntity ;
    skos:definition "Metal bracket for the front wheel for parking bicycles."@en ;
    skos:inScheme piirritev:OsmBicycleParking ;
    skos:prefLabel "Wall loops"@en .

piirritev:OsmBicyclePermissive a skos:Concept ;
    piirrite:hasRelatedOsmTag piirrite:hasOsmPermissiveHighway ;
    piirrite:osmId "permissive" ;
    rdfs:subClassOf piirrite:OsmEntity ;
    skos:definition "Roads and other objects accessible to cyclists, but not explicitly designated/signed for their use and permission can be revoked at any time."@en ;
    skos:inScheme piirritev:OsmBicycle ;
    skos:prefLabel "Permissive"@en .

piirritev:OsmBicyclePrivate a skos:Concept ;
    piirrite:osmId "private" ;
    rdfs:subClassOf piirrite:OsmEntity ;
    skos:definition "Indicates that riding bicycle is not allowed for general public, but some narrow group is allowed to do this (usually owners, employees or persons with temporary/special access)."@en ;
    skos:inScheme piirritev:OsmBicycle ;
    skos:prefLabel "Private"@en .

piirritev:OsmBicycleUseSidepath a skos:Concept ;
    piirrite:hasRelatedOsmTag piirrite:hasOsmUseSidepathHighway ;
    piirrite:osmId "use_sidepath" ;
    rdfs:subClassOf piirrite:OsmEntity ;
    skos:definition "Compulsory cycleway aside"@en ;
    skos:inScheme piirritev:OsmBicycle ;
    skos:prefLabel "Use sidepath"@en .

piirritev:OsmBin a skos:ConceptScheme ;
    piirrite:osmId "bin" ;
    skos:definition "Indicates the presence of an associated waste basket."@en ;
    skos:prefLabel "Bin, types"@en .

piirritev:OsmBoardTypeHistory a skos:Concept ;
    piirrite:osmId "history" ;
    rdfs:subClassOf piirrite:OsmEntity ;
    skos:definition ""@en ;
    skos:inScheme piirritev:OsmBoardType ;
    skos:prefLabel "History"@en .

piirritev:OsmBoardTypeNature a skos:Concept ;
    piirrite:osmId "nature" ;
    rdfs:subClassOf piirrite:OsmEntity ;
    skos:definition ""@en ;
    skos:inScheme piirritev:OsmBoardType ;
    skos:prefLabel "Nature"@en .

piirritev:OsmBoardTypePlants a skos:Concept ;
    piirrite:osmId "plants" ;
    rdfs:subClassOf piirrite:OsmEntity ;
    skos:definition ""@en ;
    skos:inScheme piirritev:OsmBoardType ;
    skos:prefLabel "Plants"@en .

piirritev:OsmBoardTypePublicTransport a skos:Concept ;
    piirrite:osmId "public_transport" ;
    rdfs:subClassOf piirrite:OsmEntity ;
    skos:definition ""@en ;
    skos:inScheme piirritev:OsmBoardType ;
    skos:prefLabel "Public transport"@en .

piirritev:OsmBoardTypeWelcomeSign a skos:Concept ;
    piirrite:osmId "welcome_sign" ;
    rdfs:subClassOf piirrite:OsmEntity ;
    skos:definition ""@en ;
    skos:inScheme piirritev:OsmBoardType ;
    skos:prefLabel "Welcome sign"@en .

piirritev:OsmBoardTypeWildlife a skos:Concept ;
    piirrite:osmId "wildlife" ;
    rdfs:subClassOf piirrite:OsmEntity ;
    skos:definition ""@en ;
    skos:inScheme piirritev:OsmBoardType ;
    skos:prefLabel "Wildlife"@en .

piirritev:OsmBoat a skos:ConceptScheme ;
    piirrite:osmId "boat" ;
    skos:definition "Access permission for boats"@en ;
    skos:prefLabel "Boat, types"@en .

piirritev:OsmBollardFixed a skos:Concept ;
    piirrite:osmId "fixed" ;
    rdfs:subClassOf piirrite:OsmEntity ;
    skos:definition ""@en ;
    skos:inScheme piirritev:OsmBollard ;
    skos:prefLabel "Fixed"@en .

piirritev:OsmBollardFoldable a skos:Concept ;
    piirrite:osmId "foldable" ;
    rdfs:subClassOf piirrite:OsmEntity ;
    skos:definition ""@en ;
    skos:inScheme piirritev:OsmBollard ;
    skos:prefLabel "Foldable"@en .

piirritev:OsmBollardRemovable a skos:Concept ;
    piirrite:osmId "removable" ;
    rdfs:subClassOf piirrite:OsmEntity ;
    skos:definition ""@en ;
    skos:inScheme piirritev:OsmBollard ;
    skos:prefLabel "Removable"@en .

piirritev:OsmBollardRising a skos:Concept ;
    piirrite:osmId "rising" ;
    rdfs:subClassOf piirrite:OsmEntity ;
    skos:definition ""@en ;
    skos:inScheme piirritev:OsmBollard ;
    skos:prefLabel "Rising"@en .

piirritev:OsmBorderTypeCity a skos:Concept ;
    piirrite:osmId "city" ;
    rdfs:subClassOf piirrite:OsmEntity ;
    skos:definition ""@en ;
    skos:inScheme piirritev:OsmBorderType ;
    skos:prefLabel "City"@en .

piirritev:OsmBorderTypeCounty a skos:Concept ;
    piirrite:osmId "county" ;
    rdfs:subClassOf piirrite:OsmEntity ;
    skos:definition ""@en ;
    skos:inScheme piirritev:OsmBorderType ;
    skos:prefLabel "County"@en .

piirritev:OsmBorderTypeFreguesia a skos:Concept ;
    piirrite:osmId "freguesia" ;
    rdfs:subClassOf piirrite:OsmEntity ;
    skos:definition ""@en ;
    skos:inScheme piirritev:OsmBorderType ;
    skos:prefLabel "Freguesia"@en .

piirritev:OsmBorderTypeNation a skos:Concept ;
    piirrite:osmId "nation" ;
    rdfs:subClassOf piirrite:OsmEntity ;
    skos:definition "To tag national borders, you should most likely simply use admin_level=2 instead of this tag. It is mainly in use in Africa and south east Asia but also on the pacific coast of Mexico and the USA."@en ;
    skos:inScheme piirritev:OsmBorderType ;
    skos:prefLabel "Nation"@en .

piirritev:OsmBoundaryAdministrative a skos:Concept ;
    piirrite:hasRelatedOsmTag piirrite:hasOsmAdministrativeAdminLevel,
        piirrite:hasOsmAdministrativeName ;
    piirrite:osmId "administrative" ;
    rdfs:subClassOf piirrite:OsmEntity ;
    skos:definition "An administrative boundary recognised by governments for administrative purposes."@en ;
    skos:inScheme piirritev:OsmBoundary ;
    skos:prefLabel "Administrative"@en .

piirritev:OsmBoundaryCensus a skos:Concept ;
    piirrite:hasRelatedOsmTag piirrite:hasOsmCensusName ;
    piirrite:osmId "census" ;
    rdfs:subClassOf piirrite:OsmEntity ;
    skos:definition "A census-designated boundary delineating a statistical area, not necessarily observable on the ground."@en ;
    skos:inScheme piirritev:OsmBoundary ;
    skos:prefLabel "Census"@en .

piirritev:OsmBoundaryForestCompartment a skos:Concept ;
    piirrite:hasRelatedOsmTag piirrite:hasOsmForestCompartmentRef ;
    piirrite:osmId "forest_compartment" ;
    rdfs:subClassOf piirrite:OsmEntity ;
    skos:definition "A marked subdivision of delimited forest, which is used for planning, management & navigation."@en ;
    skos:inScheme piirritev:OsmBoundary ;
    skos:prefLabel "Forest compartment"@en .

piirritev:OsmBoundaryHealth a skos:Concept ;
    piirrite:osmId "health" ;
    rdfs:subClassOf piirrite:OsmEntity ;
    skos:definition ""@en ;
    skos:inScheme piirritev:OsmBoundary ;
    skos:prefLabel "Health"@en .

piirritev:OsmBoundaryHistoric a skos:Concept ;
    piirrite:hasRelatedOsmTag piirrite:hasOsmHistoricAdminLevel,
        piirrite:hasOsmHistoricEndDate,
        piirrite:hasOsmHistoricName,
        piirrite:hasOsmHistoricStartDate ;
    piirrite:osmId "historic" ;
    rdfs:subClassOf piirrite:OsmEntity ;
    skos:definition "A historic administrative boundary (use judiciously)."@en ;
    skos:inScheme piirritev:OsmBoundary ;
    skos:prefLabel "Historic"@en .

piirritev:OsmBoundaryLocalAuthority a skos:Concept ;
    piirrite:osmId "local_authority" ;
    rdfs:subClassOf piirrite:OsmEntity ;
    skos:definition "Describes the territory of a local authority."@en ;
    skos:inScheme piirritev:OsmBoundary ;
    skos:prefLabel "Local authority"@en .

piirritev:OsmBoundaryMarker a skos:Concept ;
    piirrite:hasRelatedOsmTag piirrite:hasOsmMarkerFormat,
        piirrite:hasOsmMarkerInscription,
        piirrite:hasOsmMarkerMaterial,
        piirrite:hasOsmMarkerName,
        piirrite:hasOsmMarkerRef ;
    piirrite:osmId "marker" ;
    rdfs:subClassOf piirrite:OsmEntity ;
    skos:definition "A physical marker that identifies a boundary"@en ;
    skos:inScheme piirritev:OsmBoundary ;
    skos:prefLabel "Marker"@en .

piirritev:OsmBoundaryPlace a skos:Concept ;
    piirrite:hasRelatedOsmTag piirrite:hasOsmPlaceType ;
    piirrite:osmId "place" ;
    rdfs:subClassOf piirrite:OsmEntity ;
    skos:definition "The boundaries of a key:place, when these boundaries can be defined but these are not administrative boundaries."@en ;
    skos:inScheme piirritev:OsmBoundary ;
    skos:prefLabel "Place"@en .

piirritev:OsmBoundaryPolitical a skos:Concept ;
    piirrite:hasRelatedOsmTag piirrite:hasOsmPoliticalPoliticalDivision ;
    piirrite:osmId "political" ;
    rdfs:subClassOf piirrite:OsmEntity ;
    skos:definition "Political boundary, such as an electoral ward or parliamentary constituency."@en ;
    skos:inScheme piirritev:OsmBoundary ;
    skos:prefLabel "Political"@en .

piirritev:OsmBoundaryPostalCode a skos:Concept ;
    piirrite:hasRelatedOsmTag piirrite:hasOsmPostalCodeType ;
    piirrite:osmId "postal_code" ;
    rdfs:subClassOf piirrite:OsmEntity ;
    skos:definition "A postal code boundary"@en ;
    skos:inScheme piirritev:OsmBoundary ;
    skos:prefLabel "Postal code"@en .

piirritev:OsmBoundaryProtectedArea a skos:Concept ;
    piirrite:hasRelatedOsmTag piirrite:hasOsmProtectedAreaName,
        piirrite:hasOsmProtectedAreaOfficialName,
        piirrite:hasOsmProtectedAreaType ;
    piirrite:osmId "protected_area" ;
    rdfs:subClassOf piirrite:OsmEntity ;
    skos:definition "Used to mark boundaries of protected areas including national parks, wilderness, marine protection areas, heritage sites and other, similar areas."@en ;
    skos:inScheme piirritev:OsmBoundary ;
    skos:prefLabel "Protected area"@en .

piirritev:OsmBoundaryReligiousAdministration a skos:Concept ;
    piirrite:hasRelatedOsmTag piirrite:hasOsmReligiousAdministrationAdminLevel,
        piirrite:hasOsmReligiousAdministrationName,
        piirrite:hasOsmReligiousAdministrationReligion ;
    piirrite:osmId "religious_administration" ;
    rdfs:subClassOf piirrite:OsmEntity ;
    skos:definition "Administrative boundaries of institutionalised religions."@en ;
    skos:inScheme piirritev:OsmBoundary ;
    skos:prefLabel "Religious administration"@en .

piirritev:OsmBranch a skos:ConceptScheme ;
    piirrite:osmId "branch" ;
    skos:definition "Identifies which branch of a brand or chain this object represents, or controversially the name of a branch railway."@en ;
    skos:prefLabel "Branch, types"@en .

piirritev:OsmBrand7-Eleven a skos:Concept ;
    piirrite:osmId "7-Eleven" ;
    rdfs:subClassOf piirrite:OsmEntity ;
    skos:definition ""@en ;
    skos:inScheme piirritev:OsmBrand ;
    skos:prefLabel "7-eleven"@en .

piirritev:OsmBrandBp a skos:Concept ;
    piirrite:osmId "BP" ;
    rdfs:subClassOf piirrite:OsmEntity ;
    skos:definition ""@en ;
    skos:inScheme piirritev:OsmBrand ;
    skos:prefLabel "Bp"@en .

piirritev:OsmBrandBurgerKing a skos:Concept ;
    piirrite:osmId "Burger_King" ;
    rdfs:subClassOf piirrite:OsmEntity ;
    skos:definition ""@en ;
    skos:inScheme piirritev:OsmBrand ;
    skos:prefLabel "Burger king"@en .

piirritev:OsmBrandCanadaPost a skos:Concept ;
    piirrite:osmId "Canada_Post" ;
    rdfs:subClassOf piirrite:OsmEntity ;
    skos:definition ""@en ;
    skos:inScheme piirritev:OsmBrand ;
    skos:prefLabel "Canada post"@en .

piirritev:OsmBrandDeutschePost a skos:Concept ;
    piirrite:hasRelatedOsmTag piirrite:hasOsmDeutschePostAmenity ;
    piirrite:osmId "Deutsche_Post" ;
    rdfs:subClassOf piirrite:OsmEntity ;
    skos:definition "A brand of Germany's biggest postal service."@en ;
    skos:inScheme piirritev:OsmBrand ;
    skos:prefLabel "Deutsche post"@en .

piirritev:OsmBrandDollarGeneral a skos:Concept ;
    piirrite:osmId "Dollar_General" ;
    rdfs:subClassOf piirrite:OsmEntity ;
    skos:definition ""@en ;
    skos:inScheme piirritev:OsmBrand ;
    skos:prefLabel "Dollar general"@en .

piirritev:OsmBrandHelloCycling a skos:Concept ;
    piirrite:osmId "HELLO_CYCLING" ;
    rdfs:subClassOf piirrite:OsmEntity ;
    skos:definition ""@en ;
    skos:inScheme piirritev:OsmBrand ;
    skos:prefLabel "Hello cycling"@en .

piirritev:OsmBrandKfc a skos:Concept ;
    piirrite:osmId "KFC" ;
    rdfs:subClassOf piirrite:OsmEntity ;
    skos:definition ""@en ;
    skos:inScheme piirritev:OsmBrand ;
    skos:prefLabel "Kfc"@en .

piirritev:OsmBrandLaPoste a skos:Concept ;
    piirrite:osmId "La_Poste" ;
    rdfs:subClassOf piirrite:OsmEntity ;
    skos:definition ""@en ;
    skos:inScheme piirritev:OsmBrand ;
    skos:prefLabel "La poste"@en .

piirritev:OsmBrandLidl a skos:Concept ;
    piirrite:osmId "Lidl" ;
    rdfs:subClassOf piirrite:OsmEntity ;
    skos:definition ""@en ;
    skos:inScheme piirritev:OsmBrand ;
    skos:prefLabel "Lidl"@en .

piirritev:OsmBrandMcdonalds a skos:Concept ;
    piirrite:osmId "McDonalds" ;
    rdfs:subClassOf piirrite:OsmEntity ;
    skos:definition ""@en ;
    skos:inScheme piirritev:OsmBrand ;
    skos:prefLabel "Mcdonalds"@en .

piirritev:OsmBrandNationalGrid a skos:Concept ;
    piirrite:osmId "National_Grid" ;
    rdfs:subClassOf piirrite:OsmEntity ;
    skos:definition ""@en ;
    skos:inScheme piirritev:OsmBrand ;
    skos:prefLabel "National grid"@en .

piirritev:OsmBrandOzon a skos:Concept ;
    piirrite:osmId "Ozon" ;
    rdfs:subClassOf piirrite:OsmEntity ;
    skos:definition ""@en ;
    skos:inScheme piirritev:OsmBrand ;
    skos:prefLabel "Ozon"@en .

piirritev:OsmBrandPaczkomatInpost a skos:Concept ;
    piirrite:osmId "Paczkomat_InPost" ;
    rdfs:subClassOf piirrite:OsmEntity ;
    skos:definition ""@en ;
    skos:inScheme piirritev:OsmBrand ;
    skos:prefLabel "Paczkomat inpost"@en .

piirritev:OsmBrandRoyalMail a skos:Concept ;
    piirrite:osmId "Royal_Mail" ;
    rdfs:subClassOf piirrite:OsmEntity ;
    skos:definition ""@en ;
    skos:inScheme piirritev:OsmBrand ;
    skos:prefLabel "Royal mail"@en .

piirritev:OsmBrandShell a skos:Concept ;
    piirrite:osmId "Shell" ;
    rdfs:subClassOf piirrite:OsmEntity ;
    skos:definition ""@en ;
    skos:inScheme piirritev:OsmBrand ;
    skos:prefLabel "Shell"@en .

piirritev:OsmBrandStarbucks a skos:Concept ;
    piirrite:osmId "Starbucks" ;
    rdfs:subClassOf piirrite:OsmEntity ;
    skos:definition ""@en ;
    skos:inScheme piirritev:OsmBrand ;
    skos:prefLabel "Starbucks"@en .

piirritev:OsmBrandSubway a skos:Concept ;
    piirrite:osmId "Subway" ;
    rdfs:subClassOf piirrite:OsmEntity ;
    skos:definition ""@en ;
    skos:inScheme piirritev:OsmBrand ;
    skos:prefLabel "Subway"@en .

piirritev:OsmBrand a skos:Concept ;
    piirrite:osmId "" ;
    rdfs:subClassOf piirrite:OsmEntity ;
    skos:definition ""@en ;
    skos:inScheme piirritev:OsmBrand ;
    skos:prefLabel ""@en .

piirritev:OsmBrand a skos:Concept ;
    piirrite:osmId "" ;
    rdfs:subClassOf piirrite:OsmEntity ;
    skos:definition ""@en ;
    skos:inScheme piirritev:OsmBrand ;
    skos:prefLabel ""@en .

piirritev:OsmBridgeAqueduct a skos:Concept ;
    piirrite:osmId "aqueduct" ;
    rdfs:subClassOf piirrite:OsmEntity ;
    skos:definition "A bridge which conveys an artificial waterway over a road, valley or waterway."@en ;
    skos:inScheme piirritev:OsmBridge ;
    skos:prefLabel "Aqueduct"@en .

piirritev:OsmBridgeBoardwalk a skos:Concept ;
    piirrite:hasRelatedOsmTag piirrite:hasOsmBoardwalkHighway ;
    piirrite:osmId "boardwalk" ;
    rdfs:subClassOf piirrite:OsmEntity ;
    skos:definition "Plank walkway"@en ;
    skos:inScheme piirritev:OsmBridge ;
    skos:prefLabel "Boardwalk"@en .

piirritev:OsmBridgeViaduct a skos:Concept ;
    piirrite:hasRelatedOsmTag piirrite:hasOsmViaductHighway,
        piirrite:hasOsmViaductLength,
        piirrite:hasOsmViaductName,
        piirrite:hasOsmViaductRailway,
        piirrite:hasOsmViaductRuins,
        piirrite:hasOsmViaductStartDate,
        piirrite:hasOsmViaductWikipedia ;
    piirrite:osmId "viaduct" ;
    rdfs:subClassOf piirrite:OsmEntity ;
    skos:definition "A long rail, road, or other bridge made up of many short spans."@en ;
    skos:inScheme piirritev:OsmBridge ;
    skos:prefLabel "Viaduct"@en .

piirritev:OsmBuildingAgricultural a skos:Concept ;
    piirrite:hasRelatedOsmTag piirrite:hasOsmAgriculturalLanduse ;
    piirrite:osmId "agricultural" ;
    rdfs:subClassOf piirrite:OsmEntity ;
    skos:definition "A building built for agricultural purposes"@en ;
    skos:inScheme piirritev:OsmBuilding ;
    skos:prefLabel "Agricultural"@en .

piirritev:OsmBuildingAllotmentHouse a skos:Concept ;
    piirrite:osmId "allotment_house" ;
    rdfs:subClassOf piirrite:OsmEntity ;
    skos:definition "A small outbuilding for short visits in a allotment garden."@en ;
    skos:inScheme piirritev:OsmBuilding ;
    skos:prefLabel "Allotment house"@en .

piirritev:OsmBuildingApartments a skos:Concept ;
    piirrite:osmId "apartments" ;
    rdfs:subClassOf piirrite:OsmEntity ;
    skos:definition "A building arranged into individual dwellings, often on separate floors. May also have retail outlets on the ground floor."@en ;
    skos:inScheme piirritev:OsmBuilding ;
    skos:prefLabel "Apartments"@en .

piirritev:OsmBuildingBarn a skos:Concept ;
    piirrite:hasRelatedOsmTag piirrite:hasOsmBarnLanduse ;
    piirrite:osmId "barn" ;
    rdfs:subClassOf piirrite:OsmEntity ;
    skos:definition "An agricultural building that can be used for storage and as a covered workplace."@en ;
    skos:inScheme piirritev:OsmBuilding ;
    skos:prefLabel "Barn"@en .

piirritev:OsmBuildingBoathouse a skos:Concept ;
    piirrite:osmId "boathouse" ;
    rdfs:subClassOf piirrite:OsmEntity ;
    skos:definition "A building for storing boats"@en ;
    skos:inScheme piirritev:OsmBuilding ;
    skos:prefLabel "Boathouse"@en .

piirritev:OsmBuildingBungalow a skos:Concept ;
    piirrite:osmId "bungalow" ;
    rdfs:subClassOf piirrite:OsmEntity ;
    skos:definition "Simple single-storey flat house."@en ;
    skos:inScheme piirritev:OsmBuilding ;
    skos:prefLabel "Bungalow"@en .

piirritev:OsmBuildingBunker a skos:Concept ;
    piirrite:hasRelatedOsmTag piirrite:hasOsmBunkerMilitary ;
    piirrite:osmId "bunker" ;
    rdfs:subClassOf piirrite:OsmEntity ;
    skos:definition "A hardened military building."@en ;
    skos:inScheme piirritev:OsmBuilding ;
    skos:prefLabel "Bunker"@en .

piirritev:OsmBuildingCabin a skos:Concept ;
    piirrite:osmId "cabin" ;
    rdfs:subClassOf piirrite:OsmEntity ;
    skos:definition "A small, roughly built house typically found in rural areas."@en ;
    skos:inScheme piirritev:OsmBuilding ;
    skos:prefLabel "Cabin"@en .

piirritev:OsmBuildingCarport a skos:Concept ;
    piirrite:hasRelatedOsmTag piirrite:hasOsmCarportCapacity,
        piirrite:hasOsmCarportHeight ;
    piirrite:osmId "carport" ;
    rdfs:subClassOf piirrite:OsmEntity ;
    skos:definition "A carport is a covered structure used to offer limited protection to vehicles, primarily cars, from the elements."@en ;
    skos:inScheme piirritev:OsmBuilding ;
    skos:prefLabel "Carport"@en .

piirritev:OsmBuildingChapel a skos:Concept ;
    piirrite:hasRelatedOsmTag piirrite:hasOsmChapelAmenity,
        piirrite:hasOsmChapelReligion ;
    piirrite:osmId "chapel" ;
    rdfs:subClassOf piirrite:OsmEntity ;
    skos:definition "Building built as chapel."@en ;
    skos:inScheme piirritev:OsmBuilding ;
    skos:prefLabel "Chapel"@en .

piirritev:OsmBuildingChurch a skos:Concept ;
    piirrite:hasRelatedOsmTag piirrite:hasOsmChurchAmenity,
        piirrite:hasOsmChurchName,
        piirrite:hasOsmChurchReligion ;
    piirrite:osmId "church" ;
    rdfs:subClassOf piirrite:OsmEntity ;
    skos:definition "A building that was built as a church.  osmcarto-rendering = File:Area building=yes.png  osmcarto-rendering-size = 100px"@en ;
    skos:inScheme piirritev:OsmBuilding ;
    skos:prefLabel "Church"@en .

piirritev:OsmBuildingCivic a skos:Concept ;
    piirrite:hasRelatedOsmTag piirrite:hasOsmCivicAmenity,
        piirrite:hasOsmCivicLeisure ;
    piirrite:osmId "civic" ;
    rdfs:subClassOf piirrite:OsmEntity ;
    skos:definition "A building originally built as civic building to hosting any civic amenity (town hall, library, swimming pool etc.)."@en ;
    skos:inScheme piirritev:OsmBuilding ;
    skos:prefLabel "Civic"@en .

piirritev:OsmBuildingCollapsed a skos:Concept ;
    piirrite:osmId "collapsed" ;
    rdfs:subClassOf piirrite:OsmEntity ;
    skos:definition "Using this tag is discouraged, use key:demolished:building or tag:building=ruins or delete object instead."@en ;
    skos:inScheme piirritev:OsmBuilding ;
    skos:prefLabel "Collapsed"@en .

piirritev:OsmBuildingCollege a skos:Concept ;
    piirrite:hasRelatedOsmTag piirrite:hasOsmCollegeAddr,
        piirrite:hasOsmCollegeName ;
    piirrite:osmId "college" ;
    rdfs:subClassOf piirrite:OsmEntity ;
    skos:definition "A building constructed to house a college."@en ;
    skos:inScheme piirritev:OsmBuilding ;
    skos:prefLabel "College"@en .

piirritev:OsmBuildingCommercial a skos:Concept ;
    piirrite:hasRelatedOsmTag piirrite:hasOsmCommercialOffice ;
    piirrite:osmId "commercial" ;
    rdfs:subClassOf piirrite:OsmEntity ;
    skos:definition "A building constructed for non-specific commercial activities to take place there."@en ;
    skos:inScheme piirritev:OsmBuilding ;
    skos:prefLabel "Commercial"@en .

piirritev:OsmBuildingConservatory a skos:Concept ;
    piirrite:hasRelatedOsmTag piirrite:hasOsmConservatoryAccess,
        piirrite:hasOsmConservatoryHeight,
        piirrite:hasOsmConservatoryOperator ;
    piirrite:osmId "conservatory" ;
    rdfs:subClassOf piirrite:OsmEntity ;
    skos:definition "Conservatory - a building or room having glass or tarpaulin roofing and walls used as an indoor garden or a sunroom (winter garden)."@en ;
    skos:inScheme piirritev:OsmBuilding ;
    skos:prefLabel "Conservatory"@en .

piirritev:OsmBuildingConstruction a skos:Concept ;
    piirrite:hasRelatedOsmTag piirrite:hasOsmConstructionType ;
    piirrite:osmId "construction" ;
    rdfs:subClassOf piirrite:OsmEntity ;
    skos:definition "A building under construction"@en ;
    skos:inScheme piirritev:OsmBuilding ;
    skos:prefLabel "Construction"@en .

piirritev:OsmBuildingContainer a skos:Concept ;
    piirrite:osmId "container" ;
    rdfs:subClassOf piirrite:OsmEntity ;
    skos:definition "A container used as a permanent building."@en ;
    skos:inScheme piirritev:OsmBuilding ;
    skos:prefLabel "Container"@en .

piirritev:OsmBuildingCowshed a skos:Concept ;
    piirrite:hasRelatedOsmTag piirrite:hasOsmCowshedLanduse ;
    piirrite:osmId "cowshed" ;
    rdfs:subClassOf piirrite:OsmEntity ;
    skos:definition "A building for housing cows."@en ;
    skos:inScheme piirritev:OsmBuilding ;
    skos:prefLabel "Cowshed"@en .

piirritev:OsmBuildingDetached a skos:Concept ;
    piirrite:osmId "detached" ;
    rdfs:subClassOf piirrite:OsmEntity ;
    skos:definition "A detached house: a free-standing residential building usually housing a single family."@en ;
    skos:inScheme piirritev:OsmBuilding ;
    skos:prefLabel "Detached"@en .

piirritev:OsmBuildingDigester a skos:Concept ;
    piirrite:hasRelatedOsmTag piirrite:hasOsmDigesterOperator,
        piirrite:hasOsmDigesterPower,
        piirrite:hasOsmDigesterRef ;
    piirrite:osmId "digester" ;
    rdfs:subClassOf piirrite:OsmEntity ;
    skos:definition "A building constructed as a digester, a bioreactor for the production of biogas from biomass."@en ;
    skos:inScheme piirritev:OsmBuilding ;
    skos:prefLabel "Digester"@en .

piirritev:OsmBuildingDormitory a skos:Concept ;
    piirrite:hasRelatedOsmTag piirrite:hasOsmDormitoryName,
        piirrite:hasOsmDormitoryOperator ;
    piirrite:osmId "dormitory" ;
    rdfs:subClassOf piirrite:OsmEntity ;
    skos:definition "Sleeping and living quarters provided by an institution."@en ;
    skos:inScheme piirritev:OsmBuilding ;
    skos:prefLabel "Dormitory"@en .

piirritev:OsmBuildingFarm a skos:Concept ;
    piirrite:hasRelatedOsmTag piirrite:hasOsmFarmName ;
    piirrite:osmId "farm" ;
    rdfs:subClassOf piirrite:OsmEntity ;
    skos:definition "A farmhouse is the main building of a farm"@en ;
    skos:inScheme piirritev:OsmBuilding ;
    skos:prefLabel "Farm"@en .

piirritev:OsmBuildingFarmAuxiliary a skos:Concept ;
    piirrite:hasRelatedOsmTag piirrite:hasOsmFarmAuxiliaryLanduse ;
    piirrite:osmId "farm_auxiliary" ;
    rdfs:subClassOf piirrite:OsmEntity ;
    skos:definition "A building on a farm that is not a dwelling."@en ;
    skos:inScheme piirritev:OsmBuilding ;
    skos:prefLabel "Farm auxiliary"@en .

piirritev:OsmBuildingFireStation a skos:Concept ;
    piirrite:hasRelatedOsmTag piirrite:hasOsmFireStationAmenity ;
    piirrite:osmId "fire_station" ;
    rdfs:subClassOf piirrite:OsmEntity ;
    skos:definition "A building constructed to house fire fighting equipment."@en ;
    skos:inScheme piirritev:OsmBuilding ;
    skos:prefLabel "Fire station"@en .

piirritev:OsmBuildingGarage a skos:Concept ;
    piirrite:hasRelatedOsmTag piirrite:hasOsmGarageLanduse ;
    piirrite:osmId "garage" ;
    rdfs:subClassOf piirrite:OsmEntity ;
    skos:definition "Denotes a single-owner private garage"@en ;
    skos:inScheme piirritev:OsmBuilding ;
    skos:prefLabel "Garage"@en .

piirritev:OsmBuildingGarages a skos:Concept ;
    piirrite:hasRelatedOsmTag piirrite:hasOsmGaragesAmenity,
        piirrite:hasOsmGaragesBuilding ;
    piirrite:osmId "garages" ;
    rdfs:subClassOf piirrite:OsmEntity ;
    skos:definition "A block of private garages each with a separate owner."@en ;
    skos:inScheme piirritev:OsmBuilding ;
    skos:prefLabel "Garages"@en .

piirritev:OsmBuildingGer a skos:Concept ;
    piirrite:osmId "ger" ;
    rdfs:subClassOf piirrite:OsmEntity ;
    skos:definition "A portable, round tent (yurt or ger)"@en ;
    skos:inScheme piirritev:OsmBuilding ;
    skos:prefLabel "Ger"@en .

piirritev:OsmBuildingGovernment a skos:Concept ;
    piirrite:osmId "government" ;
    rdfs:subClassOf piirrite:OsmEntity ;
    skos:definition "A building built to house government offices."@en ;
    skos:inScheme piirritev:OsmBuilding ;
    skos:prefLabel "Government"@en .

piirritev:OsmBuildingGrandstand a skos:Concept ;
    piirrite:osmId "grandstand" ;
    rdfs:subClassOf piirrite:OsmEntity ;
    skos:definition "A grandstand at racecourse or sports ground."@en ;
    skos:inScheme piirritev:OsmBuilding ;
    skos:prefLabel "Grandstand"@en .

piirritev:OsmBuildingGreenhouse a skos:Concept ;
    piirrite:osmId "greenhouse" ;
    rdfs:subClassOf piirrite:OsmEntity ;
    skos:definition "A building in which plants are grown"@en ;
    skos:inScheme piirritev:OsmBuilding ;
    skos:prefLabel "Greenhouse"@en .

piirritev:OsmBuildingHangar a skos:Concept ;
    piirrite:hasRelatedOsmTag piirrite:hasOsmHangarAeroway ;
    piirrite:osmId "hangar" ;
    rdfs:subClassOf piirrite:OsmEntity ;
    skos:definition "A building that was built as a hangar for the storage of aeroplanes, helicopters or space-craft."@en ;
    skos:inScheme piirritev:OsmBuilding ;
    skos:prefLabel "Hangar"@en .

piirritev:OsmBuildingHospital a skos:Concept ;
    piirrite:hasRelatedOsmTag piirrite:hasOsmHospitalAmenity ;
    piirrite:osmId "hospital" ;
    rdfs:subClassOf piirrite:OsmEntity ;
    skos:definition "A building which forms part of a hospital."@en ;
    skos:inScheme piirritev:OsmBuilding ;
    skos:prefLabel "Hospital"@en .

piirritev:OsmBuildingHotel a skos:Concept ;
    piirrite:osmId "hotel" ;
    rdfs:subClassOf piirrite:OsmEntity ;
    skos:definition "A building designed with separate rooms available for overnight accommodation."@en ;
    skos:inScheme piirritev:OsmBuilding ;
    skos:prefLabel "Hotel"@en .

piirritev:OsmBuildingHouse a skos:Concept ;
    piirrite:hasRelatedOsmTag piirrite:hasOsmHouseAddr ;
    piirrite:osmId "house" ;
    rdfs:subClassOf piirrite:OsmEntity ;
    skos:definition "A single dwelling unit usually inhabited by one family.  osmcarto-rendering = File:Area building=yes.png  osmcarto-rendering-size = 28px"@en ;
    skos:inScheme piirritev:OsmBuilding ;
    skos:prefLabel "House"@en .

piirritev:OsmBuildingHouseboat a skos:Concept ;
    piirrite:osmId "houseboat" ;
    rdfs:subClassOf piirrite:OsmEntity ;
    skos:definition "A boat (re)constructed as a floating home, staying at a single permanent location."@en ;
    skos:inScheme piirritev:OsmBuilding ;
    skos:prefLabel "Houseboat"@en .

piirritev:OsmBuildingHut a skos:Concept ;
    piirrite:osmId "hut" ;
    rdfs:subClassOf piirrite:OsmEntity ;
    skos:definition "A small and crude shelter."@en ;
    skos:inScheme piirritev:OsmBuilding ;
    skos:prefLabel "Hut"@en .

piirritev:OsmBuildingIndustrial a skos:Concept ;
    piirrite:hasRelatedOsmTag piirrite:hasOsmIndustrialType ;
    piirrite:osmId "industrial" ;
    rdfs:subClassOf piirrite:OsmEntity ;
    skos:definition "A building constructed to house some manufacturing process"@en ;
    skos:inScheme piirritev:OsmBuilding ;
    skos:prefLabel "Industrial"@en .

piirritev:OsmBuildingKindergarten a skos:Concept ;
    piirrite:hasRelatedOsmTag piirrite:hasOsmKindergartenAmenity,
        piirrite:hasOsmKindergartenName ;
    piirrite:osmId "kindergarten" ;
    rdfs:subClassOf piirrite:OsmEntity ;
    skos:definition "A generic kindergarten building."@en ;
    skos:inScheme piirritev:OsmBuilding ;
    skos:prefLabel "Kindergarten"@en .

piirritev:OsmBuildingKiosk a skos:Concept ;
    piirrite:hasRelatedOsmTag piirrite:hasOsmKioskShop ;
    piirrite:osmId "kiosk" ;
    rdfs:subClassOf piirrite:OsmEntity ;
    skos:definition "A small one room retail building, with clients not entering the building."@en ;
    skos:inScheme piirritev:OsmBuilding ;
    skos:prefLabel "Kiosk"@en .

piirritev:OsmBuildingManufacture a skos:Concept ;
    piirrite:osmId "manufacture" ;
    rdfs:subClassOf piirrite:OsmEntity ;
    skos:definition ""@en ;
    skos:inScheme piirritev:OsmBuilding ;
    skos:prefLabel "Manufacture"@en .

piirritev:OsmBuildingMosque a skos:Concept ;
    piirrite:hasRelatedOsmTag piirrite:hasOsmMosqueAmenity,
        piirrite:hasOsmMosqueName,
        piirrite:hasOsmMosqueOpeningHours,
        piirrite:hasOsmMosqueReligion,
        piirrite:hasOsmMosqueWebsite,
        piirrite:hasOsmMosqueWheelchair ;
    piirrite:osmId "mosque" ;
    rdfs:subClassOf piirrite:OsmEntity ;
    skos:definition "A building that was built as a mosque."@en ;
    skos:inScheme piirritev:OsmBuilding ;
    skos:prefLabel "Mosque"@en .

piirritev:OsmBuildingOffice a skos:Concept ;
    piirrite:osmId "office" ;
    rdfs:subClassOf piirrite:OsmEntity ;
    skos:definition "A building that was originally built as an office building which contains spaces mainly designed to be used for offices."@en ;
    skos:inScheme piirritev:OsmBuilding ;
    skos:prefLabel "Office"@en .

piirritev:OsmBuildingOutbuilding a skos:Concept ;
    piirrite:osmId "outbuilding" ;
    rdfs:subClassOf piirrite:OsmEntity ;
    skos:definition "A less important building near to and on the same piece of land as a larger building."@en ;
    skos:inScheme piirritev:OsmBuilding ;
    skos:prefLabel "Outbuilding"@en .

piirritev:OsmBuildingParking a skos:Concept ;
    piirrite:hasRelatedOsmTag piirrite:hasOsmParkingAmenity,
        piirrite:hasOsmParkingType ;
    piirrite:osmId "parking" ;
    rdfs:subClassOf piirrite:OsmEntity ;
    skos:definition "Structure purpose-built for parking cars."@en ;
    skos:inScheme piirritev:OsmBuilding ;
    skos:prefLabel "Parking"@en .

piirritev:OsmBuildingPavilion a skos:Concept ;
    piirrite:osmId "pavilion" ;
    rdfs:subClassOf piirrite:OsmEntity ;
    skos:definition "A building providing facilities for users of sports grounds"@en ;
    skos:inScheme piirritev:OsmBuilding ;
    skos:prefLabel "Pavilion"@en .

piirritev:OsmBuildingPublic a skos:Concept ;
    piirrite:hasRelatedOsmTag piirrite:hasOsmPublicAmenity,
        piirrite:hasOsmPublicLeisure ;
    piirrite:osmId "public" ;
    rdfs:subClassOf piirrite:OsmEntity ;
    skos:definition "A building constructed as accessible to the public (town hall, police station, court house)."@en ;
    skos:inScheme piirritev:OsmBuilding ;
    skos:prefLabel "Public"@en .

piirritev:OsmBuildingResidential a skos:Concept ;
    piirrite:osmId "residential" ;
    rdfs:subClassOf piirrite:OsmEntity ;
    skos:definition "A general tag for a building constructed primarily for residential purposes."@en ;
    skos:inScheme piirritev:OsmBuilding ;
    skos:prefLabel "Residential"@en .

piirritev:OsmBuildingRetail a skos:Concept ;
    piirrite:hasRelatedOsmTag piirrite:hasOsmRetailLanduse,
        piirrite:hasOsmRetailShop ;
    piirrite:osmId "retail" ;
    rdfs:subClassOf piirrite:OsmEntity ;
    skos:definition "A building that was originally built as a retail building for selling goods to the public."@en ;
    skos:inScheme piirritev:OsmBuilding ;
    skos:prefLabel "Retail"@en .

piirritev:OsmBuildingRoof a skos:Concept ;
    piirrite:hasRelatedOsmTag piirrite:hasOsmRoofLayer ;
    piirrite:osmId "roof" ;
    rdfs:subClassOf piirrite:OsmEntity ;
    skos:definition "A building open on at least two sides."@en ;
    skos:inScheme piirritev:OsmBuilding ;
    skos:prefLabel "Roof"@en .

piirritev:OsmBuildingRuins a skos:Concept ;
    piirrite:osmId "ruins" ;
    rdfs:subClassOf piirrite:OsmEntity ;
    skos:definition "Frequently used to mark ruined buildings. However, this usage conflicts with general use of building tag. In theory it should only be used for buildings constructed to look like ruins."@en ;
    skos:inScheme piirritev:OsmBuilding ;
    skos:prefLabel "Ruins"@en .

piirritev:OsmBuildingSchool a skos:Concept ;
    piirrite:osmId "school" ;
    rdfs:subClassOf piirrite:OsmEntity ;
    skos:definition "A building originally built as a school building."@en ;
    skos:inScheme piirritev:OsmBuilding ;
    skos:prefLabel "School"@en .

piirritev:OsmBuildingSemidetachedHouse a skos:Concept ;
    piirrite:osmId "semidetached_house" ;
    rdfs:subClassOf piirrite:OsmEntity ;
    skos:definition "A house that shares a common wall with another on one side."@en ;
    skos:inScheme piirritev:OsmBuilding ;
    skos:prefLabel "Semidetached house"@en .

piirritev:OsmBuildingService a skos:Concept ;
    piirrite:hasRelatedOsmTag piirrite:hasOsmServicePower,
        piirrite:hasOsmServiceSubstation,
        piirrite:hasOsmServiceTelecom,
        piirrite:hasOsmServiceUtility ;
    piirrite:osmId "service" ;
    rdfs:subClassOf piirrite:OsmEntity ;
    skos:definition "Service building usually is a small unmanned building with certain machinery (like pumps or transformers)."@en ;
    skos:inScheme piirritev:OsmBuilding ;
    skos:prefLabel "Service"@en .

piirritev:OsmBuildingShed a skos:Concept ;
    piirrite:osmId "shed" ;
    rdfs:subClassOf piirrite:OsmEntity ;
    skos:definition "A small, simple structure used as storage or workshop"@en ;
    skos:inScheme piirritev:OsmBuilding ;
    skos:prefLabel "Shed"@en .

piirritev:OsmBuildingSilo a skos:Concept ;
    piirrite:hasRelatedOsmTag piirrite:hasOsmSiloContent,
        piirrite:hasOsmSiloCrop,
        piirrite:hasOsmSiloHeight,
        piirrite:hasOsmSiloManMade,
        piirrite:hasOsmSiloOperator ;
    piirrite:osmId "silo" ;
    rdfs:subClassOf piirrite:OsmEntity ;
    skos:definition "A silo is a building for storing bulk materials."@en ;
    skos:inScheme piirritev:OsmBuilding ;
    skos:prefLabel "Silo"@en .

piirritev:OsmBuildingSlurryTank a skos:Concept ;
    piirrite:osmId "slurry_tank" ;
    rdfs:subClassOf piirrite:OsmEntity ;
    skos:definition "A cylindrical concrete structure holding liquid manure."@en ;
    skos:inScheme piirritev:OsmBuilding ;
    skos:prefLabel "Slurry tank"@en .

piirritev:OsmBuildingSportsCentre a skos:Concept ;
    piirrite:hasRelatedOsmTag piirrite:hasOsmSportsCentreSport ;
    piirrite:osmId "sports_centre" ;
    rdfs:subClassOf piirrite:OsmEntity ;
    skos:definition "A building that was built as a sports centre"@en ;
    skos:inScheme piirritev:OsmBuilding ;
    skos:prefLabel "Sports centre"@en .

piirritev:OsmBuildingSportsHall a skos:Concept ;
    piirrite:hasRelatedOsmTag piirrite:hasOsmSportsHallLeisure,
        piirrite:hasOsmSportsHallSport ;
    piirrite:osmId "sports_hall" ;
    rdfs:subClassOf piirrite:OsmEntity ;
    skos:definition "A building that was built as a sports hall"@en ;
    skos:inScheme piirritev:OsmBuilding ;
    skos:prefLabel "Sports hall"@en .

piirritev:OsmBuildingStable a skos:Concept ;
    piirrite:osmId "stable" ;
    rdfs:subClassOf piirrite:OsmEntity ;
    skos:definition "A building constructed as a stable for horses"@en ;
    skos:inScheme piirritev:OsmBuilding ;
    skos:prefLabel "Stable"@en .

piirritev:OsmBuildingStadium a skos:Concept ;
    piirrite:hasRelatedOsmTag piirrite:hasOsmStadiumLeisure,
        piirrite:hasOsmStadiumSport ;
    piirrite:osmId "stadium" ;
    rdfs:subClassOf piirrite:OsmEntity ;
    skos:definition "A building which was built as stadium."@en ;
    skos:inScheme piirritev:OsmBuilding ;
    skos:prefLabel "Stadium"@en .

piirritev:OsmBuildingStaticCaravan a skos:Concept ;
    piirrite:osmId "static_caravan" ;
    rdfs:subClassOf piirrite:OsmEntity ;
    skos:definition "A mobile home (caravan) (semi)permanently left on a single site."@en ;
    skos:inScheme piirritev:OsmBuilding ;
    skos:prefLabel "Static caravan"@en .

piirritev:OsmBuildingStiltHouse a skos:Concept ;
    piirrite:osmId "stilt_house" ;
    rdfs:subClassOf piirrite:OsmEntity ;
    skos:definition "A house raised on piles over the surface of the soil or a body of water."@en ;
    skos:inScheme piirritev:OsmBuilding ;
    skos:prefLabel "Stilt house"@en .

piirritev:OsmBuildingStorageTank a skos:Concept ;
    piirrite:hasRelatedOsmTag piirrite:hasOsmStorageTankCapacity,
        piirrite:hasOsmStorageTankContent,
        piirrite:hasOsmStorageTankHeight,
        piirrite:hasOsmStorageTankLocation,
        piirrite:hasOsmStorageTankManMade,
        piirrite:hasOsmStorageTankMaterial,
        piirrite:hasOsmStorageTankOperator ;
    piirrite:osmId "storage_tank" ;
    rdfs:subClassOf piirrite:OsmEntity ;
    skos:definition "A storage tank"@en ;
    skos:inScheme piirritev:OsmBuilding ;
    skos:prefLabel "Storage tank"@en .

piirritev:OsmBuildingSty a skos:Concept ;
    piirrite:hasRelatedOsmTag piirrite:hasOsmStyLanduse ;
    piirrite:osmId "sty" ;
    rdfs:subClassOf piirrite:OsmEntity ;
    skos:definition "A building for raising domestic pigs."@en ;
    skos:inScheme piirritev:OsmBuilding ;
    skos:prefLabel "Sty"@en .

piirritev:OsmBuildingSupermarket a skos:Concept ;
    piirrite:osmId "supermarket" ;
    rdfs:subClassOf piirrite:OsmEntity ;
    skos:definition "A building built as a supermarket"@en ;
    skos:inScheme piirritev:OsmBuilding ;
    skos:prefLabel "Supermarket"@en .

piirritev:OsmBuildingTemple a skos:Concept ;
    piirrite:hasRelatedOsmTag piirrite:hasOsmTempleAmenity,
        piirrite:hasOsmTempleReligion ;
    piirrite:osmId "temple" ;
    rdfs:subClassOf piirrite:OsmEntity ;
    skos:definition "A building that was built as a temple"@en ;
    skos:inScheme piirritev:OsmBuilding ;
    skos:prefLabel "Temple"@en .

piirritev:OsmBuildingTent a skos:Concept ;
    piirrite:hasRelatedOsmTag piirrite:hasOsmTentName,
        piirrite:hasOsmTentSeasonal ;
    piirrite:osmId "tent" ;
    rdfs:subClassOf piirrite:OsmEntity ;
    skos:definition "A building mainly consisting of sheets of fabric or similar"@en ;
    skos:inScheme piirritev:OsmBuilding ;
    skos:prefLabel "Tent"@en .

piirritev:OsmBuildingTerrace a skos:Concept ;
    piirrite:hasRelatedOsmTag piirrite:hasOsmTerraceBuilding,
        piirrite:hasOsmTerraceHouse ;
    piirrite:osmId "terrace" ;
    rdfs:subClassOf piirrite:OsmEntity ;
    skos:definition "The outline of a linear row of residential dwellings, each of which normally has its own entrance, which form a terrace (\"row-house\" or \"townhouse\" in North American English)."@en ;
    skos:inScheme piirritev:OsmBuilding ;
    skos:prefLabel "Terrace"@en .

piirritev:OsmBuildingToilets a skos:Concept ;
    piirrite:hasRelatedOsmTag piirrite:hasOsmToiletsAmenity,
        piirrite:hasOsmToiletsWheelchair ;
    piirrite:osmId "toilets" ;
    rdfs:subClassOf piirrite:OsmEntity ;
    skos:definition "A building designed for toilets."@en ;
    skos:inScheme piirritev:OsmBuilding ;
    skos:prefLabel "Toilets"@en .

piirritev:OsmBuildingTomb a skos:Concept ;
    piirrite:osmId "tomb" ;
    rdfs:subClassOf piirrite:OsmEntity ;
    skos:definition ""@en ;
    skos:inScheme piirritev:OsmBuilding ;
    skos:prefLabel "Tomb"@en .

piirritev:OsmBuildingTrainStation a skos:Concept ;
    piirrite:hasRelatedOsmTag piirrite:hasOsmTrainStationInternetAccess,
        piirrite:hasOsmTrainStationRailway ;
    piirrite:osmId "train_station" ;
    rdfs:subClassOf piirrite:OsmEntity ;
    skos:definition "A train station building osmcarto-rendering=File:Area amenity=place of worship.png osmcarto-rendering-size=28px"@en ;
    skos:inScheme piirritev:OsmBuilding ;
    skos:prefLabel "Train station"@en .

piirritev:OsmBuildingTransformerTower a skos:Concept ;
    piirrite:hasRelatedOsmTag piirrite:hasOsmTransformerTowerPower,
        piirrite:hasOsmTransformerTowerSubstation ;
    piirrite:osmId "transformer_tower" ;
    rdfs:subClassOf piirrite:OsmEntity ;
    skos:definition "A small but tall building constructed to comprise a transformer and connect to an overhead power line."@en ;
    skos:inScheme piirritev:OsmBuilding ;
    skos:prefLabel "Transformer tower"@en .

piirritev:OsmBuildingTransportation a skos:Concept ;
    piirrite:hasRelatedOsmTag piirrite:hasOsmTransportationPublicTransport ;
    piirrite:osmId "transportation" ;
    rdfs:subClassOf piirrite:OsmEntity ;
    skos:definition "A building related to the public transportation."@en ;
    skos:inScheme piirritev:OsmBuilding ;
    skos:prefLabel "Transportation"@en .

piirritev:OsmBuildingTrullo a skos:Concept ;
    piirrite:osmId "trullo" ;
    rdfs:subClassOf piirrite:OsmEntity ;
    skos:definition "A stone hut with a conical roof, built without mortar"@en ;
    skos:inScheme piirritev:OsmBuilding ;
    skos:prefLabel "Trullo"@en .

piirritev:OsmBuildingUniversity a skos:Concept ;
    piirrite:hasRelatedOsmTag piirrite:hasOsmUniversityName ;
    piirrite:osmId "university" ;
    rdfs:subClassOf piirrite:OsmEntity ;
    skos:definition "A university building."@en ;
    skos:inScheme piirritev:OsmBuilding ;
    skos:prefLabel "University"@en .

piirritev:OsmBuildingWarehouse a skos:Concept ;
    piirrite:osmId "warehouse" ;
    rdfs:subClassOf piirrite:OsmEntity ;
    skos:definition "A building that was originally built as a commercial building for storage of goods."@en ;
    skos:inScheme piirritev:OsmBuilding ;
    skos:prefLabel "Warehouse"@en .

piirritev:OsmBusDesignated a skos:Concept ;
    piirrite:hasRelatedOsmTag piirrite:hasOsmDesignatedHighway ;
    piirrite:osmId "designated" ;
    rdfs:subClassOf piirrite:OsmEntity ;
    skos:definition "Roads and other objects designated/signed to use for public transport buses."@en ;
    skos:inScheme piirritev:OsmBus ;
    skos:prefLabel "Designated"@en .

piirritev:OsmButtonOperated a skos:ConceptScheme ;
    piirrite:osmId "button_operated" ;
    skos:definition "Used to indicate that some functionality may be (or needs to be) activated by pressing a button."@en ;
    skos:prefLabel "Button operated, types"@en .

piirritev:OsmCables a skos:ConceptScheme ;
    piirrite:osmId "cables" ;
    skos:definition "Number of electrically separated, individual or bundled, power-carrying conductors in a power segment, section or circuit."@en ;
    skos:prefLabel "Cables, types"@en .

piirritev:OsmCapacity a skos:ConceptScheme ;
    piirrite:osmId "capacity" ;
    skos:definition "Describes the capacity a facility is suitable for."@en ;
    skos:prefLabel "Capacity, types"@en .

piirritev:OsmCemeteryGrave a skos:Concept ;
    piirrite:hasRelatedOsmTag piirrite:hasOsmGraveDescription,
        piirrite:hasOsmGraveInscription,
        piirrite:hasOsmGraveName,
        piirrite:hasOsmGraveSubject,
        piirrite:hasOsmGraveWikidata,
        piirrite:hasOsmGraveWikipedia ;
    piirrite:osmId "grave" ;
    rdfs:subClassOf piirrite:OsmEntity ;
    skos:definition "A place dug into the ground for the burial of a corpse, often marked with a gravestone."@en ;
    skos:inScheme piirritev:OsmCemetery ;
    skos:prefLabel "Grave"@en .

piirritev:OsmCemeterySector a skos:Concept ;
    piirrite:osmId "sector" ;
    rdfs:subClassOf piirrite:OsmEntity ;
    skos:definition "Cemetery sector (numbered/named part of the cemetery)"@en ;
    skos:inScheme piirritev:OsmCemetery ;
    skos:prefLabel "Sector"@en .

piirritev:OsmCheckDate a skos:ConceptScheme ;
    piirrite:osmId "check_date" ;
    skos:definition "Date of latest review of the data. Format: YYYY-MM-DD."@en ;
    skos:prefLabel "Check date, types"@en .

piirritev:OsmCircuits a skos:ConceptScheme ;
    piirrite:osmId "circuits" ;
    skos:definition "Number of electrical circuits in a power section, line, or cable."@en ;
    skos:prefLabel "Circuits, types"@en .

piirritev:OsmCircumference a skos:ConceptScheme ;
    piirrite:osmId "circumference" ;
    skos:definition "Circumference (in metres) of a tree's trunk at the height of 1.3 metre above ground."@en ;
    skos:prefLabel "Circumference, types"@en .

piirritev:OsmCollectionTimes a skos:ConceptScheme ;
    piirrite:osmId "collection_times" ;
    skos:definition "The collection times of a post box or recycling container"@en ;
    skos:prefLabel "Collection times, types"@en .

piirritev:OsmColourGrey a skos:Concept ;
    piirrite:osmId "grey" ;
    rdfs:subClassOf piirrite:OsmEntity ;
    skos:definition ""@en ;
    skos:inScheme piirritev:OsmColour ;
    skos:prefLabel "Grey"@en .

piirritev:OsmComment a skos:ConceptScheme ;
    piirrite:osmId "comment" ;
    skos:definition "group=annotations"@en ;
    skos:prefLabel "Comment, types"@en .

piirritev:OsmConditionDeficient a skos:Concept ;
    piirrite:osmId "deficient" ;
    rdfs:subClassOf piirrite:OsmEntity ;
    skos:definition ""@en ;
    skos:inScheme piirritev:OsmCondition ;
    skos:prefLabel "Deficient"@en .

piirritev:OsmConditionFair a skos:Concept ;
    piirrite:osmId "fair" ;
    rdfs:subClassOf piirrite:OsmEntity ;
    skos:definition ""@en ;
    skos:inScheme piirritev:OsmCondition ;
    skos:prefLabel "Fair"@en .

piirritev:OsmConditionGood a skos:Concept ;
    piirrite:osmId "good" ;
    rdfs:subClassOf piirrite:OsmEntity ;
    skos:definition ""@en ;
    skos:inScheme piirritev:OsmCondition ;
    skos:prefLabel "Good"@en .

piirritev:OsmConstructionApartments a skos:Concept ;
    piirrite:hasRelatedOsmTag piirrite:hasOsmApartmentsBuilding ;
    piirrite:osmId "apartments" ;
    rdfs:subClassOf piirrite:OsmEntity ;
    skos:definition "Used together with tag:building=construction to mark that a building under construction is a residential building used by multiple families/groups."@en ;
    skos:inScheme piirritev:OsmConstruction ;
    skos:prefLabel "Apartments"@en .

piirritev:OsmConstructionBuilding a skos:Concept ;
    piirrite:osmId "building" ;
    rdfs:subClassOf piirrite:OsmEntity ;
    skos:definition "Denotes that a construction site creates a building. May be deemed controversial."@en ;
    skos:inScheme piirritev:OsmConstruction ;
    skos:prefLabel "Building"@en .

piirritev:OsmConstructionDate a skos:ConceptScheme ;
    piirrite:osmId "construction_date" ;
    skos:definition "Indicates the date the construction of the feature was finished."@en ;
    skos:prefLabel "Construction date, types"@en .

piirritev:OsmConstructionFootway a skos:Concept ;
    piirrite:osmId "footway" ;
    rdfs:subClassOf piirrite:OsmEntity ;
    skos:definition ""@en ;
    skos:inScheme piirritev:OsmConstruction ;
    skos:prefLabel "Footway"@en .

piirritev:OsmConstructionHouse a skos:Concept ;
    piirrite:hasRelatedOsmTag piirrite:hasOsmHouseBuilding ;
    piirrite:osmId "house" ;
    rdfs:subClassOf piirrite:OsmEntity ;
    skos:definition "Used together with tag:building=construction to mark that building under construction is a house."@en ;
    skos:inScheme piirritev:OsmConstruction ;
    skos:prefLabel "House"@en .

piirritev:OsmConstructionMotorway a skos:Concept ;
    piirrite:osmId "motorway" ;
    rdfs:subClassOf piirrite:OsmEntity ;
    skos:definition ""@en ;
    skos:inScheme piirritev:OsmConstruction ;
    skos:prefLabel "Motorway"@en .

piirritev:OsmConstructionMotorwayLink a skos:Concept ;
    piirrite:osmId "motorway_link" ;
    rdfs:subClassOf piirrite:OsmEntity ;
    skos:definition ""@en ;
    skos:inScheme piirritev:OsmConstruction ;
    skos:prefLabel "Motorway link"@en .

piirritev:OsmConstructionPrimary a skos:Concept ;
    piirrite:osmId "primary" ;
    rdfs:subClassOf piirrite:OsmEntity ;
    skos:definition ""@en ;
    skos:inScheme piirritev:OsmConstruction ;
    skos:prefLabel "Primary"@en .

piirritev:OsmConstructionRail a skos:Concept ;
    piirrite:osmId "rail" ;
    rdfs:subClassOf piirrite:OsmEntity ;
    skos:definition ""@en ;
    skos:inScheme piirritev:OsmConstruction ;
    skos:prefLabel "Rail"@en .

piirritev:OsmConstructionResidential a skos:Concept ;
    piirrite:osmId "residential" ;
    rdfs:subClassOf piirrite:OsmEntity ;
    skos:definition ""@en ;
    skos:inScheme piirritev:OsmConstruction ;
    skos:prefLabel "Residential"@en .

piirritev:OsmConstructionSecondary a skos:Concept ;
    piirrite:osmId "secondary" ;
    rdfs:subClassOf piirrite:OsmEntity ;
    skos:definition ""@en ;
    skos:inScheme piirritev:OsmConstruction ;
    skos:prefLabel "Secondary"@en .

piirritev:OsmConstructionService a skos:Concept ;
    piirrite:osmId "service" ;
    rdfs:subClassOf piirrite:OsmEntity ;
    skos:definition ""@en ;
    skos:inScheme piirritev:OsmConstruction ;
    skos:prefLabel "Service"@en .

piirritev:OsmConstructionShed a skos:Concept ;
    piirrite:osmId "shed" ;
    rdfs:subClassOf piirrite:OsmEntity ;
    skos:definition "Specifies that building construction is about a shed construction"@en ;
    skos:inScheme piirritev:OsmConstruction ;
    skos:prefLabel "Shed"@en .

piirritev:OsmConstructionTertiary a skos:Concept ;
    piirrite:osmId "tertiary" ;
    rdfs:subClassOf piirrite:OsmEntity ;
    skos:definition ""@en ;
    skos:inScheme piirritev:OsmConstruction ;
    skos:prefLabel "Tertiary"@en .

piirritev:OsmConstructionTrunk a skos:Concept ;
    piirrite:osmId "trunk" ;
    rdfs:subClassOf piirrite:OsmEntity ;
    skos:definition ""@en ;
    skos:inScheme piirritev:OsmConstruction ;
    skos:prefLabel "Trunk"@en .

piirritev:OsmConstructionUnclassified a skos:Concept ;
    piirrite:osmId "unclassified" ;
    rdfs:subClassOf piirrite:OsmEntity ;
    skos:definition ""@en ;
    skos:inScheme piirritev:OsmConstruction ;
    skos:prefLabel "Unclassified"@en .

piirritev:OsmContentFuel a skos:Concept ;
    piirrite:hasRelatedOsmTag piirrite:hasOsmFuelManMade ;
    piirrite:osmId "fuel" ;
    rdfs:subClassOf piirrite:OsmEntity ;
    skos:definition "The content of a storage tank is fuel."@en ;
    skos:inScheme piirritev:OsmContent ;
    skos:prefLabel "Fuel"@en .

piirritev:OsmContentOil a skos:Concept ;
    piirrite:hasRelatedOsmTag piirrite:hasOsmOilManMade ;
    piirrite:osmId "oil" ;
    rdfs:subClassOf piirrite:OsmEntity ;
    skos:definition "The content of a storage tank is oil (mostly mineral oil or petroleum)."@en ;
    skos:inScheme piirritev:OsmContent ;
    skos:prefLabel "Oil"@en .

piirritev:OsmContentSilage a skos:Concept ;
    piirrite:hasRelatedOsmTag piirrite:hasOsmSilageManMade ;
    piirrite:osmId "silage" ;
    rdfs:subClassOf piirrite:OsmEntity ;
    skos:definition "The content of a storage tank is silage."@en ;
    skos:inScheme piirritev:OsmContent ;
    skos:prefLabel "Silage"@en .

piirritev:OsmContentSlurry a skos:Concept ;
    piirrite:hasRelatedOsmTag piirrite:hasOsmSlurryManMade ;
    piirrite:osmId "slurry" ;
    rdfs:subClassOf piirrite:OsmEntity ;
    skos:definition "A storage of liquid manure."@en ;
    skos:inScheme piirritev:OsmContent ;
    skos:prefLabel "Slurry"@en .

piirritev:OsmContentWater a skos:Concept ;
    piirrite:hasRelatedOsmTag piirrite:hasOsmWaterManMade ;
    piirrite:osmId "water" ;
    rdfs:subClassOf piirrite:OsmEntity ;
    skos:definition "The content of a storage tank is water"@en ;
    skos:inScheme piirritev:OsmContent ;
    skos:prefLabel "Water"@en .

piirritev:OsmCouplings a skos:ConceptScheme ;
    piirrite:osmId "couplings" ;
    skos:definition "For specifying the number of places on a fire hydrant or dry riser inlet where a hose can connect."@en ;
    skos:prefLabel "Couplings, types"@en .

piirritev:OsmCoveredBooth a skos:Concept ;
    piirrite:osmId "booth" ;
    rdfs:subClassOf piirrite:OsmEntity ;
    skos:definition ""@en ;
    skos:inScheme piirritev:OsmCovered ;
    skos:prefLabel "Booth"@en .

piirritev:OsmCraftBrewery a skos:Concept ;
    piirrite:hasRelatedOsmTag piirrite:hasOsmBreweryBuilding,
        piirrite:hasOsmBreweryMicrobrewery ;
    piirrite:osmId "brewery" ;
    rdfs:subClassOf piirrite:OsmEntity ;
    skos:definition "A dedicated building for the making of beer."@en ;
    skos:inScheme piirritev:OsmCraft ;
    skos:prefLabel "Brewery"@en .

piirritev:OsmCraftCarpenter a skos:Concept ;
    piirrite:hasRelatedOsmTag piirrite:hasOsmCarpenterName,
        piirrite:hasOsmCarpenterOpeningHours,
        piirrite:hasOsmCarpenterOperator,
        piirrite:hasOsmCarpenterType,
        piirrite:hasOsmCarpenterWebsite,
        piirrite:hasOsmCarpenterWheelchair ;
    piirrite:osmId "carpenter" ;
    rdfs:subClassOf piirrite:OsmEntity ;
    skos:definition "A workplace or office of carpenters that work with timber to construct, install and maintain buildings, furniture, and other objects."@en ;
    skos:inScheme piirritev:OsmCraft ;
    skos:prefLabel "Carpenter"@en .

piirritev:OsmCraftElectrician a skos:Concept ;
    piirrite:hasRelatedOsmTag piirrite:hasOsmElectricianName,
        piirrite:hasOsmElectricianOpeningHours,
        piirrite:hasOsmElectricianOperator ;
    piirrite:osmId "electrician" ;
    rdfs:subClassOf piirrite:OsmEntity ;
    skos:definition "A person or company that works with electricity or electrical systems."@en ;
    skos:inScheme piirritev:OsmCraft ;
    skos:prefLabel "Electrician"@en .

piirritev:OsmCraftElectronicsRepair a skos:Concept ;
    piirrite:hasRelatedOsmTag piirrite:hasOsmElectronicsRepairName,
        piirrite:hasOsmElectronicsRepairRepair ;
    piirrite:osmId "electronics_repair" ;
    rdfs:subClassOf piirrite:OsmEntity ;
    skos:definition "Repair shops and service centres which provides repair of computers, phones, appliance etc."@en ;
    skos:inScheme piirritev:OsmCraft ;
    skos:prefLabel "Electronics repair"@en .

piirritev:OsmCraftGrindingMill a skos:Concept ;
    piirrite:hasRelatedOsmTag piirrite:hasOsmGrindingMillName,
        piirrite:hasOsmGrindingMillOpeningHours,
        piirrite:hasOsmGrindingMillOperator,
        piirrite:hasOsmGrindingMillPhone,
        piirrite:hasOsmGrindingMillWebsite ;
    piirrite:osmId "grinding_mill" ;
    rdfs:subClassOf piirrite:OsmEntity ;
    skos:definition "A device that breaks solid materials into smaller pieces by grinding, crushing, or cutting. The aftermath is powdered product, not liquid extract like oil mill."@en ;
    skos:inScheme piirritev:OsmCraft ;
    skos:prefLabel "Grinding mill"@en .

piirritev:OsmCraftHvac a skos:Concept ;
    piirrite:osmId "hvac" ;
    rdfs:subClassOf piirrite:OsmEntity ;
    skos:definition "A workplace or office of a person or company that install and maintain HVAC systems (Heating, Ventilating, and Air Conditioning)."@en ;
    skos:inScheme piirritev:OsmCraft ;
    skos:prefLabel "Hvac"@en .

piirritev:OsmCraftMetalConstruction a skos:Concept ;
    piirrite:hasRelatedOsmTag piirrite:hasOsmMetalConstructionName,
        piirrite:hasOsmMetalConstructionOpeningHours,
        piirrite:hasOsmMetalConstructionOperator,
        piirrite:hasOsmMetalConstructionPhone,
        piirrite:hasOsmMetalConstructionWebsite,
        piirrite:hasOsmMetalConstructionWheelchair ;
    piirrite:osmId "metal_construction" ;
    rdfs:subClassOf piirrite:OsmEntity ;
    skos:definition "Workplace or office of a person who work with metal. This applies to: planning, construction, trade, repair."@en ;
    skos:inScheme piirritev:OsmCraft ;
    skos:prefLabel "Metal construction"@en .

piirritev:OsmCraftPhotographer a skos:Concept ;
    piirrite:hasRelatedOsmTag piirrite:hasOsmPhotographerName,
        piirrite:hasOsmPhotographerOpeningHours,
        piirrite:hasOsmPhotographerPhone,
        piirrite:hasOsmPhotographerWebsite,
        piirrite:hasOsmPhotographerWheelchair ;
    piirrite:osmId "photographer" ;
    rdfs:subClassOf piirrite:OsmEntity ;
    skos:definition "A workplace or office of a person who takes photographs using a camera."@en ;
    skos:inScheme piirritev:OsmCraft ;
    skos:prefLabel "Photographer"@en .

piirritev:OsmCraftPlumber a skos:Concept ;
    piirrite:hasRelatedOsmTag piirrite:hasOsmPlumberName,
        piirrite:hasOsmPlumberOpeningHours,
        piirrite:hasOsmPlumberOperator,
        piirrite:hasOsmPlumberWebsite,
        piirrite:hasOsmPlumberWheelchair ;
    piirrite:osmId "plumber" ;
    rdfs:subClassOf piirrite:OsmEntity ;
    skos:definition "A workplace or office of a skilled tradesperson who specializes in (drinking) water supply, sewage and drainage systems."@en ;
    skos:inScheme piirritev:OsmCraft ;
    skos:prefLabel "Plumber"@en .

piirritev:OsmCraftShoemaker a skos:Concept ;
    piirrite:osmId "shoemaker" ;
    rdfs:subClassOf piirrite:OsmEntity ;
    skos:definition "A place where shoes, boots, sandals, clogs and moccasins are created, repaired or altered to fit personal needs."@en ;
    skos:inScheme piirritev:OsmCraft ;
    skos:prefLabel "Shoemaker"@en .

piirritev:OsmCraftTailor a skos:Concept ;
    piirrite:hasRelatedOsmTag piirrite:hasOsmTailorCraft,
        piirrite:hasOsmTailorOpeningHours,
        piirrite:hasOsmTailorOperator,
        piirrite:hasOsmTailorPhone,
        piirrite:hasOsmTailorShop,
        piirrite:hasOsmTailorWebsite ;
    piirrite:osmId "tailor" ;
    rdfs:subClassOf piirrite:OsmEntity ;
    skos:definition "A place where clothing is made, repaired, or altered professionally, especially suits and men's clothing."@en ;
    skos:inScheme piirritev:OsmCraft ;
    skos:prefLabel "Tailor"@en .

piirritev:OsmCraftWinery a skos:Concept ;
    piirrite:hasRelatedOsmTag piirrite:hasOsmWineryBrand,
        piirrite:hasOsmWineryDrink,
        piirrite:hasOsmWineryEmail,
        piirrite:hasOsmWineryName,
        piirrite:hasOsmWineryOpeningHours,
        piirrite:hasOsmWineryOperator,
        piirrite:hasOsmWineryPhone,
        piirrite:hasOsmWineryWebsite,
        piirrite:hasOsmWineryWheelchair ;
    piirrite:osmId "winery" ;
    rdfs:subClassOf piirrite:OsmEntity ;
    skos:definition "A place where wine is produced"@en ;
    skos:inScheme piirritev:OsmCraft ;
    skos:prefLabel "Winery"@en .

piirritev:OsmCreatedByAlmienCoastlines a skos:Concept ;
    piirrite:osmId "almien_coastlines" ;
    rdfs:subClassOf piirrite:OsmEntity ;
    skos:definition ""@en ;
    skos:inScheme piirritev:OsmCreatedBy ;
    skos:prefLabel "Almien coastlines"@en .

piirritev:OsmCreatedByArcgisExporter a skos:Concept ;
    piirrite:osmId "ArcGIS_Exporter" ;
    rdfs:subClassOf piirrite:OsmEntity ;
    skos:definition ""@en ;
    skos:inScheme piirritev:OsmCreatedBy ;
    skos:prefLabel "Arcgis exporter"@en .

piirritev:OsmCreatedByCoastbot a skos:Concept ;
    piirrite:osmId "coastbot" ;
    rdfs:subClassOf piirrite:OsmEntity ;
    skos:definition ""@en ;
    skos:inScheme piirritev:OsmCreatedBy ;
    skos:prefLabel "Coastbot"@en .

piirritev:OsmCreatedByDmgroomCoastlines a skos:Concept ;
    piirrite:osmId "dmgroom_coastlines" ;
    rdfs:subClassOf piirrite:OsmEntity ;
    skos:definition ""@en ;
    skos:inScheme piirritev:OsmCreatedBy ;
    skos:prefLabel "Dmgroom coastlines"@en .

piirritev:OsmCreatedByEditop a skos:Concept ;
    piirrite:osmId "Editop" ;
    rdfs:subClassOf piirrite:OsmEntity ;
    skos:definition ""@en ;
    skos:inScheme piirritev:OsmCreatedBy ;
    skos:prefLabel "Editop"@en .

piirritev:OsmCreatedByGeobasenhn2Osm a skos:Concept ;
    piirrite:osmId "geobaseNHN2osm" ;
    rdfs:subClassOf piirrite:OsmEntity ;
    skos:definition ""@en ;
    skos:inScheme piirritev:OsmCreatedBy ;
    skos:prefLabel "Geobasenhn2osm"@en .

piirritev:OsmCreatedByGpsbabel-135 a skos:Concept ;
    piirrite:osmId "GPSBabel-1_3_5" ;
    rdfs:subClassOf piirrite:OsmEntity ;
    skos:definition ""@en ;
    skos:inScheme piirritev:OsmCreatedBy ;
    skos:prefLabel "Gpsbabel-1 3 5"@en .

piirritev:OsmCreatedByGpsbabel-136 a skos:Concept ;
    piirrite:osmId "GPSBabel-1_3_6" ;
    rdfs:subClassOf piirrite:OsmEntity ;
    skos:definition ""@en ;
    skos:inScheme piirritev:OsmCreatedBy ;
    skos:prefLabel "Gpsbabel-1 3 6"@en .

piirritev:OsmCreatedByJosm a skos:Concept ;
    piirrite:osmId "JOSM" ;
    rdfs:subClassOf piirrite:OsmEntity ;
    skos:definition ""@en ;
    skos:inScheme piirritev:OsmCreatedBy ;
    skos:prefLabel "Josm"@en .

piirritev:OsmCreatedByMerkaartor011 a skos:Concept ;
    piirrite:osmId "Merkaartor_0_11" ;
    rdfs:subClassOf piirrite:OsmEntity ;
    skos:definition ""@en ;
    skos:inScheme piirritev:OsmCreatedBy ;
    skos:prefLabel "Merkaartor 0 11"@en .

piirritev:OsmCreatedByMerkaartor012 a skos:Concept ;
    piirrite:osmId "Merkaartor_0_12" ;
    rdfs:subClassOf piirrite:OsmEntity ;
    skos:definition ""@en ;
    skos:inScheme piirritev:OsmCreatedBy ;
    skos:prefLabel "Merkaartor 0 12"@en .

piirritev:OsmCreatedByMerkaartor013 a skos:Concept ;
    piirrite:osmId "Merkaartor_0_13" ;
    rdfs:subClassOf piirrite:OsmEntity ;
    skos:definition ""@en ;
    skos:inScheme piirritev:OsmCreatedBy ;
    skos:prefLabel "Merkaartor 0 13"@en .

piirritev:OsmCreatedByPolyshp2Osm a skos:Concept ;
    piirrite:osmId "polyshp2osm" ;
    rdfs:subClassOf piirrite:OsmEntity ;
    skos:definition ""@en ;
    skos:inScheme piirritev:OsmCreatedBy ;
    skos:prefLabel "Polyshp2osm"@en .

piirritev:OsmCreatedByPotlatch010B a skos:Concept ;
    piirrite:osmId "Potlatch_0_10b" ;
    rdfs:subClassOf piirrite:OsmEntity ;
    skos:definition ""@en ;
    skos:inScheme piirritev:OsmCreatedBy ;
    skos:prefLabel "Potlatch 0 10b"@en .

piirritev:OsmCreatedByPotlatch010F a skos:Concept ;
    piirrite:osmId "Potlatch_0_10f" ;
    rdfs:subClassOf piirrite:OsmEntity ;
    skos:definition ""@en ;
    skos:inScheme piirritev:OsmCreatedBy ;
    skos:prefLabel "Potlatch 0 10f"@en .

piirritev:OsmCreatedByPotlatch09C a skos:Concept ;
    piirrite:osmId "Potlatch_0_9c" ;
    rdfs:subClassOf piirrite:OsmEntity ;
    skos:definition ""@en ;
    skos:inScheme piirritev:OsmCreatedBy ;
    skos:prefLabel "Potlatch 0 9c"@en .

piirritev:OsmCreatedByShp2Osm a skos:Concept ;
    piirrite:osmId "shp2osm" ;
    rdfs:subClassOf piirrite:OsmEntity ;
    skos:definition ""@en ;
    skos:inScheme piirritev:OsmCreatedBy ;
    skos:prefLabel "Shp2osm"@en .

piirritev:OsmCreatedByShpupload a skos:Concept ;
    piirrite:osmId "shpupload" ;
    rdfs:subClassOf piirrite:OsmEntity ;
    skos:definition ""@en ;
    skos:inScheme piirritev:OsmCreatedBy ;
    skos:prefLabel "Shpupload"@en .

piirritev:OsmCreatedByYahooapplet10 a skos:Concept ;
    piirrite:osmId "YahooApplet_1_0" ;
    rdfs:subClassOf piirrite:OsmEntity ;
    skos:definition ""@en ;
    skos:inScheme piirritev:OsmCreatedBy ;
    skos:prefLabel "Yahooapplet 1 0"@en .

piirritev:OsmCropCereal a skos:Concept ;
    piirrite:osmId "cereal" ;
    rdfs:subClassOf piirrite:OsmEntity ;
    skos:definition "Unspecified cereal crop fieldimage=File:Cereal_field_at_Sutton_Courtney_-_geograph.org.uk_-_1348877.jpg"@en ;
    skos:inScheme piirritev:OsmCrop ;
    skos:prefLabel "Cereal"@en .

piirritev:OsmCropCorn a skos:Concept ;
    piirrite:osmId "corn" ;
    rdfs:subClassOf piirrite:OsmEntity ;
    skos:definition ""@en ;
    skos:inScheme piirritev:OsmCrop ;
    skos:prefLabel "Corn"@en .

piirritev:OsmCropGrape a skos:Concept ;
    piirrite:osmId "grape" ;
    rdfs:subClassOf piirrite:OsmEntity ;
    skos:definition "Specifies that grapes are grown here."@en ;
    skos:inScheme piirritev:OsmCrop ;
    skos:prefLabel "Grape"@en .

piirritev:OsmCropGrass a skos:Concept ;
    piirrite:osmId "grass" ;
    rdfs:subClassOf piirrite:OsmEntity ;
    skos:definition "Unspecified grass crop."@en ;
    skos:inScheme piirritev:OsmCrop ;
    skos:prefLabel "Grass"@en .

piirritev:OsmCropHop a skos:Concept ;
    piirrite:hasRelatedOsmTag piirrite:hasOsmHopLanduse ;
    piirrite:osmId "hop" ;
    rdfs:subClassOf piirrite:OsmEntity ;
    skos:definition "Specifies that an area of farmland is being used to grow hops."@en ;
    skos:inScheme piirritev:OsmCrop ;
    skos:prefLabel "Hop"@en .

piirritev:OsmCropMarketGardening a skos:Concept ;
    piirrite:osmId "market_gardening" ;
    rdfs:subClassOf piirrite:OsmEntity ;
    skos:definition ""@en ;
    skos:inScheme piirritev:OsmCrop ;
    skos:prefLabel "Market gardening"@en .

piirritev:OsmCropRice a skos:Concept ;
    piirrite:hasRelatedOsmTag piirrite:hasOsmRiceLanduse ;
    piirrite:osmId "rice" ;
    rdfs:subClassOf piirrite:OsmEntity ;
    skos:definition "Specifies that an area of farmland is being used to grow rice."@en ;
    skos:inScheme piirritev:OsmCrop ;
    skos:prefLabel "Rice"@en .

piirritev:OsmCropSugarcane a skos:Concept ;
    piirrite:osmId "sugarcane" ;
    rdfs:subClassOf piirrite:OsmEntity ;
    skos:definition "Specifies that an area of farmland is being used to grow sugarcane"@en ;
    skos:inScheme piirritev:OsmCrop ;
    skos:prefLabel "Sugarcane"@en .

piirritev:OsmCropTea a skos:Concept ;
    piirrite:hasRelatedOsmTag piirrite:hasOsmTeaLanduse ;
    piirrite:osmId "tea" ;
    rdfs:subClassOf piirrite:OsmEntity ;
    skos:definition "Specifies that an agricultural feature produces tea leaves."@en ;
    skos:inScheme piirritev:OsmCrop ;
    skos:prefLabel "Tea"@en .

piirritev:OsmCropWheat a skos:Concept ;
    piirrite:osmId "wheat" ;
    rdfs:subClassOf piirrite:OsmEntity ;
    skos:definition "Specifies that an area of farmland is being used to grow wheat."@en ;
    skos:inScheme piirritev:OsmCrop ;
    skos:prefLabel "Wheat"@en .

piirritev:OsmCrossingInformal a skos:Concept ;
    piirrite:osmId "informal" ;
    rdfs:subClassOf piirrite:OsmEntity ;
    skos:definition "Unmarked place where pedestrians are most likely to want to cross the street exactly there"@en ;
    skos:inScheme piirritev:OsmCrossing ;
    skos:prefLabel "Informal"@en .

piirritev:OsmCrossingMarked a skos:Concept ;
    piirrite:hasRelatedOsmTag piirrite:hasOsmMarkedBicycle,
        piirrite:hasOsmMarkedCrossingRef,
        piirrite:hasOsmMarkedCycleway,
        piirrite:hasOsmMarkedFootway,
        piirrite:hasOsmMarkedHighway,
        piirrite:hasOsmMarkedKerb,
        piirrite:hasOsmMarkedLit,
        piirrite:hasOsmMarkedRailway,
        piirrite:hasOsmMarkedTactilePaving,
        piirrite:hasOsmMarkedWheelchair ;
    piirrite:osmId "marked" ;
    rdfs:subClassOf piirrite:OsmEntity ;
    skos:definition "A generic crossing with no traffic-signals of any type, just road markings."@en ;
    skos:inScheme piirritev:OsmCrossing ;
    skos:prefLabel "Marked"@en .

piirritev:OsmCrossingRefPelican a skos:Concept ;
    piirrite:hasRelatedOsmTag piirrite:hasOsmPelicanButtonOperated,
        piirrite:hasOsmPelicanTactilePaving ;
    piirrite:osmId "pelican" ;
    rdfs:subClassOf piirrite:OsmEntity ;
    skos:definition "Pelican pedestrian crossings."@en ;
    skos:inScheme piirritev:OsmCrossingRef ;
    skos:prefLabel "Pelican"@en .

piirritev:OsmCrossingRefToucan a skos:Concept ;
    piirrite:osmId "toucan" ;
    rdfs:subClassOf piirrite:OsmEntity ;
    skos:definition ""@en ;
    skos:inScheme piirritev:OsmCrossingRef ;
    skos:prefLabel "Toucan"@en .

piirritev:OsmCrossingRefZebra a skos:Concept ;
    piirrite:hasRelatedOsmTag piirrite:hasOsmZebraCrossing,
        piirrite:hasOsmZebraKerb,
        piirrite:hasOsmZebraLit,
        piirrite:hasOsmZebraSupervised,
        piirrite:hasOsmZebraTactilePaving,
        piirrite:hasOsmZebraWheelchair ;
    piirrite:osmId "zebra" ;
    rdfs:subClassOf piirrite:OsmEntity ;
    skos:definition "A legal zebra crossing."@en ;
    skos:inScheme piirritev:OsmCrossingRef ;
    skos:prefLabel "Zebra"@en .

piirritev:OsmCrossingTrafficSignals a skos:Concept ;
    piirrite:hasRelatedOsmTag piirrite:hasOsmTrafficSignalsCycleway,
        piirrite:hasOsmTrafficSignalsFootway,
        piirrite:hasOsmTrafficSignalsHighway ;
    piirrite:osmId "traffic_signals" ;
    rdfs:subClassOf piirrite:OsmEntity ;
    skos:definition "Traffic light controlled pedestrian crossings."@en ;
    skos:inScheme piirritev:OsmCrossing ;
    skos:prefLabel "Traffic signals"@en .

piirritev:OsmCrossingUncontrolled a skos:Concept ;
    piirrite:osmId "uncontrolled" ;
    rdfs:subClassOf piirrite:OsmEntity ;
    skos:definition "A generic crossing with road markings, but no traffic-signals of any type."@en ;
    skos:inScheme piirritev:OsmCrossing ;
    skos:prefLabel "Uncontrolled"@en .

piirritev:OsmCrossingUnmarked a skos:Concept ;
    piirrite:hasRelatedOsmTag piirrite:hasOsmUnmarkedCycleway,
        piirrite:hasOsmUnmarkedFootway,
        piirrite:hasOsmUnmarkedHighway,
        piirrite:hasOsmUnmarkedKerb,
        piirrite:hasOsmUnmarkedRailway,
        piirrite:hasOsmUnmarkedTactilePaving,
        piirrite:hasOsmUnmarkedTrafficCalming,
        piirrite:hasOsmUnmarkedWheelchair ;
    piirrite:osmId "unmarked" ;
    rdfs:subClassOf piirrite:OsmEntity ;
    skos:definition "Pedestrian crossings without road markings or traffic signals."@en ;
    skos:inScheme piirritev:OsmCrossing ;
    skos:prefLabel "Unmarked"@en .

piirritev:OsmCrossingZebra a skos:Concept ;
    piirrite:osmId "zebra" ;
    rdfs:subClassOf piirrite:OsmEntity ;
    skos:definition ""@en ;
    skos:inScheme piirritev:OsmCrossing ;
    skos:prefLabel "Zebra"@en .

piirritev:OsmDelivery a skos:ConceptScheme ;
    piirrite:osmId "delivery" ;
    skos:definition "Sets whether the restaurant or shop offers delivery service."@en ;
    skos:prefLabel "Delivery, types"@en .

piirritev:OsmDenominationAnglican a skos:Concept ;
    piirrite:osmId "anglican" ;
    rdfs:subClassOf piirrite:OsmEntity ;
    skos:definition ""@en ;
    skos:inScheme piirritev:OsmDenomination ;
    skos:prefLabel "Anglican"@en .

piirritev:OsmDenominationBaptist a skos:Concept ;
    piirrite:osmId "baptist" ;
    rdfs:subClassOf piirrite:OsmEntity ;
    skos:definition ""@en ;
    skos:inScheme piirritev:OsmDenomination ;
    skos:prefLabel "Baptist"@en .

piirritev:OsmDenominationCatholic a skos:Concept ;
    piirrite:hasRelatedOsmTag piirrite:hasOsmCatholicAmenity,
        piirrite:hasOsmCatholicLanduse ;
    piirrite:osmId "catholic" ;
    rdfs:subClassOf piirrite:OsmEntity ;
    skos:definition "Unspecified Catholic denomination."@en ;
    skos:inScheme piirritev:OsmDenomination ;
    skos:prefLabel "Catholic"@en .

piirritev:OsmDenominationEvangelical a skos:Concept ;
    piirrite:osmId "evangelical" ;
    rdfs:subClassOf piirrite:OsmEntity ;
    skos:definition ""@en ;
    skos:inScheme piirritev:OsmDenomination ;
    skos:prefLabel "Evangelical"@en .

piirritev:OsmDenominationGreekOrthodox a skos:Concept ;
    piirrite:osmId "greek_orthodox" ;
    rdfs:subClassOf piirrite:OsmEntity ;
    skos:definition ""@en ;
    skos:inScheme piirritev:OsmDenomination ;
    skos:prefLabel "Greek orthodox"@en .

piirritev:OsmDenominationJehovahsWitness a skos:Concept ;
    piirrite:hasRelatedOsmTag piirrite:hasOsmJehovahsWitnessAmenity,
        piirrite:hasOsmJehovahsWitnessBuilding ;
    piirrite:osmId "jehovahs_witness" ;
    rdfs:subClassOf piirrite:OsmEntity ;
    skos:definition "Meeting place where Jehovah's Witnesses hold religious services."@en ;
    skos:inScheme piirritev:OsmDenomination ;
    skos:prefLabel "Jehovahs witness"@en .

piirritev:OsmDenominationLutheran a skos:Concept ;
    piirrite:osmId "lutheran" ;
    rdfs:subClassOf piirrite:OsmEntity ;
    skos:definition ""@en ;
    skos:inScheme piirritev:OsmDenomination ;
    skos:prefLabel "Lutheran"@en .

piirritev:OsmDenominationMethodist a skos:Concept ;
    piirrite:osmId "methodist" ;
    rdfs:subClassOf piirrite:OsmEntity ;
    skos:definition ""@en ;
    skos:inScheme piirritev:OsmDenomination ;
    skos:prefLabel "Methodist"@en .

piirritev:OsmDenominationOrthodox a skos:Concept ;
    piirrite:osmId "orthodox" ;
    rdfs:subClassOf piirrite:OsmEntity ;
    skos:definition ""@en ;
    skos:inScheme piirritev:OsmDenomination ;
    skos:prefLabel "Orthodox"@en .

piirritev:OsmDenominationPentecostal a skos:Concept ;
    piirrite:osmId "pentecostal" ;
    rdfs:subClassOf piirrite:OsmEntity ;
    skos:definition ""@en ;
    skos:inScheme piirritev:OsmDenomination ;
    skos:prefLabel "Pentecostal"@en .

piirritev:OsmDenominationPresbyterian a skos:Concept ;
    piirrite:osmId "presbyterian" ;
    rdfs:subClassOf piirrite:OsmEntity ;
    skos:definition ""@en ;
    skos:inScheme piirritev:OsmDenomination ;
    skos:prefLabel "Presbyterian"@en .

piirritev:OsmDenominationProtestant a skos:Concept ;
    piirrite:osmId "protestant" ;
    rdfs:subClassOf piirrite:OsmEntity ;
    skos:definition ""@en ;
    skos:inScheme piirritev:OsmDenomination ;
    skos:prefLabel "Protestant"@en .

piirritev:OsmDenominationRomanCatholic a skos:Concept ;
    piirrite:osmId "roman_catholic" ;
    rdfs:subClassOf piirrite:OsmEntity ;
    skos:definition ""@en ;
    skos:inScheme piirritev:OsmDenomination ;
    skos:prefLabel "Roman catholic"@en .

piirritev:OsmDenominationRussianOrthodox a skos:Concept ;
    piirrite:osmId "russian_orthodox" ;
    rdfs:subClassOf piirrite:OsmEntity ;
    skos:definition ""@en ;
    skos:inScheme piirritev:OsmDenomination ;
    skos:prefLabel "Russian orthodox"@en .

piirritev:OsmDenominationSunni a skos:Concept ;
    piirrite:osmId "sunni" ;
    rdfs:subClassOf piirrite:OsmEntity ;
    skos:definition ""@en ;
    skos:inScheme piirritev:OsmDenomination ;
    skos:prefLabel "Sunni"@en .

piirritev:OsmDenominationTheravada a skos:Concept ;
    piirrite:osmId "theravada" ;
    rdfs:subClassOf piirrite:OsmEntity ;
    skos:definition ""@en ;
    skos:inScheme piirritev:OsmDenomination ;
    skos:prefLabel "Theravada"@en .

piirritev:OsmDenotationAgricultural a skos:Concept ;
    piirrite:hasRelatedOsmTag piirrite:hasOsmAgriculturalCrop,
        piirrite:hasOsmAgriculturalProduce,
        piirrite:hasOsmAgriculturalSpecies,
        piirrite:hasOsmAgriculturalTrees ;
    piirrite:osmId "agricultural" ;
    rdfs:subClassOf piirrite:OsmEntity ;
    skos:definition "A tree in agricultural use"@en ;
    skos:inScheme piirritev:OsmDenotation ;
    skos:prefLabel "Agricultural"@en .

piirritev:OsmDenotationAvenue a skos:Concept ;
    piirrite:osmId "avenue" ;
    rdfs:subClassOf piirrite:OsmEntity ;
    skos:definition "A tree aligned along a road."@en ;
    skos:inScheme piirritev:OsmDenotation ;
    skos:prefLabel "Avenue"@en .

piirritev:OsmDenotationDecoration a skos:Concept ;
    piirrite:osmId "decoration" ;
    rdfs:subClassOf piirrite:OsmEntity ;
    skos:definition ""@en ;
    skos:inScheme piirritev:OsmDenotation ;
    skos:prefLabel "Decoration"@en .

piirritev:OsmDenotationGarden a skos:Concept ;
    piirrite:osmId "garden" ;
    rdfs:subClassOf piirrite:OsmEntity ;
    skos:definition "A tree located within a garden."@en ;
    skos:inScheme piirritev:OsmDenotation ;
    skos:prefLabel "Garden"@en .

piirritev:OsmDenotationLandmark a skos:Concept ;
    piirrite:osmId "landmark" ;
    rdfs:subClassOf piirrite:OsmEntity ;
    skos:definition "A tree or other feature remarkable due to its size or prominent location, usually visible from great distances and useful for navigation."@en ;
    skos:inScheme piirritev:OsmDenotation ;
    skos:prefLabel "Landmark"@en .

piirritev:OsmDenotationNaturalMonument a skos:Concept ;
    piirrite:osmId "natural_monument" ;
    rdfs:subClassOf piirrite:OsmEntity ;
    skos:definition "An especially old tree, often with a particular shape and usually protected for its uniqueness."@en ;
    skos:inScheme piirritev:OsmDenotation ;
    skos:prefLabel "Natural monument"@en .

piirritev:OsmDenotationPark a skos:Concept ;
    piirrite:osmId "park" ;
    rdfs:subClassOf piirrite:OsmEntity ;
    skos:definition "A tree located within an urban park."@en ;
    skos:inScheme piirritev:OsmDenotation ;
    skos:prefLabel "Park"@en .

piirritev:OsmDenotationSingle a skos:Concept ;
    piirrite:osmId "single" ;
    rdfs:subClassOf piirrite:OsmEntity ;
    skos:definition ""@en ;
    skos:inScheme piirritev:OsmDenotation ;
    skos:prefLabel "Single"@en .

piirritev:OsmDenotationStreet a skos:Concept ;
    piirrite:osmId "street" ;
    rdfs:subClassOf piirrite:OsmEntity ;
    skos:definition ""@en ;
    skos:inScheme piirritev:OsmDenotation ;
    skos:prefLabel "Street"@en .

piirritev:OsmDenotationUrban a skos:Concept ;
    piirrite:osmId "urban" ;
    rdfs:subClassOf piirrite:OsmEntity ;
    skos:definition "An \"urban\" tree, usually found within settlements, e.g. in parks or spread through residential areas."@en ;
    skos:inScheme piirritev:OsmDenotation ;
    skos:prefLabel "Urban"@en .

piirritev:OsmDeparturesBoardRealtime a skos:Concept ;
    piirrite:osmId "realtime" ;
    rdfs:subClassOf piirrite:OsmEntity ;
    skos:definition ""@en ;
    skos:inScheme piirritev:OsmDeparturesBoard ;
    skos:prefLabel "Realtime"@en .

piirritev:OsmDeparturesBoardTimetable a skos:Concept ;
    piirrite:osmId "timetable" ;
    rdfs:subClassOf piirrite:OsmEntity ;
    skos:definition ""@en ;
    skos:inScheme piirritev:OsmDeparturesBoard ;
    skos:prefLabel "Timetable"@en .

piirritev:OsmDepth a skos:ConceptScheme ;
    piirrite:osmId "depth" ;
    skos:definition "The depth of a feature, in metres."@en ;
    skos:prefLabel "Depth, types"@en .

piirritev:OsmDescriptionAnnexe a skos:Concept ;
    piirrite:osmId "Annexe" ;
    rdfs:subClassOf piirrite:OsmEntity ;
    skos:definition ""@en ;
    skos:inScheme piirritev:OsmDescription ;
    skos:prefLabel "Annexe"@en .

piirritev:OsmDescriptionCastaa a skos:Concept ;
    piirrite:osmId "Castaa" ;
    rdfs:subClassOf piirrite:OsmEntity ;
    skos:definition ""@en ;
    skos:inScheme piirritev:OsmDescription ;
    skos:prefLabel "Castaa"@en .

piirritev:OsmDescriptionMaize a skos:Concept ;
    piirrite:osmId "Maize" ;
    rdfs:subClassOf piirrite:OsmEntity ;
    skos:definition ""@en ;
    skos:inScheme piirritev:OsmDescription ;
    skos:prefLabel "Maize"@en .

piirritev:OsmDescriptionSubcentre a skos:Concept ;
    piirrite:osmId "SubCentre" ;
    rdfs:subClassOf piirrite:OsmEntity ;
    skos:definition ""@en ;
    skos:inScheme piirritev:OsmDescription ;
    skos:prefLabel "Subcentre"@en .

piirritev:OsmDesignAsymmetric a skos:Concept ;
    piirrite:osmId "asymmetric" ;
    rdfs:subClassOf piirrite:OsmEntity ;
    skos:definition ""@en ;
    skos:inScheme piirritev:OsmDesign ;
    skos:prefLabel "Asymmetric"@en .

piirritev:OsmDesignBarrel a skos:Concept ;
    piirrite:osmId "barrel" ;
    rdfs:subClassOf piirrite:OsmEntity ;
    skos:definition ""@en ;
    skos:inScheme piirritev:OsmDesign ;
    skos:prefLabel "Barrel"@en .

piirritev:OsmDesignDelta a skos:Concept ;
    piirrite:osmId "delta" ;
    rdfs:subClassOf piirrite:OsmEntity ;
    skos:definition ""@en ;
    skos:inScheme piirritev:OsmDesign ;
    skos:prefLabel "Delta"@en .

piirritev:OsmDesignDonau a skos:Concept ;
    piirrite:osmId "donau" ;
    rdfs:subClassOf piirrite:OsmEntity ;
    skos:definition ""@en ;
    skos:inScheme piirritev:OsmDesign ;
    skos:prefLabel "Donau"@en .

piirritev:OsmDesignFlag a skos:Concept ;
    piirrite:osmId "flag" ;
    rdfs:subClassOf piirrite:OsmEntity ;
    skos:definition ""@en ;
    skos:inScheme piirritev:OsmDesign ;
    skos:prefLabel "Flag"@en .

piirritev:OsmDesignGuyedH-Frame a skos:Concept ;
    piirrite:osmId "guyed_h-frame" ;
    rdfs:subClassOf piirrite:OsmEntity ;
    skos:definition ""@en ;
    skos:inScheme piirritev:OsmDesign ;
    skos:prefLabel "Guyed h-frame"@en .

piirritev:OsmDesignGuyedV-Frame a skos:Concept ;
    piirrite:osmId "guyed_v-frame" ;
    rdfs:subClassOf piirrite:OsmEntity ;
    skos:definition ""@en ;
    skos:inScheme piirritev:OsmDesign ;
    skos:prefLabel "Guyed v-frame"@en .

piirritev:OsmDesignH-Frame a skos:Concept ;
    piirrite:osmId "h-frame" ;
    rdfs:subClassOf piirrite:OsmEntity ;
    skos:definition ""@en ;
    skos:inScheme piirritev:OsmDesign ;
    skos:prefLabel "H-frame"@en .

piirritev:OsmDesignOne-Level a skos:Concept ;
    piirrite:osmId "one-level" ;
    rdfs:subClassOf piirrite:OsmEntity ;
    skos:definition ""@en ;
    skos:inScheme piirritev:OsmDesign ;
    skos:prefLabel "One-level"@en .

piirritev:OsmDesignPortal a skos:Concept ;
    piirrite:osmId "portal" ;
    rdfs:subClassOf piirrite:OsmEntity ;
    skos:definition ""@en ;
    skos:inScheme piirritev:OsmDesign ;
    skos:prefLabel "Portal"@en .

piirritev:OsmDesignThree-Level a skos:Concept ;
    piirrite:osmId "three-level" ;
    rdfs:subClassOf piirrite:OsmEntity ;
    skos:definition ""@en ;
    skos:inScheme piirritev:OsmDesign ;
    skos:prefLabel "Three-level"@en .

piirritev:OsmDesignTriangle a skos:Concept ;
    piirrite:osmId "triangle" ;
    rdfs:subClassOf piirrite:OsmEntity ;
    skos:definition ""@en ;
    skos:inScheme piirritev:OsmDesign ;
    skos:prefLabel "Triangle"@en .

piirritev:OsmDesignTwo-Level a skos:Concept ;
    piirrite:osmId "two-level" ;
    rdfs:subClassOf piirrite:OsmEntity ;
    skos:definition ""@en ;
    skos:inScheme piirritev:OsmDesign ;
    skos:prefLabel "Two-level"@en .

piirritev:OsmDesignationCivilParish a skos:Concept ;
    piirrite:hasRelatedOsmTag piirrite:hasOsmCivilParishAdminLevel,
        piirrite:hasOsmCivilParishBoundary,
        piirrite:hasOsmCivilParishGovernment ;
    piirrite:osmId "civil_parish" ;
    rdfs:subClassOf piirrite:OsmEntity ;
    skos:definition "An administrative district forming part of local government."@en ;
    skos:inScheme piirritev:OsmDesignation ;
    skos:prefLabel "Civil parish"@en .

piirritev:OsmDesignationPublicBridleway a skos:Concept ;
    piirrite:hasRelatedOsmTag piirrite:hasOsmPublicBridlewayAccess,
        piirrite:hasOsmPublicBridlewayProwRef,
        piirrite:hasOsmPublicBridlewaySurface ;
    piirrite:osmId "public_bridleway" ;
    rdfs:subClassOf piirrite:OsmEntity ;
    skos:definition "A legal classification of a highway on which the public have a right to travel on foot, horseback, and by bicycle."@en ;
    skos:inScheme piirritev:OsmDesignation ;
    skos:prefLabel "Public bridleway"@en .

piirritev:OsmDesignationPublicFootpath a skos:Concept ;
    piirrite:hasRelatedOsmTag piirrite:hasOsmPublicFootpathAccess,
        piirrite:hasOsmPublicFootpathProwRef,
        piirrite:hasOsmPublicFootpathSurface ;
    piirrite:osmId "public_footpath" ;
    rdfs:subClassOf piirrite:OsmEntity ;
    skos:definition "A legal classification of a highway on which the public have a right to travel on foot."@en ;
    skos:inScheme piirritev:OsmDesignation ;
    skos:prefLabel "Public footpath"@en .

piirritev:OsmDestination a skos:ConceptScheme ;
    piirrite:osmId "destination" ;
    skos:definition "Destination when following a linear feature."@en ;
    skos:prefLabel "Destination, types"@en .

piirritev:OsmDiameter a skos:ConceptScheme ;
    piirrite:osmId "diameter" ;
    skos:definition "nominal diameter in millimeter"@en ;
    skos:prefLabel "Diameter, types"@en .

piirritev:OsmDiameterCrown a skos:ConceptScheme ;
    piirrite:osmId "diameter_crown" ;
    skos:definition ""@en ;
    skos:prefLabel "Diameter crown, types"@en .

piirritev:OsmDirectionBackward a skos:Concept ;
    piirrite:osmId "backward" ;
    rdfs:subClassOf piirrite:OsmEntity ;
    skos:definition ""@en ;
    skos:inScheme piirritev:OsmDirection ;
    skos:prefLabel "Backward"@en .

piirritev:OsmDirectionBoth a skos:Concept ;
    piirrite:osmId "both" ;
    rdfs:subClassOf piirrite:OsmEntity ;
    skos:definition ""@en ;
    skos:inScheme piirritev:OsmDirection ;
    skos:prefLabel "Both"@en .

piirritev:OsmDirectionClockwise a skos:Concept ;
    piirrite:osmId "clockwise" ;
    rdfs:subClassOf piirrite:OsmEntity ;
    skos:definition ""@en ;
    skos:inScheme piirritev:OsmDirection ;
    skos:prefLabel "Clockwise"@en .

piirritev:OsmDirectionE a skos:Concept ;
    piirrite:osmId "E" ;
    rdfs:subClassOf piirrite:OsmEntity ;
    skos:definition ""@en ;
    skos:inScheme piirritev:OsmDirection ;
    skos:prefLabel "E"@en .

piirritev:OsmDirectionForward a skos:Concept ;
    piirrite:osmId "forward" ;
    rdfs:subClassOf piirrite:OsmEntity ;
    skos:definition ""@en ;
    skos:inScheme piirritev:OsmDirection ;
    skos:prefLabel "Forward"@en .

piirritev:OsmDirectionS a skos:Concept ;
    piirrite:osmId "S" ;
    rdfs:subClassOf piirrite:OsmEntity ;
    skos:definition ""@en ;
    skos:inScheme piirritev:OsmDirection ;
    skos:prefLabel "S"@en .

piirritev:OsmDirectionSe a skos:Concept ;
    piirrite:osmId "SE" ;
    rdfs:subClassOf piirrite:OsmEntity ;
    skos:definition ""@en ;
    skos:inScheme piirritev:OsmDirection ;
    skos:prefLabel "Se"@en .

piirritev:OsmDirectionSse a skos:Concept ;
    piirrite:osmId "SSE" ;
    rdfs:subClassOf piirrite:OsmEntity ;
    skos:definition ""@en ;
    skos:inScheme piirritev:OsmDirection ;
    skos:prefLabel "Sse"@en .

piirritev:OsmDirectionSsw a skos:Concept ;
    piirrite:osmId "SSW" ;
    rdfs:subClassOf piirrite:OsmEntity ;
    skos:definition ""@en ;
    skos:inScheme piirritev:OsmDirection ;
    skos:prefLabel "Ssw"@en .

piirritev:OsmDirectionSw a skos:Concept ;
    piirrite:osmId "SW" ;
    rdfs:subClassOf piirrite:OsmEntity ;
    skos:definition ""@en ;
    skos:inScheme piirritev:OsmDirection ;
    skos:prefLabel "Sw"@en .

piirritev:OsmDirectionW a skos:Concept ;
    piirrite:osmId "W" ;
    rdfs:subClassOf piirrite:OsmEntity ;
    skos:definition ""@en ;
    skos:inScheme piirritev:OsmDirection ;
    skos:prefLabel "W"@en .

piirritev:OsmDispensing a skos:ConceptScheme ;
    piirrite:osmId "dispensing" ;
    skos:definition "Whether a pharmacy dispenses prescription drugs or not."@en ;
    skos:prefLabel "Dispensing, types"@en .

piirritev:OsmDistance a skos:ConceptScheme ;
    piirrite:osmId "distance" ;
    skos:definition "Distance (i.e. extent; length from start to finish) of a route given in kilometres, or distance along a route marked by milestone."@en ;
    skos:prefLabel "Distance, types"@en .

piirritev:OsmDisused a skos:ConceptScheme ;
    piirrite:osmId "disused" ;
    skos:definition "Specifies if a feature is disused but in a reasonable state of repair."@en ;
    skos:prefLabel "Disused, types"@en .

piirritev:OsmDogLeashed a skos:Concept ;
    piirrite:osmId "leashed" ;
    rdfs:subClassOf piirrite:OsmEntity ;
    skos:definition "Indicates that dogs are allowed if on leash."@en ;
    skos:inScheme piirritev:OsmDog ;
    skos:prefLabel "Leashed"@en .

piirritev:OsmDrinkingWater a skos:ConceptScheme ;
    piirrite:osmId "drinking_water" ;
    skos:definition "Indication whether a feature provides drinking water."@en ;
    skos:prefLabel "Drinking water, types"@en .

piirritev:OsmDriveThrough a skos:ConceptScheme ;
    piirrite:osmId "drive_through" ;
    skos:definition "To indicate whether an amenity offers a drive-through service."@en ;
    skos:prefLabel "Drive through, types"@en .

piirritev:OsmDualCarriageway a skos:ConceptScheme ;
    piirrite:osmId "dual_carriageway" ;
    skos:definition "Specifies whether a highway is a dual-carriageway (divided) road"@en ;
    skos:prefLabel "Dual carriageway, types"@en .

piirritev:OsmEducationKindergarten a skos:Concept ;
    piirrite:hasRelatedOsmTag piirrite:hasOsmKindergartenName,
        piirrite:hasOsmKindergartenOperator,
        piirrite:hasOsmKindergartenPhone ;
    piirrite:osmId "kindergarten" ;
    rdfs:subClassOf piirrite:OsmEntity ;
    skos:definition "A place for looking after preschool children and (typically) giving early education."@en ;
    skos:inScheme piirritev:OsmEducation ;
    skos:prefLabel "Kindergarten"@en .

piirritev:OsmEducationSchool a skos:Concept ;
    piirrite:hasRelatedOsmTag piirrite:hasOsmSchoolAmenity,
        piirrite:hasOsmSchoolGrades ;
    piirrite:osmId "school" ;
    rdfs:subClassOf piirrite:OsmEntity ;
    skos:definition "A primary or secondary school (pupils typically aged 6 to 18)."@en ;
    skos:inScheme piirritev:OsmEducation ;
    skos:prefLabel "School"@en .

piirritev:OsmEle a skos:ConceptScheme ;
    piirrite:osmId "ele" ;
    skos:definition "Elevation of a point above sea level, in metres."@en ;
    skos:prefLabel "Ele, types"@en .

piirritev:OsmElectrifiedContactLine a skos:Concept ;
    piirrite:hasRelatedOsmTag piirrite:hasOsmContactLineRailway ;
    piirrite:osmId "contact_line" ;
    rdfs:subClassOf piirrite:OsmEntity ;
    skos:definition "An overhead line."@en ;
    skos:inScheme piirritev:OsmElectrified ;
    skos:prefLabel "Contact line"@en .

piirritev:OsmElectrifiedRail a skos:Concept ;
    piirrite:hasRelatedOsmTag piirrite:hasOsmRailRailway ;
    piirrite:osmId "rail" ;
    rdfs:subClassOf piirrite:OsmEntity ;
    skos:definition "Electrified with a third rail system."@en ;
    skos:inScheme piirritev:OsmElectrified ;
    skos:prefLabel "Rail"@en .

piirritev:OsmEmail a skos:ConceptScheme ;
    piirrite:osmId "email" ;
    skos:definition "An email address associated with the object"@en ;
    skos:prefLabel "Email, types"@en .

piirritev:OsmEmbankment a skos:ConceptScheme ;
    piirrite:osmId "embankment" ;
    skos:definition "A dyke or raised bank to carry a road, railway, or canal across a low-lying or wet area."@en ;
    skos:prefLabel "Embankment, types"@en .

piirritev:OsmEmergencyAccessPoint a skos:Concept ;
    piirrite:hasRelatedOsmTag piirrite:hasOsmAccessPointName,
        piirrite:hasOsmAccessPointOperator,
        piirrite:hasOsmAccessPointRef ;
    piirrite:osmId "access_point" ;
    rdfs:subClassOf piirrite:OsmEntity ;
    skos:definition "A sign number which can be used to define your current position in case of an emergency"@en ;
    skos:inScheme piirritev:OsmEmergency ;
    skos:prefLabel "Access point"@en .

piirritev:OsmEmergencyAmbulanceStation a skos:Concept ;
    piirrite:hasRelatedOsmTag piirrite:hasOsmAmbulanceStationName,
        piirrite:hasOsmAmbulanceStationOperator ;
    piirrite:osmId "ambulance_station" ;
    rdfs:subClassOf piirrite:OsmEntity ;
    skos:definition "An ambulance station is a structure or other area set aside for storage of ambulance vehicles, medical equipment, personal protective equipment, and other medical supplies."@en ;
    skos:inScheme piirritev:OsmEmergency ;
    skos:prefLabel "Ambulance station"@en .

piirritev:OsmEmergencyAssemblyPoint a skos:Concept ;
    piirrite:hasRelatedOsmTag piirrite:hasOsmAssemblyPointCheckDate,
        piirrite:hasOsmAssemblyPointName,
        piirrite:hasOsmAssemblyPointOperator,
        piirrite:hasOsmAssemblyPointRef ;
    piirrite:osmId "assembly_point" ;
    rdfs:subClassOf piirrite:OsmEntity ;
    skos:definition "A designated (safe) place where people can gather or must report to during an emergency or a fire drill."@en ;
    skos:inScheme piirritev:OsmEmergency ;
    skos:prefLabel "Assembly point"@en .

piirritev:OsmEmergencyDefibrillator a skos:Concept ;
    piirrite:hasRelatedOsmTag piirrite:hasOsmDefibrillatorAccess,
        piirrite:hasOsmDefibrillatorOpeningHours,
        piirrite:hasOsmDefibrillatorPhone ;
    piirrite:osmId "defibrillator" ;
    rdfs:subClassOf piirrite:OsmEntity ;
    skos:definition "Defibrillator (AED), an external and portable electronic device that diagnoses and can correct arrhythmia of the heart automatically."@en ;
    skos:inScheme piirritev:OsmEmergency ;
    skos:prefLabel "Defibrillator"@en .

piirritev:OsmEmergencyDesignated a skos:Concept ;
    piirrite:hasRelatedOsmTag piirrite:hasOsmDesignatedSurface ;
    piirrite:osmId "designated" ;
    rdfs:subClassOf piirrite:OsmEntity ;
    skos:definition "An emergency access road"@en ;
    skos:inScheme piirritev:OsmEmergency ;
    skos:prefLabel "Designated"@en .

piirritev:OsmEmergencyFireExtinguisher a skos:Concept ;
    piirrite:osmId "fire_extinguisher" ;
    rdfs:subClassOf piirrite:OsmEntity ;
    skos:definition "An active fire protection device used to extinguish or control small fires, often in emergency situations."@en ;
    skos:inScheme piirritev:OsmEmergency ;
    skos:prefLabel "Fire extinguisher"@en .

piirritev:OsmEmergencyFireHydrant a skos:Concept ;
    piirrite:hasRelatedOsmTag piirrite:hasOsmFireHydrantRef,
        piirrite:hasOsmFireHydrantType,
        piirrite:hasOsmFireHydrantWaterSource ;
    piirrite:osmId "fire_hydrant" ;
    rdfs:subClassOf piirrite:OsmEntity ;
    skos:definition "An active fire protection measure, and a source of water provided in most urban, suburban, and rural areas with municipal water service to enable fire fighters to tap into the municipal water supply to assist in extinguishing a fire."@en ;
    skos:inScheme piirritev:OsmEmergency ;
    skos:prefLabel "Fire hydrant"@en .

piirritev:OsmEmergencyLifeRing a skos:Concept ;
    piirrite:hasRelatedOsmTag piirrite:hasOsmLifeRingColour,
        piirrite:hasOsmLifeRingOperator,
        piirrite:hasOsmLifeRingRef,
        piirrite:hasOsmLifeRingSupport ;
    piirrite:osmId "life_ring" ;
    rdfs:subClassOf piirrite:OsmEntity ;
    skos:definition "A floating ring to throw out to someone who is struggling in water."@en ;
    skos:inScheme piirritev:OsmEmergency ;
    skos:prefLabel "Life ring"@en .

piirritev:OsmEmergencyPhone a skos:Concept ;
    piirrite:hasRelatedOsmTag piirrite:hasOsmPhoneOperator,
        piirrite:hasOsmPhoneRef ;
    piirrite:osmId "phone" ;
    rdfs:subClassOf piirrite:OsmEntity ;
    skos:definition "Emergency telephone osmcarto-rendering=File:Emergency-phone.16.svg osmcarto-rendering-size=28px"@en ;
    skos:inScheme piirritev:OsmEmergency ;
    skos:prefLabel "Phone"@en .

piirritev:OsmEmergencySiren a skos:Concept ;
    piirrite:hasRelatedOsmTag piirrite:hasOsmSirenOperator,
        piirrite:hasOsmSirenWebsite ;
    piirrite:osmId "siren" ;
    rdfs:subClassOf piirrite:OsmEntity ;
    skos:definition "A loud noise maker, such as an air raid siren or a tornado siren."@en ;
    skos:inScheme piirritev:OsmEmergency ;
    skos:prefLabel "Siren"@en .

piirritev:OsmEmergencySuctionPoint a skos:Concept ;
    piirrite:osmId "suction_point" ;
    rdfs:subClassOf piirrite:OsmEntity ;
    skos:definition "A preferred point to pump water off a river or other waters for a fire department."@en ;
    skos:inScheme piirritev:OsmEmergency ;
    skos:prefLabel "Suction point"@en .

piirritev:OsmEmergencyWaterTank a skos:Concept ;
    piirrite:hasRelatedOsmTag piirrite:hasOsmWaterTankAccess,
        piirrite:hasOsmWaterTankCapacity,
        piirrite:hasOsmWaterTankContent,
        piirrite:hasOsmWaterTankIntermittent,
        piirrite:hasOsmWaterTankName,
        piirrite:hasOsmWaterTankOperator,
        piirrite:hasOsmWaterTankWaterVolume ;
    piirrite:osmId "water_tank" ;
    rdfs:subClassOf piirrite:OsmEntity ;
    skos:definition "A large water basin or tank for a fire department to take water."@en ;
    skos:inScheme piirritev:OsmEmergency ;
    skos:prefLabel "Water tank"@en .

piirritev:OsmEntranceEmergency a skos:Concept ;
    piirrite:osmId "emergency" ;
    rdfs:subClassOf piirrite:OsmEntity ;
    skos:definition "An entrance or exit of a building that is intended for use in an emergency."@en ;
    skos:inScheme piirritev:OsmEntrance ;
    skos:prefLabel "Emergency"@en .

piirritev:OsmEntranceExit a skos:Concept ;
    piirrite:osmId "exit" ;
    rdfs:subClassOf piirrite:OsmEntity ;
    skos:definition "It is not an entrance, it is a one-way out of a building. You can find these at public transport locations, some larger shops, museums and theme parks."@en ;
    skos:inScheme piirritev:OsmEntrance ;
    skos:prefLabel "Exit"@en .

piirritev:OsmEntranceGarage a skos:Concept ;
    piirrite:hasRelatedOsmTag piirrite:hasOsmGarageAccess,
        piirrite:hasOsmGarageDoor ;
    piirrite:osmId "garage" ;
    rdfs:subClassOf piirrite:OsmEntity ;
    skos:definition "A garage door"@en ;
    skos:inScheme piirritev:OsmEntrance ;
    skos:prefLabel "Garage"@en .

piirritev:OsmEntranceHome a skos:Concept ;
    piirrite:osmId "home" ;
    rdfs:subClassOf piirrite:OsmEntity ;
    skos:definition "The entrance of a home, e.g. a house."@en ;
    skos:inScheme piirritev:OsmEntrance ;
    skos:prefLabel "Home"@en .

piirritev:OsmEntranceMain a skos:Concept ;
    piirrite:hasRelatedOsmTag piirrite:hasOsmMainAccess,
        piirrite:hasOsmMainWheelchair ;
    piirrite:osmId "main" ;
    rdfs:subClassOf piirrite:OsmEntity ;
    skos:definition "The main entrance of a building osmcarto-rendering=File:Entrance main.svg osmcarto-rendering-size=14px"@en ;
    skos:inScheme piirritev:OsmEntrance ;
    skos:prefLabel "Main"@en .

piirritev:OsmEntranceSecondary a skos:Concept ;
    piirrite:hasRelatedOsmTag piirrite:hasOsmSecondaryAccess,
        piirrite:hasOsmSecondaryAddr,
        piirrite:hasOsmSecondaryRef,
        piirrite:hasOsmSecondaryWheelchair ;
    piirrite:osmId "secondary" ;
    rdfs:subClassOf piirrite:OsmEntity ;
    skos:definition "Secondary entrance used for events"@en ;
    skos:inScheme piirritev:OsmEntrance ;
    skos:prefLabel "Secondary"@en .

piirritev:OsmEntranceService a skos:Concept ;
    piirrite:osmId "service" ;
    rdfs:subClassOf piirrite:OsmEntity ;
    skos:definition "A backdoor to a building or enclosed area often only for employees or for delivering. osmcarto-rendering=File:Entrance.svg osmcarto-rendering-size=14px"@en ;
    skos:inScheme piirritev:OsmEntrance ;
    skos:prefLabel "Service"@en .

piirritev:OsmEntranceShop a skos:Concept ;
    piirrite:osmId "shop" ;
    rdfs:subClassOf piirrite:OsmEntity ;
    skos:definition "A direct public entrance to a shop which is not a main building entrance."@en ;
    skos:inScheme piirritev:OsmEntrance ;
    skos:prefLabel "Shop"@en .

piirritev:OsmEntranceStaircase a skos:Concept ;
    piirrite:hasRelatedOsmTag piirrite:hasOsmStaircaseRef ;
    piirrite:osmId "staircase" ;
    rdfs:subClassOf piirrite:OsmEntity ;
    skos:definition "A staircase entrance."@en ;
    skos:inScheme piirritev:OsmEntrance ;
    skos:prefLabel "Staircase"@en .

piirritev:OsmEstWidth a skos:ConceptScheme ;
    piirrite:osmId "est_width" ;
    skos:definition "The estimated width of a feature"@en ;
    skos:prefLabel "Est width, types"@en .

piirritev:OsmExpressway a skos:ConceptScheme ;
    piirrite:osmId "expressway" ;
    skos:definition "A highway with high-speed design features and limited access to adjacent properties. Usually a dual-carriageway (divided)."@en ;
    skos:prefLabel "Expressway, types"@en .

piirritev:OsmFax a skos:ConceptScheme ;
    piirrite:osmId "fax" ;
    skos:definition "A fax number associated with the object."@en ;
    skos:prefLabel "Fax, types"@en .

piirritev:OsmFee a skos:ConceptScheme ;
    piirrite:osmId "fee" ;
    skos:definition "Yes or no, to indicate if money is charged to use this facility."@en ;
    skos:prefLabel "Fee, types"@en .

piirritev:OsmFenceTypeBarbedWire a skos:Concept ;
    piirrite:osmId "barbed_wire" ;
    rdfs:subClassOf piirrite:OsmEntity ;
    skos:definition ""@en ;
    skos:inScheme piirritev:OsmFenceType ;
    skos:prefLabel "Barbed wire"@en .

piirritev:OsmFenceTypeBars a skos:Concept ;
    piirrite:osmId "bars" ;
    rdfs:subClassOf piirrite:OsmEntity ;
    skos:definition ""@en ;
    skos:inScheme piirritev:OsmFenceType ;
    skos:prefLabel "Bars"@en .

piirritev:OsmFenceTypeChainLink a skos:Concept ;
    piirrite:osmId "chain_link" ;
    rdfs:subClassOf piirrite:OsmEntity ;
    skos:definition ""@en ;
    skos:inScheme piirritev:OsmFenceType ;
    skos:prefLabel "Chain link"@en .

piirritev:OsmFenceTypeConcrete a skos:Concept ;
    piirrite:osmId "concrete" ;
    rdfs:subClassOf piirrite:OsmEntity ;
    skos:definition ""@en ;
    skos:inScheme piirritev:OsmFenceType ;
    skos:prefLabel "Concrete"@en .

piirritev:OsmFenceTypeMetal a skos:Concept ;
    piirrite:osmId "metal" ;
    rdfs:subClassOf piirrite:OsmEntity ;
    skos:definition ""@en ;
    skos:inScheme piirritev:OsmFenceType ;
    skos:prefLabel "Metal"@en .

piirritev:OsmFenceTypePole a skos:Concept ;
    piirrite:osmId "pole" ;
    rdfs:subClassOf piirrite:OsmEntity ;
    skos:definition ""@en ;
    skos:inScheme piirritev:OsmFenceType ;
    skos:prefLabel "Pole"@en .

piirritev:OsmFenceTypeRailing a skos:Concept ;
    piirrite:osmId "railing" ;
    rdfs:subClassOf piirrite:OsmEntity ;
    skos:definition "A railing for example at the edge of a bridge to prevent persons or vehicles from falling down. Often made of metal or wood."@en ;
    skos:inScheme piirritev:OsmFenceType ;
    skos:prefLabel "Railing"@en .

piirritev:OsmFenceTypeSplitRail a skos:Concept ;
    piirrite:osmId "split_rail" ;
    rdfs:subClassOf piirrite:OsmEntity ;
    skos:definition ""@en ;
    skos:inScheme piirritev:OsmFenceType ;
    skos:prefLabel "Split rail"@en .

piirritev:OsmFenceTypeWire a skos:Concept ;
    piirrite:osmId "wire" ;
    rdfs:subClassOf piirrite:OsmEntity ;
    skos:definition ""@en ;
    skos:inScheme piirritev:OsmFenceType ;
    skos:prefLabel "Wire"@en .

piirritev:OsmFenceTypeWood a skos:Concept ;
    piirrite:osmId "wood" ;
    rdfs:subClassOf piirrite:OsmEntity ;
    skos:definition ""@en ;
    skos:inScheme piirritev:OsmFenceType ;
    skos:prefLabel "Wood"@en .

piirritev:OsmFid a skos:ConceptScheme ;
    piirrite:osmId "fid" ;
    skos:definition "Used to assign a unique identifier to each feature within a geospatial file; required by some formats such as GeoPackage."@en ;
    skos:prefLabel "Fid, types"@en .

piirritev:OsmFixmeContinue a skos:Concept ;
    piirrite:osmId "continue" ;
    rdfs:subClassOf piirrite:OsmEntity ;
    skos:definition ""@en ;
    skos:inScheme piirritev:OsmFixme ;
    skos:prefLabel "Continue"@en .

piirritev:OsmFixmeIncomplete a skos:Concept ;
    piirrite:osmId "incomplete" ;
    rdfs:subClassOf piirrite:OsmEntity ;
    skos:definition ""@en ;
    skos:inScheme piirritev:OsmFixme ;
    skos:prefLabel "Incomplete"@en .

piirritev:OsmFixmeName a skos:Concept ;
    piirrite:osmId "name" ;
    rdfs:subClassOf piirrite:OsmEntity ;
    skos:definition "To define if the object has a (possible) erroneous name."@en ;
    skos:inScheme piirritev:OsmFixme ;
    skos:prefLabel "Name"@en .

piirritev:OsmFixmePosition a skos:Concept ;
    piirrite:osmId "position" ;
    rdfs:subClassOf piirrite:OsmEntity ;
    skos:definition ""@en ;
    skos:inScheme piirritev:OsmFixme ;
    skos:prefLabel "Position"@en .

piirritev:OsmFixmePositionEstimated a skos:Concept ;
    piirrite:osmId "Position_estimated" ;
    rdfs:subClassOf piirrite:OsmEntity ;
    skos:definition ""@en ;
    skos:inScheme piirritev:OsmFixme ;
    skos:prefLabel "Position estimated"@en .

piirritev:OsmFixmeResurvey a skos:Concept ;
    piirrite:osmId "resurvey" ;
    rdfs:subClassOf piirrite:OsmEntity ;
    skos:definition ""@en ;
    skos:inScheme piirritev:OsmFixme ;
    skos:prefLabel "Resurvey"@en .

piirritev:OsmFixmeStub a skos:Concept ;
    piirrite:osmId "stub" ;
    rdfs:subClassOf piirrite:OsmEntity ;
    skos:definition ""@en ;
    skos:inScheme piirritev:OsmFixme ;
    skos:prefLabel "Stub"@en .

piirritev:OsmFloating a skos:ConceptScheme ;
    piirrite:osmId "floating" ;
    skos:definition "This property indicates whether an object floats"@en ;
    skos:prefLabel "Floating, types"@en .

piirritev:OsmFootCustomers a skos:Concept ;
    piirrite:osmId "customers" ;
    rdfs:subClassOf piirrite:OsmEntity ;
    skos:definition ""@en ;
    skos:inScheme piirritev:OsmFoot ;
    skos:prefLabel "Customers"@en .

piirritev:OsmFootDesignated a skos:Concept ;
    piirrite:osmId "designated" ;
    rdfs:subClassOf piirrite:OsmEntity ;
    skos:definition "A preferred or designated route for pedestrians."@en ;
    skos:inScheme piirritev:OsmFoot ;
    skos:prefLabel "Designated"@en .

piirritev:OsmFootDestination a skos:Concept ;
    piirrite:hasRelatedOsmTag piirrite:hasOsmDestinationHighway ;
    piirrite:osmId "destination" ;
    rdfs:subClassOf piirrite:OsmEntity ;
    skos:definition "Transit traffic forbidden for pedestrians, non-transit to a local destination allowed."@en ;
    skos:inScheme piirritev:OsmFoot ;
    skos:prefLabel "Destination"@en .

piirritev:OsmFootPermissive a skos:Concept ;
    piirrite:hasRelatedOsmTag piirrite:hasOsmPermissiveHighway ;
    piirrite:osmId "permissive" ;
    rdfs:subClassOf piirrite:OsmEntity ;
    skos:definition "Access by pedestrians is permitted but permission may be withdrawn at any time."@en ;
    skos:inScheme piirritev:OsmFoot ;
    skos:prefLabel "Permissive"@en .

piirritev:OsmFootPrivate a skos:Concept ;
    piirrite:osmId "private" ;
    rdfs:subClassOf piirrite:OsmEntity ;
    skos:definition "Indicates that walking is not allowed for public, but the owner may make exceptions at will."@en ;
    skos:inScheme piirritev:OsmFoot ;
    skos:prefLabel "Private"@en .

piirritev:OsmFootUseSidepath a skos:Concept ;
    piirrite:hasRelatedOsmTag piirrite:hasOsmUseSidepathHighway ;
    piirrite:osmId "use_sidepath" ;
    rdfs:subClassOf piirrite:OsmEntity ;
    skos:definition "Use compulsory parallel footpath instead"@en ;
    skos:inScheme piirritev:OsmFoot ;
    skos:prefLabel "Use sidepath"@en .

piirritev:OsmFootwayAccessAisle a skos:Concept ;
    piirrite:hasRelatedOsmTag piirrite:hasOsmAccessAisleType ;
    piirrite:osmId "access_aisle" ;
    rdfs:subClassOf piirrite:OsmEntity ;
    skos:definition "A marked footpath in a parking lot, typically between two parking spaces, to facilitate access to parked vehicles."@en ;
    skos:inScheme piirritev:OsmFootway ;
    skos:prefLabel "Access aisle"@en .

piirritev:OsmFootwayAlley a skos:Concept ;
    piirrite:hasRelatedOsmTag piirrite:hasOsmAlleyAccess,
        piirrite:hasOsmAlleyFootway ;
    piirrite:osmId "alley" ;
    rdfs:subClassOf piirrite:OsmEntity ;
    skos:definition "An alley is a footway usually located between properties for access to back entrances and/or emergency access. onNode = no onWay = yes onArea = no onRelation = no requires = * highway=footway combination = * {{keyaccess}} seeAlso = * footway status = in use"@en ;
    skos:inScheme piirritev:OsmFootway ;
    skos:prefLabel "Alley"@en .

piirritev:OsmFootwayCrossing a skos:Concept ;
    piirrite:hasRelatedOsmTag piirrite:hasOsmCrossingEstWidth,
        piirrite:hasOsmCrossingIncline,
        piirrite:hasOsmCrossingKerb,
        piirrite:hasOsmCrossingSmoothness,
        piirrite:hasOsmCrossingSurface,
        piirrite:hasOsmCrossingTactilePaving,
        piirrite:hasOsmCrossingType,
        piirrite:hasOsmCrossingWheelchair,
        piirrite:hasOsmCrossingWidth ;
    piirrite:osmId "crossing" ;
    rdfs:subClassOf piirrite:OsmEntity ;
    skos:definition "Specifies that the footway is a road crossing."@en ;
    skos:inScheme piirritev:OsmFootway ;
    skos:prefLabel "Crossing"@en .

piirritev:OsmFootwayLink a skos:Concept ;
    piirrite:hasRelatedOsmTag piirrite:hasOsmLinkLit,
        piirrite:hasOsmLinkSurface,
        piirrite:hasOsmLinkWheelchair ;
    piirrite:osmId "link" ;
    rdfs:subClassOf piirrite:OsmEntity ;
    skos:definition "A traversable path connecting other highways to enable routing."@en ;
    skos:inScheme piirritev:OsmFootway ;
    skos:prefLabel "Link"@en .

piirritev:OsmFootwayPath a skos:Concept ;
    piirrite:osmId "path" ;
    rdfs:subClassOf piirrite:OsmEntity ;
    skos:definition "Used for pedestrian paths not linked to roads. onNode = no onWay = yes onArea = no onRelation = no requires = * highway=footway status = in use"@en ;
    skos:inScheme piirritev:OsmFootway ;
    skos:prefLabel "Path"@en .

piirritev:OsmFootwaySidewalk a skos:Concept ;
    piirrite:hasRelatedOsmTag piirrite:hasOsmSidewalkEstWidth,
        piirrite:hasOsmSidewalkIncline,
        piirrite:hasOsmSidewalkKerb,
        piirrite:hasOsmSidewalkSmoothness,
        piirrite:hasOsmSidewalkSurface,
        piirrite:hasOsmSidewalkTactilePaving,
        piirrite:hasOsmSidewalkType,
        piirrite:hasOsmSidewalkWheelchair,
        piirrite:hasOsmSidewalkWidth ;
    piirrite:osmId "sidewalk" ;
    rdfs:subClassOf piirrite:OsmEntity ;
    skos:definition "Sidewalks as separate ways."@en ;
    skos:inScheme piirritev:OsmFootway ;
    skos:prefLabel "Sidewalk"@en .

piirritev:OsmFootwayTrafficIsland a skos:Concept ;
    piirrite:hasRelatedOsmTag piirrite:hasOsmTrafficIslandEstWidth,
        piirrite:hasOsmTrafficIslandFootway,
        piirrite:hasOsmTrafficIslandIncline,
        piirrite:hasOsmTrafficIslandKerb,
        piirrite:hasOsmTrafficIslandSmoothness,
        piirrite:hasOsmTrafficIslandSurface,
        piirrite:hasOsmTrafficIslandTactilePaving,
        piirrite:hasOsmTrafficIslandWheelchair,
        piirrite:hasOsmTrafficIslandWidth ;
    piirrite:osmId "traffic_island" ;
    rdfs:subClassOf piirrite:OsmEntity ;
    skos:definition "Parts of a footway that serves as pedestrian refuge on a traffic island. onNode = no onWay = yes onArea = no onRelation = no requires = * highway=footway combination = * {{keykerb}} * {{keyincline}} * {{keywheelchair}} * {{keysmoothness}} * {{keysurface}} * {{keytactile_paving}} * {{keywidth}} / {{keyest_width}} seeAlso = * footway=crossing * footway=sidewalk * {{Keyfootway}} * {{Keycrossing:island}} status = de facto"@en ;
    skos:inScheme piirritev:OsmFootway ;
    skos:prefLabel "Traffic island"@en .

piirritev:OsmFordSteppingStones a skos:Concept ;
    piirrite:osmId "stepping_stones" ;
    rdfs:subClassOf piirrite:OsmEntity ;
    skos:definition "A ford for crossing a waterway with stepping stones  osmcarto-rendering = File:Ford.16.svg  osmcarto-rendering-size = 28px"@en ;
    skos:inScheme piirritev:OsmFord ;
    skos:prefLabel "Stepping stones"@en .

piirritev:OsmFrequency a skos:ConceptScheme ;
    piirrite:osmId "frequency" ;
    skos:definition "For describing the frequency of electric power supply networks and devices, electrified railways, trolleybuses and communications devices. The unit is Hz (cycles per second)."@en ;
    skos:prefLabel "Frequency, types"@en .

piirritev:OsmFrom a skos:ConceptScheme ;
    piirrite:osmId "from" ;
    skos:definition "Start station"@en ;
    skos:prefLabel "From, types"@en .

piirritev:OsmGauge a skos:ConceptScheme ;
    piirrite:osmId "gauge" ;
    skos:definition "Used to describe the 'gauge' (distance between the inside of the rails) on railways."@en ;
    skos:prefLabel "Gauge, types"@en .

piirritev:OsmGenusAcer a skos:Concept ;
    piirrite:osmId "Acer" ;
    rdfs:subClassOf piirrite:OsmEntity ;
    skos:definition "Acer is a genus of trees and shrubs, commonly known as maples."@en ;
    skos:inScheme piirritev:OsmGenus ;
    skos:prefLabel "Acer"@en .

piirritev:OsmGenusAesculus a skos:Concept ;
    piirrite:osmId "Aesculus" ;
    rdfs:subClassOf piirrite:OsmEntity ;
    skos:definition ""@en ;
    skos:inScheme piirritev:OsmGenus ;
    skos:prefLabel "Aesculus"@en .

piirritev:OsmGenusAlnus a skos:Concept ;
    piirrite:osmId "Alnus" ;
    rdfs:subClassOf piirrite:OsmEntity ;
    skos:definition ""@en ;
    skos:inScheme piirritev:OsmGenus ;
    skos:prefLabel "Alnus"@en .

piirritev:OsmGenusBetula a skos:Concept ;
    piirrite:osmId "Betula" ;
    rdfs:subClassOf piirrite:OsmEntity ;
    skos:definition ""@en ;
    skos:inScheme piirritev:OsmGenus ;
    skos:prefLabel "Betula"@en .

piirritev:OsmGenusCamellia a skos:Concept ;
    piirrite:osmId "Camellia" ;
    rdfs:subClassOf piirrite:OsmEntity ;
    skos:definition ""@en ;
    skos:inScheme piirritev:OsmGenus ;
    skos:prefLabel "Camellia"@en .

piirritev:OsmGenusCarpinus a skos:Concept ;
    piirrite:osmId "Carpinus" ;
    rdfs:subClassOf piirrite:OsmEntity ;
    skos:definition ""@en ;
    skos:inScheme piirritev:OsmGenus ;
    skos:prefLabel "Carpinus"@en .

piirritev:OsmGenusCeltis a skos:Concept ;
    piirrite:osmId "Celtis" ;
    rdfs:subClassOf piirrite:OsmEntity ;
    skos:definition ""@en ;
    skos:inScheme piirritev:OsmGenus ;
    skos:prefLabel "Celtis"@en .

piirritev:OsmGenusCerasus a skos:Concept ;
    piirrite:osmId "Cerasus" ;
    rdfs:subClassOf piirrite:OsmEntity ;
    skos:definition ""@en ;
    skos:inScheme piirritev:OsmGenus ;
    skos:prefLabel "Cerasus"@en .

piirritev:OsmGenusCorylus a skos:Concept ;
    piirrite:osmId "Corylus" ;
    rdfs:subClassOf piirrite:OsmEntity ;
    skos:definition ""@en ;
    skos:inScheme piirritev:OsmGenus ;
    skos:prefLabel "Corylus"@en .

piirritev:OsmGenusElaeis a skos:Concept ;
    piirrite:osmId "Elaeis" ;
    rdfs:subClassOf piirrite:OsmEntity ;
    skos:definition ""@en ;
    skos:inScheme piirritev:OsmGenus ;
    skos:prefLabel "Elaeis"@en .

piirritev:OsmGenusEucalyptus a skos:Concept ;
    piirrite:osmId "Eucalyptus" ;
    rdfs:subClassOf piirrite:OsmEntity ;
    skos:definition ""@en ;
    skos:inScheme piirritev:OsmGenus ;
    skos:prefLabel "Eucalyptus"@en .

piirritev:OsmGenusFagus a skos:Concept ;
    piirrite:osmId "Fagus" ;
    rdfs:subClassOf piirrite:OsmEntity ;
    skos:definition ""@en ;
    skos:inScheme piirritev:OsmGenus ;
    skos:prefLabel "Fagus"@en .

piirritev:OsmGenusFraxinus a skos:Concept ;
    piirrite:osmId "Fraxinus" ;
    rdfs:subClassOf piirrite:OsmEntity ;
    skos:definition ""@en ;
    skos:inScheme piirritev:OsmGenus ;
    skos:prefLabel "Fraxinus"@en .

piirritev:OsmGenusGleditsia a skos:Concept ;
    piirrite:osmId "Gleditsia" ;
    rdfs:subClassOf piirrite:OsmEntity ;
    skos:definition ""@en ;
    skos:inScheme piirritev:OsmGenus ;
    skos:prefLabel "Gleditsia"@en .

piirritev:OsmGenusMalus a skos:Concept ;
    piirrite:osmId "Malus" ;
    rdfs:subClassOf piirrite:OsmEntity ;
    skos:definition ""@en ;
    skos:inScheme piirritev:OsmGenus ;
    skos:prefLabel "Malus"@en .

piirritev:OsmGenusMusa a skos:Concept ;
    piirrite:osmId "Musa" ;
    rdfs:subClassOf piirrite:OsmEntity ;
    skos:definition ""@en ;
    skos:inScheme piirritev:OsmGenus ;
    skos:prefLabel "Musa"@en .

piirritev:OsmGenusOlea a skos:Concept ;
    piirrite:osmId "Olea" ;
    rdfs:subClassOf piirrite:OsmEntity ;
    skos:definition ""@en ;
    skos:inScheme piirritev:OsmGenus ;
    skos:prefLabel "Olea"@en .

piirritev:OsmGenusPhoenix a skos:Concept ;
    piirrite:osmId "Phoenix" ;
    rdfs:subClassOf piirrite:OsmEntity ;
    skos:definition ""@en ;
    skos:inScheme piirritev:OsmGenus ;
    skos:prefLabel "Phoenix"@en .

piirritev:OsmGenusPicea a skos:Concept ;
    piirrite:osmId "Picea" ;
    rdfs:subClassOf piirrite:OsmEntity ;
    skos:definition ""@en ;
    skos:inScheme piirritev:OsmGenus ;
    skos:prefLabel "Picea"@en .

piirritev:OsmGenusPinus a skos:Concept ;
    piirrite:osmId "Pinus" ;
    rdfs:subClassOf piirrite:OsmEntity ;
    skos:definition ""@en ;
    skos:inScheme piirritev:OsmGenus ;
    skos:prefLabel "Pinus"@en .

piirritev:OsmGenusPlatanus a skos:Concept ;
    piirrite:osmId "Platanus" ;
    rdfs:subClassOf piirrite:OsmEntity ;
    skos:definition "Platanus is a genus of trees, commonly known as plane tree."@en ;
    skos:inScheme piirritev:OsmGenus ;
    skos:prefLabel "Platanus"@en .

piirritev:OsmGenusPopulus a skos:Concept ;
    piirrite:osmId "Populus" ;
    rdfs:subClassOf piirrite:OsmEntity ;
    skos:definition ""@en ;
    skos:inScheme piirritev:OsmGenus ;
    skos:prefLabel "Populus"@en .

piirritev:OsmGenusPrunus a skos:Concept ;
    piirrite:osmId "Prunus" ;
    rdfs:subClassOf piirrite:OsmEntity ;
    skos:definition ""@en ;
    skos:inScheme piirritev:OsmGenus ;
    skos:prefLabel "Prunus"@en .

piirritev:OsmGenusPyrus a skos:Concept ;
    piirrite:osmId "Pyrus" ;
    rdfs:subClassOf piirrite:OsmEntity ;
    skos:definition ""@en ;
    skos:inScheme piirritev:OsmGenus ;
    skos:prefLabel "Pyrus"@en .

piirritev:OsmGenusQuercus a skos:Concept ;
    piirrite:osmId "Quercus" ;
    rdfs:subClassOf piirrite:OsmEntity ;
    skos:definition "Quercus is a genus of trees and shrubs, commonly known as oak."@en ;
    skos:inScheme piirritev:OsmGenus ;
    skos:prefLabel "Quercus"@en .

piirritev:OsmGenusRobinia a skos:Concept ;
    piirrite:osmId "Robinia" ;
    rdfs:subClassOf piirrite:OsmEntity ;
    skos:definition ""@en ;
    skos:inScheme piirritev:OsmGenus ;
    skos:prefLabel "Robinia"@en .

piirritev:OsmGenusSalix a skos:Concept ;
    piirrite:osmId "Salix" ;
    rdfs:subClassOf piirrite:OsmEntity ;
    skos:definition ""@en ;
    skos:inScheme piirritev:OsmGenus ;
    skos:prefLabel "Salix"@en .

piirritev:OsmGenusSorbus a skos:Concept ;
    piirrite:osmId "Sorbus" ;
    rdfs:subClassOf piirrite:OsmEntity ;
    skos:definition ""@en ;
    skos:inScheme piirritev:OsmGenus ;
    skos:prefLabel "Sorbus"@en .

piirritev:OsmGenusTilia a skos:Concept ;
    piirrite:osmId "Tilia" ;
    rdfs:subClassOf piirrite:OsmEntity ;
    skos:definition "Tilia is a genus of trees, commonly known as limetree."@en ;
    skos:inScheme piirritev:OsmGenus ;
    skos:prefLabel "Tilia"@en .

piirritev:OsmGenusUlmus a skos:Concept ;
    piirrite:osmId "Ulmus" ;
    rdfs:subClassOf piirrite:OsmEntity ;
    skos:definition ""@en ;
    skos:inScheme piirritev:OsmGenus ;
    skos:prefLabel "Ulmus"@en .

piirritev:OsmGolfBunker a skos:Concept ;
    piirrite:osmId "bunker" ;
    rdfs:subClassOf piirrite:OsmEntity ;
    skos:definition "A bunker of a golf course: a depression near the green or fairway that is usually filled with sand. osmcarto-rendering=File:Rendering-area-sand.png osmcarto-rendering-size=100px"@en ;
    skos:inScheme piirritev:OsmGolf ;
    skos:prefLabel "Bunker"@en .

piirritev:OsmGolfCartDesignated a skos:Concept ;
    piirrite:osmId "designated" ;
    rdfs:subClassOf piirrite:OsmEntity ;
    skos:definition ""@en ;
    skos:inScheme piirritev:OsmGolfCart ;
    skos:prefLabel "Designated"@en .

piirritev:OsmGolfCartpath a skos:Concept ;
    piirrite:osmId "cartpath" ;
    rdfs:subClassOf piirrite:OsmEntity ;
    skos:definition "Path for golf cart in golf course"@en ;
    skos:inScheme piirritev:OsmGolf ;
    skos:prefLabel "Cartpath"@en .

piirritev:OsmGolfFairway a skos:Concept ;
    piirrite:osmId "fairway" ;
    rdfs:subClassOf piirrite:OsmEntity ;
    skos:definition "Fairway of a golf course: an area between the tee box and the putting green where the grass is cut even and short. osmcarto-rendering=File:Landuse_grass.png osmcarto-rendering-size=125px"@en ;
    skos:inScheme piirritev:OsmGolf ;
    skos:prefLabel "Fairway"@en .

piirritev:OsmGolfHole a skos:Concept ;
    piirrite:hasRelatedOsmTag piirrite:hasOsmHoleHandicap,
        piirrite:hasOsmHoleName,
        piirrite:hasOsmHolePar,
        piirrite:hasOsmHoleRef ;
    piirrite:osmId "hole" ;
    rdfs:subClassOf piirrite:OsmEntity ;
    skos:definition "The path from tee area to the green osmcarto-rendering=File:Power_minor_line.png osmcarto-rendering-size=125px"@en ;
    skos:inScheme piirritev:OsmGolf ;
    skos:prefLabel "Hole"@en .

piirritev:OsmGolfPath a skos:Concept ;
    piirrite:osmId "path" ;
    rdfs:subClassOf piirrite:OsmEntity ;
    skos:definition "Walking Route Common in Links Style Golf."@en ;
    skos:inScheme piirritev:OsmGolf ;
    skos:prefLabel "Path"@en .

piirritev:OsmGolfPin a skos:Concept ;
    piirrite:osmId "pin" ;
    rdfs:subClassOf piirrite:OsmEntity ;
    skos:definition "The hole of a golf course osmcarto-rendering=File:Leisure-golf-pin.svg osmcarto-rendering-size=23px"@en ;
    skos:inScheme piirritev:OsmGolf ;
    skos:prefLabel "Pin"@en .

piirritev:OsmGolfRough a skos:Concept ;
    piirrite:osmId "rough" ;
    rdfs:subClassOf piirrite:OsmEntity ;
    skos:definition "The rough of a golf course: the area between the fairway or green and the out-of-bounds markers, where the grass there is cut higher and is often coarser. osmcarto-rendering=File:Golf-rough.png osmcarto-rendering-size=125px"@en ;
    skos:inScheme piirritev:OsmGolf ;
    skos:prefLabel "Rough"@en .

piirritev:OsmGolfTee a skos:Concept ;
    piirrite:osmId "tee" ;
    rdfs:subClassOf piirrite:OsmEntity ;
    skos:definition "Teeing ground: area where play begins on a golf hole. osmcarto-rendering=File:Landuse_grass.png osmcarto-rendering-size=125px"@en ;
    skos:inScheme piirritev:OsmGolf ;
    skos:prefLabel "Tee"@en .

piirritev:OsmGolfWaterHazard a skos:Concept ;
    piirrite:hasRelatedOsmTag piirrite:hasOsmWaterHazardNatural ;
    piirrite:osmId "water_hazard" ;
    rdfs:subClassOf piirrite:OsmEntity ;
    skos:definition "A water hazard at a golf course, usually marked by yellow stakes or lines."@en ;
    skos:inScheme piirritev:OsmGolf ;
    skos:prefLabel "Water hazard"@en .

piirritev:OsmGovernmentAdministrative a skos:Concept ;
    piirrite:hasRelatedOsmTag piirrite:hasOsmAdministrativeName,
        piirrite:hasOsmAdministrativeOpeningHours,
        piirrite:hasOsmAdministrativeWheelchair ;
    piirrite:osmId "administrative" ;
    rdfs:subClassOf piirrite:OsmEntity ;
    skos:definition "A government administrative office."@en ;
    skos:inScheme piirritev:OsmGovernment ;
    skos:prefLabel "Administrative"@en .

piirritev:OsmGtfsId a skos:ConceptScheme ;
    piirrite:osmId "gtfs_id" ;
    skos:definition "Using this tag is discouraged, use key:gtfs:stop_id, key:gtfs:route_id, key:gtfs:trip_id or key:gtfs:shape_id instead."@en ;
    skos:prefLabel "Gtfs id, types"@en .

piirritev:OsmHandrail a skos:ConceptScheme ;
    piirrite:osmId "handrail" ;
    skos:definition "Defines whether there is at least one handrail."@en ;
    skos:prefLabel "Handrail, types"@en .

piirritev:OsmHazmatDesignated a skos:Concept ;
    piirrite:osmId "designated" ;
    rdfs:subClassOf piirrite:OsmEntity ;
    skos:definition ""@en ;
    skos:inScheme piirritev:OsmHazmat ;
    skos:prefLabel "Designated"@en .

piirritev:OsmHeight a skos:ConceptScheme ;
    piirrite:osmId "height" ;
    skos:definition "Height is the measurement of vertical distance. It indicates how \"tall\" something is."@en ;
    skos:prefLabel "Height, types"@en .

piirritev:OsmHeritage a skos:ConceptScheme ;
    piirrite:osmId "heritage" ;
    skos:definition "Site/building/object registered by an official heritage organisation"@en ;
    skos:prefLabel "Heritage, types"@en .

piirritev:OsmHfcsMajorCollector a skos:Concept ;
    piirrite:osmId "Major_Collector" ;
    rdfs:subClassOf piirrite:OsmEntity ;
    skos:definition ""@en ;
    skos:inScheme piirritev:OsmHfcs ;
    skos:prefLabel "Major collector"@en .

piirritev:OsmHfcsPrincipalArterial a skos:Concept ;
    piirrite:osmId "Principal_Arterial" ;
    rdfs:subClassOf piirrite:OsmEntity ;
    skos:definition ""@en ;
    skos:inScheme piirritev:OsmHfcs ;
    skos:prefLabel "Principal arterial"@en .

piirritev:OsmHfcsUrbanCollector a skos:Concept ;
    piirrite:osmId "Urban_Collector" ;
    rdfs:subClassOf piirrite:OsmEntity ;
    skos:definition ""@en ;
    skos:inScheme piirritev:OsmHfcs ;
    skos:prefLabel "Urban collector"@en .

piirritev:OsmHgvDelivery a skos:Concept ;
    piirrite:osmId "delivery" ;
    rdfs:subClassOf piirrite:OsmEntity ;
    skos:definition ""@en ;
    skos:inScheme piirritev:OsmHgv ;
    skos:prefLabel "Delivery"@en .

piirritev:OsmHgvDesignated a skos:Concept ;
    piirrite:osmId "designated" ;
    rdfs:subClassOf piirrite:OsmEntity ;
    skos:definition ""@en ;
    skos:inScheme piirritev:OsmHgv ;
    skos:prefLabel "Designated"@en .

piirritev:OsmHgvDestination a skos:Concept ;
    piirrite:osmId "destination" ;
    rdfs:subClassOf piirrite:OsmEntity ;
    skos:definition ""@en ;
    skos:inScheme piirritev:OsmHgv ;
    skos:prefLabel "Destination"@en .

piirritev:OsmHgvLocal a skos:Concept ;
    piirrite:osmId "local" ;
    rdfs:subClassOf piirrite:OsmEntity ;
    skos:definition ""@en ;
    skos:inScheme piirritev:OsmHgv ;
    skos:prefLabel "Local"@en .

piirritev:OsmHighspeed a skos:ConceptScheme ;
    piirrite:osmId "highspeed" ;
    skos:definition "High-speed rail"@en ;
    skos:prefLabel "Highspeed, types"@en .

piirritev:OsmHighwayBridleway a skos:Concept ;
    piirrite:hasRelatedOsmTag piirrite:hasOsmBridlewayName ;
    piirrite:osmId "bridleway" ;
    rdfs:subClassOf piirrite:OsmEntity ;
    skos:definition "A way intended for use by equestrians. osmcarto-rendering=File:Rendering-highway bridleway.png osmcarto-rendering-size=125px"@en ;
    skos:inScheme piirritev:OsmHighway ;
    skos:prefLabel "Bridleway"@en .

piirritev:OsmHighwayBusStop a skos:Concept ;
    piirrite:hasRelatedOsmTag piirrite:hasOsmBusStopName,
        piirrite:hasOsmBusStopPublicTransport,
        piirrite:hasOsmBusStopShelter ;
    piirrite:osmId "bus_stop" ;
    rdfs:subClassOf piirrite:OsmEntity ;
    skos:definition "A bus stop is a place where public buses stop for passengers."@en ;
    skos:inScheme piirritev:OsmHighway ;
    skos:prefLabel "Bus stop"@en .

piirritev:OsmHighwayBusway a skos:Concept ;
    piirrite:hasRelatedOsmTag piirrite:hasOsmBuswayAccess,
        piirrite:hasOsmBuswayBicycle,
        piirrite:hasOsmBuswayBusBay,
        piirrite:hasOsmBuswayColour,
        piirrite:hasOsmBuswayEmbeddedRails,
        piirrite:hasOsmBuswayFoot,
        piirrite:hasOsmBuswayHighway,
        piirrite:hasOsmBuswayName,
        piirrite:hasOsmBuswayOperator,
        piirrite:hasOsmBuswayTrolleyWire ;
    piirrite:osmId "busway" ;
    rdfs:subClassOf piirrite:OsmEntity ;
    skos:definition "A dedicated, separate roadway for buses."@en ;
    skos:inScheme piirritev:OsmHighway ;
    skos:prefLabel "Busway"@en .

piirritev:OsmHighwayConstruction a skos:Concept ;
    piirrite:hasRelatedOsmTag piirrite:hasOsmConstructionCheckDate,
        piirrite:hasOsmConstructionOpeningDate,
        piirrite:hasOsmConstructionType ;
    piirrite:osmId "construction" ;
    rdfs:subClassOf piirrite:OsmEntity ;
    skos:definition "A highway (road, track or path) currently under construction.  osmcarto-rendering = File:Rendering-highway construction tertiary carto.png  osmcarto-rendering-size = 125px"@en ;
    skos:inScheme piirritev:OsmHighway ;
    skos:prefLabel "Construction"@en .

piirritev:OsmHighwayCorridor a skos:Concept ;
    piirrite:hasRelatedOsmTag piirrite:hasOsmCorridorAccess,
        piirrite:hasOsmCorridorConveying,
        piirrite:hasOsmCorridorLevel ;
    piirrite:osmId "corridor" ;
    rdfs:subClassOf piirrite:OsmEntity ;
    skos:definition "A corridor inside a building"@en ;
    skos:inScheme piirritev:OsmHighway ;
    skos:prefLabel "Corridor"@en .

piirritev:OsmHighwayCrossing a skos:Concept ;
    piirrite:hasRelatedOsmTag piirrite:hasOsmCrossingType ;
    piirrite:osmId "crossing" ;
    rdfs:subClassOf piirrite:OsmEntity ;
    skos:definition "The location of a street crossing for pedestrians, cyclists, or equestrians."@en ;
    skos:inScheme piirritev:OsmHighway ;
    skos:prefLabel "Crossing"@en .

piirritev:OsmHighwayCycleway a skos:Concept ;
    piirrite:hasRelatedOsmTag piirrite:hasOsmCyclewayLit,
        piirrite:hasOsmCyclewayName,
        piirrite:hasOsmCyclewaySegregated,
        piirrite:hasOsmCyclewaySurface,
        piirrite:hasOsmCyclewayWidth ;
    piirrite:osmId "cycleway" ;
    rdfs:subClassOf piirrite:OsmEntity ;
    skos:definition "For designated cycleways.  osmcarto-rendering = File:Cycleway osm.png  osmcarto-rendering-size = 125px"@en ;
    skos:inScheme piirritev:OsmHighway ;
    skos:prefLabel "Cycleway"@en .

piirritev:OsmHighwayElevator a skos:Concept ;
    piirrite:hasRelatedOsmTag piirrite:hasOsmElevatorAccess,
        piirrite:hasOsmElevatorBicycle,
        piirrite:hasOsmElevatorGoods,
        piirrite:hasOsmElevatorLevel,
        piirrite:hasOsmElevatorManufacturer,
        piirrite:hasOsmElevatorWheelchair ;
    piirrite:osmId "elevator" ;
    rdfs:subClassOf piirrite:OsmEntity ;
    skos:definition "An elevator (or lift) is used to travel vertically, providing passenger and freight access between pathways at different floor levels. May be solely vertical (typical case) or inclined. osmcarto-rendering=File:Elevator-12.svg osmcarto-rendering-size=24px"@en ;
    skos:inScheme piirritev:OsmHighway ;
    skos:prefLabel "Elevator"@en .

piirritev:OsmHighwayEmergencyBay a skos:Concept ;
    piirrite:osmId "emergency_bay" ;
    rdfs:subClassOf piirrite:OsmEntity ;
    skos:definition "An area beside a highway where you can safely stop your car in case of breakdown or emergency."@en ;
    skos:inScheme piirritev:OsmHighway ;
    skos:prefLabel "Emergency bay"@en .

piirritev:OsmHighwayFootway a skos:Concept ;
    piirrite:hasRelatedOsmTag piirrite:hasOsmFootwayAccess,
        piirrite:hasOsmFootwayBicycle,
        piirrite:hasOsmFootwayCovered,
        piirrite:hasOsmFootwayInformal,
        piirrite:hasOsmFootwayLit,
        piirrite:hasOsmFootwayName,
        piirrite:hasOsmFootwaySurface,
        piirrite:hasOsmFootwayTactilePaving,
        piirrite:hasOsmFootwayType,
        piirrite:hasOsmFootwayWheelchair ;
    piirrite:osmId "footway" ;
    rdfs:subClassOf piirrite:OsmEntity ;
    skos:definition "A path mainly or exclusively for pedestrians. osmcarto-rendering=File:Rendering-highway footway.png osmcarto-rendering-size=125px"@en ;
    skos:inScheme piirritev:OsmHighway ;
    skos:prefLabel "Footway"@en .

piirritev:OsmHighwayGiveWay a skos:Concept ;
    piirrite:hasRelatedOsmTag piirrite:hasOsmGiveWayDirection ;
    piirrite:osmId "give_way" ;
    rdfs:subClassOf piirrite:OsmEntity ;
    skos:definition "Used to mark give way (also known as yield) signs or markings."@en ;
    skos:inScheme piirritev:OsmHighway ;
    skos:prefLabel "Give way"@en .

piirritev:OsmHighwayLivingStreet a skos:Concept ;
    piirrite:osmId "living_street" ;
    rdfs:subClassOf piirrite:OsmEntity ;
    skos:definition "Road with very low speed limits and other pedestrian friendly traffic rules. osmcarto-rendering=File:Living street osm.png osmcarto-rendering-size=125px"@en ;
    skos:inScheme piirritev:OsmHighway ;
    skos:prefLabel "Living street"@en .

piirritev:OsmHighwayMilestone a skos:Concept ;
    piirrite:hasRelatedOsmTag piirrite:hasOsmMilestoneCarriagewayRef,
        piirrite:hasOsmMilestoneDistance,
        piirrite:hasOsmMilestoneMarker,
        piirrite:hasOsmMilestoneRef ;
    piirrite:osmId "milestone" ;
    rdfs:subClassOf piirrite:OsmEntity ;
    skos:definition "Stone or metal marker on the side of a road indicating a reference and an approximation of the distance travelled."@en ;
    skos:inScheme piirritev:OsmHighway ;
    skos:prefLabel "Milestone"@en .

piirritev:OsmHighwayMiniRoundabout a skos:Concept ;
    piirrite:hasRelatedOsmTag piirrite:hasOsmMiniRoundaboutDirection,
        piirrite:hasOsmMiniRoundaboutName ;
    piirrite:osmId "mini_roundabout" ;
    rdfs:subClassOf piirrite:OsmEntity ;
    skos:definition "A road junction where the traffic goes around a painted circle or traversable island and has right of way. osmcarto-rendering=File:Highway mini roundabout.svg osmcarto-rendering-size=18px"@en ;
    skos:inScheme piirritev:OsmHighway ;
    skos:prefLabel "Mini roundabout"@en .

piirritev:OsmHighwayMotorway a skos:Concept ;
    piirrite:hasRelatedOsmTag piirrite:hasOsmMotorwayDestination,
        piirrite:hasOsmMotorwayLanes,
        piirrite:hasOsmMotorwayName,
        piirrite:hasOsmMotorwayRef,
        piirrite:hasOsmMotorwayToll ;
    piirrite:osmId "motorway" ;
    rdfs:subClassOf piirrite:OsmEntity ;
    skos:definition "High capacity highways designed to safely carry fast motor traffic. osmcarto-rendering=File:Rendering-highway motorway carto.png osmcarto-rendering-size=125px"@en ;
    skos:inScheme piirritev:OsmHighway ;
    skos:prefLabel "Motorway"@en .

piirritev:OsmHighwayMotorwayJunction a skos:Concept ;
    piirrite:hasRelatedOsmTag piirrite:hasOsmMotorwayJunctionName,
        piirrite:hasOsmMotorwayJunctionRef ;
    piirrite:osmId "motorway_junction" ;
    rdfs:subClassOf piirrite:OsmEntity ;
    skos:definition "An exit from a motorway or other major road."@en ;
    skos:inScheme piirritev:OsmHighway ;
    skos:prefLabel "Motorway junction"@en .

piirritev:OsmHighwayMotorwayLink a skos:Concept ;
    piirrite:hasRelatedOsmTag piirrite:hasOsmMotorwayLinkDestination,
        piirrite:hasOsmMotorwayLinkMaxspeed ;
    piirrite:osmId "motorway_link" ;
    rdfs:subClassOf piirrite:OsmEntity ;
    skos:definition "The link roads (sliproads / ramps) leading to and from a motorway.  osmcarto-rendering = File:Rendering-highway motorway link.png  osmcarto-rendering-size = 125px"@en ;
    skos:inScheme piirritev:OsmHighway ;
    skos:prefLabel "Motorway link"@en .

piirritev:OsmHighwayPassingPlace a skos:Concept ;
    piirrite:osmId "passing_place" ;
    rdfs:subClassOf piirrite:OsmEntity ;
    skos:definition "A passing place on a single track road."@en ;
    skos:inScheme piirritev:OsmHighway ;
    skos:prefLabel "Passing place"@en .

piirritev:OsmHighwayPath a skos:Concept ;
    piirrite:hasRelatedOsmTag piirrite:hasOsmPathAccess,
        piirrite:hasOsmPathBicycle,
        piirrite:hasOsmPathFoot,
        piirrite:hasOsmPathHorse,
        piirrite:hasOsmPathLit,
        piirrite:hasOsmPathName,
        piirrite:hasOsmPathSacScale,
        piirrite:hasOsmPathSegregated,
        piirrite:hasOsmPathSmoothness,
        piirrite:hasOsmPathSurface,
        piirrite:hasOsmPathTrailVisibility,
        piirrite:hasOsmPathWidth ;
    piirrite:osmId "path" ;
    rdfs:subClassOf piirrite:OsmEntity ;
    skos:definition "A generic path used by pedestrians, small vehicles, for animal riding or livestock walking. Not designated for use by two-track vehicles. Unless subtagged very broad, non-specific meaning."@en ;
    skos:inScheme piirritev:OsmHighway ;
    skos:prefLabel "Path"@en .

piirritev:OsmHighwayPedestrian a skos:Concept ;
    piirrite:hasRelatedOsmTag piirrite:hasOsmPedestrianArea,
        piirrite:hasOsmPedestrianName,
        piirrite:hasOsmPedestrianRef ;
    piirrite:osmId "pedestrian" ;
    rdfs:subClassOf piirrite:OsmEntity ;
    skos:definition "Roads mainly / exclusively for pedestrians osmcarto-rendering=File:Pedestrian with area osm.png osmcarto-rendering-size=125px osmcarto-rendering-area=File:Highway pedestrian footway path area.png osmcarto-rendering-area-size=125px"@en ;
    skos:inScheme piirritev:OsmHighway ;
    skos:prefLabel "Pedestrian"@en .

piirritev:OsmHighwayPlatform a skos:Concept ;
    piirrite:hasRelatedOsmTag piirrite:hasOsmPlatformBench,
        piirrite:hasOsmPlatformBin,
        piirrite:hasOsmPlatformName,
        piirrite:hasOsmPlatformOperator,
        piirrite:hasOsmPlatformRef,
        piirrite:hasOsmPlatformRouteRef,
        piirrite:hasOsmPlatformShelter,
        piirrite:hasOsmPlatformWheelchair ;
    piirrite:osmId "platform" ;
    rdfs:subClassOf piirrite:OsmEntity ;
    skos:definition "A platform at a bus stop or station. osmcarto-rendering-way=File:Rendering-highway_railway_platform_line.png osmcarto-rendering-way-size=125px osmcarto-rendering-area=File:Rendering-highway_railway_platform_area.png osmcarto-rendering-area-size=125px"@en ;
    skos:inScheme piirritev:OsmHighway ;
    skos:prefLabel "Platform"@en .

piirritev:OsmHighwayPrimary a skos:Concept ;
    piirrite:hasRelatedOsmTag piirrite:hasOsmPrimaryBridge,
        piirrite:hasOsmPrimaryDualCarriageway,
        piirrite:hasOsmPrimaryFrom,
        piirrite:hasOsmPrimaryIntRef,
        piirrite:hasOsmPrimaryLanes,
        piirrite:hasOsmPrimaryLit,
        piirrite:hasOsmPrimaryMaxspeed,
        piirrite:hasOsmPrimaryMinspeed,
        piirrite:hasOsmPrimaryMotorroad,
        piirrite:hasOsmPrimaryName,
        piirrite:hasOsmPrimaryOldRef,
        piirrite:hasOsmPrimaryOneway,
        piirrite:hasOsmPrimaryOperator,
        piirrite:hasOsmPrimaryRef,
        piirrite:hasOsmPrimarySurface,
        piirrite:hasOsmPrimaryTo,
        piirrite:hasOsmPrimaryTunnel ;
    piirrite:osmId "primary" ;
    rdfs:subClassOf piirrite:OsmEntity ;
    skos:definition "A major highway linking large towns. In cities, a major arterial road. osmcarto-rendering=File:Rendering-highway primary carto.png osmcarto-rendering-size=125px"@en ;
    skos:inScheme piirritev:OsmHighway ;
    skos:prefLabel "Primary"@en .

piirritev:OsmHighwayPrimaryLink a skos:Concept ;
    piirrite:hasRelatedOsmTag piirrite:hasOsmPrimaryLinkDestination,
        piirrite:hasOsmPrimaryLinkMaxspeed,
        piirrite:hasOsmPrimaryLinkOneway ;
    piirrite:osmId "primary_link" ;
    rdfs:subClassOf piirrite:OsmEntity ;
    skos:definition "Connecting slip roads/ramps of primary highways osmcarto-rendering=File:Rendering-highway primary link.png osmcarto-rendering-size=125px"@en ;
    skos:inScheme piirritev:OsmHighway ;
    skos:prefLabel "Primary link"@en .

piirritev:OsmHighwayProposed a skos:Concept ;
    piirrite:hasRelatedOsmTag piirrite:hasOsmProposedType ;
    piirrite:osmId "proposed" ;
    rdfs:subClassOf piirrite:OsmEntity ;
    skos:definition "A road that is about to be built, but where any construction work hasn't yet been started."@en ;
    skos:inScheme piirritev:OsmHighway ;
    skos:prefLabel "Proposed"@en .

piirritev:OsmHighwayRaceway a skos:Concept ;
    piirrite:hasRelatedOsmTag piirrite:hasOsmRacewaySport ;
    piirrite:osmId "raceway" ;
    rdfs:subClassOf piirrite:OsmEntity ;
    skos:definition "A racetrack for motorised racing, e.g. cars, motorbikes and karts. osmcarto-rendering=File:Rendering-highway-raceway-mapnik.png osmcarto-rendering-size=125px"@en ;
    skos:inScheme piirritev:OsmHighway ;
    skos:prefLabel "Raceway"@en .

piirritev:OsmHighwayResidential a skos:Concept ;
    piirrite:hasRelatedOsmTag piirrite:hasOsmResidentialAccess,
        piirrite:hasOsmResidentialName,
        piirrite:hasOsmResidentialOneway,
        piirrite:hasOsmResidentialSurface ;
    piirrite:osmId "residential" ;
    rdfs:subClassOf piirrite:OsmEntity ;
    skos:definition "Road in a residential area osmcarto-rendering=File:Rendering-highway residential.png osmcarto-rendering-size=125px"@en ;
    skos:inScheme piirritev:OsmHighway ;
    skos:prefLabel "Residential"@en .

piirritev:OsmHighwayRestArea a skos:Concept ;
    piirrite:hasRelatedOsmTag piirrite:hasOsmRestAreaName,
        piirrite:hasOsmRestAreaOperator,
        piirrite:hasOsmRestAreaToilets ;
    piirrite:osmId "rest_area" ;
    rdfs:subClassOf piirrite:OsmEntity ;
    skos:definition "Place where drivers can leave the road to rest, but not refuel. osmcarto-rendering=File:Rendering-highway services.png osmcarto-rendering-size=100px"@en ;
    skos:inScheme piirritev:OsmHighway ;
    skos:prefLabel "Rest area"@en .

piirritev:OsmHighwayRoad a skos:Concept ;
    piirrite:hasRelatedOsmTag piirrite:hasOsmRoadName,
        piirrite:hasOsmRoadOneway ;
    piirrite:osmId "road" ;
    rdfs:subClassOf piirrite:OsmEntity ;
    skos:definition "Road with unknown classification. osmcarto-rendering=File:Rendering-highway-road-mapnik.png osmcarto-rendering-size=125px"@en ;
    skos:inScheme piirritev:OsmHighway ;
    skos:prefLabel "Road"@en .

piirritev:OsmHighwaySecondary a skos:Concept ;
    piirrite:hasRelatedOsmTag piirrite:hasOsmSecondaryName,
        piirrite:hasOsmSecondaryRef ;
    piirrite:osmId "secondary" ;
    rdfs:subClassOf piirrite:OsmEntity ;
    skos:definition "A highway linking large towns. In cities, an arterial road of lesser importance. osmcarto-rendering=File:Rendering-highway secondary carto.png osmcarto-rendering-size=125px"@en ;
    skos:inScheme piirritev:OsmHighway ;
    skos:prefLabel "Secondary"@en .

piirritev:OsmHighwaySecondaryLink a skos:Concept ;
    piirrite:hasRelatedOsmTag piirrite:hasOsmSecondaryLinkOneway ;
    piirrite:osmId "secondary_link" ;
    rdfs:subClassOf piirrite:OsmEntity ;
    skos:definition "Connecting slip roads/ramps of secondary highways osmcarto-rendering = File:Rendering-highway secondary link.png osmcarto-rendering-size = 125px"@en ;
    skos:inScheme piirritev:OsmHighway ;
    skos:prefLabel "Secondary link"@en .

piirritev:OsmHighwayService a skos:Concept ;
    piirrite:hasRelatedOsmTag piirrite:hasOsmServiceAccess,
        piirrite:hasOsmServiceCovered,
        piirrite:hasOsmServiceLit,
        piirrite:hasOsmServiceLivingStreet,
        piirrite:hasOsmServiceMaxspeed,
        piirrite:hasOsmServiceName,
        piirrite:hasOsmServiceOneway,
        piirrite:hasOsmServiceSurface,
        piirrite:hasOsmServiceTunnel,
        piirrite:hasOsmServiceType ;
    piirrite:osmId "service" ;
    rdfs:subClassOf piirrite:OsmEntity ;
    skos:definition "Provides access to a building, service station, beach, campsite, industrial estate, business park, etc. osmcarto-rendering=File:Rendering-highway service.png osmcarto-rendering-size=125px"@en ;
    skos:inScheme piirritev:OsmHighway ;
    skos:prefLabel "Service"@en .

piirritev:OsmHighwayServices a skos:Concept ;
    piirrite:hasRelatedOsmTag piirrite:hasOsmServicesName,
        piirrite:hasOsmServicesOperator ;
    piirrite:osmId "services" ;
    rdfs:subClassOf piirrite:OsmEntity ;
    skos:definition "Place where drivers can leave a road to refuel, rest, or take refreshments. osmcarto-rendering=File:Rendering-highway services.png osmcarto-rendering-size=100px"@en ;
    skos:inScheme piirritev:OsmHighway ;
    skos:prefLabel "Services"@en .

piirritev:OsmHighwaySpeedCamera a skos:Concept ;
    piirrite:hasRelatedOsmTag piirrite:hasOsmSpeedCameraColour,
        piirrite:hasOsmSpeedCameraDirection,
        piirrite:hasOsmSpeedCameraMaxspeed,
        piirrite:hasOsmSpeedCameraOperator,
        piirrite:hasOsmSpeedCameraRef ;
    piirrite:osmId "speed_camera" ;
    rdfs:subClassOf piirrite:OsmEntity ;
    skos:definition "A fixed road-side or overhead speed camera."@en ;
    skos:inScheme piirritev:OsmHighway ;
    skos:prefLabel "Speed camera"@en .

piirritev:OsmHighwaySteps a skos:Concept ;
    piirrite:hasRelatedOsmTag piirrite:hasOsmStepsConveying,
        piirrite:hasOsmStepsIncline,
        piirrite:hasOsmStepsRamp,
        piirrite:hasOsmStepsStepCount ;
    piirrite:osmId "steps" ;
    rdfs:subClassOf piirrite:OsmEntity ;
    skos:definition "For flights of steps on footways and paths. osmcarto-rendering=File:Rendering-highway steps.png osmcarto-rendering-size=125px"@en ;
    skos:inScheme piirritev:OsmHighway ;
    skos:prefLabel "Steps"@en .

piirritev:OsmHighwayStop a skos:Concept ;
    piirrite:hasRelatedOsmTag piirrite:hasOsmStopDirection,
        piirrite:hasOsmStopType ;
    piirrite:osmId "stop" ;
    rdfs:subClassOf piirrite:OsmEntity ;
    skos:definition "A point at which a vehicle must come to a complete stop."@en ;
    skos:inScheme piirritev:OsmHighway ;
    skos:prefLabel "Stop"@en .

piirritev:OsmHighwayStreetLamp a skos:Concept ;
    piirrite:hasRelatedOsmTag piirrite:hasOsmStreetLampLampModel,
        piirrite:hasOsmStreetLampLampMount,
        piirrite:hasOsmStreetLampLampType ;
    piirrite:osmId "street_lamp" ;
    rdfs:subClassOf piirrite:OsmEntity ;
    skos:definition "A single pole with one or more lights to illuminate the street."@en ;
    skos:inScheme piirritev:OsmHighway ;
    skos:prefLabel "Street lamp"@en .

piirritev:OsmHighwayTertiary a skos:Concept ;
    piirrite:hasRelatedOsmTag piirrite:hasOsmTertiaryCycleway,
        piirrite:hasOsmTertiaryEmbeddedRails,
        piirrite:hasOsmTertiaryEstWidth,
        piirrite:hasOsmTertiaryLaneMarkings,
        piirrite:hasOsmTertiaryLanes,
        piirrite:hasOsmTertiaryLit,
        piirrite:hasOsmTertiaryLocName,
        piirrite:hasOsmTertiaryMaxspeed,
        piirrite:hasOsmTertiaryMaxweight,
        piirrite:hasOsmTertiaryName,
        piirrite:hasOsmTertiaryOldName,
        piirrite:hasOsmTertiaryOneway,
        piirrite:hasOsmTertiaryRef,
        piirrite:hasOsmTertiarySidewalk,
        piirrite:hasOsmTertiarySurface,
        piirrite:hasOsmTertiaryWidth,
        piirrite:hasOsmTertiaryWinterService ;
    piirrite:osmId "tertiary" ;
    rdfs:subClassOf piirrite:OsmEntity ;
    skos:definition "A road linking small settlements, or the local centres of a large town or city. osmcarto-rendering=File:Rendering-highway tertiary carto.png osmcarto-rendering-size=125px"@en ;
    skos:inScheme piirritev:OsmHighway ;
    skos:prefLabel "Tertiary"@en .

piirritev:OsmHighwayTertiaryLink a skos:Concept ;
    piirrite:hasRelatedOsmTag piirrite:hasOsmTertiaryLinkOneway ;
    piirrite:osmId "tertiary_link" ;
    rdfs:subClassOf piirrite:OsmEntity ;
    skos:definition "Connecting slip road/ramp of a tertiary highway. osmcarto-rendering=File:Rendering-highway tertiary link.png osmcarto-rendering-size=125px"@en ;
    skos:inScheme piirritev:OsmHighway ;
    skos:prefLabel "Tertiary link"@en .

piirritev:OsmHighwayTrack a skos:Concept ;
    piirrite:hasRelatedOsmTag piirrite:hasOsmTrackAccess,
        piirrite:hasOsmTrackName,
        piirrite:hasOsmTrackRef,
        piirrite:hasOsmTrackSmoothness,
        piirrite:hasOsmTrackSurface,
        piirrite:hasOsmTrackTracktype,
        piirrite:hasOsmTrackWidth ;
    piirrite:osmId "track" ;
    rdfs:subClassOf piirrite:OsmEntity ;
    skos:definition "A minor land-access road like a farm or forest track. osmcarto-rendering=File:Mapnik-tracktype-not-set.png osmcarto-rendering-size=125px"@en ;
    skos:inScheme piirritev:OsmHighway ;
    skos:prefLabel "Track"@en .

piirritev:OsmHighwayTrafficMirror a skos:Concept ;
    piirrite:osmId "traffic_mirror" ;
    rdfs:subClassOf piirrite:OsmEntity ;
    skos:definition "Mirror that reflects the traffic on one road when direct view is blocked."@en ;
    skos:inScheme piirritev:OsmHighway ;
    skos:prefLabel "Traffic mirror"@en .

piirritev:OsmHighwayTrafficSignals a skos:Concept ;
    piirrite:hasRelatedOsmTag piirrite:hasOsmTrafficSignalsName,
        piirrite:hasOsmTrafficSignalsRef ;
    piirrite:osmId "traffic_signals" ;
    rdfs:subClassOf piirrite:OsmEntity ;
    skos:definition "A traffic signal (or a set of those) for regulating circulation. osmcarto-rendering=File:Traffic light-16.svg osmcarto-rendering-size=28px"@en ;
    skos:inScheme piirritev:OsmHighway ;
    skos:prefLabel "Traffic signals"@en .

piirritev:OsmHighwayTrailhead a skos:Concept ;
    piirrite:hasRelatedOsmTag piirrite:hasOsmTrailheadName,
        piirrite:hasOsmTrailheadOperator ;
    piirrite:osmId "trailhead" ;
    rdfs:subClassOf piirrite:OsmEntity ;
    skos:definition "A trailhead is a designated or customary place where a trip on a trail begins or ends."@en ;
    skos:inScheme piirritev:OsmHighway ;
    skos:prefLabel "Trailhead"@en .

piirritev:OsmHighwayTrunk a skos:Concept ;
    piirrite:hasRelatedOsmTag piirrite:hasOsmTrunkDestination,
        piirrite:hasOsmTrunkExpressway,
        piirrite:hasOsmTrunkLanes,
        piirrite:hasOsmTrunkMotorroad,
        piirrite:hasOsmTrunkName,
        piirrite:hasOsmTrunkOneway,
        piirrite:hasOsmTrunkRef ;
    piirrite:osmId "trunk" ;
    rdfs:subClassOf piirrite:OsmEntity ;
    skos:definition "An important road that is not a motorway. osmcarto-rendering=File:Rendering-highway trunk carto.png osmcarto-rendering-size=125px"@en ;
    skos:inScheme piirritev:OsmHighway ;
    skos:prefLabel "Trunk"@en .

piirritev:OsmHighwayTrunkLink a skos:Concept ;
    piirrite:hasRelatedOsmTag piirrite:hasOsmTrunkLinkOneway,
        piirrite:hasOsmTrunkLinkRef ;
    piirrite:osmId "trunk_link" ;
    rdfs:subClassOf piirrite:OsmEntity ;
    skos:definition "The link road (sliproad / ramp) leading to and from a trunk highway. osmcarto-rendering=File:Rendering-highway trunk link.png osmcarto-rendering-size=125px"@en ;
    skos:inScheme piirritev:OsmHighway ;
    skos:prefLabel "Trunk link"@en .

piirritev:OsmHighwayTurningCircle a skos:Concept ;
    piirrite:hasRelatedOsmTag piirrite:hasOsmTurningCircleDiameter,
        piirrite:hasOsmTurningCircleName ;
    piirrite:osmId "turning_circle" ;
    rdfs:subClassOf piirrite:OsmEntity ;
    skos:definition "A widened area of road that allows vehicles to turn more easily. osmcarto-rendering=File:Mapping-Features-Turning-Circle.png osmcarto-rendering-size=100px"@en ;
    skos:inScheme piirritev:OsmHighway ;
    skos:prefLabel "Turning circle"@en .

piirritev:OsmHighwayTurningLoop a skos:Concept ;
    piirrite:osmId "turning_loop" ;
    rdfs:subClassOf piirrite:OsmEntity ;
    skos:definition "A widened area of a highway with a non-traversable island for turning around, often circular and at the end of a road."@en ;
    skos:inScheme piirritev:OsmHighway ;
    skos:prefLabel "Turning loop"@en .

piirritev:OsmHighwayUnclassified a skos:Concept ;
    piirrite:hasRelatedOsmTag piirrite:hasOsmUnclassifiedAbutters,
        piirrite:hasOsmUnclassifiedLanes,
        piirrite:hasOsmUnclassifiedLit,
        piirrite:hasOsmUnclassifiedName,
        piirrite:hasOsmUnclassifiedOneway,
        piirrite:hasOsmUnclassifiedSidewalk,
        piirrite:hasOsmUnclassifiedSurface ;
    piirrite:osmId "unclassified" ;
    rdfs:subClassOf piirrite:OsmEntity ;
    skos:definition "Public access road, non-residential. osmcarto-rendering=File:Rendering-highway unclassified.png osmcarto-rendering-size=125px"@en ;
    skos:inScheme piirritev:OsmHighway ;
    skos:prefLabel "Unclassified"@en .

piirritev:OsmHiking a skos:ConceptScheme ;
    piirrite:osmId "hiking" ;
    skos:definition "Information for hikers here."@en ;
    skos:prefLabel "Hiking, types"@en .

piirritev:OsmHorseDesignated a skos:Concept ;
    piirrite:osmId "designated" ;
    rdfs:subClassOf piirrite:OsmEntity ;
    skos:definition ""@en ;
    skos:inScheme piirritev:OsmHorse ;
    skos:prefLabel "Designated"@en .

piirritev:OsmHorsePermissive a skos:Concept ;
    piirrite:osmId "permissive" ;
    rdfs:subClassOf piirrite:OsmEntity ;
    skos:definition ""@en ;
    skos:inScheme piirritev:OsmHorse ;
    skos:prefLabel "Permissive"@en .

piirritev:OsmHorsePrivate a skos:Concept ;
    piirrite:osmId "private" ;
    rdfs:subClassOf piirrite:OsmEntity ;
    skos:definition ""@en ;
    skos:inScheme piirritev:OsmHorse ;
    skos:prefLabel "Private"@en .

piirritev:OsmHouseBungalow a skos:Concept ;
    piirrite:osmId "bungalow" ;
    rdfs:subClassOf piirrite:OsmEntity ;
    skos:definition "Simple single-storey house, sometimes with a second storey built into a sloped roof."@en ;
    skos:inScheme piirritev:OsmHouse ;
    skos:prefLabel "Bungalow"@en .

piirritev:OsmHouseDetached a skos:Concept ;
    piirrite:osmId "detached" ;
    rdfs:subClassOf piirrite:OsmEntity ;
    skos:definition "A detached house is a freestanding residential building usually housing a single family."@en ;
    skos:inScheme piirritev:OsmHouse ;
    skos:prefLabel "Detached"@en .

piirritev:OsmHouseResidential a skos:Concept ;
    piirrite:osmId "residential" ;
    rdfs:subClassOf piirrite:OsmEntity ;
    skos:definition ""@en ;
    skos:inScheme piirritev:OsmHouse ;
    skos:prefLabel "Residential"@en .

piirritev:OsmHouseSemi-Detached a skos:Concept ;
    piirrite:osmId "semi-detached" ;
    rdfs:subClassOf piirrite:OsmEntity ;
    skos:definition "A house that is attached to another house on one side."@en ;
    skos:inScheme piirritev:OsmHouse ;
    skos:prefLabel "Semi-detached"@en .

piirritev:OsmHouseTerrace a skos:Concept ;
    piirrite:hasRelatedOsmTag piirrite:hasOsmTerraceBuilding ;
    piirrite:osmId "terrace" ;
    rdfs:subClassOf piirrite:OsmEntity ;
    skos:definition "Used in addition to tag:building=house on the outline of a linear row of residential dwellings, each of which normally has its own entrance, which form a terrace (\"row-house\" or \"townhouse\" in North American English)."@en ;
    skos:inScheme piirritev:OsmHouse ;
    skos:prefLabel "Terrace"@en .

piirritev:OsmHouseTerraced a skos:Concept ;
    piirrite:osmId "terraced" ;
    rdfs:subClassOf piirrite:OsmEntity ;
    skos:definition "Used in addition to tag:building=house to map the individual units in a terrace. Preferred over mapping the whole terrace as one building."@en ;
    skos:inScheme piirritev:OsmHouse ;
    skos:prefLabel "Terraced"@en .

piirritev:OsmImage a skos:ConceptScheme ;
    piirrite:osmId "image" ;
    skos:definition "Reference to an image of the object."@en ;
    skos:prefLabel "Image, types"@en .

piirritev:OsmImportBudovy201004 a skos:Concept ;
    piirrite:osmId "budovy201004" ;
    rdfs:subClassOf piirrite:OsmEntity ;
    skos:definition ""@en ;
    skos:inScheme piirritev:OsmImport ;
    skos:prefLabel "Budovy201004"@en .

piirritev:OsmImportBudovy201004Drev a skos:Concept ;
    piirrite:osmId "budovy201004drev" ;
    rdfs:subClassOf piirrite:OsmEntity ;
    skos:definition ""@en ;
    skos:inScheme piirritev:OsmImport ;
    skos:prefLabel "Budovy201004drev"@en .

piirritev:OsmImportFreemapkapor a skos:Concept ;
    piirrite:osmId "freemapkapor" ;
    rdfs:subClassOf piirrite:OsmEntity ;
    skos:definition ""@en ;
    skos:inScheme piirritev:OsmImport ;
    skos:prefLabel "Freemapkapor"@en .

piirritev:OsmImportGrabremote a skos:Concept ;
    piirrite:osmId "grabremote" ;
    rdfs:subClassOf piirrite:OsmEntity ;
    skos:definition ""@en ;
    skos:inScheme piirritev:OsmImport ;
    skos:prefLabel "Grabremote"@en .

piirritev:OsmInclineDown a skos:Concept ;
    piirrite:hasRelatedOsmTag piirrite:hasOsmDownHighway ;
    piirrite:osmId "down" ;
    rdfs:subClassOf piirrite:OsmEntity ;
    skos:definition "General direction of incline for ways going down the hill"@en ;
    skos:inScheme piirritev:OsmIncline ;
    skos:prefLabel "Down"@en .

piirritev:OsmInclineUp a skos:Concept ;
    piirrite:hasRelatedOsmTag piirrite:hasOsmUpHighway ;
    piirrite:osmId "up" ;
    rdfs:subClassOf piirrite:OsmEntity ;
    skos:definition "General direction of incline for ways going up the hill"@en ;
    skos:inScheme piirritev:OsmIncline ;
    skos:prefLabel "Up"@en .

piirritev:OsmIndoorArea a skos:Concept ;
    piirrite:hasRelatedOsmTag piirrite:hasOsmAreaAccess,
        piirrite:hasOsmAreaName,
        piirrite:hasOsmAreaRef,
        piirrite:hasOsmAreaWheelchair ;
    piirrite:osmId "area" ;
    rdfs:subClassOf piirrite:OsmEntity ;
    skos:definition "An indoor area without walls along at least some of its edges."@en ;
    skos:inScheme piirritev:OsmIndoor ;
    skos:prefLabel "Area"@en .

piirritev:OsmIndoorColumn a skos:Concept ;
    piirrite:hasRelatedOsmTag piirrite:hasOsmColumnLevel ;
    piirrite:osmId "column" ;
    rdfs:subClassOf piirrite:OsmEntity ;
    skos:definition "A column that is part of the structure of the building."@en ;
    skos:inScheme piirritev:OsmIndoor ;
    skos:prefLabel "Column"@en .

piirritev:OsmIndoorCorridor a skos:Concept ;
    piirrite:hasRelatedOsmTag piirrite:hasOsmCorridorName,
        piirrite:hasOsmCorridorRef ;
    piirrite:osmId "corridor" ;
    rdfs:subClassOf piirrite:OsmEntity ;
    skos:definition "Enclosed walkway area that connects rooms."@en ;
    skos:inScheme piirritev:OsmIndoor ;
    skos:prefLabel "Corridor"@en .

piirritev:OsmIndoorDoor a skos:Concept ;
    piirrite:hasRelatedOsmTag piirrite:hasOsmDoorAccess,
        piirrite:hasOsmDoorLevel,
        piirrite:hasOsmDoorOpen,
        piirrite:hasOsmDoorOpening,
        piirrite:hasOsmDoorRef,
        piirrite:hasOsmDoorType,
        piirrite:hasOsmDoorWheelchair ;
    piirrite:osmId "door" ;
    rdfs:subClassOf piirrite:OsmEntity ;
    skos:definition "A swinging or sliding barrier that closes off rooms within a building"@en ;
    skos:inScheme piirritev:OsmIndoor ;
    skos:prefLabel "Door"@en .

piirritev:OsmIndoorRoom a skos:Concept ;
    piirrite:hasRelatedOsmTag piirrite:hasOsmRoomAccess,
        piirrite:hasOsmRoomName,
        piirrite:hasOsmRoomRef,
        piirrite:hasOsmRoomType,
        piirrite:hasOsmRoomWheelchair ;
    piirrite:osmId "room" ;
    rdfs:subClassOf piirrite:OsmEntity ;
    skos:definition "Conventional room with walls"@en ;
    skos:inScheme piirritev:OsmIndoor ;
    skos:prefLabel "Room"@en .

piirritev:OsmIndoorSeating a skos:ConceptScheme ;
    piirrite:osmId "indoor_seating" ;
    skos:definition "To indicate if a restaurant offers indoor seating."@en ;
    skos:prefLabel "Indoor seating, types"@en .

piirritev:OsmIndoorWall a skos:Concept ;
    piirrite:osmId "wall" ;
    rdfs:subClassOf piirrite:OsmEntity ;
    skos:definition "Individual (non-passable) wall element"@en ;
    skos:inScheme piirritev:OsmIndoor ;
    skos:prefLabel "Wall"@en .

piirritev:OsmIndustrialDepot a skos:Concept ;
    piirrite:hasRelatedOsmTag piirrite:hasOsmDepotName,
        piirrite:hasOsmDepotType ;
    piirrite:osmId "depot" ;
    rdfs:subClassOf piirrite:OsmEntity ;
    skos:definition "A place where vehicles are stored and served."@en ;
    skos:inScheme piirritev:OsmIndustrial ;
    skos:prefLabel "Depot"@en .

piirritev:OsmIndustrialFactory a skos:Concept ;
    piirrite:hasRelatedOsmTag piirrite:hasOsmFactoryName,
        piirrite:hasOsmFactoryProduct ;
    piirrite:osmId "factory" ;
    rdfs:subClassOf piirrite:OsmEntity ;
    skos:definition "Industrial area with factories."@en ;
    skos:inScheme piirritev:OsmIndustrial ;
    skos:prefLabel "Factory"@en .

piirritev:OsmIndustrialGrindingMill a skos:Concept ;
    piirrite:osmId "grinding_mill" ;
    rdfs:subClassOf piirrite:OsmEntity ;
    skos:definition "A device that breaks solid materials into smaller pieces by grinding, crushing, or cutting. The aftermath is powdered product, not liquid extract like oil mill."@en ;
    skos:inScheme piirritev:OsmIndustrial ;
    skos:prefLabel "Grinding mill"@en .

piirritev:OsmIndustrialOil a skos:Concept ;
    piirrite:osmId "oil" ;
    rdfs:subClassOf piirrite:OsmEntity ;
    skos:definition "Oil industry - includes the global processes of exploration, extraction, refining, and marketing petroleum products."@en ;
    skos:inScheme piirritev:OsmIndustrial ;
    skos:prefLabel "Oil"@en .

piirritev:OsmIndustrialScrapYard a skos:Concept ;
    piirrite:hasRelatedOsmTag piirrite:hasOsmScrapYardName ;
    piirrite:osmId "scrap_yard" ;
    rdfs:subClassOf piirrite:OsmEntity ;
    skos:definition "Place where decommissioned vehicles are brought for dismantling."@en ;
    skos:inScheme piirritev:OsmIndustrial ;
    skos:prefLabel "Scrap yard"@en .

piirritev:OsmIndustrialWellsite a skos:Concept ;
    piirrite:hasRelatedOsmTag piirrite:hasOsmWellsiteName,
        piirrite:hasOsmWellsiteOperator ;
    piirrite:osmId "wellsite" ;
    rdfs:subClassOf piirrite:OsmEntity ;
    skos:definition "A cleared area around oil wells for drilling rigs."@en ;
    skos:inScheme piirritev:OsmIndustrial ;
    skos:prefLabel "Wellsite"@en .

piirritev:OsmInformal a skos:ConceptScheme ;
    piirrite:osmId "informal" ;
    skos:definition "Indicates whether the feature was intentionally planned or formally set up."@en ;
    skos:prefLabel "Informal, types"@en .

piirritev:OsmInformationBoard a skos:Concept ;
    piirrite:hasRelatedOsmTag piirrite:hasOsmBoardBoardType,
        piirrite:hasOsmBoardName,
        piirrite:hasOsmBoardNetwork ;
    piirrite:osmId "board" ;
    rdfs:subClassOf piirrite:OsmEntity ;
    skos:definition "An information board."@en ;
    skos:inScheme piirritev:OsmInformation ;
    skos:prefLabel "Board"@en .

piirritev:OsmInformationGuidepost a skos:Concept ;
    piirrite:hasRelatedOsmTag piirrite:hasOsmGuidepostEle,
        piirrite:hasOsmGuidepostName,
        piirrite:hasOsmGuidepostRef ;
    piirrite:osmId "guidepost" ;
    rdfs:subClassOf piirrite:OsmEntity ;
    skos:definition "Used to mark a guidepost/signpost osmcarto-rendering=File:Guidepost-14.svg osmcarto-rendering-size=24px"@en ;
    skos:inScheme piirritev:OsmInformation ;
    skos:prefLabel "Guidepost"@en .

piirritev:OsmInformationMap a skos:Concept ;
    piirrite:hasRelatedOsmTag piirrite:hasOsmMapBicycle,
        piirrite:hasOsmMapHiking,
        piirrite:hasOsmMapHorse,
        piirrite:hasOsmMapMapSize,
        piirrite:hasOsmMapMapSource,
        piirrite:hasOsmMapMapType,
        piirrite:hasOsmMapMtb,
        piirrite:hasOsmMapSki,
        piirrite:hasOsmMapTourism ;
    piirrite:osmId "map" ;
    rdfs:subClassOf piirrite:OsmEntity ;
    skos:definition "A board with a map. osmcarto-rendering=File:Map-14.svg osmcarto-rendering-size=28px"@en ;
    skos:inScheme piirritev:OsmInformation ;
    skos:prefLabel "Map"@en .

piirritev:OsmInformationOffice a skos:Concept ;
    piirrite:hasRelatedOsmTag piirrite:hasOsmOfficeName,
        piirrite:hasOsmOfficeOpeningHours,
        piirrite:hasOsmOfficeOperator,
        piirrite:hasOsmOfficeWebsite,
        piirrite:hasOsmOfficeWheelchair ;
    piirrite:osmId "office" ;
    rdfs:subClassOf piirrite:OsmEntity ;
    skos:definition "An office where you can get information about a town or region. osmcarto-rendering=File:Office-14.svg osmcarto-rendering-size=28px"@en ;
    skos:inScheme piirritev:OsmInformation ;
    skos:prefLabel "Office"@en .

piirritev:OsmInformationRouteMarker a skos:Concept ;
    piirrite:osmId "route_marker" ;
    rdfs:subClassOf piirrite:OsmEntity ;
    skos:definition "A marker that shows the position of the way of a route. Could be a symbol, a short pole or a painted marking."@en ;
    skos:inScheme piirritev:OsmInformation ;
    skos:prefLabel "Route marker"@en .

piirritev:OsmInformationTerminal a skos:Concept ;
    piirrite:hasRelatedOsmTag piirrite:hasOsmTerminalSupport ;
    piirrite:osmId "terminal" ;
    rdfs:subClassOf piirrite:OsmEntity ;
    skos:definition "A information terminal osmcarto-rendering=File:Terminal-14.svg osmcarto-rendering-size=28px"@en ;
    skos:inScheme piirritev:OsmInformation ;
    skos:prefLabel "Terminal"@en .

piirritev:OsmInformationTrailBlaze a skos:Concept ;
    piirrite:osmId "trail_blaze" ;
    rdfs:subClassOf piirrite:OsmEntity ;
    skos:definition "A marker that shows the position of the way of a route. Could be a symbol, a short pole or a painted marking."@en ;
    skos:inScheme piirritev:OsmInformation ;
    skos:prefLabel "Trail blaze"@en .

piirritev:OsmInscription a skos:ConceptScheme ;
    piirrite:osmId "inscription" ;
    skos:definition "Text which is written on an object."@en ;
    skos:prefLabel "Inscription, types"@en .

piirritev:OsmIntName a skos:ConceptScheme ;
    piirrite:osmId "int_name" ;
    skos:definition ""@en ;
    skos:prefLabel "Int name, types"@en .

piirritev:OsmIntRefAh1 a skos:Concept ;
    piirrite:osmId "AH1" ;
    rdfs:subClassOf piirrite:OsmEntity ;
    skos:definition ""@en ;
    skos:inScheme piirritev:OsmIntRef ;
    skos:prefLabel "Ah1"@en .

piirritev:OsmIntRefAh2 a skos:Concept ;
    piirrite:osmId "AH2" ;
    rdfs:subClassOf piirrite:OsmEntity ;
    skos:definition ""@en ;
    skos:inScheme piirritev:OsmIntRef ;
    skos:prefLabel "Ah2"@en .

piirritev:OsmIntRefE22 a skos:Concept ;
    piirrite:osmId "E_22" ;
    rdfs:subClassOf piirrite:OsmEntity ;
    skos:definition ""@en ;
    skos:inScheme piirritev:OsmIntRef ;
    skos:prefLabel "E 22"@en .

piirritev:OsmIntRefE30 a skos:Concept ;
    piirrite:osmId "E_30" ;
    rdfs:subClassOf piirrite:OsmEntity ;
    skos:definition ""@en ;
    skos:inScheme piirritev:OsmIntRef ;
    skos:prefLabel "E 30"@en .

piirritev:OsmIntRefE40 a skos:Concept ;
    piirrite:osmId "E_40" ;
    rdfs:subClassOf piirrite:OsmEntity ;
    skos:definition ""@en ;
    skos:inScheme piirritev:OsmIntRef ;
    skos:prefLabel "E 40"@en .

piirritev:OsmIntRefE45 a skos:Concept ;
    piirrite:osmId "E_45" ;
    rdfs:subClassOf piirrite:OsmEntity ;
    skos:definition ""@en ;
    skos:inScheme piirritev:OsmIntRef ;
    skos:prefLabel "E 45"@en .

piirritev:OsmIntRefE70 a skos:Concept ;
    piirrite:osmId "E_70" ;
    rdfs:subClassOf piirrite:OsmEntity ;
    skos:definition ""@en ;
    skos:inScheme piirritev:OsmIntRef ;
    skos:prefLabel "E 70"@en .

piirritev:OsmIntRefE75 a skos:Concept ;
    piirrite:osmId "E_75" ;
    rdfs:subClassOf piirrite:OsmEntity ;
    skos:definition ""@en ;
    skos:inScheme piirritev:OsmIntRef ;
    skos:prefLabel "E 75"@en .

piirritev:OsmIntermittent a skos:ConceptScheme ;
    piirrite:osmId "intermittent" ;
    skos:definition "Used to indicate whether or not a waterway or water body does not permanently contain water. osmcarto-rendering-way=File:Rendering-waterway_river_intermittent.png osmcarto-rendering-way-size=100px osmcarto-rendering-area=File:Water_intermittent_100.png osmcarto-rendering-area-size=100px"@en ;
    skos:prefLabel "Intermittent, types"@en .

piirritev:OsmInternetAccessWlan a skos:Concept ;
    piirrite:hasRelatedOsmTag piirrite:hasOsmWlanInternetAccess ;
    piirrite:osmId "wlan" ;
    rdfs:subClassOf piirrite:OsmEntity ;
    skos:definition "Specifies that a feature offers a WLAN wireless internet Hotspot (Wi-Fi)"@en ;
    skos:inScheme piirritev:OsmInternetAccess ;
    skos:prefLabel "Wlan"@en .

piirritev:OsmIsIn a skos:ConceptScheme ;
    piirrite:osmId "is_in" ;
    skos:definition "The is_in tag is used to index where a place or feature is."@en ;
    skos:prefLabel "Is in, types"@en .

piirritev:OsmJunctionCircular a skos:Concept ;
    piirrite:osmId "circular" ;
    rdfs:subClassOf piirrite:OsmEntity ;
    skos:definition "A road junction where the traffic goes around a non-traversable island but does not always have right of way."@en ;
    skos:inScheme piirritev:OsmJunction ;
    skos:prefLabel "Circular"@en .

piirritev:OsmJunctionRoundabout a skos:Concept ;
    piirrite:hasRelatedOsmTag piirrite:hasOsmRoundaboutHighway ;
    piirrite:osmId "roundabout" ;
    rdfs:subClassOf piirrite:OsmEntity ;
    skos:definition "A road junction where the traffic goes around a non-traversable island and has right of way."@en ;
    skos:inScheme piirritev:OsmJunction ;
    skos:prefLabel "Roundabout"@en .

piirritev:OsmKerbFlush a skos:Concept ;
    piirrite:osmId "flush" ;
    rdfs:subClassOf piirrite:OsmEntity ;
    skos:definition ""@en ;
    skos:inScheme piirritev:OsmKerb ;
    skos:prefLabel "Flush"@en .

piirritev:OsmKerbLowered a skos:Concept ;
    piirrite:osmId "lowered" ;
    rdfs:subClassOf piirrite:OsmEntity ;
    skos:definition ""@en ;
    skos:inScheme piirritev:OsmKerb ;
    skos:prefLabel "Lowered"@en .

piirritev:OsmKerbRaised a skos:Concept ;
    piirrite:osmId "raised" ;
    rdfs:subClassOf piirrite:OsmEntity ;
    skos:definition ""@en ;
    skos:inScheme piirritev:OsmKerb ;
    skos:prefLabel "Raised"@en .

piirritev:OsmKerbRolled a skos:Concept ;
    piirrite:osmId "rolled" ;
    rdfs:subClassOf piirrite:OsmEntity ;
    skos:definition ""@en ;
    skos:inScheme piirritev:OsmKerb ;
    skos:prefLabel "Rolled"@en .

piirritev:OsmLampMountAngledMast a skos:Concept ;
    piirrite:osmId "angled_mast" ;
    rdfs:subClassOf piirrite:OsmEntity ;
    skos:definition ""@en ;
    skos:inScheme piirritev:OsmLampMount ;
    skos:prefLabel "Angled mast"@en .

piirritev:OsmLampMountBentMast a skos:Concept ;
    piirrite:osmId "bent_mast" ;
    rdfs:subClassOf piirrite:OsmEntity ;
    skos:definition ""@en ;
    skos:inScheme piirritev:OsmLampMount ;
    skos:prefLabel "Bent mast"@en .

piirritev:OsmLampMountHighMast a skos:Concept ;
    piirrite:osmId "high_mast" ;
    rdfs:subClassOf piirrite:OsmEntity ;
    skos:definition ""@en ;
    skos:inScheme piirritev:OsmLampMount ;
    skos:prefLabel "High mast"@en .

piirritev:OsmLampMountPole a skos:Concept ;
    piirrite:osmId "pole" ;
    rdfs:subClassOf piirrite:OsmEntity ;
    skos:definition ""@en ;
    skos:inScheme piirritev:OsmLampMount ;
    skos:prefLabel "Pole"@en .

piirritev:OsmLampMountStraightMast a skos:Concept ;
    piirrite:osmId "straight_mast" ;
    rdfs:subClassOf piirrite:OsmEntity ;
    skos:definition ""@en ;
    skos:inScheme piirritev:OsmLampMount ;
    skos:prefLabel "Straight mast"@en .

piirritev:OsmLampMountWall a skos:Concept ;
    piirrite:osmId "wall" ;
    rdfs:subClassOf piirrite:OsmEntity ;
    skos:definition ""@en ;
    skos:inScheme piirritev:OsmLampMount ;
    skos:prefLabel "Wall"@en .

piirritev:OsmLampTypeElectric a skos:Concept ;
    piirrite:osmId "electric" ;
    rdfs:subClassOf piirrite:OsmEntity ;
    skos:definition ""@en ;
    skos:inScheme piirritev:OsmLampType ;
    skos:prefLabel "Electric"@en .

piirritev:OsmLampTypeFluorescent a skos:Concept ;
    piirrite:osmId "fluorescent" ;
    rdfs:subClassOf piirrite:OsmEntity ;
    skos:definition ""@en ;
    skos:inScheme piirritev:OsmLampType ;
    skos:prefLabel "Fluorescent"@en .

piirritev:OsmLampTypeGaslight a skos:Concept ;
    piirrite:osmId "gaslight" ;
    rdfs:subClassOf piirrite:OsmEntity ;
    skos:definition ""@en ;
    skos:inScheme piirritev:OsmLampType ;
    skos:prefLabel "Gaslight"@en .

piirritev:OsmLampTypeLed a skos:Concept ;
    piirrite:osmId "LED",
        "led" ;
    rdfs:subClassOf piirrite:OsmEntity ;
    skos:definition ""@en ;
    skos:inScheme piirritev:OsmLampType ;
    skos:prefLabel "Led"@en .

piirritev:OsmLampTypeMetal-Halogenide a skos:Concept ;
    piirrite:osmId "metal-halogenide" ;
    rdfs:subClassOf piirrite:OsmEntity ;
    skos:definition ""@en ;
    skos:inScheme piirritev:OsmLampType ;
    skos:prefLabel "Metal-halogenide"@en .

piirritev:OsmLampTypeSodium a skos:Concept ;
    piirrite:osmId "sodium" ;
    rdfs:subClassOf piirrite:OsmEntity ;
    skos:definition ""@en ;
    skos:inScheme piirritev:OsmLampType ;
    skos:prefLabel "Sodium"@en .

piirritev:OsmLandcoverGrass a skos:Concept ;
    piirrite:osmId "grass" ;
    rdfs:subClassOf piirrite:OsmEntity ;
    skos:definition "An area covered with grass."@en ;
    skos:inScheme piirritev:OsmLandcover ;
    skos:prefLabel "Grass"@en .

piirritev:OsmLandcoverMostlyRock a skos:Concept ;
    piirrite:osmId "mostly_rock" ;
    rdfs:subClassOf piirrite:OsmEntity ;
    skos:definition "Indicates that a land is physically covered with rocks."@en ;
    skos:inScheme piirritev:OsmLandcover ;
    skos:prefLabel "Mostly rock"@en .

piirritev:OsmLandcoverScrub a skos:Concept ;
    piirrite:osmId "scrub" ;
    rdfs:subClassOf piirrite:OsmEntity ;
    skos:definition ""@en ;
    skos:inScheme piirritev:OsmLandcover ;
    skos:prefLabel "Scrub"@en .

piirritev:OsmLandcoverTrees a skos:Concept ;
    piirrite:osmId "trees" ;
    rdfs:subClassOf piirrite:OsmEntity ;
    skos:definition "An area covered with trees."@en ;
    skos:inScheme piirritev:OsmLandcover ;
    skos:prefLabel "Trees"@en .

piirritev:OsmLanduseAllotments a skos:Concept ;
    piirrite:hasRelatedOsmTag piirrite:hasOsmAllotmentsName,
        piirrite:hasOsmAllotmentsOperator ;
    piirrite:osmId "allotments" ;
    rdfs:subClassOf piirrite:OsmEntity ;
    skos:definition "allotment gardens with multiple land parcels assigned to individuals or families for gardening. osmcarto-rendering=File:Landuse-allotments.png osmcarto-rendering-size=125px onNode=no onWay=no onArea=yes onRelation=no seeAlso = * landuse=farmland * leisure=garden combination= * name * operator status=de facto"@en ;
    skos:inScheme piirritev:OsmLanduse ;
    skos:prefLabel "Allotments"@en .

piirritev:OsmLanduseAnimalKeeping a skos:Concept ;
    piirrite:hasRelatedOsmTag piirrite:hasOsmAnimalKeepingBarrier,
        piirrite:hasOsmAnimalKeepingType ;
    piirrite:osmId "animal_keeping" ;
    rdfs:subClassOf piirrite:OsmEntity ;
    skos:definition "An area of land that is used to keep animals"@en ;
    skos:inScheme piirritev:OsmLanduse ;
    skos:prefLabel "Animal keeping"@en .

piirritev:OsmLanduseAquaculture a skos:Concept ;
    piirrite:hasRelatedOsmTag piirrite:hasOsmAquacultureNatural,
        piirrite:hasOsmAquacultureType ;
    piirrite:osmId "aquaculture" ;
    rdfs:subClassOf piirrite:OsmEntity ;
    skos:definition "An area on land or water that is used to farm aquatic organisms."@en ;
    skos:inScheme piirritev:OsmLanduse ;
    skos:prefLabel "Aquaculture"@en .

piirritev:OsmLanduseBasin a skos:Concept ;
    piirrite:hasRelatedOsmTag piirrite:hasOsmBasinIntermittent,
        piirrite:hasOsmBasinName,
        piirrite:hasOsmBasinType ;
    piirrite:osmId "basin" ;
    rdfs:subClassOf piirrite:OsmEntity ;
    skos:definition "An area of land artificially graded to hold water. Includes also structures typically without water."@en ;
    skos:inScheme piirritev:OsmLanduse ;
    skos:prefLabel "Basin"@en .

piirritev:OsmLanduseBrownfield a skos:Concept ;
    piirrite:osmId "brownfield" ;
    rdfs:subClassOf piirrite:OsmEntity ;
    skos:definition "Land which was developed which is no longer in use. osmcarto-rendering=File:Rendering-landuse-construction-mapnik.png osmcarto-rendering-size=100px"@en ;
    skos:inScheme piirritev:OsmLanduse ;
    skos:prefLabel "Brownfield"@en .

piirritev:OsmLanduseCemetery a skos:Concept ;
    piirrite:hasRelatedOsmTag piirrite:hasOsmCemeteryName,
        piirrite:hasOsmCemeteryReligion ;
    piirrite:osmId "cemetery" ;
    rdfs:subClassOf piirrite:OsmEntity ;
    skos:definition "A place where people, or sometimes animals are buried that isn't part of a place of worship osmcarto-rendering=File:Landuse-cemetery.png osmcarto-rendering-size=125px"@en ;
    skos:inScheme piirritev:OsmLanduse ;
    skos:prefLabel "Cemetery"@en .

piirritev:OsmLanduseCommercial a skos:Concept ;
    piirrite:hasRelatedOsmTag piirrite:hasOsmCommercialName ;
    piirrite:osmId "commercial" ;
    rdfs:subClassOf piirrite:OsmEntity ;
    skos:definition "A commercial zone, predominantly offices or services.  osmcarto-rendering=File:Landuse-commercial.png  osmcarto-rendering-size=100px"@en ;
    skos:inScheme piirritev:OsmLanduse ;
    skos:prefLabel "Commercial"@en .

piirritev:OsmLanduseConstruction a skos:Concept ;
    piirrite:hasRelatedOsmTag piirrite:hasOsmConstructionCheckDate,
        piirrite:hasOsmConstructionName,
        piirrite:hasOsmConstructionType ;
    piirrite:osmId "construction" ;
    rdfs:subClassOf piirrite:OsmEntity ;
    skos:definition "An area being built on. osmcarto-rendering=File:Rendering-landuse-construction-mapnik.png osmcarto-rendering-size=100px"@en ;
    skos:inScheme piirritev:OsmLanduse ;
    skos:prefLabel "Construction"@en .

piirritev:OsmLanduseEducation a skos:Concept ;
    piirrite:hasRelatedOsmTag piirrite:hasOsmEducationAmenity ;
    piirrite:osmId "education" ;
    rdfs:subClassOf piirrite:OsmEntity ;
    skos:definition "An area used by educational facilities."@en ;
    skos:inScheme piirritev:OsmLanduse ;
    skos:prefLabel "Education"@en .

piirritev:OsmLanduseFarmland a skos:Concept ;
    piirrite:hasRelatedOsmTag piirrite:hasOsmFarmlandBarrier,
        piirrite:hasOsmFarmlandCrop,
        piirrite:hasOsmFarmlandName ;
    piirrite:osmId "farmland" ;
    rdfs:subClassOf piirrite:OsmEntity ;
    skos:definition "Area of farmland used mainly for tillage (annual crops). osmcarto-rendering=File:Rendering-landuse-farm-mapnik.png osmcarto-rendering-size=125px"@en ;
    skos:inScheme piirritev:OsmLanduse ;
    skos:prefLabel "Farmland"@en .

piirritev:OsmLanduseFarmyard a skos:Concept ;
    piirrite:hasRelatedOsmTag piirrite:hasOsmFarmyardName,
        piirrite:hasOsmFarmyardOperator,
        piirrite:hasOsmFarmyardType ;
    piirrite:osmId "farmyard" ;
    rdfs:subClassOf piirrite:OsmEntity ;
    skos:definition "Area of land with farm buildings (farmhouse, sheds, stables, barns, etc.). osmcarto-rendering=File:Rendering-area-landuse farmyard-mapnik.png osmcarto-rendering-size=125px"@en ;
    skos:inScheme piirritev:OsmLanduse ;
    skos:prefLabel "Farmyard"@en .

piirritev:OsmLanduseFlowerbed a skos:Concept ;
    piirrite:hasRelatedOsmTag piirrite:hasOsmFlowerbedGenus,
        piirrite:hasOsmFlowerbedOperator,
        piirrite:hasOsmFlowerbedSpecies,
        piirrite:hasOsmFlowerbedSurface,
        piirrite:hasOsmFlowerbedTaxon ;
    piirrite:osmId "flowerbed" ;
    rdfs:subClassOf piirrite:OsmEntity ;
    skos:definition "An area designated for flowers.  osmcarto-rendering = File:Landuse-flowerbed.png  osmcarto-rendering-size = 125px"@en ;
    skos:inScheme piirritev:OsmLanduse ;
    skos:prefLabel "Flowerbed"@en .

piirritev:OsmLanduseGarages a skos:Concept ;
    piirrite:hasRelatedOsmTag piirrite:hasOsmGaragesBuilding,
        piirrite:hasOsmGaragesHighway ;
    piirrite:osmId "garages" ;
    rdfs:subClassOf piirrite:OsmEntity ;
    skos:definition "An area occupied by multiple private garage buildings. osmcarto-rendering=File:Rendering-area-landuse garages-mapnik.png osmcarto-rendering-size=100px"@en ;
    skos:inScheme piirritev:OsmLanduse ;
    skos:prefLabel "Garages"@en .

piirritev:OsmLanduseGrass a skos:Concept ;
    piirrite:osmId "grass" ;
    rdfs:subClassOf piirrite:OsmEntity ;
    skos:definition "A smaller area of grass, usually mown and managed. osmcarto-rendering=File:Landuse grass.png osmcarto-rendering-size=125px"@en ;
    skos:inScheme piirritev:OsmLanduse ;
    skos:prefLabel "Grass"@en .

piirritev:OsmLanduseGreenery a skos:Concept ;
    piirrite:hasRelatedOsmTag piirrite:hasOsmGreeneryBarrier,
        piirrite:hasOsmGreeneryLanduse,
        piirrite:hasOsmGreeneryLeisure,
        piirrite:hasOsmGreeneryNatural ;
    piirrite:osmId "greenery" ;
    rdfs:subClassOf piirrite:OsmEntity ;
    skos:definition "An area covered in unspecified or various types of decorative vegetation. Consider using a more specific tag instead"@en ;
    skos:inScheme piirritev:OsmLanduse ;
    skos:prefLabel "Greenery"@en .

piirritev:OsmLanduseGreenfield a skos:Concept ;
    piirrite:hasRelatedOsmTag piirrite:hasOsmGreenfieldLanduse ;
    piirrite:osmId "greenfield" ;
    rdfs:subClassOf piirrite:OsmEntity ;
    skos:definition "Undeveloped land scheduled to turn into a construction site"@en ;
    skos:inScheme piirritev:OsmLanduse ;
    skos:prefLabel "Greenfield"@en .

piirritev:OsmLanduseGreenhouseHorticulture a skos:Concept ;
    piirrite:hasRelatedOsmTag piirrite:hasOsmGreenhouseHorticultureCrop ;
    piirrite:osmId "greenhouse_horticulture" ;
    rdfs:subClassOf piirrite:OsmEntity ;
    skos:definition "Land area used for growing plants in greenhouses. osmcarto-rendering=File:Rendering-landuse-farm-mapnik.png osmcarto-rendering-size=125px"@en ;
    skos:inScheme piirritev:OsmLanduse ;
    skos:prefLabel "Greenhouse horticulture"@en .

piirritev:OsmLanduseHighway a skos:Concept ;
    piirrite:osmId "highway" ;
    rdfs:subClassOf piirrite:OsmEntity ;
    skos:definition "A land used for a highway, including all auxiliary areas like associated footways and verges, ditches, etc."@en ;
    skos:inScheme piirritev:OsmLanduse ;
    skos:prefLabel "Highway"@en .

piirritev:OsmLanduseIndustrial a skos:Concept ;
    piirrite:hasRelatedOsmTag piirrite:hasOsmIndustrialLanduse,
        piirrite:hasOsmIndustrialManMade,
        piirrite:hasOsmIndustrialName,
        piirrite:hasOsmIndustrialPipeline,
        piirrite:hasOsmIndustrialPower,
        piirrite:hasOsmIndustrialType,
        piirrite:hasOsmIndustrialUtility ;
    piirrite:osmId "industrial" ;
    rdfs:subClassOf piirrite:OsmEntity ;
    skos:definition "An area with predominantly workshops, factories or warehouses. osmcarto-rendering=File:Landuse-industrial.png osmcarto-rendering-size=100px"@en ;
    skos:inScheme piirritev:OsmLanduse ;
    skos:prefLabel "Industrial"@en .

piirritev:OsmLanduseLandfill a skos:Concept ;
    piirrite:hasRelatedOsmTag piirrite:hasOsmLandfillInformal,
        piirrite:hasOsmLandfillName,
        piirrite:hasOsmLandfillOperator ;
    piirrite:osmId "landfill" ;
    rdfs:subClassOf piirrite:OsmEntity ;
    skos:definition "A site for permanent or long term storage of waste materials. osmcarto-rendering=File:Rendering-landuse-landfill-mapnik.png osmcarto-rendering-size=100px"@en ;
    skos:inScheme piirritev:OsmLanduse ;
    skos:prefLabel "Landfill"@en .

piirritev:OsmLanduseLogging a skos:Concept ;
    piirrite:hasRelatedOsmTag piirrite:hasOsmLoggingLanduse,
        piirrite:hasOsmLoggingNatural ;
    piirrite:osmId "logging" ;
    rdfs:subClassOf piirrite:OsmEntity ;
    skos:definition "An area where some or all trees have been cut down."@en ;
    skos:inScheme piirritev:OsmLanduse ;
    skos:prefLabel "Logging"@en .

piirritev:OsmLanduseMeadow a skos:Concept ;
    piirrite:hasRelatedOsmTag piirrite:hasOsmMeadowCrop,
        piirrite:hasOsmMeadowName,
        piirrite:hasOsmMeadowType ;
    piirrite:osmId "meadow" ;
    rdfs:subClassOf piirrite:OsmEntity ;
    skos:definition "An area of meadow or pasture: land primarily vegetated by grass and other non-woody plants, mainly used for hay or grazing. osmcarto-rendering=File:Landuse Meadow.png osmcarto-rendering-size=125px"@en ;
    skos:inScheme piirritev:OsmLanduse ;
    skos:prefLabel "Meadow"@en .

piirritev:OsmLanduseMilitary a skos:Concept ;
    piirrite:hasRelatedOsmTag piirrite:hasOsmMilitaryMilitaryService,
        piirrite:hasOsmMilitaryType ;
    piirrite:osmId "military" ;
    rdfs:subClassOf piirrite:OsmEntity ;
    skos:definition "Area used for military purposes. osmcarto-rendering=File:Landuse-military 100.png osmcarto-rendering-size=100px"@en ;
    skos:inScheme piirritev:OsmLanduse ;
    skos:prefLabel "Military"@en .

piirritev:OsmLanduseOrchard a skos:Concept ;
    piirrite:hasRelatedOsmTag piirrite:hasOsmOrchardCrop,
        piirrite:hasOsmOrchardProduce,
        piirrite:hasOsmOrchardSelfHarvesting,
        piirrite:hasOsmOrchardTrees,
        piirrite:hasOsmOrchardType ;
    piirrite:osmId "orchard" ;
    rdfs:subClassOf piirrite:OsmEntity ;
    skos:definition "Used to mark intentional planting of trees or shrubs maintained for food production"@en ;
    skos:inScheme piirritev:OsmLanduse ;
    skos:prefLabel "Orchard"@en .

piirritev:OsmLandusePlantNursery a skos:Concept ;
    piirrite:hasRelatedOsmTag piirrite:hasOsmPlantNurseryGenus,
        piirrite:hasOsmPlantNurseryName,
        piirrite:hasOsmPlantNurseryOperator,
        piirrite:hasOsmPlantNurseryPlant,
        piirrite:hasOsmPlantNurserySpecies ;
    piirrite:osmId "plant_nursery" ;
    rdfs:subClassOf piirrite:OsmEntity ;
    skos:definition "Represents land that is used solely for plant nurseries, which grow live plants."@en ;
    skos:inScheme piirritev:OsmLanduse ;
    skos:prefLabel "Plant nursery"@en .

piirritev:OsmLanduseQuarry a skos:Concept ;
    piirrite:hasRelatedOsmTag piirrite:hasOsmQuarryName,
        piirrite:hasOsmQuarryOperator,
        piirrite:hasOsmQuarryResource ;
    piirrite:osmId "quarry" ;
    rdfs:subClassOf piirrite:OsmEntity ;
    skos:definition "An area of land used for surface extraction (open-pit mining). osmcarto-rendering=File:Rendering-landuse-quarry-mapnik.png osmcarto-rendering-size=125px"@en ;
    skos:inScheme piirritev:OsmLanduse ;
    skos:prefLabel "Quarry"@en .

piirritev:OsmLanduseRailway a skos:Concept ;
    piirrite:hasRelatedOsmTag piirrite:hasOsmRailwayName ;
    piirrite:osmId "railway" ;
    rdfs:subClassOf piirrite:OsmEntity ;
    skos:definition "An area of land dedicated to train operation or support, including areas around tracks, rail corridors, yards, sidings, station complexes, and ancillary man-made objects along the tracks."@en ;
    skos:inScheme piirritev:OsmLanduse ;
    skos:prefLabel "Railway"@en .

piirritev:OsmLanduseRecreationGround a skos:Concept ;
    piirrite:hasRelatedOsmTag piirrite:hasOsmRecreationGroundName ;
    piirrite:osmId "recreation_ground" ;
    rdfs:subClassOf piirrite:OsmEntity ;
    skos:definition "An open green space for general recreation, which often includes formal or informal pitches, nets and so on. Often municipally owned, sometimes part of colleges / companies or commercially operated. osmcarto-rendering=File:Landuse-recreation ground.png osmcarto-rendering-size=125px"@en ;
    skos:inScheme piirritev:OsmLanduse ;
    skos:prefLabel "Recreation ground"@en .

piirritev:OsmLanduseReligious a skos:Concept ;
    piirrite:hasRelatedOsmTag piirrite:hasOsmReligiousBarrier,
        piirrite:hasOsmReligiousReligion ;
    piirrite:osmId "religious" ;
    rdfs:subClassOf piirrite:OsmEntity ;
    skos:definition "An area used for religious purposes. osmcarto-rendering=File:Place of worship area.png osmcarto-rendering-size=125px"@en ;
    skos:inScheme piirritev:OsmLanduse ;
    skos:prefLabel "Religious"@en .

piirritev:OsmLanduseReservoir a skos:Concept ;
    piirrite:osmId "reservoir" ;
    rdfs:subClassOf piirrite:OsmEntity ;
    skos:definition "Using this tag is discouraged; use tag:natural=water + tag:water=reservoir instead. osmcarto-rendering=File:Base layer water.png osmcarto-rendering-size=100px"@en ;
    skos:inScheme piirritev:OsmLanduse ;
    skos:prefLabel "Reservoir"@en .

piirritev:OsmLanduseResidential a skos:Concept ;
    piirrite:hasRelatedOsmTag piirrite:hasOsmResidentialType ;
    piirrite:osmId "residential" ;
    rdfs:subClassOf piirrite:OsmEntity ;
    skos:definition "A portion of land predominantly used for residential purposes.  osmcarto-rendering = File:Rendering-area-landuse-residential.png  osmcarto-rendering-size = 100px"@en ;
    skos:inScheme piirritev:OsmLanduse ;
    skos:prefLabel "Residential"@en .

piirritev:OsmLanduseRetail a skos:Concept ;
    piirrite:hasRelatedOsmTag piirrite:hasOsmRetailName,
        piirrite:hasOsmRetailOperator ;
    piirrite:osmId "retail" ;
    rdfs:subClassOf piirrite:OsmEntity ;
    skos:definition "An area that encloses predominantly shops. osmcarto-rendering=File:Landuse-retail.png osmcarto-rendering-size=100px"@en ;
    skos:inScheme piirritev:OsmLanduse ;
    skos:prefLabel "Retail"@en .

piirritev:OsmLanduseSaltPond a skos:Concept ;
    piirrite:hasRelatedOsmTag piirrite:hasOsmSaltPondName,
        piirrite:hasOsmSaltPondOperator ;
    piirrite:osmId "salt_pond" ;
    rdfs:subClassOf piirrite:OsmEntity ;
    skos:definition "A place where sea water is evaporated to extract its salt osmcarto-rendering=File:Rendering-landuse-salt-pond.png osmcarto-rendering-size=125px"@en ;
    skos:inScheme piirritev:OsmLanduse ;
    skos:prefLabel "Salt pond"@en .

piirritev:OsmLanduseStaticCaravan a skos:Concept ;
    piirrite:osmId "static_caravan" ;
    rdfs:subClassOf piirrite:OsmEntity ;
    skos:definition "A plot for static caravans."@en ;
    skos:inScheme piirritev:OsmLanduse ;
    skos:prefLabel "Static caravan"@en .

piirritev:OsmLanduseVillageGreen a skos:Concept ;
    piirrite:hasRelatedOsmTag piirrite:hasOsmVillageGreenName ;
    piirrite:osmId "village_green" ;
    rdfs:subClassOf piirrite:OsmEntity ;
    skos:definition "A village green is a distinctive area of grassy public land in a village centre. Not a generic tag for urban greenery.  osmcarto-rendering = File:Landuse-village green.png  osmcarto-rendering-size = 125px"@en ;
    skos:inScheme piirritev:OsmLanduse ;
    skos:prefLabel "Village green"@en .

piirritev:OsmLanduseVineyard a skos:Concept ;
    piirrite:hasRelatedOsmTag piirrite:hasOsmVineyardGrapeVariety,
        piirrite:hasOsmVineyardName,
        piirrite:hasOsmVineyardOrganic ;
    piirrite:osmId "vineyard" ;
    rdfs:subClassOf piirrite:OsmEntity ;
    skos:definition "Used to tag vineyards, a piece of land where grapes are grown.  osmcarto-rendering = File:Landuse-vineyard.png  osmcarto-rendering-size = 125px"@en ;
    skos:inScheme piirritev:OsmLanduse ;
    skos:prefLabel "Vineyard"@en .

piirritev:OsmLaneMarkings a skos:ConceptScheme ;
    piirrite:osmId "lane_markings" ;
    skos:definition "Specifies if a highway has painted markings to indicate the position of the lanes"@en ;
    skos:prefLabel "Lane markings, types"@en .

piirritev:OsmLanes a skos:ConceptScheme ;
    piirrite:osmId "lanes" ;
    skos:definition "Total number of traffic lanes available for motorised traffic."@en ;
    skos:prefLabel "Lanes, types"@en .

piirritev:OsmLayer a skos:ConceptScheme ;
    piirrite:osmId "layer" ;
    skos:definition "Used to mark the vertical relationship between two intersecting features."@en ;
    skos:prefLabel "Layer, types"@en .

piirritev:OsmLcnProposed a skos:Concept ;
    piirrite:osmId "proposed" ;
    rdfs:subClassOf piirrite:OsmEntity ;
    skos:definition ""@en ;
    skos:inScheme piirritev:OsmLcn ;
    skos:prefLabel "Proposed"@en .

piirritev:OsmLeafCycleDeciduous a skos:Concept ;
    piirrite:osmId "deciduous" ;
    rdfs:subClassOf piirrite:OsmEntity ;
    skos:definition "Deciduous woody vegetation"@en ;
    skos:inScheme piirritev:OsmLeafCycle ;
    skos:prefLabel "Deciduous"@en .

piirritev:OsmLeafCycleEvergreen a skos:Concept ;
    piirrite:osmId "evergreen" ;
    rdfs:subClassOf piirrite:OsmEntity ;
    skos:definition "Evergreen woody vegetation"@en ;
    skos:inScheme piirritev:OsmLeafCycle ;
    skos:prefLabel "Evergreen"@en .

piirritev:OsmLeafCycleMixed a skos:Concept ;
    piirrite:osmId "mixed" ;
    rdfs:subClassOf piirrite:OsmEntity ;
    skos:definition "Habitat with evergreen and deciduous vegetation."@en ;
    skos:inScheme piirritev:OsmLeafCycle ;
    skos:prefLabel "Mixed"@en .

piirritev:OsmLeafCycleSemiDeciduous a skos:Concept ;
    piirrite:osmId "semi_deciduous" ;
    rdfs:subClassOf piirrite:OsmEntity ;
    skos:definition "Semi-deciduous woody vegetation"@en ;
    skos:inScheme piirritev:OsmLeafCycle ;
    skos:prefLabel "Semi deciduous"@en .

piirritev:OsmLeafCycleSemiEvergreen a skos:Concept ;
    piirrite:osmId "semi_evergreen" ;
    rdfs:subClassOf piirrite:OsmEntity ;
    skos:definition "Semi-evergreen woody vegetation"@en ;
    skos:inScheme piirritev:OsmLeafCycle ;
    skos:prefLabel "Semi evergreen"@en .

piirritev:OsmLeafTypeBroadleaved a skos:Concept ;
    piirrite:osmId "broadleaved" ;
    rdfs:subClassOf piirrite:OsmEntity ;
    skos:definition "Indicates that the trees or tree is broadleaved as opposed to needleleaved or leafless.  osmcarto-rendering=File:Leaftype_broadleaved_100.png  osmcarto-rendering-size=100px"@en ;
    skos:inScheme piirritev:OsmLeafType ;
    skos:prefLabel "Broadleaved"@en .

piirritev:OsmLeafTypeMixed a skos:Concept ;
    piirrite:osmId "mixed" ;
    rdfs:subClassOf piirrite:OsmEntity ;
    skos:definition "Habitat with broadleaved and needleleaved woody vegetation  osmcarto-rendering=File:Leaftype_mixed.png  osmcarto-rendering-size=125px"@en ;
    skos:inScheme piirritev:OsmLeafType ;
    skos:prefLabel "Mixed"@en .

piirritev:OsmLeafTypeNeedleleaved a skos:Concept ;
    piirrite:osmId "needleleaved" ;
    rdfs:subClassOf piirrite:OsmEntity ;
    skos:definition "Needleleaved woody vegetation  osmcarto-rendering=File:Leaftype_needleleaved.png  osmcarto-rendering-size=125px"@en ;
    skos:inScheme piirritev:OsmLeafType ;
    skos:prefLabel "Needleleaved"@en .

piirritev:OsmLeafTypePalm a skos:Concept ;
    piirrite:osmId "palm" ;
    rdfs:subClassOf piirrite:OsmEntity ;
    skos:definition "Used for palm-shaped trees."@en ;
    skos:inScheme piirritev:OsmLeafType ;
    skos:prefLabel "Palm"@en .

piirritev:OsmLength a skos:ConceptScheme ;
    piirrite:osmId "length" ;
    skos:definition "The length of a feature. Values are interpreted as meters by default."@en ;
    skos:prefLabel "Length, types"@en .

piirritev:OsmLevel a skos:ConceptScheme ;
    piirrite:osmId "level" ;
    skos:definition "Zero-based floor number of a feature (where 0 is the ground level and -1 is the basement)."@en ;
    skos:prefLabel "Level, types"@en .

piirritev:OsmLightSourceAviation a skos:Concept ;
    piirrite:osmId "aviation" ;
    rdfs:subClassOf piirrite:OsmEntity ;
    skos:definition ""@en ;
    skos:inScheme piirritev:OsmLightSource ;
    skos:prefLabel "Aviation"@en .

piirritev:OsmLightSourceLantern a skos:Concept ;
    piirrite:osmId "lantern" ;
    rdfs:subClassOf piirrite:OsmEntity ;
    skos:definition ""@en ;
    skos:inScheme piirritev:OsmLightSource ;
    skos:prefLabel "Lantern"@en .

piirritev:OsmLitAutomatic a skos:Concept ;
    piirrite:osmId "automatic" ;
    rdfs:subClassOf piirrite:OsmEntity ;
    skos:definition ""@en ;
    skos:inScheme piirritev:OsmLit ;
    skos:prefLabel "Automatic"@en .

piirritev:OsmLivingStreet a skos:ConceptScheme ;
    piirrite:osmId "living_street" ;
    skos:definition "Used to mark that pedestrians are superior to vehicles as defined in road rules."@en ;
    skos:prefLabel "Living street, types"@en .

piirritev:OsmLoadingGaugeTsiGa a skos:Concept ;
    piirrite:osmId "TSI_GA" ;
    rdfs:subClassOf piirrite:OsmEntity ;
    skos:definition ""@en ;
    skos:inScheme piirritev:OsmLoadingGauge ;
    skos:prefLabel "Tsi ga"@en .

piirritev:OsmLoadingGaugeTsiGb a skos:Concept ;
    piirrite:osmId "TSI_GB" ;
    rdfs:subClassOf piirrite:OsmEntity ;
    skos:definition ""@en ;
    skos:inScheme piirritev:OsmLoadingGauge ;
    skos:prefLabel "Tsi gb"@en .

piirritev:OsmLoadingGaugeTsiGb1 a skos:Concept ;
    piirrite:osmId "TSI_GB1" ;
    rdfs:subClassOf piirrite:OsmEntity ;
    skos:definition ""@en ;
    skos:inScheme piirritev:OsmLoadingGauge ;
    skos:prefLabel "Tsi gb1"@en .

piirritev:OsmLoadingGaugeTsiGc a skos:Concept ;
    piirrite:osmId "TSI_GC" ;
    rdfs:subClassOf piirrite:OsmEntity ;
    skos:definition ""@en ;
    skos:inScheme piirritev:OsmLoadingGauge ;
    skos:prefLabel "Tsi gc"@en .

piirritev:OsmLocName a skos:ConceptScheme ;
    piirrite:osmId "loc_name" ;
    skos:definition ""@en ;
    skos:prefLabel "Loc name, types"@en .

piirritev:OsmLocRef a skos:ConceptScheme ;
    piirrite:osmId "loc_ref" ;
    skos:definition "Local reference number or code."@en ;
    skos:prefLabel "Loc ref, types"@en .

piirritev:OsmLocalRefA a skos:Concept ;
    piirrite:osmId "A" ;
    rdfs:subClassOf piirrite:OsmEntity ;
    skos:definition ""@en ;
    skos:inScheme piirritev:OsmLocalRef ;
    skos:prefLabel "A"@en .

piirritev:OsmLocalRefB a skos:Concept ;
    piirrite:osmId "B" ;
    rdfs:subClassOf piirrite:OsmEntity ;
    skos:definition ""@en ;
    skos:inScheme piirritev:OsmLocalRef ;
    skos:prefLabel "B"@en .

piirritev:OsmLocationAboveground a skos:Concept ;
    piirrite:osmId "aboveground" ;
    rdfs:subClassOf piirrite:OsmEntity ;
    skos:definition ""@en ;
    skos:inScheme piirritev:OsmLocation ;
    skos:prefLabel "Aboveground"@en .

piirritev:OsmLocationGround a skos:Concept ;
    piirrite:osmId "ground" ;
    rdfs:subClassOf piirrite:OsmEntity ;
    skos:definition ""@en ;
    skos:inScheme piirritev:OsmLocation ;
    skos:prefLabel "Ground"@en .

piirritev:OsmLocationIndoor a skos:Concept ;
    piirrite:osmId "indoor" ;
    rdfs:subClassOf piirrite:OsmEntity ;
    skos:definition "Indicate a given feature is indoor"@en ;
    skos:inScheme piirritev:OsmLocation ;
    skos:prefLabel "Indoor"@en .

piirritev:OsmLocationOutdoor a skos:Concept ;
    piirrite:osmId "outdoor" ;
    rdfs:subClassOf piirrite:OsmEntity ;
    skos:definition "Indicate a given feature is outdoor"@en ;
    skos:inScheme piirritev:OsmLocation ;
    skos:prefLabel "Outdoor"@en .

piirritev:OsmLocationOverground a skos:Concept ;
    piirrite:osmId "overground" ;
    rdfs:subClassOf piirrite:OsmEntity ;
    skos:definition "Indicate a given feature is installed on the ground surface and can be touched"@en ;
    skos:inScheme piirritev:OsmLocation ;
    skos:prefLabel "Overground"@en .

piirritev:OsmLocationOverhead a skos:Concept ;
    piirrite:osmId "overhead" ;
    rdfs:subClassOf piirrite:OsmEntity ;
    skos:definition "Indicate a given feature is installed over the ground at a height allowing persons or vehicles to pass underneath."@en ;
    skos:inScheme piirritev:OsmLocation ;
    skos:prefLabel "Overhead"@en .

piirritev:OsmLocationPole a skos:Concept ;
    piirrite:osmId "pole" ;
    rdfs:subClassOf piirrite:OsmEntity ;
    skos:definition ""@en ;
    skos:inScheme piirritev:OsmLocation ;
    skos:prefLabel "Pole"@en .

piirritev:OsmLocationRoof a skos:Concept ;
    piirrite:osmId "roof" ;
    rdfs:subClassOf piirrite:OsmEntity ;
    skos:definition "Indicates that a given feature is located on top of the roof."@en ;
    skos:inScheme piirritev:OsmLocation ;
    skos:prefLabel "Roof"@en .

piirritev:OsmLocationSurface a skos:Concept ;
    piirrite:hasRelatedOsmTag piirrite:hasOsmSurfaceBuilding ;
    piirrite:osmId "surface" ;
    rdfs:subClassOf piirrite:OsmEntity ;
    skos:definition "Feature is on the surface of the ground"@en ;
    skos:inScheme piirritev:OsmLocation ;
    skos:prefLabel "Surface"@en .

piirritev:OsmLocationUnderground a skos:Concept ;
    piirrite:hasRelatedOsmTag piirrite:hasOsmUndergroundManMade,
        piirrite:hasOsmUndergroundPower,
        piirrite:hasOsmUndergroundTunnel ;
    piirrite:osmId "underground" ;
    rdfs:subClassOf piirrite:OsmEntity ;
    skos:definition "Indicate a given feature is buried or dug under the surface of the ground."@en ;
    skos:inScheme piirritev:OsmLocation ;
    skos:prefLabel "Underground"@en .

piirritev:OsmLocationUnderwater a skos:Concept ;
    piirrite:hasRelatedOsmTag piirrite:hasOsmUnderwaterLocation ;
    piirrite:osmId "underwater" ;
    rdfs:subClassOf piirrite:OsmEntity ;
    skos:definition "Indicate a given feature is underwater."@en ;
    skos:inScheme piirritev:OsmLocation ;
    skos:prefLabel "Underwater"@en .

piirritev:OsmLocked a skos:ConceptScheme ;
    piirrite:osmId "locked" ;
    skos:definition "Used to mark a gate, barrier or other feature as locked or not."@en ;
    skos:prefLabel "Locked, types"@en .

piirritev:OsmMale a skos:ConceptScheme ;
    piirrite:osmId "male" ;
    skos:definition "Access restriction for persons of the male sex or gender or service is provided for these."@en ;
    skos:prefLabel "Male, types"@en .

piirritev:OsmManholeDrain a skos:Concept ;
    piirrite:hasRelatedOsmTag piirrite:hasOsmDrainColour,
        piirrite:hasOsmDrainDiameter,
        piirrite:hasOsmDrainInlet,
        piirrite:hasOsmDrainLength,
        piirrite:hasOsmDrainMaterial,
        piirrite:hasOsmDrainShape,
        piirrite:hasOsmDrainWidth ;
    piirrite:osmId "drain" ;
    rdfs:subClassOf piirrite:OsmEntity ;
    skos:definition "Manhole cover giving access to a draining system"@en ;
    skos:inScheme piirritev:OsmManhole ;
    skos:prefLabel "Drain"@en .

piirritev:OsmManholeSewer a skos:Concept ;
    piirrite:hasRelatedOsmTag piirrite:hasOsmSewerManhole ;
    piirrite:osmId "sewer" ;
    rdfs:subClassOf piirrite:OsmEntity ;
    skos:definition "Manhole cover giving maintenance access to pipelines carrying wastewater (sewage)."@en ;
    skos:inScheme piirritev:OsmManhole ;
    skos:prefLabel "Sewer"@en .

piirritev:OsmManholeTelecom a skos:Concept ;
    piirrite:osmId "telecom" ;
    rdfs:subClassOf piirrite:OsmEntity ;
    skos:definition "A manhole providing maintenance access to pipelines containing telecommunication cables"@en ;
    skos:inScheme piirritev:OsmManhole ;
    skos:prefLabel "Telecom"@en .

piirritev:OsmManufacturerEnercon a skos:Concept ;
    piirrite:osmId "Enercon" ;
    rdfs:subClassOf piirrite:OsmEntity ;
    skos:definition ""@en ;
    skos:inScheme piirritev:OsmManufacturer ;
    skos:prefLabel "Enercon"@en .

piirritev:OsmManufacturerFlockSafety a skos:Concept ;
    piirrite:osmId "Flock_Safety" ;
    rdfs:subClassOf piirrite:OsmEntity ;
    skos:definition ""@en ;
    skos:inScheme piirritev:OsmManufacturer ;
    skos:prefLabel "Flock safety"@en .

piirritev:OsmManufacturerGe a skos:Concept ;
    piirrite:osmId "GE" ;
    rdfs:subClassOf piirrite:OsmEntity ;
    skos:definition ""@en ;
    skos:inScheme piirritev:OsmManufacturer ;
    skos:prefLabel "Ge"@en .

piirritev:OsmManufacturerSiemens a skos:Concept ;
    piirrite:osmId "Siemens" ;
    rdfs:subClassOf piirrite:OsmEntity ;
    skos:definition ""@en ;
    skos:inScheme piirritev:OsmManufacturer ;
    skos:prefLabel "Siemens"@en .

piirritev:OsmManufacturerVestas a skos:Concept ;
    piirrite:osmId "Vestas" ;
    rdfs:subClassOf piirrite:OsmEntity ;
    skos:definition ""@en ;
    skos:inScheme piirritev:OsmManufacturer ;
    skos:prefLabel "Vestas"@en .

piirritev:OsmMapillary a skos:ConceptScheme ;
    piirrite:osmId "mapillary" ;
    skos:definition "Reference code for a Mapillary image"@en ;
    skos:prefLabel "Mapillary, types"@en .

piirritev:OsmMarkerAerial a skos:Concept ;
    piirrite:hasRelatedOsmTag piirrite:hasOsmAerialOperator,
        piirrite:hasOsmAerialUtility ;
    piirrite:osmId "aerial" ;
    rdfs:subClassOf piirrite:OsmEntity ;
    skos:definition "A marker designed to be seen by aerial inspection, usually composed of a roof cover on a pole"@en ;
    skos:inScheme piirritev:OsmMarker ;
    skos:prefLabel "Aerial"@en .

piirritev:OsmMarkerPost a skos:Concept ;
    piirrite:hasRelatedOsmTag piirrite:hasOsmPostOperator,
        piirrite:hasOsmPostUtility ;
    piirrite:osmId "post" ;
    rdfs:subClassOf piirrite:OsmEntity ;
    skos:definition "A standard kind of marker composed of a small pole or mast with information written on it. The support is dedicated to the marker. See plate for other situations."@en ;
    skos:inScheme piirritev:OsmMarker ;
    skos:prefLabel "Post"@en .

piirritev:OsmMarkerStone a skos:Concept ;
    piirrite:hasRelatedOsmTag piirrite:hasOsmStoneBoundary,
        piirrite:hasOsmStoneOperator,
        piirrite:hasOsmStoneUtility ;
    piirrite:osmId "stone" ;
    rdfs:subClassOf piirrite:OsmEntity ;
    skos:definition "A stone marker is a natural support on which useful information is directly etched or painted."@en ;
    skos:inScheme piirritev:OsmMarker ;
    skos:prefLabel "Stone"@en .

piirritev:OsmMaterialAluminium a skos:Concept ;
    piirrite:hasRelatedOsmTag piirrite:hasOsmAluminiumHighway,
        piirrite:hasOsmAluminiumMemorial ;
    piirrite:osmId "aluminium" ;
    rdfs:subClassOf piirrite:OsmEntity ;
    skos:definition "The main material is aluminium (aluminum)."@en ;
    skos:inScheme piirritev:OsmMaterial ;
    skos:prefLabel "Aluminium"@en .

piirritev:OsmMaterialBrass a skos:Concept ;
    piirrite:hasRelatedOsmTag piirrite:hasOsmBrassMemorial,
        piirrite:hasOsmBrassTourism ;
    piirrite:osmId "brass" ;
    rdfs:subClassOf piirrite:OsmEntity ;
    skos:definition "The main material is brass, a copper-zinc alloy."@en ;
    skos:inScheme piirritev:OsmMaterial ;
    skos:prefLabel "Brass"@en .

piirritev:OsmMaterialBrick a skos:Concept ;
    piirrite:osmId "brick" ;
    rdfs:subClassOf piirrite:OsmEntity ;
    skos:definition ""@en ;
    skos:inScheme piirritev:OsmMaterial ;
    skos:prefLabel "Brick"@en .

piirritev:OsmMaterialConcrete a skos:Concept ;
    piirrite:hasRelatedOsmTag piirrite:hasOsmConcreteMaterial,
        piirrite:hasOsmConcreteSurface ;
    piirrite:osmId "concrete" ;
    rdfs:subClassOf piirrite:OsmEntity ;
    skos:definition "The main material is concrete, a hard material composed of a mixture of sand, water and aggregates."@en ;
    skos:inScheme piirritev:OsmMaterial ;
    skos:prefLabel "Concrete"@en .

piirritev:OsmMaterialGlass a skos:Concept ;
    piirrite:hasRelatedOsmTag piirrite:hasOsmGlassBarrier,
        piirrite:hasOsmGlassDoor ;
    piirrite:osmId "glass" ;
    rdfs:subClassOf piirrite:OsmEntity ;
    skos:definition "The main material is glass."@en ;
    skos:inScheme piirritev:OsmMaterial ;
    skos:prefLabel "Glass"@en .

piirritev:OsmMaterialGranite a skos:Concept ;
    piirrite:hasRelatedOsmTag piirrite:hasOsmGraniteHistoric,
        piirrite:hasOsmGraniteManMade ;
    piirrite:osmId "granite" ;
    rdfs:subClassOf piirrite:OsmEntity ;
    skos:definition "The main material is a coarse-grained rock composed mostly of quartz and alkali feldspar."@en ;
    skos:inScheme piirritev:OsmMaterial ;
    skos:prefLabel "Granite"@en .

piirritev:OsmMaterialMasonry a skos:Concept ;
    piirrite:osmId "masonry" ;
    rdfs:subClassOf piirrite:OsmEntity ;
    skos:definition ""@en ;
    skos:inScheme piirritev:OsmMaterial ;
    skos:prefLabel "Masonry"@en .

piirritev:OsmMaterialMetal a skos:Concept ;
    piirrite:osmId "metal" ;
    rdfs:subClassOf piirrite:OsmEntity ;
    skos:definition "The main material is some kind of metal. If possible, qualify further by type."@en ;
    skos:inScheme piirritev:OsmMaterial ;
    skos:prefLabel "Metal"@en .

piirritev:OsmMaterialPlastic a skos:Concept ;
    piirrite:hasRelatedOsmTag piirrite:hasOsmPlasticSurface ;
    piirrite:osmId "plastic" ;
    rdfs:subClassOf piirrite:OsmEntity ;
    skos:definition "The main material is some kind of plastic. If possible, qualify further."@en ;
    skos:inScheme piirritev:OsmMaterial ;
    skos:prefLabel "Plastic"@en .

piirritev:OsmMaterialReinforcedConcrete a skos:Concept ;
    piirrite:hasRelatedOsmTag piirrite:hasOsmReinforcedConcreteMaterial ;
    piirrite:osmId "reinforced_concrete" ;
    rdfs:subClassOf piirrite:OsmEntity ;
    skos:definition "The main material is reinforced concrete. That is concrete strengthened with embedded steel bars."@en ;
    skos:inScheme piirritev:OsmMaterial ;
    skos:prefLabel "Reinforced concrete"@en .

piirritev:OsmMaterialRock a skos:Concept ;
    piirrite:osmId "rock" ;
    rdfs:subClassOf piirrite:OsmEntity ;
    skos:definition ""@en ;
    skos:inScheme piirritev:OsmMaterial ;
    skos:prefLabel "Rock"@en .

piirritev:OsmMaterialSandstone a skos:Concept ;
    piirrite:hasRelatedOsmTag piirrite:hasOsmSandstoneHeight,
        piirrite:hasOsmSandstoneHistoric,
        piirrite:hasOsmSandstoneInscription ;
    piirrite:osmId "sandstone" ;
    rdfs:subClassOf piirrite:OsmEntity ;
    skos:definition "The main material is a sedimentary rock composed mainly of sand-sized grains."@en ;
    skos:inScheme piirritev:OsmMaterial ;
    skos:prefLabel "Sandstone"@en .

piirritev:OsmMaterialSoil a skos:Concept ;
    piirrite:osmId "soil" ;
    rdfs:subClassOf piirrite:OsmEntity ;
    skos:definition ""@en ;
    skos:inScheme piirritev:OsmMaterial ;
    skos:prefLabel "Soil"@en .

piirritev:OsmMaterialSteel a skos:Concept ;
    piirrite:hasRelatedOsmTag piirrite:hasOsmSteelPower,
        piirrite:hasOsmSteelStructure ;
    piirrite:osmId "steel" ;
    rdfs:subClassOf piirrite:OsmEntity ;
    skos:definition "The main material is steel, an alloy of iron and carbon."@en ;
    skos:inScheme piirritev:OsmMaterial ;
    skos:prefLabel "Steel"@en .

piirritev:OsmMaterialStone a skos:Concept ;
    piirrite:hasRelatedOsmTag piirrite:hasOsmStoneMaterial,
        piirrite:hasOsmStoneSurface ;
    piirrite:osmId "stone" ;
    rdfs:subClassOf piirrite:OsmEntity ;
    skos:definition "The main material is some kind of stone. If possible, qualify further by type or origin."@en ;
    skos:inScheme piirritev:OsmMaterial ;
    skos:prefLabel "Stone"@en .

piirritev:OsmMaterialWood a skos:Concept ;
    piirrite:hasRelatedOsmTag piirrite:hasOsmWoodAmenity,
        piirrite:hasOsmWoodPower ;
    piirrite:osmId "wood" ;
    rdfs:subClassOf piirrite:OsmEntity ;
    skos:definition "The main material is wood."@en ;
    skos:inScheme piirritev:OsmMaterial ;
    skos:prefLabel "Wood"@en .

piirritev:OsmMaxaxleload a skos:ConceptScheme ;
    piirrite:osmId "maxaxleload" ;
    skos:definition "The legal maximum axleload in metric tonnes."@en ;
    skos:prefLabel "Maxaxleload, types"@en .

piirritev:OsmMaxheightBelowDefault a skos:Concept ;
    piirrite:osmId "below_default" ;
    rdfs:subClassOf piirrite:OsmEntity ;
    skos:definition ""@en ;
    skos:inScheme piirritev:OsmMaxheight ;
    skos:prefLabel "Below default"@en .

piirritev:OsmMaxheightDefault a skos:Concept ;
    piirrite:hasRelatedOsmTag piirrite:hasOsmDefaultHighway ;
    piirrite:osmId "default" ;
    rdfs:subClassOf piirrite:OsmEntity ;
    skos:definition "No specific legal height limit (no sign), default height rules apply here"@en ;
    skos:inScheme piirritev:OsmMaxheight ;
    skos:prefLabel "Default"@en .

piirritev:OsmMaxspeed a skos:ConceptScheme ;
    piirrite:osmId "maxspeed" ;
    skos:definition "Specifies the maximum legal speed limit on a road, railway or waterway."@en ;
    skos:prefLabel "Maxspeed, types"@en .

piirritev:OsmMaxstayUnlimited a skos:Concept ;
    piirrite:osmId "unlimited" ;
    rdfs:subClassOf piirrite:OsmEntity ;
    skos:definition ""@en ;
    skos:inScheme piirritev:OsmMaxstay ;
    skos:prefLabel "Unlimited"@en .

piirritev:OsmMaxweight a skos:ConceptScheme ;
    piirrite:osmId "maxweight" ;
    skos:definition "Permissible maximum actual weight in metric tonnes (or other explicitly specified unit)."@en ;
    skos:prefLabel "Maxweight, types"@en .

piirritev:OsmMeadowAgricultural a skos:Concept ;
    piirrite:osmId "agricultural" ;
    rdfs:subClassOf piirrite:OsmEntity ;
    skos:definition ""@en ;
    skos:inScheme piirritev:OsmMeadow ;
    skos:prefLabel "Agricultural"@en .

piirritev:OsmMeadowAgriculture a skos:Concept ;
    piirrite:osmId "agriculture" ;
    rdfs:subClassOf piirrite:OsmEntity ;
    skos:definition ""@en ;
    skos:inScheme piirritev:OsmMeadow ;
    skos:prefLabel "Agriculture"@en .

piirritev:OsmMeadowMeadowOrchard a skos:Concept ;
    piirrite:osmId "meadow_orchard" ;
    rdfs:subClassOf piirrite:OsmEntity ;
    skos:definition "A meadow or pasture with fruit trees."@en ;
    skos:inScheme piirritev:OsmMeadow ;
    skos:prefLabel "Meadow orchard"@en .

piirritev:OsmMeadowPasture a skos:Concept ;
    piirrite:osmId "pasture" ;
    rdfs:subClassOf piirrite:OsmEntity ;
    skos:definition "An area of land mainly used for grazing animals."@en ;
    skos:inScheme piirritev:OsmMeadow ;
    skos:prefLabel "Pasture"@en .

piirritev:OsmMinHeight a skos:ConceptScheme ;
    piirrite:osmId "min_height" ;
    skos:definition "Height of location of bottom part of building, part of building or another objects."@en ;
    skos:prefLabel "Min height, types"@en .

piirritev:OsmMinspeed a skos:ConceptScheme ;
    piirrite:osmId "minspeed" ;
    skos:definition "Specifies the minimum speed limit on a road, railway or waterway. Note that may refer to minimum achievable speed by vehicle or to minimum movement speed at given moment."@en ;
    skos:prefLabel "Minspeed, types"@en .

piirritev:OsmModel a skos:ConceptScheme ;
    piirrite:osmId "model" ;
    skos:definition "Model designation of a manufactured object."@en ;
    skos:prefLabel "Model, types"@en .

piirritev:OsmMofaDesignated a skos:Concept ;
    piirrite:osmId "designated" ;
    rdfs:subClassOf piirrite:OsmEntity ;
    skos:definition ""@en ;
    skos:inScheme piirritev:OsmMofa ;
    skos:prefLabel "Designated"@en .

piirritev:OsmMofaUseSidepath a skos:Concept ;
    piirrite:hasRelatedOsmTag piirrite:hasOsmUseSidepathHighway ;
    piirrite:osmId "use_sidepath" ;
    rdfs:subClassOf piirrite:OsmEntity ;
    skos:definition "Use compulsory parallel way instead"@en ;
    skos:inScheme piirritev:OsmMofa ;
    skos:prefLabel "Use sidepath"@en .

piirritev:OsmMopedDesignated a skos:Concept ;
    piirrite:osmId "designated" ;
    rdfs:subClassOf piirrite:OsmEntity ;
    skos:definition ""@en ;
    skos:inScheme piirritev:OsmMoped ;
    skos:prefLabel "Designated"@en .

piirritev:OsmMopedUseSidepath a skos:Concept ;
    piirrite:hasRelatedOsmTag piirrite:hasOsmUseSidepathHighway ;
    piirrite:osmId "use_sidepath" ;
    rdfs:subClassOf piirrite:OsmEntity ;
    skos:definition "Use compulsory parallel way instead"@en ;
    skos:inScheme piirritev:OsmMoped ;
    skos:prefLabel "Use sidepath"@en .

piirritev:OsmMotorVehicleAgricultural a skos:Concept ;
    piirrite:osmId "agricultural" ;
    rdfs:subClassOf piirrite:OsmEntity ;
    skos:definition "The use of the road is authorized exclusively for all types of motor vehicle which use it for agricultural purposes"@en ;
    skos:inScheme piirritev:OsmMotorVehicle ;
    skos:prefLabel "Agricultural"@en .

piirritev:OsmMotorVehicleCustomers a skos:Concept ;
    piirrite:osmId "customers" ;
    rdfs:subClassOf piirrite:OsmEntity ;
    skos:definition ""@en ;
    skos:inScheme piirritev:OsmMotorVehicle ;
    skos:prefLabel "Customers"@en .

piirritev:OsmMotorVehicleDesignated a skos:Concept ;
    piirrite:hasRelatedOsmTag piirrite:hasOsmDesignatedHighway ;
    piirrite:osmId "designated" ;
    rdfs:subClassOf piirrite:OsmEntity ;
    skos:definition "preferred or designated for motor vehicles."@en ;
    skos:inScheme piirritev:OsmMotorVehicle ;
    skos:prefLabel "Designated"@en .

piirritev:OsmMotorVehicleDestination a skos:Concept ;
    piirrite:osmId "destination" ;
    rdfs:subClassOf piirrite:OsmEntity ;
    skos:definition "indicates that transit traffic using motor vehicle is not allowed"@en ;
    skos:inScheme piirritev:OsmMotorVehicle ;
    skos:prefLabel "Destination"@en .

piirritev:OsmMotorVehicleForestry a skos:Concept ;
    piirrite:osmId "forestry" ;
    rdfs:subClassOf piirrite:OsmEntity ;
    skos:definition "The use of the road is authorized exclusively for all types of motor vehicle which use it for forestry purposes"@en ;
    skos:inScheme piirritev:OsmMotorVehicle ;
    skos:prefLabel "Forestry"@en .

piirritev:OsmMotorVehiclePermissive a skos:Concept ;
    piirrite:osmId "permissive" ;
    rdfs:subClassOf piirrite:OsmEntity ;
    skos:definition ""@en ;
    skos:inScheme piirritev:OsmMotorVehicle ;
    skos:prefLabel "Permissive"@en .

piirritev:OsmMotorVehiclePermit a skos:Concept ;
    piirrite:osmId "permit" ;
    rdfs:subClassOf piirrite:OsmEntity ;
    skos:definition ""@en ;
    skos:inScheme piirritev:OsmMotorVehicle ;
    skos:prefLabel "Permit"@en .

piirritev:OsmMotorVehiclePrivate a skos:Concept ;
    piirrite:hasRelatedOsmTag piirrite:hasOsmPrivateHighway ;
    piirrite:osmId "private" ;
    rdfs:subClassOf piirrite:OsmEntity ;
    skos:definition "Indicates that access is restricted for motor vehicles and is allowed only with permission on an individual basis. May be overridden by more specific access tags."@en ;
    skos:inScheme piirritev:OsmMotorVehicle ;
    skos:prefLabel "Private"@en .

piirritev:OsmMotorcarAgricultural a skos:Concept ;
    piirrite:osmId "agricultural" ;
    rdfs:subClassOf piirrite:OsmEntity ;
    skos:definition ""@en ;
    skos:inScheme piirritev:OsmMotorcar ;
    skos:prefLabel "Agricultural"@en .

piirritev:OsmMotorcarDesignated a skos:Concept ;
    piirrite:osmId "designated" ;
    rdfs:subClassOf piirrite:OsmEntity ;
    skos:definition ""@en ;
    skos:inScheme piirritev:OsmMotorcar ;
    skos:prefLabel "Designated"@en .

piirritev:OsmMotorcarDestination a skos:Concept ;
    piirrite:osmId "destination" ;
    rdfs:subClassOf piirrite:OsmEntity ;
    skos:definition ""@en ;
    skos:inScheme piirritev:OsmMotorcar ;
    skos:prefLabel "Destination"@en .

piirritev:OsmMotorcarPrivate a skos:Concept ;
    piirrite:osmId "private" ;
    rdfs:subClassOf piirrite:OsmEntity ;
    skos:definition ""@en ;
    skos:inScheme piirritev:OsmMotorcar ;
    skos:prefLabel "Private"@en .

piirritev:OsmMotorcycleAgricultural a skos:Concept ;
    piirrite:osmId "agricultural" ;
    rdfs:subClassOf piirrite:OsmEntity ;
    skos:definition ""@en ;
    skos:inScheme piirritev:OsmMotorcycle ;
    skos:prefLabel "Agricultural"@en .

piirritev:OsmMotorcycleDesignated a skos:Concept ;
    piirrite:osmId "designated" ;
    rdfs:subClassOf piirrite:OsmEntity ;
    skos:definition ""@en ;
    skos:inScheme piirritev:OsmMotorcycle ;
    skos:prefLabel "Designated"@en .

piirritev:OsmMotorcycleDestination a skos:Concept ;
    piirrite:osmId "destination" ;
    rdfs:subClassOf piirrite:OsmEntity ;
    skos:definition ""@en ;
    skos:inScheme piirritev:OsmMotorcycle ;
    skos:prefLabel "Destination"@en .

piirritev:OsmMotorroad a skos:ConceptScheme ;
    piirrite:osmId "motorroad" ;
    skos:definition ""@en ;
    skos:prefLabel "Motorroad, types"@en .

piirritev:OsmName1 a skos:ConceptScheme ;
    piirrite:osmId "name_1" ;
    skos:definition ""@en ;
    skos:prefLabel "Name 1, types"@en .

piirritev:OsmName7-Eleven a skos:Concept ;
    piirrite:hasRelatedOsmTag piirrite:hasOsm7-ElevenShop ;
    piirrite:osmId "7-Eleven" ;
    rdfs:subClassOf piirrite:OsmEntity ;
    skos:definition ""@en ;
    skos:inScheme piirritev:OsmName ;
    skos:prefLabel "7-eleven"@en .

piirritev:OsmNameA a skos:Concept ;
    piirrite:osmId "A" ;
    rdfs:subClassOf piirrite:OsmEntity ;
    skos:definition ""@en ;
    skos:inScheme piirritev:OsmName ;
    skos:prefLabel "A"@en .

piirritev:OsmNameB a skos:Concept ;
    piirrite:osmId "B" ;
    rdfs:subClassOf piirrite:OsmEntity ;
    skos:definition ""@en ;
    skos:inScheme piirritev:OsmName ;
    skos:prefLabel "B"@en .

piirritev:OsmNameBahnhofstrae a skos:Concept ;
    piirrite:osmId "Bahnhofstrae" ;
    rdfs:subClassOf piirrite:OsmEntity ;
    skos:definition ""@en ;
    skos:inScheme piirritev:OsmName ;
    skos:prefLabel "Bahnhofstrae"@en .

piirritev:OsmNameBergstrae a skos:Concept ;
    piirrite:osmId "Bergstrae" ;
    rdfs:subClassOf piirrite:OsmEntity ;
    skos:definition ""@en ;
    skos:inScheme piirritev:OsmName ;
    skos:prefLabel "Bergstrae"@en .

piirritev:OsmNameBp a skos:Concept ;
    piirrite:osmId "BP" ;
    rdfs:subClassOf piirrite:OsmEntity ;
    skos:definition ""@en ;
    skos:inScheme piirritev:OsmName ;
    skos:prefLabel "Bp"@en .

piirritev:OsmNameBurgerKing a skos:Concept ;
    piirrite:hasRelatedOsmTag piirrite:hasOsmBurgerKingAmenity ;
    piirrite:osmId "Burger_King" ;
    rdfs:subClassOf piirrite:OsmEntity ;
    skos:definition "American fast food restaurant chain specializing in hamburgers."@en ;
    skos:inScheme piirritev:OsmName ;
    skos:prefLabel "Burger king"@en .

piirritev:OsmNameCalle2 a skos:Concept ;
    piirrite:osmId "Calle_2" ;
    rdfs:subClassOf piirrite:OsmEntity ;
    skos:definition ""@en ;
    skos:inScheme piirritev:OsmName ;
    skos:prefLabel "Calle 2"@en .

piirritev:OsmNameCalle3 a skos:Concept ;
    piirrite:osmId "Calle_3" ;
    rdfs:subClassOf piirrite:OsmEntity ;
    skos:definition ""@en ;
    skos:inScheme piirritev:OsmName ;
    skos:prefLabel "Calle 3"@en .

piirritev:OsmNameChurchStreet a skos:Concept ;
    piirrite:osmId "Church_Street" ;
    rdfs:subClassOf piirrite:OsmEntity ;
    skos:definition ""@en ;
    skos:inScheme piirritev:OsmName ;
    skos:prefLabel "Church street"@en .

piirritev:OsmNameDollarGeneral a skos:Concept ;
    piirrite:osmId "Dollar_General" ;
    rdfs:subClassOf piirrite:OsmEntity ;
    skos:definition ""@en ;
    skos:inScheme piirritev:OsmName ;
    skos:prefLabel "Dollar general"@en .

piirritev:OsmNameDorfstrae a skos:Concept ;
    piirrite:osmId "Dorfstrae" ;
    rdfs:subClassOf piirrite:OsmEntity ;
    skos:definition ""@en ;
    skos:inScheme piirritev:OsmName ;
    skos:prefLabel "Dorfstrae"@en .

piirritev:OsmNameGartenstrae a skos:Concept ;
    piirrite:osmId "Gartenstrae" ;
    rdfs:subClassOf piirrite:OsmEntity ;
    skos:definition ""@en ;
    skos:inScheme piirritev:OsmName ;
    skos:prefLabel "Gartenstrae"@en .

piirritev:OsmNameGrandeRue a skos:Concept ;
    piirrite:osmId "Grande_Rue" ;
    rdfs:subClassOf piirrite:OsmEntity ;
    skos:definition ""@en ;
    skos:inScheme piirritev:OsmName ;
    skos:prefLabel "Grande rue"@en .

piirritev:OsmNameHauptstrae a skos:Concept ;
    piirrite:osmId "Hauptstrae" ;
    rdfs:subClassOf piirrite:OsmEntity ;
    skos:definition ""@en ;
    skos:inScheme piirritev:OsmName ;
    skos:prefLabel "Hauptstrae"@en .

piirritev:OsmNameHighStreet a skos:Concept ;
    piirrite:osmId "High_Street" ;
    rdfs:subClassOf piirrite:OsmEntity ;
    skos:definition ""@en ;
    skos:inScheme piirritev:OsmName ;
    skos:prefLabel "High street"@en .

piirritev:OsmNameHomestead a skos:Concept ;
    piirrite:osmId "Homestead" ;
    rdfs:subClassOf piirrite:OsmEntity ;
    skos:definition ""@en ;
    skos:inScheme piirritev:OsmName ;
    skos:prefLabel "Homestead"@en .

piirritev:OsmNameKfc a skos:Concept ;
    piirrite:hasRelatedOsmTag piirrite:hasOsmKfcAmenity ;
    piirrite:osmId "KFC" ;
    rdfs:subClassOf piirrite:OsmEntity ;
    skos:definition "American fast food restaurant chain specializing in fried chicken."@en ;
    skos:inScheme piirritev:OsmName ;
    skos:prefLabel "Kfc"@en .

piirritev:OsmNameLidl a skos:Concept ;
    piirrite:osmId "Lidl" ;
    rdfs:subClassOf piirrite:OsmEntity ;
    skos:definition ""@en ;
    skos:inScheme piirritev:OsmName ;
    skos:prefLabel "Lidl"@en .

piirritev:OsmNameLindenstrae a skos:Concept ;
    piirrite:osmId "Lindenstrae" ;
    rdfs:subClassOf piirrite:OsmEntity ;
    skos:definition ""@en ;
    skos:inScheme piirritev:OsmName ;
    skos:prefLabel "Lindenstrae"@en .

piirritev:OsmNameMainStreet a skos:Concept ;
    piirrite:osmId "Main_Street" ;
    rdfs:subClassOf piirrite:OsmEntity ;
    skos:definition ""@en ;
    skos:inScheme piirritev:OsmName ;
    skos:prefLabel "Main street"@en .

piirritev:OsmNameMcdonalds a skos:Concept ;
    piirrite:osmId "McDonalds" ;
    rdfs:subClassOf piirrite:OsmEntity ;
    skos:definition ""@en ;
    skos:inScheme piirritev:OsmName ;
    skos:prefLabel "Mcdonalds"@en .

piirritev:OsmNameOzon a skos:Concept ;
    piirrite:osmId "Ozon" ;
    rdfs:subClassOf piirrite:OsmEntity ;
    skos:definition ""@en ;
    skos:inScheme piirritev:OsmName ;
    skos:prefLabel "Ozon"@en .

piirritev:OsmNameRiverRoad a skos:Concept ;
    piirrite:osmId "River_Road" ;
    rdfs:subClassOf piirrite:OsmEntity ;
    skos:definition ""@en ;
    skos:inScheme piirritev:OsmName ;
    skos:prefLabel "River road"@en .

piirritev:OsmNameRuePrincipale a skos:Concept ;
    piirrite:osmId "Rue_Principale" ;
    rdfs:subClassOf piirrite:OsmEntity ;
    skos:definition ""@en ;
    skos:inScheme piirritev:OsmName ;
    skos:prefLabel "Rue principale"@en .

piirritev:OsmNameSchulstrae a skos:Concept ;
    piirrite:osmId "Schulstrae" ;
    rdfs:subClassOf piirrite:OsmEntity ;
    skos:definition ""@en ;
    skos:inScheme piirritev:OsmName ;
    skos:prefLabel "Schulstrae"@en .

piirritev:OsmNameShell a skos:Concept ;
    piirrite:osmId "Shell" ;
    rdfs:subClassOf piirrite:OsmEntity ;
    skos:definition ""@en ;
    skos:inScheme piirritev:OsmName ;
    skos:prefLabel "Shell"@en .

piirritev:OsmNameStarbucks a skos:Concept ;
    piirrite:osmId "Starbucks" ;
    rdfs:subClassOf piirrite:OsmEntity ;
    skos:definition ""@en ;
    skos:inScheme piirritev:OsmName ;
    skos:prefLabel "Starbucks"@en .

piirritev:OsmNameStationRoad a skos:Concept ;
    piirrite:osmId "Station_Road" ;
    rdfs:subClassOf piirrite:OsmEntity ;
    skos:definition ""@en ;
    skos:inScheme piirritev:OsmName ;
    skos:prefLabel "Station road"@en .

piirritev:OsmNameSubway a skos:Concept ;
    piirrite:hasRelatedOsmTag piirrite:hasOsmSubwayAmenity ;
    piirrite:osmId "Subway" ;
    rdfs:subClassOf piirrite:OsmEntity ;
    skos:definition "Name typically used for eateries from chain of fast food restaurants selling sandwiches."@en ;
    skos:inScheme piirritev:OsmName ;
    skos:prefLabel "Subway"@en .

piirritev:OsmNameViaRoma a skos:Concept ;
    piirrite:osmId "Via_Roma" ;
    rdfs:subClassOf piirrite:OsmEntity ;
    skos:definition ""@en ;
    skos:inScheme piirritev:OsmName ;
    skos:prefLabel "Via roma"@en .

piirritev:OsmName a skos:Concept ;
    piirrite:osmId "_" ;
    rdfs:subClassOf piirrite:OsmEntity ;
    skos:definition ""@en ;
    skos:inScheme piirritev:OsmName ;
    skos:prefLabel " "@en .

piirritev:OsmName a skos:Concept ;
    piirrite:osmId "" ;
    rdfs:subClassOf piirrite:OsmEntity ;
    skos:definition ""@en ;
    skos:inScheme piirritev:OsmName ;
    skos:prefLabel ""@en .

piirritev:OsmName a skos:Concept ;
    piirrite:osmId "_" ;
    rdfs:subClassOf piirrite:OsmEntity ;
    skos:definition ""@en ;
    skos:inScheme piirritev:OsmName ;
    skos:prefLabel " "@en .

piirritev:OsmName a skos:Concept ;
    piirrite:osmId "_" ;
    rdfs:subClassOf piirrite:OsmEntity ;
    skos:definition ""@en ;
    skos:inScheme piirritev:OsmName ;
    skos:prefLabel " "@en .

piirritev:OsmName a skos:Concept ;
    piirrite:osmId "_" ;
    rdfs:subClassOf piirrite:OsmEntity ;
    skos:definition ""@en ;
    skos:inScheme piirritev:OsmName ;
    skos:prefLabel " "@en .

piirritev:OsmName a skos:Concept ;
    piirrite:osmId "_" ;
    rdfs:subClassOf piirrite:OsmEntity ;
    skos:definition ""@en ;
    skos:inScheme piirritev:OsmName ;
    skos:prefLabel " "@en .

piirritev:OsmName a skos:Concept ;
    piirrite:osmId "" ;
    rdfs:subClassOf piirrite:OsmEntity ;
    skos:definition ""@en ;
    skos:inScheme piirritev:OsmName ;
    skos:prefLabel ""@en .

piirritev:OsmName a skos:Concept ;
    piirrite:osmId "_" ;
    rdfs:subClassOf piirrite:OsmEntity ;
    skos:definition ""@en ;
    skos:inScheme piirritev:OsmName ;
    skos:prefLabel " "@en .

piirritev:OsmName a skos:Concept ;
    piirrite:osmId "_" ;
    rdfs:subClassOf piirrite:OsmEntity ;
    skos:definition ""@en ;
    skos:inScheme piirritev:OsmName ;
    skos:prefLabel " "@en .

piirritev:OsmName a skos:Concept ;
    piirrite:osmId "_" ;
    rdfs:subClassOf piirrite:OsmEntity ;
    skos:definition ""@en ;
    skos:inScheme piirritev:OsmName ;
    skos:prefLabel " "@en .

piirritev:OsmName a skos:Concept ;
    piirrite:osmId "_" ;
    rdfs:subClassOf piirrite:OsmEntity ;
    skos:definition ""@en ;
    skos:inScheme piirritev:OsmName ;
    skos:prefLabel " "@en .

piirritev:OsmName a skos:Concept ;
    piirrite:osmId "_" ;
    rdfs:subClassOf piirrite:OsmEntity ;
    skos:definition ""@en ;
    skos:inScheme piirritev:OsmName ;
    skos:prefLabel " "@en .

piirritev:OsmName a skos:Concept ;
    piirrite:osmId "_" ;
    rdfs:subClassOf piirrite:OsmEntity ;
    skos:definition ""@en ;
    skos:inScheme piirritev:OsmName ;
    skos:prefLabel " "@en .

piirritev:OsmName a skos:Concept ;
    piirrite:osmId "" ;
    rdfs:subClassOf piirrite:OsmEntity ;
    skos:definition ""@en ;
    skos:inScheme piirritev:OsmName ;
    skos:prefLabel ""@en .

piirritev:OsmName- a skos:Concept ;
    piirrite:osmId "-" ;
    rdfs:subClassOf piirrite:OsmEntity ;
    skos:definition ""@en ;
    skos:inScheme piirritev:OsmName ;
    skos:prefLabel "-"@en .

piirritev:OsmName a skos:Concept ;
    piirrite:osmId "" ;
    rdfs:subClassOf piirrite:OsmEntity ;
    skos:definition ""@en ;
    skos:inScheme piirritev:OsmName ;
    skos:prefLabel ""@en .

piirritev:OsmNatName a skos:ConceptScheme ;
    piirrite:osmId "nat_name" ;
    skos:definition ""@en ;
    skos:prefLabel "Nat name, types"@en .

piirritev:OsmNatRef a skos:ConceptScheme ;
    piirrite:osmId "nat_ref" ;
    skos:definition "National reference (\"Nationally referenced as...\")."@en ;
    skos:prefLabel "Nat ref, types"@en .

piirritev:OsmNaturalBareRock a skos:Concept ;
    piirrite:osmId "bare_rock" ;
    rdfs:subClassOf piirrite:OsmEntity ;
    skos:definition "An area with sparse or no vegetation, so that the bedrock becomes visible osmcarto-rendering=File:Bare rock.png osmcarto-rendering-size=100px"@en ;
    skos:inScheme piirritev:OsmNatural ;
    skos:prefLabel "Bare rock"@en .

piirritev:OsmNaturalBay a skos:Concept ;
    piirrite:hasRelatedOsmTag piirrite:hasOsmBayWikidata,
        piirrite:hasOsmBayWikimediaCommons,
        piirrite:hasOsmBayWikipedia ;
    piirrite:osmId "bay" ;
    rdfs:subClassOf piirrite:OsmEntity ;
    skos:definition "Named area of water mostly surrounded by land but with level connection to the ocean or a lake.  osmcarto-rendering = File:Rendering-natural-bay.png  osmcarto-rendering-size = 125px"@en ;
    skos:inScheme piirritev:OsmNatural ;
    skos:prefLabel "Bay"@en .

piirritev:OsmNaturalBeach a skos:Concept ;
    piirrite:hasRelatedOsmTag piirrite:hasOsmBeachFee,
        piirrite:hasOsmBeachLifeguard,
        piirrite:hasOsmBeachName,
        piirrite:hasOsmBeachSupervised,
        piirrite:hasOsmBeachSurface ;
    piirrite:osmId "beach" ;
    rdfs:subClassOf piirrite:OsmEntity ;
    skos:definition "Landform along a body of water which consists of sand, shingle or other loose material.  osmcarto-rendering = File:Rendering-area-natural-beach.png  osmcarto-rendering-size = 100px"@en ;
    skos:inScheme piirritev:OsmNatural ;
    skos:prefLabel "Beach"@en .

piirritev:OsmNaturalCape a skos:Concept ;
    piirrite:hasRelatedOsmTag piirrite:hasOsmCapeName ;
    piirrite:osmId "cape" ;
    rdfs:subClassOf piirrite:OsmEntity ;
    skos:definition "A piece of elevated land sticking out into the sea or large lake."@en ;
    skos:inScheme piirritev:OsmNatural ;
    skos:prefLabel "Cape"@en .

piirritev:OsmNaturalCaveEntrance a skos:Concept ;
    piirrite:hasRelatedOsmTag piirrite:hasOsmCaveEntranceAccess,
        piirrite:hasOsmCaveEntranceAltName,
        piirrite:hasOsmCaveEntranceBarrier,
        piirrite:hasOsmCaveEntranceDirection,
        piirrite:hasOsmCaveEntranceEle,
        piirrite:hasOsmCaveEntranceFee,
        piirrite:hasOsmCaveEntranceLocName,
        piirrite:hasOsmCaveEntranceMaterial,
        piirrite:hasOsmCaveEntranceName,
        piirrite:hasOsmCaveEntranceNatural,
        piirrite:hasOsmCaveEntranceOpeningHours ;
    piirrite:osmId "cave_entrance" ;
    rdfs:subClassOf piirrite:OsmEntity ;
    skos:definition "An entrance to a cave: a natural underground space large enough for a human to enter osmcarto-rendering = File:Cave.14.svg osmcarto-rendering-size = 28px"@en ;
    skos:inScheme piirritev:OsmNatural ;
    skos:prefLabel "Cave entrance"@en .

piirritev:OsmNaturalCliff a skos:Concept ;
    piirrite:hasRelatedOsmTag piirrite:hasOsmCliffHeight,
        piirrite:hasOsmCliffName,
        piirrite:hasOsmCliffSurface ;
    piirrite:osmId "cliff" ;
    rdfs:subClassOf piirrite:OsmEntity ;
    skos:definition "A vertical or almost vertical natural drop in terrain, usually with a bare rock surface. The bottom of the cliff is on the right side of the way. osmcarto-rendering=File:Natural cliff-125.png osmcarto-rendering-size=125px"@en ;
    skos:inScheme piirritev:OsmNatural ;
    skos:prefLabel "Cliff"@en .

piirritev:OsmNaturalCoastline a skos:Concept ;
    piirrite:osmId "coastline" ;
    rdfs:subClassOf piirrite:OsmEntity ;
    skos:definition "The line between sea and land indicating mean high water (springs): the water lies on the right side of the way. osmcarto-rendering=File:Rendering-area-natural-coastline.png osmcarto-rendering-size=125px"@en ;
    skos:inScheme piirritev:OsmNatural ;
    skos:prefLabel "Coastline"@en .

piirritev:OsmNaturalCrevasse a skos:Concept ;
    piirrite:osmId "crevasse" ;
    rdfs:subClassOf piirrite:OsmEntity ;
    skos:definition "A large crack in a glacier"@en ;
    skos:inScheme piirritev:OsmNatural ;
    skos:prefLabel "Crevasse"@en .

piirritev:OsmNaturalEarthBank a skos:Concept ;
    piirrite:hasRelatedOsmTag piirrite:hasOsmEarthBankDepth,
        piirrite:hasOsmEarthBankSurface ;
    piirrite:osmId "earth_bank" ;
    rdfs:subClassOf piirrite:OsmEntity ;
    skos:definition "Large erosion gully or steep earth bank."@en ;
    skos:inScheme piirritev:OsmNatural ;
    skos:prefLabel "Earth bank"@en .

piirritev:OsmNaturalFell a skos:Concept ;
    piirrite:hasRelatedOsmTag piirrite:hasOsmFellEle,
        piirrite:hasOsmFellName ;
    piirrite:osmId "fell" ;
    rdfs:subClassOf piirrite:OsmEntity ;
    skos:definition "Habitat above tree line covered with grass, dwarf shrubs and mosses."@en ;
    skos:inScheme piirritev:OsmNatural ;
    skos:prefLabel "Fell"@en .

piirritev:OsmNaturalGlacier a skos:Concept ;
    piirrite:hasRelatedOsmTag piirrite:hasOsmGlacierDirection,
        piirrite:hasOsmGlacierName,
        piirrite:hasOsmGlacierNatural,
        piirrite:hasOsmGlacierSurface,
        piirrite:hasOsmGlacierType ;
    piirrite:osmId "glacier" ;
    rdfs:subClassOf piirrite:OsmEntity ;
    skos:definition "A permanent body of ice formed naturally from snow that is moving under its own weight. osmcarto-rendering-area = File:Glacier-area.png osmcarto-rendering-area-size = 100px"@en ;
    skos:inScheme piirritev:OsmNatural ;
    skos:prefLabel "Glacier"@en .

piirritev:OsmNaturalGrassland a skos:Concept ;
    piirrite:hasRelatedOsmTag piirrite:hasOsmGrasslandType ;
    piirrite:osmId "grassland" ;
    rdfs:subClassOf piirrite:OsmEntity ;
    skos:definition "An area where the vegetation is dominated by grasses and other herbaceous (non-woody) plants. osmcarto-rendering=File:Natural-Grassland.png osmcarto-rendering-size=100px"@en ;
    skos:inScheme piirritev:OsmNatural ;
    skos:prefLabel "Grassland"@en .

piirritev:OsmNaturalGully a skos:Concept ;
    piirrite:hasRelatedOsmTag piirrite:hasOsmGullyDepth,
        piirrite:hasOsmGullySurface ;
    piirrite:osmId "gully" ;
    rdfs:subClassOf piirrite:OsmEntity ;
    skos:definition "Small scale cut in relief created by water erosion."@en ;
    skos:inScheme piirritev:OsmNatural ;
    skos:prefLabel "Gully"@en .

piirritev:OsmNaturalHeath a skos:Concept ;
    piirrite:hasRelatedOsmTag piirrite:hasOsmHeathNatural ;
    piirrite:osmId "heath" ;
    rdfs:subClassOf piirrite:OsmEntity ;
    skos:definition "A dwarf-shrub habitat, characterised by open, low growing woody vegetation, often dominated by plants of the Ericaceae. osmcarto-rendering=File:Rendering-area-natural-heath-yellow.png osmcarto-rendering-size=100px"@en ;
    skos:inScheme piirritev:OsmNatural ;
    skos:prefLabel "Heath"@en .

piirritev:OsmNaturalHill a skos:Concept ;
    piirrite:hasRelatedOsmTag piirrite:hasOsmHillEle,
        piirrite:hasOsmHillName ;
    piirrite:osmId "hill" ;
    rdfs:subClassOf piirrite:OsmEntity ;
    skos:definition "A hill is a landform that is elevated above the surrounding terrain, but is smaller than a mountain."@en ;
    skos:inScheme piirritev:OsmNatural ;
    skos:prefLabel "Hill"@en .

piirritev:OsmNaturalLand a skos:Concept ;
    piirrite:osmId "land" ;
    rdfs:subClassOf piirrite:OsmEntity ;
    skos:definition "Using this tag is discouraged, use multipolygon relation for islands in lakes and rivers or tag:natural=coastline and tag:place=island for islands in the sea instead."@en ;
    skos:inScheme piirritev:OsmNatural ;
    skos:prefLabel "Land"@en .

piirritev:OsmNaturalLandform a skos:Concept ;
    piirrite:osmId "landform" ;
    rdfs:subClassOf piirrite:OsmEntity ;
    skos:definition "A various geological features."@en ;
    skos:inScheme piirritev:OsmNatural ;
    skos:prefLabel "Landform"@en .

piirritev:OsmNaturalMud a skos:Concept ;
    piirrite:osmId "mud" ;
    rdfs:subClassOf piirrite:OsmEntity ;
    skos:definition "Area covered with mud: water saturated fine grained soil without significant plant growth. osmcarto-rendering-area=File:Natural_mud_100.png osmcarto-rendering-area-size=100px"@en ;
    skos:inScheme piirritev:OsmNatural ;
    skos:prefLabel "Mud"@en .

piirritev:OsmNaturalPeak a skos:Concept ;
    piirrite:hasRelatedOsmTag piirrite:hasOsmPeakCairn,
        piirrite:hasOsmPeakEle,
        piirrite:hasOsmPeakName ;
    piirrite:osmId "peak" ;
    rdfs:subClassOf piirrite:OsmEntity ;
    skos:definition "The top (summit) of a hill or mountain. osmcarto-rendering=File:Peak-8.svg osmcarto-rendering-size=16px"@en ;
    skos:inScheme piirritev:OsmNatural ;
    skos:prefLabel "Peak"@en .

piirritev:OsmNaturalReef a skos:Concept ;
    piirrite:hasRelatedOsmTag piirrite:hasOsmReefName,
        piirrite:hasOsmReefType ;
    piirrite:osmId "reef" ;
    rdfs:subClassOf piirrite:OsmEntity ;
    skos:definition "A feature (rock, sandbar, coral, etc) lying permanently beneath the surface of the water. osmcarto-rendering=File:Natural reef-100.png"@en ;
    skos:inScheme piirritev:OsmNatural ;
    skos:prefLabel "Reef"@en .

piirritev:OsmNaturalRidge a skos:Concept ;
    piirrite:hasRelatedOsmTag piirrite:hasOsmRidgeName ;
    piirrite:osmId "ridge" ;
    rdfs:subClassOf piirrite:OsmEntity ;
    skos:definition "A mountain landform with a continuous elevated crest or linear hill osmcarto-rendering=File:Natural-ridge-125.png osmcarto-rendering-size=125px"@en ;
    skos:inScheme piirritev:OsmNatural ;
    skos:prefLabel "Ridge"@en .

piirritev:OsmNaturalRock a skos:Concept ;
    piirrite:hasRelatedOsmTag piirrite:hasOsmRockName ;
    piirrite:osmId "rock" ;
    rdfs:subClassOf piirrite:OsmEntity ;
    skos:definition "A notable rock or group of rocks attached to the underlying bedrock"@en ;
    skos:inScheme piirritev:OsmNatural ;
    skos:prefLabel "Rock"@en .

piirritev:OsmNaturalSaddle a skos:Concept ;
    piirrite:hasRelatedOsmTag piirrite:hasOsmSaddleDirection,
        piirrite:hasOsmSaddleEle,
        piirrite:hasOsmSaddleName ;
    piirrite:osmId "saddle" ;
    rdfs:subClassOf piirrite:OsmEntity ;
    skos:definition "The lowest point along a ridge or between two mountain tops. osmcarto-rendering=File:Saddle-8.svg osmcarto-rendering-size=20px"@en ;
    skos:inScheme piirritev:OsmNatural ;
    skos:prefLabel "Saddle"@en .

piirritev:OsmNaturalSand a skos:Concept ;
    piirrite:hasRelatedOsmTag piirrite:hasOsmSandLandcover,
        piirrite:hasOsmSandNatural,
        piirrite:hasOsmSandResource ;
    piirrite:osmId "sand" ;
    rdfs:subClassOf piirrite:OsmEntity ;
    skos:definition "An area covered by sand with no or very little vegetation. osmcarto-rendering=File:Rendering-area-sand.png osmcarto-rendering-size=100px"@en ;
    skos:inScheme piirritev:OsmNatural ;
    skos:prefLabel "Sand"@en .

piirritev:OsmNaturalScree a skos:Concept ;
    piirrite:osmId "scree" ;
    rdfs:subClassOf piirrite:OsmEntity ;
    skos:definition "Unconsolidated angular stones formed by rockfall and weathering from adjacent rock faces. osmcarto-rendering=File:Bare rock-125.png osmcarto-rendering-size=100px"@en ;
    skos:inScheme piirritev:OsmNatural ;
    skos:prefLabel "Scree"@en .

piirritev:OsmNaturalScrub a skos:Concept ;
    piirrite:hasRelatedOsmTag piirrite:hasOsmScrubLeafCycle,
        piirrite:hasOsmScrubLeafType,
        piirrite:hasOsmScrubName ;
    piirrite:osmId "scrub" ;
    rdfs:subClassOf piirrite:OsmEntity ;
    skos:definition "Uncultivated land covered with shrubs, bushes or stunted trees.  osmcarto-rendering = File:Rendering-area-natural-scrub.png  osmcarto-rendering-size = 100px"@en ;
    skos:inScheme piirritev:OsmNatural ;
    skos:prefLabel "Scrub"@en .

piirritev:OsmNaturalShingle a skos:Concept ;
    piirrite:osmId "shingle" ;
    rdfs:subClassOf piirrite:OsmEntity ;
    skos:definition "An accumulation of rounded rock fragments on a beach or riverbed."@en ;
    skos:inScheme piirritev:OsmNatural ;
    skos:prefLabel "Shingle"@en .

piirritev:OsmNaturalShrub a skos:Concept ;
    piirrite:hasRelatedOsmTag piirrite:hasOsmShrubCheckDate,
        piirrite:hasOsmShrubColour,
        piirrite:hasOsmShrubFruit,
        piirrite:hasOsmShrubGenus,
        piirrite:hasOsmShrubHeight,
        piirrite:hasOsmShrubName,
        piirrite:hasOsmShrubSpecies,
        piirrite:hasOsmShrubTaxon,
        piirrite:hasOsmShrubWidth ;
    piirrite:osmId "shrub" ;
    rdfs:subClassOf piirrite:OsmEntity ;
    skos:definition "A small to medium-sized single shrub, usually less than 6 meters tall."@en ;
    skos:inScheme piirritev:OsmNatural ;
    skos:prefLabel "Shrub"@en .

piirritev:OsmNaturalShrubbery a skos:Concept ;
    piirrite:hasRelatedOsmTag piirrite:hasOsmShrubberyGenus,
        piirrite:hasOsmShrubberyHeight,
        piirrite:hasOsmShrubberyLeafCycle,
        piirrite:hasOsmShrubberyLeafType,
        piirrite:hasOsmShrubberySpecies,
        piirrite:hasOsmShrubberyTaxon ;
    piirrite:osmId "shrubbery" ;
    rdfs:subClassOf piirrite:OsmEntity ;
    skos:definition "An area of woody shrubbery that is actively maintained or pruned by humans. A slightly wilder look is also possible."@en ;
    skos:inScheme piirritev:OsmNatural ;
    skos:prefLabel "Shrubbery"@en .

piirritev:OsmNaturalSinkhole a skos:Concept ;
    piirrite:hasRelatedOsmTag piirrite:hasOsmSinkholeType ;
    piirrite:osmId "sinkhole" ;
    rdfs:subClassOf piirrite:OsmEntity ;
    skos:definition "A natural depression or hole in the surface topography."@en ;
    skos:inScheme piirritev:OsmNatural ;
    skos:prefLabel "Sinkhole"@en .

piirritev:OsmNaturalSpring a skos:Concept ;
    piirrite:hasRelatedOsmTag piirrite:hasOsmSpringDrinkingWater,
        piirrite:hasOsmSpringKarst,
        piirrite:hasOsmSpringName,
        piirrite:hasOsmSpringSeasonal,
        piirrite:hasOsmSpringSinkhole ;
    piirrite:osmId "spring" ;
    rdfs:subClassOf piirrite:OsmEntity ;
    skos:definition "A place where ground water flows naturally from the ground osmcarto-rendering=File:Spring-14.svg osmcarto-rendering-size=28px"@en ;
    skos:inScheme piirritev:OsmNatural ;
    skos:prefLabel "Spring"@en .

piirritev:OsmNaturalStone a skos:Concept ;
    piirrite:hasRelatedOsmTag piirrite:hasOsmStoneHeight,
        piirrite:hasOsmStoneName,
        piirrite:hasOsmStoneWidth ;
    piirrite:osmId "stone" ;
    rdfs:subClassOf piirrite:OsmEntity ;
    skos:definition "A single notable freestanding rock, which may differ from the composition of the terrain it lies in."@en ;
    skos:inScheme piirritev:OsmNatural ;
    skos:prefLabel "Stone"@en .

piirritev:OsmNaturalTree a skos:Concept ;
    piirrite:hasRelatedOsmTag piirrite:hasOsmTreeCircumference,
        piirrite:hasOsmTreeGenus,
        piirrite:hasOsmTreeHeight,
        piirrite:hasOsmTreeLeafType,
        piirrite:hasOsmTreeSpecies,
        piirrite:hasOsmTreeStartDate,
        piirrite:hasOsmTreeTaxon ;
    piirrite:osmId "tree" ;
    rdfs:subClassOf piirrite:OsmEntity ;
    skos:definition "A single tree."@en ;
    skos:inScheme piirritev:OsmNatural ;
    skos:prefLabel "Tree"@en .

piirritev:OsmNaturalTreeRow a skos:Concept ;
    piirrite:hasRelatedOsmTag piirrite:hasOsmTreeRowHeight,
        piirrite:hasOsmTreeRowLeafCycle,
        piirrite:hasOsmTreeRowLeafType ;
    piirrite:osmId "tree_row" ;
    rdfs:subClassOf piirrite:OsmEntity ;
    skos:definition "A line of trees. osmcarto-rendering = File:Rendering-natural tree row-mapnik.png osmcarto-rendering-size = 100px"@en ;
    skos:inScheme piirritev:OsmNatural ;
    skos:prefLabel "Tree row"@en .

piirritev:OsmNaturalTreeStump a skos:Concept ;
    piirrite:osmId "tree_stump" ;
    rdfs:subClassOf piirrite:OsmEntity ;
    skos:definition "A base remaining from a cut down or broken tree."@en ;
    skos:inScheme piirritev:OsmNatural ;
    skos:prefLabel "Tree stump"@en .

piirritev:OsmNaturalValley a skos:Concept ;
    piirrite:hasRelatedOsmTag piirrite:hasOsmValleyName,
        piirrite:hasOsmValleyWaterway ;
    piirrite:osmId "valley" ;
    rdfs:subClassOf piirrite:OsmEntity ;
    skos:definition "A natural depression flanked by ridges or ranges of mountains or hills"@en ;
    skos:inScheme piirritev:OsmNatural ;
    skos:prefLabel "Valley"@en .

piirritev:OsmNaturalWater a skos:Concept ;
    piirrite:hasRelatedOsmTag piirrite:hasOsmWaterIntermittent,
        piirrite:hasOsmWaterName,
        piirrite:hasOsmWaterSalt,
        piirrite:hasOsmWaterType ;
    piirrite:osmId "water" ;
    rdfs:subClassOf piirrite:OsmEntity ;
    skos:definition "Any inland body of water, from natural such as a lake or pond to artificial like a moat or canal.  osmcarto-rendering = File:Base layer water.png  osmcarto-rendering-size = 100px"@en ;
    skos:inScheme piirritev:OsmNatural ;
    skos:prefLabel "Water"@en .

piirritev:OsmNaturalWetland a skos:Concept ;
    piirrite:hasRelatedOsmTag piirrite:hasOsmWetlandType ;
    piirrite:osmId "wetland" ;
    rdfs:subClassOf piirrite:OsmEntity ;
    skos:definition "A natural area subject to inundation or with waterlogged ground osmcarto-rendering=File:Rendering-area-natural-marsh-osmarender.png osmcarto-rendering-size=125px"@en ;
    skos:inScheme piirritev:OsmNatural ;
    skos:prefLabel "Wetland"@en .

piirritev:OsmNaturalWood a skos:Concept ;
    piirrite:hasRelatedOsmTag piirrite:hasOsmWoodLeafCycle,
        piirrite:hasOsmWoodLeafType,
        piirrite:hasOsmWoodManaged,
        piirrite:hasOsmWoodName,
        piirrite:hasOsmWoodOperator ;
    piirrite:osmId "wood" ;
    rdfs:subClassOf piirrite:OsmEntity ;
    skos:definition "Tree-covered area (a 'forest' or 'wood') osmcarto-rendering=File:Rendering-area-natural-wood.png osmcarto-rendering-size=100px"@en ;
    skos:inScheme piirritev:OsmNatural ;
    skos:prefLabel "Wood"@en .

piirritev:OsmNavigationaidAls a skos:Concept ;
    piirrite:osmId "als" ;
    rdfs:subClassOf piirrite:OsmEntity ;
    skos:definition "Approach Lighting System"@en ;
    skos:inScheme piirritev:OsmNavigationaid ;
    skos:prefLabel "Als"@en .

piirritev:OsmNavigationaidRwc a skos:Concept ;
    piirrite:osmId "rwc" ;
    rdfs:subClassOf piirrite:OsmEntity ;
    skos:definition "Beaconing runway centerline"@en ;
    skos:inScheme piirritev:OsmNavigationaid ;
    skos:prefLabel "Rwc"@en .

piirritev:OsmNavigationaidRwe a skos:Concept ;
    piirrite:osmId "rwe" ;
    rdfs:subClassOf piirrite:OsmEntity ;
    skos:definition "Beaconing runway edge"@en ;
    skos:inScheme piirritev:OsmNavigationaid ;
    skos:prefLabel "Rwe"@en .

piirritev:OsmNavigationaidTdz a skos:Concept ;
    piirrite:osmId "tdz" ;
    rdfs:subClassOf piirrite:OsmEntity ;
    skos:definition "Touchdown zone lighting"@en ;
    skos:inScheme piirritev:OsmNavigationaid ;
    skos:prefLabel "Tdz"@en .

piirritev:OsmNavigationaidTxc a skos:Concept ;
    piirrite:osmId "txc" ;
    rdfs:subClassOf piirrite:OsmEntity ;
    skos:definition "Beaconing taxiway centreline"@en ;
    skos:inScheme piirritev:OsmNavigationaid ;
    skos:prefLabel "Txc"@en .

piirritev:OsmNavigationaidTxe a skos:Concept ;
    piirrite:osmId "txe" ;
    rdfs:subClassOf piirrite:OsmEntity ;
    skos:definition "Beaconing taxiway edge"@en ;
    skos:inScheme piirritev:OsmNavigationaid ;
    skos:prefLabel "Txe"@en .

piirritev:OsmNetworkAcTransit a skos:Concept ;
    piirrite:osmId "AC_Transit" ;
    rdfs:subClassOf piirrite:OsmEntity ;
    skos:definition ""@en ;
    skos:inScheme piirritev:OsmNetwork ;
    skos:prefLabel "Ac transit"@en .

piirritev:OsmNetworkCarrisMetropolitana a skos:Concept ;
    piirrite:osmId "Carris_Metropolitana" ;
    rdfs:subClassOf piirrite:OsmEntity ;
    skos:definition ""@en ;
    skos:inScheme piirritev:OsmNetwork ;
    skos:prefLabel "Carris metropolitana"@en .

piirritev:OsmNetworkCta a skos:Concept ;
    piirrite:osmId "CTA" ;
    rdfs:subClassOf piirrite:OsmEntity ;
    skos:definition ""@en ;
    skos:inScheme piirritev:OsmNetwork ;
    skos:prefLabel "Cta"@en .

piirritev:OsmNetworkHelloCycling a skos:Concept ;
    piirrite:osmId "HELLO_CYCLING" ;
    rdfs:subClassOf piirrite:OsmEntity ;
    skos:definition ""@en ;
    skos:inScheme piirritev:OsmNetwork ;
    skos:prefLabel "Hello cycling"@en .

piirritev:OsmNetworkHvv a skos:Concept ;
    piirrite:osmId "HVV" ;
    rdfs:subClassOf piirrite:OsmEntity ;
    skos:definition ""@en ;
    skos:inScheme piirritev:OsmNetwork ;
    skos:prefLabel "Hvv"@en .

piirritev:OsmNetworkLcn a skos:Concept ;
    piirrite:hasRelatedOsmTag piirrite:hasOsmLcnName,
        piirrite:hasOsmLcnOperator,
        piirrite:hasOsmLcnRef ;
    piirrite:osmId "lcn" ;
    rdfs:subClassOf piirrite:OsmEntity ;
    skos:definition "Specifies the network as a local route."@en ;
    skos:inScheme piirritev:OsmNetwork ;
    skos:prefLabel "Lcn"@en .

piirritev:OsmNetworkLwn a skos:Concept ;
    piirrite:hasRelatedOsmTag piirrite:hasOsmLwnName,
        piirrite:hasOsmLwnOperator,
        piirrite:hasOsmLwnRef ;
    piirrite:osmId "lwn" ;
    rdfs:subClassOf piirrite:OsmEntity ;
    skos:definition "Specifies a hiking route as a local route."@en ;
    skos:inScheme piirritev:OsmNetwork ;
    skos:prefLabel "Lwn"@en .

piirritev:OsmNetworkMRso a skos:Concept ;
    piirrite:osmId "M_rso" ;
    rdfs:subClassOf piirrite:OsmEntity ;
    skos:definition ""@en ;
    skos:inScheme piirritev:OsmNetwork ;
    skos:prefLabel "M rso"@en .

piirritev:OsmNetworkMbta a skos:Concept ;
    piirrite:osmId "MBTA" ;
    rdfs:subClassOf piirrite:OsmEntity ;
    skos:definition " group ="@en ;
    skos:inScheme piirritev:OsmNetwork ;
    skos:prefLabel "Mbta"@en .

piirritev:OsmNetworkMetroTransit a skos:Concept ;
    piirrite:osmId "Metro_Transit" ;
    rdfs:subClassOf piirrite:OsmEntity ;
    skos:definition ""@en ;
    skos:inScheme piirritev:OsmNetwork ;
    skos:prefLabel "Metro transit"@en .

piirritev:OsmNetworkMitteldeutscherVerkehrsverbund a skos:Concept ;
    piirrite:osmId "Mitteldeutscher_Verkehrsverbund" ;
    rdfs:subClassOf piirrite:OsmEntity ;
    skos:definition ""@en ;
    skos:inScheme piirritev:OsmNetwork ;
    skos:prefLabel "Mitteldeutscher verkehrsverbund"@en .

piirritev:OsmNetworkNtf-4 a skos:Concept ;
    piirrite:osmId "NTF-4" ;
    rdfs:subClassOf piirrite:OsmEntity ;
    skos:definition ""@en ;
    skos:inScheme piirritev:OsmNetwork ;
    skos:prefLabel "Ntf-4"@en .

piirritev:OsmNetworkNtf-5 a skos:Concept ;
    piirrite:osmId "NTF-5" ;
    rdfs:subClassOf piirrite:OsmEntity ;
    skos:definition ""@en ;
    skos:inScheme piirritev:OsmNetwork ;
    skos:prefLabel "Ntf-5"@en .

piirritev:OsmNetworkNwn a skos:Concept ;
    piirrite:hasRelatedOsmTag piirrite:hasOsmNwnName,
        piirrite:hasOsmNwnOperator,
        piirrite:hasOsmNwnRef ;
    piirrite:osmId "nwn" ;
    rdfs:subClassOf piirrite:OsmEntity ;
    skos:definition "Specifies a hiking route as a national route."@en ;
    skos:inScheme piirritev:OsmNetwork ;
    skos:prefLabel "Nwn"@en .

piirritev:OsmNetworkNycTransit a skos:Concept ;
    piirrite:osmId "NYC_Transit" ;
    rdfs:subClassOf piirrite:OsmEntity ;
    skos:definition ""@en ;
    skos:inScheme piirritev:OsmNetwork ;
    skos:prefLabel "Nyc transit"@en .

piirritev:OsmNetworkOstwind a skos:Concept ;
    piirrite:osmId "Ostwind" ;
    rdfs:subClassOf piirrite:OsmEntity ;
    skos:definition ""@en ;
    skos:inScheme piirritev:OsmNetwork ;
    skos:prefLabel "Ostwind"@en .

piirritev:OsmNetworkRcn a skos:Concept ;
    piirrite:hasRelatedOsmTag piirrite:hasOsmRcnName,
        piirrite:hasOsmRcnOperator,
        piirrite:hasOsmRcnRef ;
    piirrite:osmId "rcn" ;
    rdfs:subClassOf piirrite:OsmEntity ;
    skos:definition "Specifies the network as a regional route."@en ;
    skos:inScheme piirritev:OsmNetwork ;
    skos:prefLabel "Rcn"@en .

piirritev:OsmNetworkRedTulum a skos:Concept ;
    piirrite:osmId "Red_Tulum" ;
    rdfs:subClassOf piirrite:OsmEntity ;
    skos:definition ""@en ;
    skos:inScheme piirritev:OsmNetwork ;
    skos:prefLabel "Red tulum"@en .

piirritev:OsmNetworkRhein-Main-Verkehrsverbund a skos:Concept ;
    piirrite:osmId "Rhein-Main-Verkehrsverbund" ;
    rdfs:subClassOf piirrite:OsmEntity ;
    skos:definition ""@en ;
    skos:inScheme piirritev:OsmNetwork ;
    skos:prefLabel "Rhein-main-verkehrsverbund"@en .

piirritev:OsmNetworkRmv a skos:Concept ;
    piirrite:osmId "RMV" ;
    rdfs:subClassOf piirrite:OsmEntity ;
    skos:definition ""@en ;
    skos:inScheme piirritev:OsmNetwork ;
    skos:prefLabel "Rmv"@en .

piirritev:OsmNetworkRwn a skos:Concept ;
    piirrite:hasRelatedOsmTag piirrite:hasOsmRwnName,
        piirrite:hasOsmRwnOperator,
        piirrite:hasOsmRwnRef ;
    piirrite:osmId "rwn" ;
    rdfs:subClassOf piirrite:OsmEntity ;
    skos:definition "Specifies a hiking route as a regional route."@en ;
    skos:inScheme piirritev:OsmNetwork ;
    skos:prefLabel "Rwn"@en .

piirritev:OsmNetworkSknetrafiken a skos:Concept ;
    piirrite:osmId "Sknetrafiken" ;
    rdfs:subClassOf piirrite:OsmEntity ;
    skos:definition ""@en ;
    skos:inScheme piirritev:OsmNetwork ;
    skos:prefLabel "Sknetrafiken"@en .

piirritev:OsmNetworkSl a skos:Concept ;
    piirrite:osmId "SL" ;
    rdfs:subClassOf piirrite:OsmEntity ;
    skos:definition ""@en ;
    skos:inScheme piirritev:OsmNetwork ;
    skos:prefLabel "Sl"@en .

piirritev:OsmNetworkSptrans a skos:Concept ;
    piirrite:osmId "SPTrans" ;
    rdfs:subClassOf piirrite:OsmEntity ;
    skos:definition ""@en ;
    skos:inScheme piirritev:OsmNetwork ;
    skos:prefLabel "Sptrans"@en .

piirritev:OsmNetworkTecl a skos:Concept ;
    piirrite:osmId "TECL" ;
    rdfs:subClassOf piirrite:OsmEntity ;
    skos:definition ""@en ;
    skos:inScheme piirritev:OsmNetwork ;
    skos:prefLabel "Tecl"@en .

piirritev:OsmNetworkTfgm a skos:Concept ;
    piirrite:osmId "TfGM" ;
    rdfs:subClassOf piirrite:OsmEntity ;
    skos:definition ""@en ;
    skos:inScheme piirritev:OsmNetwork ;
    skos:prefLabel "Tfgm"@en .

piirritev:OsmNetworkTper a skos:Concept ;
    piirrite:osmId "TPER" ;
    rdfs:subClassOf piirrite:OsmEntity ;
    skos:definition ""@en ;
    skos:inScheme piirritev:OsmNetwork ;
    skos:prefLabel "Tper"@en .

piirritev:OsmNetworkTranslink a skos:Concept ;
    piirrite:osmId "Translink" ;
    rdfs:subClassOf piirrite:OsmEntity ;
    skos:definition ""@en ;
    skos:inScheme piirritev:OsmNetwork ;
    skos:prefLabel "Translink"@en .

piirritev:OsmNetworkTransperth a skos:Concept ;
    piirrite:osmId "Transperth" ;
    rdfs:subClassOf piirrite:OsmEntity ;
    skos:definition ""@en ;
    skos:inScheme piirritev:OsmNetwork ;
    skos:prefLabel "Transperth"@en .

piirritev:OsmNetworkTransportBuses a skos:Concept ;
    piirrite:osmId "Transport_Buses" ;
    rdfs:subClassOf piirrite:OsmEntity ;
    skos:definition ""@en ;
    skos:inScheme piirritev:OsmNetwork ;
    skos:prefLabel "Transport buses"@en .

piirritev:OsmNetworkTtc a skos:Concept ;
    piirrite:osmId "TTC" ;
    rdfs:subClassOf piirrite:OsmEntity ;
    skos:definition ""@en ;
    skos:inScheme piirritev:OsmNetwork ;
    skos:prefLabel "Ttc"@en .

piirritev:OsmNetworkValleyMetro a skos:Concept ;
    piirrite:osmId "Valley_Metro" ;
    rdfs:subClassOf piirrite:OsmEntity ;
    skos:definition ""@en ;
    skos:inScheme piirritev:OsmNetwork ;
    skos:prefLabel "Valley metro"@en .

piirritev:OsmNetworkVerkehrsverbundBerlin-Brandenburg a skos:Concept ;
    piirrite:osmId "Verkehrsverbund_Berlin-Brandenburg" ;
    rdfs:subClassOf piirrite:OsmEntity ;
    skos:definition ""@en ;
    skos:inScheme piirritev:OsmNetwork ;
    skos:prefLabel "Verkehrsverbund berlin-brandenburg"@en .

piirritev:OsmNetworkVerkehrsverbundRhein-Neckar a skos:Concept ;
    piirrite:osmId "Verkehrsverbund_Rhein-Neckar" ;
    rdfs:subClassOf piirrite:OsmEntity ;
    skos:definition ""@en ;
    skos:inScheme piirritev:OsmNetwork ;
    skos:prefLabel "Verkehrsverbund rhein-neckar"@en .

piirritev:OsmNetworkVor a skos:Concept ;
    piirrite:osmId "VOR" ;
    rdfs:subClassOf piirrite:OsmEntity ;
    skos:definition ""@en ;
    skos:inScheme piirritev:OsmNetwork ;
    skos:prefLabel "Vor"@en .

piirritev:OsmNetworkVrr a skos:Concept ;
    piirrite:osmId "VRR" ;
    rdfs:subClassOf piirrite:OsmEntity ;
    skos:definition ""@en ;
    skos:inScheme piirritev:OsmNetwork ;
    skos:prefLabel "Vrr"@en .

piirritev:OsmNetworkVsttrafik a skos:Concept ;
    piirrite:osmId "Vsttrafik" ;
    rdfs:subClassOf piirrite:OsmEntity ;
    skos:definition ""@en ;
    skos:inScheme piirritev:OsmNetwork ;
    skos:prefLabel "Vsttrafik"@en .

piirritev:OsmNetworkWestfalentarif a skos:Concept ;
    piirrite:osmId "WestfalenTarif" ;
    rdfs:subClassOf piirrite:OsmEntity ;
    skos:definition ""@en ;
    skos:inScheme piirritev:OsmNetwork ;
    skos:prefLabel "Westfalentarif"@en .

piirritev:OsmNetworkZtmWarszawa a skos:Concept ;
    piirrite:osmId "ZTM_Warszawa" ;
    rdfs:subClassOf piirrite:OsmEntity ;
    skos:definition ""@en ;
    skos:inScheme piirritev:OsmNetwork ;
    skos:prefLabel "Ztm warszawa"@en .

piirritev:OsmNetworkZvv a skos:Concept ;
    piirrite:osmId "ZVV" ;
    rdfs:subClassOf piirrite:OsmEntity ;
    skos:definition ""@en ;
    skos:inScheme piirritev:OsmNetwork ;
    skos:prefLabel "Zvv"@en .

piirritev:OsmNetworkett a skos:Concept ;
    piirrite:osmId "ETT" ;
    rdfs:subClassOf piirrite:OsmEntity ;
    skos:definition ""@en ;
    skos:inScheme piirritev:OsmNetwork ;
    skos:prefLabel "ett"@en .

piirritev:OsmNetwork a skos:Concept ;
    piirrite:osmId "_" ;
    rdfs:subClassOf piirrite:OsmEntity ;
    skos:definition ""@en ;
    skos:inScheme piirritev:OsmNetwork ;
    skos:prefLabel " "@en .

piirritev:OsmNhsInterstate a skos:Concept ;
    piirrite:osmId "Interstate" ;
    rdfs:subClassOf piirrite:OsmEntity ;
    skos:definition ""@en ;
    skos:inScheme piirritev:OsmNhs ;
    skos:prefLabel "Interstate"@en .

piirritev:OsmNhsStrahnet a skos:Concept ;
    piirrite:osmId "STRAHNET" ;
    rdfs:subClassOf piirrite:OsmEntity ;
    skos:definition ""@en ;
    skos:inScheme piirritev:OsmNhs ;
    skos:prefLabel "Strahnet"@en .

piirritev:OsmNoexit a skos:ConceptScheme ;
    piirrite:osmId "noexit" ;
    skos:definition "This is a one-value key used only with the value \"yes\". See tag:noexit=yes."@en ;
    skos:prefLabel "Noexit, types"@en .

piirritev:OsmNohousenumber a skos:ConceptScheme ;
    piirrite:osmId "nohousenumber" ;
    skos:definition "For explicitly stating that no house number is assigned to a place."@en ;
    skos:prefLabel "Nohousenumber, types"@en .

piirritev:OsmNoname a skos:ConceptScheme ;
    piirrite:osmId "noname" ;
    skos:definition ""@en ;
    skos:prefLabel "Noname, types"@en .

piirritev:OsmNoref a skos:ConceptScheme ;
    piirrite:osmId "noref" ;
    skos:definition "Typically used as tag:noref=yes to explicitly state that there exists no meaningful value for key:ref tag for an object."@en ;
    skos:prefLabel "Noref, types"@en .

piirritev:OsmNoteA13-0603Xml a skos:Concept ;
    piirrite:osmId "A13-06_03_xml" ;
    rdfs:subClassOf piirrite:OsmEntity ;
    skos:definition ""@en ;
    skos:inScheme piirritev:OsmNote ;
    skos:prefLabel "A13-06 03 xml"@en .

piirritev:OsmNoteA13-0612Xml a skos:Concept ;
    piirrite:osmId "A13-06_12_xml" ;
    rdfs:subClassOf piirrite:OsmEntity ;
    skos:definition ""@en ;
    skos:inScheme piirritev:OsmNote ;
    skos:prefLabel "A13-06 12 xml"@en .

piirritev:OsmNoteC a skos:Concept ;
    piirrite:osmId "C" ;
    rdfs:subClassOf piirrite:OsmEntity ;
    skos:definition ""@en ;
    skos:inScheme piirritev:OsmNote ;
    skos:prefLabel "C"@en .

piirritev:OsmNoteIstniejcy a skos:Concept ;
    piirrite:osmId "istniejcy" ;
    rdfs:subClassOf piirrite:OsmEntity ;
    skos:definition ""@en ;
    skos:inScheme piirritev:OsmNote ;
    skos:prefLabel "Istniejcy"@en .

piirritev:OsmNoteSemiDur a skos:Concept ;
    piirrite:osmId "semi_dur" ;
    rdfs:subClassOf piirrite:OsmEntity ;
    skos:definition ""@en ;
    skos:inScheme piirritev:OsmNote ;
    skos:prefLabel "Semi dur"@en .

piirritev:OsmNote a skos:Concept ;
    piirrite:osmId "" ;
    rdfs:subClassOf piirrite:OsmEntity ;
    skos:definition ""@en ;
    skos:inScheme piirritev:OsmNote ;
    skos:prefLabel ""@en .

piirritev:OsmNote a skos:Concept ;
    piirrite:osmId "" ;
    rdfs:subClassOf piirrite:OsmEntity ;
    skos:definition ""@en ;
    skos:inScheme piirritev:OsmNote ;
    skos:prefLabel ""@en .

piirritev:OsmOfficeAccountant a skos:Concept ;
    piirrite:hasRelatedOsmTag piirrite:hasOsmAccountantEmail,
        piirrite:hasOsmAccountantName,
        piirrite:hasOsmAccountantOpeningHours,
        piirrite:hasOsmAccountantPhone,
        piirrite:hasOsmAccountantWebsite ;
    piirrite:osmId "accountant" ;
    rdfs:subClassOf piirrite:OsmEntity ;
    skos:definition "An office for an accountant. osmcarto-rendering=File:Office-16.svg osmcarto-rendering-size=28px"@en ;
    skos:inScheme piirritev:OsmOffice ;
    skos:prefLabel "Accountant"@en .

piirritev:OsmOfficeAdvertisingAgency a skos:Concept ;
    piirrite:hasRelatedOsmTag piirrite:hasOsmAdvertisingAgencyBrand,
        piirrite:hasOsmAdvertisingAgencyEmail,
        piirrite:hasOsmAdvertisingAgencyName,
        piirrite:hasOsmAdvertisingAgencyOpeningHours,
        piirrite:hasOsmAdvertisingAgencyOperator,
        piirrite:hasOsmAdvertisingAgencyPhone,
        piirrite:hasOsmAdvertisingAgencyWebsite,
        piirrite:hasOsmAdvertisingAgencyWheelchair ;
    piirrite:osmId "advertising_agency" ;
    rdfs:subClassOf piirrite:OsmEntity ;
    skos:definition "A service-based business dedicated to creating, planning, and handling advertising.  osmcarto-rendering = File:Office-16.svg  osmcarto-rendering-size = 28px"@en ;
    skos:inScheme piirritev:OsmOffice ;
    skos:prefLabel "Advertising agency"@en .

piirritev:OsmOfficeArchitect a skos:Concept ;
    piirrite:hasRelatedOsmTag piirrite:hasOsmArchitectName ;
    piirrite:osmId "architect" ;
    rdfs:subClassOf piirrite:OsmEntity ;
    skos:definition "An office for an architect or group of architects. osmcarto-rendering=File:Office-16.svg osmcarto-rendering-size=28px"@en ;
    skos:inScheme piirritev:OsmOffice ;
    skos:prefLabel "Architect"@en .

piirritev:OsmOfficeAssociation a skos:Concept ;
    piirrite:hasRelatedOsmTag piirrite:hasOsmAssociationName ;
    piirrite:osmId "association" ;
    rdfs:subClassOf piirrite:OsmEntity ;
    skos:definition "An office of a non-profit organisation, society, e.g. student, sport, consumer, automobile, bike association, etc."@en ;
    skos:inScheme piirritev:OsmOffice ;
    skos:prefLabel "Association"@en .

piirritev:OsmOfficeCompany a skos:Concept ;
    piirrite:hasRelatedOsmTag piirrite:hasOsmCompanyEmail,
        piirrite:hasOsmCompanyName,
        piirrite:hasOsmCompanyPhone,
        piirrite:hasOsmCompanyWebsite ;
    piirrite:osmId "company" ;
    rdfs:subClassOf piirrite:OsmEntity ;
    skos:definition "An office of a private company. osmcarto-rendering=File:Office-16.svg osmcarto-rendering-size=28px"@en ;
    skos:inScheme piirritev:OsmOffice ;
    skos:prefLabel "Company"@en .

piirritev:OsmOfficeDiplomatic a skos:Concept ;
    piirrite:hasRelatedOsmTag piirrite:hasOsmDiplomaticConsulate,
        piirrite:hasOsmDiplomaticCountry,
        piirrite:hasOsmDiplomaticEmbassy,
        piirrite:hasOsmDiplomaticLiaison,
        piirrite:hasOsmDiplomaticName,
        piirrite:hasOsmDiplomaticTarget ;
    piirrite:osmId "diplomatic" ;
    rdfs:subClassOf piirrite:OsmEntity ;
    skos:definition "An embassy, diplomatic mission, consulate or liaison office of a foreign government or parastatal entity in a host country.  osmcarto-rendering=File:Office-16.svg  osmcarto-rendering-size=28px"@en ;
    skos:inScheme piirritev:OsmOffice ;
    skos:prefLabel "Diplomatic"@en .

piirritev:OsmOfficeEducationalInstitution a skos:Concept ;
    piirrite:hasRelatedOsmTag piirrite:hasOsmEducationalInstitutionName,
        piirrite:hasOsmEducationalInstitutionOpeningHours,
        piirrite:hasOsmEducationalInstitutionOperator,
        piirrite:hasOsmEducationalInstitutionPhone,
        piirrite:hasOsmEducationalInstitutionWebsite,
        piirrite:hasOsmEducationalInstitutionWheelchair ;
    piirrite:osmId "educational_institution" ;
    rdfs:subClassOf piirrite:OsmEntity ;
    skos:definition "An office for an educational institution. osmcarto-rendering=File:Office-16.svg osmcarto-rendering-size=28px"@en ;
    skos:inScheme piirritev:OsmOffice ;
    skos:prefLabel "Educational institution"@en .

piirritev:OsmOfficeEmploymentAgency a skos:Concept ;
    piirrite:osmId "employment_agency" ;
    rdfs:subClassOf piirrite:OsmEntity ;
    skos:definition "An office for an employment service.  osmcarto-rendering = File:Office-16.svg  osmcarto-rendering-size = 28px"@en ;
    skos:inScheme piirritev:OsmOffice ;
    skos:prefLabel "Employment agency"@en .

piirritev:OsmOfficeEstateAgent a skos:Concept ;
    piirrite:hasRelatedOsmTag piirrite:hasOsmEstateAgentName,
        piirrite:hasOsmEstateAgentOpeningHours ;
    piirrite:osmId "estate_agent" ;
    rdfs:subClassOf piirrite:OsmEntity ;
    skos:definition "A place where you can rent or buy a house.  osmcarto-rendering = File:Office-16.svg  osmcarto-rendering-size = 28px"@en ;
    skos:inScheme piirritev:OsmOffice ;
    skos:prefLabel "Estate agent"@en .

piirritev:OsmOfficeFinancial a skos:Concept ;
    piirrite:hasRelatedOsmTag piirrite:hasOsmFinancialName,
        piirrite:hasOsmFinancialOpeningHours,
        piirrite:hasOsmFinancialWheelchair ;
    piirrite:osmId "financial" ;
    rdfs:subClassOf piirrite:OsmEntity ;
    skos:definition "An office of a company in the financial sector.  osmcarto-rendering=File:Office-16.svg  osmcarto-rendering-size=28px"@en ;
    skos:inScheme piirritev:OsmOffice ;
    skos:prefLabel "Financial"@en .

piirritev:OsmOfficeGovernment a skos:Concept ;
    piirrite:hasRelatedOsmTag piirrite:hasOsmGovernmentAdminLevel,
        piirrite:hasOsmGovernmentName,
        piirrite:hasOsmGovernmentType ;
    piirrite:osmId "government" ;
    rdfs:subClassOf piirrite:OsmEntity ;
    skos:definition "An office of a (supra)national, regional or local government agency or department osmcarto-rendering=File:Office-16.svg osmcarto-rendering-size=28px"@en ;
    skos:inScheme piirritev:OsmOffice ;
    skos:prefLabel "Government"@en .

piirritev:OsmOfficeInsurance a skos:Concept ;
    piirrite:osmId "insurance" ;
    rdfs:subClassOf piirrite:OsmEntity ;
    skos:definition "An office at which you can take out insurance policies.  osmcarto-rendering = File:Office-16.svg  osmcarto-rendering-size = 28px"@en ;
    skos:inScheme piirritev:OsmOffice ;
    skos:prefLabel "Insurance"@en .

piirritev:OsmOfficeIt a skos:Concept ;
    piirrite:hasRelatedOsmTag piirrite:hasOsmItBrand,
        piirrite:hasOsmItConsulting,
        piirrite:hasOsmItName,
        piirrite:hasOsmItOpeningHours,
        piirrite:hasOsmItOperator,
        piirrite:hasOsmItShop,
        piirrite:hasOsmItWebsite,
        piirrite:hasOsmItWheelchair ;
    piirrite:osmId "it" ;
    rdfs:subClassOf piirrite:OsmEntity ;
    skos:definition "An office for an IT company."@en ;
    skos:inScheme piirritev:OsmOffice ;
    skos:prefLabel "It"@en .

piirritev:OsmOfficeLawyer a skos:Concept ;
    piirrite:hasRelatedOsmTag piirrite:hasOsmLawyerEmail,
        piirrite:hasOsmLawyerFax,
        piirrite:hasOsmLawyerName,
        piirrite:hasOsmLawyerOpeningHours,
        piirrite:hasOsmLawyerPhone,
        piirrite:hasOsmLawyerWebsite ;
    piirrite:osmId "lawyer" ;
    rdfs:subClassOf piirrite:OsmEntity ;
    skos:definition "An office for a lawyer. osmcarto-rendering=File:Office-16.svg osmcarto-rendering-size=28px"@en ;
    skos:inScheme piirritev:OsmOffice ;
    skos:prefLabel "Lawyer"@en .

piirritev:OsmOfficeNgo a skos:Concept ;
    piirrite:hasRelatedOsmTag piirrite:hasOsmNgoName ;
    piirrite:osmId "ngo" ;
    rdfs:subClassOf piirrite:OsmEntity ;
    skos:definition "An office for a non-profit, non-governmental organisation (NGO)."@en ;
    skos:inScheme piirritev:OsmOffice ;
    skos:prefLabel "Ngo"@en .

piirritev:OsmOfficeReligion a skos:Concept ;
    piirrite:hasRelatedOsmTag piirrite:hasOsmReligionName,
        piirrite:hasOsmReligionOpeningHours,
        piirrite:hasOsmReligionOperator,
        piirrite:hasOsmReligionType ;
    piirrite:osmId "religion" ;
    rdfs:subClassOf piirrite:OsmEntity ;
    skos:definition "An office of a community of faith. osmcarto-rendering=File:Office-16.svg osmcarto-rendering-size=28px"@en ;
    skos:inScheme piirritev:OsmOffice ;
    skos:prefLabel "Religion"@en .

piirritev:OsmOfficeResearch a skos:Concept ;
    piirrite:hasRelatedOsmTag piirrite:hasOsmResearchName,
        piirrite:hasOsmResearchOperator,
        piirrite:hasOsmResearchType,
        piirrite:hasOsmResearchWebsite ;
    piirrite:osmId "research" ;
    rdfs:subClassOf piirrite:OsmEntity ;
    skos:definition "An office for research and development"@en ;
    skos:inScheme piirritev:OsmOffice ;
    skos:prefLabel "Research"@en .

piirritev:OsmOfficeTaxAdvisor a skos:Concept ;
    piirrite:osmId "tax_advisor" ;
    rdfs:subClassOf piirrite:OsmEntity ;
    skos:definition "An office for a financial expert specially trained in tax law  osmcarto-rendering = File:Office-16.svg  osmcarto-rendering-size = 28px"@en ;
    skos:inScheme piirritev:OsmOffice ;
    skos:prefLabel "Tax advisor"@en .

piirritev:OsmOfficeTelecommunication a skos:Concept ;
    piirrite:hasRelatedOsmTag piirrite:hasOsmTelecommunicationFunction,
        piirrite:hasOsmTelecommunicationName,
        piirrite:hasOsmTelecommunicationOpeningHours,
        piirrite:hasOsmTelecommunicationOperator ;
    piirrite:osmId "telecommunication" ;
    rdfs:subClassOf piirrite:OsmEntity ;
    skos:definition "An office for a telecommunication company."@en ;
    skos:inScheme piirritev:OsmOffice ;
    skos:prefLabel "Telecommunication"@en .

piirritev:OsmOfficialNameStarbucksCoffee a skos:Concept ;
    piirrite:osmId "Starbucks_Coffee" ;
    rdfs:subClassOf piirrite:OsmEntity ;
    skos:definition ""@en ;
    skos:inScheme piirritev:OsmOfficialName ;
    skos:prefLabel "Starbucks coffee"@en .

piirritev:OsmOfficialStatus a skos:ConceptScheme ;
    piirrite:osmId "official_status" ;
    skos:definition ""@en ;
    skos:prefLabel "Official status, types"@en .

piirritev:OsmOldName a skos:ConceptScheme ;
    piirrite:osmId "old_name" ;
    skos:definition "Old / previous / historic name for an element."@en ;
    skos:prefLabel "Old name, types"@en .

piirritev:OsmOldRailwayOperatorNyc a skos:Concept ;
    piirrite:osmId "NYC" ;
    rdfs:subClassOf piirrite:OsmEntity ;
    skos:definition ""@en ;
    skos:inScheme piirritev:OsmOldRailwayOperator ;
    skos:prefLabel "Nyc"@en .

piirritev:OsmOldRailwayOperatorPrr a skos:Concept ;
    piirrite:osmId "PRR" ;
    rdfs:subClassOf piirrite:OsmEntity ;
    skos:definition ""@en ;
    skos:inScheme piirritev:OsmOldRailwayOperator ;
    skos:prefLabel "Prr"@en .

piirritev:OsmOldRef a skos:ConceptScheme ;
    piirrite:osmId "old_ref" ;
    skos:definition "Historical reference."@en ;
    skos:prefLabel "Old ref, types"@en .

piirritev:OsmOnewayAlternating a skos:Concept ;
    piirrite:hasRelatedOsmTag piirrite:hasOsmAlternatingHazard,
        piirrite:hasOsmAlternatingMaxspeed ;
    piirrite:osmId "alternating" ;
    rdfs:subClassOf piirrite:OsmEntity ;
    skos:definition "Oneway that changes its direction often"@en ;
    skos:inScheme piirritev:OsmOneway ;
    skos:prefLabel "Alternating"@en .

piirritev:OsmOpeningHoursSunrise-Sunset a skos:Concept ;
    piirrite:osmId "sunrise-sunset" ;
    rdfs:subClassOf piirrite:OsmEntity ;
    skos:definition ""@en ;
    skos:inScheme piirritev:OsmOpeningHours ;
    skos:prefLabel "Sunrise-sunset"@en .

piirritev:OsmOperationalStatusOpen a skos:Concept ;
    piirrite:osmId "open" ;
    rdfs:subClassOf piirrite:OsmEntity ;
    skos:definition ""@en ;
    skos:inScheme piirritev:OsmOperationalStatus ;
    skos:prefLabel "Open"@en .

piirritev:OsmOperationalStatusOperational a skos:Concept ;
    piirrite:osmId "operational" ;
    rdfs:subClassOf piirrite:OsmEntity ;
    skos:definition ""@en ;
    skos:inScheme piirritev:OsmOperationalStatus ;
    skos:prefLabel "Operational"@en .

piirritev:OsmOperatorAdif a skos:Concept ;
    piirrite:osmId "Adif" ;
    rdfs:subClassOf piirrite:OsmEntity ;
    skos:definition ""@en ;
    skos:inScheme piirritev:OsmOperator ;
    skos:prefLabel "Adif"@en .

piirritev:OsmOperatorAtac a skos:Concept ;
    piirrite:osmId "ATAC" ;
    rdfs:subClassOf piirrite:OsmEntity ;
    skos:definition ""@en ;
    skos:inScheme piirritev:OsmOperator ;
    skos:prefLabel "Atac"@en .

piirritev:OsmOperatorBnsfRailway a skos:Concept ;
    piirrite:osmId "BNSF_Railway" ;
    rdfs:subClassOf piirrite:OsmEntity ;
    skos:definition ""@en ;
    skos:inScheme piirritev:OsmOperator ;
    skos:prefLabel "Bnsf railway"@en .

piirritev:OsmOperatorCanadaPost a skos:Concept ;
    piirrite:osmId "Canada_Post" ;
    rdfs:subClassOf piirrite:OsmEntity ;
    skos:definition ""@en ;
    skos:inScheme piirritev:OsmOperator ;
    skos:prefLabel "Canada post"@en .

piirritev:OsmOperatorCfr a skos:Concept ;
    piirrite:osmId "CFR" ;
    rdfs:subClassOf piirrite:OsmEntity ;
    skos:definition ""@en ;
    skos:inScheme piirritev:OsmOperator ;
    skos:prefLabel "Cfr"@en .

piirritev:OsmOperatorCsxTransportation a skos:Concept ;
    piirrite:osmId "CSX_Transportation" ;
    rdfs:subClassOf piirrite:OsmEntity ;
    skos:definition ""@en ;
    skos:inScheme piirritev:OsmOperator ;
    skos:prefLabel "Csx transportation"@en .

piirritev:OsmOperatorDbInfrago a skos:Concept ;
    piirrite:osmId "DB_InfraGO" ;
    rdfs:subClassOf piirrite:OsmEntity ;
    skos:definition ""@en ;
    skos:inScheme piirritev:OsmOperator ;
    skos:prefLabel "Db infrago"@en .

piirritev:OsmOperatorDbNetz a skos:Concept ;
    piirrite:osmId "DB_Netz" ;
    rdfs:subClassOf piirrite:OsmEntity ;
    skos:definition ""@en ;
    skos:inScheme piirritev:OsmOperator ;
    skos:prefLabel "Db netz"@en .

piirritev:OsmOperatorDeLijn a skos:Concept ;
    piirrite:osmId "De_Lijn" ;
    rdfs:subClassOf piirrite:OsmEntity ;
    skos:definition ""@en ;
    skos:inScheme piirritev:OsmOperator ;
    skos:prefLabel "De lijn"@en .

piirritev:OsmOperatorDeutschePost a skos:Concept ;
    piirrite:osmId "Deutsche_Post" ;
    rdfs:subClassOf piirrite:OsmEntity ;
    skos:definition ""@en ;
    skos:inScheme piirritev:OsmOperator ;
    skos:prefLabel "Deutsche post"@en .

piirritev:OsmOperatorDhl a skos:Concept ;
    piirrite:osmId "DHL" ;
    rdfs:subClassOf piirrite:OsmEntity ;
    skos:definition ""@en ;
    skos:inScheme piirritev:OsmOperator ;
    skos:prefLabel "Dhl"@en .

piirritev:OsmOperatorE-Redes a skos:Concept ;
    piirrite:osmId "E-REDES" ;
    rdfs:subClassOf piirrite:OsmEntity ;
    skos:definition ""@en ;
    skos:inScheme piirritev:OsmOperator ;
    skos:prefLabel "E-redes"@en .

piirritev:OsmOperatorEamNetz a skos:Concept ;
    piirrite:osmId "EAM_Netz" ;
    rdfs:subClassOf piirrite:OsmEntity ;
    skos:definition ""@en ;
    skos:inScheme piirritev:OsmOperator ;
    skos:prefLabel "Eam netz"@en .

piirritev:OsmOperatorEnedis a skos:Concept ;
    piirrite:hasRelatedOsmTag piirrite:hasOsmEnedisPower ;
    piirrite:osmId "Enedis" ;
    rdfs:subClassOf piirrite:OsmEntity ;
    skos:definition "French network operator for electricity distribution in metropolitan France."@en ;
    skos:inScheme piirritev:OsmOperator ;
    skos:prefLabel "Enedis"@en .

piirritev:OsmOperatorEnergieAg a skos:Concept ;
    piirrite:osmId "Energie_AG" ;
    rdfs:subClassOf piirrite:OsmEntity ;
    skos:definition ""@en ;
    skos:inScheme piirritev:OsmOperator ;
    skos:prefLabel "Energie ag"@en .

piirritev:OsmOperatorEsbNetworks a skos:Concept ;
    piirrite:osmId "ESB_Networks" ;
    rdfs:subClassOf piirrite:OsmEntity ;
    skos:definition ""@en ;
    skos:inScheme piirritev:OsmOperator ;
    skos:prefLabel "Esb networks"@en .

piirritev:OsmOperatorFederalTransferido a skos:Concept ;
    piirrite:osmId "Federal_Transferido" ;
    rdfs:subClassOf piirrite:OsmEntity ;
    skos:definition ""@en ;
    skos:inScheme piirritev:OsmOperator ;
    skos:prefLabel "Federal transferido"@en .

piirritev:OsmOperatorGrdis a skos:Concept ;
    piirrite:osmId "Grdis" ;
    rdfs:subClassOf piirrite:OsmEntity ;
    skos:definition ""@en ;
    skos:inScheme piirritev:OsmOperator ;
    skos:prefLabel "Grdis"@en .

piirritev:OsmOperatorHelpbidea a skos:Concept ;
    piirrite:osmId "helpbidea" ;
    rdfs:subClassOf piirrite:OsmEntity ;
    skos:definition ""@en ;
    skos:inScheme piirritev:OsmOperator ;
    skos:prefLabel "Helpbidea"@en .

piirritev:OsmOperatorHydro-Qubec a skos:Concept ;
    piirrite:osmId "Hydro-Qubec" ;
    rdfs:subClassOf piirrite:OsmEntity ;
    skos:definition ""@en ;
    skos:inScheme piirritev:OsmOperator ;
    skos:prefLabel "Hydro-qubec"@en .

piirritev:OsmOperatorHydroOne a skos:Concept ;
    piirrite:osmId "Hydro_One" ;
    rdfs:subClassOf piirrite:OsmEntity ;
    skos:definition ""@en ;
    skos:inScheme piirritev:OsmOperator ;
    skos:prefLabel "Hydro one"@en .

piirritev:OsmOperatorInfrabel a skos:Concept ;
    piirrite:osmId "Infrabel" ;
    rdfs:subClassOf piirrite:OsmEntity ;
    skos:definition ""@en ;
    skos:inScheme piirritev:OsmOperator ;
    skos:prefLabel "Infrabel"@en .

piirritev:OsmOperatorInpost a skos:Concept ;
    piirrite:osmId "InPost" ;
    rdfs:subClassOf piirrite:OsmEntity ;
    skos:definition ""@en ;
    skos:inScheme piirritev:OsmOperator ;
    skos:prefLabel "Inpost"@en .

piirritev:OsmOperatorJcdecaux a skos:Concept ;
    piirrite:osmId "JCDecaux" ;
    rdfs:subClassOf piirrite:OsmEntity ;
    skos:definition ""@en ;
    skos:inScheme piirritev:OsmOperator ;
    skos:prefLabel "Jcdecaux"@en .

piirritev:OsmOperatorLaPoste a skos:Concept ;
    piirrite:osmId "La_Poste" ;
    rdfs:subClassOf piirrite:OsmEntity ;
    skos:definition "La Poste is the postal operator of France."@en ;
    skos:inScheme piirritev:OsmOperator ;
    skos:prefLabel "La poste"@en .

piirritev:OsmOperatorLimasam a skos:Concept ;
    piirrite:osmId "Limasam" ;
    rdfs:subClassOf piirrite:OsmEntity ;
    skos:definition ""@en ;
    skos:inScheme piirritev:OsmOperator ;
    skos:prefLabel "Limasam"@en .

piirritev:OsmOperatorLisea a skos:Concept ;
    piirrite:osmId "LISEA" ;
    rdfs:subClassOf piirrite:OsmEntity ;
    skos:definition ""@en ;
    skos:inScheme piirritev:OsmOperator ;
    skos:prefLabel "Lisea"@en .

piirritev:OsmOperatorMeralco a skos:Concept ;
    piirrite:osmId "Meralco" ;
    rdfs:subClassOf piirrite:OsmEntity ;
    skos:definition ""@en ;
    skos:inScheme piirritev:OsmOperator ;
    skos:prefLabel "Meralco"@en .

piirritev:OsmOperatorMetroTransit a skos:Concept ;
    piirrite:osmId "Metro_Transit" ;
    rdfs:subClassOf piirrite:OsmEntity ;
    skos:definition ""@en ;
    skos:inScheme piirritev:OsmOperator ;
    skos:prefLabel "Metro transit"@en .

piirritev:OsmOperatorMiami-DadeTransit a skos:Concept ;
    piirrite:osmId "Miami-Dade_Transit" ;
    rdfs:subClassOf piirrite:OsmEntity ;
    skos:definition ""@en ;
    skos:inScheme piirritev:OsmOperator ;
    skos:prefLabel "Miami-dade transit"@en .

piirritev:OsmOperatorMv a skos:Concept ;
    piirrite:osmId "MV" ;
    rdfs:subClassOf piirrite:OsmEntity ;
    skos:definition ""@en ;
    skos:inScheme piirritev:OsmOperator ;
    skos:prefLabel "Mv"@en .

piirritev:OsmOperatorNationalGrid a skos:Concept ;
    piirrite:osmId "National_Grid" ;
    rdfs:subClassOf piirrite:OsmEntity ;
    skos:definition ""@en ;
    skos:inScheme piirritev:OsmOperator ;
    skos:prefLabel "National grid"@en .

piirritev:OsmOperatorNationalHighways a skos:Concept ;
    piirrite:osmId "National_Highways" ;
    rdfs:subClassOf piirrite:OsmEntity ;
    skos:definition ""@en ;
    skos:inScheme piirritev:OsmOperator ;
    skos:prefLabel "National highways"@en .

piirritev:OsmOperatorNatran a skos:Concept ;
    piirrite:hasRelatedOsmTag piirrite:hasOsmNatranManMade,
        piirrite:hasOsmNatranMarker,
        piirrite:hasOsmNatranPipeline ;
    piirrite:osmId "NaTran" ;
    rdfs:subClassOf piirrite:OsmEntity ;
    skos:definition "Main French gas transmission network operator."@en ;
    skos:inScheme piirritev:OsmOperator ;
    skos:prefLabel "Natran"@en .

piirritev:OsmOperatorNetworkRail a skos:Concept ;
    piirrite:osmId "Network_Rail" ;
    rdfs:subClassOf piirrite:OsmEntity ;
    skos:definition ""@en ;
    skos:inScheme piirritev:OsmOperator ;
    skos:prefLabel "Network rail"@en .

piirritev:OsmOperatorNieNetworks a skos:Concept ;
    piirrite:osmId "NIE_Networks" ;
    rdfs:subClassOf piirrite:OsmEntity ;
    skos:definition ""@en ;
    skos:inScheme piirritev:OsmOperator ;
    skos:prefLabel "Nie networks"@en .

piirritev:OsmOperatorOrange a skos:Concept ;
    piirrite:hasRelatedOsmTag piirrite:hasOsmOrangeTelecom ;
    piirrite:osmId "Orange" ;
    rdfs:subClassOf piirrite:OsmEntity ;
    skos:definition "Global telecommunication network operator based in France."@en ;
    skos:inScheme piirritev:OsmOperator ;
    skos:prefLabel "Orange"@en .

piirritev:OsmOperatorPag a skos:Concept ;
    piirrite:osmId "PAG" ;
    rdfs:subClassOf piirrite:OsmEntity ;
    skos:definition ""@en ;
    skos:inScheme piirritev:OsmOperator ;
    skos:prefLabel "Pag"@en .

piirritev:OsmOperatorPgeDystrybucja a skos:Concept ;
    piirrite:osmId "PGE_Dystrybucja" ;
    rdfs:subClassOf piirrite:OsmEntity ;
    skos:definition ""@en ;
    skos:inScheme piirritev:OsmOperator ;
    skos:prefLabel "Pge dystrybucja"@en .

piirritev:OsmOperatorPglLp a skos:Concept ;
    piirrite:osmId "PGL_LP" ;
    rdfs:subClassOf piirrite:OsmEntity ;
    skos:definition ""@en ;
    skos:inScheme piirritev:OsmOperator ;
    skos:prefLabel "Pgl lp"@en .

piirritev:OsmOperatorPosteItaliane a skos:Concept ;
    piirrite:osmId "Poste_Italiane" ;
    rdfs:subClassOf piirrite:OsmEntity ;
    skos:definition ""@en ;
    skos:inScheme piirritev:OsmOperator ;
    skos:prefLabel "Poste italiane"@en .

piirritev:OsmOperatorProrail a skos:Concept ;
    piirrite:hasRelatedOsmTag piirrite:hasOsmProrailRailway ;
    piirrite:osmId "ProRail" ;
    rdfs:subClassOf piirrite:OsmEntity ;
    skos:definition "Operated by ProRail B.V., The Netherlands"@en ;
    skos:inScheme piirritev:OsmOperator ;
    skos:prefLabel "Prorail"@en .

piirritev:OsmOperatorRfi a skos:Concept ;
    piirrite:osmId "RFI" ;
    rdfs:subClassOf piirrite:OsmEntity ;
    skos:definition ""@en ;
    skos:inScheme piirritev:OsmOperator ;
    skos:prefLabel "Rfi"@en .

piirritev:OsmOperatorRijkswaterstaat a skos:Concept ;
    piirrite:hasRelatedOsmTag piirrite:hasOsmRijkswaterstaatHighway,
        piirrite:hasOsmRijkswaterstaatManMade,
        piirrite:hasOsmRijkswaterstaatOwner,
        piirrite:hasOsmRijkswaterstaatWaterway ;
    piirrite:osmId "Rijkswaterstaat" ;
    rdfs:subClassOf piirrite:OsmEntity ;
    skos:definition "Operated by the Dutch Rijkswaterstaat"@en ;
    skos:inScheme piirritev:OsmOperator ;
    skos:prefLabel "Rijkswaterstaat"@en .

piirritev:OsmOperatorRoyalMail a skos:Concept ;
    piirrite:osmId "Royal_Mail" ;
    rdfs:subClassOf piirrite:OsmEntity ;
    skos:definition ""@en ;
    skos:inScheme piirritev:OsmOperator ;
    skos:prefLabel "Royal mail"@en .

piirritev:OsmOperatorRte a skos:Concept ;
    piirrite:hasRelatedOsmTag piirrite:hasOsmRtePower ;
    piirrite:osmId "RTE" ;
    rdfs:subClassOf piirrite:OsmEntity ;
    skos:definition "Company responsible of French power transmission network operation."@en ;
    skos:inScheme piirritev:OsmOperator ;
    skos:prefLabel "Rte"@en .

piirritev:OsmOperatorSadalesTkls a skos:Concept ;
    piirrite:osmId "Sadales_tkls" ;
    rdfs:subClassOf piirrite:OsmEntity ;
    skos:definition ""@en ;
    skos:inScheme piirritev:OsmOperator ;
    skos:prefLabel "Sadales tkls"@en .

piirritev:OsmOperatorSbb a skos:Concept ;
    piirrite:osmId "SBB" ;
    rdfs:subClassOf piirrite:OsmEntity ;
    skos:definition ""@en ;
    skos:inScheme piirritev:OsmOperator ;
    skos:prefLabel "Sbb"@en .

piirritev:OsmOperatorSchwarzwaldverein a skos:Concept ;
    piirrite:osmId "Schwarzwaldverein" ;
    rdfs:subClassOf piirrite:OsmEntity ;
    skos:definition ""@en ;
    skos:inScheme piirritev:OsmOperator ;
    skos:prefLabel "Schwarzwaldverein"@en .

piirritev:OsmOperatorSncf a skos:Concept ;
    piirrite:osmId "SNCF" ;
    rdfs:subClassOf piirrite:OsmEntity ;
    skos:definition ""@en ;
    skos:inScheme piirritev:OsmOperator ;
    skos:prefLabel "Sncf"@en .

piirritev:OsmOperatorSncfRseau a skos:Concept ;
    piirrite:osmId "SNCF_Rseau" ;
    rdfs:subClassOf piirrite:OsmEntity ;
    skos:definition ""@en ;
    skos:inScheme piirritev:OsmOperator ;
    skos:prefLabel "Sncf rseau"@en .

piirritev:OsmOperatorSrd a skos:Concept ;
    piirrite:osmId "SRD" ;
    rdfs:subClassOf piirrite:OsmEntity ;
    skos:definition ""@en ;
    skos:inScheme piirritev:OsmOperator ;
    skos:prefLabel "Srd"@en .

piirritev:OsmOperatorStadtWitten a skos:Concept ;
    piirrite:osmId "Stadt_Witten" ;
    rdfs:subClassOf piirrite:OsmEntity ;
    skos:definition ""@en ;
    skos:inScheme piirritev:OsmOperator ;
    skos:prefLabel "Stadt witten"@en .

piirritev:OsmOperatorTauron a skos:Concept ;
    piirrite:osmId "Tauron" ;
    rdfs:subClassOf piirrite:OsmEntity ;
    skos:definition ""@en ;
    skos:inScheme piirritev:OsmOperator ;
    skos:prefLabel "Tauron"@en .

piirritev:OsmOperatorTcdd a skos:Concept ;
    piirrite:osmId "TCDD" ;
    rdfs:subClassOf piirrite:OsmEntity ;
    skos:definition ""@en ;
    skos:inScheme piirritev:OsmOperator ;
    skos:prefLabel "Tcdd"@en .

piirritev:OsmOperatorTec a skos:Concept ;
    piirrite:hasRelatedOsmTag piirrite:hasOsmTecHighway,
        piirrite:hasOsmTecPublicTransport,
        piirrite:hasOsmTecRoute ;
    piirrite:osmId "TEC" ;
    rdfs:subClassOf piirrite:OsmEntity ;
    skos:definition "Operated by Transport en Commun (TEC)"@en ;
    skos:inScheme piirritev:OsmOperator ;
    skos:prefLabel "Tec"@en .

piirritev:OsmOperatorTeia a skos:Concept ;
    piirrite:osmId "TEA" ;
    rdfs:subClassOf piirrite:OsmEntity ;
    skos:definition ""@en ;
    skos:inScheme piirritev:OsmOperator ;
    skos:prefLabel "Teia"@en .

piirritev:OsmOperatorTrafikverket a skos:Concept ;
    piirrite:osmId "Trafikverket" ;
    rdfs:subClassOf piirrite:OsmEntity ;
    skos:definition ""@en ;
    skos:inScheme piirritev:OsmOperator ;
    skos:prefLabel "Trafikverket"@en .

piirritev:OsmOperatorTreda a skos:Concept ;
    piirrite:osmId "TREDA" ;
    rdfs:subClassOf piirrite:OsmEntity ;
    skos:definition ""@en ;
    skos:inScheme piirritev:OsmOperator ;
    skos:prefLabel "Treda"@en .

piirritev:OsmOperatorVejdirektoratet a skos:Concept ;
    piirrite:osmId "Vejdirektoratet" ;
    rdfs:subClassOf piirrite:OsmEntity ;
    skos:definition ""@en ;
    skos:inScheme piirritev:OsmOperator ;
    skos:prefLabel "Vejdirektoratet"@en .

piirritev:OsmOperatorVolnbusz a skos:Concept ;
    piirrite:osmId "Volnbusz" ;
    rdfs:subClassOf piirrite:OsmEntity ;
    skos:definition ""@en ;
    skos:inScheme piirritev:OsmOperator ;
    skos:prefLabel "Volnbusz"@en .

piirritev:OsmOperatorVylvirasto a skos:Concept ;
    piirrite:osmId "Vylvirasto" ;
    rdfs:subClassOf piirrite:OsmEntity ;
    skos:definition ""@en ;
    skos:inScheme piirritev:OsmOperator ;
    skos:prefLabel "Vylvirasto"@en .

piirritev:OsmOperatorYpfSA a skos:Concept ;
    piirrite:osmId "YPF_S_A_" ;
    rdfs:subClassOf piirrite:OsmEntity ;
    skos:definition ""@en ;
    skos:inScheme piirritev:OsmOperator ;
    skos:prefLabel "Ypf s a "@en .

piirritev:OsmOperatorbb-InfrastrukturAg a skos:Concept ;
    piirrite:osmId "BB-Infrastruktur_AG" ;
    rdfs:subClassOf piirrite:OsmEntity ;
    skos:definition ""@en ;
    skos:inScheme piirritev:OsmOperator ;
    skos:prefLabel "bb-infrastruktur ag"@en .

piirritev:OsmOperatorezDistribuce a skos:Concept ;
    piirrite:osmId "EZ_Distribuce" ;
    rdfs:subClassOf piirrite:OsmEntity ;
    skos:definition ""@en ;
    skos:inScheme piirritev:OsmOperator ;
    skos:prefLabel "ez distribuce"@en .

piirritev:OsmOperatorett a skos:Concept ;
    piirrite:osmId "ETT" ;
    rdfs:subClassOf piirrite:OsmEntity ;
    skos:definition ""@en ;
    skos:inScheme piirritev:OsmOperator ;
    skos:prefLabel "ett"@en .

piirritev:OsmOperatorsr a skos:Concept ;
    piirrite:osmId "SR" ;
    rdfs:subClassOf piirrite:OsmEntity ;
    skos:definition ""@en ;
    skos:inScheme piirritev:OsmOperator ;
    skos:prefLabel "sr"@en .

piirritev:OsmOperator a skos:Concept ;
    piirrite:osmId "_" ;
    rdfs:subClassOf piirrite:OsmEntity ;
    skos:definition ""@en ;
    skos:inScheme piirritev:OsmOperator ;
    skos:prefLabel " "@en .

piirritev:OsmOperator a skos:Concept ;
    piirrite:osmId "" ;
    rdfs:subClassOf piirrite:OsmEntity ;
    skos:definition ""@en ;
    skos:inScheme piirritev:OsmOperator ;
    skos:prefLabel ""@en .

piirritev:OsmOperator a skos:Concept ;
    piirrite:osmId "" ;
    rdfs:subClassOf piirrite:OsmEntity ;
    skos:definition ""@en ;
    skos:inScheme piirritev:OsmOperator ;
    skos:prefLabel ""@en .

piirritev:OsmOperator a skos:Concept ;
    piirrite:osmId "" ;
    rdfs:subClassOf piirrite:OsmEntity ;
    skos:definition ""@en ;
    skos:inScheme piirritev:OsmOperator ;
    skos:prefLabel ""@en .

piirritev:OsmOperator a skos:Concept ;
    piirrite:osmId "" ;
    rdfs:subClassOf piirrite:OsmEntity ;
    skos:definition ""@en ;
    skos:inScheme piirritev:OsmOperator ;
    skos:prefLabel ""@en .

piirritev:OsmOperator a skos:Concept ;
    piirrite:osmId "" ;
    rdfs:subClassOf piirrite:OsmEntity ;
    skos:definition ""@en ;
    skos:inScheme piirritev:OsmOperator ;
    skos:prefLabel ""@en .

piirritev:OsmOperator a skos:Concept ;
    piirrite:osmId "_" ;
    rdfs:subClassOf piirrite:OsmEntity ;
    skos:definition ""@en ;
    skos:inScheme piirritev:OsmOperator ;
    skos:prefLabel " "@en .

piirritev:OsmOperator a skos:Concept ;
    piirrite:osmId "" ;
    rdfs:subClassOf piirrite:OsmEntity ;
    skos:definition ""@en ;
    skos:inScheme piirritev:OsmOperator ;
    skos:prefLabel ""@en .

piirritev:OsmOperator a skos:Concept ;
    piirrite:osmId "" ;
    rdfs:subClassOf piirrite:OsmEntity ;
    skos:definition ""@en ;
    skos:inScheme piirritev:OsmOperator ;
    skos:prefLabel ""@en .

piirritev:OsmOrientationDiagonal a skos:Concept ;
    piirrite:osmId "diagonal" ;
    rdfs:subClassOf piirrite:OsmEntity ;
    skos:definition ""@en ;
    skos:inScheme piirritev:OsmOrientation ;
    skos:prefLabel "Diagonal"@en .

piirritev:OsmOrientationParallel a skos:Concept ;
    piirrite:osmId "parallel" ;
    rdfs:subClassOf piirrite:OsmEntity ;
    skos:definition ""@en ;
    skos:inScheme piirritev:OsmOrientation ;
    skos:prefLabel "Parallel"@en .

piirritev:OsmOrientationPerpendicular a skos:Concept ;
    piirrite:osmId "perpendicular" ;
    rdfs:subClassOf piirrite:OsmEntity ;
    skos:definition ""@en ;
    skos:inScheme piirritev:OsmOrientation ;
    skos:prefLabel "Perpendicular"@en .

piirritev:OsmOutdoorSeating a skos:ConceptScheme ;
    piirrite:osmId "outdoor_seating" ;
    skos:definition "To indicate if a restaurant or similar feature offers outdoor seating (or to specify the type of outdoor seating with tag:leisure=outdoor_seating)."@en ;
    skos:prefLabel "Outdoor seating, types"@en .

piirritev:OsmOvertaking a skos:ConceptScheme ;
    piirrite:osmId "overtaking" ;
    skos:definition "Overtaking restrictions as signposted or painted on the ground"@en ;
    skos:prefLabel "Overtaking, types"@en .

piirritev:OsmOwnerRgionWallonne a skos:Concept ;
    piirrite:osmId "Rgion_wallonne" ;
    rdfs:subClassOf piirrite:OsmEntity ;
    skos:definition ""@en ;
    skos:inScheme piirritev:OsmOwner ;
    skos:prefLabel "Rgion wallonne"@en .

piirritev:OsmOwnershipMunicipal a skos:Concept ;
    piirrite:osmId "municipal" ;
    rdfs:subClassOf piirrite:OsmEntity ;
    skos:definition ""@en ;
    skos:inScheme piirritev:OsmOwnership ;
    skos:prefLabel "Municipal"@en .

piirritev:OsmOwnershipNational a skos:Concept ;
    piirrite:osmId "national" ;
    rdfs:subClassOf piirrite:OsmEntity ;
    skos:definition ""@en ;
    skos:inScheme piirritev:OsmOwnership ;
    skos:prefLabel "National"@en .

piirritev:OsmOwnershipPrivate a skos:Concept ;
    piirrite:hasRelatedOsmTag piirrite:hasOsmPrivateAccess ;
    piirrite:osmId "private" ;
    rdfs:subClassOf piirrite:OsmEntity ;
    skos:definition "Describes object as privately owned."@en ;
    skos:inScheme piirritev:OsmOwnership ;
    skos:prefLabel "Private"@en .

piirritev:OsmOwnershipPublic a skos:Concept ;
    piirrite:osmId "public" ;
    rdfs:subClassOf piirrite:OsmEntity ;
    skos:definition ""@en ;
    skos:inScheme piirritev:OsmOwnership ;
    skos:prefLabel "Public"@en .

piirritev:OsmOwnershipState a skos:Concept ;
    piirrite:osmId "state" ;
    rdfs:subClassOf piirrite:OsmEntity ;
    skos:definition ""@en ;
    skos:inScheme piirritev:OsmOwnership ;
    skos:prefLabel "State"@en .

piirritev:OsmPar a skos:ConceptScheme ;
    piirrite:osmId "par" ;
    skos:definition "Base number of strokes required to complete a golf hole."@en ;
    skos:prefLabel "Par, types"@en .

piirritev:OsmParkRide a skos:ConceptScheme ;
    piirrite:osmId "park_ride" ;
    skos:definition "Park and ride"@en ;
    skos:prefLabel "Park ride, types"@en .

piirritev:OsmParkingCarports a skos:Concept ;
    piirrite:osmId "carports" ;
    rdfs:subClassOf piirrite:OsmEntity ;
    skos:definition "Parking fully equipped with carports."@en ;
    skos:inScheme piirritev:OsmParking ;
    skos:prefLabel "Carports"@en .

piirritev:OsmParkingLane a skos:Concept ;
    piirrite:hasRelatedOsmTag piirrite:hasOsmLaneParking ;
    piirrite:osmId "lane" ;
    rdfs:subClassOf piirrite:OsmEntity ;
    skos:definition "Parking on the carriageway, including partially on it. osmcarto-rendering=File:Parking-subtle.svg osmcarto-rendering-size=16px"@en ;
    skos:inScheme piirritev:OsmParking ;
    skos:prefLabel "Lane"@en .

piirritev:OsmParkingLayby a skos:Concept ;
    piirrite:hasRelatedOsmTag piirrite:hasOsmLaybyParking ;
    piirrite:osmId "layby" ;
    rdfs:subClassOf piirrite:OsmEntity ;
    skos:definition "Parking at a rest area, alongside a road. There is usually no physical barrier between the road and the layby. If there is then consider using rest-area."@en ;
    skos:inScheme piirritev:OsmParking ;
    skos:prefLabel "Layby"@en .

piirritev:OsmParkingMulti-Storey a skos:Concept ;
    piirrite:osmId "multi-storey" ;
    rdfs:subClassOf piirrite:OsmEntity ;
    skos:definition "Multistorey car park."@en ;
    skos:inScheme piirritev:OsmParking ;
    skos:prefLabel "Multi-storey"@en .

piirritev:OsmParkingSpaceCharging a skos:Concept ;
    piirrite:osmId "charging" ;
    rdfs:subClassOf piirrite:OsmEntity ;
    skos:definition "A parking space designated for use while charging electric vehicles. osmcarto-rendering=File:Rendering-parking space.png osmcarto-rendering-size=125px"@en ;
    skos:inScheme piirritev:OsmParkingSpace ;
    skos:prefLabel "Charging"@en .

piirritev:OsmParkingSpaceDisabled a skos:Concept ;
    piirrite:osmId "disabled" ;
    rdfs:subClassOf piirrite:OsmEntity ;
    skos:definition "A parking space specifically designated for use by people with disabilities."@en ;
    skos:inScheme piirritev:OsmParkingSpace ;
    skos:prefLabel "Disabled"@en .

piirritev:OsmParkingStreetSide a skos:Concept ;
    piirrite:hasRelatedOsmTag piirrite:hasOsmStreetSideOrientation ;
    piirrite:osmId "street_side" ;
    rdfs:subClassOf piirrite:OsmEntity ;
    skos:definition "Area suitable or designated for parking which is directly adjacent to the carriageway of a road and can be reached directly from the roadway without having to use an access way. osmcarto-rendering=File:Parking-subtle.svg osmcarto-rendering-size=18px"@en ;
    skos:inScheme piirritev:OsmParking ;
    skos:prefLabel "Street side"@en .

piirritev:OsmParkingSurface a skos:Concept ;
    piirrite:osmId "surface" ;
    rdfs:subClassOf piirrite:OsmEntity ;
    skos:definition "An open-air ground-level area explicitly designated for vehicle parking."@en ;
    skos:inScheme piirritev:OsmParking ;
    skos:prefLabel "Surface"@en .

piirritev:OsmParkingUnderground a skos:Concept ;
    piirrite:osmId "underground" ;
    rdfs:subClassOf piirrite:OsmEntity ;
    skos:definition "Underground car park"@en ;
    skos:inScheme piirritev:OsmParking ;
    skos:prefLabel "Underground"@en .

piirritev:OsmPassengerInformationDisplay a skos:ConceptScheme ;
    piirrite:osmId "passenger_information_display" ;
    skos:definition "A passenger information system."@en ;
    skos:prefLabel "Passenger information display, types"@en .

piirritev:OsmPassengerLines a skos:ConceptScheme ;
    piirrite:osmId "passenger_lines" ;
    skos:definition "Used to describe number of tracks of the railway line a certain track segment belongs to."@en ;
    skos:prefLabel "Passenger lines, types"@en .

piirritev:OsmPhone a skos:ConceptScheme ;
    piirrite:osmId "phone" ;
    skos:definition "A telephone number associated with the object. Use +CC XXX XXX XXX format, where CC is a country code."@en ;
    skos:prefLabel "Phone, types"@en .

piirritev:OsmPlacementTransition a skos:Concept ;
    piirrite:hasRelatedOsmTag piirrite:hasOsmTransitionHighway ;
    piirrite:osmId "transition" ;
    rdfs:subClassOf piirrite:OsmEntity ;
    skos:definition "Used to indicate that the shape of the OSM way follows neither the middle nor the left/right side of any lane."@en ;
    skos:inScheme piirritev:OsmPlacement ;
    skos:prefLabel "Transition"@en .

piirritev:OsmPlaygroundClimbingframe a skos:Concept ;
    piirrite:hasRelatedOsmTag piirrite:hasOsmClimbingframeBaby,
        piirrite:hasOsmClimbingframeBlind,
        piirrite:hasOsmClimbingframeCentralkey,
        piirrite:hasOsmClimbingframeLeisure,
        piirrite:hasOsmClimbingframeMaterial,
        piirrite:hasOsmClimbingframeMaxAge,
        piirrite:hasOsmClimbingframeMinAge,
        piirrite:hasOsmClimbingframeName,
        piirrite:hasOsmClimbingframeSittingDisability,
        piirrite:hasOsmClimbingframeWalkingDisability,
        piirrite:hasOsmClimbingframeWheelchair ;
    piirrite:osmId "climbingframe" ;
    rdfs:subClassOf piirrite:OsmEntity ;
    skos:definition "Climbing frame."@en ;
    skos:inScheme piirritev:OsmPlayground ;
    skos:prefLabel "Climbingframe"@en .

piirritev:OsmPlaygroundSandpit a skos:Concept ;
    piirrite:hasRelatedOsmTag piirrite:hasOsmSandpitBaby,
        piirrite:hasOsmSandpitBlind,
        piirrite:hasOsmSandpitCentralkey,
        piirrite:hasOsmSandpitLeisure,
        piirrite:hasOsmSandpitMaterial,
        piirrite:hasOsmSandpitMaxAge,
        piirrite:hasOsmSandpitMinAge,
        piirrite:hasOsmSandpitName,
        piirrite:hasOsmSandpitSittingDisability,
        piirrite:hasOsmSandpitWalkingDisability,
        piirrite:hasOsmSandpitWheelchair ;
    piirrite:osmId "sandpit" ;
    rdfs:subClassOf piirrite:OsmEntity ;
    skos:definition "Sandbox, container or shallow depression filled with soft sand."@en ;
    skos:inScheme piirritev:OsmPlayground ;
    skos:prefLabel "Sandpit"@en .

piirritev:OsmPlaygroundSeesaw a skos:Concept ;
    piirrite:hasRelatedOsmTag piirrite:hasOsmSeesawBlind,
        piirrite:hasOsmSeesawCentralkey,
        piirrite:hasOsmSeesawLeisure,
        piirrite:hasOsmSeesawMaterial,
        piirrite:hasOsmSeesawMaxAge,
        piirrite:hasOsmSeesawMinAge,
        piirrite:hasOsmSeesawName,
        piirrite:hasOsmSeesawSittingDisability,
        piirrite:hasOsmSeesawSurface,
        piirrite:hasOsmSeesawWalkingDisability,
        piirrite:hasOsmSeesawWheelchair ;
    piirrite:osmId "seesaw" ;
    rdfs:subClassOf piirrite:OsmEntity ;
    skos:definition "A seesaw for children to ride on in playgrounds."@en ;
    skos:inScheme piirritev:OsmPlayground ;
    skos:prefLabel "Seesaw"@en .

piirritev:OsmPlaygroundSlide a skos:Concept ;
    piirrite:hasRelatedOsmTag piirrite:hasOsmSlideBaby,
        piirrite:hasOsmSlideBlind,
        piirrite:hasOsmSlideCentralkey,
        piirrite:hasOsmSlideLeisure,
        piirrite:hasOsmSlideMaterial,
        piirrite:hasOsmSlideMaxAge,
        piirrite:hasOsmSlideMinAge,
        piirrite:hasOsmSlideName,
        piirrite:hasOsmSlideSittingDisability,
        piirrite:hasOsmSlideWalkingDisability,
        piirrite:hasOsmSlideWheelchair ;
    piirrite:osmId "slide" ;
    rdfs:subClassOf piirrite:OsmEntity ;
    skos:definition "A slide for children to play on in playgrounds."@en ;
    skos:inScheme piirritev:OsmPlayground ;
    skos:prefLabel "Slide"@en .

piirritev:OsmPlaygroundSpringy a skos:Concept ;
    piirrite:hasRelatedOsmTag piirrite:hasOsmSpringyLeisure,
        piirrite:hasOsmSpringyMaterial,
        piirrite:hasOsmSpringySurface ;
    piirrite:osmId "springy" ;
    rdfs:subClassOf piirrite:OsmEntity ;
    skos:definition "A seat for children on a helical spring to ride on."@en ;
    skos:inScheme piirritev:OsmPlayground ;
    skos:prefLabel "Springy"@en .

piirritev:OsmPlaygroundStructure a skos:Concept ;
    piirrite:hasRelatedOsmTag piirrite:hasOsmStructureBaby,
        piirrite:hasOsmStructureBlind,
        piirrite:hasOsmStructureCentralkey,
        piirrite:hasOsmStructureLeisure,
        piirrite:hasOsmStructureMaterial,
        piirrite:hasOsmStructureMaxAge,
        piirrite:hasOsmStructureMinAge,
        piirrite:hasOsmStructureName,
        piirrite:hasOsmStructureSittingDisability,
        piirrite:hasOsmStructureWalkingDisability,
        piirrite:hasOsmStructureWheelchair ;
    piirrite:osmId "structure" ;
    rdfs:subClassOf piirrite:OsmEntity ;
    skos:definition "Complex installation of connected playground devices comprising platforms, towers, bridges, to which further climbing/slide/swing devices can be attached to."@en ;
    skos:inScheme piirritev:OsmPlayground ;
    skos:prefLabel "Structure"@en .

piirritev:OsmPlaygroundSwing a skos:Concept ;
    piirrite:hasRelatedOsmTag piirrite:hasOsmSwingLeisure,
        piirrite:hasOsmSwingMaterial,
        piirrite:hasOsmSwingSurface ;
    piirrite:osmId "swing" ;
    rdfs:subClassOf piirrite:OsmEntity ;
    skos:definition "A swing for children to ride on."@en ;
    skos:inScheme piirritev:OsmPlayground ;
    skos:prefLabel "Swing"@en .

piirritev:OsmPoles a skos:ConceptScheme ;
    piirrite:osmId "poles" ;
    skos:definition "Used mainly in combination with power poles or power converter to specify further details."@en ;
    skos:prefLabel "Poles, types"@en .

piirritev:OsmPopulation a skos:ConceptScheme ;
    piirrite:osmId "population" ;
    skos:definition "Indicates a rough number of citizens in a given place."@en ;
    skos:prefLabel "Population, types"@en .

piirritev:OsmPostalCode a skos:ConceptScheme ;
    piirrite:osmId "postal_code" ;
    skos:definition "For tagging postal codes of streets and areas."@en ;
    skos:prefLabel "Postal code, types"@en .

piirritev:OsmPowerCable a skos:Concept ;
    piirrite:hasRelatedOsmTag piirrite:hasOsmCableCables,
        piirrite:hasOsmCableCircuits,
        piirrite:hasOsmCableLocation,
        piirrite:hasOsmCableName,
        piirrite:hasOsmCableOperator,
        piirrite:hasOsmCableRef,
        piirrite:hasOsmCableVoltage ;
    piirrite:osmId "cable" ;
    rdfs:subClassOf piirrite:OsmEntity ;
    skos:definition "An insulated cable carrying electrical power, such as transmission or distribution cables located underground and undersea cables"@en ;
    skos:inScheme piirritev:OsmPower ;
    skos:prefLabel "Cable"@en .

piirritev:OsmPowerCatenaryMast a skos:Concept ;
    piirrite:hasRelatedOsmTag piirrite:hasOsmCatenaryMastInsulation,
        piirrite:hasOsmCatenaryMastStructure,
        piirrite:hasOsmCatenaryMastTensioning ;
    piirrite:osmId "catenary_mast" ;
    rdfs:subClassOf piirrite:OsmEntity ;
    skos:definition "A pole supporting the overhead wires used to supply electricity to vehicles equipped with a pantograph such as trams and trains."@en ;
    skos:inScheme piirritev:OsmPower ;
    skos:prefLabel "Catenary mast"@en .

piirritev:OsmPowerCatenaryPortal a skos:Concept ;
    piirrite:osmId "catenary_portal" ;
    rdfs:subClassOf piirrite:OsmEntity ;
    skos:definition "Supporting structure for overhead lines (OLE), present in multi-railway lines."@en ;
    skos:inScheme piirritev:OsmPower ;
    skos:prefLabel "Catenary portal"@en .

piirritev:OsmPowerCircuit a skos:Concept ;
    piirrite:hasRelatedOsmTag piirrite:hasOsmCircuitCables,
        piirrite:hasOsmCircuitFrequency,
        piirrite:hasOsmCircuitOperator,
        piirrite:hasOsmCircuitRef,
        piirrite:hasOsmCircuitTopology,
        piirrite:hasOsmCircuitVoltage ;
    piirrite:osmId "circuit" ;
    rdfs:subClassOf piirrite:OsmEntity ;
    skos:definition "Arrangement of connected physical lines involved in the same connected power system."@en ;
    skos:inScheme piirritev:OsmPower ;
    skos:prefLabel "Circuit"@en .

piirritev:OsmPowerConnection a skos:Concept ;
    piirrite:hasRelatedOsmTag piirrite:hasOsmConnectionCables ;
    piirrite:osmId "connection" ;
    rdfs:subClassOf piirrite:OsmEntity ;
    skos:definition "A free-standing electrical connection between two or more power lines or cables."@en ;
    skos:inScheme piirritev:OsmPower ;
    skos:prefLabel "Connection"@en .

piirritev:OsmPowerGenerator a skos:Concept ;
    piirrite:hasRelatedOsmTag piirrite:hasOsmGeneratorFrequency,
        piirrite:hasOsmGeneratorName,
        piirrite:hasOsmGeneratorOperator ;
    piirrite:osmId "generator" ;
    rdfs:subClassOf piirrite:OsmEntity ;
    skos:definition "A device which converts one form of energy to another, for example, an electrical generator.  osmcarto-rendering = File:Area power.png  osmcarto-rendering-size = 125px"@en ;
    skos:inScheme piirritev:OsmPower ;
    skos:prefLabel "Generator"@en .

piirritev:OsmPowerHeliostat a skos:Concept ;
    piirrite:osmId "heliostat" ;
    rdfs:subClassOf piirrite:OsmEntity ;
    skos:definition "A mirror of a heliostat device"@en ;
    skos:inScheme piirritev:OsmPower ;
    skos:prefLabel "Heliostat"@en .

piirritev:OsmPowerInsulator a skos:Concept ;
    piirrite:hasRelatedOsmTag piirrite:hasOsmInsulatorLineArrangement,
        piirrite:hasOsmInsulatorLineAttachment,
        piirrite:hasOsmInsulatorLineManagement,
        piirrite:hasOsmInsulatorOperator ;
    piirrite:osmId "insulator" ;
    rdfs:subClassOf piirrite:OsmEntity ;
    skos:definition "An electrical insulator which connects a power line to a support structure and prevents grounding."@en ;
    skos:inScheme piirritev:OsmPower ;
    skos:prefLabel "Insulator"@en .

piirritev:OsmPowerLine a skos:Concept ;
    piirrite:hasRelatedOsmTag piirrite:hasOsmLineCables,
        piirrite:hasOsmLineCircuits,
        piirrite:hasOsmLineFrequency,
        piirrite:hasOsmLineOperator,
        piirrite:hasOsmLineRef,
        piirrite:hasOsmLineType,
        piirrite:hasOsmLineVoltage,
        piirrite:hasOsmLineWires ;
    piirrite:osmId "line" ;
    rdfs:subClassOf piirrite:OsmEntity ;
    skos:definition "High-voltage power lines used for power transmission, usually supported by towers or pylons osmcarto-rendering=File:Power line.png osmcarto-rendering-size=125px"@en ;
    skos:inScheme piirritev:OsmPower ;
    skos:prefLabel "Line"@en .

piirritev:OsmPowerPlant a skos:Concept ;
    piirrite:hasRelatedOsmTag piirrite:hasOsmPlantName,
        piirrite:hasOsmPlantOperator,
        piirrite:hasOsmPlantStartDate ;
    piirrite:osmId "plant" ;
    rdfs:subClassOf piirrite:OsmEntity ;
    skos:definition "An industrial facility where power (electricity, useful heat, biogas) is produced by individual power generator units. osmcarto-rendering=File:Area power.png osmcarto-rendering-size=100px"@en ;
    skos:inScheme piirritev:OsmPower ;
    skos:prefLabel "Plant"@en .

piirritev:OsmPowerPole a skos:Concept ;
    piirrite:hasRelatedOsmTag piirrite:hasOsmPoleDesign,
        piirrite:hasOsmPoleFrequency,
        piirrite:hasOsmPoleGuyed,
        piirrite:hasOsmPoleHeight,
        piirrite:hasOsmPoleHighway,
        piirrite:hasOsmPoleLineArrangement,
        piirrite:hasOsmPoleLineAttachment,
        piirrite:hasOsmPoleLineManagement,
        piirrite:hasOsmPoleManMade,
        piirrite:hasOsmPoleMaterial,
        piirrite:hasOsmPoleOperator,
        piirrite:hasOsmPolePhases,
        piirrite:hasOsmPolePower,
        piirrite:hasOsmPoleRating,
        piirrite:hasOsmPoleRef,
        piirrite:hasOsmPoleSubstation,
        piirrite:hasOsmPoleTower,
        piirrite:hasOsmPoleTransformer ;
    piirrite:osmId "pole" ;
    rdfs:subClassOf piirrite:OsmEntity ;
    skos:definition "A single pole supporting power lines, often a wood, steel, or concrete mast designed to carry minor power lines. osmcarto-rendering=File:Power tower small.svg osmcarto-rendering-size=6px"@en ;
    skos:inScheme piirritev:OsmPower ;
    skos:prefLabel "Pole"@en .

piirritev:OsmPowerPortal a skos:Concept ;
    piirrite:hasRelatedOsmTag piirrite:hasOsmPortalHeight,
        piirrite:hasOsmPortalOperator ;
    piirrite:osmId "portal" ;
    rdfs:subClassOf piirrite:OsmEntity ;
    skos:definition "A supporting structure for power lines, composed of vertical legs with cables between them attached to a horizontal crossarm."@en ;
    skos:inScheme piirritev:OsmPower ;
    skos:prefLabel "Portal"@en .

piirritev:OsmPowerSubstation a skos:Concept ;
    piirrite:hasRelatedOsmTag piirrite:hasOsmSubstationLocation,
        piirrite:hasOsmSubstationOperator,
        piirrite:hasOsmSubstationRef,
        piirrite:hasOsmSubstationType,
        piirrite:hasOsmSubstationVoltage ;
    piirrite:osmId "substation" ;
    rdfs:subClassOf piirrite:OsmEntity ;
    skos:definition "A facility which controls the flow of electricity in a power network with transformers, switchgear or compensators. osmcarto-rendering= File:Area power.png osmcarto-rendering-size = 125px"@en ;
    skos:inScheme piirritev:OsmPower ;
    skos:prefLabel "Substation"@en .

piirritev:OsmPowerSwitch a skos:Concept ;
    piirrite:hasRelatedOsmTag piirrite:hasOsmSwitchCables,
        piirrite:hasOsmSwitchOperator,
        piirrite:hasOsmSwitchType,
        piirrite:hasOsmSwitchVoltage ;
    piirrite:osmId "switch" ;
    rdfs:subClassOf piirrite:OsmEntity ;
    skos:definition "A device which allows electrical network operators to power up & down lines and transformers in substations or along the power grid."@en ;
    skos:inScheme piirritev:OsmPower ;
    skos:prefLabel "Switch"@en .

piirritev:OsmPowerTerminal a skos:Concept ;
    piirrite:hasRelatedOsmTag piirrite:hasOsmTerminalHeight,
        piirrite:hasOsmTerminalOperator ;
    piirrite:osmId "terminal" ;
    rdfs:subClassOf piirrite:OsmEntity ;
    skos:definition "A point of connection where an overhead power line ends on a building or wall; for example, when connecting it to an indoor substation."@en ;
    skos:inScheme piirritev:OsmPower ;
    skos:prefLabel "Terminal"@en .

piirritev:OsmPowerTower a skos:Concept ;
    piirrite:hasRelatedOsmTag piirrite:hasOsmTowerHeight,
        piirrite:hasOsmTowerLineArrangement,
        piirrite:hasOsmTowerLineAttachment,
        piirrite:hasOsmTowerLineManagement,
        piirrite:hasOsmTowerMaterial,
        piirrite:hasOsmTowerOperator,
        piirrite:hasOsmTowerRef,
        piirrite:hasOsmTowerStructure ;
    piirrite:osmId "tower" ;
    rdfs:subClassOf piirrite:OsmEntity ;
    skos:definition "A tower or pylon carrying high voltage electricity cables. Often constructed from steel latticework but tubular or solid pylons are also used. osmcarto-rendering=File:Power tower.svg osmcarto-rendering-size=14px"@en ;
    skos:inScheme piirritev:OsmPower ;
    skos:prefLabel "Tower"@en .

piirritev:OsmPowerTransformer a skos:Concept ;
    piirrite:hasRelatedOsmTag piirrite:hasOsmTransformerFrequency,
        piirrite:hasOsmTransformerLocation,
        piirrite:hasOsmTransformerOperator,
        piirrite:hasOsmTransformerRating,
        piirrite:hasOsmTransformerType,
        piirrite:hasOsmTransformerWindings ;
    piirrite:osmId "transformer" ;
    rdfs:subClassOf piirrite:OsmEntity ;
    skos:definition "A device for stepping up or down electric voltage. Large power transformers are typically located inside substations"@en ;
    skos:inScheme piirritev:OsmPower ;
    skos:prefLabel "Transformer"@en .

piirritev:OsmPriorityRoadDesignated a skos:Concept ;
    piirrite:osmId "designated" ;
    rdfs:subClassOf piirrite:OsmEntity ;
    skos:definition ""@en ;
    skos:inScheme piirritev:OsmPriorityRoad ;
    skos:prefLabel "Designated"@en .

piirritev:OsmProduceRice a skos:Concept ;
    piirrite:osmId "rice" ;
    rdfs:subClassOf piirrite:OsmEntity ;
    skos:definition ""@en ;
    skos:inScheme piirritev:OsmProduce ;
    skos:prefLabel "Rice"@en .

piirritev:OsmProduceTimber a skos:Concept ;
    piirrite:osmId "timber" ;
    rdfs:subClassOf piirrite:OsmEntity ;
    skos:definition ""@en ;
    skos:inScheme piirritev:OsmProduce ;
    skos:prefLabel "Timber"@en .

piirritev:OsmProductCharcoal a skos:Concept ;
    piirrite:osmId "charcoal" ;
    rdfs:subClassOf piirrite:OsmEntity ;
    skos:definition ""@en ;
    skos:inScheme piirritev:OsmProduct ;
    skos:prefLabel "Charcoal"@en .

piirritev:OsmProductFood a skos:Concept ;
    piirrite:hasRelatedOsmTag piirrite:hasOsmFoodBrand,
        piirrite:hasOsmFoodEmail,
        piirrite:hasOsmFoodName,
        piirrite:hasOsmFoodOpeningHours,
        piirrite:hasOsmFoodOperator,
        piirrite:hasOsmFoodPhone,
        piirrite:hasOsmFoodWebsite,
        piirrite:hasOsmFoodWheelchair ;
    piirrite:osmId "food" ;
    rdfs:subClassOf piirrite:OsmEntity ;
    skos:definition "For factories that produce food."@en ;
    skos:inScheme piirritev:OsmProduct ;
    skos:prefLabel "Food"@en .

piirritev:OsmProposedMotorway a skos:Concept ;
    piirrite:osmId "motorway" ;
    rdfs:subClassOf piirrite:OsmEntity ;
    skos:definition ""@en ;
    skos:inScheme piirritev:OsmProposed ;
    skos:prefLabel "Motorway"@en .

piirritev:OsmProposedRail a skos:Concept ;
    piirrite:osmId "rail" ;
    rdfs:subClassOf piirrite:OsmEntity ;
    skos:definition ""@en ;
    skos:inScheme piirritev:OsmProposed ;
    skos:prefLabel "Rail"@en .

piirritev:OsmProposedResidential a skos:Concept ;
    piirrite:osmId "residential" ;
    rdfs:subClassOf piirrite:OsmEntity ;
    skos:definition ""@en ;
    skos:inScheme piirritev:OsmProposed ;
    skos:prefLabel "Residential"@en .

piirritev:OsmProwRef a skos:ConceptScheme ;
    piirrite:osmId "prow_ref" ;
    skos:definition "The reference number for Public Rights of Way (United Kingdom), as held by the Local Authority."@en ;
    skos:prefLabel "Prow ref, types"@en .

piirritev:OsmPsvDesignated a skos:Concept ;
    piirrite:hasRelatedOsmTag piirrite:hasOsmDesignatedHighway ;
    piirrite:osmId "designated" ;
    rdfs:subClassOf piirrite:OsmEntity ;
    skos:definition "Roads and other objects accessible to public service vehicles and explicitly designated/signed for their use."@en ;
    skos:inScheme piirritev:OsmPsv ;
    skos:prefLabel "Designated"@en .

piirritev:OsmPumpManual a skos:Concept ;
    piirrite:hasRelatedOsmTag piirrite:hasOsmManualMechanicalDriver,
        piirrite:hasOsmManualPumpMechanism ;
    piirrite:osmId "manual" ;
    rdfs:subClassOf piirrite:OsmEntity ;
    skos:definition "A well that has a human powered pump."@en ;
    skos:inScheme piirritev:OsmPump ;
    skos:prefLabel "Manual"@en .

piirritev:OsmRailwayAbandoned a skos:Concept ;
    piirrite:hasRelatedOsmTag piirrite:hasOsmAbandonedBarrier,
        piirrite:hasOsmAbandonedCutting,
        piirrite:hasOsmAbandonedEmbankment ;
    piirrite:osmId "abandoned" ;
    rdfs:subClassOf piirrite:OsmEntity ;
    skos:definition "Former railway; the track has been removed but it's still visible that there used to be a railway."@en ;
    skos:inScheme piirritev:OsmRailway ;
    skos:prefLabel "Abandoned"@en .

piirritev:OsmRailwayBufferStop a skos:Concept ;
    piirrite:hasRelatedOsmTag piirrite:hasOsmBufferStopType ;
    piirrite:osmId "buffer_stop" ;
    rdfs:subClassOf piirrite:OsmEntity ;
    skos:definition "Barrier that exists on a railway to prevent trains from running off the end of the tracks."@en ;
    skos:inScheme piirritev:OsmRailway ;
    skos:prefLabel "Buffer stop"@en .

piirritev:OsmRailwayConstruction a skos:Concept ;
    piirrite:hasRelatedOsmTag piirrite:hasOsmConstructionCheckDate,
        piirrite:hasOsmConstructionOpeningDate,
        piirrite:hasOsmConstructionType ;
    piirrite:osmId "construction" ;
    rdfs:subClassOf piirrite:OsmEntity ;
    skos:definition "Railway feature under construction."@en ;
    skos:inScheme piirritev:OsmRailway ;
    skos:prefLabel "Construction"@en .

piirritev:OsmRailwayCrossing a skos:Concept ;
    piirrite:hasRelatedOsmTag piirrite:hasOsmCrossingType ;
    piirrite:osmId "crossing" ;
    rdfs:subClassOf piirrite:OsmEntity ;
    skos:definition "Marks the spot where pedestrians can cross a railway. osmcarto-rendering=File:Level crossing2.svg osmcarto-rendering-size=28px"@en ;
    skos:inScheme piirritev:OsmRailway ;
    skos:prefLabel "Crossing"@en .

piirritev:OsmRailwayDerail a skos:Concept ;
    piirrite:hasRelatedOsmTag piirrite:hasOsmDerailControl,
        piirrite:hasOsmDerailName,
        piirrite:hasOsmDerailOperator,
        piirrite:hasOsmDerailRef ;
    piirrite:osmId "derail" ;
    rdfs:subClassOf piirrite:OsmEntity ;
    skos:definition "Derails uncontrolled vehicles to protect the main track"@en ;
    skos:inScheme piirritev:OsmRailway ;
    skos:prefLabel "Derail"@en .

piirritev:OsmRailwayDisused a skos:Concept ;
    piirrite:osmId "disused" ;
    rdfs:subClassOf piirrite:OsmEntity ;
    skos:definition "A railway that is no longer used but where the track and infrastructure remain in place. osmcarto-rendering=File:Rendering-railway disused-125.png osmcarto-rendering-size=125px"@en ;
    skos:inScheme piirritev:OsmRailway ;
    skos:prefLabel "Disused"@en .

piirritev:OsmRailwayFacility a skos:Concept ;
    piirrite:osmId "facility" ;
    rdfs:subClassOf piirrite:OsmEntity ;
    skos:definition "A railway operating site (deprecated)."@en ;
    skos:inScheme piirritev:OsmRailway ;
    skos:prefLabel "Facility"@en .

piirritev:OsmRailwayHalt a skos:Concept ;
    piirrite:hasRelatedOsmTag piirrite:hasOsmHaltEle,
        piirrite:hasOsmHaltEndDate,
        piirrite:hasOsmHaltImage,
        piirrite:hasOsmHaltName,
        piirrite:hasOsmHaltNetwork,
        piirrite:hasOsmHaltOperator,
        piirrite:hasOsmHaltPublicTransport,
        piirrite:hasOsmHaltRequestStop,
        piirrite:hasOsmHaltStartDate,
        piirrite:hasOsmHaltSubway,
        piirrite:hasOsmHaltUicName,
        piirrite:hasOsmHaltUicRef,
        piirrite:hasOsmHaltWikipedia ;
    piirrite:osmId "halt" ;
    rdfs:subClassOf piirrite:OsmEntity ;
    skos:definition "A small station, may not have a platform, trains may only stop on request.  osmcarto-rendering = File:Rendering-railway-tram stop-mapnik.png.png  osmcarto-rendering-size = 14px"@en ;
    skos:inScheme piirritev:OsmRailway ;
    skos:prefLabel "Halt"@en .

piirritev:OsmRailwayLevelCrossing a skos:Concept ;
    piirrite:osmId "level_crossing" ;
    rdfs:subClassOf piirrite:OsmEntity ;
    skos:definition "A crossing between a railway and a road. osmcarto-rendering=File:Level crossing.svg osmcarto-rendering-size=28px"@en ;
    skos:inScheme piirritev:OsmRailway ;
    skos:prefLabel "Level crossing"@en .

piirritev:OsmRailwayLightRail a skos:Concept ;
    piirrite:hasRelatedOsmTag piirrite:hasOsmLightRailBridge,
        piirrite:hasOsmLightRailElectrified,
        piirrite:hasOsmLightRailFrequency,
        piirrite:hasOsmLightRailGauge,
        piirrite:hasOsmLightRailMaxspeed,
        piirrite:hasOsmLightRailService,
        piirrite:hasOsmLightRailTunnel,
        piirrite:hasOsmLightRailVoltage,
        piirrite:hasOsmLightRailWorkrules ;
    piirrite:osmId "light_rail" ;
    rdfs:subClassOf piirrite:OsmEntity ;
    skos:definition "Rails of a light rail. osmcarto-rendering=File:Rendering-railway light rail funicular narrow gauge-125.png osmcarto-rendering-size=125px"@en ;
    skos:inScheme piirritev:OsmRailway ;
    skos:prefLabel "Light rail"@en .

piirritev:OsmRailwayMilestone a skos:Concept ;
    piirrite:osmId "milestone" ;
    rdfs:subClassOf piirrite:OsmEntity ;
    skos:definition "A stone or metal marker along a railway denoting the distance traveled."@en ;
    skos:inScheme piirritev:OsmRailway ;
    skos:prefLabel "Milestone"@en .

piirritev:OsmRailwayMiniature a skos:Concept ;
    piirrite:osmId "miniature" ;
    rdfs:subClassOf piirrite:OsmEntity ;
    skos:definition "Railway track that carries rideable miniature trains. osmcarto-rendering=File:Rendering-railway miniature.png osmcarto-rendering-size=125px"@en ;
    skos:inScheme piirritev:OsmRailway ;
    skos:prefLabel "Miniature"@en .

piirritev:OsmRailwayNarrowGauge a skos:Concept ;
    piirrite:hasRelatedOsmTag piirrite:hasOsmNarrowGaugeBridge,
        piirrite:hasOsmNarrowGaugeGauge,
        piirrite:hasOsmNarrowGaugeName,
        piirrite:hasOsmNarrowGaugeTunnel,
        piirrite:hasOsmNarrowGaugeUsage ;
    piirrite:osmId "narrow_gauge" ;
    rdfs:subClassOf piirrite:OsmEntity ;
    skos:definition "Passenger or freight trains on narrower tracks than the typical gauge for the country or state.  osmcarto-rendering = File:Rendering-railway light rail funicular narrow gauge-125.png  osmcarto-rendering-size = 125px"@en ;
    skos:inScheme piirritev:OsmRailway ;
    skos:prefLabel "Narrow gauge"@en .

piirritev:OsmRailwayPlatform a skos:Concept ;
    piirrite:hasRelatedOsmTag piirrite:hasOsmPlatformArea,
        piirrite:hasOsmPlatformElevator,
        piirrite:hasOsmPlatformName,
        piirrite:hasOsmPlatformRef,
        piirrite:hasOsmPlatformSupervised,
        piirrite:hasOsmPlatformSurface,
        piirrite:hasOsmPlatformSurveillance,
        piirrite:hasOsmPlatformTactilePaving,
        piirrite:hasOsmPlatformWidth ;
    piirrite:osmId "platform" ;
    rdfs:subClassOf piirrite:OsmEntity ;
    skos:definition "A railway platform. osmcarto-rendering-way=File:Rendering-highway_railway_platform_line.png osmcarto-rendering-way-size=100px osmcarto-rendering-area=File:Rendering-highway_railway_platform_area.png osmcarto-rendering-area-size=100px"@en ;
    skos:inScheme piirritev:OsmRailway ;
    skos:prefLabel "Platform"@en .

piirritev:OsmRailwayPlatformEdge a skos:Concept ;
    piirrite:hasRelatedOsmTag piirrite:hasOsmPlatformEdgeHeight,
        piirrite:hasOsmPlatformEdgeRef,
        piirrite:hasOsmPlatformEdgeTactilePaving ;
    piirrite:osmId "platform_edge" ;
    rdfs:subClassOf piirrite:OsmEntity ;
    skos:definition "Edge of a platform where trains stop and passengers can enter or exit a train."@en ;
    skos:inScheme piirritev:OsmRailway ;
    skos:prefLabel "Platform edge"@en .

piirritev:OsmRailwayProposed a skos:Concept ;
    piirrite:osmId "proposed" ;
    rdfs:subClassOf piirrite:OsmEntity ;
    skos:definition ""@en ;
    skos:inScheme piirritev:OsmRailway ;
    skos:prefLabel "Proposed"@en .

piirritev:OsmRailwayRail a skos:Concept ;
    piirrite:hasRelatedOsmTag piirrite:hasOsmRailElectrified,
        piirrite:hasOsmRailFrequency,
        piirrite:hasOsmRailGauge,
        piirrite:hasOsmRailName,
        piirrite:hasOsmRailRack,
        piirrite:hasOsmRailService,
        piirrite:hasOsmRailUsage,
        piirrite:hasOsmRailVoltage ;
    piirrite:osmId "rail" ;
    rdfs:subClassOf piirrite:OsmEntity ;
    skos:definition "Rails of a typical gauge track. osmcarto-rendering=File:Rendering-railway rail.png osmcarto-rendering-size=125px"@en ;
    skos:inScheme piirritev:OsmRailway ;
    skos:prefLabel "Rail"@en .

piirritev:OsmRailwayRailwayCrossing a skos:Concept ;
    piirrite:osmId "railway_crossing" ;
    rdfs:subClassOf piirrite:OsmEntity ;
    skos:definition "Crossing rails that do not interconnect"@en ;
    skos:inScheme piirritev:OsmRailway ;
    skos:prefLabel "Railway crossing"@en .

piirritev:OsmRailwayRazed a skos:Concept ;
    piirrite:osmId "razed" ;
    rdfs:subClassOf piirrite:OsmEntity ;
    skos:definition "Former railway; Railway physical features are completely removed."@en ;
    skos:inScheme piirritev:OsmRailway ;
    skos:prefLabel "Razed"@en .

piirritev:OsmRailwaySignal a skos:Concept ;
    piirrite:osmId "signal" ;
    rdfs:subClassOf piirrite:OsmEntity ;
    skos:definition "A railway signal"@en ;
    skos:inScheme piirritev:OsmRailway ;
    skos:prefLabel "Signal"@en .

piirritev:OsmRailwaySignalBox a skos:Concept ;
    piirrite:hasRelatedOsmTag piirrite:hasOsmSignalBoxAbandoned,
        piirrite:hasOsmSignalBoxDisused,
        piirrite:hasOsmSignalBoxName,
        piirrite:hasOsmSignalBoxRazed ;
    piirrite:osmId "signal_box" ;
    rdfs:subClassOf piirrite:OsmEntity ;
    skos:definition "Signal box"@en ;
    skos:inScheme piirritev:OsmRailway ;
    skos:prefLabel "Signal box"@en .

piirritev:OsmRailwayStation a skos:Concept ;
    piirrite:hasRelatedOsmTag piirrite:hasOsmStationEle,
        piirrite:hasOsmStationEndDate,
        piirrite:hasOsmStationImage,
        piirrite:hasOsmStationName,
        piirrite:hasOsmStationNetwork,
        piirrite:hasOsmStationOperatingTimes,
        piirrite:hasOsmStationOperator,
        piirrite:hasOsmStationStartDate,
        piirrite:hasOsmStationSubway,
        piirrite:hasOsmStationUicName,
        piirrite:hasOsmStationUicRef,
        piirrite:hasOsmStationWikipedia ;
    piirrite:osmId "station" ;
    rdfs:subClassOf piirrite:OsmEntity ;
    skos:definition "A railway station.  osmcarto-rendering = File:Rendering-railway-tram stop-mapnik.png.png  osmcarto-rendering-size = 12px  osmcarto-rendering-area = File:Landuse-industrial.png  osmcarto-rendering-area-size = 100px"@en ;
    skos:inScheme piirritev:OsmRailway ;
    skos:prefLabel "Station"@en .

piirritev:OsmRailwayStop a skos:Concept ;
    piirrite:osmId "stop" ;
    rdfs:subClassOf piirrite:OsmEntity ;
    skos:definition "The spot on a railway track where a train stops at a station."@en ;
    skos:inScheme piirritev:OsmRailway ;
    skos:prefLabel "Stop"@en .

piirritev:OsmRailwaySubway a skos:Concept ;
    piirrite:osmId "subway" ;
    rdfs:subClassOf piirrite:OsmEntity ;
    skos:definition "Rails used for city public transport that are always completely separated from other traffic, often underground. osmcarto-rendering=File:Rendering-railway subway.png osmcarto-rendering-size=125px"@en ;
    skos:inScheme piirritev:OsmRailway ;
    skos:prefLabel "Subway"@en .

piirritev:OsmRailwaySubwayEntrance a skos:Concept ;
    piirrite:hasRelatedOsmTag piirrite:hasOsmSubwayEntranceEntrance,
        piirrite:hasOsmSubwayEntranceName,
        piirrite:hasOsmSubwayEntranceRef,
        piirrite:hasOsmSubwayEntranceWheelchair ;
    piirrite:osmId "subway_entrance" ;
    rdfs:subClassOf piirrite:OsmEntity ;
    skos:definition "The entrance point of a subway."@en ;
    skos:inScheme piirritev:OsmRailway ;
    skos:prefLabel "Subway entrance"@en .

piirritev:OsmRailwaySwitch a skos:Concept ;
    piirrite:hasRelatedOsmTag piirrite:hasOsmSwitchRef ;
    piirrite:osmId "switch" ;
    rdfs:subClassOf piirrite:OsmEntity ;
    skos:definition "A railway switch, turnout or points: where trains can change from one track to another track."@en ;
    skos:inScheme piirritev:OsmRailway ;
    skos:prefLabel "Switch"@en .

piirritev:OsmRailwayTram a skos:Concept ;
    piirrite:osmId "tram" ;
    rdfs:subClassOf piirrite:OsmEntity ;
    skos:definition "Tram rails or tracks.  osmcarto-rendering = File:Rendering-railway tram.png  osmcarto-rendering-size = 125px"@en ;
    skos:inScheme piirritev:OsmRailway ;
    skos:prefLabel "Tram"@en .

piirritev:OsmRailwayTramCrossing a skos:Concept ;
    piirrite:hasRelatedOsmTag piirrite:hasOsmTramCrossingRailway ;
    piirrite:osmId "tram_crossing" ;
    rdfs:subClassOf piirrite:OsmEntity ;
    skos:definition "Pedestrians can cross a tramway here."@en ;
    skos:inScheme piirritev:OsmRailway ;
    skos:prefLabel "Tram crossing"@en .

piirritev:OsmRailwayTramStop a skos:Concept ;
    piirrite:hasRelatedOsmTag piirrite:hasOsmTramStopEndDate,
        piirrite:hasOsmTramStopName,
        piirrite:hasOsmTramStopNetwork,
        piirrite:hasOsmTramStopOperator,
        piirrite:hasOsmTramStopPublicTransport,
        piirrite:hasOsmTramStopShelter,
        piirrite:hasOsmTramStopStartDate,
        piirrite:hasOsmTramStopTram ;
    piirrite:osmId "tram_stop" ;
    rdfs:subClassOf piirrite:OsmEntity ;
    skos:definition "A tram stop is a place where a passenger can embark or disembark a tram.  osmcarto-rendering = File:Rendering-railway-tram stop-mapnik.png.png  osmcarto-rendering-size = 14px"@en ;
    skos:inScheme piirritev:OsmRailway ;
    skos:prefLabel "Tram stop"@en .

piirritev:OsmRampSeparate a skos:Concept ;
    piirrite:osmId "separate" ;
    rdfs:subClassOf piirrite:OsmEntity ;
    skos:definition ""@en ;
    skos:inScheme piirritev:OsmRamp ;
    skos:prefLabel "Separate"@en .

piirritev:OsmRefA a skos:Concept ;
    piirrite:osmId "A" ;
    rdfs:subClassOf piirrite:OsmEntity ;
    skos:definition ""@en ;
    skos:inScheme piirritev:OsmRef ;
    skos:prefLabel "A"@en .

piirritev:OsmRefA1 a skos:Concept ;
    piirrite:osmId "A1" ;
    rdfs:subClassOf piirrite:OsmEntity ;
    skos:definition ""@en ;
    skos:inScheme piirritev:OsmRef ;
    skos:prefLabel "A1"@en .

piirritev:OsmRefA2 a skos:Concept ;
    piirrite:osmId "A2" ;
    rdfs:subClassOf piirrite:OsmEntity ;
    skos:definition ""@en ;
    skos:inScheme piirritev:OsmRef ;
    skos:prefLabel "A2"@en .

piirritev:OsmRefA3 a skos:Concept ;
    piirrite:osmId "A3" ;
    rdfs:subClassOf piirrite:OsmEntity ;
    skos:definition ""@en ;
    skos:inScheme piirritev:OsmRef ;
    skos:prefLabel "A3"@en .

piirritev:OsmRefA4 a skos:Concept ;
    piirrite:osmId "A4" ;
    rdfs:subClassOf piirrite:OsmEntity ;
    skos:definition ""@en ;
    skos:inScheme piirritev:OsmRef ;
    skos:prefLabel "A4"@en .

piirritev:OsmRefA6 a skos:Concept ;
    piirrite:osmId "A6" ;
    rdfs:subClassOf piirrite:OsmEntity ;
    skos:definition ""@en ;
    skos:inScheme piirritev:OsmRef ;
    skos:prefLabel "A6"@en .

piirritev:OsmRefB a skos:Concept ;
    piirrite:osmId "B" ;
    rdfs:subClassOf piirrite:OsmEntity ;
    skos:definition ""@en ;
    skos:inScheme piirritev:OsmRef ;
    skos:prefLabel "B"@en .

piirritev:OsmRefC a skos:Concept ;
    piirrite:osmId "C" ;
    rdfs:subClassOf piirrite:OsmEntity ;
    skos:definition ""@en ;
    skos:inScheme piirritev:OsmRef ;
    skos:prefLabel "C"@en .

piirritev:OsmRefD a skos:Concept ;
    piirrite:osmId "D" ;
    rdfs:subClassOf piirrite:OsmEntity ;
    skos:definition ""@en ;
    skos:inScheme piirritev:OsmRef ;
    skos:prefLabel "D"@en .

piirritev:OsmRefE a skos:Concept ;
    piirrite:osmId "E" ;
    rdfs:subClassOf piirrite:OsmEntity ;
    skos:definition ""@en ;
    skos:inScheme piirritev:OsmRef ;
    skos:prefLabel "E"@en .

piirritev:OsmRefUs1 a skos:Concept ;
    piirrite:osmId "US_1" ;
    rdfs:subClassOf piirrite:OsmEntity ;
    skos:definition ""@en ;
    skos:inScheme piirritev:OsmRef ;
    skos:prefLabel "Us 1"@en .

piirritev:OsmRegRef a skos:ConceptScheme ;
    piirrite:osmId "reg_ref" ;
    skos:definition "Regional reference"@en ;
    skos:prefLabel "Reg ref, types"@en .

piirritev:OsmReligionBuddhist a skos:Concept ;
    piirrite:hasRelatedOsmTag piirrite:hasOsmBuddhistName ;
    piirrite:osmId "buddhist" ;
    rdfs:subClassOf piirrite:OsmEntity ;
    skos:definition "Describes that a feature is related to buddhism"@en ;
    skos:inScheme piirritev:OsmReligion ;
    skos:prefLabel "Buddhist"@en .

piirritev:OsmReligionChristian a skos:Concept ;
    piirrite:osmId "christian" ;
    rdfs:subClassOf piirrite:OsmEntity ;
    skos:definition "Classify a religious feature (e.g. church) as Christian"@en ;
    skos:inScheme piirritev:OsmReligion ;
    skos:prefLabel "Christian"@en .

piirritev:OsmReligionHindu a skos:Concept ;
    piirrite:hasRelatedOsmTag piirrite:hasOsmHinduAmenity,
        piirrite:hasOsmHinduLanduse ;
    piirrite:osmId "hindu" ;
    rdfs:subClassOf piirrite:OsmEntity ;
    skos:definition "Classify a religious feature (e.g. temple) as Hindu"@en ;
    skos:inScheme piirritev:OsmReligion ;
    skos:prefLabel "Hindu"@en .

piirritev:OsmReligionJewish a skos:Concept ;
    piirrite:hasRelatedOsmTag piirrite:hasOsmJewishAmenity,
        piirrite:hasOsmJewishLanduse ;
    piirrite:osmId "jewish" ;
    rdfs:subClassOf piirrite:OsmEntity ;
    skos:definition "Classify a feature (e.g. synagogue) as Jewish. osmcarto-rendering=File:Jewish.svg osmcarto-rendering-size=28px"@en ;
    skos:inScheme piirritev:OsmReligion ;
    skos:prefLabel "Jewish"@en .

piirritev:OsmReligionMuslim a skos:Concept ;
    piirrite:hasRelatedOsmTag piirrite:hasOsmMuslimAmenity,
        piirrite:hasOsmMuslimLanduse ;
    piirrite:osmId "muslim" ;
    rdfs:subClassOf piirrite:OsmEntity ;
    skos:definition "Classify a religious feature (e.g. a mosque) as Islamic"@en ;
    skos:inScheme piirritev:OsmReligion ;
    skos:prefLabel "Muslim"@en .

piirritev:OsmReligionShinto a skos:Concept ;
    piirrite:osmId "shinto" ;
    rdfs:subClassOf piirrite:OsmEntity ;
    skos:definition "Describes that a feature is related to Shinto."@en ;
    skos:inScheme piirritev:OsmReligion ;
    skos:prefLabel "Shinto"@en .

piirritev:OsmResidentialApartments a skos:Concept ;
    piirrite:osmId "apartments" ;
    rdfs:subClassOf piirrite:OsmEntity ;
    skos:definition "Outline of an apartment complex"@en ;
    skos:inScheme piirritev:OsmResidential ;
    skos:prefLabel "Apartments"@en .

piirritev:OsmResidentialCondominium a skos:Concept ;
    piirrite:osmId "condominium" ;
    rdfs:subClassOf piirrite:OsmEntity ;
    skos:definition ""@en ;
    skos:inScheme piirritev:OsmResidential ;
    skos:prefLabel "Condominium"@en .

piirritev:OsmResidentialRural a skos:Concept ;
    piirrite:osmId "rural" ;
    rdfs:subClassOf piirrite:OsmEntity ;
    skos:definition "Residential area with low-rise buildings."@en ;
    skos:inScheme piirritev:OsmResidential ;
    skos:prefLabel "Rural"@en .

piirritev:OsmResidentialSingleFamily a skos:Concept ;
    piirrite:osmId "single_family" ;
    rdfs:subClassOf piirrite:OsmEntity ;
    skos:definition "Residential area with single family, detached houses"@en ;
    skos:inScheme piirritev:OsmResidential ;
    skos:prefLabel "Single family"@en .

piirritev:OsmResidentialTrailerPark a skos:Concept ;
    piirrite:hasRelatedOsmTag piirrite:hasOsmTrailerParkName ;
    piirrite:osmId "trailer_park" ;
    rdfs:subClassOf piirrite:OsmEntity ;
    skos:definition "Residential area consisting of prefabricated houses or static caravans (mobile homes) on small lots."@en ;
    skos:inScheme piirritev:OsmResidential ;
    skos:prefLabel "Trailer park"@en .

piirritev:OsmResidentialUrban a skos:Concept ;
    piirrite:osmId "urban" ;
    rdfs:subClassOf piirrite:OsmEntity ;
    skos:definition "Residential area with multistory buildings."@en ;
    skos:inScheme piirritev:OsmResidential ;
    skos:prefLabel "Urban"@en .

piirritev:OsmRestriction a skos:ConceptScheme ;
    piirrite:osmId "restriction" ;
    skos:definition "Type of a turn restriction at a junction or specification of parking restrictions"@en ;
    skos:prefLabel "Restriction, types"@en .

piirritev:OsmRoomOffice a skos:Concept ;
    piirrite:osmId "office" ;
    rdfs:subClassOf piirrite:OsmEntity ;
    skos:definition ""@en ;
    skos:inScheme piirritev:OsmRoom ;
    skos:prefLabel "Office"@en .

piirritev:OsmRoomShop a skos:Concept ;
    piirrite:osmId "shop" ;
    rdfs:subClassOf piirrite:OsmEntity ;
    skos:definition ""@en ;
    skos:inScheme piirritev:OsmRoom ;
    skos:prefLabel "Shop"@en .

piirritev:OsmRouteBicycle a skos:Concept ;
    piirrite:hasRelatedOsmTag piirrite:hasOsmBicycleName,
        piirrite:hasOsmBicycleNetwork,
        piirrite:hasOsmBicycleOperator,
        piirrite:hasOsmBicycleRef ;
    piirrite:osmId "bicycle" ;
    rdfs:subClassOf piirrite:OsmEntity ;
    skos:definition "Cycle routes or bicycle route are named or numbered or otherwise signed routes. May go along roads, trails or dedicated cycle paths."@en ;
    skos:inScheme piirritev:OsmRoute ;
    skos:prefLabel "Bicycle"@en .

piirritev:OsmRouteBus a skos:Concept ;
    piirrite:hasRelatedOsmTag piirrite:hasOsmBusFrom,
        piirrite:hasOsmBusName,
        piirrite:hasOsmBusNetwork,
        piirrite:hasOsmBusOperator,
        piirrite:hasOsmBusRef,
        piirrite:hasOsmBusTo ;
    piirrite:osmId "bus" ;
    rdfs:subClassOf piirrite:OsmEntity ;
    skos:definition "The route of a public bus service."@en ;
    skos:inScheme piirritev:OsmRoute ;
    skos:prefLabel "Bus"@en .

piirritev:OsmRouteFerry a skos:Concept ;
    piirrite:hasRelatedOsmTag piirrite:hasOsmFerryDuration,
        piirrite:hasOsmFerryFoot,
        piirrite:hasOsmFerryFrom,
        piirrite:hasOsmFerryHgv,
        piirrite:hasOsmFerryMotorcar,
        piirrite:hasOsmFerryName,
        piirrite:hasOsmFerryNetwork,
        piirrite:hasOsmFerryOperator,
        piirrite:hasOsmFerryRef,
        piirrite:hasOsmFerryTo,
        piirrite:hasOsmFerryType ;
    piirrite:osmId "ferry" ;
    rdfs:subClassOf piirrite:OsmEntity ;
    skos:definition "The route of a public ferry or water bus. osmcarto-rendering=File:Route_ferry.png osmcarto-rendering-size=125px"@en ;
    skos:inScheme piirritev:OsmRoute ;
    skos:prefLabel "Ferry"@en .

piirritev:OsmRouteFoot a skos:Concept ;
    piirrite:hasRelatedOsmTag piirrite:hasOsmFootDescription,
        piirrite:hasOsmFootDistance,
        piirrite:hasOsmFootName,
        piirrite:hasOsmFootOperator,
        piirrite:hasOsmFootPilgrimage,
        piirrite:hasOsmFootRoundtrip,
        piirrite:hasOsmFootSymbol ;
    piirrite:osmId "foot" ;
    rdfs:subClassOf piirrite:OsmEntity ;
    skos:definition "A signed walking Route"@en ;
    skos:inScheme piirritev:OsmRoute ;
    skos:prefLabel "Foot"@en .

piirritev:OsmRouteHiking a skos:Concept ;
    piirrite:hasRelatedOsmTag piirrite:hasOsmHikingDescription,
        piirrite:hasOsmHikingDistance,
        piirrite:hasOsmHikingName,
        piirrite:hasOsmHikingOperator,
        piirrite:hasOsmHikingPilgrimage,
        piirrite:hasOsmHikingRoundtrip,
        piirrite:hasOsmHikingSymbol ;
    piirrite:osmId "hiking" ;
    rdfs:subClassOf piirrite:OsmEntity ;
    skos:definition "A signed hiking Route"@en ;
    skos:inScheme piirritev:OsmRoute ;
    skos:prefLabel "Hiking"@en .

piirritev:OsmRouteMasterBus a skos:Concept ;
    piirrite:osmId "bus" ;
    rdfs:subClassOf piirrite:OsmEntity ;
    skos:definition ""@en ;
    skos:inScheme piirritev:OsmRouteMaster ;
    skos:prefLabel "Bus"@en .

piirritev:OsmRouteMtb a skos:Concept ;
    piirrite:hasRelatedOsmTag piirrite:hasOsmMtbName,
        piirrite:hasOsmMtbNetwork,
        piirrite:hasOsmMtbOperator,
        piirrite:hasOsmMtbRef ;
    piirrite:osmId "mtb" ;
    rdfs:subClassOf piirrite:OsmEntity ;
    skos:definition "MTB (Mountain Bike) routes are named, numbered or otherwise signed routes, designated for mountain biking. May go along roads, trails or dedicated cycle paths."@en ;
    skos:inScheme piirritev:OsmRoute ;
    skos:prefLabel "Mtb"@en .

piirritev:OsmRoutePiste a skos:Concept ;
    piirrite:hasRelatedOsmTag piirrite:hasOsmPisteType ;
    piirrite:osmId "piste" ;
    rdfs:subClassOf piirrite:OsmEntity ;
    skos:definition "Route of a winter sports piste for skiing, snowshoeing, sledding, etc. group=sports onNode=no onWay=yes onArea=no onRelation=yes requires= combination=* type=route * piste:type status=approved statuslink=Proposal:route=piste"@en ;
    skos:inScheme piirritev:OsmRoute ;
    skos:prefLabel "Piste"@en .

piirritev:OsmRoutePower a skos:Concept ;
    piirrite:osmId "power" ;
    rdfs:subClassOf piirrite:OsmEntity ;
    skos:definition ""@en ;
    skos:inScheme piirritev:OsmRoute ;
    skos:prefLabel "Power"@en .

piirritev:OsmRouteRailway a skos:Concept ;
    piirrite:hasRelatedOsmTag piirrite:hasOsmRailwayName,
        piirrite:hasOsmRailwayOperator ;
    piirrite:osmId "railway" ;
    rdfs:subClassOf piirrite:OsmEntity ;
    skos:definition "The route of a railway (e.g. the Channel Tunnel). Not to be confused with the route of a passenger train service (see tag:route=train)."@en ;
    skos:inScheme piirritev:OsmRoute ;
    skos:prefLabel "Railway"@en .

piirritev:OsmRouteRef a skos:ConceptScheme ;
    piirrite:osmId "route_ref" ;
    skos:definition "Route reference (number/code) cognizable on public transport stop signs"@en ;
    skos:prefLabel "Route ref, types"@en .

piirritev:OsmRouteRoad a skos:Concept ;
    piirrite:hasRelatedOsmTag piirrite:hasOsmRoadName,
        piirrite:hasOsmRoadRef ;
    piirrite:osmId "road" ;
    rdfs:subClassOf piirrite:OsmEntity ;
    skos:definition "Relation type used to combine road sections."@en ;
    skos:inScheme piirritev:OsmRoute ;
    skos:prefLabel "Road"@en .

piirritev:OsmRouteTrain a skos:Concept ;
    piirrite:hasRelatedOsmTag piirrite:hasOsmTrainFrom,
        piirrite:hasOsmTrainName,
        piirrite:hasOsmTrainNetwork,
        piirrite:hasOsmTrainOperator,
        piirrite:hasOsmTrainRef,
        piirrite:hasOsmTrainTo ;
    piirrite:osmId "train" ;
    rdfs:subClassOf piirrite:OsmEntity ;
    skos:definition "The route of a train service (e.g. London-Paris Eurostar)."@en ;
    skos:inScheme piirritev:OsmRoute ;
    skos:prefLabel "Train"@en .

piirritev:OsmRuinsBuilding a skos:Concept ;
    piirrite:osmId "building" ;
    rdfs:subClassOf piirrite:OsmEntity ;
    skos:definition ""@en ;
    skos:inScheme piirritev:OsmRuins ;
    skos:prefLabel "Building"@en .

piirritev:OsmSacScaleAlpineHiking a skos:Concept ;
    piirrite:osmId "alpine_hiking" ;
    rdfs:subClassOf piirrite:OsmEntity ;
    skos:definition ""@en ;
    skos:inScheme piirritev:OsmSacScale ;
    skos:prefLabel "Alpine hiking"@en .

piirritev:OsmSacScaleHiking a skos:Concept ;
    piirrite:osmId "hiking" ;
    rdfs:subClassOf piirrite:OsmEntity ;
    skos:definition ""@en ;
    skos:inScheme piirritev:OsmSacScale ;
    skos:prefLabel "Hiking"@en .

piirritev:OsmSacScaleMountainHiking a skos:Concept ;
    piirrite:osmId "mountain_hiking" ;
    rdfs:subClassOf piirrite:OsmEntity ;
    skos:definition ""@en ;
    skos:inScheme piirritev:OsmSacScale ;
    skos:prefLabel "Mountain hiking"@en .

piirritev:OsmSalt a skos:ConceptScheme ;
    piirrite:osmId "salt" ;
    skos:definition "Indicates whether water is salty."@en ;
    skos:prefLabel "Salt, types"@en .

piirritev:OsmSeasonalWetSeason a skos:Concept ;
    piirrite:osmId "wet_season" ;
    rdfs:subClassOf piirrite:OsmEntity ;
    skos:definition ""@en ;
    skos:inScheme piirritev:OsmSeasonal ;
    skos:prefLabel "Wet season"@en .

piirritev:OsmSeats a skos:ConceptScheme ;
    piirrite:osmId "seats" ;
    skos:definition "An estimate of the number of people that can comfortably sit on a bench."@en ;
    skos:prefLabel "Seats, types"@en .

piirritev:OsmSegregated a skos:ConceptScheme ;
    piirrite:osmId "segregated" ;
    skos:definition "Shows if a shared path is segregated or not."@en ;
    skos:prefLabel "Segregated, types"@en .

piirritev:OsmSelfService a skos:ConceptScheme ;
    piirrite:osmId "self_service" ;
    skos:definition "Indicates whether an object is self service."@en ;
    skos:prefLabel "Self service, types"@en .

piirritev:OsmServiceAlley a skos:Concept ;
    piirrite:osmId "alley" ;
    rdfs:subClassOf piirrite:OsmEntity ;
    skos:definition "An alley is a service road usually located between properties for access to utilities."@en ;
    skos:inScheme piirritev:OsmService ;
    skos:prefLabel "Alley"@en .

piirritev:OsmServiceCrossover a skos:Concept ;
    piirrite:hasRelatedOsmTag piirrite:hasOsmCrossoverElectrified,
        piirrite:hasOsmCrossoverGauge,
        piirrite:hasOsmCrossoverOperator ;
    piirrite:osmId "crossover" ;
    rdfs:subClassOf piirrite:OsmEntity ;
    skos:definition "A railway crossover"@en ;
    skos:inScheme piirritev:OsmService ;
    skos:prefLabel "Crossover"@en .

piirritev:OsmServiceDrive-Through a skos:Concept ;
    piirrite:hasRelatedOsmTag piirrite:hasOsmDrive-ThroughOneway ;
    piirrite:osmId "drive-through" ;
    rdfs:subClassOf piirrite:OsmEntity ;
    skos:definition "A drive-through way where customers can visit a business without leaving their cars. osmcarto-rendering=File:Rendering-highway service minor.png osmcarto-rendering-size=125px"@en ;
    skos:inScheme piirritev:OsmService ;
    skos:prefLabel "Drive-through"@en .

piirritev:OsmServiceDriveway a skos:Concept ;
    piirrite:hasRelatedOsmTag piirrite:hasOsmDrivewayAccess,
        piirrite:hasOsmDrivewayOneway ;
    piirrite:osmId "driveway" ;
    rdfs:subClassOf piirrite:OsmEntity ;
    skos:definition "Specifies that a road is a driveway, typically leading to a residence or business. osmcarto-rendering=File:Rendering-highway service minor.png osmcarto-rendering-size=125px"@en ;
    skos:inScheme piirritev:OsmService ;
    skos:prefLabel "Driveway"@en .

piirritev:OsmServiceEmergencyAccess a skos:Concept ;
    piirrite:hasRelatedOsmTag piirrite:hasOsmEmergencyAccessEmergency,
        piirrite:hasOsmEmergencyAccessSurface ;
    piirrite:osmId "emergency_access" ;
    rdfs:subClassOf piirrite:OsmEntity ;
    skos:definition "A way that is an emergency access road."@en ;
    skos:inScheme piirritev:OsmService ;
    skos:prefLabel "Emergency access"@en .

piirritev:OsmServiceIrrigation a skos:Concept ;
    piirrite:hasRelatedOsmTag piirrite:hasOsmIrrigationLocation,
        piirrite:hasOsmIrrigationWaterway ;
    piirrite:osmId "irrigation" ;
    rdfs:subClassOf piirrite:OsmEntity ;
    skos:definition "Specifies a waterway which carries water to be used for agriculture"@en ;
    skos:inScheme piirritev:OsmService ;
    skos:prefLabel "Irrigation"@en .

piirritev:OsmServiceParkingAisle a skos:Concept ;
    piirrite:hasRelatedOsmTag piirrite:hasOsmParkingAisleOneway ;
    piirrite:osmId "parking_aisle" ;
    rdfs:subClassOf piirrite:OsmEntity ;
    skos:definition "a subordinated way in a parking lot between rows of parking spaces that vehicles use to drive into and out of the spaces.  osmcarto-rendering=File:Rendering-highway service minor.png  osmcarto-rendering-size=125px"@en ;
    skos:inScheme piirritev:OsmService ;
    skos:prefLabel "Parking aisle"@en .

piirritev:OsmServiceRegional a skos:Concept ;
    piirrite:osmId "regional" ;
    rdfs:subClassOf piirrite:OsmEntity ;
    skos:definition ""@en ;
    skos:inScheme piirritev:OsmService ;
    skos:prefLabel "Regional"@en .

piirritev:OsmServiceSiding a skos:Concept ;
    piirrite:hasRelatedOsmTag piirrite:hasOsmSidingOperator,
        piirrite:hasOsmSidingRef ;
    piirrite:osmId "siding" ;
    rdfs:subClassOf piirrite:OsmEntity ;
    skos:definition "Relatively short lengths of track, running parallel to (and connected to) a main route. osmcarto-rendering=File:Rendering-railway rail service.png osmcarto-rendering-size=125px"@en ;
    skos:inScheme piirritev:OsmService ;
    skos:prefLabel "Siding"@en .

piirritev:OsmServiceSlipway a skos:Concept ;
    piirrite:osmId "slipway" ;
    rdfs:subClassOf piirrite:OsmEntity ;
    skos:definition "A ramp for launching a boat that leads into the water."@en ;
    skos:inScheme piirritev:OsmService ;
    skos:prefLabel "Slipway"@en .

piirritev:OsmServiceSpur a skos:Concept ;
    piirrite:hasRelatedOsmTag piirrite:hasOsmSpurOperator,
        piirrite:hasOsmSpurRef ;
    piirrite:osmId "spur" ;
    rdfs:subClassOf piirrite:OsmEntity ;
    skos:definition "Relatively short lengths of track, built to give one company or entity access to the main line, normally for freight-only use. osmcarto-rendering=File:Rendering-railway rail service.png osmcarto-rendering-size=125px"@en ;
    skos:inScheme piirritev:OsmService ;
    skos:prefLabel "Spur"@en .

piirritev:OsmServiceUtility a skos:Concept ;
    piirrite:osmId "utility" ;
    rdfs:subClassOf piirrite:OsmEntity ;
    skos:definition ""@en ;
    skos:inScheme piirritev:OsmService ;
    skos:prefLabel "Utility"@en .

piirritev:OsmServiceYard a skos:Concept ;
    piirrite:hasRelatedOsmTag piirrite:hasOsmYardOperator,
        piirrite:hasOsmYardRef ;
    piirrite:osmId "yard" ;
    rdfs:subClassOf piirrite:OsmEntity ;
    skos:definition "Tracks within rail yards operated by the same company as one operating main line. osmcarto-rendering=File:Rendering-railway rail service.png osmcarto-rendering-size=125px"@en ;
    skos:inScheme piirritev:OsmService ;
    skos:prefLabel "Yard"@en .

piirritev:OsmShelter a skos:ConceptScheme ;
    piirrite:osmId "shelter" ;
    skos:definition "Indicates the presence of an associated shelter."@en ;
    skos:prefLabel "Shelter, types"@en .

piirritev:OsmShelterTypeGazebo a skos:Concept ;
    piirrite:osmId "gazebo" ;
    rdfs:subClassOf piirrite:OsmEntity ;
    skos:definition "A pavilion structure, sometimes octagonal or turret-shaped, often built in a park, garden or spacious public area."@en ;
    skos:inScheme piirritev:OsmShelterType ;
    skos:prefLabel "Gazebo"@en .

piirritev:OsmShelterTypeLeanTo a skos:Concept ;
    piirrite:hasRelatedOsmTag piirrite:hasOsmLeanToBench,
        piirrite:hasOsmLeanToBin,
        piirrite:hasOsmLeanToCharge,
        piirrite:hasOsmLeanToFee,
        piirrite:hasOsmLeanToFloor,
        piirrite:hasOsmLeanToTable ;
    piirrite:osmId "lean_to" ;
    rdfs:subClassOf piirrite:OsmEntity ;
    skos:definition "A lean-to is a shed with typically three walls located in the countryside intended for camping."@en ;
    skos:inScheme piirritev:OsmShelterType ;
    skos:prefLabel "Lean to"@en .

piirritev:OsmShelterTypePicnicShelter a skos:Concept ;
    piirrite:osmId "picnic_shelter" ;
    rdfs:subClassOf piirrite:OsmEntity ;
    skos:definition "A structure on picnic sites to protect from rain."@en ;
    skos:inScheme piirritev:OsmShelterType ;
    skos:prefLabel "Picnic shelter"@en .

piirritev:OsmShelterTypePublicTransport a skos:Concept ;
    piirrite:hasRelatedOsmTag piirrite:hasOsmPublicTransportBench,
        piirrite:hasOsmPublicTransportBin,
        piirrite:hasOsmPublicTransportLit ;
    piirrite:osmId "public_transport" ;
    rdfs:subClassOf piirrite:OsmEntity ;
    skos:definition "A small shelter located at or near a public transport platform designed to provide protection for waiting passengers."@en ;
    skos:inScheme piirritev:OsmShelterType ;
    skos:prefLabel "Public transport"@en .

piirritev:OsmShelterTypeWeatherShelter a skos:Concept ;
    piirrite:osmId "weather_shelter" ;
    rdfs:subClassOf piirrite:OsmEntity ;
    skos:definition "A structure to protect from rain."@en ;
    skos:inScheme piirritev:OsmShelterType ;
    skos:prefLabel "Weather shelter"@en .

piirritev:OsmShortNameUsps a skos:Concept ;
    piirrite:osmId "USPS" ;
    rdfs:subClassOf piirrite:OsmEntity ;
    skos:definition ""@en ;
    skos:inScheme piirritev:OsmShortName ;
    skos:prefLabel "Usps"@en .

piirritev:OsmShoulderBoth a skos:Concept ;
    piirrite:osmId "both" ;
    rdfs:subClassOf piirrite:OsmEntity ;
    skos:definition ""@en ;
    skos:inScheme piirritev:OsmShoulder ;
    skos:prefLabel "Both"@en .

piirritev:OsmShoulderRight a skos:Concept ;
    piirrite:osmId "right" ;
    rdfs:subClassOf piirrite:OsmEntity ;
    skos:definition ""@en ;
    skos:inScheme piirritev:OsmShoulder ;
    skos:prefLabel "Right"@en .

piirritev:OsmSideLeft a skos:Concept ;
    piirrite:osmId "left" ;
    rdfs:subClassOf piirrite:OsmEntity ;
    skos:definition ""@en ;
    skos:inScheme piirritev:OsmSide ;
    skos:prefLabel "Left"@en .

piirritev:OsmSideRight a skos:Concept ;
    piirrite:osmId "right" ;
    rdfs:subClassOf piirrite:OsmEntity ;
    skos:definition ""@en ;
    skos:inScheme piirritev:OsmSide ;
    skos:prefLabel "Right"@en .

piirritev:OsmSidewalkBoth a skos:Concept ;
    piirrite:osmId "both" ;
    rdfs:subClassOf piirrite:OsmEntity ;
    skos:definition "Indicates that there is a sidewalk on each side of a street."@en ;
    skos:inScheme piirritev:OsmSidewalk ;
    skos:prefLabel "Both"@en .

piirritev:OsmSidewalkLeft a skos:Concept ;
    piirrite:osmId "left" ;
    rdfs:subClassOf piirrite:OsmEntity ;
    skos:definition ""@en ;
    skos:inScheme piirritev:OsmSidewalk ;
    skos:prefLabel "Left"@en .

piirritev:OsmSidewalkRight a skos:Concept ;
    piirrite:osmId "right" ;
    rdfs:subClassOf piirrite:OsmEntity ;
    skos:definition ""@en ;
    skos:inScheme piirritev:OsmSidewalk ;
    skos:prefLabel "Right"@en .

piirritev:OsmSidewalkSeparate a skos:Concept ;
    piirrite:osmId "separate" ;
    rdfs:subClassOf piirrite:OsmEntity ;
    skos:definition "Tagged on carriageway, indicates that sidewalk geometry is mapped separately"@en ;
    skos:inScheme piirritev:OsmSidewalk ;
    skos:prefLabel "Separate"@en .

piirritev:OsmSiteGeodesic a skos:Concept ;
    piirrite:osmId "geodesic" ;
    rdfs:subClassOf piirrite:OsmEntity ;
    skos:definition "Relate groups of survey point features."@en ;
    skos:inScheme piirritev:OsmSite ;
    skos:prefLabel "Geodesic"@en .

piirritev:OsmSiteParking a skos:Concept ;
    piirrite:hasRelatedOsmTag piirrite:hasOsmParkingAmenity ;
    piirrite:osmId "parking" ;
    rdfs:subClassOf piirrite:OsmEntity ;
    skos:definition "Group entrance for complex/underground parking."@en ;
    skos:inScheme piirritev:OsmSite ;
    skos:prefLabel "Parking"@en .

piirritev:OsmSiteStopArea a skos:Concept ;
    piirrite:osmId "stop_area" ;
    rdfs:subClassOf piirrite:OsmEntity ;
    skos:definition "Defines a stop area site to group public transport stops. Since there is a newer tagging scheme Public Transport v2, it is recommended to use tag:type=public_transport + tag:public_transport=stop_area instead."@en ;
    skos:inScheme piirritev:OsmSite ;
    skos:prefLabel "Stop area"@en .

piirritev:OsmSmokingOutside a skos:Concept ;
    piirrite:osmId "outside" ;
    rdfs:subClassOf piirrite:OsmEntity ;
    skos:definition ""@en ;
    skos:inScheme piirritev:OsmSmoking ;
    skos:prefLabel "Outside"@en .

piirritev:OsmSnowmobileDesignated a skos:Concept ;
    piirrite:osmId "designated" ;
    rdfs:subClassOf piirrite:OsmEntity ;
    skos:definition ""@en ;
    skos:inScheme piirritev:OsmSnowmobile ;
    skos:prefLabel "Designated"@en .

piirritev:OsmSocialFacilityAssistedLiving a skos:Concept ;
    piirrite:hasRelatedOsmTag piirrite:hasOsmAssistedLivingName,
        piirrite:hasOsmAssistedLivingOpeningHours,
        piirrite:hasOsmAssistedLivingOperator,
        piirrite:hasOsmAssistedLivingPhone,
        piirrite:hasOsmAssistedLivingWebsite,
        piirrite:hasOsmAssistedLivingWheelchair ;
    piirrite:osmId "assisted_living" ;
    rdfs:subClassOf piirrite:OsmEntity ;
    skos:definition "A residential facility like group_home, but the occupants are more independent. Usually conceived for people with minor disabilities."@en ;
    skos:inScheme piirritev:OsmSocialFacility ;
    skos:prefLabel "Assisted living"@en .

piirritev:OsmSocialFacilityGroupHome a skos:Concept ;
    piirrite:hasRelatedOsmTag piirrite:hasOsmGroupHomeCapacity,
        piirrite:hasOsmGroupHomeName,
        piirrite:hasOsmGroupHomeOperator,
        piirrite:hasOsmGroupHomePhone,
        piirrite:hasOsmGroupHomeWebsite,
        piirrite:hasOsmGroupHomeWheelchair ;
    piirrite:osmId "group_home" ;
    rdfs:subClassOf piirrite:OsmEntity ;
    skos:definition "A group home is a residence for a certain demographic, providing social and medical services, leisure activities, meals, and supervision."@en ;
    skos:inScheme piirritev:OsmSocialFacility ;
    skos:prefLabel "Group home"@en .

piirritev:OsmSocialFacilityNursingHome a skos:Concept ;
    piirrite:hasRelatedOsmTag piirrite:hasOsmNursingHomeName ;
    piirrite:osmId "nursing_home" ;
    rdfs:subClassOf piirrite:OsmEntity ;
    skos:definition "A nursing home provides permanent care to elderly, ill, or disabled people."@en ;
    skos:inScheme piirritev:OsmSocialFacility ;
    skos:prefLabel "Nursing home"@en .

piirritev:OsmSocialFacilityOutreach a skos:Concept ;
    piirrite:osmId "outreach" ;
    rdfs:subClassOf piirrite:OsmEntity ;
    skos:definition "A non-residential facility that provides social welfare services such as advocacy, counseling, job placement, veterans services, housing placement, wellness programs or leisure activities."@en ;
    skos:inScheme piirritev:OsmSocialFacility ;
    skos:prefLabel "Outreach"@en .

piirritev:OsmSource3Dshapes a skos:Concept ;
    piirrite:osmId "3dShapes" ;
    rdfs:subClassOf piirrite:OsmEntity ;
    skos:definition ""@en ;
    skos:inScheme piirritev:OsmSource ;
    skos:prefLabel "3dshapes"@en .

piirritev:OsmSourceAasacra1 a skos:Concept ;
    piirrite:osmId "aasacra1" ;
    rdfs:subClassOf piirrite:OsmEntity ;
    skos:definition ""@en ;
    skos:inScheme piirritev:OsmSource ;
    skos:prefLabel "Aasacra1"@en .

piirritev:OsmSourceAdd a skos:Concept ;
    piirrite:osmId "ADD" ;
    rdfs:subClassOf piirrite:OsmEntity ;
    skos:definition ""@en ;
    skos:inScheme piirritev:OsmSource ;
    skos:prefLabel "Add"@en .

piirritev:OsmSourceAerialImagery a skos:Concept ;
    piirrite:osmId "aerial_imagery" ;
    rdfs:subClassOf piirrite:OsmEntity ;
    skos:definition ""@en ;
    skos:inScheme piirritev:OsmSource ;
    skos:prefLabel "Aerial imagery"@en .

piirritev:OsmSourceAgis2011 a skos:Concept ;
    piirrite:osmId "AGIS_2011" ;
    rdfs:subClassOf piirrite:OsmEntity ;
    skos:definition ""@en ;
    skos:inScheme piirritev:OsmSource ;
    skos:prefLabel "Agis 2011"@en .

piirritev:OsmSourceAgis2014 a skos:Concept ;
    piirrite:osmId "AGIS_2014" ;
    rdfs:subClassOf piirrite:OsmEntity ;
    skos:definition ""@en ;
    skos:inScheme piirritev:OsmSource ;
    skos:prefLabel "Agis 2014"@en .

piirritev:OsmSourceAgisOf2011 a skos:Concept ;
    piirrite:osmId "AGIS_OF2011" ;
    rdfs:subClassOf piirrite:OsmEntity ;
    skos:definition ""@en ;
    skos:inScheme piirritev:OsmSource ;
    skos:prefLabel "Agis of2011"@en .

piirritev:OsmSourceAgiv a skos:Concept ;
    piirrite:osmId "AGIV" ;
    rdfs:subClassOf piirrite:OsmEntity ;
    skos:definition ""@en ;
    skos:inScheme piirritev:OsmSource ;
    skos:prefLabel "Agiv"@en .

piirritev:OsmSourceAhn a skos:Concept ;
    piirrite:osmId "AHN" ;
    rdfs:subClassOf piirrite:OsmEntity ;
    skos:definition ""@en ;
    skos:inScheme piirritev:OsmSource ;
    skos:prefLabel "Ahn"@en .

piirritev:OsmSourceAirbus2020 a skos:Concept ;
    piirrite:osmId "Airbus_2020" ;
    rdfs:subClassOf piirrite:OsmEntity ;
    skos:definition ""@en ;
    skos:inScheme piirritev:OsmSource ;
    skos:prefLabel "Airbus 2020"@en .

piirritev:OsmSourceAklisNiederrhein a skos:Concept ;
    piirrite:osmId "AKLIS_Niederrhein" ;
    rdfs:subClassOf piirrite:OsmEntity ;
    skos:definition ""@en ;
    skos:inScheme piirritev:OsmSource ;
    skos:prefLabel "Aklis niederrhein"@en .

piirritev:OsmSourceAkros a skos:Concept ;
    piirrite:osmId "Akros",
        "akros" ;
    rdfs:subClassOf piirrite:OsmEntity ;
    skos:definition ""@en ;
    skos:inScheme piirritev:OsmSource ;
    skos:prefLabel "Akros"@en .

piirritev:OsmSourceAlkisViersen a skos:Concept ;
    piirrite:osmId "ALKIS_Viersen" ;
    rdfs:subClassOf piirrite:OsmEntity ;
    skos:definition ""@en ;
    skos:inScheme piirritev:OsmSource ;
    skos:prefLabel "Alkis viersen"@en .

piirritev:OsmSourceAmabici a skos:Concept ;
    piirrite:osmId "amabici" ;
    rdfs:subClassOf piirrite:OsmEntity ;
    skos:definition ""@en ;
    skos:inScheme piirritev:OsmSource ;
    skos:prefLabel "Amabici"@en .

piirritev:OsmSourceAna a skos:Concept ;
    piirrite:osmId "ANA" ;
    rdfs:subClassOf piirrite:OsmEntity ;
    skos:definition ""@en ;
    skos:inScheme piirritev:OsmSource ;
    skos:prefLabel "Ana"@en .

piirritev:OsmSourceAnd a skos:Concept ;
    piirrite:osmId "AND" ;
    rdfs:subClassOf piirrite:OsmEntity ;
    skos:definition ""@en ;
    skos:inScheme piirritev:OsmSource ;
    skos:prefLabel "And"@en .

piirritev:OsmSourceAucklandCouncil a skos:Concept ;
    piirrite:osmId "Auckland_Council" ;
    rdfs:subClassOf piirrite:OsmEntity ;
    skos:definition ""@en ;
    skos:inScheme piirritev:OsmSource ;
    skos:prefLabel "Auckland council"@en .

piirritev:OsmSourceBag a skos:Concept ;
    piirrite:osmId "BAG" ;
    rdfs:subClassOf piirrite:OsmEntity ;
    skos:definition ""@en ;
    skos:inScheme piirritev:OsmSource ;
    skos:prefLabel "Bag"@en .

piirritev:OsmSourceBasemapAt a skos:Concept ;
    piirrite:osmId "basemap_at" ;
    rdfs:subClassOf piirrite:OsmEntity ;
    skos:definition ""@en ;
    skos:inScheme piirritev:OsmSource ;
    skos:prefLabel "Basemap at"@en .

piirritev:OsmSourceBasemapAt2016 a skos:Concept ;
    piirrite:osmId "basemap_at_2016" ;
    rdfs:subClassOf piirrite:OsmEntity ;
    skos:definition ""@en ;
    skos:inScheme piirritev:OsmSource ;
    skos:prefLabel "Basemap at 2016"@en .

piirritev:OsmSourceBasemapAtOrtho a skos:Concept ;
    piirrite:osmId "basemap_at_Ortho" ;
    rdfs:subClassOf piirrite:OsmEntity ;
    skos:definition ""@en ;
    skos:inScheme piirritev:OsmSource ;
    skos:prefLabel "Basemap at ortho"@en .

piirritev:OsmSourceBasemapAtOrthofoto a skos:Concept ;
    piirrite:osmId "basemap_at_Orthofoto" ;
    rdfs:subClassOf piirrite:OsmEntity ;
    skos:definition ""@en ;
    skos:inScheme piirritev:OsmSource ;
    skos:prefLabel "Basemap at orthofoto"@en .

piirritev:OsmSourceBdorthoIgn a skos:Concept ;
    piirrite:osmId "BDOrtho_IGN" ;
    rdfs:subClassOf piirrite:OsmEntity ;
    skos:definition ""@en ;
    skos:inScheme piirritev:OsmSource ;
    skos:prefLabel "Bdortho ign"@en .

piirritev:OsmSourceBgmountains a skos:Concept ;
    piirrite:osmId "bgmountains" ;
    rdfs:subClassOf piirrite:OsmEntity ;
    skos:definition ""@en ;
    skos:inScheme piirritev:OsmSource ;
    skos:prefLabel "Bgmountains"@en .

piirritev:OsmSourceBgt a skos:Concept ;
    piirrite:osmId "BGT" ;
    rdfs:subClassOf piirrite:OsmEntity ;
    skos:definition ""@en ;
    skos:inScheme piirritev:OsmSource ;
    skos:prefLabel "Bgt"@en .

piirritev:OsmSourceBgtopomaps a skos:Concept ;
    piirrite:osmId "bgtopomaps" ;
    rdfs:subClassOf piirrite:OsmEntity ;
    skos:definition ""@en ;
    skos:inScheme piirritev:OsmSource ;
    skos:prefLabel "Bgtopomaps"@en .

piirritev:OsmSourceBing a skos:Concept ;
    piirrite:osmId "BING",
        "Bing",
        "bing" ;
    rdfs:subClassOf piirrite:OsmEntity ;
    skos:definition ""@en,
        "Source of the object is from Bing imagery"@en ;
    skos:inScheme piirritev:OsmSource ;
    skos:prefLabel "Bing"@en .

piirritev:OsmSourceBing\(Adjusted\) a skos:Concept ;
    piirrite:osmId "Bing_(adjusted)" ;
    rdfs:subClassOf piirrite:OsmEntity ;
    skos:definition ""@en ;
    skos:inScheme piirritev:OsmSource ;
    skos:prefLabel "Bing (adjusted)"@en .

piirritev:OsmSourceBing2010 a skos:Concept ;
    piirrite:osmId "Bing_2010",
        "bing_2010" ;
    rdfs:subClassOf piirrite:OsmEntity ;
    skos:definition ""@en ;
    skos:inScheme piirritev:OsmSource ;
    skos:prefLabel "Bing 2010"@en .

piirritev:OsmSourceBing2011 a skos:Concept ;
    piirrite:osmId "Bing_2011" ;
    rdfs:subClassOf piirrite:OsmEntity ;
    skos:definition ""@en ;
    skos:inScheme piirritev:OsmSource ;
    skos:prefLabel "Bing 2011"@en .

piirritev:OsmSourceBing2012 a skos:Concept ;
    piirrite:osmId "Bing_2012",
        "bing2012" ;
    rdfs:subClassOf piirrite:OsmEntity ;
    skos:definition ""@en ;
    skos:inScheme piirritev:OsmSource ;
    skos:prefLabel "Bing 2012"@en,
        "Bing2012"@en .

piirritev:OsmSourceBing2012-07-30 a skos:Concept ;
    piirrite:osmId "bing_2012-07-30" ;
    rdfs:subClassOf piirrite:OsmEntity ;
    skos:definition ""@en ;
    skos:inScheme piirritev:OsmSource ;
    skos:prefLabel "Bing 2012-07-30"@en .

piirritev:OsmSourceBing2013 a skos:Concept ;
    piirrite:osmId "Bing_2013" ;
    rdfs:subClassOf piirrite:OsmEntity ;
    skos:definition ""@en ;
    skos:inScheme piirritev:OsmSource ;
    skos:prefLabel "Bing 2013"@en .

piirritev:OsmSourceBing2014 a skos:Concept ;
    piirrite:osmId "Bing_2014" ;
    rdfs:subClassOf piirrite:OsmEntity ;
    skos:definition ""@en ;
    skos:inScheme piirritev:OsmSource ;
    skos:prefLabel "Bing 2014"@en .

piirritev:OsmSourceBing2015 a skos:Concept ;
    piirrite:osmId "Bing_2015" ;
    rdfs:subClassOf piirrite:OsmEntity ;
    skos:definition ""@en ;
    skos:inScheme piirritev:OsmSource ;
    skos:prefLabel "Bing 2015"@en .

piirritev:OsmSourceBing2016 a skos:Concept ;
    piirrite:osmId "Bing_2016" ;
    rdfs:subClassOf piirrite:OsmEntity ;
    skos:definition ""@en ;
    skos:inScheme piirritev:OsmSource ;
    skos:prefLabel "Bing 2016"@en .

piirritev:OsmSourceBing2017 a skos:Concept ;
    piirrite:osmId "Bing_2017" ;
    rdfs:subClassOf piirrite:OsmEntity ;
    skos:definition ""@en ;
    skos:inScheme piirritev:OsmSource ;
    skos:prefLabel "Bing 2017"@en .

piirritev:OsmSourceBing2018 a skos:Concept ;
    piirrite:osmId "Bing_2018" ;
    rdfs:subClassOf piirrite:OsmEntity ;
    skos:definition ""@en ;
    skos:inScheme piirritev:OsmSource ;
    skos:prefLabel "Bing 2018"@en .

piirritev:OsmSourceBingAerial a skos:Concept ;
    piirrite:osmId "Bing_Aerial",
        "bing_aerial" ;
    rdfs:subClassOf piirrite:OsmEntity ;
    skos:definition ""@en ;
    skos:inScheme piirritev:OsmSource ;
    skos:prefLabel "Bing aerial"@en .

piirritev:OsmSourceBingHr a skos:Concept ;
    piirrite:osmId "bing_HR" ;
    rdfs:subClassOf piirrite:OsmEntity ;
    skos:definition ""@en ;
    skos:inScheme piirritev:OsmSource ;
    skos:prefLabel "Bing hr"@en .

piirritev:OsmSourceBingImagery a skos:Concept ;
    piirrite:osmId "Bing_Imagery",
        "Bing_imagery",
        "bing_imagery" ;
    rdfs:subClassOf piirrite:OsmEntity ;
    skos:definition ""@en ;
    skos:inScheme piirritev:OsmSource ;
    skos:prefLabel "Bing imagery"@en .

piirritev:OsmSourceBingLandsat a skos:Concept ;
    piirrite:osmId "bing_landsat" ;
    rdfs:subClassOf piirrite:OsmEntity ;
    skos:definition ""@en ;
    skos:inScheme piirritev:OsmSource ;
    skos:prefLabel "Bing landsat"@en .

piirritev:OsmSourceBingMaps a skos:Concept ;
    piirrite:osmId "Bing_Maps" ;
    rdfs:subClassOf piirrite:OsmEntity ;
    skos:definition ""@en ;
    skos:inScheme piirritev:OsmSource ;
    skos:prefLabel "Bing maps"@en .

piirritev:OsmSourceBingSat a skos:Concept ;
    piirrite:osmId "Bing_Sat",
        "bing_sat" ;
    rdfs:subClassOf piirrite:OsmEntity ;
    skos:definition ""@en ;
    skos:inScheme piirritev:OsmSource ;
    skos:prefLabel "Bing sat"@en .

piirritev:OsmSourceBingsat a skos:Concept ;
    piirrite:osmId "BingSat" ;
    rdfs:subClassOf piirrite:OsmEntity ;
    skos:definition ""@en ;
    skos:inScheme piirritev:OsmSource ;
    skos:prefLabel "Bingsat"@en .

piirritev:OsmSourceBmo2009 a skos:Concept ;
    piirrite:osmId "BMO2009" ;
    rdfs:subClassOf piirrite:OsmEntity ;
    skos:definition ""@en ;
    skos:inScheme piirritev:OsmSource ;
    skos:prefLabel "Bmo2009"@en .

piirritev:OsmSourceBymiljetaten a skos:Concept ;
    piirrite:osmId "Bymiljetaten" ;
    rdfs:subClassOf piirrite:OsmEntity ;
    skos:definition ""@en ;
    skos:inScheme piirritev:OsmSource ;
    skos:prefLabel "Bymiljetaten"@en .

piirritev:OsmSourceCadastre a skos:Concept ;
    piirrite:osmId "cadastre" ;
    rdfs:subClassOf piirrite:OsmEntity ;
    skos:definition ""@en ;
    skos:inScheme piirritev:OsmSource ;
    skos:prefLabel "Cadastre"@en .

piirritev:OsmSourceCadastre-Dgifp2025 a skos:Concept ;
    piirrite:osmId "cadastre-dgifp_2025" ;
    rdfs:subClassOf piirrite:OsmEntity ;
    skos:definition ""@en ;
    skos:inScheme piirritev:OsmSource ;
    skos:prefLabel "Cadastre-dgifp 2025"@en .

piirritev:OsmSourceCanvec a skos:Concept ;
    piirrite:osmId "CANVEC",
        "CanVec" ;
    rdfs:subClassOf piirrite:OsmEntity ;
    skos:definition ""@en ;
    skos:inScheme piirritev:OsmSource ;
    skos:prefLabel "Canvec"@en .

piirritev:OsmSourceCatastro a skos:Concept ;
    piirrite:osmId "Catastro",
        "catastro" ;
    rdfs:subClassOf piirrite:OsmEntity ;
    skos:definition ""@en ;
    skos:inScheme piirritev:OsmSource ;
    skos:prefLabel "Catastro"@en .

piirritev:OsmSourceCch a skos:Concept ;
    piirrite:osmId "CCH" ;
    rdfs:subClassOf piirrite:OsmEntity ;
    skos:definition ""@en ;
    skos:inScheme piirritev:OsmSource ;
    skos:prefLabel "Cch"@en .

piirritev:OsmSourceCcpro2016 a skos:Concept ;
    piirrite:osmId "CCPRO_2016" ;
    rdfs:subClassOf piirrite:OsmEntity ;
    skos:definition ""@en ;
    skos:inScheme piirritev:OsmSource ;
    skos:prefLabel "Ccpro 2016"@en .

piirritev:OsmSourceCcpro2021 a skos:Concept ;
    piirrite:osmId "CCPRO_2021" ;
    rdfs:subClassOf piirrite:OsmEntity ;
    skos:definition ""@en ;
    skos:inScheme piirritev:OsmSource ;
    skos:prefLabel "Ccpro 2021"@en .

piirritev:OsmSourceCidi a skos:Concept ;
    piirrite:osmId "CIDi",
        "cidi" ;
    rdfs:subClassOf piirrite:OsmEntity ;
    skos:definition ""@en ;
    skos:inScheme piirritev:OsmSource ;
    skos:prefLabel "Cidi"@en .

piirritev:OsmSourceCidiBing a skos:Concept ;
    piirrite:osmId "cidi_bing" ;
    rdfs:subClassOf piirrite:OsmEntity ;
    skos:definition ""@en ;
    skos:inScheme piirritev:OsmSource ;
    skos:prefLabel "Cidi bing"@en .

piirritev:OsmSourceCidiUci a skos:Concept ;
    piirrite:osmId "cidi_uci" ;
    rdfs:subClassOf piirrite:OsmEntity ;
    skos:definition ""@en ;
    skos:inScheme piirritev:OsmSource ;
    skos:prefLabel "Cidi uci"@en .

piirritev:OsmSourceClc2006 a skos:Concept ;
    piirrite:osmId "CLC2006" ;
    rdfs:subClassOf piirrite:OsmEntity ;
    skos:definition ""@en ;
    skos:inScheme piirritev:OsmSource ;
    skos:prefLabel "Clc2006"@en .

piirritev:OsmSourceColumbiaCounty a skos:Concept ;
    piirrite:osmId "Columbia_County" ;
    rdfs:subClassOf piirrite:OsmEntity ;
    skos:definition ""@en ;
    skos:inScheme piirritev:OsmSource ;
    skos:prefLabel "Columbia county"@en .

piirritev:OsmSourceCommune a skos:Concept ;
    piirrite:osmId "commune" ;
    rdfs:subClassOf piirrite:OsmEntity ;
    skos:definition ""@en ;
    skos:inScheme piirritev:OsmSource ;
    skos:prefLabel "Commune"@en .

piirritev:OsmSourceCorine2006 a skos:Concept ;
    piirrite:osmId "corine_2006" ;
    rdfs:subClassOf piirrite:OsmEntity ;
    skos:definition ""@en ;
    skos:inScheme piirritev:OsmSource ;
    skos:prefLabel "Corine 2006"@en .

piirritev:OsmSourceCvrd a skos:Concept ;
    piirrite:osmId "CVRD" ;
    rdfs:subClassOf piirrite:OsmEntity ;
    skos:definition ""@en ;
    skos:inScheme piirritev:OsmSource ;
    skos:prefLabel "Cvrd"@en .

piirritev:OsmSourceDane a skos:Concept ;
    piirrite:osmId "DANE" ;
    rdfs:subClassOf piirrite:OsmEntity ;
    skos:definition ""@en ;
    skos:inScheme piirritev:OsmSource ;
    skos:prefLabel "Dane"@en .

piirritev:OsmSourceDanmarksAdresseregister a skos:Concept ;
    piirrite:osmId "Danmarks_Adresseregister" ;
    rdfs:subClassOf piirrite:OsmEntity ;
    skos:definition ""@en ;
    skos:inScheme piirritev:OsmSource ;
    skos:prefLabel "Danmarks adresseregister"@en .

piirritev:OsmSourceDataRio a skos:Concept ;
    piirrite:osmId "data_rio" ;
    rdfs:subClassOf piirrite:OsmEntity ;
    skos:definition ""@en ;
    skos:inScheme piirritev:OsmSource ;
    skos:prefLabel "Data rio"@en .

piirritev:OsmSourceDataSeattleGov a skos:Concept ;
    piirrite:osmId "data_seattle_gov" ;
    rdfs:subClassOf piirrite:OsmEntity ;
    skos:definition ""@en ;
    skos:inScheme piirritev:OsmSource ;
    skos:prefLabel "Data seattle gov"@en .

piirritev:OsmSourceDataTirolGvAt a skos:Concept ;
    piirrite:osmId "data_tirol_gv_at" ;
    rdfs:subClassOf piirrite:OsmEntity ;
    skos:definition ""@en ;
    skos:inScheme piirritev:OsmSource ;
    skos:prefLabel "Data tirol gv at"@en .

piirritev:OsmSourceDatenStadttroisdorf a skos:Concept ;
    piirrite:osmId "daten_stadttroisdorf" ;
    rdfs:subClassOf piirrite:OsmEntity ;
    skos:definition ""@en ;
    skos:inScheme piirritev:OsmSource ;
    skos:prefLabel "Daten stadttroisdorf"@en .

piirritev:OsmSourceDatiEmilia-RomagnaIt a skos:Concept ;
    piirrite:osmId "dati_emilia-romagna_it" ;
    rdfs:subClassOf piirrite:OsmEntity ;
    skos:definition ""@en ;
    skos:inScheme piirritev:OsmSource ;
    skos:prefLabel "Dati emilia-romagna it"@en .

piirritev:OsmSourceDatosOficiales a skos:Concept ;
    piirrite:osmId "datos_oficiales" ;
    rdfs:subClassOf piirrite:OsmEntity ;
    skos:definition ""@en ;
    skos:inScheme piirritev:OsmSource ;
    skos:prefLabel "Datos oficiales"@en .

piirritev:OsmSourceDcgis a skos:Concept ;
    piirrite:osmId "dcgis" ;
    rdfs:subClassOf piirrite:OsmEntity ;
    skos:definition ""@en ;
    skos:inScheme piirritev:OsmSource ;
    skos:prefLabel "Dcgis"@en .

piirritev:OsmSourceDibavod a skos:Concept ;
    piirrite:osmId "dibavod" ;
    rdfs:subClassOf piirrite:OsmEntity ;
    skos:definition ""@en ;
    skos:inScheme piirritev:OsmSource ;
    skos:prefLabel "Dibavod"@en .

piirritev:OsmSourceDibavodA06 a skos:Concept ;
    piirrite:osmId "dibavod_A06" ;
    rdfs:subClassOf piirrite:OsmEntity ;
    skos:definition ""@en ;
    skos:inScheme piirritev:OsmSource ;
    skos:prefLabel "Dibavod a06"@en .

piirritev:OsmSourceDigiroadFi a skos:Concept ;
    piirrite:osmId "Digiroad_fi" ;
    rdfs:subClassOf piirrite:OsmEntity ;
    skos:definition ""@en ;
    skos:inScheme piirritev:OsmSource ;
    skos:prefLabel "Digiroad fi"@en .

piirritev:OsmSourceDigitalGlobe a skos:Concept ;
    piirrite:osmId "Digital_Globe" ;
    rdfs:subClassOf piirrite:OsmEntity ;
    skos:definition ""@en ;
    skos:inScheme piirritev:OsmSource ;
    skos:prefLabel "Digital globe"@en .

piirritev:OsmSourceDigitalglobe a skos:Concept ;
    piirrite:osmId "DigitalGlobe",
        "digitalGlobe",
        "digitalglobe" ;
    rdfs:subClassOf piirrite:OsmEntity ;
    skos:definition ""@en ;
    skos:inScheme piirritev:OsmSource ;
    skos:prefLabel "Digitalglobe"@en .

piirritev:OsmSourceDigitalglobe-Premium a skos:Concept ;
    piirrite:osmId "DigitalGlobe-Premium" ;
    rdfs:subClassOf piirrite:OsmEntity ;
    skos:definition ""@en ;
    skos:inScheme piirritev:OsmSource ;
    skos:prefLabel "Digitalglobe-premium"@en .

piirritev:OsmSourceDigitalglobe-Standard a skos:Concept ;
    piirrite:osmId "DigitalGlobe-Standard" ;
    rdfs:subClassOf piirrite:OsmEntity ;
    skos:definition ""@en ;
    skos:inScheme piirritev:OsmSource ;
    skos:prefLabel "Digitalglobe-standard"@en .

piirritev:OsmSourceDigitalglobePremium a skos:Concept ;
    piirrite:osmId "digitalGlobe_Premium" ;
    rdfs:subClassOf piirrite:OsmEntity ;
    skos:definition ""@en ;
    skos:inScheme piirritev:OsmSource ;
    skos:prefLabel "Digitalglobe premium"@en .

piirritev:OsmSourceDigitalizacja a skos:Concept ;
    piirrite:osmId "digitalizacja" ;
    rdfs:subClassOf piirrite:OsmEntity ;
    skos:definition ""@en ;
    skos:inScheme piirritev:OsmSource ;
    skos:prefLabel "Digitalizacja"@en .

piirritev:OsmSourceECzestochowaPl a skos:Concept ;
    piirrite:osmId "e_czestochowa_pl" ;
    rdfs:subClassOf piirrite:OsmEntity ;
    skos:definition ""@en ;
    skos:inScheme piirritev:OsmSource ;
    skos:prefLabel "E czestochowa pl"@en .

piirritev:OsmSourceEhealthafricaOrg a skos:Concept ;
    piirrite:osmId "ehealthafrica_org" ;
    rdfs:subClassOf piirrite:OsmEntity ;
    skos:definition ""@en ;
    skos:inScheme piirritev:OsmSource ;
    skos:prefLabel "Ehealthafrica org"@en .

piirritev:OsmSourceEmuia a skos:Concept ;
    piirrite:osmId "emuia" ;
    rdfs:subClassOf piirrite:OsmEntity ;
    skos:definition ""@en ;
    skos:inScheme piirritev:OsmSource ;
    skos:prefLabel "Emuia"@en .

piirritev:OsmSourceEmuiaGugikGovPl a skos:Concept ;
    piirrite:osmId "emuia_gugik_gov_pl" ;
    rdfs:subClassOf piirrite:OsmEntity ;
    skos:definition ""@en ;
    skos:inScheme piirritev:OsmSource ;
    skos:prefLabel "Emuia gugik gov pl"@en .

piirritev:OsmSourceEsri a skos:Concept ;
    piirrite:osmId "ESRI",
        "Esri",
        "esri" ;
    rdfs:subClassOf piirrite:OsmEntity ;
    skos:definition ""@en ;
    skos:inScheme piirritev:OsmSource ;
    skos:prefLabel "Esri"@en .

piirritev:OsmSourceEsri2022-04-28 a skos:Concept ;
    piirrite:osmId "Esri_2022-04-28" ;
    rdfs:subClassOf piirrite:OsmEntity ;
    skos:definition ""@en ;
    skos:inScheme piirritev:OsmSource ;
    skos:prefLabel "Esri 2022-04-28"@en .

piirritev:OsmSourceEsriBeta a skos:Concept ;
    piirrite:osmId "Esri_beta" ;
    rdfs:subClassOf piirrite:OsmEntity ;
    skos:definition ""@en ;
    skos:inScheme piirritev:OsmSource ;
    skos:prefLabel "Esri beta"@en .

piirritev:OsmSourceEsriVirginia a skos:Concept ;
    piirrite:osmId "esri_Virginia" ;
    rdfs:subClassOf piirrite:OsmEntity ;
    skos:definition ""@en ;
    skos:inScheme piirritev:OsmSource ;
    skos:prefLabel "Esri virginia"@en .

piirritev:OsmSourceEsriworld a skos:Concept ;
    piirrite:osmId "esriWorld" ;
    rdfs:subClassOf piirrite:OsmEntity ;
    skos:definition ""@en ;
    skos:inScheme piirritev:OsmSource ;
    skos:prefLabel "Esriworld"@en .

piirritev:OsmSourceEsriworldimagery a skos:Concept ;
    piirrite:osmId "EsriWorldImagery" ;
    rdfs:subClassOf piirrite:OsmEntity ;
    skos:definition ""@en ;
    skos:inScheme piirritev:OsmSource ;
    skos:prefLabel "Esriworldimagery"@en .

piirritev:OsmSourceEsriworldimageryclarity a skos:Concept ;
    piirrite:osmId "EsriWorldImageryClarity" ;
    rdfs:subClassOf piirrite:OsmEntity ;
    skos:definition ""@en ;
    skos:inScheme piirritev:OsmSource ;
    skos:prefLabel "Esriworldimageryclarity"@en .

piirritev:OsmSourceEstimated a skos:Concept ;
    piirrite:osmId "estimated" ;
    rdfs:subClassOf piirrite:OsmEntity ;
    skos:definition ""@en ;
    skos:inScheme piirritev:OsmSource ;
    skos:prefLabel "Estimated"@en .

piirritev:OsmSourceEthekwiniMetro a skos:Concept ;
    piirrite:osmId "eThekwini_Metro" ;
    rdfs:subClassOf piirrite:OsmEntity ;
    skos:definition ""@en ;
    skos:inScheme piirritev:OsmSource ;
    skos:prefLabel "Ethekwini metro"@en .

piirritev:OsmSourceExtrapolation a skos:Concept ;
    piirrite:osmId "extrapolation" ;
    rdfs:subClassOf piirrite:OsmEntity ;
    skos:definition ""@en ;
    skos:inScheme piirritev:OsmSource ;
    skos:prefLabel "Extrapolation"@en .

piirritev:OsmSourceFadatc9 a skos:Concept ;
    piirrite:osmId "FADAtc9" ;
    rdfs:subClassOf piirrite:OsmEntity ;
    skos:definition ""@en ;
    skos:inScheme piirritev:OsmSource ;
    skos:prefLabel "Fadatc9"@en .

piirritev:OsmSourceFieldSurvey a skos:Concept ;
    piirrite:osmId "Field_survey",
        "field_survey" ;
    rdfs:subClassOf piirrite:OsmEntity ;
    skos:definition ""@en ;
    skos:inScheme piirritev:OsmSource ;
    skos:prefLabel "Field survey"@en .

piirritev:OsmSourceFirstlook a skos:Concept ;
    piirrite:osmId "FirstLook" ;
    rdfs:subClassOf piirrite:OsmEntity ;
    skos:definition ""@en ;
    skos:inScheme piirritev:OsmSource ;
    skos:prefLabel "Firstlook"@en .

piirritev:OsmSourceFotogrametria a skos:Concept ;
    piirrite:osmId "Fotogrametria" ;
    rdfs:subClassOf piirrite:OsmEntity ;
    skos:definition ""@en ;
    skos:inScheme piirritev:OsmSource ;
    skos:prefLabel "Fotogrametria"@en .

piirritev:OsmSourceFrIgnBdortho a skos:Concept ;
    piirrite:osmId "fr_ign_bdortho" ;
    rdfs:subClassOf piirrite:OsmEntity ;
    skos:definition ""@en ;
    skos:inScheme piirritev:OsmSource ;
    skos:prefLabel "Fr ign bdortho"@en .

piirritev:OsmSourceFreshwaterAtlas a skos:Concept ;
    piirrite:osmId "Freshwater_Atlas" ;
    rdfs:subClassOf piirrite:OsmEntity ;
    skos:definition ""@en ;
    skos:inScheme piirritev:OsmSource ;
    skos:prefLabel "Freshwater atlas"@en .

piirritev:OsmSourceGdiSw a skos:Concept ;
    piirrite:osmId "GDI_SW" ;
    rdfs:subClassOf piirrite:OsmEntity ;
    skos:definition ""@en ;
    skos:inScheme piirritev:OsmSource ;
    skos:prefLabel "Gdi sw"@en .

piirritev:OsmSourceGeobase a skos:Concept ;
    piirrite:osmId "GeoBase" ;
    rdfs:subClassOf piirrite:OsmEntity ;
    skos:definition ""@en ;
    skos:inScheme piirritev:OsmSource ;
    skos:prefLabel "Geobase"@en .

piirritev:OsmSourceGeobaseNrn a skos:Concept ;
    piirrite:osmId "GeoBase_NRN" ;
    rdfs:subClassOf piirrite:OsmEntity ;
    skos:definition ""@en ;
    skos:inScheme piirritev:OsmSource ;
    skos:prefLabel "Geobase nrn"@en .

piirritev:OsmSourceGeobases2015 a skos:Concept ;
    piirrite:osmId "GEOBASES_2015" ;
    rdfs:subClassOf piirrite:OsmEntity ;
    skos:definition ""@en ;
    skos:inScheme piirritev:OsmSource ;
    skos:prefLabel "Geobases 2015"@en .

piirritev:OsmSourceGeocameroun a skos:Concept ;
    piirrite:osmId "Geocameroun" ;
    rdfs:subClassOf piirrite:OsmEntity ;
    skos:definition ""@en ;
    skos:inScheme piirritev:OsmSource ;
    skos:prefLabel "Geocameroun"@en .

piirritev:OsmSourceGeodataGovGr a skos:Concept ;
    piirrite:osmId "geodata_gov_gr" ;
    rdfs:subClassOf piirrite:OsmEntity ;
    skos:definition ""@en ;
    skos:inScheme piirritev:OsmSource ;
    skos:prefLabel "Geodata gov gr"@en .

piirritev:OsmSourceGeodatabase a skos:Concept ;
    piirrite:osmId "GeoDatabase" ;
    rdfs:subClassOf piirrite:OsmEntity ;
    skos:definition ""@en ;
    skos:inScheme piirritev:OsmSource ;
    skos:prefLabel "Geodatabase"@en .

piirritev:OsmSourceGeodatastyrelsen a skos:Concept ;
    piirrite:osmId "Geodatastyrelsen",
        "geodatastyrelsen" ;
    rdfs:subClassOf piirrite:OsmEntity ;
    skos:definition ""@en ;
    skos:inScheme piirritev:OsmSource ;
    skos:prefLabel "Geodatastyrelsen"@en .

piirritev:OsmSourceGeoeuskadi a skos:Concept ;
    piirrite:osmId "GeoEuskadi" ;
    rdfs:subClassOf piirrite:OsmEntity ;
    skos:definition ""@en ;
    skos:inScheme piirritev:OsmSource ;
    skos:prefLabel "Geoeuskadi"@en .

piirritev:OsmSourceGeoeye a skos:Concept ;
    piirrite:osmId "GeoEye" ;
    rdfs:subClassOf piirrite:OsmEntity ;
    skos:definition ""@en ;
    skos:inScheme piirritev:OsmSource ;
    skos:prefLabel "Geoeye"@en .

piirritev:OsmSourceGeoimageAt a skos:Concept ;
    piirrite:osmId "GeoImage_at",
        "Geoimage_at",
        "geoimage_at" ;
    rdfs:subClassOf piirrite:OsmEntity ;
    skos:definition ""@en ;
    skos:inScheme piirritev:OsmSource ;
    skos:prefLabel "Geoimage at"@en .

piirritev:OsmSourceGeoimageAtHigh-Res a skos:Concept ;
    piirrite:osmId "GeoImage_at_High-Res" ;
    rdfs:subClassOf piirrite:OsmEntity ;
    skos:definition ""@en ;
    skos:inScheme piirritev:OsmSource ;
    skos:prefLabel "Geoimage at high-res"@en .

piirritev:OsmSourceGeoimageAtHires a skos:Concept ;
    piirrite:osmId "geoimage_at_hires" ;
    rdfs:subClassOf piirrite:OsmEntity ;
    skos:definition ""@en ;
    skos:inScheme piirritev:OsmSource ;
    skos:prefLabel "Geoimage at hires"@en .

piirritev:OsmSourceGeoimageAtMaxres a skos:Concept ;
    piirrite:osmId "GeoImage_at_MaxRes",
        "Geoimage_at_MaxRes",
        "geoimage_at_MaxRes" ;
    rdfs:subClassOf piirrite:OsmEntity ;
    skos:definition ""@en ;
    skos:inScheme piirritev:OsmSource ;
    skos:prefLabel "Geoimage at maxres"@en .

piirritev:OsmSourceGeoportal a skos:Concept ;
    piirrite:osmId "Geoportal" ;
    rdfs:subClassOf piirrite:OsmEntity ;
    skos:definition ""@en ;
    skos:inScheme piirritev:OsmSource ;
    skos:prefLabel "Geoportal"@en .

piirritev:OsmSourceGeoportal2 a skos:Concept ;
    piirrite:osmId "geoportal2" ;
    rdfs:subClassOf piirrite:OsmEntity ;
    skos:definition ""@en ;
    skos:inScheme piirritev:OsmSource ;
    skos:prefLabel "Geoportal2"@en .

piirritev:OsmSourceGeoportalGovPl a skos:Concept ;
    piirrite:osmId "geoportal_gov_pl" ;
    rdfs:subClassOf piirrite:OsmEntity ;
    skos:definition ""@en ;
    skos:inScheme piirritev:OsmSource ;
    skos:prefLabel "Geoportal gov pl"@en .

piirritev:OsmSourceGeptis a skos:Concept ;
    piirrite:osmId "GEPTIS" ;
    rdfs:subClassOf piirrite:OsmEntity ;
    skos:definition ""@en ;
    skos:inScheme piirritev:OsmSource ;
    skos:prefLabel "Geptis"@en .

piirritev:OsmSourceGis a skos:Concept ;
    piirrite:osmId "GIS" ;
    rdfs:subClassOf piirrite:OsmEntity ;
    skos:definition ""@en ;
    skos:inScheme piirritev:OsmSource ;
    skos:prefLabel "Gis"@en .

piirritev:OsmSourceGisUmSzczecinPl a skos:Concept ;
    piirrite:osmId "gis_um_szczecin_pl" ;
    rdfs:subClassOf piirrite:OsmEntity ;
    skos:definition ""@en ;
    skos:inScheme piirritev:OsmSource ;
    skos:prefLabel "Gis um szczecin pl"@en .

piirritev:OsmSourceGns a skos:Concept ;
    piirrite:osmId "GNS" ;
    rdfs:subClassOf piirrite:OsmEntity ;
    skos:definition ""@en ;
    skos:inScheme piirritev:OsmSource ;
    skos:prefLabel "Gns"@en .

piirritev:OsmSourceGps a skos:Concept ;
    piirrite:osmId "GPS",
        "gps" ;
    rdfs:subClassOf piirrite:OsmEntity ;
    skos:definition ""@en ;
    skos:inScheme piirritev:OsmSource ;
    skos:prefLabel "Gps"@en .

piirritev:OsmSourceGpsSurvey a skos:Concept ;
    piirrite:osmId "GPS_Survey",
        "GPS_survey" ;
    rdfs:subClassOf piirrite:OsmEntity ;
    skos:definition ""@en ;
    skos:inScheme piirritev:OsmSource ;
    skos:prefLabel "Gps survey"@en .

piirritev:OsmSourceGpx a skos:Concept ;
    piirrite:osmId "gpx" ;
    rdfs:subClassOf piirrite:OsmEntity ;
    skos:definition ""@en ;
    skos:inScheme piirritev:OsmSource ;
    skos:prefLabel "Gpx"@en .

piirritev:OsmSourceGrandnancy a skos:Concept ;
    piirrite:osmId "GrandNancy" ;
    rdfs:subClassOf piirrite:OsmEntity ;
    skos:definition ""@en ;
    skos:inScheme piirritev:OsmSource ;
    skos:prefLabel "Grandnancy"@en .

piirritev:OsmSourceGrandtoulouse a skos:Concept ;
    piirrite:osmId "GrandToulouse" ;
    rdfs:subClassOf piirrite:OsmEntity ;
    skos:definition ""@en ;
    skos:inScheme piirritev:OsmSource ;
    skos:prefLabel "Grandtoulouse"@en .

piirritev:OsmSourceGrb a skos:Concept ;
    piirrite:osmId "GRB" ;
    rdfs:subClassOf piirrite:OsmEntity ;
    skos:definition ""@en ;
    skos:inScheme piirritev:OsmSource ;
    skos:prefLabel "Grb"@en .

piirritev:OsmSourceGsiOrtorectified a skos:Concept ;
    piirrite:osmId "GSI_ortorectified" ;
    rdfs:subClassOf piirrite:OsmEntity ;
    skos:definition ""@en ;
    skos:inScheme piirritev:OsmSource ;
    skos:prefLabel "Gsi ortorectified"@en .

piirritev:OsmSourceGurs a skos:Concept ;
    piirrite:osmId "GURS" ;
    rdfs:subClassOf piirrite:OsmEntity ;
    skos:definition "Data source is Geodetska uprava Republike Slovenije"@en ;
    skos:inScheme piirritev:OsmSource ;
    skos:prefLabel "Gurs"@en .

piirritev:OsmSourceGograndest a skos:Concept ;
    piirrite:osmId "GoGrandEst" ;
    rdfs:subClassOf piirrite:OsmEntity ;
    skos:definition ""@en ;
    skos:inScheme piirritev:OsmSource ;
    skos:prefLabel "Gograndest"@en .

piirritev:OsmSourceHearAed a skos:Concept ;
    piirrite:osmId "hear_aed" ;
    rdfs:subClassOf piirrite:OsmEntity ;
    skos:definition ""@en ;
    skos:inScheme piirritev:OsmSource ;
    skos:prefLabel "Hear aed"@en .

piirritev:OsmSourceHighwayBuffers a skos:Concept ;
    piirrite:osmId "highway_buffers" ;
    rdfs:subClassOf piirrite:OsmEntity ;
    skos:definition ""@en ;
    skos:inScheme piirritev:OsmSource ;
    skos:prefLabel "Highway buffers"@en .

piirritev:OsmSourceHistorical a skos:Concept ;
    piirrite:osmId "historical" ;
    rdfs:subClassOf piirrite:OsmEntity ;
    skos:definition ""@en ;
    skos:inScheme piirritev:OsmSource ;
    skos:prefLabel "Historical"@en .

piirritev:OsmSourceHot a skos:Concept ;
    piirrite:osmId "HOT" ;
    rdfs:subClassOf piirrite:OsmEntity ;
    skos:definition ""@en ;
    skos:inScheme piirritev:OsmSource ;
    skos:prefLabel "Hot"@en .

piirritev:OsmSourceHot-Uganda a skos:Concept ;
    piirrite:osmId "HOT-Uganda" ;
    rdfs:subClassOf piirrite:OsmEntity ;
    skos:definition ""@en ;
    skos:inScheme piirritev:OsmSource ;
    skos:prefLabel "Hot-uganda"@en .

piirritev:OsmSourceIbge a skos:Concept ;
    piirrite:osmId "IBGE" ;
    rdfs:subClassOf piirrite:OsmEntity ;
    skos:definition ""@en ;
    skos:inScheme piirritev:OsmSource ;
    skos:prefLabel "Ibge"@en .

piirritev:OsmSourceIdeandaluciaEs2008 a skos:Concept ;
    piirrite:osmId "ideandalucia_es_2008" ;
    rdfs:subClassOf piirrite:OsmEntity ;
    skos:definition ""@en ;
    skos:inScheme piirritev:OsmSource ;
    skos:prefLabel "Ideandalucia es 2008"@en .

piirritev:OsmSourceIdee a skos:Concept ;
    piirrite:osmId "IDEE" ;
    rdfs:subClassOf piirrite:OsmEntity ;
    skos:definition ""@en ;
    skos:inScheme piirritev:OsmSource ;
    skos:prefLabel "Idee"@en .

piirritev:OsmSourceIgvsb a skos:Concept ;
    piirrite:osmId "IGVSB" ;
    rdfs:subClassOf piirrite:OsmEntity ;
    skos:definition ""@en ;
    skos:inScheme piirritev:OsmSource ;
    skos:prefLabel "Igvsb"@en .

piirritev:OsmSourceImage a skos:Concept ;
    piirrite:osmId "image" ;
    rdfs:subClassOf piirrite:OsmEntity ;
    skos:definition ""@en ;
    skos:inScheme piirritev:OsmSource ;
    skos:prefLabel "Image"@en .

piirritev:OsmSourceIncog a skos:Concept ;
    piirrite:osmId "INCOG" ;
    rdfs:subClassOf piirrite:OsmEntity ;
    skos:definition ""@en ;
    skos:inScheme piirritev:OsmSource ;
    skos:prefLabel "Incog"@en .

piirritev:OsmSourceInegi a skos:Concept ;
    piirrite:osmId "INEGI" ;
    rdfs:subClassOf piirrite:OsmEntity ;
    skos:definition ""@en ;
    skos:inScheme piirritev:OsmSource ;
    skos:prefLabel "Inegi"@en .

piirritev:OsmSourceInterpolation a skos:Concept ;
    piirrite:osmId "interpolation" ;
    rdfs:subClassOf piirrite:OsmEntity ;
    skos:definition ""@en ;
    skos:inScheme piirritev:OsmSource ;
    skos:prefLabel "Interpolation"@en .

piirritev:OsmSourceIrs a skos:Concept ;
    piirrite:osmId "IRS",
        "irs" ;
    rdfs:subClassOf piirrite:OsmEntity ;
    skos:definition ""@en ;
    skos:inScheme piirritev:OsmSource ;
    skos:prefLabel "Irs"@en .

piirritev:OsmSourceItacyl a skos:Concept ;
    piirrite:osmId "ITACYL",
        "ITACyL" ;
    rdfs:subClassOf piirrite:OsmEntity ;
    skos:definition ""@en ;
    skos:inScheme piirritev:OsmSource ;
    skos:prefLabel "Itacyl"@en .

piirritev:OsmSourceJumpstartInternational a skos:Concept ;
    piirrite:osmId "JumpStart_International" ;
    rdfs:subClassOf piirrite:OsmEntity ;
    skos:definition ""@en ;
    skos:inScheme piirritev:OsmSource ;
    skos:prefLabel "Jumpstart international"@en .

piirritev:OsmSourceKapor2 a skos:Concept ;
    piirrite:osmId "kapor2" ;
    rdfs:subClassOf piirrite:OsmEntity ;
    skos:definition ""@en ;
    skos:inScheme piirritev:OsmSource ;
    skos:prefLabel "Kapor2"@en .

piirritev:OsmSourceKartverket a skos:Concept ;
    piirrite:osmId "Kartverket" ;
    rdfs:subClassOf piirrite:OsmEntity ;
    skos:definition ""@en ;
    skos:inScheme piirritev:OsmSource ;
    skos:prefLabel "Kartverket"@en .

piirritev:OsmSourceKartverketN50 a skos:Concept ;
    piirrite:osmId "Kartverket_N50" ;
    rdfs:subClassOf piirrite:OsmEntity ;
    skos:definition ""@en ;
    skos:inScheme piirritev:OsmSource ;
    skos:prefLabel "Kartverket n50"@en .

piirritev:OsmSourceKiban2500 a skos:Concept ;
    piirrite:osmId "KIBAN2500" ;
    rdfs:subClassOf piirrite:OsmEntity ;
    skos:definition ""@en ;
    skos:inScheme piirritev:OsmSource ;
    skos:prefLabel "Kiban2500"@en .

piirritev:OsmSourceKoldingKommune a skos:Concept ;
    piirrite:osmId "Kolding_Kommune" ;
    rdfs:subClassOf piirrite:OsmEntity ;
    skos:definition ""@en ;
    skos:inScheme piirritev:OsmSource ;
    skos:prefLabel "Kolding kommune"@en .

piirritev:OsmSourceKrtTilburg a skos:Concept ;
    piirrite:osmId "KRT_Tilburg" ;
    rdfs:subClassOf piirrite:OsmEntity ;
    skos:definition ""@en ;
    skos:inScheme piirritev:OsmSource ;
    skos:prefLabel "Krt tilburg"@en .

piirritev:OsmSourceKsj2 a skos:Concept ;
    piirrite:osmId "KSJ2" ;
    rdfs:subClassOf piirrite:OsmEntity ;
    skos:definition ""@en ;
    skos:inScheme piirritev:OsmSource ;
    skos:prefLabel "Ksj2"@en .

piirritev:OsmSourceKvlHro a skos:Concept ;
    piirrite:osmId "KVL_HRO" ;
    rdfs:subClassOf piirrite:OsmEntity ;
    skos:definition ""@en ;
    skos:inScheme piirritev:OsmSource ;
    skos:prefLabel "Kvl hro"@en .

piirritev:OsmSourceLa-Ka a skos:Concept ;
    piirrite:osmId "LA-KA" ;
    rdfs:subClassOf piirrite:OsmEntity ;
    skos:definition ""@en ;
    skos:inScheme piirritev:OsmSource ;
    skos:prefLabel "La-ka"@en .

piirritev:OsmSourceLahtiAerial a skos:Concept ;
    piirrite:osmId "Lahti_aerial" ;
    rdfs:subClassOf piirrite:OsmEntity ;
    skos:definition ""@en ;
    skos:inScheme piirritev:OsmSource ;
    skos:prefLabel "Lahti aerial"@en .

piirritev:OsmSourceLandpro08 a skos:Concept ;
    piirrite:osmId "LandPro08" ;
    rdfs:subClassOf piirrite:OsmEntity ;
    skos:definition ""@en ;
    skos:inScheme piirritev:OsmSource ;
    skos:prefLabel "Landpro08"@en .

piirritev:OsmSourceLandsat a skos:Concept ;
    piirrite:osmId "Landsat",
        "landsat" ;
    rdfs:subClassOf piirrite:OsmEntity ;
    skos:definition ""@en ;
    skos:inScheme piirritev:OsmSource ;
    skos:prefLabel "Landsat"@en .

piirritev:OsmSourceLandsatImagery a skos:Concept ;
    piirrite:osmId "Landsat_imagery" ;
    rdfs:subClassOf piirrite:OsmEntity ;
    skos:definition ""@en ;
    skos:inScheme piirritev:OsmSource ;
    skos:prefLabel "Landsat imagery"@en .

piirritev:OsmSourceLantmteriet a skos:Concept ;
    piirrite:osmId "Lantmteriet" ;
    rdfs:subClassOf piirrite:OsmEntity ;
    skos:definition ""@en ;
    skos:inScheme piirritev:OsmSource ;
    skos:prefLabel "Lantmteriet"@en .

piirritev:OsmSourceLasyPastwowe a skos:Concept ;
    piirrite:osmId "Lasy_Pastwowe" ;
    rdfs:subClassOf piirrite:OsmEntity ;
    skos:definition ""@en ;
    skos:inScheme piirritev:OsmSource ;
    skos:prefLabel "Lasy pastwowe"@en .

piirritev:OsmSourceLinz a skos:Concept ;
    piirrite:osmId "LINZ" ;
    rdfs:subClassOf piirrite:OsmEntity ;
    skos:definition ""@en ;
    skos:inScheme piirritev:OsmSource ;
    skos:prefLabel "Linz"@en .

piirritev:OsmSourceLocale a skos:Concept ;
    piirrite:osmId "locale" ;
    rdfs:subClassOf piirrite:OsmEntity ;
    skos:definition ""@en ;
    skos:inScheme piirritev:OsmSource ;
    skos:prefLabel "Locale"@en .

piirritev:OsmSourceLommaKommun a skos:Concept ;
    piirrite:osmId "Lomma_kommun" ;
    rdfs:subClassOf piirrite:OsmEntity ;
    skos:definition ""@en ;
    skos:inScheme piirritev:OsmSource ;
    skos:prefLabel "Lomma kommun"@en .

piirritev:OsmSourceLpis a skos:Concept ;
    piirrite:osmId "lpis" ;
    rdfs:subClassOf piirrite:OsmEntity ;
    skos:definition ""@en ;
    skos:inScheme piirritev:OsmSource ;
    skos:prefLabel "Lpis"@en .

piirritev:OsmSourceLsib3 a skos:Concept ;
    piirrite:osmId "LSIB3" ;
    rdfs:subClassOf piirrite:OsmEntity ;
    skos:definition ""@en ;
    skos:inScheme piirritev:OsmSource ;
    skos:prefLabel "Lsib3"@en .

piirritev:OsmSourceLspp a skos:Concept ;
    piirrite:osmId "LSPP" ;
    rdfs:subClassOf piirrite:OsmEntity ;
    skos:definition ""@en ;
    skos:inScheme piirritev:OsmSource ;
    skos:prefLabel "Lspp"@en .

piirritev:OsmSourceM-Ncppc a skos:Concept ;
    piirrite:osmId "M-NCPPC" ;
    rdfs:subClassOf piirrite:OsmEntity ;
    skos:definition ""@en ;
    skos:inScheme piirritev:OsmSource ;
    skos:prefLabel "M-ncppc"@en .

piirritev:OsmSourceMaa-Amet01062009 a skos:Concept ;
    piirrite:osmId "Maa-amet_01_06_2009" ;
    rdfs:subClassOf piirrite:OsmEntity ;
    skos:definition ""@en ;
    skos:inScheme piirritev:OsmSource ;
    skos:prefLabel "Maa-amet 01 06 2009"@en .

piirritev:OsmSourceMaa-Amet2013 a skos:Concept ;
    piirrite:osmId "Maa-amet_2013" ;
    rdfs:subClassOf piirrite:OsmEntity ;
    skos:definition ""@en ;
    skos:inScheme piirritev:OsmSource ;
    skos:prefLabel "Maa-amet 2013"@en .

piirritev:OsmSourceMaa-Amet2019 a skos:Concept ;
    piirrite:osmId "Maa-amet_2019" ;
    rdfs:subClassOf piirrite:OsmEntity ;
    skos:definition ""@en ;
    skos:inScheme piirritev:OsmSource ;
    skos:prefLabel "Maa-amet 2019"@en .

piirritev:OsmSourceMaa-Amet2023 a skos:Concept ;
    piirrite:osmId "Maa-amet_2023" ;
    rdfs:subClassOf piirrite:OsmEntity ;
    skos:definition ""@en ;
    skos:inScheme piirritev:OsmSource ;
    skos:prefLabel "Maa-amet 2023"@en .

piirritev:OsmSourceMaa-Amet2024 a skos:Concept ;
    piirrite:osmId "Maa-amet_2024" ;
    rdfs:subClassOf piirrite:OsmEntity ;
    skos:definition ""@en ;
    skos:inScheme piirritev:OsmSource ;
    skos:prefLabel "Maa-amet 2024"@en .

piirritev:OsmSourceMapaLodzPl a skos:Concept ;
    piirrite:osmId "mapa_lodz_pl" ;
    rdfs:subClassOf piirrite:OsmEntity ;
    skos:definition ""@en ;
    skos:inScheme piirritev:OsmSource ;
    skos:prefLabel "Mapa lodz pl"@en .

piirritev:OsmSourceMapbox a skos:Concept ;
    piirrite:osmId "MapBox",
        "Mapbox",
        "mapbox" ;
    rdfs:subClassOf piirrite:OsmEntity ;
    skos:definition ""@en ;
    skos:inScheme piirritev:OsmSource ;
    skos:prefLabel "Mapbox"@en .

piirritev:OsmSourceMapboxSatellite a skos:Concept ;
    piirrite:osmId "MapBox_Satellite",
        "Mapbox_Satellite",
        "Mapbox_satellite" ;
    rdfs:subClassOf piirrite:OsmEntity ;
    skos:definition ""@en ;
    skos:inScheme piirritev:OsmSource ;
    skos:prefLabel "Mapbox satellite"@en .

piirritev:OsmSourceMapillary a skos:Concept ;
    piirrite:hasRelatedOsmTag piirrite:hasOsmMapillaryType ;
    piirrite:osmId "Mapillary",
        "mapillary" ;
    rdfs:subClassOf piirrite:OsmEntity ;
    skos:definition "source of the object come from Mapillary"@en ;
    skos:inScheme piirritev:OsmSource ;
    skos:prefLabel "Mapillary"@en .

piirritev:OsmSourceMaps4Bw a skos:Concept ;
    piirrite:osmId "Maps4BW" ;
    rdfs:subClassOf piirrite:OsmEntity ;
    skos:definition ""@en ;
    skos:inScheme piirritev:OsmSource ;
    skos:prefLabel "Maps4bw"@en .

piirritev:OsmSourceMapwithai a skos:Concept ;
    piirrite:osmId "MapWithAI" ;
    rdfs:subClassOf piirrite:OsmEntity ;
    skos:definition ""@en ;
    skos:inScheme piirritev:OsmSource ;
    skos:prefLabel "Mapwithai"@en .

piirritev:OsmSourceMaxar a skos:Concept ;
    piirrite:osmId "Maxar",
        "maxar" ;
    rdfs:subClassOf piirrite:OsmEntity ;
    skos:definition ""@en ;
    skos:inScheme piirritev:OsmSource ;
    skos:prefLabel "Maxar"@en .

piirritev:OsmSourceMaxar-Premium a skos:Concept ;
    piirrite:osmId "Maxar-Premium" ;
    rdfs:subClassOf piirrite:OsmEntity ;
    skos:definition ""@en ;
    skos:inScheme piirritev:OsmSource ;
    skos:prefLabel "Maxar-premium"@en .

piirritev:OsmSourceMaxarPremium a skos:Concept ;
    piirrite:osmId "Maxar_Premium",
        "maxar_Premium" ;
    rdfs:subClassOf piirrite:OsmEntity ;
    skos:definition ""@en ;
    skos:inScheme piirritev:OsmSource ;
    skos:prefLabel "Maxar premium"@en .

piirritev:OsmSourceMaxarPremium-Luftbilder a skos:Concept ;
    piirrite:osmId "Maxar_Premium-Luftbilder" ;
    rdfs:subClassOf piirrite:OsmEntity ;
    skos:definition ""@en ;
    skos:inScheme piirritev:OsmSource ;
    skos:prefLabel "Maxar premium-luftbilder"@en .

piirritev:OsmSourceMaxarpremium a skos:Concept ;
    piirrite:osmId "MaxarPremium" ;
    rdfs:subClassOf piirrite:OsmEntity ;
    skos:definition ""@en ;
    skos:inScheme piirritev:OsmSource ;
    skos:prefLabel "Maxarpremium"@en .

piirritev:OsmSourceMdutUpc a skos:Concept ;
    piirrite:osmId "mdut_upc" ;
    rdfs:subClassOf piirrite:OsmEntity ;
    skos:definition ""@en ;
    skos:inScheme piirritev:OsmSource ;
    skos:prefLabel "Mdut upc"@en .

piirritev:OsmSourceMgc a skos:Concept ;
    piirrite:osmId "MGC" ;
    rdfs:subClassOf piirrite:OsmEntity ;
    skos:definition ""@en ;
    skos:inScheme piirritev:OsmSource ;
    skos:prefLabel "Mgc"@en .

piirritev:OsmSourceMicrosoftImport a skos:Concept ;
    piirrite:osmId "Microsoft_Import" ;
    rdfs:subClassOf piirrite:OsmEntity ;
    skos:definition ""@en ;
    skos:inScheme piirritev:OsmSource ;
    skos:prefLabel "Microsoft import"@en .

piirritev:OsmSourceMineduGobPe a skos:Concept ;
    piirrite:osmId "minedu_gob_pe" ;
    rdfs:subClassOf piirrite:OsmEntity ;
    skos:definition ""@en ;
    skos:inScheme piirritev:OsmSource ;
    skos:prefLabel "Minedu gob pe"@en .

piirritev:OsmSourceMml a skos:Concept ;
    piirrite:osmId "MML",
        "mml" ;
    rdfs:subClassOf piirrite:OsmEntity ;
    skos:definition ""@en ;
    skos:inScheme piirritev:OsmSource ;
    skos:prefLabel "Mml"@en .

piirritev:OsmSourceMml2012 a skos:Concept ;
    piirrite:osmId "MML_2012" ;
    rdfs:subClassOf piirrite:OsmEntity ;
    skos:definition ""@en ;
    skos:inScheme piirritev:OsmSource ;
    skos:prefLabel "Mml 2012"@en .

piirritev:OsmSourceMml2017 a skos:Concept ;
    piirrite:osmId "MML2017" ;
    rdfs:subClassOf piirrite:OsmEntity ;
    skos:definition ""@en ;
    skos:inScheme piirritev:OsmSource ;
    skos:prefLabel "Mml2017"@en .

piirritev:OsmSourceMmlOrthofoto a skos:Concept ;
    piirrite:osmId "MML_Orthofoto" ;
    rdfs:subClassOf piirrite:OsmEntity ;
    skos:definition ""@en ;
    skos:inScheme piirritev:OsmSource ;
    skos:prefLabel "Mml orthofoto"@en .

piirritev:OsmSourceMmlOrto a skos:Concept ;
    piirrite:osmId "MML_orto" ;
    rdfs:subClassOf piirrite:OsmEntity ;
    skos:definition ""@en ;
    skos:inScheme piirritev:OsmSource ;
    skos:prefLabel "Mml orto"@en .

piirritev:OsmSourceMoa a skos:Concept ;
    piirrite:osmId "MOA" ;
    rdfs:subClassOf piirrite:OsmEntity ;
    skos:definition ""@en ;
    skos:inScheme piirritev:OsmSource ;
    skos:prefLabel "Moa"@en .

piirritev:OsmSourceMsFootprts a skos:Concept ;
    piirrite:osmId "MS_Footprts" ;
    rdfs:subClassOf piirrite:OsmEntity ;
    skos:definition ""@en ;
    skos:inScheme piirritev:OsmSource ;
    skos:prefLabel "Ms footprts"@en .

piirritev:OsmSourceN50Map a skos:Concept ;
    piirrite:osmId "N50map" ;
    rdfs:subClassOf piirrite:OsmEntity ;
    skos:definition ""@en ;
    skos:inScheme piirritev:OsmSource ;
    skos:prefLabel "N50map"@en .

piirritev:OsmSourceNaip a skos:Concept ;
    piirrite:osmId "NAIP" ;
    rdfs:subClassOf piirrite:OsmEntity ;
    skos:definition "National Agriculture Imagery Program: aerial imagery acquired by the US Department of Agriculture"@en ;
    skos:inScheme piirritev:OsmSource ;
    skos:prefLabel "Naip"@en .

piirritev:OsmSourceNaptanImport a skos:Concept ;
    piirrite:osmId "naptan_import" ;
    rdfs:subClassOf piirrite:OsmEntity ;
    skos:definition ""@en ;
    skos:inScheme piirritev:OsmSource ;
    skos:prefLabel "Naptan import"@en .

piirritev:OsmSourceNearmap a skos:Concept ;
    piirrite:osmId "nearmap" ;
    rdfs:subClassOf piirrite:OsmEntity ;
    skos:definition ""@en ;
    skos:inScheme piirritev:OsmSource ;
    skos:prefLabel "Nearmap"@en .

piirritev:OsmSourceNextview a skos:Concept ;
    piirrite:osmId "NextView",
        "Nextview" ;
    rdfs:subClassOf piirrite:OsmEntity ;
    skos:definition ""@en ;
    skos:inScheme piirritev:OsmSource ;
    skos:prefLabel "Nextview"@en .

piirritev:OsmSourceNga-Gns a skos:Concept ;
    piirrite:osmId "NGA-GNS" ;
    rdfs:subClassOf piirrite:OsmEntity ;
    skos:definition ""@en ;
    skos:inScheme piirritev:OsmSource ;
    skos:prefLabel "Nga-gns"@en .

piirritev:OsmSourceNgaGns a skos:Concept ;
    piirrite:osmId "NGA_GNS" ;
    rdfs:subClassOf piirrite:OsmEntity ;
    skos:definition ""@en ;
    skos:inScheme piirritev:OsmSource ;
    skos:prefLabel "Nga gns"@en .

piirritev:OsmSourceNgi a skos:Concept ;
    piirrite:osmId "ngi" ;
    rdfs:subClassOf piirrite:OsmEntity ;
    skos:definition ""@en ;
    skos:inScheme piirritev:OsmSource ;
    skos:prefLabel "Ngi"@en .

piirritev:OsmSourceNgi-Riverimport a skos:Concept ;
    piirrite:osmId "NGI-RiverImport" ;
    rdfs:subClassOf piirrite:OsmEntity ;
    skos:definition ""@en ;
    skos:inScheme piirritev:OsmSource ;
    skos:prefLabel "Ngi-riverimport"@en .

piirritev:OsmSourceNhGranit a skos:Concept ;
    piirrite:osmId "NH_GRANIT" ;
    rdfs:subClassOf piirrite:OsmEntity ;
    skos:definition ""@en ;
    skos:inScheme piirritev:OsmSource ;
    skos:prefLabel "Nh granit"@en .

piirritev:OsmSourceNhd a skos:Concept ;
    piirrite:osmId "NHD" ;
    rdfs:subClassOf piirrite:OsmEntity ;
    skos:definition ""@en ;
    skos:inScheme piirritev:OsmSource ;
    skos:prefLabel "Nhd"@en .

piirritev:OsmSourceNhdFlowlines a skos:Concept ;
    piirrite:osmId "NHD_flowlines" ;
    rdfs:subClassOf piirrite:OsmEntity ;
    skos:definition ""@en ;
    skos:inScheme piirritev:OsmSource ;
    skos:prefLabel "Nhd flowlines"@en .

piirritev:OsmSourceNhdWaterbodies a skos:Concept ;
    piirrite:osmId "NHD_waterbodies" ;
    rdfs:subClassOf piirrite:OsmEntity ;
    skos:definition ""@en ;
    skos:inScheme piirritev:OsmSource ;
    skos:prefLabel "Nhd waterbodies"@en .

piirritev:OsmSourceNigeriase4AllGovNg a skos:Concept ;
    piirrite:osmId "nigeriase4all_gov_ng" ;
    rdfs:subClassOf piirrite:OsmEntity ;
    skos:definition ""@en ;
    skos:inScheme piirritev:OsmSource ;
    skos:prefLabel "Nigeriase4all gov ng"@en .

piirritev:OsmSourceNj2002Lulc a skos:Concept ;
    piirrite:osmId "NJ2002LULC" ;
    rdfs:subClassOf piirrite:OsmEntity ;
    skos:definition ""@en ;
    skos:inScheme piirritev:OsmSource ;
    skos:prefLabel "Nj2002lulc"@en .

piirritev:OsmSourceNlc a skos:Concept ;
    piirrite:osmId "nlc" ;
    rdfs:subClassOf piirrite:OsmEntity ;
    skos:definition ""@en ;
    skos:inScheme piirritev:OsmSource ;
    skos:prefLabel "Nlc"@en .

piirritev:OsmSourceNlroads a skos:Concept ;
    piirrite:osmId "NLRoads" ;
    rdfs:subClassOf piirrite:OsmEntity ;
    skos:definition ""@en ;
    skos:inScheme piirritev:OsmSource ;
    skos:prefLabel "Nlroads"@en .

piirritev:OsmSourceNlsFiDatabase a skos:Concept ;
    piirrite:osmId "nls_fi_database" ;
    rdfs:subClassOf piirrite:OsmEntity ;
    skos:definition ""@en ;
    skos:inScheme piirritev:OsmSource ;
    skos:prefLabel "Nls fi database"@en .

piirritev:OsmSourceNlsc a skos:Concept ;
    piirrite:osmId "NLSC" ;
    rdfs:subClassOf piirrite:OsmEntity ;
    skos:definition ""@en ;
    skos:inScheme piirritev:OsmSource ;
    skos:prefLabel "Nlsc"@en .

piirritev:OsmSourceNpe a skos:Concept ;
    piirrite:osmId "NPE",
        "npe" ;
    rdfs:subClassOf piirrite:OsmEntity ;
    skos:definition ""@en ;
    skos:inScheme piirritev:OsmSource ;
    skos:prefLabel "Npe"@en .

piirritev:OsmSourceNrcan-Canvec-100 a skos:Concept ;
    piirrite:osmId "NRCan-CanVec-10_0" ;
    rdfs:subClassOf piirrite:OsmEntity ;
    skos:definition ""@en ;
    skos:inScheme piirritev:OsmSource ;
    skos:prefLabel "Nrcan-canvec-10 0"@en .

piirritev:OsmSourceNrcan-Canvec-70 a skos:Concept ;
    piirrite:osmId "NRCan-CanVec-7_0" ;
    rdfs:subClassOf piirrite:OsmEntity ;
    skos:definition ""@en ;
    skos:inScheme piirritev:OsmSource ;
    skos:prefLabel "Nrcan-canvec-7 0"@en .

piirritev:OsmSourceNrcan-Canvec-80 a skos:Concept ;
    piirrite:osmId "NRCan-CanVec-8_0" ;
    rdfs:subClassOf piirrite:OsmEntity ;
    skos:definition ""@en ;
    skos:inScheme piirritev:OsmSource ;
    skos:prefLabel "Nrcan-canvec-8 0"@en .

piirritev:OsmSourceNrngeobasev20 a skos:Concept ;
    piirrite:osmId "NRNGeobaseV2_0" ;
    rdfs:subClassOf piirrite:OsmEntity ;
    skos:definition ""@en ;
    skos:inScheme piirritev:OsmSource ;
    skos:prefLabel "Nrngeobasev2 0"@en .

piirritev:OsmSourceNrw-Atlas a skos:Concept ;
    piirrite:osmId "NRW-Atlas" ;
    rdfs:subClassOf piirrite:OsmEntity ;
    skos:definition ""@en ;
    skos:inScheme piirritev:OsmSource ;
    skos:prefLabel "Nrw-atlas"@en .

piirritev:OsmSourceNrw-Atlas\(Alk\) a skos:Concept ;
    piirrite:osmId "NRW-Atlas_(ALK)" ;
    rdfs:subClassOf piirrite:OsmEntity ;
    skos:definition ""@en ;
    skos:inScheme piirritev:OsmSource ;
    skos:prefLabel "Nrw-atlas (alk)"@en .

piirritev:OsmSourceNrwAtlas a skos:Concept ;
    piirrite:osmId "NRW_Atlas" ;
    rdfs:subClassOf piirrite:OsmEntity ;
    skos:definition ""@en ;
    skos:inScheme piirritev:OsmSource ;
    skos:prefLabel "Nrw atlas"@en .

piirritev:OsmSourceNvNmd2018 a skos:Concept ;
    piirrite:osmId "NV_NMD2018" ;
    rdfs:subClassOf piirrite:OsmEntity ;
    skos:definition ""@en ;
    skos:inScheme piirritev:OsmSource ;
    skos:prefLabel "Nv nmd2018"@en .

piirritev:OsmSourceNysGis a skos:Concept ;
    piirrite:osmId "NYS_GIS" ;
    rdfs:subClassOf piirrite:OsmEntity ;
    skos:definition ""@en ;
    skos:inScheme piirritev:OsmSource ;
    skos:prefLabel "Nys gis"@en .

piirritev:OsmSourceOaklandCounty a skos:Concept ;
    piirrite:osmId "Oakland_County" ;
    rdfs:subClassOf piirrite:OsmEntity ;
    skos:definition ""@en ;
    skos:inScheme piirritev:OsmSource ;
    skos:prefLabel "Oakland county"@en .

piirritev:OsmSourceOffenedatenMoersDe a skos:Concept ;
    piirrite:osmId "offenedaten_moers_de" ;
    rdfs:subClassOf piirrite:OsmEntity ;
    skos:definition ""@en ;
    skos:inScheme piirritev:OsmSource ;
    skos:prefLabel "Offenedaten moers de"@en .

piirritev:OsmSourceOgdVienna a skos:Concept ;
    piirrite:osmId "OGD_Vienna" ;
    rdfs:subClassOf piirrite:OsmEntity ;
    skos:definition ""@en ;
    skos:inScheme piirritev:OsmSource ;
    skos:prefLabel "Ogd vienna"@en .

piirritev:OsmSourceOpenData a skos:Concept ;
    piirrite:osmId "open_data" ;
    rdfs:subClassOf piirrite:OsmEntity ;
    skos:definition ""@en ;
    skos:inScheme piirritev:OsmSource ;
    skos:prefLabel "Open data"@en .

piirritev:OsmSourceOpenaerialmap a skos:Concept ;
    piirrite:osmId "OpenAerialMap" ;
    rdfs:subClassOf piirrite:OsmEntity ;
    skos:definition ""@en ;
    skos:inScheme piirritev:OsmSource ;
    skos:prefLabel "Openaerialmap"@en .

piirritev:OsmSourceOpendataHro a skos:Concept ;
    piirrite:osmId "OpenData_HRO" ;
    rdfs:subClassOf piirrite:OsmEntity ;
    skos:definition ""@en ;
    skos:inScheme piirritev:OsmSource ;
    skos:prefLabel "Opendata hro"@en .

piirritev:OsmSourceOpendataParisFr a skos:Concept ;
    piirrite:osmId "opendata_paris_fr" ;
    rdfs:subClassOf piirrite:OsmEntity ;
    skos:definition ""@en ;
    skos:inScheme piirritev:OsmSource ;
    skos:prefLabel "Opendata paris fr"@en .

piirritev:OsmSourceOpendatatelangana a skos:Concept ;
    piirrite:osmId "OpenDataTelangana" ;
    rdfs:subClassOf piirrite:OsmEntity ;
    skos:definition ""@en ;
    skos:inScheme piirritev:OsmSource ;
    skos:prefLabel "Opendatatelangana"@en .

piirritev:OsmSourceOpengovernmentdata a skos:Concept ;
    piirrite:osmId "OpenGovernmentData" ;
    rdfs:subClassOf piirrite:OsmEntity ;
    skos:definition ""@en ;
    skos:inScheme piirritev:OsmSource ;
    skos:prefLabel "Opengovernmentdata"@en .

piirritev:OsmSourceOpentopomap a skos:Concept ;
    piirrite:osmId "OpenTopoMap" ;
    rdfs:subClassOf piirrite:OsmEntity ;
    skos:definition ""@en ;
    skos:inScheme piirritev:OsmSource ;
    skos:prefLabel "Opentopomap"@en .

piirritev:OsmSourceOrt10Lt a skos:Concept ;
    piirrite:osmId "ORT10LT" ;
    rdfs:subClassOf piirrite:OsmEntity ;
    skos:definition ""@en ;
    skos:inScheme piirritev:OsmSource ;
    skos:prefLabel "Ort10lt"@en .

piirritev:OsmSourceOrthoHr a skos:Concept ;
    piirrite:osmId "Ortho_HR" ;
    rdfs:subClassOf piirrite:OsmEntity ;
    skos:definition ""@en ;
    skos:inScheme piirritev:OsmSource ;
    skos:prefLabel "Ortho hr"@en .

piirritev:OsmSourceOrthophotos2006Sitn50Cm a skos:Concept ;
    piirrite:osmId "Orthophotos2006sitn50cm" ;
    rdfs:subClassOf piirrite:OsmEntity ;
    skos:definition ""@en ;
    skos:inScheme piirritev:OsmSource ;
    skos:prefLabel "Orthophotos2006sitn50cm"@en .

piirritev:OsmSourceOrto a skos:Concept ;
    piirrite:osmId "orto" ;
    rdfs:subClassOf piirrite:OsmEntity ;
    skos:definition ""@en ;
    skos:inScheme piirritev:OsmSource ;
    skos:prefLabel "Orto"@en .

piirritev:OsmSourceOrtofotomozaikaSr a skos:Concept ;
    piirrite:osmId "Ortofotomozaika_SR" ;
    rdfs:subClassOf piirrite:OsmEntity ;
    skos:definition ""@en ;
    skos:inScheme piirritev:OsmSource ;
    skos:prefLabel "Ortofotomozaika sr"@en .

piirritev:OsmSourceOs-OpendataStreetview a skos:Concept ;
    piirrite:osmId "OS-OpenData_StreetView" ;
    rdfs:subClassOf piirrite:OsmEntity ;
    skos:definition ""@en ;
    skos:inScheme piirritev:OsmSource ;
    skos:prefLabel "Os-opendata streetview"@en .

piirritev:OsmSourceOs7 a skos:Concept ;
    piirrite:osmId "OS7" ;
    rdfs:subClassOf piirrite:OsmEntity ;
    skos:definition ""@en ;
    skos:inScheme piirritev:OsmSource ;
    skos:prefLabel "Os7"@en .

piirritev:OsmSourceOsVectormap a skos:Concept ;
    piirrite:osmId "OS_Vectormap" ;
    rdfs:subClassOf piirrite:OsmEntity ;
    skos:definition ""@en ;
    skos:inScheme piirritev:OsmSource ;
    skos:prefLabel "Os vectormap"@en .

piirritev:OsmSourceOsm-Gpx a skos:Concept ;
    piirrite:osmId "osm-gpx" ;
    rdfs:subClassOf piirrite:OsmEntity ;
    skos:definition ""@en ;
    skos:inScheme piirritev:OsmSource ;
    skos:prefLabel "Osm-gpx"@en .

piirritev:OsmSourceOurairportsCom a skos:Concept ;
    piirrite:osmId "ourairports_com" ;
    rdfs:subClassOf piirrite:OsmEntity ;
    skos:definition ""@en ;
    skos:inScheme piirritev:OsmSource ;
    skos:prefLabel "Ourairports com"@en .

piirritev:OsmSourcePaci a skos:Concept ;
    piirrite:osmId "PACI" ;
    rdfs:subClassOf piirrite:OsmEntity ;
    skos:definition ""@en ;
    skos:inScheme piirritev:OsmSource ;
    skos:prefLabel "Paci"@en .

piirritev:OsmSourceParticipa2021 a skos:Concept ;
    piirrite:osmId "participa2021",
        "participa_2021" ;
    rdfs:subClassOf piirrite:OsmEntity ;
    skos:definition ""@en ;
    skos:inScheme piirritev:OsmSource ;
    skos:prefLabel "Participa 2021"@en,
        "Participa2021"@en .

piirritev:OsmSourcePcrs2022 a skos:Concept ;
    piirrite:osmId "PCRS_2022" ;
    rdfs:subClassOf piirrite:OsmEntity ;
    skos:definition ""@en ;
    skos:inScheme piirritev:OsmSource ;
    skos:prefLabel "Pcrs 2022"@en .

piirritev:OsmSourcePcrsRaster a skos:Concept ;
    piirrite:osmId "PCRS_Raster",
        "PCRS_raster" ;
    rdfs:subClassOf piirrite:OsmEntity ;
    skos:definition ""@en ;
    skos:inScheme piirritev:OsmSource ;
    skos:prefLabel "Pcrs raster"@en .

piirritev:OsmSourcePdokWaterschap a skos:Concept ;
    piirrite:osmId "PDOK_Waterschap" ;
    rdfs:subClassOf piirrite:OsmEntity ;
    skos:definition ""@en ;
    skos:inScheme piirritev:OsmSource ;
    skos:prefLabel "Pdok waterschap"@en .

piirritev:OsmSourcePgs a skos:Concept ;
    piirrite:osmId "PGS" ;
    rdfs:subClassOf piirrite:OsmEntity ;
    skos:definition "Prototype Global Shoreline: coastline data from the US National Geospatial-Intelligence Agency"@en ;
    skos:inScheme piirritev:OsmSource ;
    skos:prefLabel "Pgs"@en .

piirritev:OsmSourcePlanAt2008 a skos:Concept ;
    piirrite:osmId "plan_at_2008" ;
    rdfs:subClassOf piirrite:OsmEntity ;
    skos:definition ""@en ;
    skos:inScheme piirritev:OsmSource ;
    skos:prefLabel "Plan at 2008"@en .

piirritev:OsmSourcePlanAt2009 a skos:Concept ;
    piirrite:osmId "plan_at_2009" ;
    rdfs:subClassOf piirrite:OsmEntity ;
    skos:definition ""@en ;
    skos:inScheme piirritev:OsmSource ;
    skos:prefLabel "Plan at 2009"@en .

piirritev:OsmSourcePleiades-2016 a skos:Concept ;
    piirrite:osmId "Pleiades-2016" ;
    rdfs:subClassOf piirrite:OsmEntity ;
    skos:definition ""@en ;
    skos:inScheme piirritev:OsmSource ;
    skos:prefLabel "Pleiades-2016"@en .

piirritev:OsmSourcePmsp a skos:Concept ;
    piirrite:osmId "pmsp" ;
    rdfs:subClassOf piirrite:OsmEntity ;
    skos:definition ""@en ;
    skos:inScheme piirritev:OsmSource ;
    skos:prefLabel "Pmsp"@en .

piirritev:OsmSourcePodgikGorzw a skos:Concept ;
    piirrite:osmId "PODGIK_Gorzw" ;
    rdfs:subClassOf piirrite:OsmEntity ;
    skos:definition ""@en ;
    skos:inScheme piirritev:OsmSource ;
    skos:prefLabel "Podgik gorzw"@en .

piirritev:OsmSourcePowiatMikoowski a skos:Concept ;
    piirrite:osmId "Powiat_mikoowski" ;
    rdfs:subClassOf piirrite:OsmEntity ;
    skos:definition ""@en ;
    skos:inScheme piirritev:OsmSource ;
    skos:prefLabel "Powiat mikoowski"@en .

piirritev:OsmSourcePrng a skos:Concept ;
    piirrite:osmId "PRNG" ;
    rdfs:subClassOf piirrite:OsmEntity ;
    skos:definition "Data imported from Pastwowy Rejestr Nazw Geograficznych."@en ;
    skos:inScheme piirritev:OsmSource ;
    skos:prefLabel "Prng"@en .

piirritev:OsmSourceProrail a skos:Concept ;
    piirrite:osmId "ProRail" ;
    rdfs:subClassOf piirrite:OsmEntity ;
    skos:definition ""@en ;
    skos:inScheme piirritev:OsmSource ;
    skos:prefLabel "Prorail"@en .

piirritev:OsmSourceRaba-Kgz a skos:Concept ;
    piirrite:osmId "RABA-KGZ" ;
    rdfs:subClassOf piirrite:OsmEntity ;
    skos:definition "Data imported from Database of actual use of agricultural and forest land (Evidenca dejanske rabe kmetijskih in gozdnih zemlji, \"RABA\") from Slovenian Ministry of Agriculture and the Environment"@en ;
    skos:inScheme piirritev:OsmSource ;
    skos:prefLabel "Raba-kgz"@en .

piirritev:OsmSourceRafvg a skos:Concept ;
    piirrite:osmId "RAFVG" ;
    rdfs:subClassOf piirrite:OsmEntity ;
    skos:definition ""@en ;
    skos:inScheme piirritev:OsmSource ;
    skos:prefLabel "Rafvg"@en .

piirritev:OsmSourceRedRoi a skos:Concept ;
    piirrite:osmId "Red_ROI" ;
    rdfs:subClassOf piirrite:OsmEntity ;
    skos:definition ""@en ;
    skos:inScheme piirritev:OsmSource ;
    skos:prefLabel "Red roi"@en .

piirritev:OsmSourceRefWwwRgcCd a skos:Concept ;
    piirrite:osmId "www_rgc_cd" ;
    rdfs:subClassOf piirrite:OsmEntity ;
    skos:definition ""@en ;
    skos:inScheme piirritev:OsmSourceRef ;
    skos:prefLabel "Www rgc cd"@en .

piirritev:OsmSourceRegioneLiguria a skos:Concept ;
    piirrite:osmId "Regione_Liguria" ;
    rdfs:subClassOf piirrite:OsmEntity ;
    skos:definition ""@en ;
    skos:inScheme piirritev:OsmSource ;
    skos:prefLabel "Regione liguria"@en .

piirritev:OsmSourceRegioneToscana a skos:Concept ;
    piirrite:osmId "Regione_Toscana" ;
    rdfs:subClassOf piirrite:OsmEntity ;
    skos:definition ""@en ;
    skos:inScheme piirritev:OsmSource ;
    skos:prefLabel "Regione toscana"@en .

piirritev:OsmSourceRennesMtropole a skos:Concept ;
    piirrite:osmId "Rennes_Mtropole" ;
    rdfs:subClassOf piirrite:OsmEntity ;
    skos:definition ""@en ;
    skos:inScheme piirritev:OsmSource ;
    skos:prefLabel "Rennes mtropole"@en .

piirritev:OsmSourceResilientes a skos:Concept ;
    piirrite:osmId "resilientes" ;
    rdfs:subClassOf piirrite:OsmEntity ;
    skos:definition ""@en ;
    skos:inScheme piirritev:OsmSource ;
    skos:prefLabel "Resilientes"@en .

piirritev:OsmSourceRgeAlti a skos:Concept ;
    piirrite:osmId "RGE_Alti" ;
    rdfs:subClassOf piirrite:OsmEntity ;
    skos:definition ""@en ;
    skos:inScheme piirritev:OsmSource ;
    skos:prefLabel "Rge alti"@en .

piirritev:OsmSourceRigis a skos:Concept ;
    piirrite:osmId "RIGIS" ;
    rdfs:subClassOf piirrite:OsmEntity ;
    skos:definition ""@en ;
    skos:inScheme piirritev:OsmSource ;
    skos:prefLabel "Rigis"@en .

piirritev:OsmSourceRosreestr a skos:Concept ;
    piirrite:osmId "rosreestr" ;
    rdfs:subClassOf piirrite:OsmEntity ;
    skos:definition ""@en ;
    skos:inScheme piirritev:OsmSource ;
    skos:prefLabel "Rosreestr"@en .

piirritev:OsmSourceRuian a skos:Concept ;
    piirrite:osmId "ruian" ;
    rdfs:subClassOf piirrite:OsmEntity ;
    skos:definition "Using this tag is discouraged, use tag:source=cuzk:ruian instead."@en ;
    skos:inScheme piirritev:OsmSource ;
    skos:prefLabel "Ruian"@en .

piirritev:OsmSourceSagns a skos:Concept ;
    piirrite:osmId "sagns" ;
    rdfs:subClassOf piirrite:OsmEntity ;
    skos:definition ""@en ;
    skos:inScheme piirritev:OsmSource ;
    skos:prefLabel "Sagns"@en .

piirritev:OsmSourceSas a skos:Concept ;
    piirrite:osmId "sas" ;
    rdfs:subClassOf piirrite:OsmEntity ;
    skos:definition ""@en ;
    skos:inScheme piirritev:OsmSource ;
    skos:prefLabel "Sas"@en .

piirritev:OsmSourceScanexIrs a skos:Concept ;
    piirrite:osmId "ScanEx_IRS" ;
    rdfs:subClassOf piirrite:OsmEntity ;
    skos:definition ""@en ;
    skos:inScheme piirritev:OsmSource ;
    skos:prefLabel "Scanex irs"@en .

piirritev:OsmSourceSentinel-2 a skos:Concept ;
    piirrite:osmId "Sentinel-2" ;
    rdfs:subClassOf piirrite:OsmEntity ;
    skos:definition ""@en ;
    skos:inScheme piirritev:OsmSource ;
    skos:prefLabel "Sentinel-2"@en .

piirritev:OsmSourceSigcdmx a skos:Concept ;
    piirrite:osmId "SIGCDMX" ;
    rdfs:subClassOf piirrite:OsmEntity ;
    skos:definition ""@en ;
    skos:inScheme piirritev:OsmSource ;
    skos:prefLabel "Sigcdmx"@en .

piirritev:OsmSourceSobzeros a skos:Concept ;
    piirrite:osmId "sobzeros" ;
    rdfs:subClassOf piirrite:OsmEntity ;
    skos:definition ""@en ;
    skos:inScheme piirritev:OsmSource ;
    skos:prefLabel "Sobzeros"@en .

piirritev:OsmSourceSous-SurveillanceNet a skos:Concept ;
    piirrite:osmId "sous-surveillance_net" ;
    rdfs:subClassOf piirrite:OsmEntity ;
    skos:definition ""@en ;
    skos:inScheme piirritev:OsmSource ;
    skos:prefLabel "Sous-surveillance net"@en .

piirritev:OsmSourceStackbox a skos:Concept ;
    piirrite:osmId "stackbox" ;
    rdfs:subClassOf piirrite:OsmEntity ;
    skos:definition ""@en ;
    skos:inScheme piirritev:OsmSource ;
    skos:prefLabel "Stackbox"@en .

piirritev:OsmSourceStadtverwaltungMarl a skos:Concept ;
    piirrite:osmId "Stadtverwaltung_Marl" ;
    rdfs:subClassOf piirrite:OsmEntity ;
    skos:definition ""@en ;
    skos:inScheme piirritev:OsmSource ;
    skos:prefLabel "Stadtverwaltung marl"@en .

piirritev:OsmSourceStatcan92-500-X a skos:Concept ;
    piirrite:osmId "StatCan_92-500-X" ;
    rdfs:subClassOf piirrite:OsmEntity ;
    skos:definition ""@en ;
    skos:inScheme piirritev:OsmSource ;
    skos:prefLabel "Statcan 92-500-x"@en .

piirritev:OsmSourceStatkartN50 a skos:Concept ;
    piirrite:osmId "Statkart_N50" ;
    rdfs:subClassOf piirrite:OsmEntity ;
    skos:definition ""@en ;
    skos:inScheme piirritev:OsmSource ;
    skos:prefLabel "Statkart n50"@en .

piirritev:OsmSourceStrava a skos:Concept ;
    piirrite:osmId "Strava" ;
    rdfs:subClassOf piirrite:OsmEntity ;
    skos:definition ""@en ;
    skos:inScheme piirritev:OsmSource ;
    skos:prefLabel "Strava"@en .

piirritev:OsmSourceStravaHeatmap a skos:Concept ;
    piirrite:osmId "strava_heatmap" ;
    rdfs:subClassOf piirrite:OsmEntity ;
    skos:definition ""@en ;
    skos:inScheme piirritev:OsmSource ;
    skos:prefLabel "Strava heatmap"@en .

piirritev:OsmSourceSuperadlen a skos:Concept ;
    piirrite:osmId "Superadlen" ;
    rdfs:subClassOf piirrite:OsmEntity ;
    skos:definition ""@en ;
    skos:inScheme piirritev:OsmSource ;
    skos:prefLabel "Superadlen"@en .

piirritev:OsmSourceSurvey a skos:Concept ;
    piirrite:osmId "Survey",
        "survey" ;
    rdfs:subClassOf piirrite:OsmEntity ;
    skos:definition ""@en,
        "For a survey to a specific object."@en ;
    skos:inScheme piirritev:OsmSource ;
    skos:prefLabel "Survey"@en .

piirritev:OsmSourceSurveymm a skos:Concept ;
    piirrite:osmId "surveymm" ;
    rdfs:subClassOf piirrite:OsmEntity ;
    skos:definition ""@en ;
    skos:inScheme piirritev:OsmSource ;
    skos:prefLabel "Surveymm"@en .

piirritev:OsmSourceSwisstopoSwissimage a skos:Concept ;
    piirrite:osmId "swisstopo_SWISSIMAGE" ;
    rdfs:subClassOf piirrite:OsmEntity ;
    skos:definition ""@en ;
    skos:inScheme piirritev:OsmSource ;
    skos:prefLabel "Swisstopo swissimage"@en .

piirritev:OsmSourceTallerc a skos:Concept ;
    piirrite:osmId "tallerc" ;
    rdfs:subClassOf piirrite:OsmEntity ;
    skos:definition ""@en ;
    skos:inScheme piirritev:OsmSource ;
    skos:prefLabel "Tallerc"@en .

piirritev:OsmSourceTallerc9 a skos:Concept ;
    piirrite:osmId "tallerc9" ;
    rdfs:subClassOf piirrite:OsmEntity ;
    skos:definition ""@en ;
    skos:inScheme piirritev:OsmSource ;
    skos:prefLabel "Tallerc9"@en .

piirritev:OsmSourceTesisnanawa a skos:Concept ;
    piirrite:osmId "tesisnanawa" ;
    rdfs:subClassOf piirrite:OsmEntity ;
    skos:definition ""@en ;
    skos:inScheme piirritev:OsmSource ;
    skos:prefLabel "Tesisnanawa"@en .

piirritev:OsmSourceTfgChacoi a skos:Concept ;
    piirrite:osmId "tfg_chacoi" ;
    rdfs:subClassOf piirrite:OsmEntity ;
    skos:definition ""@en ;
    skos:inScheme piirritev:OsmSource ;
    skos:prefLabel "Tfg chacoi"@en .

piirritev:OsmSourceThunderforestLandschaft a skos:Concept ;
    piirrite:osmId "Thunderforest_Landschaft" ;
    rdfs:subClassOf piirrite:OsmEntity ;
    skos:definition ""@en ;
    skos:inScheme piirritev:OsmSource ;
    skos:prefLabel "Thunderforest landschaft"@en .

piirritev:OsmSourceToulousemetropole a skos:Concept ;
    piirrite:osmId "ToulouseMetropole" ;
    rdfs:subClassOf piirrite:OsmEntity ;
    skos:definition ""@en ;
    skos:inScheme piirritev:OsmSource ;
    skos:prefLabel "Toulousemetropole"@en .

piirritev:OsmSourceTuristautakHu a skos:Concept ;
    piirrite:osmId "turistautak_hu" ;
    rdfs:subClassOf piirrite:OsmEntity ;
    skos:definition ""@en ;
    skos:inScheme piirritev:OsmSource ;
    skos:prefLabel "Turistautak hu"@en .

piirritev:OsmSourceUbos2014 a skos:Concept ;
    piirrite:osmId "UBOS_2014",
        "Ubos_2014" ;
    rdfs:subClassOf piirrite:OsmEntity ;
    skos:definition ""@en ;
    skos:inScheme piirritev:OsmSource ;
    skos:prefLabel "Ubos 2014"@en .

piirritev:OsmSourceUcap a skos:Concept ;
    piirrite:osmId "ucap" ;
    rdfs:subClassOf piirrite:OsmEntity ;
    skos:definition ""@en ;
    skos:inScheme piirritev:OsmSource ;
    skos:prefLabel "Ucap"@en .

piirritev:OsmSourceUmGorzw a skos:Concept ;
    piirrite:osmId "UM_Gorzw" ;
    rdfs:subClassOf piirrite:OsmEntity ;
    skos:definition ""@en ;
    skos:inScheme piirritev:OsmSource ;
    skos:prefLabel "Um gorzw"@en .

piirritev:OsmSourceUmJastrzbie-Zdrj a skos:Concept ;
    piirrite:osmId "UM_Jastrzbie-Zdrj" ;
    rdfs:subClassOf piirrite:OsmEntity ;
    skos:definition ""@en ;
    skos:inScheme piirritev:OsmSource ;
    skos:prefLabel "Um jastrzbie-zdrj"@en .

piirritev:OsmSourceUmKatowice a skos:Concept ;
    piirrite:osmId "UM_Katowice" ;
    rdfs:subClassOf piirrite:OsmEntity ;
    skos:definition ""@en ;
    skos:inScheme piirritev:OsmSource ;
    skos:prefLabel "Um katowice"@en .

piirritev:OsmSourceUmOpole a skos:Concept ;
    piirrite:osmId "UM_Opole" ;
    rdfs:subClassOf piirrite:OsmEntity ;
    skos:definition ""@en ;
    skos:inScheme piirritev:OsmSource ;
    skos:prefLabel "Um opole"@en .

piirritev:OsmSourceUmRacibrz a skos:Concept ;
    piirrite:osmId "UM_Racibrz" ;
    rdfs:subClassOf piirrite:OsmEntity ;
    skos:definition ""@en ;
    skos:inScheme piirritev:OsmSource ;
    skos:prefLabel "Um racibrz"@en .

piirritev:OsmSourceUmRzeszw a skos:Concept ;
    piirrite:osmId "UM_Rzeszw" ;
    rdfs:subClassOf piirrite:OsmEntity ;
    skos:definition ""@en ;
    skos:inScheme piirritev:OsmSource ;
    skos:prefLabel "Um rzeszw"@en .

piirritev:OsmSourceUmZabrze a skos:Concept ;
    piirrite:osmId "UM_Zabrze" ;
    rdfs:subClassOf piirrite:OsmEntity ;
    skos:definition ""@en ;
    skos:inScheme piirritev:OsmSource ;
    skos:prefLabel "Um zabrze"@en .

piirritev:OsmSourceUmhvrvisstovanWwwUsFo a skos:Concept ;
    piirrite:osmId "Umhvrvisstovan_www_us_fo" ;
    rdfs:subClassOf piirrite:OsmEntity ;
    skos:definition ""@en ;
    skos:inScheme piirritev:OsmSource ;
    skos:prefLabel "Umhvrvisstovan www us fo"@en .

piirritev:OsmSourceUnicef a skos:Concept ;
    piirrite:osmId "UNICEF" ;
    rdfs:subClassOf piirrite:OsmEntity ;
    skos:definition ""@en ;
    skos:inScheme piirritev:OsmSource ;
    skos:prefLabel "Unicef"@en .

piirritev:OsmSourceUnmil a skos:Concept ;
    piirrite:osmId "UNMIL" ;
    rdfs:subClassOf piirrite:OsmEntity ;
    skos:definition ""@en ;
    skos:inScheme piirritev:OsmSource ;
    skos:prefLabel "Unmil"@en .

piirritev:OsmSourceUrbanismPmbRo a skos:Concept ;
    piirrite:osmId "urbanism_pmb_ro" ;
    rdfs:subClassOf piirrite:OsmEntity ;
    skos:definition ""@en ;
    skos:inScheme piirritev:OsmSource ;
    skos:prefLabel "Urbanism pmb ro"@en .

piirritev:OsmSourceUsgs a skos:Concept ;
    piirrite:osmId "USGS" ;
    rdfs:subClassOf piirrite:OsmEntity ;
    skos:definition ""@en ;
    skos:inScheme piirritev:OsmSource ;
    skos:prefLabel "Usgs"@en .

piirritev:OsmSourceUsgs-Nhd a skos:Concept ;
    piirrite:osmId "USGS-NHD" ;
    rdfs:subClassOf piirrite:OsmEntity ;
    skos:definition ""@en ;
    skos:inScheme piirritev:OsmSource ;
    skos:prefLabel "Usgs-nhd"@en .

piirritev:OsmSourceUsgsGeonames a skos:Concept ;
    piirrite:osmId "USGS_Geonames" ;
    rdfs:subClassOf piirrite:OsmEntity ;
    skos:definition ""@en ;
    skos:inScheme piirritev:OsmSource ;
    skos:prefLabel "Usgs geonames"@en .

piirritev:OsmSourceUsgsOrtho a skos:Concept ;
    piirrite:osmId "USGS_Ortho" ;
    rdfs:subClassOf piirrite:OsmEntity ;
    skos:definition ""@en ;
    skos:inScheme piirritev:OsmSource ;
    skos:prefLabel "Usgs ortho"@en .

piirritev:OsmSourceUsgsTreecover2010 a skos:Concept ;
    piirrite:osmId "USGS_treecover2010" ;
    rdfs:subClassOf piirrite:OsmEntity ;
    skos:definition ""@en ;
    skos:inScheme piirritev:OsmSource ;
    skos:prefLabel "Usgs treecover2010"@en .

piirritev:OsmSourceVicmapAddress a skos:Concept ;
    piirrite:osmId "Vicmap_Address" ;
    rdfs:subClassOf piirrite:OsmEntity ;
    skos:definition ""@en ;
    skos:inScheme piirritev:OsmSource ;
    skos:prefLabel "Vicmap address"@en .

piirritev:OsmSourceVicmapHydro a skos:Concept ;
    piirrite:osmId "VicMap_Hydro" ;
    rdfs:subClassOf piirrite:OsmEntity ;
    skos:definition ""@en ;
    skos:inScheme piirritev:OsmSource ;
    skos:prefLabel "Vicmap hydro"@en .

piirritev:OsmSourceWakegis a skos:Concept ;
    piirrite:osmId "WakeGIS" ;
    rdfs:subClassOf piirrite:OsmEntity ;
    skos:definition ""@en ;
    skos:inScheme piirritev:OsmSource ;
    skos:prefLabel "Wakegis"@en .

piirritev:OsmSourceWcGis a skos:Concept ;
    piirrite:osmId "WC_GIS" ;
    rdfs:subClassOf piirrite:OsmEntity ;
    skos:definition ""@en ;
    skos:inScheme piirritev:OsmSource ;
    skos:prefLabel "Wc gis"@en .

piirritev:OsmSourceWienAt a skos:Concept ;
    piirrite:osmId "wien_at" ;
    rdfs:subClassOf piirrite:OsmEntity ;
    skos:definition ""@en ;
    skos:inScheme piirritev:OsmSource ;
    skos:prefLabel "Wien at"@en .

piirritev:OsmSourceWienGvAt a skos:Concept ;
    piirrite:osmId "wien_gv_at" ;
    rdfs:subClassOf piirrite:OsmEntity ;
    skos:definition ""@en ;
    skos:inScheme piirritev:OsmSource ;
    skos:prefLabel "Wien gv at"@en .

piirritev:OsmSourceWmca a skos:Concept ;
    piirrite:osmId "WMCA" ;
    rdfs:subClassOf piirrite:OsmEntity ;
    skos:definition ""@en ;
    skos:inScheme piirritev:OsmSource ;
    skos:prefLabel "Wmca"@en .

piirritev:OsmSourceWroclawgis a skos:Concept ;
    piirrite:osmId "WroclawGIS" ;
    rdfs:subClassOf piirrite:OsmEntity ;
    skos:definition ""@en ;
    skos:inScheme piirritev:OsmSource ;
    skos:prefLabel "Wroclawgis"@en .

piirritev:OsmSourceWwwGeoportalGovPl a skos:Concept ;
    piirrite:osmId "www_geoportal_gov_pl" ;
    rdfs:subClassOf piirrite:OsmEntity ;
    skos:definition ""@en ;
    skos:inScheme piirritev:OsmSource ;
    skos:prefLabel "Www geoportal gov pl"@en .

piirritev:OsmSourceWwwUbosOrg a skos:Concept ;
    piirrite:osmId "www_ubos_org" ;
    rdfs:subClassOf piirrite:OsmEntity ;
    skos:definition ""@en ;
    skos:inScheme piirritev:OsmSource ;
    skos:prefLabel "Www ubos org"@en .

piirritev:OsmSourceYahoo a skos:Concept ;
    piirrite:osmId "Yahoo",
        "yahoo" ;
    rdfs:subClassOf piirrite:OsmEntity ;
    skos:definition ""@en ;
    skos:inScheme piirritev:OsmSource ;
    skos:prefLabel "Yahoo"@en .

piirritev:OsmSourceYahooHires a skos:Concept ;
    piirrite:osmId "Yahoo_hires" ;
    rdfs:subClassOf piirrite:OsmEntity ;
    skos:definition ""@en ;
    skos:inScheme piirritev:OsmSource ;
    skos:prefLabel "Yahoo hires"@en .

piirritev:OsmSourceYahooImagery a skos:Concept ;
    piirrite:osmId "Yahoo_Imagery",
        "Yahoo_imagery",
        "yahoo_imagery" ;
    rdfs:subClassOf piirrite:OsmEntity ;
    skos:definition ""@en ;
    skos:inScheme piirritev:OsmSource ;
    skos:prefLabel "Yahoo imagery"@en .

piirritev:OsmSourceYahooWms a skos:Concept ;
    piirrite:osmId "yahoo_wms" ;
    rdfs:subClassOf piirrite:OsmEntity ;
    skos:definition ""@en ;
    skos:inScheme piirritev:OsmSource ;
    skos:prefLabel "Yahoo wms"@en .

piirritev:OsmSourceZbgis a skos:Concept ;
    piirrite:osmId "ZBGIS" ;
    rdfs:subClassOf piirrite:OsmEntity ;
    skos:definition ""@en ;
    skos:inScheme piirritev:OsmSource ;
    skos:prefLabel "Zbgis"@en .

piirritev:OsmSource a skos:Concept ;
    piirrite:osmId "_" ;
    rdfs:subClassOf piirrite:OsmEntity ;
    skos:definition ""@en ;
    skos:inScheme piirritev:OsmSource ;
    skos:prefLabel " "@en .

piirritev:OsmSource a skos:Concept ;
    piirrite:osmId "" ;
    rdfs:subClassOf piirrite:OsmEntity ;
    skos:definition ""@en ;
    skos:inScheme piirritev:OsmSource ;
    skos:prefLabel ""@en .

piirritev:OsmSource a skos:Concept ;
    piirrite:osmId "" ;
    rdfs:subClassOf piirrite:OsmEntity ;
    skos:definition ""@en ;
    skos:inScheme piirritev:OsmSource ;
    skos:prefLabel ""@en .

piirritev:OsmSource a skos:Concept ;
    piirrite:osmId "" ;
    rdfs:subClassOf piirrite:OsmEntity ;
    skos:definition ""@en ;
    skos:inScheme piirritev:OsmSource ;
    skos:prefLabel ""@en .

piirritev:OsmSource a skos:Concept ;
    piirrite:osmId "" ;
    rdfs:subClassOf piirrite:OsmEntity ;
    skos:definition ""@en ;
    skos:inScheme piirritev:OsmSource ;
    skos:prefLabel ""@en .

piirritev:OsmSource a skos:Concept ;
    piirrite:osmId "" ;
    rdfs:subClassOf piirrite:OsmEntity ;
    skos:definition ""@en ;
    skos:inScheme piirritev:OsmSource ;
    skos:prefLabel ""@en .

piirritev:OsmSource a skos:Concept ;
    piirrite:osmId "" ;
    rdfs:subClassOf piirrite:OsmEntity ;
    skos:definition ""@en ;
    skos:inScheme piirritev:OsmSource ;
    skos:prefLabel ""@en .

piirritev:OsmSource a skos:Concept ;
    piirrite:osmId "" ;
    rdfs:subClassOf piirrite:OsmEntity ;
    skos:definition ""@en ;
    skos:inScheme piirritev:OsmSource ;
    skos:prefLabel ""@en .

piirritev:OsmSource a skos:Concept ;
    piirrite:osmId "" ;
    rdfs:subClassOf piirrite:OsmEntity ;
    skos:definition ""@en ;
    skos:inScheme piirritev:OsmSource ;
    skos:prefLabel ""@en .

piirritev:OsmSource a skos:Concept ;
    piirrite:osmId "" ;
    rdfs:subClassOf piirrite:OsmEntity ;
    skos:definition ""@en ;
    skos:inScheme piirritev:OsmSource ;
    skos:prefLabel ""@en .

piirritev:OsmSource a skos:Concept ;
    piirrite:osmId "" ;
    rdfs:subClassOf piirrite:OsmEntity ;
    skos:definition ""@en ;
    skos:inScheme piirritev:OsmSource ;
    skos:prefLabel ""@en .

piirritev:OsmSource a skos:Concept ;
    piirrite:osmId "" ;
    rdfs:subClassOf piirrite:OsmEntity ;
    skos:definition ""@en ;
    skos:inScheme piirritev:OsmSource ;
    skos:prefLabel ""@en .

piirritev:OsmSource a skos:Concept ;
    piirrite:osmId "" ;
    rdfs:subClassOf piirrite:OsmEntity ;
    skos:definition ""@en ;
    skos:inScheme piirritev:OsmSource ;
    skos:prefLabel ""@en .

piirritev:OsmSource a skos:Concept ;
    piirrite:osmId "" ;
    rdfs:subClassOf piirrite:OsmEntity ;
    skos:definition ""@en ;
    skos:inScheme piirritev:OsmSource ;
    skos:prefLabel ""@en .

piirritev:OsmSource a skos:Concept ;
    piirrite:osmId "" ;
    rdfs:subClassOf piirrite:OsmEntity ;
    skos:definition ""@en ;
    skos:inScheme piirritev:OsmSource ;
    skos:prefLabel ""@en .

piirritev:OsmSource a skos:Concept ;
    piirrite:osmId "" ;
    rdfs:subClassOf piirrite:OsmEntity ;
    skos:definition ""@en ;
    skos:inScheme piirritev:OsmSource ;
    skos:prefLabel ""@en .

piirritev:OsmSource a skos:Concept ;
    piirrite:osmId "" ;
    rdfs:subClassOf piirrite:OsmEntity ;
    skos:definition ""@en ;
    skos:inScheme piirritev:OsmSource ;
    skos:prefLabel ""@en .

piirritev:OsmSource a skos:Concept ;
    piirrite:osmId "" ;
    rdfs:subClassOf piirrite:OsmEntity ;
    skos:definition ""@en ;
    skos:inScheme piirritev:OsmSource ;
    skos:prefLabel ""@en .

piirritev:OsmSource a skos:Concept ;
    piirrite:osmId "" ;
    rdfs:subClassOf piirrite:OsmEntity ;
    skos:definition ""@en ;
    skos:inScheme piirritev:OsmSource ;
    skos:prefLabel ""@en .

piirritev:OsmSource a skos:Concept ;
    piirrite:osmId "" ;
    rdfs:subClassOf piirrite:OsmEntity ;
    skos:definition ""@en ;
    skos:inScheme piirritev:OsmSource ;
    skos:prefLabel ""@en .

piirritev:OsmSource a skos:Concept ;
    piirrite:osmId "" ;
    rdfs:subClassOf piirrite:OsmEntity ;
    skos:definition ""@en ;
    skos:inScheme piirritev:OsmSource ;
    skos:prefLabel ""@en .

piirritev:OsmSource a skos:Concept ;
    piirrite:osmId "" ;
    rdfs:subClassOf piirrite:OsmEntity ;
    skos:definition ""@en ;
    skos:inScheme piirritev:OsmSource ;
    skos:prefLabel ""@en .

piirritev:OsmSpeciesAcerCampestre a skos:Concept ;
    piirrite:osmId "Acer_campestre" ;
    rdfs:subClassOf piirrite:OsmEntity ;
    skos:definition ""@en ;
    skos:inScheme piirritev:OsmSpecies ;
    skos:prefLabel "Acer campestre"@en .

piirritev:OsmSpeciesAcerNegundo a skos:Concept ;
    piirrite:osmId "Acer_negundo" ;
    rdfs:subClassOf piirrite:OsmEntity ;
    skos:definition ""@en ;
    skos:inScheme piirritev:OsmSpecies ;
    skos:prefLabel "Acer negundo"@en .

piirritev:OsmSpeciesAcerPseudoplatanus a skos:Concept ;
    piirrite:osmId "Acer_pseudoplatanus" ;
    rdfs:subClassOf piirrite:OsmEntity ;
    skos:definition ""@en ;
    skos:inScheme piirritev:OsmSpecies ;
    skos:prefLabel "Acer pseudoplatanus"@en .

piirritev:OsmSpeciesAcerRubrum a skos:Concept ;
    piirrite:osmId "Acer_rubrum" ;
    rdfs:subClassOf piirrite:OsmEntity ;
    skos:definition ""@en ;
    skos:inScheme piirritev:OsmSpecies ;
    skos:prefLabel "Acer rubrum"@en .

piirritev:OsmSpeciesAcerSaccharinum a skos:Concept ;
    piirrite:osmId "Acer_saccharinum" ;
    rdfs:subClassOf piirrite:OsmEntity ;
    skos:definition ""@en ;
    skos:inScheme piirritev:OsmSpecies ;
    skos:prefLabel "Acer saccharinum"@en .

piirritev:OsmSpeciesAcerSaccharum a skos:Concept ;
    piirrite:osmId "Acer_saccharum" ;
    rdfs:subClassOf piirrite:OsmEntity ;
    skos:definition ""@en ;
    skos:inScheme piirritev:OsmSpecies ;
    skos:prefLabel "Acer saccharum"@en .

piirritev:OsmSpeciesAesculusHippocastanum a skos:Concept ;
    piirrite:osmId "Aesculus_hippocastanum" ;
    rdfs:subClassOf piirrite:OsmEntity ;
    skos:definition ""@en ;
    skos:inScheme piirritev:OsmSpecies ;
    skos:prefLabel "Aesculus hippocastanum"@en .

piirritev:OsmSpeciesBetulaPendula a skos:Concept ;
    piirrite:osmId "Betula_pendula" ;
    rdfs:subClassOf piirrite:OsmEntity ;
    skos:definition ""@en ;
    skos:inScheme piirritev:OsmSpecies ;
    skos:prefLabel "Betula pendula"@en .

piirritev:OsmSpeciesCarpinusBetulus a skos:Concept ;
    piirrite:osmId "Carpinus_betulus" ;
    rdfs:subClassOf piirrite:OsmEntity ;
    skos:definition ""@en ;
    skos:inScheme piirritev:OsmSpecies ;
    skos:prefLabel "Carpinus betulus"@en .

piirritev:OsmSpeciesCastaneaSativa a skos:Concept ;
    piirrite:osmId "Castanea_sativa" ;
    rdfs:subClassOf piirrite:OsmEntity ;
    skos:definition ""@en ;
    skos:inScheme piirritev:OsmSpecies ;
    skos:prefLabel "Castanea sativa"@en .

piirritev:OsmSpeciesCeltisAustralis a skos:Concept ;
    piirrite:osmId "Celtis_australis" ;
    rdfs:subClassOf piirrite:OsmEntity ;
    skos:definition ""@en ;
    skos:inScheme piirritev:OsmSpecies ;
    skos:prefLabel "Celtis australis"@en .

piirritev:OsmSpeciesCocosNucifera a skos:Concept ;
    piirrite:osmId "Cocos_nucifera" ;
    rdfs:subClassOf piirrite:OsmEntity ;
    skos:definition ""@en ;
    skos:inScheme piirritev:OsmSpecies ;
    skos:prefLabel "Cocos nucifera"@en .

piirritev:OsmSpeciesCorylusColurna a skos:Concept ;
    piirrite:osmId "Corylus_colurna" ;
    rdfs:subClassOf piirrite:OsmEntity ;
    skos:definition ""@en ;
    skos:inScheme piirritev:OsmSpecies ;
    skos:prefLabel "Corylus colurna"@en .

piirritev:OsmSpeciesCupressusSempervirens a skos:Concept ;
    piirrite:osmId "Cupressus_sempervirens" ;
    rdfs:subClassOf piirrite:OsmEntity ;
    skos:definition ""@en ;
    skos:inScheme piirritev:OsmSpecies ;
    skos:prefLabel "Cupressus sempervirens"@en .

piirritev:OsmSpeciesFagusSylvatica a skos:Concept ;
    piirrite:osmId "Fagus_sylvatica" ;
    rdfs:subClassOf piirrite:OsmEntity ;
    skos:definition ""@en ;
    skos:inScheme piirritev:OsmSpecies ;
    skos:prefLabel "Fagus sylvatica"@en .

piirritev:OsmSpeciesFraxinusAmericana a skos:Concept ;
    piirrite:osmId "Fraxinus_americana" ;
    rdfs:subClassOf piirrite:OsmEntity ;
    skos:definition ""@en ;
    skos:inScheme piirritev:OsmSpecies ;
    skos:prefLabel "Fraxinus americana"@en .

piirritev:OsmSpeciesFraxinusExcelsior a skos:Concept ;
    piirrite:osmId "Fraxinus_excelsior" ;
    rdfs:subClassOf piirrite:OsmEntity ;
    skos:definition ""@en ;
    skos:inScheme piirritev:OsmSpecies ;
    skos:prefLabel "Fraxinus excelsior"@en .

piirritev:OsmSpeciesFraxinusPennsylvanica a skos:Concept ;
    piirrite:osmId "Fraxinus_pennsylvanica" ;
    rdfs:subClassOf piirrite:OsmEntity ;
    skos:definition ""@en ;
    skos:inScheme piirritev:OsmSpecies ;
    skos:prefLabel "Fraxinus pennsylvanica"@en .

piirritev:OsmSpeciesGinkgoBiloba a skos:Concept ;
    piirrite:osmId "Ginkgo_biloba" ;
    rdfs:subClassOf piirrite:OsmEntity ;
    skos:definition ""@en ;
    skos:inScheme piirritev:OsmSpecies ;
    skos:prefLabel "Ginkgo biloba"@en .

piirritev:OsmSpeciesGleditsiaTriacanthos a skos:Concept ;
    piirrite:osmId "Gleditsia_triacanthos" ;
    rdfs:subClassOf piirrite:OsmEntity ;
    skos:definition ""@en ;
    skos:inScheme piirritev:OsmSpecies ;
    skos:prefLabel "Gleditsia triacanthos"@en .

piirritev:OsmSpeciesJuglansRegia a skos:Concept ;
    piirrite:osmId "Juglans_regia" ;
    rdfs:subClassOf piirrite:OsmEntity ;
    skos:definition ""@en ;
    skos:inScheme piirritev:OsmSpecies ;
    skos:prefLabel "Juglans regia"@en .

piirritev:OsmSpeciesLiquidambarStyraciflua a skos:Concept ;
    piirrite:osmId "Liquidambar_styraciflua" ;
    rdfs:subClassOf piirrite:OsmEntity ;
    skos:definition ""@en ;
    skos:inScheme piirritev:OsmSpecies ;
    skos:prefLabel "Liquidambar styraciflua"@en .

piirritev:OsmSpeciesOleaEuropaea a skos:Concept ;
    piirrite:osmId "Olea_europaea" ;
    rdfs:subClassOf piirrite:OsmEntity ;
    skos:definition ""@en ;
    skos:inScheme piirritev:OsmSpecies ;
    skos:prefLabel "Olea europaea"@en .

piirritev:OsmSpeciesPinusMugo a skos:Concept ;
    piirrite:osmId "Pinus_mugo" ;
    rdfs:subClassOf piirrite:OsmEntity ;
    skos:definition ""@en ;
    skos:inScheme piirritev:OsmSpecies ;
    skos:prefLabel "Pinus mugo"@en .

piirritev:OsmSpeciesPinusPinea a skos:Concept ;
    piirrite:osmId "Pinus_pinea" ;
    rdfs:subClassOf piirrite:OsmEntity ;
    skos:definition ""@en ;
    skos:inScheme piirritev:OsmSpecies ;
    skos:prefLabel "Pinus pinea"@en .

piirritev:OsmSpeciesPinusSylvestris a skos:Concept ;
    piirrite:osmId "Pinus_sylvestris" ;
    rdfs:subClassOf piirrite:OsmEntity ;
    skos:definition ""@en ;
    skos:inScheme piirritev:OsmSpecies ;
    skos:prefLabel "Pinus sylvestris"@en .

piirritev:OsmSpeciesPlatanusAcerifolia a skos:Concept ;
    piirrite:osmId "Platanus_acerifolia" ;
    rdfs:subClassOf piirrite:OsmEntity ;
    skos:definition ""@en ;
    skos:inScheme piirritev:OsmSpecies ;
    skos:prefLabel "Platanus acerifolia"@en .

piirritev:OsmSpeciesPopulusNigra a skos:Concept ;
    piirrite:osmId "Populus_nigra" ;
    rdfs:subClassOf piirrite:OsmEntity ;
    skos:definition ""@en ;
    skos:inScheme piirritev:OsmSpecies ;
    skos:prefLabel "Populus nigra"@en .

piirritev:OsmSpeciesPrunusAvium a skos:Concept ;
    piirrite:osmId "Prunus_avium" ;
    rdfs:subClassOf piirrite:OsmEntity ;
    skos:definition ""@en ;
    skos:inScheme piirritev:OsmSpecies ;
    skos:prefLabel "Prunus avium"@en .

piirritev:OsmSpeciesPrunusCerasifera a skos:Concept ;
    piirrite:osmId "Prunus_cerasifera" ;
    rdfs:subClassOf piirrite:OsmEntity ;
    skos:definition ""@en ;
    skos:inScheme piirritev:OsmSpecies ;
    skos:prefLabel "Prunus cerasifera"@en .

piirritev:OsmSpeciesPrunusSerrulata a skos:Concept ;
    piirrite:osmId "Prunus_serrulata" ;
    rdfs:subClassOf piirrite:OsmEntity ;
    skos:definition ""@en ;
    skos:inScheme piirritev:OsmSpecies ;
    skos:prefLabel "Prunus serrulata"@en .

piirritev:OsmSpeciesPyrusCalleryana a skos:Concept ;
    piirrite:osmId "Pyrus_calleryana" ;
    rdfs:subClassOf piirrite:OsmEntity ;
    skos:definition ""@en ;
    skos:inScheme piirritev:OsmSpecies ;
    skos:prefLabel "Pyrus calleryana"@en .

piirritev:OsmSpeciesQuercusIlex a skos:Concept ;
    piirrite:osmId "Quercus_ilex" ;
    rdfs:subClassOf piirrite:OsmEntity ;
    skos:definition ""@en ;
    skos:inScheme piirritev:OsmSpecies ;
    skos:prefLabel "Quercus ilex"@en .

piirritev:OsmSpeciesQuercusRobur a skos:Concept ;
    piirrite:hasRelatedOsmTag piirrite:hasOsmQuercusRoburCircumference,
        piirrite:hasOsmQuercusRoburHeight,
        piirrite:hasOsmQuercusRoburLeafCycle,
        piirrite:hasOsmQuercusRoburLeafType,
        piirrite:hasOsmQuercusRoburStartDate ;
    piirrite:osmId "Quercus_robur" ;
    rdfs:subClassOf piirrite:OsmEntity ;
    skos:definition "A pedunculate oak. osmcarto-rendering=File:Tree-16.svg osmcarto-rendering-size=16px"@en ;
    skos:inScheme piirritev:OsmSpecies ;
    skos:prefLabel "Quercus robur"@en .

piirritev:OsmSpeciesQuercusRubra a skos:Concept ;
    piirrite:osmId "Quercus_rubra" ;
    rdfs:subClassOf piirrite:OsmEntity ;
    skos:definition ""@en ;
    skos:inScheme piirritev:OsmSpecies ;
    skos:prefLabel "Quercus rubra"@en .

piirritev:OsmSpeciesRobiniaPseudoacacia a skos:Concept ;
    piirrite:osmId "Robinia_pseudoacacia" ;
    rdfs:subClassOf piirrite:OsmEntity ;
    skos:definition ""@en ;
    skos:inScheme piirritev:OsmSpecies ;
    skos:prefLabel "Robinia pseudoacacia"@en .

piirritev:OsmSpeciesTiliaCordata a skos:Concept ;
    piirrite:hasRelatedOsmTag piirrite:hasOsmTiliaCordataCircumference,
        piirrite:hasOsmTiliaCordataHeight,
        piirrite:hasOsmTiliaCordataLeafCycle,
        piirrite:hasOsmTiliaCordataLeafType,
        piirrite:hasOsmTiliaCordataStartDate ;
    piirrite:osmId "Tilia_cordata" ;
    rdfs:subClassOf piirrite:OsmEntity ;
    skos:definition "A small-leaved lime. osmcarto-rendering=File:Tree-16.svg osmcarto-rendering-size=16px"@en ;
    skos:inScheme piirritev:OsmSpecies ;
    skos:prefLabel "Tilia cordata"@en .

piirritev:OsmSpeciesTiliaPlatyphyllos a skos:Concept ;
    piirrite:osmId "Tilia_platyphyllos" ;
    rdfs:subClassOf piirrite:OsmEntity ;
    skos:definition ""@en ;
    skos:inScheme piirritev:OsmSpecies ;
    skos:prefLabel "Tilia platyphyllos"@en .

piirritev:OsmSpeciesTiliaTomentosa a skos:Concept ;
    piirrite:osmId "Tilia_tomentosa" ;
    rdfs:subClassOf piirrite:OsmEntity ;
    skos:definition ""@en ;
    skos:inScheme piirritev:OsmSpecies ;
    skos:prefLabel "Tilia tomentosa"@en .

piirritev:OsmSportAmericanFootball a skos:Concept ;
    piirrite:hasRelatedOsmTag piirrite:hasOsmAmericanFootballLeisure ;
    piirrite:osmId "american_football" ;
    rdfs:subClassOf piirrite:OsmEntity ;
    skos:definition "A sport played by two teams of eleven players on a rectangular field with goalposts at each end."@en ;
    skos:inScheme piirritev:OsmSport ;
    skos:prefLabel "American football"@en .

piirritev:OsmSportAthletics a skos:Concept ;
    piirrite:hasRelatedOsmTag piirrite:hasOsmAthleticsLeisure ;
    piirrite:osmId "athletics" ;
    rdfs:subClassOf piirrite:OsmEntity ;
    skos:definition "A collection of sports which combines various athletic contests based on the skills of running, jumping, and throwing."@en ;
    skos:inScheme piirritev:OsmSport ;
    skos:prefLabel "Athletics"@en .

piirritev:OsmSportBaseball a skos:Concept ;
    piirrite:hasRelatedOsmTag piirrite:hasOsmBaseballLeisure ;
    piirrite:osmId "baseball" ;
    rdfs:subClassOf piirrite:OsmEntity ;
    skos:definition "A bat-and-ball game played between two teams of nine players on a field (pitch or stadium) each who take turns batting and fielding."@en ;
    skos:inScheme piirritev:OsmSport ;
    skos:prefLabel "Baseball"@en .

piirritev:OsmSportBasketball a skos:Concept ;
    piirrite:hasRelatedOsmTag piirrite:hasOsmBasketballLeisure,
        piirrite:hasOsmBasketballName,
        piirrite:hasOsmBasketballSurface ;
    piirrite:osmId "basketball" ;
    rdfs:subClassOf piirrite:OsmEntity ;
    skos:definition "A sport played by two teams of five players on a rectangular court."@en ;
    skos:inScheme piirritev:OsmSport ;
    skos:prefLabel "Basketball"@en .

piirritev:OsmSportBeachvolleyball a skos:Concept ;
    piirrite:hasRelatedOsmTag piirrite:hasOsmBeachvolleyballLeisure,
        piirrite:hasOsmBeachvolleyballName,
        piirrite:hasOsmBeachvolleyballSurface ;
    piirrite:osmId "beachvolleyball" ;
    rdfs:subClassOf piirrite:OsmEntity ;
    skos:definition "Volleyball played on a sand court."@en ;
    skos:inScheme piirritev:OsmSport ;
    skos:prefLabel "Beachvolleyball"@en .

piirritev:OsmSportBoules a skos:Concept ;
    piirrite:hasRelatedOsmTag piirrite:hasOsmBoulesLeisure,
        piirrite:hasOsmBoulesSport,
        piirrite:hasOsmBoulesSurface,
        piirrite:hasOsmBoulesType ;
    piirrite:osmId "boules" ;
    rdfs:subClassOf piirrite:OsmEntity ;
    skos:definition "A group of games in which the objective is to throw or roll heavy balls as close as possible to a small target ball, also called ptanque, lyonnaise, bocce, or bocce volo."@en ;
    skos:inScheme piirritev:OsmSport ;
    skos:prefLabel "Boules"@en .

piirritev:OsmSportBowls a skos:Concept ;
    piirrite:hasRelatedOsmTag piirrite:hasOsmBowlsLeisure,
        piirrite:hasOsmBowlsSurface ;
    piirrite:osmId "bowls" ;
    rdfs:subClassOf piirrite:OsmEntity ;
    skos:definition "Sport in which the objective is to roll biased balls so that they stop close to a smaller ball."@en ;
    skos:inScheme piirritev:OsmSport ;
    skos:prefLabel "Bowls"@en .

piirritev:OsmSportClimbing a skos:Concept ;
    piirrite:hasRelatedOsmTag piirrite:hasOsmClimbingLanduse,
        piirrite:hasOsmClimbingLeisure,
        piirrite:hasOsmClimbingSurface,
        piirrite:hasOsmClimbingType ;
    piirrite:osmId "climbing" ;
    rdfs:subClassOf piirrite:OsmEntity ;
    skos:definition "Marks elements to represent natural climbing sites (climbing areas, sectors, crags, frozen waterfalls, etc.) or artificial climbs (climbing walls, indoor climbing halls, etc.)."@en ;
    skos:inScheme piirritev:OsmSport ;
    skos:prefLabel "Climbing"@en .

piirritev:OsmSportCricket a skos:Concept ;
    piirrite:hasRelatedOsmTag piirrite:hasOsmCricketLanduse,
        piirrite:hasOsmCricketLeisure,
        piirrite:hasOsmCricketSport,
        piirrite:hasOsmCricketSurface ;
    piirrite:osmId "cricket" ;
    rdfs:subClassOf piirrite:OsmEntity ;
    skos:definition "A bat-and-ball sport contested by two teams, usually of eleven players, each on a large grass Cricket pitch. Played on a large circular or oval-shaped grassy Cricket field ground."@en ;
    skos:inScheme piirritev:OsmSport ;
    skos:prefLabel "Cricket"@en .

piirritev:OsmSportCycling a skos:Concept ;
    piirrite:hasRelatedOsmTag piirrite:hasOsmCyclingLanduse,
        piirrite:hasOsmCyclingLeisure,
        piirrite:hasOsmCyclingSurface,
        piirrite:hasOsmCyclingType ;
    piirrite:osmId "cycling" ;
    rdfs:subClassOf piirrite:OsmEntity ;
    skos:definition "The use of bicycles for sport, also called bicycling, mountain biking or biking."@en ;
    skos:inScheme piirritev:OsmSport ;
    skos:prefLabel "Cycling"@en .

piirritev:OsmSportEquestrian a skos:Concept ;
    piirrite:hasRelatedOsmTag piirrite:hasOsmEquestrianBuilding,
        piirrite:hasOsmEquestrianLeisure ;
    piirrite:osmId "equestrian" ;
    rdfs:subClassOf piirrite:OsmEntity ;
    skos:definition "A sport practised with the horse as a partner; but for horse racing use tag:sport=horse_racing."@en ;
    skos:inScheme piirritev:OsmSport ;
    skos:prefLabel "Equestrian"@en .

piirritev:OsmSportFitness a skos:Concept ;
    piirrite:hasRelatedOsmTag piirrite:hasOsmFitnessLeisure ;
    piirrite:osmId "fitness" ;
    rdfs:subClassOf piirrite:OsmEntity ;
    skos:definition "To mark a physical feature related to fitness sports."@en ;
    skos:inScheme piirritev:OsmSport ;
    skos:prefLabel "Fitness"@en .

piirritev:OsmSportFourSquare a skos:Concept ;
    piirrite:hasRelatedOsmTag piirrite:hasOsmFourSquareLeisure ;
    piirrite:osmId "four_square" ;
    rdfs:subClassOf piirrite:OsmEntity ;
    skos:definition "A hand ball game played on a square court."@en ;
    skos:inScheme piirritev:OsmSport ;
    skos:prefLabel "Four square"@en .

piirritev:OsmSportFutsal a skos:Concept ;
    piirrite:hasRelatedOsmTag piirrite:hasOsmFutsalAmenity,
        piirrite:hasOsmFutsalBuilding,
        piirrite:hasOsmFutsalLeisure,
        piirrite:hasOsmFutsalName,
        piirrite:hasOsmFutsalSport,
        piirrite:hasOsmFutsalSurface ;
    piirrite:osmId "futsal" ;
    rdfs:subClassOf piirrite:OsmEntity ;
    skos:definition "Futsal is a sport played by two teams of five players on a rectangular court."@en ;
    skos:inScheme piirritev:OsmSport ;
    skos:prefLabel "Futsal"@en .

piirritev:OsmSportGolf a skos:Concept ;
    piirrite:osmId "golf" ;
    rdfs:subClassOf piirrite:OsmEntity ;
    skos:definition "A stick and ball game played from a 'tee' to a hole."@en ;
    skos:inScheme piirritev:OsmSport ;
    skos:prefLabel "Golf"@en .

piirritev:OsmSportKarting a skos:Concept ;
    piirrite:hasRelatedOsmTag piirrite:hasOsmKartingHighway ;
    piirrite:osmId "karting" ;
    rdfs:subClassOf piirrite:OsmEntity ;
    skos:definition "A motorized race using small open four wheeled vehicles."@en ;
    skos:inScheme piirritev:OsmSport ;
    skos:prefLabel "Karting"@en .

piirritev:OsmSportMotocross a skos:Concept ;
    piirrite:hasRelatedOsmTag piirrite:hasOsmMotocrossHighway ;
    piirrite:osmId "motocross" ;
    rdfs:subClassOf piirrite:OsmEntity ;
    skos:definition "Motorcycle racing on unpaved surfaces."@en ;
    skos:inScheme piirritev:OsmSport ;
    skos:prefLabel "Motocross"@en .

piirritev:OsmSportMotor a skos:Concept ;
    piirrite:hasRelatedOsmTag piirrite:hasOsmMotorHighway ;
    piirrite:osmId "motor" ;
    rdfs:subClassOf piirrite:OsmEntity ;
    skos:definition "Motorsport: a sport with motorised vehicles, e.g. car racing."@en ;
    skos:inScheme piirritev:OsmSport ;
    skos:prefLabel "Motor"@en .

piirritev:OsmSportMulti a skos:Concept ;
    piirrite:hasRelatedOsmTag piirrite:hasOsmMultiLeisure,
        piirrite:hasOsmMultiName,
        piirrite:hasOsmMultiOpeningHours,
        piirrite:hasOsmMultiOperator ;
    piirrite:osmId "multi" ;
    rdfs:subClassOf piirrite:OsmEntity ;
    skos:definition "Property added to otherwise marked sports facility to indicate as suitable for more than one sport, without listing them"@en ;
    skos:inScheme piirritev:OsmSport ;
    skos:prefLabel "Multi"@en .

piirritev:OsmSportNetball a skos:Concept ;
    piirrite:hasRelatedOsmTag piirrite:hasOsmNetballLeisure,
        piirrite:hasOsmNetballName,
        piirrite:hasOsmNetballSurface ;
    piirrite:osmId "netball" ;
    rdfs:subClassOf piirrite:OsmEntity ;
    skos:definition "A hand ball competition between two teams on a rectangular court."@en ;
    skos:inScheme piirritev:OsmSport ;
    skos:prefLabel "Netball"@en .

piirritev:OsmSportPadel a skos:Concept ;
    piirrite:hasRelatedOsmTag piirrite:hasOsmPadelLeisure ;
    piirrite:osmId "padel" ;
    rdfs:subClassOf piirrite:OsmEntity ;
    skos:definition "A racket sport typically played in pairs, where the objective is to bounce the ball in the opponents court, with the option of using the walls during play."@en ;
    skos:inScheme piirritev:OsmSport ;
    skos:prefLabel "Padel"@en .

piirritev:OsmSportPickleball a skos:Concept ;
    piirrite:osmId "pickleball" ;
    rdfs:subClassOf piirrite:OsmEntity ;
    skos:definition "Pickleball, a tennis-like game played with a slower ball on a smaller court."@en ;
    skos:inScheme piirritev:OsmSport ;
    skos:prefLabel "Pickleball"@en .

piirritev:OsmSportRunning a skos:Concept ;
    piirrite:hasRelatedOsmTag piirrite:hasOsmRunningClub,
        piirrite:hasOsmRunningLeisure,
        piirrite:hasOsmRunningShop ;
    piirrite:osmId "running" ;
    rdfs:subClassOf piirrite:OsmEntity ;
    skos:definition "Human propulsion using legs and feet only."@en ;
    skos:inScheme piirritev:OsmSport ;
    skos:prefLabel "Running"@en .

piirritev:OsmSportShooting a skos:Concept ;
    piirrite:hasRelatedOsmTag piirrite:hasOsmShootingName,
        piirrite:hasOsmShootingOperator,
        piirrite:hasOsmShootingType ;
    piirrite:osmId "shooting" ;
    rdfs:subClassOf piirrite:OsmEntity ;
    skos:definition "Identifies given object as used for practicing shooting sports."@en ;
    skos:inScheme piirritev:OsmSport ;
    skos:prefLabel "Shooting"@en .

piirritev:OsmSportSkateboard a skos:Concept ;
    piirrite:hasRelatedOsmTag piirrite:hasOsmSkateboardLeisure ;
    piirrite:osmId "skateboard" ;
    rdfs:subClassOf piirrite:OsmEntity ;
    skos:definition "An area designated and equipped for skateboarding."@en ;
    skos:inScheme piirritev:OsmSport ;
    skos:prefLabel "Skateboard"@en .

piirritev:OsmSportSoccer a skos:Concept ;
    piirrite:hasRelatedOsmTag piirrite:hasOsmSoccerBuilding,
        piirrite:hasOsmSoccerLeisure,
        piirrite:hasOsmSoccerLit,
        piirrite:hasOsmSoccerManMade,
        piirrite:hasOsmSoccerName,
        piirrite:hasOsmSoccerOpeningHours,
        piirrite:hasOsmSoccerOperator,
        piirrite:hasOsmSoccerSurface ;
    piirrite:osmId "soccer" ;
    rdfs:subClassOf piirrite:OsmEntity ;
    skos:definition "To mark a physical feature related to association football, more commonly known as football or soccer."@en ;
    skos:inScheme piirritev:OsmSport ;
    skos:prefLabel "Soccer"@en .

piirritev:OsmSportSwimming a skos:Concept ;
    piirrite:hasRelatedOsmTag piirrite:hasOsmSwimmingLeisure ;
    piirrite:osmId "swimming" ;
    rdfs:subClassOf piirrite:OsmEntity ;
    skos:definition "A place where people swim for sport."@en ;
    skos:inScheme piirritev:OsmSport ;
    skos:prefLabel "Swimming"@en .

piirritev:OsmSportTableTennis a skos:Concept ;
    piirrite:hasRelatedOsmTag piirrite:hasOsmTableTennisBounce,
        piirrite:hasOsmTableTennisCapacity,
        piirrite:hasOsmTableTennisHeight,
        piirrite:hasOsmTableTennisIncline,
        piirrite:hasOsmTableTennisLeisure,
        piirrite:hasOsmTableTennisLength,
        piirrite:hasOsmTableTennisMaterial,
        piirrite:hasOsmTableTennisPlayability,
        piirrite:hasOsmTableTennisShop,
        piirrite:hasOsmTableTennisWidth ;
    piirrite:osmId "table_tennis" ;
    rdfs:subClassOf piirrite:OsmEntity ;
    skos:definition "A bat and ball game played over a table."@en ;
    skos:inScheme piirritev:OsmSport ;
    skos:prefLabel "Table tennis"@en .

piirritev:OsmSportTennis a skos:Concept ;
    piirrite:hasRelatedOsmTag piirrite:hasOsmTennisLeisure,
        piirrite:hasOsmTennisLit,
        piirrite:hasOsmTennisName,
        piirrite:hasOsmTennisSurface ;
    piirrite:osmId "tennis" ;
    rdfs:subClassOf piirrite:OsmEntity ;
    skos:definition "A competition where two or four players use a ball and rackets over a net."@en ;
    skos:inScheme piirritev:OsmSport ;
    skos:prefLabel "Tennis"@en .

piirritev:OsmSportVolleyball a skos:Concept ;
    piirrite:hasRelatedOsmTag piirrite:hasOsmVolleyballLeisure,
        piirrite:hasOsmVolleyballName,
        piirrite:hasOsmVolleyballOperator ;
    piirrite:osmId "volleyball" ;
    rdfs:subClassOf piirrite:OsmEntity ;
    skos:definition "A team sport in which two teams of six players are separated by a net."@en ;
    skos:inScheme piirritev:OsmSport ;
    skos:prefLabel "Volleyball"@en .

piirritev:OsmStandingLow a skos:Concept ;
    piirrite:osmId "low" ;
    rdfs:subClassOf piirrite:OsmEntity ;
    skos:definition ""@en ;
    skos:inScheme piirritev:OsmStanding ;
    skos:prefLabel "Low"@en .

piirritev:OsmStandingVeryLow a skos:Concept ;
    piirrite:osmId "very_low" ;
    rdfs:subClassOf piirrite:OsmEntity ;
    skos:definition ""@en ;
    skos:inScheme piirritev:OsmStanding ;
    skos:prefLabel "Very low"@en .

piirritev:OsmStartDate19761991 a skos:Concept ;
    piirrite:osmId "1976__1991" ;
    rdfs:subClassOf piirrite:OsmEntity ;
    skos:definition ""@en ;
    skos:inScheme piirritev:OsmStartDate ;
    skos:prefLabel "1976  1991"@en .

piirritev:OsmStatusAbandoned a skos:Concept ;
    piirrite:osmId "abandoned" ;
    rdfs:subClassOf piirrite:OsmEntity ;
    skos:definition ""@en ;
    skos:inScheme piirritev:OsmStatus ;
    skos:prefLabel "Abandoned"@en .

piirritev:OsmStatus a skos:Concept ;
    piirrite:osmId "" ;
    rdfs:subClassOf piirrite:OsmEntity ;
    skos:definition ""@en ;
    skos:inScheme piirritev:OsmStatus ;
    skos:prefLabel ""@en .

piirritev:OsmStepCount a skos:ConceptScheme ;
    piirrite:osmId "step_count" ;
    skos:definition "Number of individual steps in a stair, part of a stair or on a stile."@en ;
    skos:prefLabel "Step count, types"@en .

piirritev:OsmStopAll a skos:Concept ;
    piirrite:osmId "all" ;
    rdfs:subClassOf piirrite:OsmEntity ;
    skos:definition ""@en ;
    skos:inScheme piirritev:OsmStop ;
    skos:prefLabel "All"@en .

piirritev:OsmStructureLattice a skos:Concept ;
    piirrite:osmId "lattice" ;
    rdfs:subClassOf piirrite:OsmEntity ;
    skos:definition ""@en ;
    skos:inScheme piirritev:OsmStructure ;
    skos:prefLabel "Lattice"@en .

piirritev:OsmStructureSolid a skos:Concept ;
    piirrite:osmId "solid" ;
    rdfs:subClassOf piirrite:OsmEntity ;
    skos:definition ""@en ;
    skos:inScheme piirritev:OsmStructure ;
    skos:prefLabel "Solid"@en .

piirritev:OsmStructureTubular a skos:Concept ;
    piirrite:osmId "tubular" ;
    rdfs:subClassOf piirrite:OsmEntity ;
    skos:definition ""@en ;
    skos:inScheme piirritev:OsmStructure ;
    skos:prefLabel "Tubular"@en .

piirritev:OsmSubstanceGas a skos:Concept ;
    piirrite:hasRelatedOsmTag piirrite:hasOsmGasManMade ;
    piirrite:osmId "gas" ;
    rdfs:subClassOf piirrite:OsmEntity ;
    skos:definition "The substance transported in pipelines or processed in related facilities is a natural gas."@en ;
    skos:inScheme piirritev:OsmSubstance ;
    skos:prefLabel "Gas"@en .

piirritev:OsmSubstanceHotWater a skos:Concept ;
    piirrite:hasRelatedOsmTag piirrite:hasOsmHotWaterManMade ;
    piirrite:osmId "hot_water" ;
    rdfs:subClassOf piirrite:OsmEntity ;
    skos:definition "A pipeline in which hot water flows."@en ;
    skos:inScheme piirritev:OsmSubstance ;
    skos:prefLabel "Hot water"@en .

piirritev:OsmSubstanceOil a skos:Concept ;
    piirrite:hasRelatedOsmTag piirrite:hasOsmOilManMade ;
    piirrite:osmId "oil" ;
    rdfs:subClassOf piirrite:OsmEntity ;
    skos:definition "A pipeline in which oil flows."@en ;
    skos:inScheme piirritev:OsmSubstance ;
    skos:prefLabel "Oil"@en .

piirritev:OsmSubstanceWater a skos:Concept ;
    piirrite:hasRelatedOsmTag piirrite:hasOsmWaterManMade ;
    piirrite:osmId "water" ;
    rdfs:subClassOf piirrite:OsmEntity ;
    skos:definition "Fresh water"@en ;
    skos:inScheme piirritev:OsmSubstance ;
    skos:prefLabel "Water"@en .

piirritev:OsmSubstationDistribution a skos:Concept ;
    piirrite:hasRelatedOsmTag piirrite:hasOsmDistributionCompensator,
        piirrite:hasOsmDistributionLocation,
        piirrite:hasOsmDistributionOperator,
        piirrite:hasOsmDistributionPipeline,
        piirrite:hasOsmDistributionPower,
        piirrite:hasOsmDistributionTransformer,
        piirrite:hasOsmDistributionVoltage ;
    piirrite:osmId "distribution" ;
    rdfs:subClassOf piirrite:OsmEntity ;
    skos:definition "Substation that mainly relates to regional distribution networks without any individual subscriber delivery. It often includes sites with regional or local coverage."@en ;
    skos:inScheme piirritev:OsmSubstation ;
    skos:prefLabel "Distribution"@en .

piirritev:OsmSubstationIndustrial a skos:Concept ;
    piirrite:hasRelatedOsmTag piirrite:hasOsmIndustrialLocation,
        piirrite:hasOsmIndustrialOperator,
        piirrite:hasOsmIndustrialPower,
        piirrite:hasOsmIndustrialVoltage ;
    piirrite:osmId "industrial" ;
    rdfs:subClassOf piirrite:OsmEntity ;
    skos:definition "Private space dedicated to industrial or heavy business activities feeding. Each substation of this kind is operated by a given client and not by the traditional public grid company."@en ;
    skos:inScheme piirritev:OsmSubstation ;
    skos:prefLabel "Industrial"@en .

piirritev:OsmSubstationTransmission a skos:Concept ;
    piirrite:hasRelatedOsmTag piirrite:hasOsmTransmissionLocation,
        piirrite:hasOsmTransmissionOperator,
        piirrite:hasOsmTransmissionPower,
        piirrite:hasOsmTransmissionVoltage ;
    piirrite:osmId "transmission" ;
    rdfs:subClassOf piirrite:OsmEntity ;
    skos:definition "A place to connect and switch power transmission lines which transport power between production and consumption places. Inside voltage is mainly over 100 kV."@en ;
    skos:inScheme piirritev:OsmSubstation ;
    skos:prefLabel "Transmission"@en .

piirritev:OsmSupervised a skos:ConceptScheme ;
    piirrite:osmId "supervised" ;
    skos:definition "Indicates whether there is a person who supervises the place"@en ;
    skos:prefLabel "Supervised, types"@en .

piirritev:OsmSupportCeiling a skos:Concept ;
    piirrite:osmId "ceiling" ;
    rdfs:subClassOf piirrite:OsmEntity ;
    skos:definition ""@en ;
    skos:inScheme piirritev:OsmSupport ;
    skos:prefLabel "Ceiling"@en .

piirritev:OsmSupportGround a skos:Concept ;
    piirrite:osmId "ground" ;
    rdfs:subClassOf piirrite:OsmEntity ;
    skos:definition ""@en ;
    skos:inScheme piirritev:OsmSupport ;
    skos:prefLabel "Ground"@en .

piirritev:OsmSupportPole a skos:Concept ;
    piirrite:osmId "pole" ;
    rdfs:subClassOf piirrite:OsmEntity ;
    skos:definition ""@en ;
    skos:inScheme piirritev:OsmSupport ;
    skos:prefLabel "Pole"@en .

piirritev:OsmSupportPowerPole a skos:Concept ;
    piirrite:osmId "power_pole" ;
    rdfs:subClassOf piirrite:OsmEntity ;
    skos:definition ""@en ;
    skos:inScheme piirritev:OsmSupport ;
    skos:prefLabel "Power pole"@en .

piirritev:OsmSupportWall a skos:Concept ;
    piirrite:osmId "wall" ;
    rdfs:subClassOf piirrite:OsmEntity ;
    skos:definition ""@en ;
    skos:inScheme piirritev:OsmSupport ;
    skos:prefLabel "Wall"@en .

piirritev:OsmSupportWallMounted a skos:Concept ;
    piirrite:osmId "wall_mounted" ;
    rdfs:subClassOf piirrite:OsmEntity ;
    skos:definition ""@en ;
    skos:inScheme piirritev:OsmSupport ;
    skos:prefLabel "Wall mounted"@en .

piirritev:OsmSurfaceArtificialTurf a skos:Concept ;
    piirrite:hasRelatedOsmTag piirrite:hasOsmArtificialTurfLeisure ;
    piirrite:osmId "artificial_turf" ;
    rdfs:subClassOf piirrite:OsmEntity ;
    skos:definition "A surface made from synthetic materials to look and feel like natural grass. Often used for tracks and pitches of sports such as football, baseball, etc."@en ;
    skos:inScheme piirritev:OsmSurface ;
    skos:prefLabel "Artificial turf"@en .

piirritev:OsmSurfaceAsphalt a skos:Concept ;
    piirrite:osmId "asphalt" ;
    rdfs:subClassOf piirrite:OsmEntity ;
    skos:definition "Specifies that object is paved with asphalt concrete."@en ;
    skos:inScheme piirritev:OsmSurface ;
    skos:prefLabel "Asphalt"@en .

piirritev:OsmSurfaceClay a skos:Concept ;
    piirrite:hasRelatedOsmTag piirrite:hasOsmClayLeisure ;
    piirrite:osmId "clay" ;
    rdfs:subClassOf piirrite:OsmEntity ;
    skos:definition "A tennis court surface made of crushed stone, brick, shale, or other unbound mineral aggregate."@en ;
    skos:inScheme piirritev:OsmSurface ;
    skos:prefLabel "Clay"@en .

piirritev:OsmSurfaceCobblestone a skos:Concept ;
    piirrite:hasRelatedOsmTag piirrite:hasOsmCobblestoneHighway ;
    piirrite:osmId "cobblestone" ;
    rdfs:subClassOf piirrite:OsmEntity ;
    skos:definition "Generic value for cobblestone, used for both sett and true cobblestone."@en ;
    skos:inScheme piirritev:OsmSurface ;
    skos:prefLabel "Cobblestone"@en .

piirritev:OsmSurfaceCompacted a skos:Concept ;
    piirrite:hasRelatedOsmTag piirrite:hasOsmCompactedHighway,
        piirrite:hasOsmCompactedSmoothness,
        piirrite:hasOsmCompactedTracktype ;
    piirrite:osmId "compacted" ;
    rdfs:subClassOf piirrite:OsmEntity ;
    skos:definition "Surface made of artificially compacted gravel and sand."@en ;
    skos:inScheme piirritev:OsmSurface ;
    skos:prefLabel "Compacted"@en .

piirritev:OsmSurfaceConcrete a skos:Concept ;
    piirrite:osmId "concrete" ;
    rdfs:subClassOf piirrite:OsmEntity ;
    skos:definition "A surface of cement based concrete, cast in place. osmcarto-rendering="@en ;
    skos:inScheme piirritev:OsmSurface ;
    skos:prefLabel "Concrete"@en .

piirritev:OsmSurfaceDirt a skos:Concept ;
    piirrite:osmId "dirt" ;
    rdfs:subClassOf piirrite:OsmEntity ;
    skos:definition "Used for where surface is exposed earth/soil/dirt but it is not sand or gravel or rock."@en ;
    skos:inScheme piirritev:OsmSurface ;
    skos:prefLabel "Dirt"@en .

piirritev:OsmSurfaceEarth a skos:Concept ;
    piirrite:osmId "earth" ;
    rdfs:subClassOf piirrite:OsmEntity ;
    skos:definition "Used for where surface is exposed earth/soil/dirt but it is not sand or gravel or rock."@en ;
    skos:inScheme piirritev:OsmSurface ;
    skos:prefLabel "Earth"@en .

piirritev:OsmSurfaceFineGravel a skos:Concept ;
    piirrite:hasRelatedOsmTag piirrite:hasOsmFineGravelHighway,
        piirrite:hasOsmFineGravelSmoothness ;
    piirrite:osmId "fine_gravel" ;
    rdfs:subClassOf piirrite:OsmEntity ;
    skos:definition "Loose, small gravel, not compacted, typically used on paths and driveways with minimal traffic."@en ;
    skos:inScheme piirritev:OsmSurface ;
    skos:prefLabel "Fine gravel"@en .

piirritev:OsmSurfaceGrass a skos:Concept ;
    piirrite:osmId "grass" ;
    rdfs:subClassOf piirrite:OsmEntity ;
    skos:definition "Specifies that object has grass as a surface."@en ;
    skos:inScheme piirritev:OsmSurface ;
    skos:prefLabel "Grass"@en .

piirritev:OsmSurfaceGrassPaver a skos:Concept ;
    piirrite:osmId "grass_paver" ;
    rdfs:subClassOf piirrite:OsmEntity ;
    skos:definition "Specifies that object is paved with grass paver  paving with large deliberate voids in it."@en ;
    skos:inScheme piirritev:OsmSurface ;
    skos:prefLabel "Grass paver"@en .

piirritev:OsmSurfaceGravel a skos:Concept ;
    piirrite:osmId "gravel" ;
    rdfs:subClassOf piirrite:OsmEntity ;
    skos:definition "This tag has very large meaning range. Used for cases ranging from huge gravel pieces like track ballast used as surface, through small pieces of gravel to compacted surface."@en ;
    skos:inScheme piirritev:OsmSurface ;
    skos:prefLabel "Gravel"@en .

piirritev:OsmSurfaceGround a skos:Concept ;
    piirrite:osmId "ground" ;
    rdfs:subClassOf piirrite:OsmEntity ;
    skos:definition "No special surface, the ground itself has marks of human or animal usage. This value gives only a rough description; if possible, use a more precise value such as grass, clay, sand, earth, gravel or pebblestone."@en ;
    skos:inScheme piirritev:OsmSurface ;
    skos:prefLabel "Ground"@en .

piirritev:OsmSurfaceMetal a skos:Concept ;
    piirrite:osmId "metal" ;
    rdfs:subClassOf piirrite:OsmEntity ;
    skos:definition "Used for metal-surfaced bridges, or for temporary tracks over fields for normal road vehicles or site traffic."@en ;
    skos:inScheme piirritev:OsmSurface ;
    skos:prefLabel "Metal"@en .

piirritev:OsmSurfaceMud a skos:Concept ;
    piirrite:osmId "mud" ;
    rdfs:subClassOf piirrite:OsmEntity ;
    skos:definition "Specifies that object has mud as a surface  all the time or at least very frequently."@en ;
    skos:inScheme piirritev:OsmSurface ;
    skos:prefLabel "Mud"@en .

piirritev:OsmSurfacePaved a skos:Concept ;
    piirrite:osmId "paved" ;
    rdfs:subClassOf piirrite:OsmEntity ;
    skos:definition "Describes the surface of a feature roughly as predominantly paved over the whole surface area; i.e., covered with paving stones, concrete, bitumen or asphalt. This value gives only a rough description; use a more precise value if possible."@en ;
    skos:inScheme piirritev:OsmSurface ;
    skos:prefLabel "Paved"@en .

piirritev:OsmSurfacePavingStones a skos:Concept ;
    piirrite:osmId "paving_stones" ;
    rdfs:subClassOf piirrite:OsmEntity ;
    skos:definition "A surface paved with artificial blocks (block pavers, bricks) or natural stones (flagstones), with a flat top."@en ;
    skos:inScheme piirritev:OsmSurface ;
    skos:prefLabel "Paving stones"@en .

piirritev:OsmSurfacePebblestone a skos:Concept ;
    piirrite:hasRelatedOsmTag piirrite:hasOsmPebblestoneHighway,
        piirrite:hasOsmPebblestoneNatural,
        piirrite:hasOsmPebblestoneSmoothness ;
    piirrite:osmId "pebblestone" ;
    rdfs:subClassOf piirrite:OsmEntity ;
    skos:definition " image = File:Pebbleswithquarzite.jpg"@en ;
    skos:inScheme piirritev:OsmSurface ;
    skos:prefLabel "Pebblestone"@en .

piirritev:OsmSurfaceRock a skos:Concept ;
    piirrite:hasRelatedOsmTag piirrite:hasOsmRockHighway,
        piirrite:hasOsmRockMaterial ;
    piirrite:osmId "rock" ;
    rdfs:subClassOf piirrite:OsmEntity ;
    skos:definition "Rocky surface of path or other similar object"@en ;
    skos:inScheme piirritev:OsmSurface ;
    skos:prefLabel "Rock"@en .

piirritev:OsmSurfaceSand a skos:Concept ;
    piirrite:osmId "sand" ;
    rdfs:subClassOf piirrite:OsmEntity ;
    skos:definition "Specifies that object has sand as a surface."@en ;
    skos:inScheme piirritev:OsmSurface ;
    skos:prefLabel "Sand"@en .

piirritev:OsmSurfaceSett a skos:Concept ;
    piirrite:hasRelatedOsmTag piirrite:hasOsmSettHighway ;
    piirrite:osmId "sett" ;
    rdfs:subClassOf piirrite:OsmEntity ;
    skos:definition "Sett paving, formed from natural stones cut to have a flat top (with regular or irregular shape)."@en ;
    skos:inScheme piirritev:OsmSurface ;
    skos:prefLabel "Sett"@en .

piirritev:OsmSurfaceStone a skos:Concept ;
    piirrite:hasRelatedOsmTag piirrite:hasOsmStoneMaterial ;
    piirrite:osmId "stone" ;
    rdfs:subClassOf piirrite:OsmEntity ;
    skos:definition "Specifies that object is paved with stone"@en ;
    skos:inScheme piirritev:OsmSurface ;
    skos:prefLabel "Stone"@en .

piirritev:OsmSurfaceSurvey a skos:ConceptScheme ;
    piirrite:osmId "surface_survey" ;
    skos:definition "Used to indicate the date when the surface feature of a highway was surveyed and tagged, mainly in Romania."@en ;
    skos:prefLabel "Surface survey, types"@en .

piirritev:OsmSurfaceTartan a skos:Concept ;
    piirrite:hasRelatedOsmTag piirrite:hasOsmTartanLeisure ;
    piirrite:osmId "tartan" ;
    rdfs:subClassOf piirrite:OsmEntity ;
    skos:definition "A synthetic, all-weather surface typically used in running."@en ;
    skos:inScheme piirritev:OsmSurface ;
    skos:prefLabel "Tartan"@en .

piirritev:OsmSurfaceUnhewnCobblestone a skos:Concept ;
    piirrite:osmId "unhewn_cobblestone" ;
    rdfs:subClassOf piirrite:OsmEntity ;
    skos:definition "Raw cobblestone of natural, uncut, rounded stones."@en ;
    skos:inScheme piirritev:OsmSurface ;
    skos:prefLabel "Unhewn cobblestone"@en .

piirritev:OsmSurfaceUnpaved a skos:Concept ;
    piirrite:hasRelatedOsmTag piirrite:hasOsmUnpavedHighway,
        piirrite:hasOsmUnpavedSmoothness ;
    piirrite:osmId "unpaved" ;
    rdfs:subClassOf piirrite:OsmEntity ;
    skos:definition "Indicates that the feature has an unpaved surface, such as gravel or grass."@en ;
    skos:inScheme piirritev:OsmSurface ;
    skos:prefLabel "Unpaved"@en .

piirritev:OsmSurfaceWood a skos:Concept ;
    piirrite:osmId "wood" ;
    rdfs:subClassOf piirrite:OsmEntity ;
    skos:definition "Object with wooden surface. Used for bridges, plank walkways, and garden decking."@en ;
    skos:inScheme piirritev:OsmSurface ;
    skos:prefLabel "Wood"@en .

piirritev:OsmSurfaceWoodchips a skos:Concept ;
    piirrite:osmId "woodchips" ;
    rdfs:subClassOf piirrite:OsmEntity ;
    skos:definition "Specifies that object has woodchips as a surface."@en ;
    skos:inScheme piirritev:OsmSurface ;
    skos:prefLabel "Woodchips"@en .

piirritev:OsmSurveillanceIndoor a skos:Concept ;
    piirrite:osmId "indoor" ;
    rdfs:subClassOf piirrite:OsmEntity ;
    skos:definition ""@en ;
    skos:inScheme piirritev:OsmSurveillance ;
    skos:prefLabel "Indoor"@en .

piirritev:OsmSurveillanceOutdoor a skos:Concept ;
    piirrite:osmId "outdoor" ;
    rdfs:subClassOf piirrite:OsmEntity ;
    skos:definition ""@en ;
    skos:inScheme piirritev:OsmSurveillance ;
    skos:prefLabel "Outdoor"@en .

piirritev:OsmSurveillancePublic a skos:Concept ;
    piirrite:osmId "public" ;
    rdfs:subClassOf piirrite:OsmEntity ;
    skos:definition ""@en ;
    skos:inScheme piirritev:OsmSurveillance ;
    skos:prefLabel "Public"@en .

piirritev:OsmSurveillanceTraffic a skos:Concept ;
    piirrite:osmId "traffic" ;
    rdfs:subClassOf piirrite:OsmEntity ;
    skos:definition ""@en ;
    skos:inScheme piirritev:OsmSurveillance ;
    skos:prefLabel "Traffic"@en .

piirritev:OsmSwimmingPoolInground a skos:Concept ;
    piirrite:osmId "inground" ;
    rdfs:subClassOf piirrite:OsmEntity ;
    skos:definition ""@en ;
    skos:inScheme piirritev:OsmSwimmingPool ;
    skos:prefLabel "Inground"@en .

piirritev:OsmSwimmingPoolOutdoor a skos:Concept ;
    piirrite:osmId "outdoor" ;
    rdfs:subClassOf piirrite:OsmEntity ;
    skos:definition ""@en ;
    skos:inScheme piirritev:OsmSwimmingPool ;
    skos:prefLabel "Outdoor"@en .

piirritev:OsmSwimmingPoolPersonal a skos:Concept ;
    piirrite:osmId "personal" ;
    rdfs:subClassOf piirrite:OsmEntity ;
    skos:definition ""@en ;
    skos:inScheme piirritev:OsmSwimmingPool ;
    skos:prefLabel "Personal"@en .

piirritev:OsmSwitchCircuitBreaker a skos:Concept ;
    piirrite:hasRelatedOsmTag piirrite:hasOsmCircuitBreakerCables,
        piirrite:hasOsmCircuitBreakerOperator,
        piirrite:hasOsmCircuitBreakerPower,
        piirrite:hasOsmCircuitBreakerVoltage ;
    piirrite:osmId "circuit_breaker" ;
    rdfs:subClassOf piirrite:OsmEntity ;
    skos:definition "A circuit-breaker is the only kind of power switch which offers enough protection (safety) against abnormal power currents and can be operated when bound circuit is loaded."@en ;
    skos:inScheme piirritev:OsmSwitch ;
    skos:prefLabel "Circuit breaker"@en .

piirritev:OsmSwitchDisconnector a skos:Concept ;
    piirrite:hasRelatedOsmTag piirrite:hasOsmDisconnectorCables,
        piirrite:hasOsmDisconnectorOperator,
        piirrite:hasOsmDisconnectorPower,
        piirrite:hasOsmDisconnectorVoltage ;
    piirrite:osmId "disconnector" ;
    rdfs:subClassOf piirrite:OsmEntity ;
    skos:definition "A disconnector is capable to open circuits when a negligible current have to be broken. It provides a sufficient protection to high voltages when open but mustn't be operated when the power circuit is loaded."@en ;
    skos:inScheme piirritev:OsmSwitch ;
    skos:prefLabel "Disconnector"@en .

piirritev:OsmSwitchMechanical a skos:Concept ;
    piirrite:hasRelatedOsmTag piirrite:hasOsmMechanicalCables,
        piirrite:hasOsmMechanicalOperator,
        piirrite:hasOsmMechanicalPower,
        piirrite:hasOsmMechanicalVoltage ;
    piirrite:osmId "mechanical" ;
    rdfs:subClassOf piirrite:OsmEntity ;
    skos:definition "A mechanical switch is the most common form of power switch devices. Such a switch can carry normal currents and currents under abnormal specification but only breaks the first one."@en ;
    skos:inScheme piirritev:OsmSwitch ;
    skos:prefLabel "Mechanical"@en .

piirritev:OsmSymbol a skos:ConceptScheme ;
    piirrite:osmId "symbol" ;
    skos:definition "Human-readable description of route symbols that are used as waymarkers or on guideposts. In the context of road markings also used to specify symbolic road markings."@en ;
    skos:prefLabel "Symbol, types"@en .

piirritev:OsmTactilePavingContrasted a skos:Concept ;
    piirrite:osmId "contrasted" ;
    rdfs:subClassOf piirrite:OsmEntity ;
    skos:definition ""@en ;
    skos:inScheme piirritev:OsmTactilePaving ;
    skos:prefLabel "Contrasted"@en .

piirritev:OsmTactilePavingIncorrect a skos:Concept ;
    piirrite:osmId "incorrect" ;
    rdfs:subClassOf piirrite:OsmEntity ;
    skos:definition "Indicates incorrect tactile paving."@en ;
    skos:inScheme piirritev:OsmTactilePaving ;
    skos:prefLabel "Incorrect"@en .

piirritev:OsmTakeawayOnly a skos:Concept ;
    piirrite:osmId "only" ;
    rdfs:subClassOf piirrite:OsmEntity ;
    skos:definition ""@en ;
    skos:inScheme piirritev:OsmTakeaway ;
    skos:prefLabel "Only"@en .

piirritev:OsmTaxonAesculusHippocastanum a skos:Concept ;
    piirrite:osmId "Aesculus_hippocastanum" ;
    rdfs:subClassOf piirrite:OsmEntity ;
    skos:definition ""@en ;
    skos:inScheme piirritev:OsmTaxon ;
    skos:prefLabel "Aesculus hippocastanum"@en .

piirritev:OsmTaxonArecaceae a skos:Concept ;
    piirrite:osmId "Arecaceae" ;
    rdfs:subClassOf piirrite:OsmEntity ;
    skos:definition "a palm tree also known as Arecaceae or Palmae"@en ;
    skos:inScheme piirritev:OsmTaxon ;
    skos:prefLabel "Arecaceae"@en .

piirritev:OsmTidal a skos:ConceptScheme ;
    piirrite:osmId "tidal" ;
    skos:definition "An area in the tidal range."@en ;
    skos:prefLabel "Tidal, types"@en .

piirritev:OsmTo a skos:ConceptScheme ;
    piirrite:osmId "to" ;
    skos:definition "Destination station."@en ;
    skos:prefLabel "To, types"@en .

piirritev:OsmToilets a skos:ConceptScheme ;
    piirrite:osmId "toilets" ;
    skos:definition "Indicates if a feature has a toilet."@en ;
    skos:prefLabel "Toilets, types"@en .

piirritev:OsmToll a skos:ConceptScheme ;
    piirrite:osmId "toll" ;
    skos:definition "Toll roads charge money for general traffic."@en ;
    skos:prefLabel "Toll, types"@en .

piirritev:OsmTourismAlpineHut a skos:Concept ;
    piirrite:hasRelatedOsmTag piirrite:hasOsmAlpineHutEle,
        piirrite:hasOsmAlpineHutName ;
    piirrite:osmId "alpine_hut" ;
    rdfs:subClassOf piirrite:OsmEntity ;
    skos:definition "A remote building located in the mountains intended to provide board and lodging. osmcarto-rendering=File:Alpinehut.svg osmcarto-rendering-size=28px"@en ;
    skos:inScheme piirritev:OsmTourism ;
    skos:prefLabel "Alpine hut"@en .

piirritev:OsmTourismApartment a skos:Concept ;
    piirrite:hasRelatedOsmTag piirrite:hasOsmApartmentBalcony,
        piirrite:hasOsmApartmentBrand,
        piirrite:hasOsmApartmentCapacity,
        piirrite:hasOsmApartmentEmail,
        piirrite:hasOsmApartmentInternetAccess,
        piirrite:hasOsmApartmentOpeningHours,
        piirrite:hasOsmApartmentOperator,
        piirrite:hasOsmApartmentPhone,
        piirrite:hasOsmApartmentWebsite ;
    piirrite:osmId "apartment" ;
    rdfs:subClassOf piirrite:OsmEntity ;
    skos:definition "A furnished apartment or flat with cooking and bathroom facilities that can be rented for holiday vacations. osmcarto-rendering=File:Apartment.svg osmcarto-rendering-size=28px"@en ;
    skos:inScheme piirritev:OsmTourism ;
    skos:prefLabel "Apartment"@en .

piirritev:OsmTourismArtwork a skos:Concept ;
    piirrite:hasRelatedOsmTag piirrite:hasOsmArtworkArtistName,
        piirrite:hasOsmArtworkArtworkSubject,
        piirrite:hasOsmArtworkArtworkType,
        piirrite:hasOsmArtworkDescription,
        piirrite:hasOsmArtworkHeight,
        piirrite:hasOsmArtworkHeritage,
        piirrite:hasOsmArtworkImage,
        piirrite:hasOsmArtworkInscription,
        piirrite:hasOsmArtworkLocation,
        piirrite:hasOsmArtworkMaterial,
        piirrite:hasOsmArtworkName,
        piirrite:hasOsmArtworkStartDate,
        piirrite:hasOsmArtworkSupport,
        piirrite:hasOsmArtworkType,
        piirrite:hasOsmArtworkWebsite,
        piirrite:hasOsmArtworkWikidata,
        piirrite:hasOsmArtworkWikipedia ;
    piirrite:osmId "artwork" ;
    rdfs:subClassOf piirrite:OsmEntity ;
    skos:definition "A public piece of art. osmcarto-rendering=File:Artwork-14.svg osmcarto-rendering-size=28px"@en ;
    skos:inScheme piirritev:OsmTourism ;
    skos:prefLabel "Artwork"@en .

piirritev:OsmTourismAttraction a skos:Concept ;
    piirrite:hasRelatedOsmTag piirrite:hasOsmAttractionName ;
    piirrite:osmId "attraction" ;
    rdfs:subClassOf piirrite:OsmEntity ;
    skos:definition "An object of interest for a tourist, or a purpose-built tourist attraction"@en ;
    skos:inScheme piirritev:OsmTourism ;
    skos:prefLabel "Attraction"@en .

piirritev:OsmTourismCampPitch a skos:Concept ;
    piirrite:hasRelatedOsmTag piirrite:hasOsmCampPitchRef ;
    piirrite:osmId "camp_pitch" ;
    rdfs:subClassOf piirrite:OsmEntity ;
    skos:definition "A tent or caravan pitch location within a campsite or caravan site."@en ;
    skos:inScheme piirritev:OsmTourism ;
    skos:prefLabel "Camp pitch"@en .

piirritev:OsmTourismCampSite a skos:Concept ;
    piirrite:hasRelatedOsmTag piirrite:hasOsmCampSiteName,
        piirrite:hasOsmCampSiteOperator,
        piirrite:hasOsmCampSitePhone,
        piirrite:hasOsmCampSiteWebsite ;
    piirrite:osmId "camp_site" ;
    rdfs:subClassOf piirrite:OsmEntity ;
    skos:definition "An area where people can camp overnight using tents, camper vans, or caravans. osmcarto-rendering=File:Camping.16.svg osmcarto-rendering-size=28px osmcarto-rendering-area = File:Area_tourism%3Dcampsite.png osmcarto-rendering-area-size = 100px"@en ;
    skos:inScheme piirritev:OsmTourism ;
    skos:prefLabel "Camp site"@en .

piirritev:OsmTourismCaravanSite a skos:Concept ;
    piirrite:hasRelatedOsmTag piirrite:hasOsmCaravanSiteCapacity,
        piirrite:hasOsmCaravanSiteFee,
        piirrite:hasOsmCaravanSiteName,
        piirrite:hasOsmCaravanSitePowerSupply,
        piirrite:hasOsmCaravanSiteWebsite ;
    piirrite:osmId "caravan_site" ;
    rdfs:subClassOf piirrite:OsmEntity ;
    skos:definition "A place where you can stay in a caravan overnight or for longer periods."@en ;
    skos:inScheme piirritev:OsmTourism ;
    skos:prefLabel "Caravan site"@en .

piirritev:OsmTourismChalet a skos:Concept ;
    piirrite:hasRelatedOsmTag piirrite:hasOsmChaletAddr,
        piirrite:hasOsmChaletBrand,
        piirrite:hasOsmChaletBuilding,
        piirrite:hasOsmChaletClub,
        piirrite:hasOsmChaletEmail,
        piirrite:hasOsmChaletInternetAccess,
        piirrite:hasOsmChaletOperator,
        piirrite:hasOsmChaletPetsAllowed,
        piirrite:hasOsmChaletPhone,
        piirrite:hasOsmChaletWebsite ;
    piirrite:osmId "chalet" ;
    rdfs:subClassOf piirrite:OsmEntity ;
    skos:definition "A holiday cottage with self-contained cooking and bathroom facilities. osmcarto-rendering=File:Chalet.svg osmcarto-rendering-size=28px"@en ;
    skos:inScheme piirritev:OsmTourism ;
    skos:prefLabel "Chalet"@en .

piirritev:OsmTourismGallery a skos:Concept ;
    piirrite:hasRelatedOsmTag piirrite:hasOsmGalleryFee,
        piirrite:hasOsmGalleryName,
        piirrite:hasOsmGalleryOpeningHours,
        piirrite:hasOsmGalleryOperator,
        piirrite:hasOsmGalleryPhone,
        piirrite:hasOsmGalleryWebsite,
        piirrite:hasOsmGalleryWheelchair ;
    piirrite:osmId "gallery" ;
    rdfs:subClassOf piirrite:OsmEntity ;
    skos:definition "An area or building that displays a variety of visual art exhibitions."@en ;
    skos:inScheme piirritev:OsmTourism ;
    skos:prefLabel "Gallery"@en .

piirritev:OsmTourismGuestHouse a skos:Concept ;
    piirrite:hasRelatedOsmTag piirrite:hasOsmGuestHouseName,
        piirrite:hasOsmGuestHouseOperator ;
    piirrite:osmId "guest_house" ;
    rdfs:subClassOf piirrite:OsmEntity ;
    skos:definition "Accommodation smaller than a hotel and typically owner-operated, such as bed&breakfasts etc. osmcarto-rendering=File:Tourism guest house.svg osmcarto-rendering-size=28px"@en ;
    skos:inScheme piirritev:OsmTourism ;
    skos:prefLabel "Guest house"@en .

piirritev:OsmTourismHostel a skos:Concept ;
    piirrite:hasRelatedOsmTag piirrite:hasOsmHostelName,
        piirrite:hasOsmHostelOperator ;
    piirrite:osmId "hostel" ;
    rdfs:subClassOf piirrite:OsmEntity ;
    skos:definition "Cheap accommodation with shared bedrooms. osmcarto-rendering=File:Hostel-16.svg osmcarto-rendering-size=28px"@en ;
    skos:inScheme piirritev:OsmTourism ;
    skos:prefLabel "Hostel"@en .

piirritev:OsmTourismHotel a skos:Concept ;
    piirrite:hasRelatedOsmTag piirrite:hasOsmHotelAirConditioning,
        piirrite:hasOsmHotelBeds,
        piirrite:hasOsmHotelBrand,
        piirrite:hasOsmHotelBuilding,
        piirrite:hasOsmHotelCheckIn,
        piirrite:hasOsmHotelCheckOut,
        piirrite:hasOsmHotelDisused,
        piirrite:hasOsmHotelDryer,
        piirrite:hasOsmHotelInternetAccess,
        piirrite:hasOsmHotelName,
        piirrite:hasOsmHotelOldName,
        piirrite:hasOsmHotelOpeningHours,
        piirrite:hasOsmHotelOperator,
        piirrite:hasOsmHotelPhone,
        piirrite:hasOsmHotelReservation,
        piirrite:hasOsmHotelRooms,
        piirrite:hasOsmHotelService,
        piirrite:hasOsmHotelSmoking,
        piirrite:hasOsmHotelStars,
        piirrite:hasOsmHotelSwimmingPool,
        piirrite:hasOsmHotelWashingMachine,
        piirrite:hasOsmHotelWebsite,
        piirrite:hasOsmHotelWheelchair ;
    piirrite:osmId "hotel" ;
    rdfs:subClassOf piirrite:OsmEntity ;
    skos:definition "Hotel  an establishment that provides paid lodging. osmcarto-rendering=File:Hotel-16.svg osmcarto-rendering-size=28px"@en ;
    skos:inScheme piirritev:OsmTourism ;
    skos:prefLabel "Hotel"@en .

piirritev:OsmTourismInformation a skos:Concept ;
    piirrite:hasRelatedOsmTag piirrite:hasOsmInformationDescription,
        piirrite:hasOsmInformationName ;
    piirrite:osmId "information" ;
    rdfs:subClassOf piirrite:OsmEntity ;
    skos:definition "Information for tourists and visitors, including information offices"@en ;
    skos:inScheme piirritev:OsmTourism ;
    skos:prefLabel "Information"@en .

piirritev:OsmTourismMotel a skos:Concept ;
    piirrite:hasRelatedOsmTag piirrite:hasOsmMotelName,
        piirrite:hasOsmMotelOperator ;
    piirrite:osmId "motel" ;
    rdfs:subClassOf piirrite:OsmEntity ;
    skos:definition "Short term accommodation, particularly for people travelling by car. osmcarto-rendering=File:Motel-16.svg osmcarto-rendering-size=28px"@en ;
    skos:inScheme piirritev:OsmTourism ;
    skos:prefLabel "Motel"@en .

piirritev:OsmTourismMuseum a skos:Concept ;
    piirrite:hasRelatedOsmTag piirrite:hasOsmMuseumName,
        piirrite:hasOsmMuseumOpeningHours,
        piirrite:hasOsmMuseumOperator,
        piirrite:hasOsmMuseumType ;
    piirrite:osmId "museum" ;
    rdfs:subClassOf piirrite:OsmEntity ;
    skos:definition "A museum: an institution with exhibitions on scientific, historical, cultural topics osmcarto-rendering=File:Museum-16.svg osmcarto-rendering-size=28px"@en ;
    skos:inScheme piirritev:OsmTourism ;
    skos:prefLabel "Museum"@en .

piirritev:OsmTourismPicnicSite a skos:Concept ;
    piirrite:hasRelatedOsmTag piirrite:hasOsmPicnicSiteBbq,
        piirrite:hasOsmPicnicSiteCovered,
        piirrite:hasOsmPicnicSiteDrinkingWater,
        piirrite:hasOsmPicnicSiteFirepit,
        piirrite:hasOsmPicnicSiteFireplace,
        piirrite:hasOsmPicnicSiteOpenfire ;
    piirrite:osmId "picnic_site" ;
    rdfs:subClassOf piirrite:OsmEntity ;
    skos:definition "A locality that is suitable for outdoors eating, with facilities to aid a picnic such as tables and benches. osmcarto-rendering = File:Picnic site.svg osmcarto-rendering-size = 28px osmcarto-rendering-area=File:Area tourism=campsite.png osmcarto-rendering-area-size=125px"@en ;
    skos:inScheme piirritev:OsmTourism ;
    skos:prefLabel "Picnic site"@en .

piirritev:OsmTourismThemePark a skos:Concept ;
    piirrite:hasRelatedOsmTag piirrite:hasOsmThemeParkName,
        piirrite:hasOsmThemeParkOpeningHours,
        piirrite:hasOsmThemeParkOperator ;
    piirrite:osmId "theme_park" ;
    rdfs:subClassOf piirrite:OsmEntity ;
    skos:definition "An amusement park where entertainment is provided by rides, games, concessions. osmcarto-rendering=File:Rendering-theme park.png osmcarto-rendering-size=125px"@en ;
    skos:inScheme piirritev:OsmTourism ;
    skos:prefLabel "Theme park"@en .

piirritev:OsmTourismViewpoint a skos:Concept ;
    piirrite:hasRelatedOsmTag piirrite:hasOsmViewpointDescription,
        piirrite:hasOsmViewpointDirection,
        piirrite:hasOsmViewpointManMade,
        piirrite:hasOsmViewpointName,
        piirrite:hasOsmViewpointNatural ;
    piirrite:osmId "viewpoint" ;
    rdfs:subClassOf piirrite:OsmEntity ;
    skos:definition "A place worth visiting, often high, with a good view of surrounding countryside or notable buildings. osmcarto-rendering=File:Viewpoint-16.svg osmcarto-rendering-size=28px"@en ;
    skos:inScheme piirritev:OsmTourism ;
    skos:prefLabel "Viewpoint"@en .

piirritev:OsmTourismWildernessHut a skos:Concept ;
    piirrite:hasRelatedOsmTag piirrite:hasOsmWildernessHutAccess,
        piirrite:hasOsmWildernessHutCapacity,
        piirrite:hasOsmWildernessHutDescription,
        piirrite:hasOsmWildernessHutEle,
        piirrite:hasOsmWildernessHutFee,
        piirrite:hasOsmWildernessHutFireplace,
        piirrite:hasOsmWildernessHutOperator ;
    piirrite:osmId "wilderness_hut" ;
    rdfs:subClassOf piirrite:OsmEntity ;
    skos:definition "A remote building, typically unserviced, providing temporary shelter and sleeping accommodation. osmcarto-rendering=File:Wilderness hut.svg osmcarto-rendering-size=28px"@en ;
    skos:inScheme piirritev:OsmTourism ;
    skos:prefLabel "Wilderness hut"@en .

piirritev:OsmTracks a skos:ConceptScheme ;
    piirrite:osmId "tracks" ;
    skos:definition "Number of tracks which are represented by this way"@en ;
    skos:prefLabel "Tracks, types"@en .

piirritev:OsmTrafficSignCityLimit a skos:Concept ;
    piirrite:hasRelatedOsmTag piirrite:hasOsmCityLimitDirection,
        piirrite:hasOsmCityLimitName ;
    piirrite:osmId "city_limit" ;
    rdfs:subClassOf piirrite:OsmEntity ;
    skos:definition "City-limit sign"@en ;
    skos:inScheme piirritev:OsmTrafficSign ;
    skos:prefLabel "City limit"@en .

piirritev:OsmTrafficSignMaxspeed a skos:Concept ;
    piirrite:osmId "maxspeed" ;
    rdfs:subClassOf piirrite:OsmEntity ;
    skos:definition ""@en ;
    skos:inScheme piirritev:OsmTrafficSign ;
    skos:prefLabel "Maxspeed"@en .

piirritev:OsmTrafficSignStop a skos:Concept ;
    piirrite:osmId "stop" ;
    rdfs:subClassOf piirrite:OsmEntity ;
    skos:definition ""@en ;
    skos:inScheme piirritev:OsmTrafficSign ;
    skos:prefLabel "Stop"@en .

piirritev:OsmTrafficSignalsPedestrianCrossing a skos:Concept ;
    piirrite:osmId "pedestrian_crossing" ;
    rdfs:subClassOf piirrite:OsmEntity ;
    skos:definition ""@en ;
    skos:inScheme piirritev:OsmTrafficSignals ;
    skos:prefLabel "Pedestrian crossing"@en .

piirritev:OsmTrafficSignalsSignal a skos:Concept ;
    piirrite:osmId "signal" ;
    rdfs:subClassOf piirrite:OsmEntity ;
    skos:definition ""@en ;
    skos:inScheme piirritev:OsmTrafficSignals ;
    skos:prefLabel "Signal"@en .

piirritev:OsmTrafficSignalsTrafficLights a skos:Concept ;
    piirrite:osmId "traffic_lights" ;
    rdfs:subClassOf piirrite:OsmEntity ;
    skos:definition ""@en ;
    skos:inScheme piirritev:OsmTrafficSignals ;
    skos:prefLabel "Traffic lights"@en .

piirritev:OsmTrailVisibilityBad a skos:Concept ;
    piirrite:osmId "bad" ;
    rdfs:subClassOf piirrite:OsmEntity ;
    skos:definition ""@en ;
    skos:inScheme piirritev:OsmTrailVisibility ;
    skos:prefLabel "Bad"@en .

piirritev:OsmTrailVisibilityExcellent a skos:Concept ;
    piirrite:osmId "excellent" ;
    rdfs:subClassOf piirrite:OsmEntity ;
    skos:definition ""@en ;
    skos:inScheme piirritev:OsmTrailVisibility ;
    skos:prefLabel "Excellent"@en .

piirritev:OsmTrailVisibilityGood a skos:Concept ;
    piirrite:osmId "good" ;
    rdfs:subClassOf piirrite:OsmEntity ;
    skos:definition ""@en ;
    skos:inScheme piirritev:OsmTrailVisibility ;
    skos:prefLabel "Good"@en .

piirritev:OsmTrailVisibilityHorrible a skos:Concept ;
    piirrite:osmId "horrible" ;
    rdfs:subClassOf piirrite:OsmEntity ;
    skos:definition ""@en ;
    skos:inScheme piirritev:OsmTrailVisibility ;
    skos:prefLabel "Horrible"@en .

piirritev:OsmTrailVisibilityIntermediate a skos:Concept ;
    piirrite:osmId "intermediate" ;
    rdfs:subClassOf piirrite:OsmEntity ;
    skos:definition ""@en ;
    skos:inScheme piirritev:OsmTrailVisibility ;
    skos:prefLabel "Intermediate"@en .

piirritev:OsmTrailblazedSymbols a skos:Concept ;
    piirrite:osmId "symbols" ;
    rdfs:subClassOf piirrite:OsmEntity ;
    skos:definition ""@en ;
    skos:inScheme piirritev:OsmTrailblazed ;
    skos:prefLabel "Symbols"@en .

piirritev:OsmTrain a skos:ConceptScheme ;
    piirrite:osmId "train" ;
    skos:definition "Specifies whether trains stop at a feature"@en ;
    skos:prefLabel "Train, types"@en .

piirritev:OsmTram a skos:ConceptScheme ;
    piirrite:osmId "tram" ;
    skos:definition "Specifies whether trams stop at a feature"@en ;
    skos:prefLabel "Tram, types"@en .

piirritev:OsmTransformerDistribution a skos:Concept ;
    piirrite:hasRelatedOsmTag piirrite:hasOsmDistributionFrequency,
        piirrite:hasOsmDistributionOperator,
        piirrite:hasOsmDistributionPhases,
        piirrite:hasOsmDistributionRating ;
    piirrite:osmId "distribution" ;
    rdfs:subClassOf piirrite:OsmEntity ;
    skos:definition "A standalone distribution transformer transfers power from the distribution grid to directly connected electricity consumers. Installed outside of any substation."@en ;
    skos:inScheme piirritev:OsmTransformer ;
    skos:prefLabel "Distribution"@en .

piirritev:OsmTransformerMain a skos:Concept ;
    piirrite:hasRelatedOsmTag piirrite:hasOsmMainFrequency,
        piirrite:hasOsmMainOperator,
        piirrite:hasOsmMainPhases,
        piirrite:hasOsmMainRating ;
    piirrite:osmId "main" ;
    rdfs:subClassOf piirrite:OsmEntity ;
    skos:definition "A power transformer that forwards power between different voltage grids inside a substation."@en ;
    skos:inScheme piirritev:OsmTransformer ;
    skos:prefLabel "Main"@en .

piirritev:OsmTrolleyWire a skos:ConceptScheme ;
    piirrite:osmId "trolley_wire" ;
    skos:definition "Overhead contact lines for a trolleybus service."@en ;
    skos:prefLabel "Trolley wire, types"@en .

piirritev:OsmTunnelBuildingPassage a skos:Concept ;
    piirrite:hasRelatedOsmTag piirrite:hasOsmBuildingPassageHighway ;
    piirrite:osmId "building_passage" ;
    rdfs:subClassOf piirrite:OsmEntity ;
    skos:definition "A tunnel passage that goes through/under a building, but is not inside the building itself."@en ;
    skos:inScheme piirritev:OsmTunnel ;
    skos:prefLabel "Building passage"@en .

piirritev:OsmTunnelCulvert a skos:Concept ;
    piirrite:hasRelatedOsmTag piirrite:hasOsmCulvertDiameter,
        piirrite:hasOsmCulvertLayer,
        piirrite:hasOsmCulvertWaterway ;
    piirrite:osmId "culvert" ;
    rdfs:subClassOf piirrite:OsmEntity ;
    skos:definition "For a stream/drain/ditch/river passing under a road. Use it on the section of waterway passing under the road. osmcarto-rendering=File:Rendering-waterway river tunnel.png osmcarto-rendering-size=125px"@en ;
    skos:inScheme piirritev:OsmTunnel ;
    skos:prefLabel "Culvert"@en .

piirritev:OsmTunnelFlooded a skos:Concept ;
    piirrite:hasRelatedOsmTag piirrite:hasOsmFloodedUsage,
        piirrite:hasOsmFloodedWaterway ;
    piirrite:osmId "flooded" ;
    rdfs:subClassOf piirrite:OsmEntity ;
    skos:definition "A long (over 100 meters) tunnel where flowing water or other fluid prevent humans from safely walking inside."@en ;
    skos:inScheme piirritev:OsmTunnel ;
    skos:prefLabel "Flooded"@en .

piirritev:OsmTypeAssociatedstreet a skos:Concept ;
    piirrite:osmId "associatedStreet" ;
    rdfs:subClassOf piirrite:OsmEntity ;
    skos:definition "Marks relation as associatedStreet."@en ;
    skos:inScheme piirritev:OsmType ;
    skos:prefLabel "Associatedstreet"@en .

piirritev:OsmTypeBoundary a skos:Concept ;
    piirrite:osmId "boundary" ;
    rdfs:subClassOf piirrite:OsmEntity ;
    skos:definition ""@en ;
    skos:inScheme piirritev:OsmType ;
    skos:prefLabel "Boundary"@en .

piirritev:OsmTypeBuilding a skos:Concept ;
    piirrite:osmId "building" ;
    rdfs:subClassOf piirrite:OsmEntity ;
    skos:definition ""@en ;
    skos:inScheme piirritev:OsmType ;
    skos:prefLabel "Building"@en .

piirritev:OsmTypeConnectivity a skos:Concept ;
    piirrite:osmId "connectivity" ;
    rdfs:subClassOf piirrite:OsmEntity ;
    skos:definition ""@en ;
    skos:inScheme piirritev:OsmType ;
    skos:prefLabel "Connectivity"@en .

piirritev:OsmTypeDestinationSign a skos:Concept ;
    piirrite:osmId "destination_sign" ;
    rdfs:subClassOf piirrite:OsmEntity ;
    skos:definition ""@en ;
    skos:inScheme piirritev:OsmType ;
    skos:prefLabel "Destination sign"@en .

piirritev:OsmTypeEnforcement a skos:Concept ;
    piirrite:osmId "enforcement" ;
    rdfs:subClassOf piirrite:OsmEntity ;
    skos:definition ""@en ;
    skos:inScheme piirritev:OsmType ;
    skos:prefLabel "Enforcement"@en .

piirritev:OsmTypeMultipolygon a skos:Concept ;
    piirrite:osmId "multipolygon" ;
    rdfs:subClassOf piirrite:OsmEntity ;
    skos:definition ""@en ;
    skos:inScheme piirritev:OsmType ;
    skos:prefLabel "Multipolygon"@en .

piirritev:OsmTypePalm a skos:Concept ;
    piirrite:osmId "palm" ;
    rdfs:subClassOf piirrite:OsmEntity ;
    skos:definition ""@en ;
    skos:inScheme piirritev:OsmType ;
    skos:prefLabel "Palm"@en .

piirritev:OsmTypePower a skos:Concept ;
    piirrite:osmId "power" ;
    rdfs:subClassOf piirrite:OsmEntity ;
    skos:definition ""@en ;
    skos:inScheme piirritev:OsmType ;
    skos:prefLabel "Power"@en .

piirritev:OsmTypeProvidesFeature a skos:Concept ;
    piirrite:osmId "provides_feature" ;
    rdfs:subClassOf piirrite:OsmEntity ;
    skos:definition ""@en ;
    skos:inScheme piirritev:OsmType ;
    skos:prefLabel "Provides feature"@en .

piirritev:OsmTypePublicTransport a skos:Concept ;
    piirrite:hasRelatedOsmTag piirrite:hasOsmPublicTransportName,
        piirrite:hasOsmPublicTransportOperator,
        piirrite:hasOsmPublicTransportRef,
        piirrite:hasOsmPublicTransportType ;
    piirrite:osmId "public_transport" ;
    rdfs:subClassOf piirrite:OsmEntity ;
    skos:definition "Represents a public transport related relation."@en ;
    skos:inScheme piirritev:OsmType ;
    skos:prefLabel "Public transport"@en .

piirritev:OsmTypeRestriction a skos:Concept ;
    piirrite:osmId "restriction" ;
    rdfs:subClassOf piirrite:OsmEntity ;
    skos:definition ""@en ;
    skos:inScheme piirritev:OsmType ;
    skos:prefLabel "Restriction"@en .

piirritev:OsmTypeRoute a skos:Concept ;
    piirrite:osmId "route" ;
    rdfs:subClassOf piirrite:OsmEntity ;
    skos:definition ""@en ;
    skos:inScheme piirritev:OsmType ;
    skos:prefLabel "Route"@en .

piirritev:OsmTypeRouteMaster a skos:Concept ;
    piirrite:osmId "route_master" ;
    rdfs:subClassOf piirrite:OsmEntity ;
    skos:definition ""@en ;
    skos:inScheme piirritev:OsmType ;
    skos:prefLabel "Route master"@en .

piirritev:OsmTypeSite a skos:Concept ;
    piirrite:osmId "site" ;
    rdfs:subClassOf piirrite:OsmEntity ;
    skos:definition ""@en ;
    skos:inScheme piirritev:OsmType ;
    skos:prefLabel "Site"@en .

piirritev:OsmTypeStreet a skos:Concept ;
    piirrite:osmId "street" ;
    rdfs:subClassOf piirrite:OsmEntity ;
    skos:definition ""@en ;
    skos:inScheme piirritev:OsmType ;
    skos:prefLabel "Street"@en .

piirritev:OsmTypeWaterway a skos:Concept ;
    piirrite:osmId "waterway" ;
    rdfs:subClassOf piirrite:OsmEntity ;
    skos:definition ""@en ;
    skos:inScheme piirritev:OsmType ;
    skos:prefLabel "Waterway"@en .

piirritev:OsmUicRef a skos:ConceptScheme ;
    piirrite:osmId "uic_ref" ;
    skos:definition "The UIC reference is used to identify railway stations."@en ;
    skos:prefLabel "Uic ref, types"@en .

piirritev:OsmUnsignedRef a skos:ConceptScheme ;
    piirrite:osmId "unsigned_ref" ;
    skos:definition "Indicates a route number that has assigned ref that is not prominently signposted with a reassurance marker."@en ;
    skos:prefLabel "Unsigned ref, types"@en .

piirritev:OsmUrl a skos:ConceptScheme ;
    piirrite:osmId "url" ;
    skos:definition "Specifying an url related to a feature."@en ;
    skos:prefLabel "Url, types"@en .

piirritev:OsmUsageBranch a skos:Concept ;
    piirrite:osmId "branch" ;
    rdfs:subClassOf piirrite:OsmEntity ;
    skos:definition "Specifies that a railway is a branch line, with less traffic and lower speed than main lines, often single tracked, not electrified, constructed to lower specifications than a main line. May connect a place to a mainline or serve to connect mainlines"@en ;
    skos:inScheme piirritev:OsmUsage ;
    skos:prefLabel "Branch"@en .

piirritev:OsmUsageGathering a skos:Concept ;
    piirrite:hasRelatedOsmTag piirrite:hasOsmGatheringManMade ;
    piirrite:osmId "gathering" ;
    rdfs:subClassOf piirrite:OsmEntity ;
    skos:definition "Specific pipeline usage dedicated to path leading fluids from tag:substation=field_gathering to tag:substation=central_processing sites"@en ;
    skos:inScheme piirritev:OsmUsage ;
    skos:prefLabel "Gathering"@en .

piirritev:OsmUsageIndustrial a skos:Concept ;
    piirrite:osmId "industrial" ;
    rdfs:subClassOf piirrite:OsmEntity ;
    skos:definition "Specifies that a railway (or aerialway) is an industrial line, railway tracks in private use that serve only freight transport to/from ports, industrial complexes or mining areas, and for connecting these to the public network."@en ;
    skos:inScheme piirritev:OsmUsage ;
    skos:prefLabel "Industrial"@en .

piirritev:OsmUsageIrrigation a skos:Concept ;
    piirrite:hasRelatedOsmTag piirrite:hasOsmIrrigationLocation,
        piirrite:hasOsmIrrigationWaterway ;
    piirrite:osmId "irrigation" ;
    rdfs:subClassOf piirrite:OsmEntity ;
    skos:definition "Specifies a waterway which carries water intended for agriculture."@en ;
    skos:inScheme piirritev:OsmUsage ;
    skos:prefLabel "Irrigation"@en .

piirritev:OsmUsageMain a skos:Concept ;
    piirrite:osmId "main" ;
    rdfs:subClassOf piirrite:OsmEntity ;
    skos:definition "Specifies that a railway is a main line, presumably heavy traffic, often double tracked and/or electrified, may be high speed."@en ;
    skos:inScheme piirritev:OsmUsage ;
    skos:prefLabel "Main"@en .

piirritev:OsmUsageTourism a skos:Concept ;
    piirrite:hasRelatedOsmTag piirrite:hasOsmTourismService ;
    piirrite:osmId "tourism" ;
    rdfs:subClassOf piirrite:OsmEntity ;
    skos:definition "Specifies that a railway is a tourism line: rail tracks for tourists, around museums, historic or \"heritage\" trains, often only on weekends and holidays and/or seasonally, most preserved railways"@en ;
    skos:inScheme piirritev:OsmUsage ;
    skos:prefLabel "Tourism"@en .

piirritev:OsmUsageTransmission a skos:Concept ;
    piirrite:hasRelatedOsmTag piirrite:hasOsmTransmissionManMade,
        piirrite:hasOsmTransmissionWaterway ;
    piirrite:osmId "transmission" ;
    rdfs:subClassOf piirrite:OsmEntity ;
    skos:definition "Features involved in long distance carriage of fluids or goods and connecting to more specific and local usage networks. It excludes vehicle carriage, referring to transportation."@en ;
    skos:inScheme piirritev:OsmUsage ;
    skos:prefLabel "Transmission"@en .

piirritev:OsmUtilityGas a skos:Concept ;
    piirrite:hasRelatedOsmTag piirrite:hasOsmGasBuilding,
        piirrite:hasOsmGasLanduse,
        piirrite:hasOsmGasManMade,
        piirrite:hasOsmGasMarker,
        piirrite:hasOsmGasOperator,
        piirrite:hasOsmGasSubstance ;
    piirrite:osmId "gas" ;
    rdfs:subClassOf piirrite:OsmEntity ;
    skos:definition "Infrastructure related to gas transmission and distribution towards industries and domestic consumers."@en ;
    skos:inScheme piirritev:OsmUtility ;
    skos:prefLabel "Gas"@en .

piirritev:OsmUtilityPower a skos:Concept ;
    piirrite:hasRelatedOsmTag piirrite:hasOsmPowerBuilding,
        piirrite:hasOsmPowerLanduse,
        piirrite:hasOsmPowerManMade,
        piirrite:hasOsmPowerMarker,
        piirrite:hasOsmPowerOperator,
        piirrite:hasOsmPowerType ;
    piirrite:osmId "power" ;
    rdfs:subClassOf piirrite:OsmEntity ;
    skos:definition "Infrastructure related to electricity transmission and distribution towards industries and domestic consumers."@en ;
    skos:inScheme piirritev:OsmUtility ;
    skos:prefLabel "Power"@en .

piirritev:OsmUtilityStreetLighting a skos:Concept ;
    piirrite:hasRelatedOsmTag piirrite:hasOsmStreetLightingOperator,
        piirrite:hasOsmStreetLightingUsage ;
    piirrite:osmId "street_lighting" ;
    rdfs:subClassOf piirrite:OsmEntity ;
    skos:definition "Activity related to street, roads and cities lighting"@en ;
    skos:inScheme piirritev:OsmUtility ;
    skos:prefLabel "Street lighting"@en .

piirritev:OsmUtilityTelecom a skos:Concept ;
    piirrite:hasRelatedOsmTag piirrite:hasOsmTelecomBuilding,
        piirrite:hasOsmTelecomLanduse,
        piirrite:hasOsmTelecomManMade,
        piirrite:hasOsmTelecomMarker,
        piirrite:hasOsmTelecomOperator,
        piirrite:hasOsmTelecomType ;
    piirrite:osmId "telecom" ;
    rdfs:subClassOf piirrite:OsmEntity ;
    skos:definition "Infrastructure related to telecommunications networks providing phone and internet service towards industries and domestic subscribers."@en ;
    skos:inScheme piirritev:OsmUtility ;
    skos:prefLabel "Telecom"@en .

piirritev:OsmVehicleAgricultural a skos:Concept ;
    piirrite:osmId "agricultural" ;
    rdfs:subClassOf piirrite:OsmEntity ;
    skos:definition "The use of the road is authorized exclusively for all types of vehicles which use it for agricultural purposes"@en ;
    skos:inScheme piirritev:OsmVehicle ;
    skos:prefLabel "Agricultural"@en .

piirritev:OsmVehicleDestination a skos:Concept ;
    piirrite:osmId "destination" ;
    rdfs:subClassOf piirrite:OsmEntity ;
    skos:definition "Indicates that transit traffic using vehicle is not allowed."@en ;
    skos:inScheme piirritev:OsmVehicle ;
    skos:prefLabel "Destination"@en .

piirritev:OsmVehicleForestry a skos:Concept ;
    piirrite:osmId "forestry" ;
    rdfs:subClassOf piirrite:OsmEntity ;
    skos:definition "The use of the road is authorized exclusively for all types of vehicles which use it for agricultural purposes"@en ;
    skos:inScheme piirritev:OsmVehicle ;
    skos:prefLabel "Forestry"@en .

piirritev:OsmVehiclePrivate a skos:Concept ;
    piirrite:osmId "private" ;
    rdfs:subClassOf piirrite:OsmEntity ;
    skos:definition ""@en ;
    skos:inScheme piirritev:OsmVehicle ;
    skos:prefLabel "Private"@en .

piirritev:OsmVoltage a skos:ConceptScheme ;
    piirrite:osmId "voltage" ;
    skos:definition "For describing the voltage of power lines, cables, and substations."@en ;
    skos:prefLabel "Voltage, types"@en .

piirritev:OsmWallBrick a skos:Concept ;
    piirrite:osmId "brick" ;
    rdfs:subClassOf piirrite:OsmEntity ;
    skos:definition "A brick wall is a wall constructed from bricks and mortar."@en ;
    skos:inScheme piirritev:OsmWall ;
    skos:prefLabel "Brick"@en .

piirritev:OsmWallConcrete a skos:Concept ;
    piirrite:osmId "concrete" ;
    rdfs:subClassOf piirrite:OsmEntity ;
    skos:definition ""@en ;
    skos:inScheme piirritev:OsmWall ;
    skos:prefLabel "Concrete"@en .

piirritev:OsmWallDryStone a skos:Concept ;
    piirrite:osmId "dry_stone" ;
    rdfs:subClassOf piirrite:OsmEntity ;
    skos:definition "A dry stone wall is a wall constructed from stones without mortar to bind them together."@en ;
    skos:inScheme piirritev:OsmWall ;
    skos:prefLabel "Dry stone"@en .

piirritev:OsmWallStone a skos:Concept ;
    piirrite:osmId "stone" ;
    rdfs:subClassOf piirrite:OsmEntity ;
    skos:definition "A stone wall is a wall constructed from stones and mortar."@en ;
    skos:inScheme piirritev:OsmWall ;
    skos:prefLabel "Stone"@en .

piirritev:OsmWard a skos:ConceptScheme ;
    piirrite:osmId "ward" ;
    skos:definition "Used differently around the world."@en ;
    skos:prefLabel "Ward, types"@en .

piirritev:OsmWasteDogExcrement a skos:Concept ;
    piirrite:hasRelatedOsmTag piirrite:hasOsmDogExcrementVending ;
    piirrite:osmId "dog_excrement" ;
    rdfs:subClassOf piirrite:OsmEntity ;
    skos:definition "A bin made for the disposal of dog excrement."@en ;
    skos:inScheme piirritev:OsmWaste ;
    skos:prefLabel "Dog excrement"@en .

piirritev:OsmWasteMixed a skos:Concept ;
    piirrite:osmId "mixed" ;
    rdfs:subClassOf piirrite:OsmEntity ;
    skos:definition ""@en ;
    skos:inScheme piirritev:OsmWaste ;
    skos:prefLabel "Mixed"@en .

piirritev:OsmWasteTrash a skos:Concept ;
    piirrite:osmId "trash" ;
    rdfs:subClassOf piirrite:OsmEntity ;
    skos:definition "A bin made for the disposal of trash/rubbish."@en ;
    skos:inScheme piirritev:OsmWaste ;
    skos:prefLabel "Trash"@en .

piirritev:OsmWaterBasin a skos:Concept ;
    piirrite:hasRelatedOsmTag piirrite:hasOsmBasinIntermittent,
        piirrite:hasOsmBasinName,
        piirrite:hasOsmBasinType ;
    piirrite:osmId "basin" ;
    rdfs:subClassOf piirrite:OsmEntity ;
    skos:definition "An area of land artificially graded to hold water. Includes also structures typically without water."@en ;
    skos:inScheme piirritev:OsmWater ;
    skos:prefLabel "Basin"@en .

piirritev:OsmWaterCanal a skos:Concept ;
    piirrite:hasRelatedOsmTag piirrite:hasOsmCanalIntermittent,
        piirrite:hasOsmCanalName ;
    piirrite:osmId "canal" ;
    rdfs:subClassOf piirrite:OsmEntity ;
    skos:definition "The area covered by the water of a canal"@en ;
    skos:inScheme piirritev:OsmWater ;
    skos:prefLabel "Canal"@en .

piirritev:OsmWaterDitch a skos:Concept ;
    piirrite:hasRelatedOsmTag piirrite:hasOsmDitchWater,
        piirrite:hasOsmDitchWaterway ;
    piirrite:osmId "ditch" ;
    rdfs:subClassOf piirrite:OsmEntity ;
    skos:definition "The water covered area of a waterway=ditch - a simple artificial waterway serving as a barrier or for draining surrounding land."@en ;
    skos:inScheme piirritev:OsmWater ;
    skos:prefLabel "Ditch"@en .

piirritev:OsmWaterDrain a skos:Concept ;
    piirrite:hasRelatedOsmTag piirrite:hasOsmDrainIntermittent ;
    piirrite:osmId "drain" ;
    rdfs:subClassOf piirrite:OsmEntity ;
    skos:definition "The water covered area of a tag:waterway=drain - an artificial waterway, lined with concrete or similar, used to carry superfluous water."@en ;
    skos:inScheme piirritev:OsmWater ;
    skos:prefLabel "Drain"@en .

piirritev:OsmWaterFishpond a skos:Concept ;
    piirrite:osmId "fishpond" ;
    rdfs:subClassOf piirrite:OsmEntity ;
    skos:definition "Water basin constructed specifically for fish farming or recreational fishing."@en ;
    skos:inScheme piirritev:OsmWater ;
    skos:prefLabel "Fishpond"@en .

piirritev:OsmWaterLagoon a skos:Concept ;
    piirrite:hasRelatedOsmTag piirrite:hasOsmLagoonName,
        piirrite:hasOsmLagoonSalt ;
    piirrite:osmId "lagoon" ;
    rdfs:subClassOf piirrite:OsmEntity ;
    skos:definition "A body of shallow sea water or brackish water separated from the sea by a barrier."@en ;
    skos:inScheme piirritev:OsmWater ;
    skos:prefLabel "Lagoon"@en .

piirritev:OsmWaterLake a skos:Concept ;
    piirrite:hasRelatedOsmTag piirrite:hasOsmLakeIntermittent,
        piirrite:hasOsmLakeName,
        piirrite:hasOsmLakeSalt,
        piirrite:hasOsmLakeWikidata ;
    piirrite:osmId "lake" ;
    rdfs:subClassOf piirrite:OsmEntity ;
    skos:definition "A natural or semi-natural body of relatively still fresh or salt water which is surrounded by land."@en ;
    skos:inScheme piirritev:OsmWater ;
    skos:prefLabel "Lake"@en .

piirritev:OsmWaterOxbow a skos:Concept ;
    piirrite:hasRelatedOsmTag piirrite:hasOsmOxbowName ;
    piirrite:osmId "oxbow" ;
    rdfs:subClassOf piirrite:OsmEntity ;
    skos:definition "U-shaped body of water formed when a wide meander from the main stem of a river is cut off to create a lake."@en ;
    skos:inScheme piirritev:OsmWater ;
    skos:prefLabel "Oxbow"@en .

piirritev:OsmWaterPond a skos:Concept ;
    piirrite:hasRelatedOsmTag piirrite:hasOsmPondIntermittent,
        piirrite:hasOsmPondName ;
    piirrite:osmId "pond" ;
    rdfs:subClassOf piirrite:OsmEntity ;
    skos:definition "A small body of standing water, man-made in most cases"@en ;
    skos:inScheme piirritev:OsmWater ;
    skos:prefLabel "Pond"@en .

piirritev:OsmWaterReservoir a skos:Concept ;
    piirrite:hasRelatedOsmTag piirrite:hasOsmReservoirIntermittent,
        piirrite:hasOsmReservoirName,
        piirrite:hasOsmReservoirSeasonal,
        piirrite:hasOsmReservoirSwimming ;
    piirrite:osmId "reservoir" ;
    rdfs:subClassOf piirrite:OsmEntity ;
    skos:definition "An artificial lake which may be used to store water. Usually formed by a dam over a natural water course."@en ;
    skos:inScheme piirritev:OsmWater ;
    skos:prefLabel "Reservoir"@en .

piirritev:OsmWaterRiver a skos:Concept ;
    piirrite:hasRelatedOsmTag piirrite:hasOsmRiverIntermittent ;
    piirrite:osmId "river" ;
    rdfs:subClassOf piirrite:OsmEntity ;
    skos:definition "The water covered area of a river."@en ;
    skos:inScheme piirritev:OsmWater ;
    skos:prefLabel "River"@en .

piirritev:OsmWaterSourceIrrigated a skos:Concept ;
    piirrite:osmId "irrigated" ;
    rdfs:subClassOf piirrite:OsmEntity ;
    skos:definition ""@en ;
    skos:inScheme piirritev:OsmWaterSource ;
    skos:prefLabel "Irrigated"@en .

piirritev:OsmWaterSourceMain a skos:Concept ;
    piirrite:hasRelatedOsmTag piirrite:hasOsmMainEmergency ;
    piirrite:osmId "main" ;
    rdfs:subClassOf piirrite:OsmEntity ;
    skos:definition "The water used by a given feature is got from a water distribution pipe"@en ;
    skos:inScheme piirritev:OsmWaterSource ;
    skos:prefLabel "Main"@en .

piirritev:OsmWaterSourceSeasonal a skos:Concept ;
    piirrite:osmId "seasonal" ;
    rdfs:subClassOf piirrite:OsmEntity ;
    skos:definition ""@en ;
    skos:inScheme piirritev:OsmWaterSource ;
    skos:prefLabel "Seasonal"@en .

piirritev:OsmWaterStream a skos:Concept ;
    piirrite:hasRelatedOsmTag piirrite:hasOsmStreamIntermittent ;
    piirrite:osmId "stream" ;
    rdfs:subClassOf piirrite:OsmEntity ;
    skos:definition "The water covered area of a stream: a naturally-formed watercourse which is narrower than a river"@en ;
    skos:inScheme piirritev:OsmWater ;
    skos:prefLabel "Stream"@en .

piirritev:OsmWaterWastewater a skos:Concept ;
    piirrite:osmId "wastewater" ;
    rdfs:subClassOf piirrite:OsmEntity ;
    skos:definition "A clarifier or settling basin of a wastewater treatment plant."@en ;
    skos:inScheme piirritev:OsmWater ;
    skos:prefLabel "Wastewater"@en .

piirritev:OsmWaterwayArtificial a skos:Concept ;
    piirrite:osmId "artificial" ;
    rdfs:subClassOf piirrite:OsmEntity ;
    skos:definition "Tag used in poorly done import, despite high usage is not used in real mapping."@en ;
    skos:inScheme piirritev:OsmWaterway ;
    skos:prefLabel "Artificial"@en .

piirritev:OsmWaterwayCanal a skos:Concept ;
    piirrite:hasRelatedOsmTag piirrite:hasOsmCanalAbandoned,
        piirrite:hasOsmCanalBoat,
        piirrite:hasOsmCanalBridge,
        piirrite:hasOsmCanalCemt,
        piirrite:hasOsmCanalCutting,
        piirrite:hasOsmCanalDemolished,
        piirrite:hasOsmCanalDisused,
        piirrite:hasOsmCanalDraft,
        piirrite:hasOsmCanalEmbankment,
        piirrite:hasOsmCanalLock,
        piirrite:hasOsmCanalMaxspeed,
        piirrite:hasOsmCanalMotorboat,
        piirrite:hasOsmCanalName,
        piirrite:hasOsmCanalNatural,
        piirrite:hasOsmCanalShip,
        piirrite:hasOsmCanalTunnel,
        piirrite:hasOsmCanalUsage,
        piirrite:hasOsmCanalWater,
        piirrite:hasOsmCanalWidth ;
    piirrite:osmId "canal" ;
    rdfs:subClassOf piirrite:OsmEntity ;
    skos:definition "An artificial open flow waterway used to carry useful water for transportation, waterpower, or irrigation. osmcarto-rendering=File:Rendering-river.png osmcarto-rendering-size=125px"@en ;
    skos:inScheme piirritev:OsmWaterway ;
    skos:prefLabel "Canal"@en .

piirritev:OsmWaterwayDam a skos:Concept ;
    piirrite:hasRelatedOsmTag piirrite:hasOsmDamName ;
    piirrite:osmId "dam" ;
    rdfs:subClassOf piirrite:OsmEntity ;
    skos:definition "A barrier built across a river or stream to block and regulate the flow of the river. osmcarto-rendering-node=File:Dam node.svg osmcarto-rendering-node-size=28px osmcarto-rendering-way=File:Rendering-waterway-dam-way.png osmcarto-rendering-way-size=100px osmcarto-rendering-area=File:Dam area 100.png osmcarto-rendering-area-size=100px"@en ;
    skos:inScheme piirritev:OsmWaterway ;
    skos:prefLabel "Dam"@en .

piirritev:OsmWaterwayDitch a skos:Concept ;
    piirrite:hasRelatedOsmTag piirrite:hasOsmDitchDepth,
        piirrite:hasOsmDitchIntermittent,
        piirrite:hasOsmDitchSeasonal,
        piirrite:hasOsmDitchTunnel,
        piirrite:hasOsmDitchUsage,
        piirrite:hasOsmDitchWidth ;
    piirrite:osmId "ditch" ;
    rdfs:subClassOf piirrite:OsmEntity ;
    skos:definition "A small artificial drainage waterway, usually unlined. osmcarto-rendering=File:Rendering-stream.png osmcarto-rendering-size=125px"@en ;
    skos:inScheme piirritev:OsmWaterway ;
    skos:prefLabel "Ditch"@en .

piirritev:OsmWaterwayDrain a skos:Concept ;
    piirrite:hasRelatedOsmTag piirrite:hasOsmDrainIntermittent,
        piirrite:hasOsmDrainLayer,
        piirrite:hasOsmDrainName,
        piirrite:hasOsmDrainOperator,
        piirrite:hasOsmDrainTunnel,
        piirrite:hasOsmDrainWidth ;
    piirrite:osmId "drain" ;
    rdfs:subClassOf piirrite:OsmEntity ;
    skos:definition "An artificial free flow waterway used for carrying superfluous water, usually lined with concrete. osmcarto-rendering=File:Rendering-stream.png osmcarto-rendering-size=125px"@en ;
    skos:inScheme piirritev:OsmWaterway ;
    skos:prefLabel "Drain"@en .

piirritev:OsmWaterwayDrystream a skos:Concept ;
    piirrite:osmId "drystream" ;
    rdfs:subClassOf piirrite:OsmEntity ;
    skos:definition "A negative form of erosion relief formed by the activity of temporary streams."@en ;
    skos:inScheme piirritev:OsmWaterway ;
    skos:prefLabel "Drystream"@en .

piirritev:OsmWaterwayFlowline a skos:Concept ;
    piirrite:osmId "flowline" ;
    rdfs:subClassOf piirrite:OsmEntity ;
    skos:definition "Slow-moving flow through a water body."@en ;
    skos:inScheme piirritev:OsmWaterway ;
    skos:prefLabel "Flowline"@en .

piirritev:OsmWaterwayLockGate a skos:Concept ;
    piirrite:osmId "lock_gate" ;
    rdfs:subClassOf piirrite:OsmEntity ;
    skos:definition "A gate of a lock"@en ;
    skos:inScheme piirritev:OsmWaterway ;
    skos:prefLabel "Lock gate"@en .

piirritev:OsmWaterwayPressurised a skos:Concept ;
    piirrite:hasRelatedOsmTag piirrite:hasOsmPressurisedDiameter,
        piirrite:hasOsmPressurisedLocation,
        piirrite:hasOsmPressurisedManMade,
        piirrite:hasOsmPressurisedTunnel,
        piirrite:hasOsmPressurisedUsage ;
    piirrite:osmId "pressurised" ;
    rdfs:subClassOf piirrite:OsmEntity ;
    skos:definition "An artificial waterway where water flows in a closed space without air"@en ;
    skos:inScheme piirritev:OsmWaterway ;
    skos:prefLabel "Pressurised"@en .

piirritev:OsmWaterwayRapids a skos:Concept ;
    piirrite:osmId "rapids" ;
    rdfs:subClassOf piirrite:OsmEntity ;
    skos:definition "A fast-flowing and turbulent section of a waterway which is not a waterfall."@en ;
    skos:inScheme piirritev:OsmWaterway ;
    skos:prefLabel "Rapids"@en .

piirritev:OsmWaterwayRiver a skos:Concept ;
    piirrite:hasRelatedOsmTag piirrite:hasOsmRiverName,
        piirrite:hasOsmRiverWidth ;
    piirrite:osmId "river" ;
    rdfs:subClassOf piirrite:OsmEntity ;
    skos:definition "The linear flow of a river, in flow direction."@en ;
    skos:inScheme piirritev:OsmWaterway ;
    skos:prefLabel "River"@en .

piirritev:OsmWaterwayStream a skos:Concept ;
    piirrite:hasRelatedOsmTag piirrite:hasOsmStreamIntermittent,
        piirrite:hasOsmStreamName,
        piirrite:hasOsmStreamTunnel,
        piirrite:hasOsmStreamWidth ;
    piirrite:osmId "stream" ;
    rdfs:subClassOf piirrite:OsmEntity ;
    skos:definition "A naturally-forming waterway that is too narrow to be classed as a river. osmcarto-rendering=File:Rendering-stream.png osmcarto-rendering-size=125px"@en ;
    skos:inScheme piirritev:OsmWaterway ;
    skos:prefLabel "Stream"@en .

piirritev:OsmWaterwayTidalChannel a skos:Concept ;
    piirrite:hasRelatedOsmTag piirrite:hasOsmTidalChannelName,
        piirrite:hasOsmTidalChannelSalt,
        piirrite:hasOsmTidalChannelWidth ;
    piirrite:osmId "tidal_channel" ;
    rdfs:subClassOf piirrite:OsmEntity ;
    skos:definition "A natural intertidal waterway in mangroves, salt marshes, and tidal flats with water flow in the direction of the tide."@en ;
    skos:inScheme piirritev:OsmWaterway ;
    skos:prefLabel "Tidal channel"@en .

piirritev:OsmWaterwayWaterfall a skos:Concept ;
    piirrite:hasRelatedOsmTag piirrite:hasOsmWaterfallHeight,
        piirrite:hasOsmWaterfallName,
        piirrite:hasOsmWaterfallWidth ;
    piirrite:osmId "waterfall" ;
    rdfs:subClassOf piirrite:OsmEntity ;
    skos:definition "A place where water flows over a vertical drop or a series of drops in the course of a stream or river. osmcarto-rendering=File:Waterfall-14.svg osmcarto-rendering-size=28px"@en ;
    skos:inScheme piirritev:OsmWaterway ;
    skos:prefLabel "Waterfall"@en .

piirritev:OsmWaterwayWeir a skos:Concept ;
    piirrite:hasRelatedOsmTag piirrite:hasOsmWeirName ;
    piirrite:osmId "weir" ;
    rdfs:subClassOf piirrite:OsmEntity ;
    skos:definition "A barrier built across a river to control water speed and depth. Designed to let water flow over the top all the time or at least in specific conditions. osmcarto-rendering-node=File:Weir node.svg osmcarto-rendering-node-size=28px osmcarto-rendering-way=File:Rendering-waterway-weir-way.png osmcarto-rendering-way-size=125px"@en ;
    skos:inScheme piirritev:OsmWaterway ;
    skos:prefLabel "Weir"@en .

piirritev:OsmWebsite a skos:ConceptScheme ;
    piirrite:osmId "website" ;
    skos:definition "Specifies the link to the official website for a feature."@en ;
    skos:prefLabel "Website, types"@en .

piirritev:OsmWetlandBog a skos:Concept ;
    piirrite:osmId "bog" ;
    rdfs:subClassOf piirrite:OsmEntity ;
    skos:definition "Acidic peat producing wetland. osmcarto-rendering-area=File:Natural_wetland_bog.png osmcarto-rendering-area-size=100px"@en ;
    skos:inScheme piirritev:OsmWetland ;
    skos:prefLabel "Bog"@en .

piirritev:OsmWetlandFen a skos:Concept ;
    piirrite:osmId "fen" ;
    rdfs:subClassOf piirrite:OsmEntity ;
    skos:definition "Groundwater-fed peatforming wetland covered by mosses, grasses, sedges, reeds, and wildflowers. osmcarto-rendering=File:Natural_wetland_marsh.png osmcarto-rendering-size=100px"@en ;
    skos:inScheme piirritev:OsmWetland ;
    skos:prefLabel "Fen"@en .

piirritev:OsmWetlandMangrove a skos:Concept ;
    piirrite:osmId "mangrove" ;
    rdfs:subClassOf piirrite:OsmEntity ;
    skos:definition "Mangrove ecosystem is formed by forests of salt tolerant mangrove trees in the tidal zone of tropical coasts with water temperatures above 20 C. osmcarto-rendering=File:Natural wetland mangrove.png osmcarto-rendering-size=100px"@en ;
    skos:inScheme piirritev:OsmWetland ;
    skos:prefLabel "Mangrove"@en .

piirritev:OsmWetlandMarsh a skos:Concept ;
    piirrite:osmId "marsh" ;
    rdfs:subClassOf piirrite:OsmEntity ;
    skos:definition "Marsh is periodically saturated, flooded, or ponded with water and characterized by herbaceous (non-woody) vegetation adapted to wet soil conditions. osmcarto-rendering-area=File:Natural_wetland_marsh.png osmcarto-rendering-area-size=100px"@en ;
    skos:inScheme piirritev:OsmWetland ;
    skos:prefLabel "Marsh"@en .

piirritev:OsmWetlandReedbed a skos:Concept ;
    piirrite:osmId "reedbed" ;
    rdfs:subClassOf piirrite:OsmEntity ;
    skos:definition "An inundated area dominated by certain tall non-woody plants (reeds, bulrushes, cattail). osmcarto-rendering-area=File:Natural_wetland_reed.png osmcarto-rendering-area-size=100px"@en ;
    skos:inScheme piirritev:OsmWetland ;
    skos:prefLabel "Reedbed"@en .

piirritev:OsmWetlandSaltmarsh a skos:Concept ;
    piirrite:osmId "saltmarsh" ;
    rdfs:subClassOf piirrite:OsmEntity ;
    skos:definition "Either a coastal or dry inland marsh, therefore characterized by herbaceous plants with special adaptations to saline environments. osmcarto-rendering-area=File:Natural_wetland_saltmarsh_100.png osmcarto-rendering-area-size=100px"@en ;
    skos:inScheme piirritev:OsmWetland ;
    skos:prefLabel "Saltmarsh"@en .

piirritev:OsmWetlandStringBog a skos:Concept ;
    piirrite:osmId "string_bog" ;
    rdfs:subClassOf piirrite:OsmEntity ;
    skos:definition "Bog consisting of slightly elevated ridges and islands, with woody plants, alternating with flat, wet sedge mat areas. osmcarto-rendering-area=File:Natural_wetland_bog.png osmcarto-rendering-area-size=100px"@en ;
    skos:inScheme piirritev:OsmWetland ;
    skos:prefLabel "String bog"@en .

piirritev:OsmWetlandSwamp a skos:Concept ;
    piirrite:osmId "swamp" ;
    rdfs:subClassOf piirrite:OsmEntity ;
    skos:definition "An area of waterlogged forest, with dense vegetation. osmcarto-rendering-area=File:Natural_wetland_swamp.png osmcarto-rendering-area-size=100px"@en ;
    skos:inScheme piirritev:OsmWetland ;
    skos:prefLabel "Swamp"@en .

piirritev:OsmWetlandTidalflat a skos:Concept ;
    piirrite:osmId "tidalflat" ;
    rdfs:subClassOf piirrite:OsmEntity ;
    skos:definition "Tidally inundated areas of bare mud or similar sediments. osmcarto-rendering-area=File:Wetland_tidalflat_100.png osmcarto-rendering-area-size=100px"@en ;
    skos:inScheme piirritev:OsmWetland ;
    skos:prefLabel "Tidalflat"@en .

piirritev:OsmWetlandWetMeadow a skos:Concept ;
    piirrite:osmId "wet_meadow" ;
    rdfs:subClassOf piirrite:OsmEntity ;
    skos:definition "Semi-wetland meadow osmcarto-rendering-area=File:Natural_wetland_marsh.png osmcarto-rendering-area-size=100px"@en ;
    skos:inScheme piirritev:OsmWetland ;
    skos:prefLabel "Wet meadow"@en .

piirritev:OsmWheelchairDesignated a skos:Concept ;
    piirrite:osmId "designated" ;
    rdfs:subClassOf piirrite:OsmEntity ;
    skos:definition ""@en ;
    skos:inScheme piirritev:OsmWheelchair ;
    skos:prefLabel "Designated"@en .

piirritev:OsmWheelchairLimited a skos:Concept ;
    piirrite:osmId "limited" ;
    rdfs:subClassOf piirrite:OsmEntity ;
    skos:definition ""@en ;
    skos:inScheme piirritev:OsmWheelchair ;
    skos:prefLabel "Limited"@en .

piirritev:OsmWidth a skos:ConceptScheme ;
    piirrite:osmId "width" ;
    skos:definition "The width of a feature. If not specified, the default unit is the metre."@en ;
    skos:prefLabel "Width, types"@en .

piirritev:OsmWikidata a skos:ConceptScheme ;
    piirrite:osmId "wikidata" ;
    skos:definition "The ID of the Wikidata item about the feature."@en ;
    skos:prefLabel "Wikidata, types"@en .

piirritev:OsmWikimediaCommons a skos:ConceptScheme ;
    piirrite:osmId "wikimedia_commons" ;
    skos:definition "Links to related Wikimedia Commons' media of the feature (syntax File:xxxxxx.xxx / Category:xxxxx)."@en ;
    skos:prefLabel "Wikimedia commons, types"@en .

piirritev:OsmWikipedia a skos:ConceptScheme ;
    piirrite:osmId "wikipedia" ;
    skos:definition "Provides a link to Wikipedia's article about the feature."@en ;
    skos:prefLabel "Wikipedia, types"@en .

piirritev:OsmWiresDouble a skos:Concept ;
    piirrite:osmId "double" ;
    rdfs:subClassOf piirrite:OsmEntity ;
    skos:definition ""@en ;
    skos:inScheme piirritev:OsmWires ;
    skos:prefLabel "Double"@en .

piirritev:OsmWiresSingle a skos:Concept ;
    piirrite:osmId "single" ;
    rdfs:subClassOf piirrite:OsmEntity ;
    skos:definition ""@en ;
    skos:inScheme piirritev:OsmWires ;
    skos:prefLabel "Single"@en .

piirritev:OsmWorkrules a skos:ConceptScheme ;
    piirrite:osmId "workrules" ;
    skos:definition "Describes which workrules (law) applies for a piece of railway."@en ;
    skos:prefLabel "Workrules, types"@en .

piirritev:OsmZone a skos:ConceptScheme ;
    piirrite:osmId "zone" ;
    skos:definition "Used to mark streets (or parking areas) which are part of a zone."@en ;
    skos:prefLabel "Zone, types"@en .

piirritev:OsmBus a skos:ConceptScheme ;
    piirrite:osmId "bus" ;
    skos:definition "Legal access permissions for public transport buses, OR the type of public transport vehicle."@en ;
    skos:prefLabel "Bus, types"@en .

piirritev:OsmColour a skos:ConceptScheme ;
    piirrite:osmId "colour" ;
    skos:definition "The colour associated with the object"@en ;
    skos:prefLabel "Colour, types"@en .

piirritev:OsmCovered a skos:ConceptScheme ;
    piirrite:osmId "covered" ;
    skos:definition "A property to denote if an object is covered by something."@en ;
    skos:prefLabel "Covered, types"@en .

piirritev:OsmDog a skos:ConceptScheme ;
    piirrite:osmId "dog" ;
    skos:definition "Describes if dogs are allowed"@en ;
    skos:prefLabel "Dog, types"@en .

piirritev:OsmFord a skos:ConceptScheme ;
    piirrite:osmId "ford" ;
    skos:definition "A small part of a highway where a waterway runs over it. osmcarto-rendering=File:Ford.16.svg osmcarto-rendering-size=28px"@en ;
    skos:prefLabel "Ford, types"@en .

piirritev:OsmGolfCart a skos:ConceptScheme ;
    piirrite:osmId "golf_cart" ;
    skos:definition "Access restrictions for golf carts"@en ;
    skos:prefLabel "Golf cart, types"@en .

piirritev:OsmGovernment a skos:ConceptScheme ;
    piirrite:osmId "government" ;
    skos:definition "Indicates the subtypes of government agencies and institutions."@en ;
    skos:prefLabel "Government, types"@en .

piirritev:OsmHazmat a skos:ConceptScheme ;
    piirrite:osmId "hazmat" ;
    skos:definition "Restrictions on vehicles transporting hazardous materials."@en ;
    skos:prefLabel "Hazmat, types"@en .

piirritev:OsmInternetAccess a skos:ConceptScheme ;
    piirrite:osmId "internet_access" ;
    skos:definition "Indicates if an object offers internet access. The access can be with given computers or WLAN access. The only limitation is that the internet access has to be public."@en ;
    skos:prefLabel "Internet access, types"@en .

piirritev:OsmLcn a skos:ConceptScheme ;
    piirrite:osmId "lcn" ;
    skos:definition ""@en ;
    skos:prefLabel "Lcn, types"@en .

piirritev:OsmLit a skos:ConceptScheme ;
    piirrite:osmId "lit" ;
    skos:definition "Indicates whether a feature is lit."@en ;
    skos:prefLabel "Lit, types"@en .

piirritev:OsmMaxstay a skos:ConceptScheme ;
    piirrite:osmId "maxstay" ;
    skos:definition "Maximum time you are allowed to stay somewhere."@en ;
    skos:prefLabel "Maxstay, types"@en .

piirritev:OsmOfficialName a skos:ConceptScheme ;
    piirrite:osmId "official_name" ;
    skos:definition "The official name of the feature, or the name as used by governments and other official organizations. Usually tagged when object has unwieldy and typically not used name that was officially assigned."@en ;
    skos:prefLabel "Official name, types"@en .

piirritev:OsmOneway a skos:ConceptScheme ;
    piirrite:osmId "oneway" ;
    skos:definition "Linear features that users can only go one direction in. Used in highways, zip lines, and other features."@en ;
    skos:prefLabel "Oneway, types"@en .

piirritev:OsmOpeningHours a skos:ConceptScheme ;
    piirrite:osmId "opening_hours" ;
    skos:definition "Describes when something is open or closed in a standard format."@en ;
    skos:prefLabel "Opening hours, types"@en .

piirritev:OsmOwner a skos:ConceptScheme ;
    piirrite:osmId "owner" ;
    skos:definition "The name of the owner of a given map feature"@en ;
    skos:prefLabel "Owner, types"@en .

piirritev:OsmPlacement a skos:ConceptScheme ;
    piirrite:osmId "placement" ;
    skos:definition "Used to specify the placement of the OSM-way relative to the road it represents."@en ;
    skos:prefLabel "Placement, types"@en .

piirritev:OsmPriorityRoad a skos:ConceptScheme ;
    piirrite:osmId "priority_road" ;
    skos:definition "A signposted priority road."@en ;
    skos:prefLabel "Priority road, types"@en .

piirritev:OsmPsv a skos:ConceptScheme ;
    piirrite:osmId "psv" ;
    skos:definition "Access permission for Public Service Vehicles: buses and sometimes taxis or other vehicles."@en ;
    skos:prefLabel "Psv, types"@en .

piirritev:OsmPump a skos:ConceptScheme ;
    piirrite:osmId "pump" ;
    skos:definition "Presence and technology of a pump on a source of water."@en ;
    skos:prefLabel "Pump, types"@en .

piirritev:OsmRamp a skos:ConceptScheme ;
    piirrite:osmId "ramp" ;
    skos:definition "Whether a ramp for bicycles, strollers, wheelchairs and/or luggage is built into a stairway"@en ;
    skos:prefLabel "Ramp, types"@en .

piirritev:OsmRouteMaster a skos:ConceptScheme ;
    piirrite:osmId "route_master" ;
    skos:definition "Defines the type of vehicle operated on a public transport route_master relation"@en ;
    skos:prefLabel "Route master, types"@en .

piirritev:OsmRuins a skos:ConceptScheme ;
    piirrite:osmId "ruins" ;
    skos:definition "Indicate that a structure is in ruins or specifies the type of ruins of an tag:historic=ruins."@en ;
    skos:prefLabel "Ruins, types"@en .

piirritev:OsmSeasonal a skos:ConceptScheme ;
    piirrite:osmId "seasonal" ;
    skos:definition "Describes features that depend on seasonal conditions"@en ;
    skos:prefLabel "Seasonal, types"@en .

piirritev:OsmShortName a skos:ConceptScheme ;
    piirrite:osmId "short_name" ;
    skos:definition "A recognizable, commonly used short version of the main name."@en ;
    skos:prefLabel "Short name, types"@en .

piirritev:OsmSmoking a skos:ConceptScheme ;
    piirrite:osmId "smoking" ;
    skos:definition "For marking applicable smoking rules. However, if a law mandates a given smoking rule, that need not be mapped."@en ;
    skos:prefLabel "Smoking, types"@en .

piirritev:OsmSnowmobile a skos:ConceptScheme ;
    piirrite:osmId "snowmobile" ;
    skos:definition "defining access rights for snowmobile to use way or amenity"@en ;
    skos:prefLabel "Snowmobile, types"@en .

piirritev:OsmSourceRef a skos:ConceptScheme ;
    piirrite:osmId "source_ref" ;
    skos:definition "Used to link external sources of information: photos, video links"@en ;
    skos:prefLabel "Source ref, types"@en .

piirritev:OsmStartDate a skos:ConceptScheme ;
    piirrite:osmId "start_date" ;
    skos:definition "Date when feature opened or the construction of the feature finished."@en ;
    skos:prefLabel "Start date, types"@en .

piirritev:OsmStop a skos:ConceptScheme ;
    piirrite:osmId "stop" ;
    skos:definition "A junction at which vehicles on some or all approaches must stop."@en ;
    skos:prefLabel "Stop, types"@en .

piirritev:OsmTakeaway a skos:ConceptScheme ;
    piirrite:osmId "takeaway" ;
    skos:definition "Whether the restaurant offers meals for pick-up that can be consumed elsewhere."@en ;
    skos:prefLabel "Takeaway, types"@en .

piirritev:OsmTrailblazed a skos:ConceptScheme ;
    piirrite:osmId "trailblazed" ;
    skos:definition "Markings on outdoor paths and trails by signs, markers, poles, cairns or in another way."@en ;
    skos:prefLabel "Trailblazed, types"@en .

piirritev:OsmAerialway a skos:ConceptScheme ;
    piirrite:osmId "aerialway" ;
    skos:definition "Used for various forms of transport for passengers and goods that use wires, including cable-cars, chair-lifts and drag-lifts."@en ;
    skos:prefLabel "Aerialway, types"@en .

piirritev:OsmCemetery a skos:ConceptScheme ;
    piirrite:osmId "cemetery" ;
    skos:definition "Specifies parts of a cemetery, single graves or special kinds of cemeteries."@en ;
    skos:prefLabel "Cemetery, types"@en .

piirritev:OsmDeparturesBoard a skos:ConceptScheme ;
    piirrite:osmId "departures_board" ;
    skos:definition "A board in an airport, train station, bus terminal or stop, etc displaying the information about future departures."@en ;
    skos:prefLabel "Departures board, types"@en .

piirritev:OsmEducation a skos:ConceptScheme ;
    piirrite:osmId "education" ;
    skos:definition "Sometimes used to map schools, kindergartens, universities, and other educational features."@en ;
    skos:prefLabel "Education, types"@en .

piirritev:OsmElectrified a skos:ConceptScheme ;
    piirrite:osmId "electrified" ;
    skos:definition "Indicates infrastructure to supply vehicles with electricity, on rail tracks or highways."@en ;
    skos:prefLabel "Electrified, types"@en .

piirritev:OsmIncline a skos:ConceptScheme ;
    piirrite:osmId "incline" ;
    skos:definition "Incline steepness"@en ;
    skos:prefLabel "Incline, types"@en .

piirritev:OsmJunction a skos:ConceptScheme ;
    piirrite:osmId "junction" ;
    skos:definition "Describing the kind of a junction."@en ;
    skos:prefLabel "Junction, types"@en .

piirritev:OsmLightSource a skos:ConceptScheme ;
    piirrite:osmId "light_source" ;
    skos:definition ""@en ;
    skos:prefLabel "Light source, types"@en .

piirritev:OsmLocalRef a skos:ConceptScheme ;
    piirrite:osmId "local_ref" ;
    skos:definition "Letters and/or numbers identifying a public transport stop within a larger stop group"@en ;
    skos:prefLabel "Local ref, types"@en .

piirritev:OsmMaxheight a skos:ConceptScheme ;
    piirrite:osmId "maxheight" ;
    skos:definition "The legal maximum height."@en ;
    skos:prefLabel "Maxheight, types"@en .

piirritev:OsmMofa a skos:ConceptScheme ;
    piirrite:osmId "mofa" ;
    skos:definition "Access permission for mofas"@en ;
    skos:prefLabel "Mofa, types"@en .

piirritev:OsmMoped a skos:ConceptScheme ;
    piirrite:osmId "moped" ;
    skos:definition "Access permission for mopeds"@en ;
    skos:prefLabel "Moped, types"@en .

piirritev:OsmNhs a skos:ConceptScheme ;
    piirrite:osmId "NHS" ;
    skos:definition "Specifies, if the road is part of a National Highway System."@en ;
    skos:prefLabel "Nhs, types"@en .

piirritev:OsmOldRailwayOperator a skos:ConceptScheme ;
    piirrite:osmId "old_railway_operator" ;
    skos:definition "Used for indicating the former operator of a railway line, whether active or abandoned."@en ;
    skos:prefLabel "Old railway operator, types"@en .

piirritev:OsmOperationalStatus a skos:ConceptScheme ;
    piirrite:osmId "operational_status" ;
    skos:definition "Observation of the current functional status of a mapped feature - now discouraged"@en ;
    skos:prefLabel "Operational status, types"@en .

piirritev:OsmParkingSpace a skos:ConceptScheme ;
    piirrite:osmId "parking_space" ;
    skos:definition "Indicates the type of the parking space."@en ;
    skos:prefLabel "Parking space, types"@en .

piirritev:OsmProduce a skos:ConceptScheme ;
    piirrite:osmId "produce" ;
    skos:definition "Describes a feature's agricultural output produced through a natural process of growing or breeding."@en ;
    skos:prefLabel "Produce, types"@en .

piirritev:OsmProduct a skos:ConceptScheme ;
    piirrite:osmId "product" ;
    skos:definition "The output or product that a feature produces."@en ;
    skos:prefLabel "Product, types"@en .

piirritev:OsmRoom a skos:ConceptScheme ;
    piirrite:osmId "room" ;
    skos:definition "Defines the function of a given room."@en ;
    skos:prefLabel "Room, types"@en .

piirritev:OsmShoulder a skos:ConceptScheme ;
    piirrite:osmId "shoulder" ;
    skos:definition "Presence of shoulder in highway"@en ;
    skos:prefLabel "Shoulder, types"@en .

piirritev:OsmSide a skos:ConceptScheme ;
    piirrite:osmId "side" ;
    skos:definition "Specifies which side of a way an associated feature is located."@en ;
    skos:prefLabel "Side, types"@en .

piirritev:OsmStanding a skos:ConceptScheme ;
    piirrite:osmId "standing" ;
    skos:definition "Seems to be an import by and large from \"Plan polyvalent Douala\" in Cameroon."@en ;
    skos:prefLabel "Standing, types"@en .

piirritev:OsmStatus a skos:ConceptScheme ;
    piirrite:osmId "status" ;
    skos:definition "group="@en ;
    skos:prefLabel "Status, types"@en .

piirritev:OsmTactilePaving a skos:ConceptScheme ;
    piirrite:osmId "tactile_paving" ;
    skos:definition "Indicates whether a blind or visually impaired pedestrian can detect or follow the feature using a cane."@en ;
    skos:prefLabel "Tactile paving, types"@en .

piirritev:OsmTaxon a skos:ConceptScheme ;
    piirrite:osmId "taxon" ;
    skos:definition "Describes the taxon of a feature."@en ;
    skos:prefLabel "Taxon, types"@en .

piirritev:OsmTransformer a skos:ConceptScheme ;
    piirrite:osmId "transformer" ;
    skos:definition "The purpose of a power transformer."@en ;
    skos:prefLabel "Transformer, types"@en .

piirritev:OsmWheelchair a skos:ConceptScheme ;
    piirrite:osmId "wheelchair" ;
    skos:definition "Indicate if a special place can be used with wheelchairs"@en ;
    skos:prefLabel "Wheelchair, types"@en .

piirritev:OsmWires a skos:ConceptScheme ;
    piirrite:osmId "wires" ;
    skos:definition "Number of wires per power cable. \"single\" (1), \"double\" (2), \"triple\" (3) or \"quad\" (4)."@en ;
    skos:prefLabel "Wires, types"@en .

piirritev:OsmAge a skos:ConceptScheme ;
    piirrite:osmId "age" ;
    skos:definition "Describes the maturity of a tree."@en ;
    skos:prefLabel "Age, types"@en .

piirritev:OsmBridge a skos:ConceptScheme ;
    piirrite:osmId "bridge" ;
    skos:definition "A bridge is an artificial construction that spans features such as roads, railways, paths, waterways or valleys and carries a road, railway or other feature."@en ;
    skos:prefLabel "Bridge, types"@en .

piirritev:OsmCondition a skos:ConceptScheme ;
    piirrite:osmId "condition" ;
    skos:definition "Describes the physical condition of an object (good, bad)"@en ;
    skos:prefLabel "Condition, types"@en .

piirritev:OsmCrossingRef a skos:ConceptScheme ;
    piirrite:osmId "crossing_ref" ;
    skos:definition "Used to reference a specific type of crossing."@en ;
    skos:prefLabel "Crossing ref, types"@en .

piirritev:OsmDesignation a skos:ConceptScheme ;
    piirrite:osmId "designation" ;
    skos:definition "The legal classification of an object, usually used on key:highway features."@en ;
    skos:prefLabel "Designation, types"@en .

piirritev:OsmHfcs a skos:ConceptScheme ;
    piirrite:osmId "HFCS" ;
    skos:definition "The highway functional classification of a road in the United States as designated by a state department of transportation."@en ;
    skos:prefLabel "Hfcs, types"@en .

piirritev:OsmHorse a skos:ConceptScheme ;
    piirrite:osmId "horse" ;
    skos:definition "Access permission for equestrians."@en ;
    skos:prefLabel "Horse, types"@en .

piirritev:OsmManhole a skos:ConceptScheme ;
    piirrite:osmId "manhole" ;
    skos:definition "Hole with a cover that allows access to an underground service location, just large enough for a human to climb through."@en ;
    skos:prefLabel "Manhole, types"@en .

piirritev:OsmMarker a skos:ConceptScheme ;
    piirrite:osmId "marker" ;
    skos:definition "Shape and function of a physical spot indicating underground utility infrastructure, highway milestones or private property limits"@en ;
    skos:prefLabel "Marker, types"@en .

piirritev:OsmMotorcycle a skos:ConceptScheme ;
    piirrite:osmId "motorcycle" ;
    skos:definition "Access permission for motorcycles."@en ;
    skos:prefLabel "Motorcycle, types"@en .

piirritev:OsmOrientation a skos:ConceptScheme ;
    piirrite:osmId "orientation" ;
    skos:definition "Indicates the orientation of the feature with respect to the flow of vehicles or passerby."@en ;
    skos:prefLabel "Orientation, types"@en .

piirritev:OsmProposed a skos:ConceptScheme ;
    piirrite:osmId "proposed" ;
    skos:definition "The proposed tag may be used for any road, railway or route that is in planning phase."@en ;
    skos:prefLabel "Proposed, types"@en .

piirritev:OsmSacScale a skos:ConceptScheme ;
    piirrite:osmId "sac_scale" ;
    skos:definition "A difficulty rating scheme for hiking trails."@en ;
    skos:prefLabel "Sac scale, types"@en .

piirritev:OsmSite a skos:ConceptScheme ;
    piirrite:osmId "site" ;
    skos:definition "Used to describe geodesic sites, site relations, public transport stop areas and other sites"@en ;
    skos:prefLabel "Site, types"@en .

piirritev:OsmStructure a skos:ConceptScheme ;
    piirrite:osmId "structure" ;
    skos:definition "Describes the structure of masts (e.g. of high-voltage line masts or catenary masts)."@en ;
    skos:prefLabel "Structure, types"@en .

piirritev:OsmSubstation a skos:ConceptScheme ;
    piirrite:osmId "substation" ;
    skos:definition "Specifies substation role in a utility network."@en ;
    skos:prefLabel "Substation, types"@en .

piirritev:OsmSwimmingPool a skos:ConceptScheme ;
    piirrite:osmId "swimming_pool" ;
    skos:definition "Indicates whether a feature has a swimming pool or not or describes the type of pool."@en ;
    skos:prefLabel "Swimming pool, types"@en .

piirritev:OsmSwitch a skos:ConceptScheme ;
    piirrite:osmId "switch" ;
    skos:definition "Specifies switch function in a network"@en ;
    skos:prefLabel "Switch, types"@en .

piirritev:OsmTrafficSign a skos:ConceptScheme ;
    piirrite:osmId "traffic_sign" ;
    skos:definition "Traffic signs give instructions or provide information to road users."@en ;
    skos:prefLabel "Traffic sign, types"@en .

piirritev:OsmTrafficSignals a skos:ConceptScheme ;
    piirrite:osmId "traffic_signals" ;
    skos:definition "Gives details about the type or function of traffic signals."@en ;
    skos:prefLabel "Traffic signals, types"@en .

piirritev:OsmTunnel a skos:ConceptScheme ;
    piirrite:osmId "tunnel" ;
    skos:definition "A tunnel is an underground passageway built for a road or similar."@en ;
    skos:prefLabel "Tunnel, types"@en .

piirritev:OsmWaste a skos:ConceptScheme ;
    piirrite:osmId "waste" ;
    skos:definition "The type of waste in waste disposal."@en ;
    skos:prefLabel "Waste, types"@en .

piirritev:OsmWaterSource a skos:ConceptScheme ;
    piirrite:osmId "water_source" ;
    skos:definition "Indicates the source of the water for features that provide or use water."@en ;
    skos:prefLabel "Water source, types"@en .

piirritev:OsmArtworkType a skos:ConceptScheme ;
    piirrite:osmId "artwork_type" ;
    skos:definition "Describes the type of an artwork."@en ;
    skos:prefLabel "Artwork type, types"@en .

piirritev:OsmBollard a skos:ConceptScheme ;
    piirrite:osmId "bollard" ;
    skos:definition "Finer-grained classification of a bollard."@en ;
    skos:prefLabel "Bollard, types"@en .

piirritev:OsmBorderType a skos:ConceptScheme ;
    piirrite:osmId "border_type" ;
    skos:definition "Distinguishes a boundary by its formal designation in the real world, or distinguishes between a country's different maritime limits."@en ;
    skos:prefLabel "Border type, types"@en .

piirritev:OsmDescription a skos:ConceptScheme ;
    piirrite:osmId "description" ;
    skos:definition "To provide additional information about the related element to the end map user."@en ;
    skos:prefLabel "Description, types"@en .

piirritev:OsmHgv a skos:ConceptScheme ;
    piirrite:osmId "hgv" ;
    skos:definition "Access permission for heavy goods vehicle; in most countries goods vehicles with a permissible maximum mass over 3.5 tonnes"@en ;
    skos:prefLabel "Hgv, types"@en .

piirritev:OsmImport a skos:ConceptScheme ;
    piirrite:osmId "import" ;
    skos:definition "Unnecessary duplicate of key:source."@en ;
    skos:prefLabel "Import, types"@en .

piirritev:OsmKerb a skos:ConceptScheme ;
    piirrite:osmId "kerb" ;
    skos:definition "Used to indicate height and thus accessibility of a kerb."@en ;
    skos:prefLabel "Kerb, types"@en .

piirritev:OsmLandcover a skos:ConceptScheme ;
    piirrite:osmId "landcover" ;
    skos:definition "A key to describe the physical coverage of an area."@en ;
    skos:prefLabel "Landcover, types"@en .

piirritev:OsmLeafType a skos:ConceptScheme ;
    piirrite:osmId "leaf_type" ;
    skos:definition "Describes the type of leaves"@en ;
    skos:prefLabel "Leaf type, types"@en .

piirritev:OsmLoadingGauge a skos:ConceptScheme ;
    piirrite:osmId "loading_gauge" ;
    skos:definition "Used to show what freight wagons can go on a track."@en ;
    skos:prefLabel "Loading gauge, types"@en .

piirritev:OsmMeadow a skos:ConceptScheme ;
    piirrite:osmId "meadow" ;
    skos:definition "Used to indicate the kind of meadow."@en ;
    skos:prefLabel "Meadow, types"@en .

piirritev:OsmMotorcar a skos:ConceptScheme ;
    piirrite:osmId "motorcar" ;
    skos:definition "Access permission for cars."@en ;
    skos:prefLabel "Motorcar, types"@en .

piirritev:OsmSidewalk a skos:ConceptScheme ;
    piirrite:osmId "sidewalk" ;
    skos:definition "Indicates the presence or absence of a sidewalk (pavement/footway)."@en ;
    skos:prefLabel "Sidewalk, types"@en .

piirritev:OsmSocialFacility a skos:ConceptScheme ;
    piirrite:osmId "social_facility" ;
    skos:definition "Specifies the type of a facility that provides social services."@en ;
    skos:prefLabel "Social facility, types"@en .

piirritev:OsmSubstance a skos:ConceptScheme ;
    piirrite:osmId "substance" ;
    skos:definition "Specifies the substance transported in pipelines or processed in related facilities."@en ;
    skos:prefLabel "Substance, types"@en .

piirritev:OsmSurveillance a skos:ConceptScheme ;
    piirrite:osmId "surveillance" ;
    skos:definition "Indicates whether a location is under surveillance or what type of surveilled area it is."@en ;
    skos:prefLabel "Surveillance, types"@en .

piirritev:OsmUtility a skos:ConceptScheme ;
    piirrite:osmId "utility" ;
    skos:definition "Specifies the type of utility infrastructure which a feature represents."@en ;
    skos:prefLabel "Utility, types"@en .

piirritev:OsmVehicle a skos:ConceptScheme ;
    piirrite:osmId "vehicle" ;
    skos:definition "Access permission for all vehicles"@en ;
    skos:prefLabel "Vehicle, types"@en .

piirritev:OsmWall a skos:ConceptScheme ;
    piirrite:osmId "wall" ;
    skos:definition "Used to provide more detailed information about a tag:barrier=wall. The value should indicate the principle feature of the wall, which might be the type, purpose, or building material of the wall."@en ;
    skos:prefLabel "Wall, types"@en .

piirritev:OsmBicycleParking a skos:ConceptScheme ;
    piirrite:osmId "bicycle_parking" ;
    skos:definition "For describing the type of bicycle parking."@en ;
    skos:prefLabel "Bicycle parking, types"@en .

piirritev:OsmContent a skos:ConceptScheme ;
    piirrite:osmId "content" ;
    skos:definition "To describe the contents of a feature used to store materials."@en ;
    skos:prefLabel "Content, types"@en .

piirritev:OsmLeafCycle a skos:ConceptScheme ;
    piirrite:osmId "leaf_cycle" ;
    skos:definition "Describes the phenology of leaves"@en ;
    skos:prefLabel "Leaf cycle, types"@en .

piirritev:OsmManufacturer a skos:ConceptScheme ;
    piirrite:osmId "manufacturer" ;
    skos:definition "Manufacturer of an object"@en ;
    skos:prefLabel "Manufacturer, types"@en .

piirritev:OsmOwnership a skos:ConceptScheme ;
    piirrite:osmId "ownership" ;
    skos:definition "Indicates what type of organization owns land, facility, etc."@en ;
    skos:prefLabel "Ownership, types"@en .

piirritev:OsmShelterType a skos:ConceptScheme ;
    piirrite:osmId "shelter_type" ;
    skos:definition "Indicates the use and structure type of a shelter."@en ;
    skos:prefLabel "Shelter type, types"@en .

piirritev:OsmTrailVisibility a skos:ConceptScheme ;
    piirrite:osmId "trail_visibility" ;
    skos:definition "Classification scheme for trail (not route) visibility and way-finding skill required."@en ;
    skos:prefLabel "Trail visibility, types"@en .

piirritev:OsmBoardType a skos:ConceptScheme ;
    piirrite:osmId "board_type" ;
    skos:definition "Specifies the details of an tag:information=board"@en ;
    skos:prefLabel "Board type, types"@en .

piirritev:OsmCrossing a skos:ConceptScheme ;
    piirrite:osmId "crossing" ;
    skos:definition "Further refinement for nodes already tagged with tag:highway=crossing or tag:railway=crossing"@en ;
    skos:prefLabel "Crossing, types"@en .

piirritev:OsmFoot a skos:ConceptScheme ;
    piirrite:osmId "foot" ;
    skos:definition "Access permission for pedestrians"@en ;
    skos:prefLabel "Foot, types"@en .

piirritev:OsmHouse a skos:ConceptScheme ;
    piirrite:osmId "house" ;
    skos:definition "The type of a house. Used in combination with tag:building=house."@en ;
    skos:prefLabel "House, types"@en .

piirritev:OsmIndoor a skos:ConceptScheme ;
    piirrite:osmId "indoor" ;
    skos:definition "Key used with the Simple Indoor Tagging scheme."@en ;
    skos:prefLabel "Indoor, types"@en .

piirritev:OsmIndustrial a skos:ConceptScheme ;
    piirrite:osmId "industrial" ;
    skos:definition "Type of industry or type of industrial object."@en ;
    skos:prefLabel "Industrial, types"@en .

piirritev:OsmLampMount a skos:ConceptScheme ;
    piirrite:osmId "lamp_mount" ;
    skos:definition "Lamp holder of a street lamp"@en ;
    skos:prefLabel "Lamp mount, types"@en .

piirritev:OsmLampType a skos:ConceptScheme ;
    piirrite:osmId "lamp_type" ;
    skos:definition "Type of lamp."@en ;
    skos:prefLabel "Lamp type, types"@en .

piirritev:OsmNavigationaid a skos:ConceptScheme ;
    piirrite:osmId "navigationaid" ;
    skos:definition "A type of facility that supports navigation for aircraft"@en ;
    skos:prefLabel "Navigationaid, types"@en .

piirritev:OsmReligion a skos:ConceptScheme ;
    piirrite:osmId "religion" ;
    skos:definition "Defines the specific religion."@en ;
    skos:prefLabel "Religion, types"@en .

piirritev:OsmResidential a skos:ConceptScheme ;
    piirrite:osmId "residential" ;
    skos:definition "Subtag of tag:landuse=residential used to mark the type of residential area"@en ;
    skos:prefLabel "Residential, types"@en .

piirritev:OsmSupport a skos:ConceptScheme ;
    piirrite:osmId "support" ;
    skos:definition "Type of support for certain features"@en ;
    skos:prefLabel "Support, types"@en .

piirritev:OsmAttribution a skos:ConceptScheme ;
    piirrite:osmId "attribution" ;
    skos:definition "The data source of the information used to tag and/or place this element (often considered deprecated)"@en ;
    skos:prefLabel "Attribution, types"@en .

piirritev:OsmBicycle a skos:ConceptScheme ;
    piirrite:osmId "bicycle" ;
    skos:definition "Access permission for cyclists."@en ;
    skos:prefLabel "Bicycle, types"@en .

piirritev:OsmFixme a skos:ConceptScheme ;
    piirrite:osmId "fixme" ;
    skos:definition "Description of a (possible) error in the map."@en ;
    skos:prefLabel "Fixme, types"@en .

piirritev:OsmFootway a skos:ConceptScheme ;
    piirrite:osmId "footway" ;
    skos:definition "Further refinement of footways"@en ;
    skos:prefLabel "Footway, types"@en .

piirritev:OsmInformation a skos:ConceptScheme ;
    piirrite:osmId "information" ;
    skos:definition "Refines detail for tag:tourism=information."@en ;
    skos:prefLabel "Information, types"@en .

piirritev:OsmNote a skos:ConceptScheme ;
    piirrite:osmId "note" ;
    skos:definition "A note to yourself or to other mappers."@en ;
    skos:prefLabel "Note, types"@en .

piirritev:OsmParking a skos:ConceptScheme ;
    piirrite:osmId "parking" ;
    skos:definition "Indicates the type of the parking facility"@en ;
    skos:prefLabel "Parking, types"@en .

piirritev:OsmPlayground a skos:ConceptScheme ;
    piirrite:osmId "playground" ;
    skos:definition "Specifies the type of playground equipment."@en ;
    skos:prefLabel "Playground, types"@en .

piirritev:OsmUsage a skos:ConceptScheme ;
    piirrite:osmId "usage" ;
    skos:definition "Describes the primary usage of railways, pipeline or waterways"@en ;
    skos:prefLabel "Usage, types"@en .

piirritev:OsmIntRef a skos:ConceptScheme ;
    piirrite:osmId "int_ref" ;
    skos:definition "International reference number or code on roads, highway exits, routes, etc."@en ;
    skos:prefLabel "Int ref, types"@en .

piirritev:OsmMotorVehicle a skos:ConceptScheme ;
    piirrite:osmId "motor_vehicle" ;
    skos:definition "Access permission for motor vehicles"@en ;
    skos:prefLabel "Motor vehicle, types"@en .

piirritev:OsmEntrance a skos:ConceptScheme ;
    piirrite:osmId "entrance" ;
    skos:definition "To mark the location of an entrance."@en ;
    skos:prefLabel "Entrance, types"@en .

piirritev:OsmGolf a skos:ConceptScheme ;
    piirrite:osmId "golf" ;
    skos:definition "To map the details on a golf course"@en ;
    skos:prefLabel "Golf, types"@en .

piirritev:OsmAccess a skos:ConceptScheme ;
    piirrite:osmId "access" ;
    skos:definition "For describing the legal accessibility of a feature."@en ;
    skos:prefLabel "Access, types"@en .

piirritev:OsmCrop a skos:ConceptScheme ;
    piirrite:osmId "crop" ;
    skos:definition "The crop produced by cultivated land."@en ;
    skos:prefLabel "Crop, types"@en .

piirritev:OsmDenotation a skos:ConceptScheme ;
    piirrite:osmId "denotation" ;
    skos:definition "Defines the denotation of a tree"@en ;
    skos:prefLabel "Denotation, types"@en .

piirritev:OsmFenceType a skos:ConceptScheme ;
    piirrite:osmId "fence_type" ;
    skos:definition "Describes the type of a fence."@en ;
    skos:prefLabel "Fence type, types"@en .

piirritev:OsmWetland a skos:ConceptScheme ;
    piirrite:osmId "wetland" ;
    skos:definition "Type of wetland."@en ;
    skos:prefLabel "Wetland, types"@en .

piirritev:OsmDirection a skos:ConceptScheme ;
    piirrite:osmId "direction" ;
    skos:definition "Specifies the direction of a feature."@en ;
    skos:prefLabel "Direction, types"@en .

piirritev:OsmLocation a skos:ConceptScheme ;
    piirrite:osmId "location" ;
    skos:definition "To define the location of a feature which may be above or under ground or in relation to objects such as roofs, bridges or buildings."@en ;
    skos:prefLabel "Location, types"@en .

piirritev:OsmRef a skos:ConceptScheme ;
    piirrite:osmId "ref" ;
    skos:definition "Used for reference numbers or codes. Common for roads, highway exits, routes, entrances to big buildings etc."@en ;
    skos:prefLabel "Ref, types"@en .

piirritev:OsmRoute a skos:ConceptScheme ;
    piirrite:osmId "route" ;
    skos:definition "A customary or regular line of passage or travel, often predetermined and publicized."@en ;
    skos:prefLabel "Route, types"@en .

piirritev:OsmBoundary a skos:ConceptScheme ;
    piirrite:osmId "boundary" ;
    skos:definition "Used to mark the borders of areas, mostly political, but possibly also of other administrative areas."@en ;
    skos:prefLabel "Boundary, types"@en .

piirritev:OsmCraft a skos:ConceptScheme ;
    piirrite:osmId "craft" ;
    skos:definition "A place producing or processing customized goods"@en ;
    skos:prefLabel "Craft, types"@en .

piirritev:OsmEmergency a skos:ConceptScheme ;
    piirrite:osmId "emergency" ;
    skos:definition "Describes various emergency services, facilities, amenities or the possibility of access for emergency services"@en ;
    skos:prefLabel "Emergency, types"@en .

piirritev:OsmDesign a skos:ConceptScheme ;
    piirrite:osmId "design" ;
    skos:definition "Describes the design of poles or pylons carrying high voltage electricity cables"@en ;
    skos:prefLabel "Design, types"@en .

piirritev:OsmService a skos:ConceptScheme ;
    piirrite:osmId "service" ;
    skos:definition "Additional information about a service highway/railway/waterway, or about services offered at a business."@en ;
    skos:prefLabel "Service, types"@en .

piirritev:OsmWater a skos:ConceptScheme ;
    piirrite:osmId "water" ;
    skos:definition "Specification of a water body."@en ;
    skos:prefLabel "Water, types"@en .

piirritev:OsmAeroway a skos:ConceptScheme ;
    piirrite:osmId "aeroway" ;
    skos:definition "For physical infrastructure used to support aircraft, air travel, spacecraft and space flight."@en ;
    skos:prefLabel "Aeroway, types"@en .

piirritev:OsmConstruction a skos:ConceptScheme ;
    piirrite:osmId "construction" ;
    skos:definition "Used together with the top-level tags like tag:highway=construction or tag:building=construction to describe the type of feature which is currently under construction."@en ;
    skos:prefLabel "Construction, types"@en .

piirritev:OsmWaterway a skos:ConceptScheme ;
    piirrite:osmId "waterway" ;
    skos:definition "Used to mark rivers or other kind of waterways."@en ;
    skos:prefLabel "Waterway, types"@en .

piirritev:OsmDenomination a skos:ConceptScheme ;
    piirrite:osmId "denomination" ;
    skos:definition "Defines the subgroup of a specific religion."@en ;
    skos:prefLabel "Denomination, types"@en .

piirritev:OsmMaterial a skos:ConceptScheme ;
    piirrite:osmId "material" ;
    skos:definition "Describes the main material of a physical feature."@en ;
    skos:prefLabel "Material, types"@en .

piirritev:OsmPower a skos:ConceptScheme ;
    piirrite:osmId "power" ;
    skos:definition "Facilities for generation and distribution of electrical power."@en ;
    skos:prefLabel "Power, types"@en .

piirritev:OsmType a skos:ConceptScheme ;
    piirrite:osmId "type" ;
    skos:definition "Type of a relation."@en ;
    skos:prefLabel "Type, types"@en .

piirritev:OsmCreatedBy a skos:ConceptScheme ;
    piirrite:osmId "created_by" ;
    skos:definition "The editor or script that created the changeset, node, way or relation. Used before 2009, now only on changesets."@en ;
    skos:prefLabel "Created by, types"@en .

piirritev:OsmOffice a skos:ConceptScheme ;
    piirrite:osmId "office" ;
    skos:definition "A place of business predominately providing services."@en ;
    skos:prefLabel "Office, types"@en .

piirritev:OsmTourism a skos:ConceptScheme ;
    piirrite:osmId "tourism" ;
    skos:definition "A place or object of specific interest to tourists."@en ;
    skos:prefLabel "Tourism, types"@en .

piirritev:OsmBrand a skos:ConceptScheme ;
    piirrite:osmId "brand" ;
    skos:definition "The identity of a specific product, service, or business. Often trademarks"@en ;
    skos:prefLabel "Brand, types"@en .

piirritev:OsmBarrier a skos:ConceptScheme ;
    piirrite:osmId "barrier" ;
    skos:definition "A barrier is a physical structure which blocks or impedes movement."@en ;
    skos:prefLabel "Barrier, types"@en .

piirritev:OsmSurface a skos:ConceptScheme ;
    piirrite:osmId "surface" ;
    skos:definition "Describes the surface of a feature."@en ;
    skos:prefLabel "Surface, types"@en .

piirritev:OsmRailway a skos:ConceptScheme ;
    piirrite:osmId "railway" ;
    skos:definition "Used for railways and railway infrastructure."@en ;
    skos:prefLabel "Railway, types"@en .

piirritev:OsmGenus a skos:ConceptScheme ;
    piirrite:osmId "genus" ;
    skos:definition "The scientific name of the genus for a living or fossil organism."@en ;
    skos:prefLabel "Genus, types"@en .

piirritev:OsmSport a skos:ConceptScheme ;
    piirrite:osmId "sport" ;
    skos:definition "For categorising any specific sport."@en ;
    skos:prefLabel "Sport, types"@en .

piirritev:OsmLanduse a skos:ConceptScheme ;
    piirrite:osmId "landuse" ;
    skos:definition "Mainly used for describing the primary use of areas of land."@en ;
    skos:prefLabel "Landuse, types"@en .

piirritev:OsmNatural a skos:ConceptScheme ;
    piirrite:osmId "natural" ;
    skos:definition "Natural physical landscape features, including those modified or created by humans."@en ;
    skos:prefLabel "Natural, types"@en .

piirritev:OsmSpecies a skos:ConceptScheme ;
    piirrite:osmId "species" ;
    skos:definition "The scientific name for a living or fossil organism."@en ;
    skos:prefLabel "Species, types"@en .

piirritev:OsmNetwork a skos:ConceptScheme ;
    piirrite:osmId "network" ;
    skos:definition "A system of routes (or bicycle rental stations) typically maintained or designated by a single agency or organization, or for bicycle and walking routes, an indication of the scope of the route."@en ;
    skos:prefLabel "Network, types"@en .

piirritev:OsmHighway a skos:ConceptScheme ;
    piirrite:osmId "highway" ;
    skos:definition "Used for roads and road-related facilities."@en ;
    skos:prefLabel "Highway, types"@en .

piirritev:OsmName a skos:ConceptScheme ;
    piirrite:osmId "name" ;
    skos:definition "The primary name: in general, the most prominent signposted name or the most common name in the local language(s)."@en ;
    skos:prefLabel "Name, types"@en .

piirritev:OsmOperator a skos:ConceptScheme ;
    piirrite:osmId "operator" ;
    skos:definition "ompany, corporation, person or any other entity who is directly in charge of the current operation of a map object"@en ;
    skos:prefLabel "Operator, types"@en .

piirritev:OsmBuilding a skos:ConceptScheme ;
    piirrite:osmId "building" ;
    skos:definition "To mark the outline of a building, a man-made structure with a roof, standing more or less permanently in one place.  osmcarto-rendering = File:Area building=yes.png  osmcarto-rendering-size = 28px"@en ;
    skos:prefLabel "Building, types"@en .

piirritev:OsmAmenity a skos:ConceptScheme ;
    piirrite:osmId "amenity" ;
    skos:definition "For describing useful and important facilities for visitors and residents."@en ;
    skos:prefLabel "Amenity, types"@en .

piirritev:OsmSource a skos:ConceptScheme ;
    piirrite:osmId "source" ;
    skos:definition "For indicating the source of all tags added to the OSM database."@en ;
    skos:prefLabel "Source, types"@en .

