@prefix piirrite: <http://piirrite.univ-lyon1.fr/ontology/core#> .
@prefix piirritev: <http://piirrite.univ-lyon1.fr/vocabulary#> .
@prefix rdfs: <http://www.w3.org/2000/01/rdf-schema#> .
@prefix skos: <http://www.w3.org/2004/02/skos/core#> .

piirritev:Abandoned a skos:ConceptScheme ;
    piirrite:osmId "abandoned" ;
    skos:definition "A man-made feature abandoned and no longer maintained. Also see key:abandoned:*."@en ;
    skos:prefLabel "Abandoned, types"@en .

piirritev:Access a skos:ConceptScheme ;
    piirrite:osmId "access" ;
    skos:definition "For describing the legal accessibility of a feature."@en ;
    skos:prefLabel "Access, types"@en .

piirritev:AdminLevel a skos:ConceptScheme ;
    piirrite:osmId "admin_level" ;
    skos:definition "Indicates the level of an administrative boundary."@en ;
    skos:prefLabel "Admin level, types"@en .

piirritev:AerialwayPylon a skos:Concept ;
    piirrite:hasRelatedOsmTag piirrite:hasPylonRef ;
    piirrite:osmId "pylon" ;
    rdfs:subClassOf piirrite:OsmEntity ;
    skos:definition "A pylon supporting the aerialway cable."@en ;
    skos:inScheme piirritev:Aerialway ;
    skos:prefLabel "Pylon"@en .

piirritev:AerialwayStation a skos:Concept ;
    piirrite:hasRelatedOsmTag piirrite:hasStationEle,
        piirrite:hasStationName,
        piirrite:hasStationOperator ;
    piirrite:osmId "station" ;
    rdfs:subClassOf piirrite:OsmEntity ;
    skos:definition "A station where passengers and/or goods can enter and/or leave the aerialway  osmcarto-rendering = File:Rendering-railway-tram stop-mapnik.png.png  osmcarto-rendering-size = 14px"@en ;
    skos:inScheme piirritev:Aerialway ;
    skos:prefLabel "Station"@en .

piirritev:AerowayAerodrome a skos:Concept ;
    piirrite:hasRelatedOsmTag piirrite:hasAerodromeDescription,
        piirrite:hasAerodromeIata,
        piirrite:hasAerodromeIcao,
        piirrite:hasAerodromeName,
        piirrite:hasAerodromeOperator,
        piirrite:hasAerodromeWebsite,
        piirrite:hasAerodromeWikipedia ;
    piirrite:osmId "aerodrome" ;
    rdfs:subClassOf piirrite:OsmEntity ;
    skos:definition "An aerodrome, airport or airfield  osmcarto-rendering = File:Aerodrome.svg  osmcarto-rendering-size = 28px  osmcarto-rendering-area = File:Area transportation.png  osmcarto-rendering-area-size = 100px"@en ;
    skos:inScheme piirritev:Aeroway ;
    skos:prefLabel "Aerodrome"@en .

piirritev:AerowayApron a skos:Concept ;
    piirrite:hasRelatedOsmTag piirrite:hasApronAeroway,
        piirrite:hasApronName,
        piirrite:hasApronRef,
        piirrite:hasApronSurface ;
    piirrite:osmId "apron" ;
    rdfs:subClassOf piirrite:OsmEntity ;
    skos:definition "An area of an airport where planes are parked, unloaded, loaded, refueled, or boarded.  osmcarto-rendering = File:Osmarender-apron.png  osmcarto-rendering-size = 100px"@en ;
    skos:inScheme piirritev:Aeroway ;
    skos:prefLabel "Apron"@en .

piirritev:AerowayGate a skos:Concept ;
    piirrite:hasRelatedOsmTag piirrite:hasGateRef ;
    piirrite:osmId "gate" ;
    rdfs:subClassOf piirrite:OsmEntity ;
    skos:definition "The bounded space, inside the airport terminal, where passengers wait before boarding their flight"@en ;
    skos:inScheme piirritev:Aeroway ;
    skos:prefLabel "Gate"@en .

piirritev:AerowayHangar a skos:Concept ;
    piirrite:hasRelatedOsmTag piirrite:hasHangarBuilding,
        piirrite:hasHangarName,
        piirrite:hasHangarRef ;
    piirrite:osmId "hangar" ;
    rdfs:subClassOf piirrite:OsmEntity ;
    skos:definition "A large airport building with extensive floor area that is used for housing aircraft or spacecraft."@en ;
    skos:inScheme piirritev:Aeroway ;
    skos:prefLabel "Hangar"@en .

piirritev:AerowayHelipad a skos:Concept ;
    piirrite:hasRelatedOsmTag piirrite:hasHelipadIcao,
        piirrite:hasHelipadMaxrotordiameter,
        piirrite:hasHelipadMaxweight,
        piirrite:hasHelipadName,
        piirrite:hasHelipadRef ;
    piirrite:osmId "helipad" ;
    rdfs:subClassOf piirrite:OsmEntity ;
    skos:definition "A landing area or platform designed for helicopters. It might be part of an aerodrome, heliport, hospital, hotel etc.  osmcarto-rendering = File:Helipad.16.svg  osmcarto-rendering-size = 28px  osmcarto-rendering-area = File:Rendering-aeroway area.png  osmcarto-rendering-area-size = 100px"@en ;
    skos:inScheme piirritev:Aeroway ;
    skos:prefLabel "Helipad"@en .

piirritev:AerowayHoldingPosition a skos:Concept ;
    piirrite:osmId "holding_position" ;
    rdfs:subClassOf piirrite:OsmEntity ;
    skos:definition "A point behind which aircraft are considered clear of a crossing way"@en ;
    skos:inScheme piirritev:Aeroway ;
    skos:prefLabel "Holding position"@en .

piirritev:AerowayJetBridge a skos:Concept ;
    piirrite:hasRelatedOsmTag piirrite:hasJetBridgeHighway,
        piirrite:hasJetBridgeRef ;
    piirrite:osmId "jet_bridge" ;
    rdfs:subClassOf piirrite:OsmEntity ;
    skos:definition "An enclosed, movable connector that extends from an airport terminal to an airplane"@en ;
    skos:inScheme piirritev:Aeroway ;
    skos:prefLabel "Jet bridge"@en .

piirritev:AerowayNavigationaid a skos:Concept ;
    piirrite:hasRelatedOsmTag piirrite:hasNavigationaidType ;
    piirrite:osmId "navigationaid" ;
    rdfs:subClassOf piirrite:OsmEntity ;
    skos:definition "A facility that supports visual navigation for aircraft"@en ;
    skos:inScheme piirritev:Aeroway ;
    skos:prefLabel "Navigationaid"@en .

piirritev:AerowayParkingPosition a skos:Concept ;
    piirrite:hasRelatedOsmTag piirrite:hasParkingPositionEle,
        piirrite:hasParkingPositionRef,
        piirrite:hasParkingPositionSurface ;
    piirrite:osmId "parking_position" ;
    rdfs:subClassOf piirrite:OsmEntity ;
    skos:definition "A location where an airplane can park."@en ;
    skos:inScheme piirritev:Aeroway ;
    skos:prefLabel "Parking position"@en .

piirritev:AerowayRunway a skos:Concept ;
    piirrite:hasRelatedOsmTag piirrite:hasRunwayCenterline,
        piirrite:hasRunwayEle,
        piirrite:hasRunwayLength,
        piirrite:hasRunwayRef,
        piirrite:hasRunwaySurface,
        piirrite:hasRunwayWidth ;
    piirrite:osmId "runway" ;
    rdfs:subClassOf piirrite:OsmEntity ;
    skos:definition "A designated strip of surface on which aircrafts can take off and land.  osmcarto-rendering = File:Rendering-aeroway runway.png  osmcarto-rendering-size = 100px"@en ;
    skos:inScheme piirritev:Aeroway ;
    skos:prefLabel "Runway"@en .

piirritev:AerowayTaxilane a skos:Concept ;
    piirrite:osmId "taxilane" ;
    rdfs:subClassOf piirrite:OsmEntity ;
    skos:definition "A path for aircraft in an airport that is part of the aircraft parking area or apron"@en ;
    skos:inScheme piirritev:Aeroway ;
    skos:prefLabel "Taxilane"@en .

piirritev:AerowayTaxiway a skos:Concept ;
    piirrite:hasRelatedOsmTag piirrite:hasTaxiwayRef,
        piirrite:hasTaxiwaySurface ;
    piirrite:osmId "taxiway" ;
    rdfs:subClassOf piirrite:OsmEntity ;
    skos:definition "A route where airplanes manouevre between runways and parking areas within an aerodrome  osmcarto-rendering = File:Rendering-aeroway taxiway.png  osmcarto-rendering-size = 100px"@en ;
    skos:inScheme piirritev:Aeroway ;
    skos:prefLabel "Taxiway"@en .

piirritev:AerowayTerminal a skos:Concept ;
    piirrite:hasRelatedOsmTag piirrite:hasTerminalBuilding,
        piirrite:hasTerminalEntrance,
        piirrite:hasTerminalName,
        piirrite:hasTerminalRef ;
    piirrite:osmId "terminal" ;
    rdfs:subClassOf piirrite:OsmEntity ;
    skos:definition "An airport passenger building  osmcarto-rendering = File:Area amenity=place of worship.png"@en ;
    skos:inScheme piirritev:Aeroway ;
    skos:prefLabel "Terminal"@en .

piirritev:AerowayWindsock a skos:Concept ;
    piirrite:hasRelatedOsmTag piirrite:hasWindsockLit ;
    piirrite:osmId "windsock" ;
    rdfs:subClassOf piirrite:OsmEntity ;
    skos:definition "An object that shows wind direction and speed."@en ;
    skos:inScheme piirritev:Aeroway ;
    skos:prefLabel "Windsock"@en .

piirritev:AgeMature a skos:Concept ;
    piirrite:osmId "mature" ;
    rdfs:subClassOf piirrite:OsmEntity ;
    skos:definition ""@en ;
    skos:inScheme piirritev:Age ;
    skos:prefLabel "Mature"@en .

piirritev:AgeSemi-Mature a skos:Concept ;
    piirrite:osmId "semi-mature" ;
    rdfs:subClassOf piirrite:OsmEntity ;
    skos:definition ""@en ;
    skos:inScheme piirritev:Age ;
    skos:prefLabel "Semi-mature"@en .

piirritev:AgeYoung a skos:Concept ;
    piirrite:osmId "young" ;
    rdfs:subClassOf piirrite:OsmEntity ;
    skos:definition ""@en ;
    skos:inScheme piirritev:Age ;
    skos:prefLabel "Young"@en .

piirritev:AirConditioning a skos:ConceptScheme ;
    piirrite:osmId "air_conditioning" ;
    skos:definition "Indication whether a feature has air-conditioning"@en ;
    skos:prefLabel "Air conditioning, types"@en .

piirritev:AltName a skos:ConceptScheme ;
    piirrite:osmId "alt_name" ;
    skos:definition "Alternative name or names by which the feature is known in the local language; for names in other languages, use name:xy where xy is the ISO 639 language code; not to be confused with name:alt, which is for the name in the Altai language"@en ;
    skos:prefLabel "Alt name, types"@en .

piirritev:AmenityAnimalBreeding a skos:Concept ;
    piirrite:hasRelatedOsmTag piirrite:hasAnimalBreedingName,
        piirrite:hasAnimalBreedingOperator ;
    piirrite:osmId "animal_breeding" ;
    rdfs:subClassOf piirrite:OsmEntity ;
    skos:definition "A facility where animals are bred, usually to sell them."@en ;
    skos:inScheme piirritev:Amenity ;
    skos:prefLabel "Animal breeding"@en .

piirritev:AmenityArtsCentre a skos:Concept ;
    piirrite:hasRelatedOsmTag piirrite:hasArtsCentreDescription,
        piirrite:hasArtsCentreName,
        piirrite:hasArtsCentreOperator ;
    piirrite:osmId "arts_centre" ;
    rdfs:subClassOf piirrite:OsmEntity ;
    skos:definition "An arts centre. A venue where a variety of arts are performed or conducted  osmcarto-rendering = File:Arts centre.svg  osmcarto-rendering-size = 28px  osmcarto-rendering-area = File:Rendering-area-amenity-school.png  osmcarto-rendering-area-size = 100px"@en ;
    skos:inScheme piirritev:Amenity ;
    skos:prefLabel "Arts centre"@en .

piirritev:AmenityAtm a skos:Concept ;
    piirrite:hasRelatedOsmTag piirrite:hasAtmDriveThrough,
        piirrite:hasAtmOperator ;
    piirrite:osmId "atm" ;
    rdfs:subClassOf piirrite:OsmEntity ;
    skos:definition "A device that provides the clients of a financial institution with access to financial transactions."@en ;
    skos:inScheme piirritev:Amenity ;
    skos:prefLabel "Atm"@en .

piirritev:AmenityBank a skos:Concept ;
    piirrite:hasRelatedOsmTag piirrite:hasBankAtm,
        piirrite:hasBankBic,
        piirrite:hasBankBranch,
        piirrite:hasBankBrand,
        piirrite:hasBankDriveThrough,
        piirrite:hasBankName,
        piirrite:hasBankOpeningHours,
        piirrite:hasBankOperator,
        piirrite:hasBankWheelchair ;
    piirrite:osmId "bank" ;
    rdfs:subClassOf piirrite:OsmEntity ;
    skos:definition "A financial establishment where customers can, among other services, deposit money and take loans.  osmcarto-rendering = File:Bank-16.svg  osmcarto-rendering-size = 28px"@en ;
    skos:inScheme piirritev:Amenity ;
    skos:prefLabel "Bank"@en .

piirritev:AmenityBar a skos:Concept ;
    piirrite:hasRelatedOsmTag piirrite:hasBarBrewery,
        piirrite:hasBarDistillery,
        piirrite:hasBarLiveMusic,
        piirrite:hasBarMicrobrewery,
        piirrite:hasBarName,
        piirrite:hasBarOpeningHours,
        piirrite:hasBarOperator,
        piirrite:hasBarWebsite,
        piirrite:hasBarWheelchair,
        piirrite:hasBarWinery ;
    piirrite:osmId "bar" ;
    rdfs:subClassOf piirrite:OsmEntity ;
    skos:definition " osmcarto-rendering = File:Bar-16.svg  osmcarto-rendering-size = 28px"@en ;
    skos:inScheme piirritev:Amenity ;
    skos:prefLabel "Bar"@en .

piirritev:AmenityBbq a skos:Concept ;
    piirrite:hasRelatedOsmTag piirrite:hasBbqCovered,
        piirrite:hasBbqFuel ;
    piirrite:osmId "bbq" ;
    rdfs:subClassOf piirrite:OsmEntity ;
    skos:definition "A permanently built place for having a BBQ.  osmcarto-rendering = File:Bbq-14.svg  osmcarto-rendering-size = 28px"@en ;
    skos:inScheme piirritev:Amenity ;
    skos:prefLabel "Bbq"@en .

piirritev:AmenityBench a skos:Concept ;
    piirrite:hasRelatedOsmTag piirrite:hasBenchArmrest,
        piirrite:hasBenchBackrest,
        piirrite:hasBenchColour,
        piirrite:hasBenchCovered,
        piirrite:hasBenchDirection,
        piirrite:hasBenchHistoric,
        piirrite:hasBenchInscription,
        piirrite:hasBenchLength,
        piirrite:hasBenchMaterial,
        piirrite:hasBenchMemorial,
        piirrite:hasBenchOperator,
        piirrite:hasBenchSeats,
        piirrite:hasBenchSide,
        piirrite:hasBenchStartDate,
        piirrite:hasBenchTwoSided,
        piirrite:hasBenchWheelchair ;
    piirrite:osmId "bench" ;
    rdfs:subClassOf piirrite:OsmEntity ;
    skos:definition "A place for people to sit, allowing room for one or more people.  osmcarto-rendering = File:Bench-16.svg  osmcarto-rendering-size = 28px"@en ;
    skos:inScheme piirritev:Amenity ;
    skos:prefLabel "Bench"@en .

piirritev:AmenityBicycleParking a skos:Concept ;
    piirrite:hasRelatedOsmTag piirrite:hasBicycleParkingAccess,
        piirrite:hasBicycleParkingCapacity,
        piirrite:hasBicycleParkingCargoBike,
        piirrite:hasBicycleParkingCovered,
        piirrite:hasBicycleParkingCyclestreetsId,
        piirrite:hasBicycleParkingFee,
        piirrite:hasBicycleParkingIndoor,
        piirrite:hasBicycleParkingMaxstay,
        piirrite:hasBicycleParkingName,
        piirrite:hasBicycleParkingOperator,
        piirrite:hasBicycleParkingSurveillance,
        piirrite:hasBicycleParkingType ;
    piirrite:osmId "bicycle_parking" ;
    rdfs:subClassOf piirrite:OsmEntity ;
    skos:definition "A parking space designed for bicycles.  osmcarto-rendering = File:Parking-bicycle-16.svg  osmcarto-rendering-size = 28px  osmcarto-rendering-area = File:Area parking.png  osmcarto-rendering-area-size = 100px"@en ;
    skos:inScheme piirritev:Amenity ;
    skos:prefLabel "Bicycle parking"@en .

piirritev:AmenityBicycleRental a skos:Concept ;
    piirrite:hasRelatedOsmTag piirrite:hasBicycleRentalCapacity,
        piirrite:hasBicycleRentalName,
        piirrite:hasBicycleRentalNetwork,
        piirrite:hasBicycleRentalOperator,
        piirrite:hasBicycleRentalRef ;
    piirrite:osmId "bicycle_rental" ;
    rdfs:subClassOf piirrite:OsmEntity ;
    skos:definition "A place, often unattended, where you can pick up and drop off rented bikes.  osmcarto-rendering = File:Rental-bicycle-16.svg  osmcarto-rendering-size = 28px"@en ;
    skos:inScheme piirritev:Amenity ;
    skos:prefLabel "Bicycle rental"@en .

piirritev:AmenityBiergarten a skos:Concept ;
    piirrite:hasRelatedOsmTag piirrite:hasBiergartenName ;
    piirrite:osmId "biergarten" ;
    rdfs:subClassOf piirrite:OsmEntity ;
    skos:definition "An open-air seating area where beer is served.  osmcarto-rendering = File:Biergarten-16.svg  osmcarto-rendering-size = 28px"@en ;
    skos:inScheme piirritev:Amenity ;
    skos:prefLabel "Biergarten"@en .

piirritev:AmenityBusStation a skos:Concept ;
    piirrite:hasRelatedOsmTag piirrite:hasBusStationName,
        piirrite:hasBusStationOperator ;
    piirrite:osmId "bus_station" ;
    rdfs:subClassOf piirrite:OsmEntity ;
    skos:definition "A bus station would usually be a terminus where many routes stop / start, and where you can change between routes, etc.  osmcarto-rendering = File:Amenity bus station.svg  osmcarto-rendering-size = 28px  osmcarto-rendering-area = File:Area transportation.png  osmcarto-rendering-area-size = 100px"@en ;
    skos:inScheme piirritev:Amenity ;
    skos:prefLabel "Bus station"@en .

piirritev:AmenityCafe a skos:Concept ;
    piirrite:hasRelatedOsmTag piirrite:hasCafeAirConditioning,
        piirrite:hasCafeAmenity,
        piirrite:hasCafeBakery,
        piirrite:hasCafeBrand,
        piirrite:hasCafeCapacity,
        piirrite:hasCafeChangingTable,
        piirrite:hasCafeCuisine,
        piirrite:hasCafeDog,
        piirrite:hasCafeDrinkingStraw,
        piirrite:hasCafeIceCream,
        piirrite:hasCafeIndoorSeating,
        piirrite:hasCafeInternetAccess,
        piirrite:hasCafeLaptop,
        piirrite:hasCafeName,
        piirrite:hasCafeOpeningHours,
        piirrite:hasCafeOperator,
        piirrite:hasCafeOutdoorSeating,
        piirrite:hasCafePastry,
        piirrite:hasCafePhone,
        piirrite:hasCafeSelfService,
        piirrite:hasCafeSmoking,
        piirrite:hasCafeTakeaway,
        piirrite:hasCafeTelevision,
        piirrite:hasCafeToilets,
        piirrite:hasCafeWebsite,
        piirrite:hasCafeWheelchair ;
    piirrite:osmId "cafe" ;
    rdfs:subClassOf piirrite:OsmEntity ;
    skos:definition "A generally informal place with sit-down facilities selling beverages and light meals and/or snacks.  osmcarto-rendering = File:Cafe-16.svg  osmcarto-rendering-size = 28px"@en ;
    skos:inScheme piirritev:Amenity ;
    skos:prefLabel "Cafe"@en .

piirritev:AmenityCarRental a skos:Concept ;
    piirrite:hasRelatedOsmTag piirrite:hasCarRentalName,
        piirrite:hasCarRentalOpeningHours,
        piirrite:hasCarRentalOperator,
        piirrite:hasCarRentalPhone,
        piirrite:hasCarRentalWebsite ;
    piirrite:osmId "car_rental" ;
    rdfs:subClassOf piirrite:OsmEntity ;
    skos:definition "A place from which cars can be rented.  osmcarto-rendering = File:Rental-car-16.svg  osmcarto-rendering-size = 28px"@en ;
    skos:inScheme piirritev:Amenity ;
    skos:prefLabel "Car rental"@en .

piirritev:AmenityCarSharing a skos:Concept ;
    piirrite:hasRelatedOsmTag piirrite:hasCarSharingName,
        piirrite:hasCarSharingNetwork,
        piirrite:hasCarSharingOperator ;
    piirrite:osmId "car_sharing" ;
    rdfs:subClassOf piirrite:OsmEntity ;
    skos:definition "Carsharing station, where you get your booked car, often separate areas on parking places."@en ;
    skos:inScheme piirritev:Amenity ;
    skos:prefLabel "Car sharing"@en .

piirritev:AmenityCarWash a skos:Concept ;
    piirrite:hasRelatedOsmTag piirrite:hasCarWashAccess,
        piirrite:hasCarWashAmenity,
        piirrite:hasCarWashAutomated,
        piirrite:hasCarWashBrand,
        piirrite:hasCarWashBus,
        piirrite:hasCarWashDogWashing,
        piirrite:hasCarWashMaxheight,
        piirrite:hasCarWashMaxwidth,
        piirrite:hasCarWashName,
        piirrite:hasCarWashOpeningHours,
        piirrite:hasCarWashOperator,
        piirrite:hasCarWashPhone,
        piirrite:hasCarWashSelfService,
        piirrite:hasCarWashTouchlessWash,
        piirrite:hasCarWashTruckWash,
        piirrite:hasCarWashVacuumCleaner,
        piirrite:hasCarWashWebsite ;
    piirrite:osmId "car_wash" ;
    rdfs:subClassOf piirrite:OsmEntity ;
    skos:definition "A facility used to clean the exterior of motor vehicles  osmcarto-rendering = File:Car wash-14.svg  osmcarto-rendering-size = 28px"@en ;
    skos:inScheme piirritev:Amenity ;
    skos:prefLabel "Car wash"@en .

piirritev:AmenityChargingStation a skos:Concept ;
    piirrite:hasRelatedOsmTag piirrite:hasChargingStationAccess,
        piirrite:hasChargingStationBrand,
        piirrite:hasChargingStationCapacity ;
    piirrite:osmId "charging_station" ;
    rdfs:subClassOf piirrite:OsmEntity ;
    skos:definition "A location where battery electric vehicles can be charged.  osmcarto-rendering = File:Charging station.16.svg  osmcarto-rendering-size = 28px"@en ;
    skos:inScheme piirritev:Amenity ;
    skos:prefLabel "Charging station"@en .

piirritev:AmenityChildcare a skos:Concept ;
    piirrite:osmId "childcare" ;
    rdfs:subClassOf piirrite:OsmEntity ;
    skos:definition "A place where children are looked after which is not an tag:amenity=kindergarten.  osmcarto-rendering = File:Social amenity darken 80-16.svg  osmcarto-rendering-size = 28px"@en ;
    skos:inScheme piirritev:Amenity ;
    skos:prefLabel "Childcare"@en .

piirritev:AmenityCinema a skos:Concept ;
    piirrite:hasRelatedOsmTag piirrite:hasCinemaName ;
    piirrite:osmId "cinema" ;
    rdfs:subClassOf piirrite:OsmEntity ;
    skos:definition "A movie theater, a place showing movies.  osmcarto-rendering = File:Cinema-16.svg  osmcarto-rendering-size = 28px"@en ;
    skos:inScheme piirritev:Amenity ;
    skos:prefLabel "Cinema"@en .

piirritev:AmenityClinic a skos:Concept ;
    piirrite:hasRelatedOsmTag piirrite:hasClinicName,
        piirrite:hasClinicOpeningHours ;
    piirrite:osmId "clinic" ;
    rdfs:subClassOf piirrite:OsmEntity ;
    skos:definition "A clinic is a medical centre, with more staff than a doctor's office, that does not admit inpatients.  osmcarto-rendering = File:Doctors-14.svg  osmcarto-rendering-size = 28px  osmcarto-rendering-area = File:Rendering-area-amenity-school.png  osmcarto-rendering-area-size = 100px"@en ;
    skos:inScheme piirritev:Amenity ;
    skos:prefLabel "Clinic"@en .

piirritev:AmenityClock a skos:Concept ;
    piirrite:osmId "clock" ;
    rdfs:subClassOf piirrite:OsmEntity ;
    skos:definition "A publicly visible clock"@en ;
    skos:inScheme piirritev:Amenity ;
    skos:prefLabel "Clock"@en .

piirritev:AmenityCollege a skos:Concept ;
    piirrite:hasRelatedOsmTag piirrite:hasCollegeName,
        piirrite:hasCollegeOperator,
        piirrite:hasCollegePhone,
        piirrite:hasCollegeWebsite ;
    piirrite:osmId "college" ;
    rdfs:subClassOf piirrite:OsmEntity ;
    skos:definition "A place for further education, a post-secondary education institution which is not a University  osmcarto-rendering-area = File:Rendering-area-amenity-school.png  osmcarto-rendering-area-size = 125px"@en ;
    skos:inScheme piirritev:Amenity ;
    skos:prefLabel "College"@en .

piirritev:AmenityCommunityCentre a skos:Concept ;
    piirrite:hasRelatedOsmTag piirrite:hasCommunityCentreType ;
    piirrite:osmId "community_centre" ;
    rdfs:subClassOf piirrite:OsmEntity ;
    skos:definition "A place mostly used for local events, festivities and group activities.  osmcarto-rendering = File:Community centre-14.svg  osmcarto-rendering-size = 28px  osmcarto-rendering-area = File:Rendering-area-amenity-school.png  osmcarto-rendering-area-size = 100px"@en ;
    skos:inScheme piirritev:Amenity ;
    skos:prefLabel "Community centre"@en .

piirritev:AmenityCompressedAir a skos:Concept ;
    piirrite:hasRelatedOsmTag piirrite:hasCompressedAirAccess,
        piirrite:hasCompressedAirFee,
        piirrite:hasCompressedAirOpeningHours,
        piirrite:hasCompressedAirPressure,
        piirrite:hasCompressedAirValves ;
    piirrite:osmId "compressed_air" ;
    rdfs:subClassOf piirrite:OsmEntity ;
    skos:definition "A device to inflate tyres, mostly of motor vehicles."@en ;
    skos:inScheme piirritev:Amenity ;
    skos:prefLabel "Compressed air"@en .

piirritev:AmenityCourthouse a skos:Concept ;
    piirrite:hasRelatedOsmTag piirrite:hasCourthouseAdminLevel,
        piirrite:hasCourthouseName,
        piirrite:hasCourthouseOpeningHours,
        piirrite:hasCourthouseOperator,
        piirrite:hasCourthousePhone,
        piirrite:hasCourthouseWebsite,
        piirrite:hasCourthouseWheelchair ;
    piirrite:osmId "courthouse" ;
    rdfs:subClassOf piirrite:OsmEntity ;
    skos:definition "A building which is home to a court of law, which administers justice according to the rule of law.  osmcarto-rendering = File:Courthouse-16.svg  osmcarto-rendering-size = 28px"@en ;
    skos:inScheme piirritev:Amenity ;
    skos:prefLabel "Courthouse"@en .

piirritev:AmenityDentist a skos:Concept ;
    piirrite:hasRelatedOsmTag piirrite:hasDentistName ;
    piirrite:osmId "dentist" ;
    rdfs:subClassOf piirrite:OsmEntity ;
    skos:definition "A dentist practice / surgery.  osmcarto-rendering = File:Dentist-14.svg  osmcarto-rendering-size = 28px"@en ;
    skos:inScheme piirritev:Amenity ;
    skos:prefLabel "Dentist"@en .

piirritev:AmenityDoctors a skos:Concept ;
    piirrite:hasRelatedOsmTag piirrite:hasDoctorsHealthcare,
        piirrite:hasDoctorsName ;
    piirrite:osmId "doctors" ;
    rdfs:subClassOf piirrite:OsmEntity ;
    skos:definition "A doctor's office, a place to get medical attention or a check up from a physician.  osmcarto-rendering = File:Doctors-14.svg  osmcarto-rendering-size = 28px"@en ;
    skos:inScheme piirritev:Amenity ;
    skos:prefLabel "Doctors"@en .

piirritev:AmenityDrinkingWater a skos:Concept ;
    piirrite:hasRelatedOsmTag piirrite:hasDrinkingWaterAccess,
        piirrite:hasDrinkingWaterBottle,
        piirrite:hasDrinkingWaterCapacity,
        piirrite:hasDrinkingWaterDescription,
        piirrite:hasDrinkingWaterFountain,
        piirrite:hasDrinkingWaterIndoor,
        piirrite:hasDrinkingWaterName,
        piirrite:hasDrinkingWaterOperator ;
    piirrite:osmId "drinking_water" ;
    rdfs:subClassOf piirrite:OsmEntity ;
    skos:definition "A drinking water source which provides potable water for consumption.  osmcarto-rendering = File:Drinking-water-16.svg  osmcarto-rendering-size = 28px"@en ;
    skos:inScheme piirritev:Amenity ;
    skos:prefLabel "Drinking water"@en .

piirritev:AmenityDrivingSchool a skos:Concept ;
    piirrite:hasRelatedOsmTag piirrite:hasDrivingSchoolLicenseClasses,
        piirrite:hasDrivingSchoolName ;
    piirrite:osmId "driving_school" ;
    rdfs:subClassOf piirrite:OsmEntity ;
    skos:definition "A school to learn to drive a motor vehicle. osmcarto-rendering=File:Shop-other-16.svg osmcarto-rendering-size=28px"@en ;
    skos:inScheme piirritev:Amenity ;
    skos:prefLabel "Driving school"@en .

piirritev:AmenityEventsVenue a skos:Concept ;
    piirrite:hasRelatedOsmTag piirrite:hasEventsVenueAmenity,
        piirrite:hasEventsVenueOpeningHours,
        piirrite:hasEventsVenueOperator,
        piirrite:hasEventsVenuePhone,
        piirrite:hasEventsVenueWebsite,
        piirrite:hasEventsVenueWheelchair ;
    piirrite:osmId "events_venue" ;
    rdfs:subClassOf piirrite:OsmEntity ;
    skos:definition "A place that provides facilities for events such as banquets, weddings etc."@en ;
    skos:inScheme piirritev:Amenity ;
    skos:prefLabel "Events venue"@en .

piirritev:AmenityFastFood a skos:Concept ;
    piirrite:hasRelatedOsmTag piirrite:hasFastFoodCuisine,
        piirrite:hasFastFoodDelivery,
        piirrite:hasFastFoodName,
        piirrite:hasFastFoodTakeaway ;
    piirrite:osmId "fast_food" ;
    rdfs:subClassOf piirrite:OsmEntity ;
    skos:definition "A place which offers self-service and take-away food. osmcarto-rendering=File:Fast-food-16.svg osmcarto-rendering-size=28px"@en ;
    skos:inScheme piirritev:Amenity ;
    skos:prefLabel "Fast food"@en .

piirritev:AmenityFerryTerminal a skos:Concept ;
    piirrite:hasRelatedOsmTag piirrite:hasFerryTerminalCargo,
        piirrite:hasFerryTerminalName,
        piirrite:hasFerryTerminalOperator ;
    piirrite:osmId "ferry_terminal" ;
    rdfs:subClassOf piirrite:OsmEntity ;
    skos:definition "A place where people, cars etc. can board and leave a ferry. osmcarto-rendering = File:Ferry-icon.svg osmcarto-rendering-size = 28px osmcarto-rendering-area = File:Area transportation.png osmcarto-rendering-area-size = 100px"@en ;
    skos:inScheme piirritev:Amenity ;
    skos:prefLabel "Ferry terminal"@en .

piirritev:AmenityFireStation a skos:Concept ;
    piirrite:hasRelatedOsmTag piirrite:hasFireStationBranch,
        piirrite:hasFireStationBuilding,
        piirrite:hasFireStationName,
        piirrite:hasFireStationOperator,
        piirrite:hasFireStationPhone,
        piirrite:hasFireStationWebsite ;
    piirrite:osmId "fire_station" ;
    rdfs:subClassOf piirrite:OsmEntity ;
    skos:definition "A station from which a fire brigade operates."@en ;
    skos:inScheme piirritev:Amenity ;
    skos:prefLabel "Fire station"@en .

piirritev:AmenityFoodCourt a skos:Concept ;
    piirrite:hasRelatedOsmTag piirrite:hasFoodCourtCuisine,
        piirrite:hasFoodCourtName,
        piirrite:hasFoodCourtOpeningHours,
        piirrite:hasFoodCourtOperator,
        piirrite:hasFoodCourtPhone,
        piirrite:hasFoodCourtSeasonal,
        piirrite:hasFoodCourtSmoking,
        piirrite:hasFoodCourtWheelchair ;
    piirrite:osmId "food_court" ;
    rdfs:subClassOf piirrite:OsmEntity ;
    skos:definition "A place with sit-down facilities shared by multiple self-service food vendors. osmcarto-rendering=File:Restaurant-14.svg osmcarto-rendering-size=28px"@en ;
    skos:inScheme piirritev:Amenity ;
    skos:prefLabel "Food court"@en .

piirritev:AmenityFountain a skos:Concept ;
    piirrite:hasRelatedOsmTag piirrite:hasFountainDrinkingWater,
        piirrite:hasFountainName ;
    piirrite:osmId "fountain" ;
    rdfs:subClassOf piirrite:OsmEntity ;
    skos:definition "A fountain with cultural, decorational or historical significance or which serves a recreational purpose. osmcarto-rendering=File:Fountain-14.svg osmcarto-rendering-size=28px"@en ;
    skos:inScheme piirritev:Amenity ;
    skos:prefLabel "Fountain"@en .

piirritev:AmenityFuel a skos:Concept ;
    piirrite:hasRelatedOsmTag piirrite:hasFuelBrand,
        piirrite:hasFuelCapacity,
        piirrite:hasFuelMaxheight,
        piirrite:hasFuelName,
        piirrite:hasFuelOpeningHours,
        piirrite:hasFuelOperator,
        piirrite:hasFuelPhone,
        piirrite:hasFuelSelfService,
        piirrite:hasFuelWebsite ;
    piirrite:osmId "fuel" ;
    rdfs:subClassOf piirrite:OsmEntity ;
    skos:definition "A retail facility for refueling motor vehicles osmcarto-rendering=File:Fuel-16.svg osmcarto-rendering-size=28px"@en ;
    skos:inScheme piirritev:Amenity ;
    skos:prefLabel "Fuel"@en .

piirritev:AmenityGraveYard a skos:Concept ;
    piirrite:hasRelatedOsmTag piirrite:hasGraveYardName,
        piirrite:hasGraveYardReligion ;
    piirrite:osmId "grave_yard" ;
    rdfs:subClassOf piirrite:OsmEntity ;
    skos:definition "A place where people (or sometimes animals) are buried, usually close to a place of worship. osmcarto-rendering=File:Landuse-cemetery.png osmcarto-rendering-size=125px"@en ;
    skos:inScheme piirritev:Amenity ;
    skos:prefLabel "Grave yard"@en .

piirritev:AmenityGritBin a skos:Concept ;
    piirrite:hasRelatedOsmTag piirrite:hasGritBinAccess ;
    piirrite:osmId "grit_bin" ;
    rdfs:subClassOf piirrite:OsmEntity ;
    skos:definition "A container that holds sand, salt and gravel to spread on roads for winter safety."@en ;
    skos:inScheme piirritev:Amenity ;
    skos:prefLabel "Grit bin"@en .

piirritev:AmenityHospital a skos:Concept ;
    piirrite:hasRelatedOsmTag piirrite:hasHospitalBeds,
        piirrite:hasHospitalEmergency,
        piirrite:hasHospitalHealthcare,
        piirrite:hasHospitalName,
        piirrite:hasHospitalOperator,
        piirrite:hasHospitalPhone,
        piirrite:hasHospitalWebsite ;
    piirrite:osmId "hospital" ;
    rdfs:subClassOf piirrite:OsmEntity ;
    skos:definition "A hospital providing in-patient medical treatment. osmcarto-rendering=File:Hospital-14.svg osmcarto-rendering-size=28px osmcarto-rendering-area = File:Rendering-area-amenity-school.png osmcarto-rendering-area-size = 100px"@en ;
    skos:inScheme piirritev:Amenity ;
    skos:prefLabel "Hospital"@en .

piirritev:AmenityHuntingStand a skos:Concept ;
    piirrite:hasRelatedOsmTag piirrite:hasHuntingStandAmenity,
        piirrite:hasHuntingStandDirection,
        piirrite:hasHuntingStandHeight,
        piirrite:hasHuntingStandHide,
        piirrite:hasHuntingStandLadder,
        piirrite:hasHuntingStandLock,
        piirrite:hasHuntingStandLockable,
        piirrite:hasHuntingStandRaised,
        piirrite:hasHuntingStandShelter,
        piirrite:hasHuntingStandTree,
        piirrite:hasHuntingStandType ;
    piirrite:osmId "hunting_stand" ;
    rdfs:subClassOf piirrite:OsmEntity ;
    skos:definition "An open or enclosed platform used by hunters to place themselves, usually at an elevated height above the terrain."@en ;
    skos:inScheme piirritev:Amenity ;
    skos:prefLabel "Hunting stand"@en .

piirritev:AmenityIceCream a skos:Concept ;
    piirrite:hasRelatedOsmTag piirrite:hasIceCreamName,
        piirrite:hasIceCreamOpeningHours ;
    piirrite:osmId "ice_cream" ;
    rdfs:subClassOf piirrite:OsmEntity ;
    skos:definition "A place that sells ice cream and/or frozen yoghurt over the counter. osmcarto-rendering=File:Ice-cream-14.svg osmcarto-rendering-size=28px"@en ;
    skos:inScheme piirritev:Amenity ;
    skos:prefLabel "Ice cream"@en .

piirritev:AmenityInternetCafe a skos:Concept ;
    piirrite:hasRelatedOsmTag piirrite:hasInternetCafeAddr,
        piirrite:hasInternetCafeName,
        piirrite:hasInternetCafeOpeningHours,
        piirrite:hasInternetCafeOperator,
        piirrite:hasInternetCafeOutdoorSeating,
        piirrite:hasInternetCafeSmoking ;
    piirrite:osmId "internet_cafe" ;
    rdfs:subClassOf piirrite:OsmEntity ;
    skos:definition "A place whose principal role is providing internet services. osmcarto-rendering = File:Internet cafe-14.svg osmcarto-rendering-size = 28px"@en ;
    skos:inScheme piirritev:Amenity ;
    skos:prefLabel "Internet cafe"@en .

piirritev:AmenityKindergarten a skos:Concept ;
    piirrite:hasRelatedOsmTag piirrite:hasKindergartenName,
        piirrite:hasKindergartenOperator ;
    piirrite:osmId "kindergarten" ;
    rdfs:subClassOf piirrite:OsmEntity ;
    skos:definition "A place for looking after preschool children and (typically) giving early education. osmcarto-rendering-node=File:Rendering-amenity-kindergarten.png osmcarto-rendering-node-size=125px osmcarto-rendering-area=File:Rendering-area-amenity-school.png osmcarto-rendering-area-size=125px"@en ;
    skos:inScheme piirritev:Amenity ;
    skos:prefLabel "Kindergarten"@en .

piirritev:AmenityLavoir a skos:Concept ;
    piirrite:hasRelatedOsmTag piirrite:hasLavoirAccess,
        piirrite:hasLavoirCovered ;
    piirrite:osmId "lavoir" ;
    rdfs:subClassOf piirrite:OsmEntity ;
    skos:definition "A public place where people come to wash their clothes manually"@en ;
    skos:inScheme piirritev:Amenity ;
    skos:prefLabel "Lavoir"@en .

piirritev:AmenityLetterBox a skos:Concept ;
    piirrite:osmId "letter_box" ;
    rdfs:subClassOf piirrite:OsmEntity ;
    skos:definition "Private mailboxes where mailmen or other people deposit letters to specific addresses."@en ;
    skos:inScheme piirritev:Amenity ;
    skos:prefLabel "Letter box"@en .

piirritev:AmenityLibrary a skos:Concept ;
    piirrite:hasRelatedOsmTag piirrite:hasLibraryBooks,
        piirrite:hasLibraryName,
        piirrite:hasLibraryPhone,
        piirrite:hasLibraryWebsite ;
    piirrite:osmId "library" ;
    rdfs:subClassOf piirrite:OsmEntity ;
    skos:definition "A place to read and/or borrow books. osmcarto-rendering=File:Library-16.svg osmcarto-rendering-size=28px"@en ;
    skos:inScheme piirritev:Amenity ;
    skos:prefLabel "Library"@en .

piirritev:AmenityLoadingDock a skos:Concept ;
    piirrite:hasRelatedOsmTag piirrite:hasLoadingDockDoor,
        piirrite:hasLoadingDockMaxheight,
        piirrite:hasLoadingDockMaxlength,
        piirrite:hasLoadingDockMaxwidth,
        piirrite:hasLoadingDockRef ;
    piirrite:osmId "loading_dock" ;
    rdfs:subClassOf piirrite:OsmEntity ;
    skos:definition "A loading dock is an entrance to a building used for loading and unloading goods vehicles."@en ;
    skos:inScheme piirritev:Amenity ;
    skos:prefLabel "Loading dock"@en .

piirritev:AmenityLounger a skos:Concept ;
    piirrite:hasRelatedOsmTag piirrite:hasLoungerColour,
        piirrite:hasLoungerDirection,
        piirrite:hasLoungerMaterial,
        piirrite:hasLoungerOperator,
        piirrite:hasLoungerSeasonal ;
    piirrite:osmId "lounger" ;
    rdfs:subClassOf piirrite:OsmEntity ;
    skos:definition "An object for people to lie down."@en ;
    skos:inScheme piirritev:Amenity ;
    skos:prefLabel "Lounger"@en .

piirritev:AmenityMarketplace a skos:Concept ;
    piirrite:hasRelatedOsmTag piirrite:hasMarketplaceBuilding,
        piirrite:hasMarketplaceName,
        piirrite:hasMarketplaceOpeningHours,
        piirrite:hasMarketplaceOperator,
        piirrite:hasMarketplaceOrganic ;
    piirrite:osmId "marketplace" ;
    rdfs:subClassOf piirrite:OsmEntity ;
    skos:definition "A marketplace where goods and services are traded daily or weekly. osmcarto-rendering=File:Marketplace-14.svg osmcarto-rendering-size=28px osmcarto-rendering-area=File:Landuse-retail.png osmcarto-rendering-area-size=100px"@en ;
    skos:inScheme piirritev:Amenity ;
    skos:prefLabel "Marketplace"@en .

piirritev:AmenityMonastery a skos:Concept ;
    piirrite:hasRelatedOsmTag piirrite:hasMonasteryCommunity,
        piirrite:hasMonasteryName,
        piirrite:hasMonasteryReligion ;
    piirrite:osmId "monastery" ;
    rdfs:subClassOf piirrite:OsmEntity ;
    skos:definition "An active monastery or convent, occupied by a community of monks or nuns living under religious vows."@en ;
    skos:inScheme piirritev:Amenity ;
    skos:prefLabel "Monastery"@en .

piirritev:AmenityMotorcycleParking a skos:Concept ;
    piirrite:hasRelatedOsmTag piirrite:hasMotorcycleParkingAccess,
        piirrite:hasMotorcycleParkingBuilding,
        piirrite:hasMotorcycleParkingCapacity,
        piirrite:hasMotorcycleParkingCovered,
        piirrite:hasMotorcycleParkingFee,
        piirrite:hasMotorcycleParkingMaxstay,
        piirrite:hasMotorcycleParkingName,
        piirrite:hasMotorcycleParkingOperator,
        piirrite:hasMotorcycleParkingParking,
        piirrite:hasMotorcycleParkingRef ;
    piirrite:osmId "motorcycle_parking" ;
    rdfs:subClassOf piirrite:OsmEntity ;
    skos:definition "A place which is designated for parking motorcycles."@en ;
    skos:inScheme piirritev:Amenity ;
    skos:prefLabel "Motorcycle parking"@en .

piirritev:AmenityMusicSchool a skos:Concept ;
    piirrite:hasRelatedOsmTag piirrite:hasMusicSchoolName,
        piirrite:hasMusicSchoolOperator,
        piirrite:hasMusicSchoolPhone,
        piirrite:hasMusicSchoolWebsite,
        piirrite:hasMusicSchoolWheelchair ;
    piirrite:osmId "music_school" ;
    rdfs:subClassOf piirrite:OsmEntity ;
    skos:definition "Music school, an educational institution specialized in the study, training, and research of music"@en ;
    skos:inScheme piirritev:Amenity ;
    skos:prefLabel "Music school"@en .

piirritev:AmenityNightclub a skos:Concept ;
    piirrite:hasRelatedOsmTag piirrite:hasNightclubLiveMusic,
        piirrite:hasNightclubMusic,
        piirrite:hasNightclubName,
        piirrite:hasNightclubOpeningHours,
        piirrite:hasNightclubOperator,
        piirrite:hasNightclubPhone,
        piirrite:hasNightclubWebsite,
        piirrite:hasNightclubWheelchair ;
    piirrite:osmId "nightclub" ;
    rdfs:subClassOf piirrite:OsmEntity ;
    skos:definition "A place to dance and drink at night. Also known as a disco. osmcarto-rendering=File:Nightclub-16.svg osmcarto-rendering-size=28px"@en ;
    skos:inScheme piirritev:Amenity ;
    skos:prefLabel "Nightclub"@en .

piirritev:AmenityNursingHome a skos:Concept ;
    piirrite:hasRelatedOsmTag piirrite:hasNursingHomeBuilding,
        piirrite:hasNursingHomePhone,
        piirrite:hasNursingHomeWebsite ;
    piirrite:osmId "nursing_home" ;
    rdfs:subClassOf piirrite:OsmEntity ;
    skos:definition "A home for disabled/elderly persons who need permanent care. osmcarto-rendering=File:Social amenity darken 80-16.svg osmcarto-rendering-size=28px"@en ;
    skos:inScheme piirritev:Amenity ;
    skos:prefLabel "Nursing home"@en .

piirritev:AmenityParcelLocker a skos:Concept ;
    piirrite:osmId "parcel_locker" ;
    rdfs:subClassOf piirrite:OsmEntity ;
    skos:definition "Machine for picking up and sending parcels.  osmcarto-rendering = File:Parcel locker.svg  osmcarto-rendering-size = 28px"@en ;
    skos:inScheme piirritev:Amenity ;
    skos:prefLabel "Parcel locker"@en .

piirritev:AmenityParking a skos:Concept ;
    piirrite:hasRelatedOsmTag piirrite:hasParkingAccess,
        piirrite:hasParkingCapacity,
        piirrite:hasParkingFee,
        piirrite:hasParkingMaxstay,
        piirrite:hasParkingName,
        piirrite:hasParkingOperator,
        piirrite:hasParkingType ;
    piirrite:osmId "parking" ;
    rdfs:subClassOf piirrite:OsmEntity ;
    skos:definition "A place for parking cars."@en ;
    skos:inScheme piirritev:Amenity ;
    skos:prefLabel "Parking"@en .

piirritev:AmenityParkingEntrance a skos:Concept ;
    piirrite:hasRelatedOsmTag piirrite:hasParkingEntranceParking ;
    piirrite:osmId "parking_entrance" ;
    rdfs:subClassOf piirrite:OsmEntity ;
    skos:definition "An entrance to an underground or multi storey parking facility."@en ;
    skos:inScheme piirritev:Amenity ;
    skos:prefLabel "Parking entrance"@en .

piirritev:AmenityParkingSpace a skos:Concept ;
    piirrite:hasRelatedOsmTag piirrite:hasParkingSpaceSite,
        piirrite:hasParkingSpaceType ;
    piirrite:osmId "parking_space" ;
    rdfs:subClassOf piirrite:OsmEntity ;
    skos:definition "A single parking space on a parking lot. osmcarto-rendering=File:Rendering-parking space.png osmcarto-rendering-size=125px"@en ;
    skos:inScheme piirritev:Amenity ;
    skos:prefLabel "Parking space"@en .

piirritev:AmenityPaymentTerminal a skos:Concept ;
    piirrite:hasRelatedOsmTag piirrite:hasPaymentTerminalBrand,
        piirrite:hasPaymentTerminalOperator ;
    piirrite:osmId "payment_terminal" ;
    rdfs:subClassOf piirrite:OsmEntity ;
    skos:definition "Self-service payment kiosk/terminal."@en ;
    skos:inScheme piirritev:Amenity ;
    skos:prefLabel "Payment terminal"@en .

piirritev:AmenityPharmacy a skos:Concept ;
    piirrite:hasRelatedOsmTag piirrite:hasPharmacyDispensing,
        piirrite:hasPharmacyDriveThrough,
        piirrite:hasPharmacyHealthcare,
        piirrite:hasPharmacyMedicalSupply,
        piirrite:hasPharmacyName,
        piirrite:hasPharmacyOperator,
        piirrite:hasPharmacyWebsite ;
    piirrite:osmId "pharmacy" ;
    rdfs:subClassOf piirrite:OsmEntity ;
    skos:definition "A shop where a pharmacist sells medications."@en ;
    skos:inScheme piirritev:Amenity ;
    skos:prefLabel "Pharmacy"@en .

piirritev:AmenityPolice a skos:Concept ;
    piirrite:hasRelatedOsmTag piirrite:hasPoliceDetention,
        piirrite:hasPoliceName,
        piirrite:hasPoliceOpeningHours,
        piirrite:hasPoliceOperator,
        piirrite:hasPoliceType,
        piirrite:hasPoliceWheelchair ;
    piirrite:osmId "police" ;
    rdfs:subClassOf piirrite:OsmEntity ;
    skos:definition "A police station is a facility where police officers patrol from and that is a first point of contact for civilians. osmcarto-rendering=File:Police-16.svg osmcarto-rendering-size=24px osmcarto-rendering-area=File:Police fire station 100.png osmcarto-rendering-area-size=100px"@en ;
    skos:inScheme piirritev:Amenity ;
    skos:prefLabel "Police"@en .

piirritev:AmenityPostBox a skos:Concept ;
    piirrite:hasRelatedOsmTag piirrite:hasPostBoxCheckDate,
        piirrite:hasPostBoxCollectionTimes,
        piirrite:hasPostBoxDriveThrough,
        piirrite:hasPostBoxOperator,
        piirrite:hasPostBoxRef ;
    piirrite:osmId "post_box" ;
    rdfs:subClassOf piirrite:OsmEntity ;
    skos:definition "A box to deposit outgoing postal items."@en ;
    skos:inScheme piirritev:Amenity ;
    skos:prefLabel "Post box"@en .

piirritev:AmenityPostOffice a skos:Concept ;
    piirrite:hasRelatedOsmTag piirrite:hasPostOfficeAmenity,
        piirrite:hasPostOfficeAtm,
        piirrite:hasPostOfficeBrand,
        piirrite:hasPostOfficeChangeMachine,
        piirrite:hasPostOfficeName,
        piirrite:hasPostOfficeOperator,
        piirrite:hasPostOfficeRef,
        piirrite:hasPostOfficeType,
        piirrite:hasPostOfficeVending ;
    piirrite:osmId "post_office" ;
    rdfs:subClassOf piirrite:OsmEntity ;
    skos:definition "A place where letters and parcels may be sent or collected. osmcarto-rendering=File:Post office-14.svg osmcarto-rendering-size=28px"@en ;
    skos:inScheme piirritev:Amenity ;
    skos:prefLabel "Post office"@en .

piirritev:AmenityPrepSchool a skos:Concept ;
    piirrite:hasRelatedOsmTag piirrite:hasPrepSchoolName,
        piirrite:hasPrepSchoolOpeningHours ;
    piirrite:osmId "prep_school" ;
    rdfs:subClassOf piirrite:OsmEntity ;
    skos:definition "Tutor or test prep centre."@en ;
    skos:inScheme piirritev:Amenity ;
    skos:prefLabel "Prep school"@en .

piirritev:AmenityPrison a skos:Concept ;
    piirrite:hasRelatedOsmTag piirrite:hasPrisonAccess,
        piirrite:hasPrisonBarrier,
        piirrite:hasPrisonName,
        piirrite:hasPrisonOperator,
        piirrite:hasPrisonType ;
    piirrite:osmId "prison" ;
    rdfs:subClassOf piirrite:OsmEntity ;
    skos:definition "A prison or jail where people are incarcerated before trial or after conviction osmcarto-rendering=File:Prison-16.svg osmcarto-rendering-size=28px osmcarto-rendering-area=File:Area_amenity%3Dprison.png osmcarto-rendering-area-size=100px"@en ;
    skos:inScheme piirritev:Amenity ;
    skos:prefLabel "Prison"@en .

piirritev:AmenityPub a skos:Concept ;
    piirrite:hasRelatedOsmTag piirrite:hasPubBrewery,
        piirrite:hasPubContact,
        piirrite:hasPubCuisine,
        piirrite:hasPubDistillery,
        piirrite:hasPubDrink,
        piirrite:hasPubInternetAccess,
        piirrite:hasPubLiveMusic,
        piirrite:hasPubMicrobrewery,
        piirrite:hasPubName,
        piirrite:hasPubOpeningHours,
        piirrite:hasPubOperator,
        piirrite:hasPubOutdoorSeating,
        piirrite:hasPubWinery ;
    piirrite:osmId "pub" ;
    rdfs:subClassOf piirrite:OsmEntity ;
    skos:definition "osmcarto-rendering=File:Pub-16.svg osmcarto-rendering-size=28px"@en ;
    skos:inScheme piirritev:Amenity ;
    skos:prefLabel "Pub"@en .

piirritev:AmenityPublicBath a skos:Concept ;
    piirrite:hasRelatedOsmTag piirrite:hasPublicBathFee,
        piirrite:hasPublicBathFemale,
        piirrite:hasPublicBathGenderSegregated,
        piirrite:hasPublicBathMale,
        piirrite:hasPublicBathName,
        piirrite:hasPublicBathNudism,
        piirrite:hasPublicBathOutdoor,
        piirrite:hasPublicBathShower,
        piirrite:hasPublicBathUnisex ;
    piirrite:osmId "public_bath" ;
    rdfs:subClassOf piirrite:OsmEntity ;
    skos:definition "A facility for communal bathing that is open to the public."@en ;
    skos:inScheme piirritev:Amenity ;
    skos:prefLabel "Public bath"@en .

piirritev:AmenityPublicBookcase a skos:Concept ;
    piirrite:hasRelatedOsmTag piirrite:hasPublicBookcaseBrand,
        piirrite:hasPublicBookcaseCapacity,
        piirrite:hasPublicBookcaseDescription,
        piirrite:hasPublicBookcaseLocation,
        piirrite:hasPublicBookcaseName,
        piirrite:hasPublicBookcaseOpeningHours,
        piirrite:hasPublicBookcaseOperator,
        piirrite:hasPublicBookcaseWebsite ;
    piirrite:osmId "public_bookcase" ;
    rdfs:subClassOf piirrite:OsmEntity ;
    skos:definition "A street furniture containing books. Take one, leave one."@en ;
    skos:inScheme piirritev:Amenity ;
    skos:prefLabel "Public bookcase"@en .

piirritev:AmenityPublicBuilding a skos:Concept ;
    piirrite:osmId "public_building" ;
    rdfs:subClassOf piirrite:OsmEntity ;
    skos:definition "Using this tag is discouraged, use tag:building=public or tag:building=civic or a feature tag like tag:office=government, tag:amenity=townhall instead."@en ;
    skos:inScheme piirritev:Amenity ;
    skos:prefLabel "Public building"@en .

piirritev:AmenityRecycling a skos:Concept ;
    piirrite:hasRelatedOsmTag piirrite:hasRecyclingCapacity,
        piirrite:hasRecyclingFee,
        piirrite:hasRecyclingOpeningHours,
        piirrite:hasRecyclingOperator,
        piirrite:hasRecyclingRef ;
    piirrite:osmId "recycling" ;
    rdfs:subClassOf piirrite:OsmEntity ;
    skos:definition "A container or centre that accepts waste material for reuse or recycling. osmcarto-rendering=File:Recycling-16.svg osmcarto-rendering-size=28px"@en ;
    skos:inScheme piirritev:Amenity ;
    skos:prefLabel "Recycling"@en .

piirritev:AmenityRestaurant a skos:Concept ;
    piirrite:hasRelatedOsmTag piirrite:hasRestaurantAirConditioning,
        piirrite:hasRestaurantAmenity,
        piirrite:hasRestaurantBar,
        piirrite:hasRestaurantBrand,
        piirrite:hasRestaurantBreakfast,
        piirrite:hasRestaurantCapacity,
        piirrite:hasRestaurantChangingTable,
        piirrite:hasRestaurantCuisine,
        piirrite:hasRestaurantDelivery,
        piirrite:hasRestaurantDinner,
        piirrite:hasRestaurantDog,
        piirrite:hasRestaurantDriveThrough,
        piirrite:hasRestaurantHighchair,
        piirrite:hasRestaurantImage,
        piirrite:hasRestaurantInternetAccess,
        piirrite:hasRestaurantKidsArea,
        piirrite:hasRestaurantLevel,
        piirrite:hasRestaurantLunch,
        piirrite:hasRestaurantMicrobrewery,
        piirrite:hasRestaurantName,
        piirrite:hasRestaurantOpeningHours,
        piirrite:hasRestaurantOperator,
        piirrite:hasRestaurantOutdoorSeating,
        piirrite:hasRestaurantPhone,
        piirrite:hasRestaurantReservation,
        piirrite:hasRestaurantSmoking,
        piirrite:hasRestaurantStars,
        piirrite:hasRestaurantStartDate,
        piirrite:hasRestaurantTakeaway,
        piirrite:hasRestaurantTelevision,
        piirrite:hasRestaurantToilets,
        piirrite:hasRestaurantWebsite,
        piirrite:hasRestaurantWheelchair,
        piirrite:hasRestaurantWikimediaCommons ;
    piirrite:osmId "restaurant" ;
    rdfs:subClassOf piirrite:OsmEntity ;
    skos:definition "A restaurant sells full sit-down meals with servers, and may sell alcohol.  osmcarto-rendering = File:Restaurant-14.svg  osmcarto-rendering-size = 28px"@en ;
    skos:inScheme piirritev:Amenity ;
    skos:prefLabel "Restaurant"@en .

piirritev:AmenitySchool a skos:Concept ;
    piirrite:hasRelatedOsmTag piirrite:hasSchoolName,
        piirrite:hasSchoolOperator ;
    piirrite:osmId "school" ;
    rdfs:subClassOf piirrite:OsmEntity ;
    skos:definition "A primary or secondary school (pupils typically aged 6 to 18). osmcarto-rendering-node = File:Rendering-amenity-school.png osmcarto-rendering-node-size = 125px osmcarto-rendering-area = File:Rendering-area-amenity-school.png osmcarto-rendering-area-size = 125px"@en ;
    skos:inScheme piirritev:Amenity ;
    skos:prefLabel "School"@en .

piirritev:AmenityShelter a skos:Concept ;
    piirrite:hasRelatedOsmTag piirrite:hasShelterAccess,
        piirrite:hasShelterBench,
        piirrite:hasShelterBin,
        piirrite:hasShelterBuilding,
        piirrite:hasShelterDrinkingWater,
        piirrite:hasShelterHighway,
        piirrite:hasShelterLockable,
        piirrite:hasShelterLocked,
        piirrite:hasShelterPicnicTable,
        piirrite:hasShelterPublicTransport,
        piirrite:hasShelterShelterType,
        piirrite:hasShelterSurface,
        piirrite:hasShelterTable,
        piirrite:hasShelterTourism,
        piirrite:hasShelterType ;
    piirrite:osmId "shelter" ;
    rdfs:subClassOf piirrite:OsmEntity ;
    skos:definition "A small structure for protection against bad weather conditions osmcarto-rendering=File:Shelter-14.svg osmcarto-rendering-size=28px"@en ;
    skos:inScheme piirritev:Amenity ;
    skos:prefLabel "Shelter"@en .

piirritev:AmenityShower a skos:Concept ;
    piirrite:hasRelatedOsmTag piirrite:hasShowerAccess,
        piirrite:hasShowerCapacity,
        piirrite:hasShowerCentralkey,
        piirrite:hasShowerFee,
        piirrite:hasShowerFemale,
        piirrite:hasShowerHotWater,
        piirrite:hasShowerIndoor,
        piirrite:hasShowerMale,
        piirrite:hasShowerName,
        piirrite:hasShowerOpeningHours,
        piirrite:hasShowerOperator,
        piirrite:hasShowerOutdoor,
        piirrite:hasShowerSupervised,
        piirrite:hasShowerUnisex,
        piirrite:hasShowerWheelchair ;
    piirrite:osmId "shower" ;
    rdfs:subClassOf piirrite:OsmEntity ;
    skos:definition "Public showers, where people can bathe under water sprays"@en ;
    skos:inScheme piirritev:Amenity ;
    skos:prefLabel "Shower"@en .

piirritev:AmenitySocialCentre a skos:Concept ;
    piirrite:hasRelatedOsmTag piirrite:hasSocialCentreBuilding,
        piirrite:hasSocialCentreName ;
    piirrite:osmId "social_centre" ;
    rdfs:subClassOf piirrite:OsmEntity ;
    skos:definition "A centre of fraternities, sororities, professional societies, union halls and other nonprofit organizations."@en ;
    skos:inScheme piirritev:Amenity ;
    skos:prefLabel "Social centre"@en .

piirritev:AmenitySocialFacility a skos:Concept ;
    piirrite:hasRelatedOsmTag piirrite:hasSocialFacilityName,
        piirrite:hasSocialFacilityType ;
    piirrite:osmId "social_facility" ;
    rdfs:subClassOf piirrite:OsmEntity ;
    skos:definition "A facility that provides social services."@en ;
    skos:inScheme piirritev:Amenity ;
    skos:prefLabel "Social facility"@en .

piirritev:AmenityStudio a skos:Concept ;
    piirrite:hasRelatedOsmTag piirrite:hasStudioName,
        piirrite:hasStudioPhone,
        piirrite:hasStudioType,
        piirrite:hasStudioWebsite ;
    piirrite:osmId "studio" ;
    rdfs:subClassOf piirrite:OsmEntity ;
    skos:definition "A studio used for creating radio or television programmes and broadcasting them. It can also be used to mark a music recording studio."@en ;
    skos:inScheme piirritev:Amenity ;
    skos:prefLabel "Studio"@en .

piirritev:AmenityTaxi a skos:Concept ;
    piirrite:hasRelatedOsmTag piirrite:hasTaxiName,
        piirrite:hasTaxiOperator,
        piirrite:hasTaxiPhone,
        piirrite:hasTaxiTaxiVehicle ;
    piirrite:osmId "taxi" ;
    rdfs:subClassOf piirrite:OsmEntity ;
    skos:definition "A place where taxis wait for passengers. Often near where many people congregate. osmcarto-rendering=File:Taxi.16.svg osmcarto-rendering-size=28px osmcarto-rendering-area=File:Area parking.png osmcarto-rendering-area-size=100px"@en ;
    skos:inScheme piirritev:Amenity ;
    skos:prefLabel "Taxi"@en .

piirritev:AmenityTelephone a skos:Concept ;
    piirrite:hasRelatedOsmTag piirrite:hasTelephoneIndoor,
        piirrite:hasTelephoneOperator,
        piirrite:hasTelephonePhone,
        piirrite:hasTelephoneRef ;
    piirrite:osmId "telephone" ;
    rdfs:subClassOf piirrite:OsmEntity ;
    skos:definition "A public telephone. osmcarto-rendering=File:Telephone.16.svg osmcarto-rendering-size=28px"@en ;
    skos:inScheme piirritev:Amenity ;
    skos:prefLabel "Telephone"@en .

piirritev:AmenityTheatre a skos:Concept ;
    piirrite:hasRelatedOsmTag piirrite:hasTheatreName,
        piirrite:hasTheatreOpeningHours,
        piirrite:hasTheatreOperator,
        piirrite:hasTheatrePhone,
        piirrite:hasTheatreWebsite,
        piirrite:hasTheatreWheelchair ;
    piirrite:osmId "theatre" ;
    rdfs:subClassOf piirrite:OsmEntity ;
    skos:definition "A place where live performances occur, such as plays, musicals and formal concerts.  osmcarto-rendering = File:Theatre-16.svg  osmcarto-rendering-size = 28px"@en ;
    skos:inScheme piirritev:Amenity ;
    skos:prefLabel "Theatre"@en .

piirritev:AmenityTicketValidator a skos:Concept ;
    piirrite:hasRelatedOsmTag piirrite:hasTicketValidatorBarrier,
        piirrite:hasTicketValidatorNetwork,
        piirrite:hasTicketValidatorOperator ;
    piirrite:osmId "ticket_validator" ;
    rdfs:subClassOf piirrite:OsmEntity ;
    skos:definition "An analog device which validates public transport tickets, or devices which are integrated in systems to gain access to an area or service like public transport or parking garages."@en ;
    skos:inScheme piirritev:Amenity ;
    skos:prefLabel "Ticket validator"@en .

piirritev:AmenityToilets a skos:Concept ;
    piirrite:hasRelatedOsmTag piirrite:hasToiletsChangingTable,
        piirrite:hasToiletsComposting,
        piirrite:hasToiletsDrinkingWater,
        piirrite:hasToiletsFee,
        piirrite:hasToiletsHotWater,
        piirrite:hasToiletsIndoor,
        piirrite:hasToiletsOpeningHours,
        piirrite:hasToiletsOperator,
        piirrite:hasToiletsSupervised,
        piirrite:hasToiletsType,
        piirrite:hasToiletsWheelchair ;
    piirrite:osmId "toilets" ;
    rdfs:subClassOf piirrite:OsmEntity ;
    skos:definition "Indicates publicly accessible toilets.  osmcarto-rendering = File:Toilets-16.svg  osmcarto-rendering-size = 28px"@en ;
    skos:inScheme piirritev:Amenity ;
    skos:prefLabel "Toilets"@en .

piirritev:AmenityTownhall a skos:Concept ;
    piirrite:hasRelatedOsmTag piirrite:hasTownhallBuilding,
        piirrite:hasTownhallName,
        piirrite:hasTownhallOperator ;
    piirrite:osmId "townhall" ;
    rdfs:subClassOf piirrite:OsmEntity ;
    skos:definition "A townhall serves as a community administrative center or meeting place. osmcarto-rendering=File:Town-hall-16.svg osmcarto-rendering-size=28px"@en ;
    skos:inScheme piirritev:Amenity ;
    skos:prefLabel "Townhall"@en .

piirritev:AmenityTrolleyBay a skos:Concept ;
    piirrite:osmId "trolley_bay" ;
    rdfs:subClassOf piirrite:OsmEntity ;
    skos:definition "A trolley bay (aka cart corral) is the place where trolleys are \"parked\"."@en ;
    skos:inScheme piirritev:Amenity ;
    skos:prefLabel "Trolley bay"@en .

piirritev:AmenityUniversity a skos:Concept ;
    piirrite:hasRelatedOsmTag piirrite:hasUniversityName,
        piirrite:hasUniversityOperator,
        piirrite:hasUniversityType ;
    piirrite:osmId "university" ;
    rdfs:subClassOf piirrite:OsmEntity ;
    skos:definition "An educational institution designed for instruction, examination, or both, of students in many branches of advanced learning."@en ;
    skos:inScheme piirritev:Amenity ;
    skos:prefLabel "University"@en .

piirritev:AmenityVehicleInspection a skos:Concept ;
    piirrite:hasRelatedOsmTag piirrite:hasVehicleInspectionName,
        piirrite:hasVehicleInspectionOpeningHours,
        piirrite:hasVehicleInspectionOperator,
        piirrite:hasVehicleInspectionPhone,
        piirrite:hasVehicleInspectionWebsite ;
    piirrite:osmId "vehicle_inspection" ;
    rdfs:subClassOf piirrite:OsmEntity ;
    skos:definition "A place where legally-required vehicle inspection may be performed osmcarto-rendering = File:Vehicle inspection-14.svg osmcarto-rendering-size = 28px"@en ;
    skos:inScheme piirritev:Amenity ;
    skos:prefLabel "Vehicle inspection"@en .

piirritev:AmenityVendingMachine a skos:Concept ;
    piirrite:hasRelatedOsmTag piirrite:hasVendingMachineOperator,
        piirrite:hasVendingMachineRef,
        piirrite:hasVendingMachineVending ;
    piirrite:osmId "vending_machine" ;
    rdfs:subClassOf piirrite:OsmEntity ;
    skos:definition "A vending machine sells food, drinks, tickets or other goods automatically."@en ;
    skos:inScheme piirritev:Amenity ;
    skos:prefLabel "Vending machine"@en .

piirritev:AmenityVeterinary a skos:Concept ;
    piirrite:hasRelatedOsmTag piirrite:hasVeterinaryName ;
    piirrite:osmId "veterinary" ;
    rdfs:subClassOf piirrite:OsmEntity ;
    skos:definition "A place that deals with the prevention, diagnosis and treatment of disease in animals. osmcarto-rendering=File:Veterinary-14.svg osmcarto-rendering-size=28px"@en ;
    skos:inScheme piirritev:Amenity ;
    skos:prefLabel "Veterinary"@en .

piirritev:AmenityWasteBasket a skos:Concept ;
    piirrite:hasRelatedOsmTag piirrite:hasWasteBasketWaste ;
    piirrite:osmId "waste_basket" ;
    rdfs:subClassOf piirrite:OsmEntity ;
    skos:definition "A single small container for depositing garbage that is easily accessible for pedestrians. osmcarto-rendering=File:Waste-basket-12.svg osmcarto-rendering-size=24px"@en ;
    skos:inScheme piirritev:Amenity ;
    skos:prefLabel "Waste basket"@en .

piirritev:AmenityWasteDisposal a skos:Concept ;
    piirrite:hasRelatedOsmTag piirrite:hasWasteDisposalAccess,
        piirrite:hasWasteDisposalFee,
        piirrite:hasWasteDisposalOperator,
        piirrite:hasWasteDisposalWaste ;
    piirrite:osmId "waste_disposal" ;
    rdfs:subClassOf piirrite:OsmEntity ;
    skos:definition "A medium or large disposal bin, typically for bagged up household or industrial waste."@en ;
    skos:inScheme piirritev:Amenity ;
    skos:prefLabel "Waste disposal"@en .

piirritev:AmenityWaterPoint a skos:Concept ;
    piirrite:osmId "water_point" ;
    rdfs:subClassOf piirrite:OsmEntity ;
    skos:definition "A place where you can get large amounts of drinking water for refilling fresh water holding tanks."@en ;
    skos:inScheme piirritev:Amenity ;
    skos:prefLabel "Water point"@en .

piirritev:AmenityWateringPlace a skos:Concept ;
    piirrite:hasRelatedOsmTag piirrite:hasWateringPlaceName ;
    piirrite:osmId "watering_place" ;
    rdfs:subClassOf piirrite:OsmEntity ;
    skos:definition "A place where water is contained and animals such as horses can drink."@en ;
    skos:inScheme piirritev:Amenity ;
    skos:prefLabel "Watering place"@en .

piirritev:AmenityWeighbridge a skos:Concept ;
    piirrite:hasRelatedOsmTag piirrite:hasWeighbridgeHighway,
        piirrite:hasWeighbridgeOperator ;
    piirrite:osmId "weighbridge" ;
    rdfs:subClassOf piirrite:OsmEntity ;
    skos:definition "A large weight scale to weigh vehicles and goods."@en ;
    skos:inScheme piirritev:Amenity ;
    skos:prefLabel "Weighbridge"@en .

piirritev:Area a skos:ConceptScheme ;
    piirrite:osmId "area" ;
    skos:definition "Indicates whether a closed way represents an area or just a circular way."@en ;
    skos:prefLabel "Area, types"@en .

piirritev:Armrest a skos:ConceptScheme ;
    piirrite:osmId "armrest" ;
    skos:definition "Whether a bench has any armrests."@en ;
    skos:prefLabel "Armrest, types"@en .

piirritev:ArtistName a skos:ConceptScheme ;
    piirrite:osmId "artist_name" ;
    skos:definition "A name of an artist who created the piece of art."@en ;
    skos:prefLabel "Artist name, types"@en .

piirritev:ArtworkType a skos:ConceptScheme ;
    piirrite:osmId "artwork_type" ;
    skos:definition "Describes the type of an artwork."@en ;
    skos:prefLabel "Artwork type, types"@en .

piirritev:Atm a skos:ConceptScheme ;
    piirrite:osmId "atm" ;
    skos:definition ""@en ;
    skos:prefLabel "Atm, types"@en .

piirritev:AttributionBakersfieldGis a skos:Concept ;
    piirrite:osmId "Bakersfield_GIS" ;
    rdfs:subClassOf piirrite:OsmEntity ;
    skos:definition ""@en ;
    skos:inScheme piirritev:Attribution ;
    skos:prefLabel "Bakersfield gis"@en .

piirritev:AttributionMassdot a skos:Concept ;
    piirrite:osmId "massDOT" ;
    rdfs:subClassOf piirrite:OsmEntity ;
    skos:definition ""@en ;
    skos:inScheme piirritev:Attribution ;
    skos:prefLabel "Massdot"@en .

piirritev:AttributionNhd a skos:Concept ;
    piirrite:osmId "NHD" ;
    rdfs:subClassOf piirrite:OsmEntity ;
    skos:definition ""@en ;
    skos:inScheme piirritev:Attribution ;
    skos:prefLabel "Nhd"@en .

piirritev:AttributionTiger a skos:Concept ;
    piirrite:osmId "tiger" ;
    rdfs:subClassOf piirrite:OsmEntity ;
    skos:definition ""@en ;
    skos:inScheme piirritev:Attribution ;
    skos:prefLabel "Tiger"@en .

piirritev:AttributionUs-Nfs a skos:Concept ;
    piirrite:osmId "US-NFS" ;
    rdfs:subClassOf piirrite:OsmEntity ;
    skos:definition ""@en ;
    skos:inScheme piirritev:Attribution ;
    skos:prefLabel "Us-nfs"@en .

piirritev:AttributionUs-Nps a skos:Concept ;
    piirrite:osmId "US-NPS" ;
    rdfs:subClassOf piirrite:OsmEntity ;
    skos:definition ""@en ;
    skos:inScheme piirritev:Attribution ;
    skos:prefLabel "Us-nps"@en .

piirritev:AttributionUsgs-Nhd a skos:Concept ;
    piirrite:osmId "USGS-NHD" ;
    rdfs:subClassOf piirrite:OsmEntity ;
    skos:definition ""@en ;
    skos:inScheme piirritev:Attribution ;
    skos:prefLabel "Usgs-nhd"@en .

piirritev:Backrest a skos:ConceptScheme ;
    piirrite:osmId "backrest" ;
    skos:definition "Whether a bench has a backrest (or backrests)."@en ;
    skos:prefLabel "Backrest, types"@en .

piirritev:BarrierBlock a skos:Concept ;
    piirrite:osmId "block" ;
    rdfs:subClassOf piirrite:OsmEntity ;
    skos:definition "One or more large immobile block(s) usually barring free access along a way. osmcarto-rendering=File:Barrier.svg osmcarto-rendering-size=28px"@en ;
    skos:inScheme piirritev:Barrier ;
    skos:prefLabel "Block"@en .

piirritev:BarrierBollard a skos:Concept ;
    piirrite:hasRelatedOsmTag piirrite:hasBollardType ;
    piirrite:osmId "bollard" ;
    rdfs:subClassOf piirrite:OsmEntity ;
    skos:definition "One or more solid (usually concrete or metal) pillar(s) used to control traffic.  osmcarto-rendering = File:Barrier.svg  osmcarto-rendering-size = 28px"@en ;
    skos:inScheme piirritev:Barrier ;
    skos:prefLabel "Bollard"@en .

piirritev:BarrierCattleGrid a skos:Concept ;
    piirrite:osmId "cattle_grid" ;
    rdfs:subClassOf piirrite:OsmEntity ;
    skos:definition "A hole in the road surface covered in a series of bars that allow wheeled vehicles but not animals to cross.  osmcarto-rendering = File:Barrier cattle grid-14.svg  osmcarto-rendering-size = 28px"@en ;
    skos:inScheme piirritev:Barrier ;
    skos:prefLabel "Cattle grid"@en .

piirritev:BarrierChain a skos:Concept ;
    piirrite:hasRelatedOsmTag piirrite:hasChainAccess,
        piirrite:hasChainLocked,
        piirrite:hasChainWheelchair ;
    piirrite:osmId "chain" ;
    rdfs:subClassOf piirrite:OsmEntity ;
    skos:definition "A chain used to prevent motorised vehicles. osmcarto-rendering=File:Barrier fence mapnik.png osmcarto-rendering-size=125px"@en ;
    skos:inScheme piirritev:Barrier ;
    skos:prefLabel "Chain"@en .

piirritev:BarrierCityWall a skos:Concept ;
    piirrite:hasRelatedOsmTag piirrite:hasCityWallHistoric,
        piirrite:hasCityWallTwoSided ;
    piirrite:osmId "city_wall" ;
    rdfs:subClassOf piirrite:OsmEntity ;
    skos:definition "A fortification used to defend settlements in ancient to modern times.  osmcarto-rendering = File:City-wall-render-eg1.png  osmcarto-rendering-size = 125px"@en ;
    skos:inScheme piirritev:Barrier ;
    skos:prefLabel "City wall"@en .

piirritev:BarrierCycleBarrier a skos:Concept ;
    piirrite:hasRelatedOsmTag piirrite:hasCycleBarrierAccess,
        piirrite:hasCycleBarrierOpening,
        piirrite:hasCycleBarrierOverlap,
        piirrite:hasCycleBarrierSpacing,
        piirrite:hasCycleBarrierType,
        piirrite:hasCycleBarrierWheelchair ;
    piirrite:osmId "cycle_barrier" ;
    rdfs:subClassOf piirrite:OsmEntity ;
    skos:definition "A barrier along a path that slows or prevents access for bicycle users. osmcarto-rendering=File:Cycle barrier-14.svg osmcarto-rendering-size=28px"@en ;
    skos:inScheme piirritev:Barrier ;
    skos:prefLabel "Cycle barrier"@en .

piirritev:BarrierDitch a skos:Concept ;
    piirrite:hasRelatedOsmTag piirrite:hasDitchIntermittent,
        piirrite:hasDitchType,
        piirrite:hasDitchWidth ;
    piirrite:osmId "ditch" ;
    rdfs:subClassOf piirrite:OsmEntity ;
    skos:definition "A ditch or a trench is a long and narrow man-made barrier dug in the ground to prevent access to the other side.  osmcarto-rendering = File:Barrier fence mapnik.png  osmcarto-rendering-size = 125px"@en ;
    skos:inScheme piirritev:Barrier ;
    skos:prefLabel "Ditch"@en .

piirritev:BarrierEntrance a skos:Concept ;
    piirrite:hasRelatedOsmTag piirrite:hasEntranceWidth ;
    piirrite:osmId "entrance" ;
    rdfs:subClassOf piirrite:OsmEntity ;
    skos:definition "An opening or gap in a barrier."@en ;
    skos:inScheme piirritev:Barrier ;
    skos:prefLabel "Entrance"@en .

piirritev:BarrierFence a skos:Concept ;
    piirrite:hasRelatedOsmTag piirrite:hasFenceFenceType,
        piirrite:hasFenceHeight ;
    piirrite:osmId "fence" ;
    rdfs:subClassOf piirrite:OsmEntity ;
    skos:definition "A freestanding structure designed to restrict or prevent movement across a boundary, generally distinguished from a wall by the lightness of its construction. osmcarto-rendering=File:Barrier fence mapnik.png osmcarto-rendering-size=125px"@en ;
    skos:inScheme piirritev:Barrier ;
    skos:prefLabel "Fence"@en .

piirritev:BarrierGate a skos:Concept ;
    piirrite:hasRelatedOsmTag piirrite:hasGateAccess,
        piirrite:hasGateAmenity,
        piirrite:hasGateBarrier,
        piirrite:hasGateBicycle,
        piirrite:hasGateFoot,
        piirrite:hasGateHeight,
        piirrite:hasGateLocked,
        piirrite:hasGateMaxwidth,
        piirrite:hasGateWidth ;
    piirrite:osmId "gate" ;
    rdfs:subClassOf piirrite:OsmEntity ;
    skos:definition "A section in a wall or fence which can be opened to allow access. osmcarto-rendering=File:Barrier gate.svg osmcarto-rendering-size=24px"@en ;
    skos:inScheme piirritev:Barrier ;
    skos:prefLabel "Gate"@en .

piirritev:BarrierGuardRail a skos:Concept ;
    piirrite:hasRelatedOsmTag piirrite:hasGuardRailBarrier,
        piirrite:hasGuardRailFenceType ;
    piirrite:osmId "guard_rail" ;
    rdfs:subClassOf piirrite:OsmEntity ;
    skos:definition "A rail, typically metal, designed to keep vehicles within their roadway and prevent collisions or runaways. Right side is the smooth side facing the roadway. In most editors, the side with arrows points towards the road."@en ;
    skos:inScheme piirritev:Barrier ;
    skos:prefLabel "Guard rail"@en .

piirritev:BarrierHandrail a skos:Concept ;
    piirrite:hasRelatedOsmTag piirrite:hasHandrailType ;
    piirrite:osmId "handrail" ;
    rdfs:subClassOf piirrite:OsmEntity ;
    skos:definition "A rail designed to be grasped by the hand so as to provide stability or support."@en ;
    skos:inScheme piirritev:Barrier ;
    skos:prefLabel "Handrail"@en .

piirritev:BarrierHedge a skos:Concept ;
    piirrite:hasRelatedOsmTag piirrite:hasHedgeGenus,
        piirrite:hasHedgeHeight,
        piirrite:hasHedgeLeafCycle,
        piirrite:hasHedgeLeafType,
        piirrite:hasHedgeSpecies,
        piirrite:hasHedgeTaxon,
        piirrite:hasHedgeWidth ;
    piirrite:osmId "hedge" ;
    rdfs:subClassOf piirrite:OsmEntity ;
    skos:definition "A line of closely spaced shrubs and tree species, which form a barrier or mark the boundary of an area. osmcarto-rendering=File:Barrier hedge.png osmcarto-rendering-size=125px"@en ;
    skos:inScheme piirritev:Barrier ;
    skos:prefLabel "Hedge"@en .

piirritev:BarrierHeightRestrictor a skos:Concept ;
    piirrite:hasRelatedOsmTag piirrite:hasHeightRestrictorMaxheight ;
    piirrite:osmId "height_restrictor" ;
    rdfs:subClassOf piirrite:OsmEntity ;
    skos:definition "A height restrictor which prevents access of vehicles higher than a set limit."@en ;
    skos:inScheme piirritev:Barrier ;
    skos:prefLabel "Height restrictor"@en .

piirritev:BarrierJerseyBarrier a skos:Concept ;
    piirrite:hasRelatedOsmTag piirrite:hasJerseyBarrierAccess ;
    piirrite:osmId "jersey_barrier" ;
    rdfs:subClassOf piirrite:OsmEntity ;
    skos:definition "A barrier made of heavy prefabricated blocks. osmcarto-rendering=File:Barrier fence mapnik.png osmcarto-rendering-size=125px"@en ;
    skos:inScheme piirritev:Barrier ;
    skos:prefLabel "Jersey barrier"@en .

piirritev:BarrierKerb a skos:Concept ;
    piirrite:hasRelatedOsmTag piirrite:hasKerbHeight,
        piirrite:hasKerbTactilePaving,
        piirrite:hasKerbWheelchair ;
    piirrite:osmId "kerb" ;
    rdfs:subClassOf piirrite:OsmEntity ;
    skos:definition "A stone edging to a pavement or raised path. osmcarto-rendering= osmcarto-rendering-size="@en ;
    skos:inScheme piirritev:Barrier ;
    skos:prefLabel "Kerb"@en .

piirritev:BarrierKissingGate a skos:Concept ;
    piirrite:hasRelatedOsmTag piirrite:hasKissingGateMaxwidth ;
    piirrite:osmId "kissing_gate" ;
    rdfs:subClassOf piirrite:OsmEntity ;
    skos:definition "A type of gate where you have to go into an enclosure and open a gate to get through. osmcarto-rendering = File:Kissing gate-14.svg osmcarto-rendering-size = 28px"@en ;
    skos:inScheme piirritev:Barrier ;
    skos:prefLabel "Kissing gate"@en .

piirritev:BarrierLiftGate a skos:Concept ;
    piirrite:hasRelatedOsmTag piirrite:hasLiftGateAccess,
        piirrite:hasLiftGateLocked ;
    piirrite:osmId "lift_gate" ;
    rdfs:subClassOf piirrite:OsmEntity ;
    skos:definition "A bar or pole pivoted (rotates upwards to open) in such a way as to allow the boom to block vehicular access through a controlled point. osmcarto-rendering=File:Liftgate-7.svg osmcarto-rendering-size=28px"@en ;
    skos:inScheme piirritev:Barrier ;
    skos:prefLabel "Lift gate"@en .

piirritev:BarrierLog a skos:Concept ;
    piirrite:hasRelatedOsmTag piirrite:hasLogAccess ;
    piirrite:osmId "log" ;
    rdfs:subClassOf piirrite:OsmEntity ;
    skos:definition "A log blocking access. osmcarto-rendering=File:Barrier.svg osmcarto-rendering-size=28px"@en ;
    skos:inScheme piirritev:Barrier ;
    skos:prefLabel "Log"@en .

piirritev:BarrierRetainingWall a skos:Concept ;
    piirrite:hasRelatedOsmTag piirrite:hasRetainingWallHeight,
        piirrite:hasRetainingWallMaterial ;
    piirrite:osmId "retaining_wall" ;
    rdfs:subClassOf piirrite:OsmEntity ;
    skos:definition "A linear structure that holds back soil or rock. (Lower side to right.)"@en ;
    skos:inScheme piirritev:Barrier ;
    skos:prefLabel "Retaining wall"@en .

piirritev:BarrierSlidingGate a skos:Concept ;
    piirrite:hasRelatedOsmTag piirrite:hasSlidingGateAccess,
        piirrite:hasSlidingGateBicycle,
        piirrite:hasSlidingGateFoot,
        piirrite:hasSlidingGateMaxwidth ;
    piirrite:osmId "sliding_gate" ;
    rdfs:subClassOf piirrite:OsmEntity ;
    skos:definition "A section in a wall or fence which slides or rolls to the side to allow access (note: barrier=gate is the standard tagging for such objects, this tag is used primarily by Grab employees)."@en ;
    skos:inScheme piirritev:Barrier ;
    skos:prefLabel "Sliding gate"@en .

piirritev:BarrierStile a skos:Concept ;
    piirrite:osmId "stile" ;
    rdfs:subClassOf piirrite:OsmEntity ;
    skos:definition "A structure which provides people a passage through or over a boundary via steps, ladders or narrow gaps. osmcarto-rendering=File:Barrier stile-14.svg osmcarto-rendering-size=28px"@en ;
    skos:inScheme piirritev:Barrier ;
    skos:prefLabel "Stile"@en .

piirritev:BarrierSwingGate a skos:Concept ;
    piirrite:hasRelatedOsmTag piirrite:hasSwingGateAccess,
        piirrite:hasSwingGateLocked ;
    piirrite:osmId "swing_gate" ;
    rdfs:subClassOf piirrite:OsmEntity ;
    skos:definition "A gate consisting of a bar or pole pivoted (rotates sidewards to open) in such a way as to allow the boom to block vehicular access through a controlled point. osmcarto-rendering=File:Liftgate-7.svg osmcarto-rendering-size=28px"@en ;
    skos:inScheme piirritev:Barrier ;
    skos:prefLabel "Swing gate"@en .

piirritev:BarrierTollBooth a skos:Concept ;
    piirrite:osmId "toll_booth" ;
    rdfs:subClassOf piirrite:OsmEntity ;
    skos:definition "A place where a road usage toll or fee is collected."@en ;
    skos:inScheme piirritev:Barrier ;
    skos:prefLabel "Toll booth"@en .

piirritev:BarrierTurnstile a skos:Concept ;
    piirrite:osmId "turnstile" ;
    rdfs:subClassOf piirrite:OsmEntity ;
    skos:definition "A turnstile, a passage on foot designed to allow one person at a time to pass osmcarto-rendering=File:Barrier.svg osmcarto-rendering-size=28px"@en ;
    skos:inScheme piirritev:Barrier ;
    skos:prefLabel "Turnstile"@en .

piirritev:BarrierWall a skos:Concept ;
    piirrite:hasRelatedOsmTag piirrite:hasWallHeight,
        piirrite:hasWallMaterial,
        piirrite:hasWallType,
        piirrite:hasWallWidth ;
    piirrite:osmId "wall" ;
    rdfs:subClassOf piirrite:OsmEntity ;
    skos:definition "A freestanding structure, designed to restrict or prevent movement across a boundary, typically made from solid brick, concrete or rocks, and almost always built so that it is opaque to vision. osmcarto-rendering=File:Barrier fence mapnik.png osmcarto-rendering-size=125px"@en ;
    skos:inScheme piirritev:Barrier ;
    skos:prefLabel "Wall"@en .

piirritev:BarrierWicketGate a skos:Concept ;
    piirrite:hasRelatedOsmTag piirrite:hasWicketGateAccess,
        piirrite:hasWicketGateEntrance,
        piirrite:hasWicketGateMaterial,
        piirrite:hasWicketGateOpeningHours,
        piirrite:hasWicketGateWidth ;
    piirrite:osmId "wicket_gate" ;
    rdfs:subClassOf piirrite:OsmEntity ;
    skos:definition "A pedestrian door or gate built into a wall or fence near or within a larger gate."@en ;
    skos:inScheme piirritev:Barrier ;
    skos:prefLabel "Wicket gate"@en .

piirritev:Bench a skos:ConceptScheme ;
    piirrite:osmId "bench" ;
    skos:definition "Indicates the presence of an associated bench."@en ;
    skos:prefLabel "Bench, types"@en .

piirritev:Bicycle a skos:ConceptScheme ;
    piirrite:osmId "bicycle" ;
    skos:definition "Access permission for cyclists."@en ;
    skos:prefLabel "Bicycle, types"@en .

piirritev:BicycleParkingBollard a skos:Concept ;
    piirrite:hasRelatedOsmTag piirrite:hasBollardCapacity,
        piirrite:hasBollardCovered,
        piirrite:hasBollardSupervised ;
    piirrite:osmId "bollard" ;
    rdfs:subClassOf piirrite:OsmEntity ;
    skos:definition "Bollard with a unique central pole and arms allowing to securely lock a bike."@en ;
    skos:inScheme piirritev:BicycleParking ;
    skos:prefLabel "Bollard"@en .

piirritev:BicycleParkingRack a skos:Concept ;
    piirrite:hasRelatedOsmTag piirrite:hasRackCapacity,
        piirrite:hasRackCovered,
        piirrite:hasRackSupervised ;
    piirrite:osmId "rack" ;
    rdfs:subClassOf piirrite:OsmEntity ;
    skos:definition "Coathanger or ring types of metal brackets to hang bike front wheel only."@en ;
    skos:inScheme piirritev:BicycleParking ;
    skos:prefLabel "Rack"@en .

piirritev:BicycleParkingShed a skos:Concept ;
    piirrite:osmId "shed" ;
    rdfs:subClassOf piirrite:OsmEntity ;
    skos:definition ""@en ;
    skos:inScheme piirritev:BicycleParking ;
    skos:prefLabel "Shed"@en .

piirritev:BicycleParkingStands a skos:Concept ;
    piirrite:hasRelatedOsmTag piirrite:hasStandsCapacity,
        piirrite:hasStandsCovered,
        piirrite:hasStandsSupervised ;
    piirrite:osmId "stands" ;
    rdfs:subClassOf piirrite:OsmEntity ;
    skos:definition "Metal bracket to park bicycles."@en ;
    skos:inScheme piirritev:BicycleParking ;
    skos:prefLabel "Stands"@en .

piirritev:BicycleParkingWallLoops a skos:Concept ;
    piirrite:hasRelatedOsmTag piirrite:hasWallLoopsCapacity,
        piirrite:hasWallLoopsCovered,
        piirrite:hasWallLoopsSupervised ;
    piirrite:osmId "wall_loops" ;
    rdfs:subClassOf piirrite:OsmEntity ;
    skos:definition "Metal bracket for the front wheel for parking bicycles."@en ;
    skos:inScheme piirritev:BicycleParking ;
    skos:prefLabel "Wall loops"@en .

piirritev:Bin a skos:ConceptScheme ;
    piirrite:osmId "bin" ;
    skos:definition "Indicates the presence of an associated waste basket."@en ;
    skos:prefLabel "Bin, types"@en .

piirritev:BoardTypeHistory a skos:Concept ;
    piirrite:osmId "history" ;
    rdfs:subClassOf piirrite:OsmEntity ;
    skos:definition ""@en ;
    skos:inScheme piirritev:BoardType ;
    skos:prefLabel "History"@en .

piirritev:BoardTypeNature a skos:Concept ;
    piirrite:osmId "nature" ;
    rdfs:subClassOf piirrite:OsmEntity ;
    skos:definition ""@en ;
    skos:inScheme piirritev:BoardType ;
    skos:prefLabel "Nature"@en .

piirritev:BoardTypePlants a skos:Concept ;
    piirrite:osmId "plants" ;
    rdfs:subClassOf piirrite:OsmEntity ;
    skos:definition ""@en ;
    skos:inScheme piirritev:BoardType ;
    skos:prefLabel "Plants"@en .

piirritev:BoardTypePublicTransport a skos:Concept ;
    piirrite:osmId "public_transport" ;
    rdfs:subClassOf piirrite:OsmEntity ;
    skos:definition ""@en ;
    skos:inScheme piirritev:BoardType ;
    skos:prefLabel "Public transport"@en .

piirritev:BoardTypeWelcomeSign a skos:Concept ;
    piirrite:osmId "welcome_sign" ;
    rdfs:subClassOf piirrite:OsmEntity ;
    skos:definition ""@en ;
    skos:inScheme piirritev:BoardType ;
    skos:prefLabel "Welcome sign"@en .

piirritev:BoardTypeWildlife a skos:Concept ;
    piirrite:osmId "wildlife" ;
    rdfs:subClassOf piirrite:OsmEntity ;
    skos:definition ""@en ;
    skos:inScheme piirritev:BoardType ;
    skos:prefLabel "Wildlife"@en .

piirritev:Boat a skos:ConceptScheme ;
    piirrite:osmId "boat" ;
    skos:definition "Access permission for boats"@en ;
    skos:prefLabel "Boat, types"@en .

piirritev:BollardFixed a skos:Concept ;
    piirrite:osmId "fixed" ;
    rdfs:subClassOf piirrite:OsmEntity ;
    skos:definition ""@en ;
    skos:inScheme piirritev:Bollard ;
    skos:prefLabel "Fixed"@en .

piirritev:BollardFoldable a skos:Concept ;
    piirrite:osmId "foldable" ;
    rdfs:subClassOf piirrite:OsmEntity ;
    skos:definition ""@en ;
    skos:inScheme piirritev:Bollard ;
    skos:prefLabel "Foldable"@en .

piirritev:BollardRemovable a skos:Concept ;
    piirrite:osmId "removable" ;
    rdfs:subClassOf piirrite:OsmEntity ;
    skos:definition ""@en ;
    skos:inScheme piirritev:Bollard ;
    skos:prefLabel "Removable"@en .

piirritev:BollardRising a skos:Concept ;
    piirrite:osmId "rising" ;
    rdfs:subClassOf piirrite:OsmEntity ;
    skos:definition ""@en ;
    skos:inScheme piirritev:Bollard ;
    skos:prefLabel "Rising"@en .

piirritev:BorderType a skos:ConceptScheme ;
    piirrite:osmId "border_type" ;
    skos:definition "Distinguishes a boundary by its formal designation in the real world, or distinguishes between a country's different maritime limits."@en ;
    skos:prefLabel "Border type, types"@en .

piirritev:BoundaryAdministrative a skos:Concept ;
    piirrite:hasRelatedOsmTag piirrite:hasAdministrativeAdminLevel,
        piirrite:hasAdministrativeName ;
    piirrite:osmId "administrative" ;
    rdfs:subClassOf piirrite:OsmEntity ;
    skos:definition "An administrative boundary recognised by governments for administrative purposes."@en ;
    skos:inScheme piirritev:Boundary ;
    skos:prefLabel "Administrative"@en .

piirritev:BoundaryCensus a skos:Concept ;
    piirrite:hasRelatedOsmTag piirrite:hasCensusName ;
    piirrite:osmId "census" ;
    rdfs:subClassOf piirrite:OsmEntity ;
    skos:definition "A census-designated boundary delineating a statistical area, not necessarily observable on the ground."@en ;
    skos:inScheme piirritev:Boundary ;
    skos:prefLabel "Census"@en .

piirritev:BoundaryForestCompartment a skos:Concept ;
    piirrite:hasRelatedOsmTag piirrite:hasForestCompartmentRef ;
    piirrite:osmId "forest_compartment" ;
    rdfs:subClassOf piirrite:OsmEntity ;
    skos:definition "A marked subdivision of delimited forest, which is used for planning, management & navigation."@en ;
    skos:inScheme piirritev:Boundary ;
    skos:prefLabel "Forest compartment"@en .

piirritev:BoundaryHealth a skos:Concept ;
    piirrite:osmId "health" ;
    rdfs:subClassOf piirrite:OsmEntity ;
    skos:definition ""@en ;
    skos:inScheme piirritev:Boundary ;
    skos:prefLabel "Health"@en .

piirritev:BoundaryHistoric a skos:Concept ;
    piirrite:hasRelatedOsmTag piirrite:hasHistoricAdminLevel,
        piirrite:hasHistoricEndDate,
        piirrite:hasHistoricName,
        piirrite:hasHistoricStartDate ;
    piirrite:osmId "historic" ;
    rdfs:subClassOf piirrite:OsmEntity ;
    skos:definition "A historic administrative boundary (use judiciously)."@en ;
    skos:inScheme piirritev:Boundary ;
    skos:prefLabel "Historic"@en .

piirritev:BoundaryLocalAuthority a skos:Concept ;
    piirrite:osmId "local_authority" ;
    rdfs:subClassOf piirrite:OsmEntity ;
    skos:definition "Describes the territory of a local authority."@en ;
    skos:inScheme piirritev:Boundary ;
    skos:prefLabel "Local authority"@en .

piirritev:BoundaryMarker a skos:Concept ;
    piirrite:hasRelatedOsmTag piirrite:hasMarkerFormat,
        piirrite:hasMarkerInscription,
        piirrite:hasMarkerMaterial,
        piirrite:hasMarkerName,
        piirrite:hasMarkerRef ;
    piirrite:osmId "marker" ;
    rdfs:subClassOf piirrite:OsmEntity ;
    skos:definition "A physical marker that identifies a boundary"@en ;
    skos:inScheme piirritev:Boundary ;
    skos:prefLabel "Marker"@en .

piirritev:BoundaryPlace a skos:Concept ;
    piirrite:hasRelatedOsmTag piirrite:hasPlaceType ;
    piirrite:osmId "place" ;
    rdfs:subClassOf piirrite:OsmEntity ;
    skos:definition "The boundaries of a key:place, when these boundaries can be defined but these are not administrative boundaries."@en ;
    skos:inScheme piirritev:Boundary ;
    skos:prefLabel "Place"@en .

piirritev:BoundaryPolitical a skos:Concept ;
    piirrite:hasRelatedOsmTag piirrite:hasPoliticalPoliticalDivision ;
    piirrite:osmId "political" ;
    rdfs:subClassOf piirrite:OsmEntity ;
    skos:definition "Political boundary, such as an electoral ward or parliamentary constituency."@en ;
    skos:inScheme piirritev:Boundary ;
    skos:prefLabel "Political"@en .

piirritev:BoundaryPostalCode a skos:Concept ;
    piirrite:hasRelatedOsmTag piirrite:hasPostalCodeType ;
    piirrite:osmId "postal_code" ;
    rdfs:subClassOf piirrite:OsmEntity ;
    skos:definition "A postal code boundary"@en ;
    skos:inScheme piirritev:Boundary ;
    skos:prefLabel "Postal code"@en .

piirritev:BoundaryProtectedArea a skos:Concept ;
    piirrite:hasRelatedOsmTag piirrite:hasProtectedAreaName,
        piirrite:hasProtectedAreaOfficialName,
        piirrite:hasProtectedAreaType ;
    piirrite:osmId "protected_area" ;
    rdfs:subClassOf piirrite:OsmEntity ;
    skos:definition "Used to mark boundaries of protected areas including national parks, wilderness, marine protection areas, heritage sites and other, similar areas."@en ;
    skos:inScheme piirritev:Boundary ;
    skos:prefLabel "Protected area"@en .

piirritev:BoundaryReligiousAdministration a skos:Concept ;
    piirrite:hasRelatedOsmTag piirrite:hasReligiousAdministrationAdminLevel,
        piirrite:hasReligiousAdministrationName,
        piirrite:hasReligiousAdministrationReligion ;
    piirrite:osmId "religious_administration" ;
    rdfs:subClassOf piirrite:OsmEntity ;
    skos:definition "Administrative boundaries of institutionalised religions."@en ;
    skos:inScheme piirritev:Boundary ;
    skos:prefLabel "Religious administration"@en .

piirritev:Branch a skos:ConceptScheme ;
    piirrite:osmId "branch" ;
    skos:definition "Identifies which branch of a brand or chain this object represents, or controversially the name of a branch railway."@en ;
    skos:prefLabel "Branch, types"@en .

piirritev:Brand a skos:ConceptScheme ;
    piirrite:osmId "brand" ;
    skos:definition "The identity of a specific product, service, or business. Often trademarks"@en ;
    skos:prefLabel "Brand, types"@en .

piirritev:BridgeAqueduct a skos:Concept ;
    piirrite:osmId "aqueduct" ;
    rdfs:subClassOf piirrite:OsmEntity ;
    skos:definition "A bridge which conveys an artificial waterway over a road, valley or waterway."@en ;
    skos:inScheme piirritev:Bridge ;
    skos:prefLabel "Aqueduct"@en .

piirritev:BridgeBoardwalk a skos:Concept ;
    piirrite:hasRelatedOsmTag piirrite:hasBoardwalkHighway ;
    piirrite:osmId "boardwalk" ;
    rdfs:subClassOf piirrite:OsmEntity ;
    skos:definition "Plank walkway"@en ;
    skos:inScheme piirritev:Bridge ;
    skos:prefLabel "Boardwalk"@en .

piirritev:BridgeViaduct a skos:Concept ;
    piirrite:hasRelatedOsmTag piirrite:hasViaductHighway,
        piirrite:hasViaductLength,
        piirrite:hasViaductName,
        piirrite:hasViaductRailway,
        piirrite:hasViaductRuins,
        piirrite:hasViaductStartDate,
        piirrite:hasViaductWikipedia ;
    piirrite:osmId "viaduct" ;
    rdfs:subClassOf piirrite:OsmEntity ;
    skos:definition "A long rail, road, or other bridge made up of many short spans."@en ;
    skos:inScheme piirritev:Bridge ;
    skos:prefLabel "Viaduct"@en .

piirritev:BuildingAgricultural a skos:Concept ;
    piirrite:hasRelatedOsmTag piirrite:hasAgriculturalLanduse ;
    piirrite:osmId "agricultural" ;
    rdfs:subClassOf piirrite:OsmEntity ;
    skos:definition "A building built for agricultural purposes"@en ;
    skos:inScheme piirritev:Building ;
    skos:prefLabel "Agricultural"@en .

piirritev:BuildingAllotmentHouse a skos:Concept ;
    piirrite:osmId "allotment_house" ;
    rdfs:subClassOf piirrite:OsmEntity ;
    skos:definition "A small outbuilding for short visits in a allotment garden."@en ;
    skos:inScheme piirritev:Building ;
    skos:prefLabel "Allotment house"@en .

piirritev:BuildingApartments a skos:Concept ;
    piirrite:osmId "apartments" ;
    rdfs:subClassOf piirrite:OsmEntity ;
    skos:definition "A building arranged into individual dwellings, often on separate floors. May also have retail outlets on the ground floor."@en ;
    skos:inScheme piirritev:Building ;
    skos:prefLabel "Apartments"@en .

piirritev:BuildingBarn a skos:Concept ;
    piirrite:hasRelatedOsmTag piirrite:hasBarnLanduse ;
    piirrite:osmId "barn" ;
    rdfs:subClassOf piirrite:OsmEntity ;
    skos:definition "An agricultural building that can be used for storage and as a covered workplace."@en ;
    skos:inScheme piirritev:Building ;
    skos:prefLabel "Barn"@en .

piirritev:BuildingBoathouse a skos:Concept ;
    piirrite:osmId "boathouse" ;
    rdfs:subClassOf piirrite:OsmEntity ;
    skos:definition "A building for storing boats"@en ;
    skos:inScheme piirritev:Building ;
    skos:prefLabel "Boathouse"@en .

piirritev:BuildingBungalow a skos:Concept ;
    piirrite:osmId "bungalow" ;
    rdfs:subClassOf piirrite:OsmEntity ;
    skos:definition "Simple single-storey flat house."@en ;
    skos:inScheme piirritev:Building ;
    skos:prefLabel "Bungalow"@en .

piirritev:BuildingBunker a skos:Concept ;
    piirrite:hasRelatedOsmTag piirrite:hasBunkerMilitary ;
    piirrite:osmId "bunker" ;
    rdfs:subClassOf piirrite:OsmEntity ;
    skos:definition "A hardened military building."@en ;
    skos:inScheme piirritev:Building ;
    skos:prefLabel "Bunker"@en .

piirritev:BuildingCabin a skos:Concept ;
    piirrite:osmId "cabin" ;
    rdfs:subClassOf piirrite:OsmEntity ;
    skos:definition "A small, roughly built house typically found in rural areas."@en ;
    skos:inScheme piirritev:Building ;
    skos:prefLabel "Cabin"@en .

piirritev:BuildingCarport a skos:Concept ;
    piirrite:hasRelatedOsmTag piirrite:hasCarportCapacity,
        piirrite:hasCarportHeight ;
    piirrite:osmId "carport" ;
    rdfs:subClassOf piirrite:OsmEntity ;
    skos:definition "A carport is a covered structure used to offer limited protection to vehicles, primarily cars, from the elements."@en ;
    skos:inScheme piirritev:Building ;
    skos:prefLabel "Carport"@en .

piirritev:BuildingChapel a skos:Concept ;
    piirrite:hasRelatedOsmTag piirrite:hasChapelAmenity,
        piirrite:hasChapelReligion ;
    piirrite:osmId "chapel" ;
    rdfs:subClassOf piirrite:OsmEntity ;
    skos:definition "Building built as chapel."@en ;
    skos:inScheme piirritev:Building ;
    skos:prefLabel "Chapel"@en .

piirritev:BuildingChurch a skos:Concept ;
    piirrite:hasRelatedOsmTag piirrite:hasChurchAmenity,
        piirrite:hasChurchName,
        piirrite:hasChurchReligion ;
    piirrite:osmId "church" ;
    rdfs:subClassOf piirrite:OsmEntity ;
    skos:definition "A building that was built as a church.  osmcarto-rendering = File:Area building=yes.png  osmcarto-rendering-size = 100px"@en ;
    skos:inScheme piirritev:Building ;
    skos:prefLabel "Church"@en .

piirritev:BuildingCivic a skos:Concept ;
    piirrite:hasRelatedOsmTag piirrite:hasCivicAmenity,
        piirrite:hasCivicLeisure ;
    piirrite:osmId "civic" ;
    rdfs:subClassOf piirrite:OsmEntity ;
    skos:definition "A building originally built as civic building to hosting any civic amenity (town hall, library, swimming pool etc.)."@en ;
    skos:inScheme piirritev:Building ;
    skos:prefLabel "Civic"@en .

piirritev:BuildingCollapsed a skos:Concept ;
    piirrite:osmId "collapsed" ;
    rdfs:subClassOf piirrite:OsmEntity ;
    skos:definition "Using this tag is discouraged, use key:demolished:building or tag:building=ruins or delete object instead."@en ;
    skos:inScheme piirritev:Building ;
    skos:prefLabel "Collapsed"@en .

piirritev:BuildingCollege a skos:Concept ;
    piirrite:hasRelatedOsmTag piirrite:hasCollegeAddr,
        piirrite:hasCollegeName ;
    piirrite:osmId "college" ;
    rdfs:subClassOf piirrite:OsmEntity ;
    skos:definition "A building constructed to house a college."@en ;
    skos:inScheme piirritev:Building ;
    skos:prefLabel "College"@en .

piirritev:BuildingCommercial a skos:Concept ;
    piirrite:hasRelatedOsmTag piirrite:hasCommercialOffice ;
    piirrite:osmId "commercial" ;
    rdfs:subClassOf piirrite:OsmEntity ;
    skos:definition "A building constructed for non-specific commercial activities to take place there."@en ;
    skos:inScheme piirritev:Building ;
    skos:prefLabel "Commercial"@en .

piirritev:BuildingConservatory a skos:Concept ;
    piirrite:hasRelatedOsmTag piirrite:hasConservatoryAccess,
        piirrite:hasConservatoryHeight,
        piirrite:hasConservatoryOperator ;
    piirrite:osmId "conservatory" ;
    rdfs:subClassOf piirrite:OsmEntity ;
    skos:definition "Conservatory - a building or room having glass or tarpaulin roofing and walls used as an indoor garden or a sunroom (winter garden)."@en ;
    skos:inScheme piirritev:Building ;
    skos:prefLabel "Conservatory"@en .

piirritev:BuildingConstruction a skos:Concept ;
    piirrite:hasRelatedOsmTag piirrite:hasConstructionType ;
    piirrite:osmId "construction" ;
    rdfs:subClassOf piirrite:OsmEntity ;
    skos:definition "A building under construction"@en ;
    skos:inScheme piirritev:Building ;
    skos:prefLabel "Construction"@en .

piirritev:BuildingContainer a skos:Concept ;
    piirrite:osmId "container" ;
    rdfs:subClassOf piirrite:OsmEntity ;
    skos:definition "A container used as a permanent building."@en ;
    skos:inScheme piirritev:Building ;
    skos:prefLabel "Container"@en .

piirritev:BuildingCowshed a skos:Concept ;
    piirrite:hasRelatedOsmTag piirrite:hasCowshedLanduse ;
    piirrite:osmId "cowshed" ;
    rdfs:subClassOf piirrite:OsmEntity ;
    skos:definition "A building for housing cows."@en ;
    skos:inScheme piirritev:Building ;
    skos:prefLabel "Cowshed"@en .

piirritev:BuildingDetached a skos:Concept ;
    piirrite:osmId "detached" ;
    rdfs:subClassOf piirrite:OsmEntity ;
    skos:definition "A detached house: a free-standing residential building usually housing a single family."@en ;
    skos:inScheme piirritev:Building ;
    skos:prefLabel "Detached"@en .

piirritev:BuildingDigester a skos:Concept ;
    piirrite:hasRelatedOsmTag piirrite:hasDigesterOperator,
        piirrite:hasDigesterPower,
        piirrite:hasDigesterRef ;
    piirrite:osmId "digester" ;
    rdfs:subClassOf piirrite:OsmEntity ;
    skos:definition "A building constructed as a digester, a bioreactor for the production of biogas from biomass."@en ;
    skos:inScheme piirritev:Building ;
    skos:prefLabel "Digester"@en .

piirritev:BuildingDormitory a skos:Concept ;
    piirrite:hasRelatedOsmTag piirrite:hasDormitoryName,
        piirrite:hasDormitoryOperator ;
    piirrite:osmId "dormitory" ;
    rdfs:subClassOf piirrite:OsmEntity ;
    skos:definition "Sleeping and living quarters provided by an institution."@en ;
    skos:inScheme piirritev:Building ;
    skos:prefLabel "Dormitory"@en .

piirritev:BuildingFarm a skos:Concept ;
    piirrite:hasRelatedOsmTag piirrite:hasFarmName ;
    piirrite:osmId "farm" ;
    rdfs:subClassOf piirrite:OsmEntity ;
    skos:definition "A farmhouse is the main building of a farm"@en ;
    skos:inScheme piirritev:Building ;
    skos:prefLabel "Farm"@en .

piirritev:BuildingFarmAuxiliary a skos:Concept ;
    piirrite:hasRelatedOsmTag piirrite:hasFarmAuxiliaryLanduse ;
    piirrite:osmId "farm_auxiliary" ;
    rdfs:subClassOf piirrite:OsmEntity ;
    skos:definition "A building on a farm that is not a dwelling."@en ;
    skos:inScheme piirritev:Building ;
    skos:prefLabel "Farm auxiliary"@en .

piirritev:BuildingFireStation a skos:Concept ;
    piirrite:hasRelatedOsmTag piirrite:hasFireStationAmenity ;
    piirrite:osmId "fire_station" ;
    rdfs:subClassOf piirrite:OsmEntity ;
    skos:definition "A building constructed to house fire fighting equipment."@en ;
    skos:inScheme piirritev:Building ;
    skos:prefLabel "Fire station"@en .

piirritev:BuildingGarage a skos:Concept ;
    piirrite:hasRelatedOsmTag piirrite:hasGarageLanduse ;
    piirrite:osmId "garage" ;
    rdfs:subClassOf piirrite:OsmEntity ;
    skos:definition "Denotes a single-owner private garage"@en ;
    skos:inScheme piirritev:Building ;
    skos:prefLabel "Garage"@en .

piirritev:BuildingGarages a skos:Concept ;
    piirrite:hasRelatedOsmTag piirrite:hasGaragesAmenity,
        piirrite:hasGaragesBuilding ;
    piirrite:osmId "garages" ;
    rdfs:subClassOf piirrite:OsmEntity ;
    skos:definition "A block of private garages each with a separate owner."@en ;
    skos:inScheme piirritev:Building ;
    skos:prefLabel "Garages"@en .

piirritev:BuildingGer a skos:Concept ;
    piirrite:osmId "ger" ;
    rdfs:subClassOf piirrite:OsmEntity ;
    skos:definition "A portable, round tent (yurt or ger)"@en ;
    skos:inScheme piirritev:Building ;
    skos:prefLabel "Ger"@en .

piirritev:BuildingGovernment a skos:Concept ;
    piirrite:osmId "government" ;
    rdfs:subClassOf piirrite:OsmEntity ;
    skos:definition "A building built to house government offices."@en ;
    skos:inScheme piirritev:Building ;
    skos:prefLabel "Government"@en .

piirritev:BuildingGrandstand a skos:Concept ;
    piirrite:osmId "grandstand" ;
    rdfs:subClassOf piirrite:OsmEntity ;
    skos:definition "A grandstand at racecourse or sports ground."@en ;
    skos:inScheme piirritev:Building ;
    skos:prefLabel "Grandstand"@en .

piirritev:BuildingGreenhouse a skos:Concept ;
    piirrite:osmId "greenhouse" ;
    rdfs:subClassOf piirrite:OsmEntity ;
    skos:definition "A building in which plants are grown"@en ;
    skos:inScheme piirritev:Building ;
    skos:prefLabel "Greenhouse"@en .

piirritev:BuildingHangar a skos:Concept ;
    piirrite:hasRelatedOsmTag piirrite:hasHangarAeroway ;
    piirrite:osmId "hangar" ;
    rdfs:subClassOf piirrite:OsmEntity ;
    skos:definition "A building that was built as a hangar for the storage of aeroplanes, helicopters or space-craft."@en ;
    skos:inScheme piirritev:Building ;
    skos:prefLabel "Hangar"@en .

piirritev:BuildingHospital a skos:Concept ;
    piirrite:hasRelatedOsmTag piirrite:hasHospitalAmenity ;
    piirrite:osmId "hospital" ;
    rdfs:subClassOf piirrite:OsmEntity ;
    skos:definition "A building which forms part of a hospital."@en ;
    skos:inScheme piirritev:Building ;
    skos:prefLabel "Hospital"@en .

piirritev:BuildingHotel a skos:Concept ;
    piirrite:osmId "hotel" ;
    rdfs:subClassOf piirrite:OsmEntity ;
    skos:definition "A building designed with separate rooms available for overnight accommodation."@en ;
    skos:inScheme piirritev:Building ;
    skos:prefLabel "Hotel"@en .

piirritev:BuildingHouse a skos:Concept ;
    piirrite:hasRelatedOsmTag piirrite:hasHouseAddr ;
    piirrite:osmId "house" ;
    rdfs:subClassOf piirrite:OsmEntity ;
    skos:definition "A single dwelling unit usually inhabited by one family.  osmcarto-rendering = File:Area building=yes.png  osmcarto-rendering-size = 28px"@en ;
    skos:inScheme piirritev:Building ;
    skos:prefLabel "House"@en .

piirritev:BuildingHouseboat a skos:Concept ;
    piirrite:osmId "houseboat" ;
    rdfs:subClassOf piirrite:OsmEntity ;
    skos:definition "A boat (re)constructed as a floating home, staying at a single permanent location."@en ;
    skos:inScheme piirritev:Building ;
    skos:prefLabel "Houseboat"@en .

piirritev:BuildingHut a skos:Concept ;
    piirrite:osmId "hut" ;
    rdfs:subClassOf piirrite:OsmEntity ;
    skos:definition "A small and crude shelter."@en ;
    skos:inScheme piirritev:Building ;
    skos:prefLabel "Hut"@en .

piirritev:BuildingIndustrial a skos:Concept ;
    piirrite:hasRelatedOsmTag piirrite:hasIndustrialType ;
    piirrite:osmId "industrial" ;
    rdfs:subClassOf piirrite:OsmEntity ;
    skos:definition "A building constructed to house some manufacturing process"@en ;
    skos:inScheme piirritev:Building ;
    skos:prefLabel "Industrial"@en .

piirritev:BuildingKindergarten a skos:Concept ;
    piirrite:hasRelatedOsmTag piirrite:hasKindergartenAmenity,
        piirrite:hasKindergartenName ;
    piirrite:osmId "kindergarten" ;
    rdfs:subClassOf piirrite:OsmEntity ;
    skos:definition "A generic kindergarten building."@en ;
    skos:inScheme piirritev:Building ;
    skos:prefLabel "Kindergarten"@en .

piirritev:BuildingKiosk a skos:Concept ;
    piirrite:hasRelatedOsmTag piirrite:hasKioskShop ;
    piirrite:osmId "kiosk" ;
    rdfs:subClassOf piirrite:OsmEntity ;
    skos:definition "A building that was originally built as kiosk - a small one room retail building, with clients not entering the building."@en ;
    skos:inScheme piirritev:Building ;
    skos:prefLabel "Kiosk"@en .

piirritev:BuildingManufacture a skos:Concept ;
    piirrite:osmId "manufacture" ;
    rdfs:subClassOf piirrite:OsmEntity ;
    skos:definition ""@en ;
    skos:inScheme piirritev:Building ;
    skos:prefLabel "Manufacture"@en .

piirritev:BuildingMosque a skos:Concept ;
    piirrite:hasRelatedOsmTag piirrite:hasMosqueAmenity,
        piirrite:hasMosqueName,
        piirrite:hasMosqueOpeningHours,
        piirrite:hasMosqueReligion,
        piirrite:hasMosqueWebsite,
        piirrite:hasMosqueWheelchair ;
    piirrite:osmId "mosque" ;
    rdfs:subClassOf piirrite:OsmEntity ;
    skos:definition "A building that was built as a mosque."@en ;
    skos:inScheme piirritev:Building ;
    skos:prefLabel "Mosque"@en .

piirritev:BuildingOffice a skos:Concept ;
    piirrite:osmId "office" ;
    rdfs:subClassOf piirrite:OsmEntity ;
    skos:definition "A building that was originally built as an office building which contains spaces mainly designed to be used for offices."@en ;
    skos:inScheme piirritev:Building ;
    skos:prefLabel "Office"@en .

piirritev:BuildingOutbuilding a skos:Concept ;
    piirrite:osmId "outbuilding" ;
    rdfs:subClassOf piirrite:OsmEntity ;
    skos:definition "A less important building near to and on the same piece of land as a larger building."@en ;
    skos:inScheme piirritev:Building ;
    skos:prefLabel "Outbuilding"@en .

piirritev:BuildingParking a skos:Concept ;
    piirrite:hasRelatedOsmTag piirrite:hasParkingAmenity,
        piirrite:hasParkingType ;
    piirrite:osmId "parking" ;
    rdfs:subClassOf piirrite:OsmEntity ;
    skos:definition "Structure purpose-built for parking cars."@en ;
    skos:inScheme piirritev:Building ;
    skos:prefLabel "Parking"@en .

piirritev:BuildingPavilion a skos:Concept ;
    piirrite:osmId "pavilion" ;
    rdfs:subClassOf piirrite:OsmEntity ;
    skos:definition "A building providing facilities for users of sports grounds"@en ;
    skos:inScheme piirritev:Building ;
    skos:prefLabel "Pavilion"@en .

piirritev:BuildingPublic a skos:Concept ;
    piirrite:hasRelatedOsmTag piirrite:hasPublicAmenity,
        piirrite:hasPublicLeisure ;
    piirrite:osmId "public" ;
    rdfs:subClassOf piirrite:OsmEntity ;
    skos:definition "A building constructed as accessible to the public (town hall, police station, court house)."@en ;
    skos:inScheme piirritev:Building ;
    skos:prefLabel "Public"@en .

piirritev:BuildingResidential a skos:Concept ;
    piirrite:osmId "residential" ;
    rdfs:subClassOf piirrite:OsmEntity ;
    skos:definition "A general tag for a building constructed primarily for residential purposes."@en ;
    skos:inScheme piirritev:Building ;
    skos:prefLabel "Residential"@en .

piirritev:BuildingRetail a skos:Concept ;
    piirrite:hasRelatedOsmTag piirrite:hasRetailLanduse,
        piirrite:hasRetailShop ;
    piirrite:osmId "retail" ;
    rdfs:subClassOf piirrite:OsmEntity ;
    skos:definition "A building that was originally built as a retail building for selling goods to the public."@en ;
    skos:inScheme piirritev:Building ;
    skos:prefLabel "Retail"@en .

piirritev:BuildingRoof a skos:Concept ;
    piirrite:hasRelatedOsmTag piirrite:hasRoofLayer ;
    piirrite:osmId "roof" ;
    rdfs:subClassOf piirrite:OsmEntity ;
    skos:definition "A building open on at least two sides."@en ;
    skos:inScheme piirritev:Building ;
    skos:prefLabel "Roof"@en .

piirritev:BuildingRuins a skos:Concept ;
    piirrite:osmId "ruins" ;
    rdfs:subClassOf piirrite:OsmEntity ;
    skos:definition "Frequently used to mark ruined buildings. However, this usage conflicts with general use of building tag. In theory it should only be used for buildings constructed to look like ruins."@en ;
    skos:inScheme piirritev:Building ;
    skos:prefLabel "Ruins"@en .

piirritev:BuildingSchool a skos:Concept ;
    piirrite:osmId "school" ;
    rdfs:subClassOf piirrite:OsmEntity ;
    skos:definition "A building originally built as a school building."@en ;
    skos:inScheme piirritev:Building ;
    skos:prefLabel "School"@en .

piirritev:BuildingSemidetachedHouse a skos:Concept ;
    piirrite:osmId "semidetached_house" ;
    rdfs:subClassOf piirrite:OsmEntity ;
    skos:definition "A house that shares a common wall with another on one side."@en ;
    skos:inScheme piirritev:Building ;
    skos:prefLabel "Semidetached house"@en .

piirritev:BuildingService a skos:Concept ;
    piirrite:hasRelatedOsmTag piirrite:hasServicePower,
        piirrite:hasServiceSubstation,
        piirrite:hasServiceTelecom,
        piirrite:hasServiceUtility ;
    piirrite:osmId "service" ;
    rdfs:subClassOf piirrite:OsmEntity ;
    skos:definition "Service building usually is a small unmanned building with certain machinery (like pumps or transformers)."@en ;
    skos:inScheme piirritev:Building ;
    skos:prefLabel "Service"@en .

piirritev:BuildingShed a skos:Concept ;
    piirrite:osmId "shed" ;
    rdfs:subClassOf piirrite:OsmEntity ;
    skos:definition "A small, simple structure used as storage or workshop"@en ;
    skos:inScheme piirritev:Building ;
    skos:prefLabel "Shed"@en .

piirritev:BuildingSilo a skos:Concept ;
    piirrite:hasRelatedOsmTag piirrite:hasSiloContent,
        piirrite:hasSiloCrop,
        piirrite:hasSiloHeight,
        piirrite:hasSiloManMade,
        piirrite:hasSiloOperator ;
    piirrite:osmId "silo" ;
    rdfs:subClassOf piirrite:OsmEntity ;
    skos:definition "A silo is a building for storing bulk materials."@en ;
    skos:inScheme piirritev:Building ;
    skos:prefLabel "Silo"@en .

piirritev:BuildingSlurryTank a skos:Concept ;
    piirrite:osmId "slurry_tank" ;
    rdfs:subClassOf piirrite:OsmEntity ;
    skos:definition "A cylindrical concrete structure holding liquid manure."@en ;
    skos:inScheme piirritev:Building ;
    skos:prefLabel "Slurry tank"@en .

piirritev:BuildingSportsCentre a skos:Concept ;
    piirrite:hasRelatedOsmTag piirrite:hasSportsCentreSport ;
    piirrite:osmId "sports_centre" ;
    rdfs:subClassOf piirrite:OsmEntity ;
    skos:definition "A building that was built as a sports centre"@en ;
    skos:inScheme piirritev:Building ;
    skos:prefLabel "Sports centre"@en .

piirritev:BuildingSportsHall a skos:Concept ;
    piirrite:hasRelatedOsmTag piirrite:hasSportsHallLeisure,
        piirrite:hasSportsHallSport ;
    piirrite:osmId "sports_hall" ;
    rdfs:subClassOf piirrite:OsmEntity ;
    skos:definition "A building that was built as a sports hall"@en ;
    skos:inScheme piirritev:Building ;
    skos:prefLabel "Sports hall"@en .

piirritev:BuildingStable a skos:Concept ;
    piirrite:osmId "stable" ;
    rdfs:subClassOf piirrite:OsmEntity ;
    skos:definition "A building constructed as a stable for horses"@en ;
    skos:inScheme piirritev:Building ;
    skos:prefLabel "Stable"@en .

piirritev:BuildingStadium a skos:Concept ;
    piirrite:hasRelatedOsmTag piirrite:hasStadiumLeisure,
        piirrite:hasStadiumSport ;
    piirrite:osmId "stadium" ;
    rdfs:subClassOf piirrite:OsmEntity ;
    skos:definition "A building which was built as stadium."@en ;
    skos:inScheme piirritev:Building ;
    skos:prefLabel "Stadium"@en .

piirritev:BuildingStaticCaravan a skos:Concept ;
    piirrite:osmId "static_caravan" ;
    rdfs:subClassOf piirrite:OsmEntity ;
    skos:definition "A mobile home (caravan) (semi)permanently left on a single site."@en ;
    skos:inScheme piirritev:Building ;
    skos:prefLabel "Static caravan"@en .

piirritev:BuildingStiltHouse a skos:Concept ;
    piirrite:osmId "stilt_house" ;
    rdfs:subClassOf piirrite:OsmEntity ;
    skos:definition "A house raised on piles over the surface of the soil or a body of water."@en ;
    skos:inScheme piirritev:Building ;
    skos:prefLabel "Stilt house"@en .

piirritev:BuildingStorageTank a skos:Concept ;
    piirrite:hasRelatedOsmTag piirrite:hasStorageTankCapacity,
        piirrite:hasStorageTankContent,
        piirrite:hasStorageTankHeight,
        piirrite:hasStorageTankLocation,
        piirrite:hasStorageTankManMade,
        piirrite:hasStorageTankMaterial,
        piirrite:hasStorageTankOperator ;
    piirrite:osmId "storage_tank" ;
    rdfs:subClassOf piirrite:OsmEntity ;
    skos:definition "A storage tank"@en ;
    skos:inScheme piirritev:Building ;
    skos:prefLabel "Storage tank"@en .

piirritev:BuildingSty a skos:Concept ;
    piirrite:hasRelatedOsmTag piirrite:hasStyLanduse ;
    piirrite:osmId "sty" ;
    rdfs:subClassOf piirrite:OsmEntity ;
    skos:definition "A building for raising domestic pigs."@en ;
    skos:inScheme piirritev:Building ;
    skos:prefLabel "Sty"@en .

piirritev:BuildingSupermarket a skos:Concept ;
    piirrite:osmId "supermarket" ;
    rdfs:subClassOf piirrite:OsmEntity ;
    skos:definition "A building built as a supermarket"@en ;
    skos:inScheme piirritev:Building ;
    skos:prefLabel "Supermarket"@en .

piirritev:BuildingTemple a skos:Concept ;
    piirrite:hasRelatedOsmTag piirrite:hasTempleAmenity,
        piirrite:hasTempleReligion ;
    piirrite:osmId "temple" ;
    rdfs:subClassOf piirrite:OsmEntity ;
    skos:definition "A building that was built as a temple"@en ;
    skos:inScheme piirritev:Building ;
    skos:prefLabel "Temple"@en .

piirritev:BuildingTent a skos:Concept ;
    piirrite:hasRelatedOsmTag piirrite:hasTentName,
        piirrite:hasTentSeasonal ;
    piirrite:osmId "tent" ;
    rdfs:subClassOf piirrite:OsmEntity ;
    skos:definition "A building mainly consisting of sheets of fabric or similar"@en ;
    skos:inScheme piirritev:Building ;
    skos:prefLabel "Tent"@en .

piirritev:BuildingTerrace a skos:Concept ;
    piirrite:hasRelatedOsmTag piirrite:hasTerraceBuilding,
        piirrite:hasTerraceHouse ;
    piirrite:osmId "terrace" ;
    rdfs:subClassOf piirrite:OsmEntity ;
    skos:definition "The outline of a linear row of residential dwellings, each of which normally has its own entrance, which form a terrace (\"row-house\" or \"townhouse\" in North American English)."@en ;
    skos:inScheme piirritev:Building ;
    skos:prefLabel "Terrace"@en .

piirritev:BuildingToilets a skos:Concept ;
    piirrite:hasRelatedOsmTag piirrite:hasToiletsAmenity,
        piirrite:hasToiletsWheelchair ;
    piirrite:osmId "toilets" ;
    rdfs:subClassOf piirrite:OsmEntity ;
    skos:definition "A building designed for toilets."@en ;
    skos:inScheme piirritev:Building ;
    skos:prefLabel "Toilets"@en .

piirritev:BuildingTomb a skos:Concept ;
    piirrite:osmId "tomb" ;
    rdfs:subClassOf piirrite:OsmEntity ;
    skos:definition ""@en ;
    skos:inScheme piirritev:Building ;
    skos:prefLabel "Tomb"@en .

piirritev:BuildingTrainStation a skos:Concept ;
    piirrite:hasRelatedOsmTag piirrite:hasTrainStationInternetAccess,
        piirrite:hasTrainStationRailway ;
    piirrite:osmId "train_station" ;
    rdfs:subClassOf piirrite:OsmEntity ;
    skos:definition "A train station building osmcarto-rendering=File:Area amenity=place of worship.png osmcarto-rendering-size=28px"@en ;
    skos:inScheme piirritev:Building ;
    skos:prefLabel "Train station"@en .

piirritev:BuildingTransformerTower a skos:Concept ;
    piirrite:hasRelatedOsmTag piirrite:hasTransformerTowerPower,
        piirrite:hasTransformerTowerSubstation ;
    piirrite:osmId "transformer_tower" ;
    rdfs:subClassOf piirrite:OsmEntity ;
    skos:definition "A small but tall building constructed to comprise a transformer and connect to an overhead power line."@en ;
    skos:inScheme piirritev:Building ;
    skos:prefLabel "Transformer tower"@en .

piirritev:BuildingTransportation a skos:Concept ;
    piirrite:hasRelatedOsmTag piirrite:hasTransportationPublicTransport ;
    piirrite:osmId "transportation" ;
    rdfs:subClassOf piirrite:OsmEntity ;
    skos:definition "A building related to the public transportation."@en ;
    skos:inScheme piirritev:Building ;
    skos:prefLabel "Transportation"@en .

piirritev:BuildingTrullo a skos:Concept ;
    piirrite:osmId "trullo" ;
    rdfs:subClassOf piirrite:OsmEntity ;
    skos:definition "A stone hut with a conical roof, built without mortar"@en ;
    skos:inScheme piirritev:Building ;
    skos:prefLabel "Trullo"@en .

piirritev:BuildingUniversity a skos:Concept ;
    piirrite:hasRelatedOsmTag piirrite:hasUniversityName ;
    piirrite:osmId "university" ;
    rdfs:subClassOf piirrite:OsmEntity ;
    skos:definition "A university building."@en ;
    skos:inScheme piirritev:Building ;
    skos:prefLabel "University"@en .

piirritev:BuildingWarehouse a skos:Concept ;
    piirrite:osmId "warehouse" ;
    rdfs:subClassOf piirrite:OsmEntity ;
    skos:definition "A building that was originally built as a commercial building for storage of goods."@en ;
    skos:inScheme piirritev:Building ;
    skos:prefLabel "Warehouse"@en .

piirritev:BusDesignated a skos:Concept ;
    piirrite:hasRelatedOsmTag piirrite:hasDesignatedHighway ;
    piirrite:osmId "designated" ;
    rdfs:subClassOf piirrite:OsmEntity ;
    skos:definition "Roads and other objects designated/signed to use for public transport buses."@en ;
    skos:inScheme piirritev:Bus ;
    skos:prefLabel "Designated"@en .

piirritev:ButtonOperated a skos:ConceptScheme ;
    piirrite:osmId "button_operated" ;
    skos:definition "Used to indicate that some functionality may be (or needs to be) activated by pressing a button."@en ;
    skos:prefLabel "Button operated, types"@en .

piirritev:Cables a skos:ConceptScheme ;
    piirrite:osmId "cables" ;
    skos:definition "Number of electrically separated, individual or bundled, power-carrying conductors in a power segment, section or circuit."@en ;
    skos:prefLabel "Cables, types"@en .

piirritev:Capacity a skos:ConceptScheme ;
    piirrite:osmId "capacity" ;
    skos:definition "Describes the capacity a facility is suitable for."@en ;
    skos:prefLabel "Capacity, types"@en .

piirritev:Cemetery a skos:ConceptScheme ;
    piirrite:osmId "cemetery" ;
    skos:definition "Specifies parts of a cemetery, single graves or special kinds of cemeteries."@en ;
    skos:prefLabel "Cemetery, types"@en .

piirritev:CheckDate a skos:ConceptScheme ;
    piirrite:osmId "check_date" ;
    skos:definition "Date of latest review of the data. Format: YYYY-MM-DD."@en ;
    skos:prefLabel "Check date, types"@en .

piirritev:Circuits a skos:ConceptScheme ;
    piirrite:osmId "circuits" ;
    skos:definition "Number of electrical circuits in a power section, line, or cable."@en ;
    skos:prefLabel "Circuits, types"@en .

piirritev:Circumference a skos:ConceptScheme ;
    piirrite:osmId "circumference" ;
    skos:definition "Circumference (in metres) of a tree's trunk at the height of 1.3 metre above ground."@en ;
    skos:prefLabel "Circumference, types"@en .

piirritev:CollectionTimes a skos:ConceptScheme ;
    piirrite:osmId "collection_times" ;
    skos:definition "The collection times of a post box or recycling container"@en ;
    skos:prefLabel "Collection times, types"@en .

piirritev:ColourGrey a skos:Concept ;
    piirrite:osmId "grey" ;
    rdfs:subClassOf piirrite:OsmEntity ;
    skos:definition ""@en ;
    skos:inScheme piirritev:Colour ;
    skos:prefLabel "Grey"@en .

piirritev:Comment a skos:ConceptScheme ;
    piirrite:osmId "comment" ;
    skos:definition "group=annotations"@en ;
    skos:prefLabel "Comment, types"@en .

piirritev:ConditionDeficient a skos:Concept ;
    piirrite:osmId "deficient" ;
    rdfs:subClassOf piirrite:OsmEntity ;
    skos:definition ""@en ;
    skos:inScheme piirritev:Condition ;
    skos:prefLabel "Deficient"@en .

piirritev:ConditionFair a skos:Concept ;
    piirrite:osmId "fair" ;
    rdfs:subClassOf piirrite:OsmEntity ;
    skos:definition ""@en ;
    skos:inScheme piirritev:Condition ;
    skos:prefLabel "Fair"@en .

piirritev:ConditionGood a skos:Concept ;
    piirrite:osmId "good" ;
    rdfs:subClassOf piirrite:OsmEntity ;
    skos:definition ""@en ;
    skos:inScheme piirritev:Condition ;
    skos:prefLabel "Good"@en .

piirritev:ConstructionApartments a skos:Concept ;
    piirrite:hasRelatedOsmTag piirrite:hasApartmentsBuilding ;
    piirrite:osmId "apartments" ;
    rdfs:subClassOf piirrite:OsmEntity ;
    skos:definition "Used together with tag:building=construction to mark that a building under construction is a residential building used by multiple families/groups."@en ;
    skos:inScheme piirritev:Construction ;
    skos:prefLabel "Apartments"@en .

piirritev:ConstructionBuilding a skos:Concept ;
    piirrite:osmId "building" ;
    rdfs:subClassOf piirrite:OsmEntity ;
    skos:definition "Denotes that a construction site creates a building. May be deemed controversial."@en ;
    skos:inScheme piirritev:Construction ;
    skos:prefLabel "Building"@en .

piirritev:ConstructionDate a skos:ConceptScheme ;
    piirrite:osmId "construction_date" ;
    skos:definition "Indicates the date the construction of the feature was finished."@en ;
    skos:prefLabel "Construction date, types"@en .

piirritev:ConstructionFootway a skos:Concept ;
    piirrite:osmId "footway" ;
    rdfs:subClassOf piirrite:OsmEntity ;
    skos:definition ""@en ;
    skos:inScheme piirritev:Construction ;
    skos:prefLabel "Footway"@en .

piirritev:ConstructionHouse a skos:Concept ;
    piirrite:hasRelatedOsmTag piirrite:hasHouseBuilding ;
    piirrite:osmId "house" ;
    rdfs:subClassOf piirrite:OsmEntity ;
    skos:definition "Used together with tag:building=construction to mark that building under construction is a house."@en ;
    skos:inScheme piirritev:Construction ;
    skos:prefLabel "House"@en .

piirritev:ConstructionMotorway a skos:Concept ;
    piirrite:osmId "motorway" ;
    rdfs:subClassOf piirrite:OsmEntity ;
    skos:definition ""@en ;
    skos:inScheme piirritev:Construction ;
    skos:prefLabel "Motorway"@en .

piirritev:ConstructionMotorwayLink a skos:Concept ;
    piirrite:osmId "motorway_link" ;
    rdfs:subClassOf piirrite:OsmEntity ;
    skos:definition ""@en ;
    skos:inScheme piirritev:Construction ;
    skos:prefLabel "Motorway link"@en .

piirritev:ConstructionPrimary a skos:Concept ;
    piirrite:osmId "primary" ;
    rdfs:subClassOf piirrite:OsmEntity ;
    skos:definition ""@en ;
    skos:inScheme piirritev:Construction ;
    skos:prefLabel "Primary"@en .

piirritev:ConstructionRail a skos:Concept ;
    piirrite:osmId "rail" ;
    rdfs:subClassOf piirrite:OsmEntity ;
    skos:definition ""@en ;
    skos:inScheme piirritev:Construction ;
    skos:prefLabel "Rail"@en .

piirritev:ConstructionResidential a skos:Concept ;
    piirrite:osmId "residential" ;
    rdfs:subClassOf piirrite:OsmEntity ;
    skos:definition ""@en ;
    skos:inScheme piirritev:Construction ;
    skos:prefLabel "Residential"@en .

piirritev:ConstructionSecondary a skos:Concept ;
    piirrite:osmId "secondary" ;
    rdfs:subClassOf piirrite:OsmEntity ;
    skos:definition ""@en ;
    skos:inScheme piirritev:Construction ;
    skos:prefLabel "Secondary"@en .

piirritev:ConstructionService a skos:Concept ;
    piirrite:osmId "service" ;
    rdfs:subClassOf piirrite:OsmEntity ;
    skos:definition ""@en ;
    skos:inScheme piirritev:Construction ;
    skos:prefLabel "Service"@en .

piirritev:ConstructionShed a skos:Concept ;
    piirrite:osmId "shed" ;
    rdfs:subClassOf piirrite:OsmEntity ;
    skos:definition "Specifies that building construction is about a shed construction"@en ;
    skos:inScheme piirritev:Construction ;
    skos:prefLabel "Shed"@en .

piirritev:ConstructionTertiary a skos:Concept ;
    piirrite:osmId "tertiary" ;
    rdfs:subClassOf piirrite:OsmEntity ;
    skos:definition ""@en ;
    skos:inScheme piirritev:Construction ;
    skos:prefLabel "Tertiary"@en .

piirritev:ConstructionTrunk a skos:Concept ;
    piirrite:osmId "trunk" ;
    rdfs:subClassOf piirrite:OsmEntity ;
    skos:definition ""@en ;
    skos:inScheme piirritev:Construction ;
    skos:prefLabel "Trunk"@en .

piirritev:ConstructionUnclassified a skos:Concept ;
    piirrite:osmId "unclassified" ;
    rdfs:subClassOf piirrite:OsmEntity ;
    skos:definition ""@en ;
    skos:inScheme piirritev:Construction ;
    skos:prefLabel "Unclassified"@en .

piirritev:Content a skos:ConceptScheme ;
    piirrite:osmId "content" ;
    skos:definition "To describe the contents of a feature used to store materials."@en ;
    skos:prefLabel "Content, types"@en .

piirritev:Couplings a skos:ConceptScheme ;
    piirrite:osmId "couplings" ;
    skos:definition "For specifying the number of places on a fire hydrant or dry riser inlet where a hose can connect."@en ;
    skos:prefLabel "Couplings, types"@en .

piirritev:CoveredBooth a skos:Concept ;
    piirrite:osmId "booth" ;
    rdfs:subClassOf piirrite:OsmEntity ;
    skos:definition ""@en ;
    skos:inScheme piirritev:Covered ;
    skos:prefLabel "Booth"@en .

piirritev:Craft a skos:ConceptScheme ;
    piirrite:osmId "craft" ;
    skos:definition "A place producing or processing customized goods"@en ;
    skos:prefLabel "Craft, types"@en .

piirritev:CreatedByAlmienCoastlines a skos:Concept ;
    piirrite:osmId "almien_coastlines" ;
    rdfs:subClassOf piirrite:OsmEntity ;
    skos:definition ""@en ;
    skos:inScheme piirritev:CreatedBy ;
    skos:prefLabel "Almien coastlines"@en .

piirritev:CreatedByArcgisExporter a skos:Concept ;
    piirrite:osmId "ArcGIS_Exporter" ;
    rdfs:subClassOf piirrite:OsmEntity ;
    skos:definition ""@en ;
    skos:inScheme piirritev:CreatedBy ;
    skos:prefLabel "Arcgis exporter"@en .

piirritev:CreatedByCoastbot a skos:Concept ;
    piirrite:osmId "coastbot" ;
    rdfs:subClassOf piirrite:OsmEntity ;
    skos:definition ""@en ;
    skos:inScheme piirritev:CreatedBy ;
    skos:prefLabel "Coastbot"@en .

piirritev:CreatedByDmgroomCoastlines a skos:Concept ;
    piirrite:osmId "dmgroom_coastlines" ;
    rdfs:subClassOf piirrite:OsmEntity ;
    skos:definition ""@en ;
    skos:inScheme piirritev:CreatedBy ;
    skos:prefLabel "Dmgroom coastlines"@en .

piirritev:CreatedByEditop a skos:Concept ;
    piirrite:osmId "Editop" ;
    rdfs:subClassOf piirrite:OsmEntity ;
    skos:definition ""@en ;
    skos:inScheme piirritev:CreatedBy ;
    skos:prefLabel "Editop"@en .

piirritev:CreatedByGeobasenhn2Osm a skos:Concept ;
    piirrite:osmId "geobaseNHN2osm" ;
    rdfs:subClassOf piirrite:OsmEntity ;
    skos:definition ""@en ;
    skos:inScheme piirritev:CreatedBy ;
    skos:prefLabel "Geobasenhn2osm"@en .

piirritev:CreatedByGpsbabel-135 a skos:Concept ;
    piirrite:osmId "GPSBabel-1_3_5" ;
    rdfs:subClassOf piirrite:OsmEntity ;
    skos:definition ""@en ;
    skos:inScheme piirritev:CreatedBy ;
    skos:prefLabel "Gpsbabel-1 3 5"@en .

piirritev:CreatedByGpsbabel-136 a skos:Concept ;
    piirrite:osmId "GPSBabel-1_3_6" ;
    rdfs:subClassOf piirrite:OsmEntity ;
    skos:definition ""@en ;
    skos:inScheme piirritev:CreatedBy ;
    skos:prefLabel "Gpsbabel-1 3 6"@en .

piirritev:CreatedByJosm a skos:Concept ;
    piirrite:osmId "JOSM" ;
    rdfs:subClassOf piirrite:OsmEntity ;
    skos:definition ""@en ;
    skos:inScheme piirritev:CreatedBy ;
    skos:prefLabel "Josm"@en .

piirritev:CreatedByMerkaartor011 a skos:Concept ;
    piirrite:osmId "Merkaartor_0_11" ;
    rdfs:subClassOf piirrite:OsmEntity ;
    skos:definition ""@en ;
    skos:inScheme piirritev:CreatedBy ;
    skos:prefLabel "Merkaartor 0 11"@en .

piirritev:CreatedByMerkaartor012 a skos:Concept ;
    piirrite:osmId "Merkaartor_0_12" ;
    rdfs:subClassOf piirrite:OsmEntity ;
    skos:definition ""@en ;
    skos:inScheme piirritev:CreatedBy ;
    skos:prefLabel "Merkaartor 0 12"@en .

piirritev:CreatedByMerkaartor013 a skos:Concept ;
    piirrite:osmId "Merkaartor_0_13" ;
    rdfs:subClassOf piirrite:OsmEntity ;
    skos:definition ""@en ;
    skos:inScheme piirritev:CreatedBy ;
    skos:prefLabel "Merkaartor 0 13"@en .

piirritev:CreatedByPolyshp2Osm a skos:Concept ;
    piirrite:osmId "polyshp2osm" ;
    rdfs:subClassOf piirrite:OsmEntity ;
    skos:definition ""@en ;
    skos:inScheme piirritev:CreatedBy ;
    skos:prefLabel "Polyshp2osm"@en .

piirritev:CreatedByPotlatch010B a skos:Concept ;
    piirrite:osmId "Potlatch_0_10b" ;
    rdfs:subClassOf piirrite:OsmEntity ;
    skos:definition ""@en ;
    skos:inScheme piirritev:CreatedBy ;
    skos:prefLabel "Potlatch 0 10b"@en .

piirritev:CreatedByPotlatch010F a skos:Concept ;
    piirrite:osmId "Potlatch_0_10f" ;
    rdfs:subClassOf piirrite:OsmEntity ;
    skos:definition ""@en ;
    skos:inScheme piirritev:CreatedBy ;
    skos:prefLabel "Potlatch 0 10f"@en .

piirritev:CreatedByPotlatch09C a skos:Concept ;
    piirrite:osmId "Potlatch_0_9c" ;
    rdfs:subClassOf piirrite:OsmEntity ;
    skos:definition ""@en ;
    skos:inScheme piirritev:CreatedBy ;
    skos:prefLabel "Potlatch 0 9c"@en .

piirritev:CreatedByShp2Osm a skos:Concept ;
    piirrite:osmId "shp2osm" ;
    rdfs:subClassOf piirrite:OsmEntity ;
    skos:definition ""@en ;
    skos:inScheme piirritev:CreatedBy ;
    skos:prefLabel "Shp2osm"@en .

piirritev:CreatedByShpupload a skos:Concept ;
    piirrite:osmId "shpupload" ;
    rdfs:subClassOf piirrite:OsmEntity ;
    skos:definition ""@en ;
    skos:inScheme piirritev:CreatedBy ;
    skos:prefLabel "Shpupload"@en .

piirritev:CreatedByYahooapplet10 a skos:Concept ;
    piirrite:osmId "YahooApplet_1_0" ;
    rdfs:subClassOf piirrite:OsmEntity ;
    skos:definition ""@en ;
    skos:inScheme piirritev:CreatedBy ;
    skos:prefLabel "Yahooapplet 1 0"@en .

piirritev:CropCereal a skos:Concept ;
    piirrite:osmId "cereal" ;
    rdfs:subClassOf piirrite:OsmEntity ;
    skos:definition "Unspecified cereal crop fieldimage=File:Cereal_field_at_Sutton_Courtney_-_geograph.org.uk_-_1348877.jpg"@en ;
    skos:inScheme piirritev:Crop ;
    skos:prefLabel "Cereal"@en .

piirritev:CropCorn a skos:Concept ;
    piirrite:osmId "corn" ;
    rdfs:subClassOf piirrite:OsmEntity ;
    skos:definition ""@en ;
    skos:inScheme piirritev:Crop ;
    skos:prefLabel "Corn"@en .

piirritev:CropGrape a skos:Concept ;
    piirrite:osmId "grape" ;
    rdfs:subClassOf piirrite:OsmEntity ;
    skos:definition "Specifies that grapes are grown here."@en ;
    skos:inScheme piirritev:Crop ;
    skos:prefLabel "Grape"@en .

piirritev:CropGrass a skos:Concept ;
    piirrite:osmId "grass" ;
    rdfs:subClassOf piirrite:OsmEntity ;
    skos:definition "Unspecified grass crop."@en ;
    skos:inScheme piirritev:Crop ;
    skos:prefLabel "Grass"@en .

piirritev:CropHop a skos:Concept ;
    piirrite:hasRelatedOsmTag piirrite:hasHopLanduse ;
    piirrite:osmId "hop" ;
    rdfs:subClassOf piirrite:OsmEntity ;
    skos:definition "Specifies that an area of farmland is being used to grow hops."@en ;
    skos:inScheme piirritev:Crop ;
    skos:prefLabel "Hop"@en .

piirritev:CropMarketGardening a skos:Concept ;
    piirrite:osmId "market_gardening" ;
    rdfs:subClassOf piirrite:OsmEntity ;
    skos:definition ""@en ;
    skos:inScheme piirritev:Crop ;
    skos:prefLabel "Market gardening"@en .

piirritev:CropRice a skos:Concept ;
    piirrite:hasRelatedOsmTag piirrite:hasRiceLanduse ;
    piirrite:osmId "rice" ;
    rdfs:subClassOf piirrite:OsmEntity ;
    skos:definition "Specifies that an area of farmland is being used to grow rice."@en ;
    skos:inScheme piirritev:Crop ;
    skos:prefLabel "Rice"@en .

piirritev:CropSugarcane a skos:Concept ;
    piirrite:osmId "sugarcane" ;
    rdfs:subClassOf piirrite:OsmEntity ;
    skos:definition "Specifies that an area of farmland is being used to grow sugarcane"@en ;
    skos:inScheme piirritev:Crop ;
    skos:prefLabel "Sugarcane"@en .

piirritev:CropTea a skos:Concept ;
    piirrite:hasRelatedOsmTag piirrite:hasTeaLanduse ;
    piirrite:osmId "tea" ;
    rdfs:subClassOf piirrite:OsmEntity ;
    skos:definition "Specifies that an agricultural feature produces tea leaves."@en ;
    skos:inScheme piirritev:Crop ;
    skos:prefLabel "Tea"@en .

piirritev:CropWheat a skos:Concept ;
    piirrite:osmId "wheat" ;
    rdfs:subClassOf piirrite:OsmEntity ;
    skos:definition "Specifies that an area of farmland is being used to grow wheat."@en ;
    skos:inScheme piirritev:Crop ;
    skos:prefLabel "Wheat"@en .

piirritev:Crossing a skos:ConceptScheme ;
    piirrite:osmId "crossing" ;
    skos:definition "Further refinement for nodes already tagged with tag:highway=crossing or tag:railway=crossing"@en ;
    skos:prefLabel "Crossing, types"@en .

piirritev:CrossingRefPelican a skos:Concept ;
    piirrite:hasRelatedOsmTag piirrite:hasPelicanButtonOperated,
        piirrite:hasPelicanTactilePaving ;
    piirrite:osmId "pelican" ;
    rdfs:subClassOf piirrite:OsmEntity ;
    skos:definition "Pelican pedestrian crossings."@en ;
    skos:inScheme piirritev:CrossingRef ;
    skos:prefLabel "Pelican"@en .

piirritev:CrossingRefToucan a skos:Concept ;
    piirrite:osmId "toucan" ;
    rdfs:subClassOf piirrite:OsmEntity ;
    skos:definition ""@en ;
    skos:inScheme piirritev:CrossingRef ;
    skos:prefLabel "Toucan"@en .

piirritev:CrossingRefZebra a skos:Concept ;
    piirrite:hasRelatedOsmTag piirrite:hasZebraCrossing,
        piirrite:hasZebraKerb,
        piirrite:hasZebraLit,
        piirrite:hasZebraSupervised,
        piirrite:hasZebraTactilePaving,
        piirrite:hasZebraWheelchair ;
    piirrite:osmId "zebra" ;
    rdfs:subClassOf piirrite:OsmEntity ;
    skos:definition "A legal zebra crossing."@en ;
    skos:inScheme piirritev:CrossingRef ;
    skos:prefLabel "Zebra"@en .

piirritev:Delivery a skos:ConceptScheme ;
    piirrite:osmId "delivery" ;
    skos:definition "Sets whether the restaurant or shop offers delivery service."@en ;
    skos:prefLabel "Delivery, types"@en .

piirritev:DenominationAnglican a skos:Concept ;
    piirrite:osmId "anglican" ;
    rdfs:subClassOf piirrite:OsmEntity ;
    skos:definition ""@en ;
    skos:inScheme piirritev:Denomination ;
    skos:prefLabel "Anglican"@en .

piirritev:DenominationBaptist a skos:Concept ;
    piirrite:osmId "baptist" ;
    rdfs:subClassOf piirrite:OsmEntity ;
    skos:definition ""@en ;
    skos:inScheme piirritev:Denomination ;
    skos:prefLabel "Baptist"@en .

piirritev:DenominationCatholic a skos:Concept ;
    piirrite:hasRelatedOsmTag piirrite:hasCatholicAmenity,
        piirrite:hasCatholicLanduse ;
    piirrite:osmId "catholic" ;
    rdfs:subClassOf piirrite:OsmEntity ;
    skos:definition "Unspecified Catholic denomination."@en ;
    skos:inScheme piirritev:Denomination ;
    skos:prefLabel "Catholic"@en .

piirritev:DenominationEvangelical a skos:Concept ;
    piirrite:osmId "evangelical" ;
    rdfs:subClassOf piirrite:OsmEntity ;
    skos:definition ""@en ;
    skos:inScheme piirritev:Denomination ;
    skos:prefLabel "Evangelical"@en .

piirritev:DenominationGreekOrthodox a skos:Concept ;
    piirrite:osmId "greek_orthodox" ;
    rdfs:subClassOf piirrite:OsmEntity ;
    skos:definition ""@en ;
    skos:inScheme piirritev:Denomination ;
    skos:prefLabel "Greek orthodox"@en .

piirritev:DenominationJehovahsWitness a skos:Concept ;
    piirrite:hasRelatedOsmTag piirrite:hasJehovahsWitnessAmenity,
        piirrite:hasJehovahsWitnessBuilding ;
    piirrite:osmId "jehovahs_witness" ;
    rdfs:subClassOf piirrite:OsmEntity ;
    skos:definition "Meeting place where Jehovah's Witnesses hold religious services."@en ;
    skos:inScheme piirritev:Denomination ;
    skos:prefLabel "Jehovahs witness"@en .

piirritev:DenominationLutheran a skos:Concept ;
    piirrite:osmId "lutheran" ;
    rdfs:subClassOf piirrite:OsmEntity ;
    skos:definition ""@en ;
    skos:inScheme piirritev:Denomination ;
    skos:prefLabel "Lutheran"@en .

piirritev:DenominationMethodist a skos:Concept ;
    piirrite:osmId "methodist" ;
    rdfs:subClassOf piirrite:OsmEntity ;
    skos:definition ""@en ;
    skos:inScheme piirritev:Denomination ;
    skos:prefLabel "Methodist"@en .

piirritev:DenominationOrthodox a skos:Concept ;
    piirrite:osmId "orthodox" ;
    rdfs:subClassOf piirrite:OsmEntity ;
    skos:definition ""@en ;
    skos:inScheme piirritev:Denomination ;
    skos:prefLabel "Orthodox"@en .

piirritev:DenominationPentecostal a skos:Concept ;
    piirrite:osmId "pentecostal" ;
    rdfs:subClassOf piirrite:OsmEntity ;
    skos:definition ""@en ;
    skos:inScheme piirritev:Denomination ;
    skos:prefLabel "Pentecostal"@en .

piirritev:DenominationPresbyterian a skos:Concept ;
    piirrite:osmId "presbyterian" ;
    rdfs:subClassOf piirrite:OsmEntity ;
    skos:definition ""@en ;
    skos:inScheme piirritev:Denomination ;
    skos:prefLabel "Presbyterian"@en .

piirritev:DenominationProtestant a skos:Concept ;
    piirrite:osmId "protestant" ;
    rdfs:subClassOf piirrite:OsmEntity ;
    skos:definition ""@en ;
    skos:inScheme piirritev:Denomination ;
    skos:prefLabel "Protestant"@en .

piirritev:DenominationRomanCatholic a skos:Concept ;
    piirrite:osmId "roman_catholic" ;
    rdfs:subClassOf piirrite:OsmEntity ;
    skos:definition ""@en ;
    skos:inScheme piirritev:Denomination ;
    skos:prefLabel "Roman catholic"@en .

piirritev:DenominationRussianOrthodox a skos:Concept ;
    piirrite:osmId "russian_orthodox" ;
    rdfs:subClassOf piirrite:OsmEntity ;
    skos:definition ""@en ;
    skos:inScheme piirritev:Denomination ;
    skos:prefLabel "Russian orthodox"@en .

piirritev:DenominationSunni a skos:Concept ;
    piirrite:osmId "sunni" ;
    rdfs:subClassOf piirrite:OsmEntity ;
    skos:definition ""@en ;
    skos:inScheme piirritev:Denomination ;
    skos:prefLabel "Sunni"@en .

piirritev:DenominationTheravada a skos:Concept ;
    piirrite:osmId "theravada" ;
    rdfs:subClassOf piirrite:OsmEntity ;
    skos:definition ""@en ;
    skos:inScheme piirritev:Denomination ;
    skos:prefLabel "Theravada"@en .

piirritev:DenotationAgricultural a skos:Concept ;
    piirrite:hasRelatedOsmTag piirrite:hasAgriculturalCrop,
        piirrite:hasAgriculturalProduce,
        piirrite:hasAgriculturalSpecies,
        piirrite:hasAgriculturalTrees ;
    piirrite:osmId "agricultural" ;
    rdfs:subClassOf piirrite:OsmEntity ;
    skos:definition "A tree in agricultural use"@en ;
    skos:inScheme piirritev:Denotation ;
    skos:prefLabel "Agricultural"@en .

piirritev:DenotationAvenue a skos:Concept ;
    piirrite:osmId "avenue" ;
    rdfs:subClassOf piirrite:OsmEntity ;
    skos:definition "A tree aligned along a road."@en ;
    skos:inScheme piirritev:Denotation ;
    skos:prefLabel "Avenue"@en .

piirritev:DenotationDecoration a skos:Concept ;
    piirrite:osmId "decoration" ;
    rdfs:subClassOf piirrite:OsmEntity ;
    skos:definition ""@en ;
    skos:inScheme piirritev:Denotation ;
    skos:prefLabel "Decoration"@en .

piirritev:DenotationGarden a skos:Concept ;
    piirrite:osmId "garden" ;
    rdfs:subClassOf piirrite:OsmEntity ;
    skos:definition "A tree located within a garden."@en ;
    skos:inScheme piirritev:Denotation ;
    skos:prefLabel "Garden"@en .

piirritev:DenotationLandmark a skos:Concept ;
    piirrite:osmId "landmark" ;
    rdfs:subClassOf piirrite:OsmEntity ;
    skos:definition "A tree or other feature remarkable due to its size or prominent location, usually visible from great distances and useful for navigation."@en ;
    skos:inScheme piirritev:Denotation ;
    skos:prefLabel "Landmark"@en .

piirritev:DenotationNaturalMonument a skos:Concept ;
    piirrite:osmId "natural_monument" ;
    rdfs:subClassOf piirrite:OsmEntity ;
    skos:definition "An especially old tree, often with a particular shape and usually protected for its uniqueness."@en ;
    skos:inScheme piirritev:Denotation ;
    skos:prefLabel "Natural monument"@en .

piirritev:DenotationPark a skos:Concept ;
    piirrite:osmId "park" ;
    rdfs:subClassOf piirrite:OsmEntity ;
    skos:definition "A tree located within an urban park."@en ;
    skos:inScheme piirritev:Denotation ;
    skos:prefLabel "Park"@en .

piirritev:DenotationSingle a skos:Concept ;
    piirrite:osmId "single" ;
    rdfs:subClassOf piirrite:OsmEntity ;
    skos:definition ""@en ;
    skos:inScheme piirritev:Denotation ;
    skos:prefLabel "Single"@en .

piirritev:DenotationStreet a skos:Concept ;
    piirrite:osmId "street" ;
    rdfs:subClassOf piirrite:OsmEntity ;
    skos:definition ""@en ;
    skos:inScheme piirritev:Denotation ;
    skos:prefLabel "Street"@en .

piirritev:DenotationUrban a skos:Concept ;
    piirrite:osmId "urban" ;
    rdfs:subClassOf piirrite:OsmEntity ;
    skos:definition "An \"urban\" tree, usually found within settlements, e.g. in parks or spread through residential areas."@en ;
    skos:inScheme piirritev:Denotation ;
    skos:prefLabel "Urban"@en .

piirritev:DeparturesBoard a skos:ConceptScheme ;
    piirrite:osmId "departures_board" ;
    skos:definition "A board in an airport, train station, bus terminal or stop, etc displaying the information about future departures."@en ;
    skos:prefLabel "Departures board, types"@en .

piirritev:Depth a skos:ConceptScheme ;
    piirrite:osmId "depth" ;
    skos:definition "The depth of a feature, in metres."@en ;
    skos:prefLabel "Depth, types"@en .

piirritev:DescriptionAnnexe a skos:Concept ;
    piirrite:osmId "Annexe" ;
    rdfs:subClassOf piirrite:OsmEntity ;
    skos:definition ""@en ;
    skos:inScheme piirritev:Description ;
    skos:prefLabel "Annexe"@en .

piirritev:DescriptionCastaa a skos:Concept ;
    piirrite:osmId "Castaa" ;
    rdfs:subClassOf piirrite:OsmEntity ;
    skos:definition ""@en ;
    skos:inScheme piirritev:Description ;
    skos:prefLabel "Castaa"@en .

piirritev:DescriptionMaize a skos:Concept ;
    piirrite:osmId "Maize" ;
    rdfs:subClassOf piirrite:OsmEntity ;
    skos:definition ""@en ;
    skos:inScheme piirritev:Description ;
    skos:prefLabel "Maize"@en .

piirritev:DescriptionSubcentre a skos:Concept ;
    piirrite:osmId "SubCentre" ;
    rdfs:subClassOf piirrite:OsmEntity ;
    skos:definition ""@en ;
    skos:inScheme piirritev:Description ;
    skos:prefLabel "Subcentre"@en .

piirritev:Design a skos:ConceptScheme ;
    piirrite:osmId "design" ;
    skos:definition "Describes the design of poles or pylons carrying high voltage electricity cables"@en ;
    skos:prefLabel "Design, types"@en .

piirritev:DesignationCivilParish a skos:Concept ;
    piirrite:hasRelatedOsmTag piirrite:hasCivilParishAdminLevel,
        piirrite:hasCivilParishBoundary,
        piirrite:hasCivilParishGovernment ;
    piirrite:osmId "civil_parish" ;
    rdfs:subClassOf piirrite:OsmEntity ;
    skos:definition "An administrative district forming part of local government."@en ;
    skos:inScheme piirritev:Designation ;
    skos:prefLabel "Civil parish"@en .

piirritev:DesignationPublicBridleway a skos:Concept ;
    piirrite:hasRelatedOsmTag piirrite:hasPublicBridlewayAccess,
        piirrite:hasPublicBridlewayProwRef,
        piirrite:hasPublicBridlewaySurface ;
    piirrite:osmId "public_bridleway" ;
    rdfs:subClassOf piirrite:OsmEntity ;
    skos:definition "A legal classification of a highway on which the public have a right to travel on foot, horseback, and by bicycle."@en ;
    skos:inScheme piirritev:Designation ;
    skos:prefLabel "Public bridleway"@en .

piirritev:DesignationPublicFootpath a skos:Concept ;
    piirrite:hasRelatedOsmTag piirrite:hasPublicFootpathAccess,
        piirrite:hasPublicFootpathProwRef,
        piirrite:hasPublicFootpathSurface ;
    piirrite:osmId "public_footpath" ;
    rdfs:subClassOf piirrite:OsmEntity ;
    skos:definition "A legal classification of a highway on which the public have a right to travel on foot."@en ;
    skos:inScheme piirritev:Designation ;
    skos:prefLabel "Public footpath"@en .

piirritev:Destination a skos:ConceptScheme ;
    piirrite:osmId "destination" ;
    skos:definition "Destination when following a linear feature."@en ;
    skos:prefLabel "Destination, types"@en .

piirritev:Diameter a skos:ConceptScheme ;
    piirrite:osmId "diameter" ;
    skos:definition "nominal diameter in millimeter"@en ;
    skos:prefLabel "Diameter, types"@en .

piirritev:DiameterCrown a skos:ConceptScheme ;
    piirrite:osmId "diameter_crown" ;
    skos:definition ""@en ;
    skos:prefLabel "Diameter crown, types"@en .

piirritev:DirectionBackward a skos:Concept ;
    piirrite:osmId "backward" ;
    rdfs:subClassOf piirrite:OsmEntity ;
    skos:definition ""@en ;
    skos:inScheme piirritev:Direction ;
    skos:prefLabel "Backward"@en .

piirritev:DirectionBoth a skos:Concept ;
    piirrite:osmId "both" ;
    rdfs:subClassOf piirrite:OsmEntity ;
    skos:definition ""@en ;
    skos:inScheme piirritev:Direction ;
    skos:prefLabel "Both"@en .

piirritev:DirectionClockwise a skos:Concept ;
    piirrite:osmId "clockwise" ;
    rdfs:subClassOf piirrite:OsmEntity ;
    skos:definition ""@en ;
    skos:inScheme piirritev:Direction ;
    skos:prefLabel "Clockwise"@en .

piirritev:DirectionE a skos:Concept ;
    piirrite:osmId "E" ;
    rdfs:subClassOf piirrite:OsmEntity ;
    skos:definition ""@en ;
    skos:inScheme piirritev:Direction ;
    skos:prefLabel "E"@en .

piirritev:DirectionForward a skos:Concept ;
    piirrite:osmId "forward" ;
    rdfs:subClassOf piirrite:OsmEntity ;
    skos:definition ""@en ;
    skos:inScheme piirritev:Direction ;
    skos:prefLabel "Forward"@en .

piirritev:DirectionS a skos:Concept ;
    piirrite:osmId "S" ;
    rdfs:subClassOf piirrite:OsmEntity ;
    skos:definition ""@en ;
    skos:inScheme piirritev:Direction ;
    skos:prefLabel "S"@en .

piirritev:DirectionSe a skos:Concept ;
    piirrite:osmId "SE" ;
    rdfs:subClassOf piirrite:OsmEntity ;
    skos:definition ""@en ;
    skos:inScheme piirritev:Direction ;
    skos:prefLabel "Se"@en .

piirritev:DirectionSse a skos:Concept ;
    piirrite:osmId "SSE" ;
    rdfs:subClassOf piirrite:OsmEntity ;
    skos:definition ""@en ;
    skos:inScheme piirritev:Direction ;
    skos:prefLabel "Sse"@en .

piirritev:DirectionSsw a skos:Concept ;
    piirrite:osmId "SSW" ;
    rdfs:subClassOf piirrite:OsmEntity ;
    skos:definition ""@en ;
    skos:inScheme piirritev:Direction ;
    skos:prefLabel "Ssw"@en .

piirritev:DirectionSw a skos:Concept ;
    piirrite:osmId "SW" ;
    rdfs:subClassOf piirrite:OsmEntity ;
    skos:definition ""@en ;
    skos:inScheme piirritev:Direction ;
    skos:prefLabel "Sw"@en .

piirritev:DirectionW a skos:Concept ;
    piirrite:osmId "W" ;
    rdfs:subClassOf piirrite:OsmEntity ;
    skos:definition ""@en ;
    skos:inScheme piirritev:Direction ;
    skos:prefLabel "W"@en .

piirritev:Dispensing a skos:ConceptScheme ;
    piirrite:osmId "dispensing" ;
    skos:definition "Whether a pharmacy dispenses prescription drugs or not."@en ;
    skos:prefLabel "Dispensing, types"@en .

piirritev:Distance a skos:ConceptScheme ;
    piirrite:osmId "distance" ;
    skos:definition "Distance (i.e. extent; length from start to finish) of a route given in kilometres, or distance along a route marked by milestone."@en ;
    skos:prefLabel "Distance, types"@en .

piirritev:Disused a skos:ConceptScheme ;
    piirrite:osmId "disused" ;
    skos:definition "Specifies if a feature is disused but in a reasonable state of repair."@en ;
    skos:prefLabel "Disused, types"@en .

piirritev:Dog a skos:ConceptScheme ;
    piirrite:osmId "dog" ;
    skos:definition "Describes if dogs are allowed"@en ;
    skos:prefLabel "Dog, types"@en .

piirritev:DrinkingWater a skos:ConceptScheme ;
    piirrite:osmId "drinking_water" ;
    skos:definition "Indication whether a feature provides drinking water."@en ;
    skos:prefLabel "Drinking water, types"@en .

piirritev:DriveThrough a skos:ConceptScheme ;
    piirrite:osmId "drive_through" ;
    skos:definition "To indicate whether an amenity offers a drive-through service."@en ;
    skos:prefLabel "Drive through, types"@en .

piirritev:DualCarriageway a skos:ConceptScheme ;
    piirrite:osmId "dual_carriageway" ;
    skos:definition "Specifies whether a highway is a dual-carriageway (divided) road"@en ;
    skos:prefLabel "Dual carriageway, types"@en .

piirritev:EducationKindergarten a skos:Concept ;
    piirrite:hasRelatedOsmTag piirrite:hasKindergartenName,
        piirrite:hasKindergartenOperator,
        piirrite:hasKindergartenPhone ;
    piirrite:osmId "kindergarten" ;
    rdfs:subClassOf piirrite:OsmEntity ;
    skos:definition "A place for looking after preschool children and (typically) giving early education."@en ;
    skos:inScheme piirritev:Education ;
    skos:prefLabel "Kindergarten"@en .

piirritev:EducationSchool a skos:Concept ;
    piirrite:hasRelatedOsmTag piirrite:hasSchoolAmenity,
        piirrite:hasSchoolGrades ;
    piirrite:osmId "school" ;
    rdfs:subClassOf piirrite:OsmEntity ;
    skos:definition "A primary or secondary school (pupils typically aged 6 to 18)."@en ;
    skos:inScheme piirritev:Education ;
    skos:prefLabel "School"@en .

piirritev:Ele a skos:ConceptScheme ;
    piirrite:osmId "ele" ;
    skos:definition "Elevation of a point above sea level, in metres."@en ;
    skos:prefLabel "Ele, types"@en .

piirritev:ElectrifiedContactLine a skos:Concept ;
    piirrite:hasRelatedOsmTag piirrite:hasContactLineRailway ;
    piirrite:osmId "contact_line" ;
    rdfs:subClassOf piirrite:OsmEntity ;
    skos:definition "An overhead line."@en ;
    skos:inScheme piirritev:Electrified ;
    skos:prefLabel "Contact line"@en .

piirritev:ElectrifiedRail a skos:Concept ;
    piirrite:hasRelatedOsmTag piirrite:hasRailRailway ;
    piirrite:osmId "rail" ;
    rdfs:subClassOf piirrite:OsmEntity ;
    skos:definition "Electrified with a third rail system."@en ;
    skos:inScheme piirritev:Electrified ;
    skos:prefLabel "Rail"@en .

piirritev:Email a skos:ConceptScheme ;
    piirrite:osmId "email" ;
    skos:definition "An email address associated with the object"@en ;
    skos:prefLabel "Email, types"@en .

piirritev:Embankment a skos:ConceptScheme ;
    piirrite:osmId "embankment" ;
    skos:definition "A dyke or raised bank to carry a road, railway, or canal across a low-lying or wet area."@en ;
    skos:prefLabel "Embankment, types"@en .

piirritev:EmergencyAccessPoint a skos:Concept ;
    piirrite:hasRelatedOsmTag piirrite:hasAccessPointName,
        piirrite:hasAccessPointOperator,
        piirrite:hasAccessPointRef ;
    piirrite:osmId "access_point" ;
    rdfs:subClassOf piirrite:OsmEntity ;
    skos:definition "A sign number which can be used to define your current position in case of an emergency"@en ;
    skos:inScheme piirritev:Emergency ;
    skos:prefLabel "Access point"@en .

piirritev:EmergencyAmbulanceStation a skos:Concept ;
    piirrite:hasRelatedOsmTag piirrite:hasAmbulanceStationName,
        piirrite:hasAmbulanceStationOperator ;
    piirrite:osmId "ambulance_station" ;
    rdfs:subClassOf piirrite:OsmEntity ;
    skos:definition "An ambulance station is a structure or other area set aside for storage of ambulance vehicles, medical equipment, personal protective equipment, and other medical supplies."@en ;
    skos:inScheme piirritev:Emergency ;
    skos:prefLabel "Ambulance station"@en .

piirritev:EmergencyAssemblyPoint a skos:Concept ;
    piirrite:hasRelatedOsmTag piirrite:hasAssemblyPointCheckDate,
        piirrite:hasAssemblyPointName,
        piirrite:hasAssemblyPointOperator,
        piirrite:hasAssemblyPointRef ;
    piirrite:osmId "assembly_point" ;
    rdfs:subClassOf piirrite:OsmEntity ;
    skos:definition "A designated (safe) place where people can gather or must report to during an emergency or a fire drill."@en ;
    skos:inScheme piirritev:Emergency ;
    skos:prefLabel "Assembly point"@en .

piirritev:EmergencyDefibrillator a skos:Concept ;
    piirrite:hasRelatedOsmTag piirrite:hasDefibrillatorAccess,
        piirrite:hasDefibrillatorOpeningHours,
        piirrite:hasDefibrillatorPhone ;
    piirrite:osmId "defibrillator" ;
    rdfs:subClassOf piirrite:OsmEntity ;
    skos:definition "Defibrillator (AED), an external and portable electronic device that diagnoses and can correct arrhythmia of the heart automatically."@en ;
    skos:inScheme piirritev:Emergency ;
    skos:prefLabel "Defibrillator"@en .

piirritev:EmergencyDesignated a skos:Concept ;
    piirrite:hasRelatedOsmTag piirrite:hasDesignatedSurface ;
    piirrite:osmId "designated" ;
    rdfs:subClassOf piirrite:OsmEntity ;
    skos:definition "An emergency access road"@en ;
    skos:inScheme piirritev:Emergency ;
    skos:prefLabel "Designated"@en .

piirritev:EmergencyFireExtinguisher a skos:Concept ;
    piirrite:osmId "fire_extinguisher" ;
    rdfs:subClassOf piirrite:OsmEntity ;
    skos:definition "An active fire protection device used to extinguish or control small fires, often in emergency situations."@en ;
    skos:inScheme piirritev:Emergency ;
    skos:prefLabel "Fire extinguisher"@en .

piirritev:EmergencyFireHydrant a skos:Concept ;
    piirrite:hasRelatedOsmTag piirrite:hasFireHydrantRef,
        piirrite:hasFireHydrantType,
        piirrite:hasFireHydrantWaterSource ;
    piirrite:osmId "fire_hydrant" ;
    rdfs:subClassOf piirrite:OsmEntity ;
    skos:definition "An active fire protection measure, and a source of water provided in most urban, suburban, and rural areas with municipal water service to enable fire fighters to tap into the municipal water supply to assist in extinguishing a fire."@en ;
    skos:inScheme piirritev:Emergency ;
    skos:prefLabel "Fire hydrant"@en .

piirritev:EmergencyLifeRing a skos:Concept ;
    piirrite:hasRelatedOsmTag piirrite:hasLifeRingColour,
        piirrite:hasLifeRingOperator,
        piirrite:hasLifeRingRef,
        piirrite:hasLifeRingSupport ;
    piirrite:osmId "life_ring" ;
    rdfs:subClassOf piirrite:OsmEntity ;
    skos:definition "A floating ring to throw out to someone who is struggling in water."@en ;
    skos:inScheme piirritev:Emergency ;
    skos:prefLabel "Life ring"@en .

piirritev:EmergencyPhone a skos:Concept ;
    piirrite:hasRelatedOsmTag piirrite:hasPhoneOperator,
        piirrite:hasPhoneRef ;
    piirrite:osmId "phone" ;
    rdfs:subClassOf piirrite:OsmEntity ;
    skos:definition "Emergency telephone osmcarto-rendering=File:Emergency-phone.16.svg osmcarto-rendering-size=28px"@en ;
    skos:inScheme piirritev:Emergency ;
    skos:prefLabel "Phone"@en .

piirritev:EmergencySiren a skos:Concept ;
    piirrite:hasRelatedOsmTag piirrite:hasSirenOperator,
        piirrite:hasSirenWebsite ;
    piirrite:osmId "siren" ;
    rdfs:subClassOf piirrite:OsmEntity ;
    skos:definition "A loud noise maker, such as an air raid siren or a tornado siren."@en ;
    skos:inScheme piirritev:Emergency ;
    skos:prefLabel "Siren"@en .

piirritev:EmergencySuctionPoint a skos:Concept ;
    piirrite:osmId "suction_point" ;
    rdfs:subClassOf piirrite:OsmEntity ;
    skos:definition "A preferred point to pump water off a river or other waters for a fire department."@en ;
    skos:inScheme piirritev:Emergency ;
    skos:prefLabel "Suction point"@en .

piirritev:EmergencyWaterTank a skos:Concept ;
    piirrite:hasRelatedOsmTag piirrite:hasWaterTankAccess,
        piirrite:hasWaterTankCapacity,
        piirrite:hasWaterTankContent,
        piirrite:hasWaterTankIntermittent,
        piirrite:hasWaterTankName,
        piirrite:hasWaterTankOperator,
        piirrite:hasWaterTankWaterVolume ;
    piirrite:osmId "water_tank" ;
    rdfs:subClassOf piirrite:OsmEntity ;
    skos:definition "A large water basin or tank for a fire department to take water."@en ;
    skos:inScheme piirritev:Emergency ;
    skos:prefLabel "Water tank"@en .

piirritev:Entrance a skos:ConceptScheme ;
    piirrite:osmId "entrance" ;
    skos:definition "To mark the location of an entrance."@en ;
    skos:prefLabel "Entrance, types"@en .

piirritev:EstWidth a skos:ConceptScheme ;
    piirrite:osmId "est_width" ;
    skos:definition "The estimated width of a feature"@en ;
    skos:prefLabel "Est width, types"@en .

piirritev:Expressway a skos:ConceptScheme ;
    piirrite:osmId "expressway" ;
    skos:definition "A highway with high-speed design features and limited access to adjacent properties. Usually a dual-carriageway (divided)."@en ;
    skos:prefLabel "Expressway, types"@en .

piirritev:Fax a skos:ConceptScheme ;
    piirrite:osmId "fax" ;
    skos:definition "A fax number associated with the object."@en ;
    skos:prefLabel "Fax, types"@en .

piirritev:Fee a skos:ConceptScheme ;
    piirrite:osmId "fee" ;
    skos:definition "Yes or no, to indicate if money is charged to use this facility."@en ;
    skos:prefLabel "Fee, types"@en .

piirritev:FenceTypeBarbedWire a skos:Concept ;
    piirrite:osmId "barbed_wire" ;
    rdfs:subClassOf piirrite:OsmEntity ;
    skos:definition ""@en ;
    skos:inScheme piirritev:FenceType ;
    skos:prefLabel "Barbed wire"@en .

piirritev:FenceTypeBars a skos:Concept ;
    piirrite:osmId "bars" ;
    rdfs:subClassOf piirrite:OsmEntity ;
    skos:definition ""@en ;
    skos:inScheme piirritev:FenceType ;
    skos:prefLabel "Bars"@en .

piirritev:FenceTypeChainLink a skos:Concept ;
    piirrite:osmId "chain_link" ;
    rdfs:subClassOf piirrite:OsmEntity ;
    skos:definition ""@en ;
    skos:inScheme piirritev:FenceType ;
    skos:prefLabel "Chain link"@en .

piirritev:FenceTypeConcrete a skos:Concept ;
    piirrite:osmId "concrete" ;
    rdfs:subClassOf piirrite:OsmEntity ;
    skos:definition ""@en ;
    skos:inScheme piirritev:FenceType ;
    skos:prefLabel "Concrete"@en .

piirritev:FenceTypeMetal a skos:Concept ;
    piirrite:osmId "metal" ;
    rdfs:subClassOf piirrite:OsmEntity ;
    skos:definition ""@en ;
    skos:inScheme piirritev:FenceType ;
    skos:prefLabel "Metal"@en .

piirritev:FenceTypePole a skos:Concept ;
    piirrite:osmId "pole" ;
    rdfs:subClassOf piirrite:OsmEntity ;
    skos:definition ""@en ;
    skos:inScheme piirritev:FenceType ;
    skos:prefLabel "Pole"@en .

piirritev:FenceTypeRailing a skos:Concept ;
    piirrite:osmId "railing" ;
    rdfs:subClassOf piirrite:OsmEntity ;
    skos:definition "A railing for example at the edge of a bridge to prevent persons or vehicles from falling down. Often made of metal or wood."@en ;
    skos:inScheme piirritev:FenceType ;
    skos:prefLabel "Railing"@en .

piirritev:FenceTypeSplitRail a skos:Concept ;
    piirrite:osmId "split_rail" ;
    rdfs:subClassOf piirrite:OsmEntity ;
    skos:definition ""@en ;
    skos:inScheme piirritev:FenceType ;
    skos:prefLabel "Split rail"@en .

piirritev:FenceTypeWire a skos:Concept ;
    piirrite:osmId "wire" ;
    rdfs:subClassOf piirrite:OsmEntity ;
    skos:definition ""@en ;
    skos:inScheme piirritev:FenceType ;
    skos:prefLabel "Wire"@en .

piirritev:FenceTypeWood a skos:Concept ;
    piirrite:osmId "wood" ;
    rdfs:subClassOf piirrite:OsmEntity ;
    skos:definition ""@en ;
    skos:inScheme piirritev:FenceType ;
    skos:prefLabel "Wood"@en .

piirritev:Fid a skos:ConceptScheme ;
    piirrite:osmId "fid" ;
    skos:definition "Used to assign a unique identifier to each feature within a geospatial file; required by some formats such as GeoPackage."@en ;
    skos:prefLabel "Fid, types"@en .

piirritev:FixmeContinue a skos:Concept ;
    piirrite:osmId "continue" ;
    rdfs:subClassOf piirrite:OsmEntity ;
    skos:definition ""@en ;
    skos:inScheme piirritev:Fixme ;
    skos:prefLabel "Continue"@en .

piirritev:FixmeIncomplete a skos:Concept ;
    piirrite:osmId "incomplete" ;
    rdfs:subClassOf piirrite:OsmEntity ;
    skos:definition ""@en ;
    skos:inScheme piirritev:Fixme ;
    skos:prefLabel "Incomplete"@en .

piirritev:FixmeName a skos:Concept ;
    piirrite:osmId "name" ;
    rdfs:subClassOf piirrite:OsmEntity ;
    skos:definition "To define if the object has a (possible) erroneous name."@en ;
    skos:inScheme piirritev:Fixme ;
    skos:prefLabel "Name"@en .

piirritev:FixmePosition a skos:Concept ;
    piirrite:osmId "position" ;
    rdfs:subClassOf piirrite:OsmEntity ;
    skos:definition ""@en ;
    skos:inScheme piirritev:Fixme ;
    skos:prefLabel "Position"@en .

piirritev:FixmePositionEstimated a skos:Concept ;
    piirrite:osmId "Position_estimated" ;
    rdfs:subClassOf piirrite:OsmEntity ;
    skos:definition ""@en ;
    skos:inScheme piirritev:Fixme ;
    skos:prefLabel "Position estimated"@en .

piirritev:FixmeResurvey a skos:Concept ;
    piirrite:osmId "resurvey" ;
    rdfs:subClassOf piirrite:OsmEntity ;
    skos:definition ""@en ;
    skos:inScheme piirritev:Fixme ;
    skos:prefLabel "Resurvey"@en .

piirritev:FixmeStub a skos:Concept ;
    piirrite:osmId "stub" ;
    rdfs:subClassOf piirrite:OsmEntity ;
    skos:definition ""@en ;
    skos:inScheme piirritev:Fixme ;
    skos:prefLabel "Stub"@en .

piirritev:Floating a skos:ConceptScheme ;
    piirrite:osmId "floating" ;
    skos:definition "This property indicates whether an object floats"@en ;
    skos:prefLabel "Floating, types"@en .

piirritev:FootCustomers a skos:Concept ;
    piirrite:osmId "customers" ;
    rdfs:subClassOf piirrite:OsmEntity ;
    skos:definition ""@en ;
    skos:inScheme piirritev:Foot ;
    skos:prefLabel "Customers"@en .

piirritev:FootDesignated a skos:Concept ;
    piirrite:osmId "designated" ;
    rdfs:subClassOf piirrite:OsmEntity ;
    skos:definition "A preferred or designated route for pedestrians."@en ;
    skos:inScheme piirritev:Foot ;
    skos:prefLabel "Designated"@en .

piirritev:FootDestination a skos:Concept ;
    piirrite:hasRelatedOsmTag piirrite:hasDestinationHighway ;
    piirrite:osmId "destination" ;
    rdfs:subClassOf piirrite:OsmEntity ;
    skos:definition "Transit traffic forbidden for pedestrians, non-transit to a local destination allowed."@en ;
    skos:inScheme piirritev:Foot ;
    skos:prefLabel "Destination"@en .

piirritev:FootPermissive a skos:Concept ;
    piirrite:hasRelatedOsmTag piirrite:hasPermissiveHighway ;
    piirrite:osmId "permissive" ;
    rdfs:subClassOf piirrite:OsmEntity ;
    skos:definition "Access by pedestrians is permitted but permission may be withdrawn at any time."@en ;
    skos:inScheme piirritev:Foot ;
    skos:prefLabel "Permissive"@en .

piirritev:FootPrivate a skos:Concept ;
    piirrite:osmId "private" ;
    rdfs:subClassOf piirrite:OsmEntity ;
    skos:definition "Indicates that walking is not allowed for public, but the owner may make exceptions at will."@en ;
    skos:inScheme piirritev:Foot ;
    skos:prefLabel "Private"@en .

piirritev:FootUseSidepath a skos:Concept ;
    piirrite:hasRelatedOsmTag piirrite:hasUseSidepathHighway ;
    piirrite:osmId "use_sidepath" ;
    rdfs:subClassOf piirrite:OsmEntity ;
    skos:definition "Use compulsory parallel footpath instead"@en ;
    skos:inScheme piirritev:Foot ;
    skos:prefLabel "Use sidepath"@en .

piirritev:FootwayAccessAisle a skos:Concept ;
    piirrite:hasRelatedOsmTag piirrite:hasAccessAisleType ;
    piirrite:osmId "access_aisle" ;
    rdfs:subClassOf piirrite:OsmEntity ;
    skos:definition "A marked footpath in a parking lot, typically between two parking spaces, to facilitate access to parked vehicles."@en ;
    skos:inScheme piirritev:Footway ;
    skos:prefLabel "Access aisle"@en .

piirritev:FootwayAlley a skos:Concept ;
    piirrite:hasRelatedOsmTag piirrite:hasAlleyAccess,
        piirrite:hasAlleyFootway ;
    piirrite:osmId "alley" ;
    rdfs:subClassOf piirrite:OsmEntity ;
    skos:definition "An alley is a footway usually located between properties for access to back entrances and/or emergency access. onNode = no onWay = yes onArea = no onRelation = no requires = * highway=footway combination = * {{keyaccess}} seeAlso = * footway status = in use"@en ;
    skos:inScheme piirritev:Footway ;
    skos:prefLabel "Alley"@en .

piirritev:FootwayCrossing a skos:Concept ;
    piirrite:hasRelatedOsmTag piirrite:hasCrossingEstWidth,
        piirrite:hasCrossingIncline,
        piirrite:hasCrossingKerb,
        piirrite:hasCrossingSmoothness,
        piirrite:hasCrossingSurface,
        piirrite:hasCrossingTactilePaving,
        piirrite:hasCrossingType,
        piirrite:hasCrossingWheelchair,
        piirrite:hasCrossingWidth ;
    piirrite:osmId "crossing" ;
    rdfs:subClassOf piirrite:OsmEntity ;
    skos:definition "Specifies that the footway is a road crossing."@en ;
    skos:inScheme piirritev:Footway ;
    skos:prefLabel "Crossing"@en .

piirritev:FootwayLink a skos:Concept ;
    piirrite:hasRelatedOsmTag piirrite:hasLinkLit,
        piirrite:hasLinkSurface,
        piirrite:hasLinkWheelchair ;
    piirrite:osmId "link" ;
    rdfs:subClassOf piirrite:OsmEntity ;
    skos:definition "A traversable path connecting other highways to enable routing."@en ;
    skos:inScheme piirritev:Footway ;
    skos:prefLabel "Link"@en .

piirritev:FootwayPath a skos:Concept ;
    piirrite:osmId "path" ;
    rdfs:subClassOf piirrite:OsmEntity ;
    skos:definition "Used for pedestrian paths not linked to roads. onNode = no onWay = yes onArea = no onRelation = no requires = * highway=footway status = in use"@en ;
    skos:inScheme piirritev:Footway ;
    skos:prefLabel "Path"@en .

piirritev:FootwaySidewalk a skos:Concept ;
    piirrite:hasRelatedOsmTag piirrite:hasSidewalkEstWidth,
        piirrite:hasSidewalkIncline,
        piirrite:hasSidewalkKerb,
        piirrite:hasSidewalkSmoothness,
        piirrite:hasSidewalkSurface,
        piirrite:hasSidewalkTactilePaving,
        piirrite:hasSidewalkType,
        piirrite:hasSidewalkWheelchair,
        piirrite:hasSidewalkWidth ;
    piirrite:osmId "sidewalk" ;
    rdfs:subClassOf piirrite:OsmEntity ;
    skos:definition "Sidewalks as separate ways."@en ;
    skos:inScheme piirritev:Footway ;
    skos:prefLabel "Sidewalk"@en .

piirritev:FootwayTrafficIsland a skos:Concept ;
    piirrite:hasRelatedOsmTag piirrite:hasTrafficIslandEstWidth,
        piirrite:hasTrafficIslandFootway,
        piirrite:hasTrafficIslandIncline,
        piirrite:hasTrafficIslandKerb,
        piirrite:hasTrafficIslandSmoothness,
        piirrite:hasTrafficIslandSurface,
        piirrite:hasTrafficIslandTactilePaving,
        piirrite:hasTrafficIslandWheelchair,
        piirrite:hasTrafficIslandWidth ;
    piirrite:osmId "traffic_island" ;
    rdfs:subClassOf piirrite:OsmEntity ;
    skos:definition "Parts of a footway that serves as pedestrian refuge on a traffic island. onNode = no onWay = yes onArea = no onRelation = no requires = * highway=footway combination = * {{keykerb}} * {{keyincline}} * {{keywheelchair}} * {{keysmoothness}} * {{keysurface}} * {{keytactile_paving}} * {{keywidth}} / {{keyest_width}} seeAlso = * footway=crossing * footway=sidewalk * {{Keyfootway}} * {{Keycrossing:island}} status = de facto"@en ;
    skos:inScheme piirritev:Footway ;
    skos:prefLabel "Traffic island"@en .

piirritev:FordSteppingStones a skos:Concept ;
    piirrite:osmId "stepping_stones" ;
    rdfs:subClassOf piirrite:OsmEntity ;
    skos:definition "A ford for crossing a waterway with stepping stones  osmcarto-rendering = File:Ford.16.svg  osmcarto-rendering-size = 28px"@en ;
    skos:inScheme piirritev:Ford ;
    skos:prefLabel "Stepping stones"@en .

piirritev:Frequency a skos:ConceptScheme ;
    piirrite:osmId "frequency" ;
    skos:definition "For describing the frequency of electric power supply networks and devices, electrified railways, trolleybuses and communications devices. The unit is Hz (cycles per second)."@en ;
    skos:prefLabel "Frequency, types"@en .

piirritev:From a skos:ConceptScheme ;
    piirrite:osmId "from" ;
    skos:definition "Start station"@en ;
    skos:prefLabel "From, types"@en .

piirritev:Gauge a skos:ConceptScheme ;
    piirrite:osmId "gauge" ;
    skos:definition "Used to describe the 'gauge' (distance between the inside of the rails) on railways."@en ;
    skos:prefLabel "Gauge, types"@en .

piirritev:Genus a skos:ConceptScheme ;
    piirrite:osmId "genus" ;
    skos:definition "The scientific name of the genus for a living or fossil organism."@en ;
    skos:prefLabel "Genus, types"@en .

piirritev:GolfBunker a skos:Concept ;
    piirrite:osmId "bunker" ;
    rdfs:subClassOf piirrite:OsmEntity ;
    skos:definition "A bunker of a golf course: a depression near the green or fairway that is usually filled with sand. osmcarto-rendering=File:Rendering-area-sand.png osmcarto-rendering-size=100px"@en ;
    skos:inScheme piirritev:Golf ;
    skos:prefLabel "Bunker"@en .

piirritev:GolfCartDesignated a skos:Concept ;
    piirrite:osmId "designated" ;
    rdfs:subClassOf piirrite:OsmEntity ;
    skos:definition ""@en ;
    skos:inScheme piirritev:GolfCart ;
    skos:prefLabel "Designated"@en .

piirritev:GolfCartpath a skos:Concept ;
    piirrite:osmId "cartpath" ;
    rdfs:subClassOf piirrite:OsmEntity ;
    skos:definition "Path for golf cart in golf course"@en ;
    skos:inScheme piirritev:Golf ;
    skos:prefLabel "Cartpath"@en .

piirritev:GolfFairway a skos:Concept ;
    piirrite:osmId "fairway" ;
    rdfs:subClassOf piirrite:OsmEntity ;
    skos:definition "Fairway of a golf course: an area between the tee box and the putting green where the grass is cut even and short. osmcarto-rendering=File:Landuse_grass.png osmcarto-rendering-size=125px"@en ;
    skos:inScheme piirritev:Golf ;
    skos:prefLabel "Fairway"@en .

piirritev:GolfHole a skos:Concept ;
    piirrite:hasRelatedOsmTag piirrite:hasHoleHandicap,
        piirrite:hasHoleName,
        piirrite:hasHolePar,
        piirrite:hasHoleRef ;
    piirrite:osmId "hole" ;
    rdfs:subClassOf piirrite:OsmEntity ;
    skos:definition "The path from tee area to the green osmcarto-rendering=File:Power_minor_line.png osmcarto-rendering-size=125px"@en ;
    skos:inScheme piirritev:Golf ;
    skos:prefLabel "Hole"@en .

piirritev:GolfPath a skos:Concept ;
    piirrite:osmId "path" ;
    rdfs:subClassOf piirrite:OsmEntity ;
    skos:definition "Walking Route Common in Links Style Golf."@en ;
    skos:inScheme piirritev:Golf ;
    skos:prefLabel "Path"@en .

piirritev:GolfPin a skos:Concept ;
    piirrite:osmId "pin" ;
    rdfs:subClassOf piirrite:OsmEntity ;
    skos:definition "The hole of a golf course osmcarto-rendering=File:Leisure-golf-pin.svg osmcarto-rendering-size=23px"@en ;
    skos:inScheme piirritev:Golf ;
    skos:prefLabel "Pin"@en .

piirritev:GolfRough a skos:Concept ;
    piirrite:osmId "rough" ;
    rdfs:subClassOf piirrite:OsmEntity ;
    skos:definition "The rough of a golf course: the area between the fairway or green and the out-of-bounds markers, where the grass there is cut higher and is often coarser. osmcarto-rendering=File:Golf-rough.png osmcarto-rendering-size=125px"@en ;
    skos:inScheme piirritev:Golf ;
    skos:prefLabel "Rough"@en .

piirritev:GolfTee a skos:Concept ;
    piirrite:osmId "tee" ;
    rdfs:subClassOf piirrite:OsmEntity ;
    skos:definition "Teeing ground: area where play begins on a golf hole. osmcarto-rendering=File:Landuse_grass.png osmcarto-rendering-size=125px"@en ;
    skos:inScheme piirritev:Golf ;
    skos:prefLabel "Tee"@en .

piirritev:GolfWaterHazard a skos:Concept ;
    piirrite:hasRelatedOsmTag piirrite:hasWaterHazardNatural ;
    piirrite:osmId "water_hazard" ;
    rdfs:subClassOf piirrite:OsmEntity ;
    skos:definition "A water hazard at a golf course, usually marked by yellow stakes or lines."@en ;
    skos:inScheme piirritev:Golf ;
    skos:prefLabel "Water hazard"@en .

piirritev:Government a skos:ConceptScheme ;
    piirrite:osmId "government" ;
    skos:definition "Indicates the subtypes of government agencies and institutions."@en ;
    skos:prefLabel "Government, types"@en .

piirritev:GtfsId a skos:ConceptScheme ;
    piirrite:osmId "gtfs_id" ;
    skos:definition "Using this tag is discouraged, use key:gtfs:stop_id, key:gtfs:route_id, key:gtfs:trip_id or key:gtfs:shape_id instead."@en ;
    skos:prefLabel "Gtfs id, types"@en .

piirritev:Handrail a skos:ConceptScheme ;
    piirrite:osmId "handrail" ;
    skos:definition "Defines whether there is at least one handrail."@en ;
    skos:prefLabel "Handrail, types"@en .

piirritev:HazmatDesignated a skos:Concept ;
    piirrite:osmId "designated" ;
    rdfs:subClassOf piirrite:OsmEntity ;
    skos:definition ""@en ;
    skos:inScheme piirritev:Hazmat ;
    skos:prefLabel "Designated"@en .

piirritev:Height a skos:ConceptScheme ;
    piirrite:osmId "height" ;
    skos:definition "Height is the measurement of vertical distance. It indicates how \"tall\" something is."@en ;
    skos:prefLabel "Height, types"@en .

piirritev:Heritage a skos:ConceptScheme ;
    piirrite:osmId "heritage" ;
    skos:definition "Site/building/object registered by an official heritage organisation"@en ;
    skos:prefLabel "Heritage, types"@en .

piirritev:HfcsMajorCollector a skos:Concept ;
    piirrite:osmId "Major_Collector" ;
    rdfs:subClassOf piirrite:OsmEntity ;
    skos:definition ""@en ;
    skos:inScheme piirritev:Hfcs ;
    skos:prefLabel "Major collector"@en .

piirritev:HfcsPrincipalArterial a skos:Concept ;
    piirrite:osmId "Principal_Arterial" ;
    rdfs:subClassOf piirrite:OsmEntity ;
    skos:definition ""@en ;
    skos:inScheme piirritev:Hfcs ;
    skos:prefLabel "Principal arterial"@en .

piirritev:HfcsUrbanCollector a skos:Concept ;
    piirrite:osmId "Urban_Collector" ;
    rdfs:subClassOf piirrite:OsmEntity ;
    skos:definition ""@en ;
    skos:inScheme piirritev:Hfcs ;
    skos:prefLabel "Urban collector"@en .

piirritev:HgvDelivery a skos:Concept ;
    piirrite:osmId "delivery" ;
    rdfs:subClassOf piirrite:OsmEntity ;
    skos:definition ""@en ;
    skos:inScheme piirritev:Hgv ;
    skos:prefLabel "Delivery"@en .

piirritev:HgvDesignated a skos:Concept ;
    piirrite:osmId "designated" ;
    rdfs:subClassOf piirrite:OsmEntity ;
    skos:definition ""@en ;
    skos:inScheme piirritev:Hgv ;
    skos:prefLabel "Designated"@en .

piirritev:HgvDestination a skos:Concept ;
    piirrite:osmId "destination" ;
    rdfs:subClassOf piirrite:OsmEntity ;
    skos:definition ""@en ;
    skos:inScheme piirritev:Hgv ;
    skos:prefLabel "Destination"@en .

piirritev:HgvLocal a skos:Concept ;
    piirrite:osmId "local" ;
    rdfs:subClassOf piirrite:OsmEntity ;
    skos:definition ""@en ;
    skos:inScheme piirritev:Hgv ;
    skos:prefLabel "Local"@en .

piirritev:Highspeed a skos:ConceptScheme ;
    piirrite:osmId "highspeed" ;
    skos:definition "High-speed rail"@en ;
    skos:prefLabel "Highspeed, types"@en .

piirritev:HighwayBridleway a skos:Concept ;
    piirrite:hasRelatedOsmTag piirrite:hasBridlewayName ;
    piirrite:osmId "bridleway" ;
    rdfs:subClassOf piirrite:OsmEntity ;
    skos:definition "A way intended for use by equestrians. osmcarto-rendering=File:Rendering-highway bridleway.png osmcarto-rendering-size=125px"@en ;
    skos:inScheme piirritev:Highway ;
    skos:prefLabel "Bridleway"@en .

piirritev:HighwayBusStop a skos:Concept ;
    piirrite:hasRelatedOsmTag piirrite:hasBusStopName,
        piirrite:hasBusStopPublicTransport,
        piirrite:hasBusStopShelter ;
    piirrite:osmId "bus_stop" ;
    rdfs:subClassOf piirrite:OsmEntity ;
    skos:definition "A bus stop is a place where public buses stop for passengers."@en ;
    skos:inScheme piirritev:Highway ;
    skos:prefLabel "Bus stop"@en .

piirritev:HighwayBusway a skos:Concept ;
    piirrite:hasRelatedOsmTag piirrite:hasBuswayAccess,
        piirrite:hasBuswayBicycle,
        piirrite:hasBuswayBusBay,
        piirrite:hasBuswayColour,
        piirrite:hasBuswayEmbeddedRails,
        piirrite:hasBuswayFoot,
        piirrite:hasBuswayHighway,
        piirrite:hasBuswayName,
        piirrite:hasBuswayOperator,
        piirrite:hasBuswayTrolleyWire ;
    piirrite:osmId "busway" ;
    rdfs:subClassOf piirrite:OsmEntity ;
    skos:definition "A dedicated, separate roadway for buses."@en ;
    skos:inScheme piirritev:Highway ;
    skos:prefLabel "Busway"@en .

piirritev:HighwayConstruction a skos:Concept ;
    piirrite:hasRelatedOsmTag piirrite:hasConstructionCheckDate,
        piirrite:hasConstructionOpeningDate,
        piirrite:hasConstructionType ;
    piirrite:osmId "construction" ;
    rdfs:subClassOf piirrite:OsmEntity ;
    skos:definition "A highway (road, track or path) currently under construction.  osmcarto-rendering = File:Rendering-highway construction tertiary carto.png  osmcarto-rendering-size = 125px"@en ;
    skos:inScheme piirritev:Highway ;
    skos:prefLabel "Construction"@en .

piirritev:HighwayCorridor a skos:Concept ;
    piirrite:hasRelatedOsmTag piirrite:hasCorridorAccess,
        piirrite:hasCorridorConveying,
        piirrite:hasCorridorLevel ;
    piirrite:osmId "corridor" ;
    rdfs:subClassOf piirrite:OsmEntity ;
    skos:definition "A corridor inside a building"@en ;
    skos:inScheme piirritev:Highway ;
    skos:prefLabel "Corridor"@en .

piirritev:HighwayCrossing a skos:Concept ;
    piirrite:hasRelatedOsmTag piirrite:hasCrossingType ;
    piirrite:osmId "crossing" ;
    rdfs:subClassOf piirrite:OsmEntity ;
    skos:definition "The location of a street crossing for pedestrians, cyclists, or equestrians."@en ;
    skos:inScheme piirritev:Highway ;
    skos:prefLabel "Crossing"@en .

piirritev:HighwayCycleway a skos:Concept ;
    piirrite:hasRelatedOsmTag piirrite:hasCyclewayLit,
        piirrite:hasCyclewayName,
        piirrite:hasCyclewaySegregated,
        piirrite:hasCyclewaySurface,
        piirrite:hasCyclewayWidth ;
    piirrite:osmId "cycleway" ;
    rdfs:subClassOf piirrite:OsmEntity ;
    skos:definition "For designated cycleways.  osmcarto-rendering = File:Cycleway osm.png  osmcarto-rendering-size = 125px"@en ;
    skos:inScheme piirritev:Highway ;
    skos:prefLabel "Cycleway"@en .

piirritev:HighwayElevator a skos:Concept ;
    piirrite:hasRelatedOsmTag piirrite:hasElevatorAccess,
        piirrite:hasElevatorBicycle,
        piirrite:hasElevatorGoods,
        piirrite:hasElevatorLevel,
        piirrite:hasElevatorManufacturer,
        piirrite:hasElevatorWheelchair ;
    piirrite:osmId "elevator" ;
    rdfs:subClassOf piirrite:OsmEntity ;
    skos:definition "An elevator (or lift) is used to travel vertically, providing passenger and freight access between pathways at different floor levels. May be solely vertical (typical case) or inclined. osmcarto-rendering=File:Elevator-12.svg osmcarto-rendering-size=24px"@en ;
    skos:inScheme piirritev:Highway ;
    skos:prefLabel "Elevator"@en .

piirritev:HighwayEmergencyBay a skos:Concept ;
    piirrite:osmId "emergency_bay" ;
    rdfs:subClassOf piirrite:OsmEntity ;
    skos:definition "An area beside a highway where you can safely stop your car in case of breakdown or emergency."@en ;
    skos:inScheme piirritev:Highway ;
    skos:prefLabel "Emergency bay"@en .

piirritev:HighwayFootway a skos:Concept ;
    piirrite:hasRelatedOsmTag piirrite:hasFootwayAccess,
        piirrite:hasFootwayBicycle,
        piirrite:hasFootwayCovered,
        piirrite:hasFootwayInformal,
        piirrite:hasFootwayLit,
        piirrite:hasFootwayName,
        piirrite:hasFootwaySurface,
        piirrite:hasFootwayTactilePaving,
        piirrite:hasFootwayType,
        piirrite:hasFootwayWheelchair ;
    piirrite:osmId "footway" ;
    rdfs:subClassOf piirrite:OsmEntity ;
    skos:definition "A path mainly or exclusively for pedestrians. osmcarto-rendering=File:Rendering-highway footway.png osmcarto-rendering-size=125px"@en ;
    skos:inScheme piirritev:Highway ;
    skos:prefLabel "Footway"@en .

piirritev:HighwayGiveWay a skos:Concept ;
    piirrite:hasRelatedOsmTag piirrite:hasGiveWayDirection ;
    piirrite:osmId "give_way" ;
    rdfs:subClassOf piirrite:OsmEntity ;
    skos:definition "Used to mark give way (also known as yield) signs or markings."@en ;
    skos:inScheme piirritev:Highway ;
    skos:prefLabel "Give way"@en .

piirritev:HighwayLivingStreet a skos:Concept ;
    piirrite:osmId "living_street" ;
    rdfs:subClassOf piirrite:OsmEntity ;
    skos:definition "Road with very low speed limits and other pedestrian friendly traffic rules. osmcarto-rendering=File:Living street osm.png osmcarto-rendering-size=125px"@en ;
    skos:inScheme piirritev:Highway ;
    skos:prefLabel "Living street"@en .

piirritev:HighwayMilestone a skos:Concept ;
    piirrite:hasRelatedOsmTag piirrite:hasMilestoneCarriagewayRef,
        piirrite:hasMilestoneDistance,
        piirrite:hasMilestoneMarker,
        piirrite:hasMilestoneRef ;
    piirrite:osmId "milestone" ;
    rdfs:subClassOf piirrite:OsmEntity ;
    skos:definition "Stone or metal marker on the side of a road indicating a reference and an approximation of the distance travelled."@en ;
    skos:inScheme piirritev:Highway ;
    skos:prefLabel "Milestone"@en .

piirritev:HighwayMiniRoundabout a skos:Concept ;
    piirrite:hasRelatedOsmTag piirrite:hasMiniRoundaboutDirection,
        piirrite:hasMiniRoundaboutName ;
    piirrite:osmId "mini_roundabout" ;
    rdfs:subClassOf piirrite:OsmEntity ;
    skos:definition "A road junction where the traffic goes around a painted circle or traversable island and has right of way. osmcarto-rendering=File:Highway mini roundabout.svg osmcarto-rendering-size=18px"@en ;
    skos:inScheme piirritev:Highway ;
    skos:prefLabel "Mini roundabout"@en .

piirritev:HighwayMotorway a skos:Concept ;
    piirrite:hasRelatedOsmTag piirrite:hasMotorwayDestination,
        piirrite:hasMotorwayLanes,
        piirrite:hasMotorwayName,
        piirrite:hasMotorwayRef,
        piirrite:hasMotorwayToll ;
    piirrite:osmId "motorway" ;
    rdfs:subClassOf piirrite:OsmEntity ;
    skos:definition "High capacity highways designed to safely carry fast motor traffic. osmcarto-rendering=File:Rendering-highway motorway carto.png osmcarto-rendering-size=125px"@en ;
    skos:inScheme piirritev:Highway ;
    skos:prefLabel "Motorway"@en .

piirritev:HighwayMotorwayJunction a skos:Concept ;
    piirrite:hasRelatedOsmTag piirrite:hasMotorwayJunctionName,
        piirrite:hasMotorwayJunctionRef ;
    piirrite:osmId "motorway_junction" ;
    rdfs:subClassOf piirrite:OsmEntity ;
    skos:definition "An exit from a motorway or other major road."@en ;
    skos:inScheme piirritev:Highway ;
    skos:prefLabel "Motorway junction"@en .

piirritev:HighwayMotorwayLink a skos:Concept ;
    piirrite:hasRelatedOsmTag piirrite:hasMotorwayLinkDestination,
        piirrite:hasMotorwayLinkMaxspeed ;
    piirrite:osmId "motorway_link" ;
    rdfs:subClassOf piirrite:OsmEntity ;
    skos:definition "The link roads (sliproads / ramps) leading to and from a motorway.  osmcarto-rendering = File:Rendering-highway motorway link.png  osmcarto-rendering-size = 125px"@en ;
    skos:inScheme piirritev:Highway ;
    skos:prefLabel "Motorway link"@en .

piirritev:HighwayPassingPlace a skos:Concept ;
    piirrite:osmId "passing_place" ;
    rdfs:subClassOf piirrite:OsmEntity ;
    skos:definition "A passing place on a single track road."@en ;
    skos:inScheme piirritev:Highway ;
    skos:prefLabel "Passing place"@en .

piirritev:HighwayPath a skos:Concept ;
    piirrite:hasRelatedOsmTag piirrite:hasPathAccess,
        piirrite:hasPathBicycle,
        piirrite:hasPathFoot,
        piirrite:hasPathHorse,
        piirrite:hasPathLit,
        piirrite:hasPathName,
        piirrite:hasPathSacScale,
        piirrite:hasPathSegregated,
        piirrite:hasPathSmoothness,
        piirrite:hasPathSurface,
        piirrite:hasPathTrailVisibility,
        piirrite:hasPathWidth ;
    piirrite:osmId "path" ;
    rdfs:subClassOf piirrite:OsmEntity ;
    skos:definition "A generic path used by pedestrians, small vehicles, for animal riding or livestock walking. Not designated for use by two-track vehicles. Unless subtagged very broad, non-specific meaning."@en ;
    skos:inScheme piirritev:Highway ;
    skos:prefLabel "Path"@en .

piirritev:HighwayPedestrian a skos:Concept ;
    piirrite:hasRelatedOsmTag piirrite:hasPedestrianArea,
        piirrite:hasPedestrianName,
        piirrite:hasPedestrianRef ;
    piirrite:osmId "pedestrian" ;
    rdfs:subClassOf piirrite:OsmEntity ;
    skos:definition "Roads mainly / exclusively for pedestrians osmcarto-rendering=File:Pedestrian with area osm.png osmcarto-rendering-size=125px osmcarto-rendering-area=File:Highway pedestrian footway path area.png osmcarto-rendering-area-size=125px"@en ;
    skos:inScheme piirritev:Highway ;
    skos:prefLabel "Pedestrian"@en .

piirritev:HighwayPlatform a skos:Concept ;
    piirrite:hasRelatedOsmTag piirrite:hasPlatformBench,
        piirrite:hasPlatformBin,
        piirrite:hasPlatformName,
        piirrite:hasPlatformOperator,
        piirrite:hasPlatformRef,
        piirrite:hasPlatformRouteRef,
        piirrite:hasPlatformShelter,
        piirrite:hasPlatformWheelchair ;
    piirrite:osmId "platform" ;
    rdfs:subClassOf piirrite:OsmEntity ;
    skos:definition "A platform at a bus stop or station. osmcarto-rendering-way=File:Rendering-highway_railway_platform_line.png osmcarto-rendering-way-size=125px osmcarto-rendering-area=File:Rendering-highway_railway_platform_area.png osmcarto-rendering-area-size=125px"@en ;
    skos:inScheme piirritev:Highway ;
    skos:prefLabel "Platform"@en .

piirritev:HighwayPrimary a skos:Concept ;
    piirrite:hasRelatedOsmTag piirrite:hasPrimaryBridge,
        piirrite:hasPrimaryDualCarriageway,
        piirrite:hasPrimaryFrom,
        piirrite:hasPrimaryIntRef,
        piirrite:hasPrimaryLanes,
        piirrite:hasPrimaryLit,
        piirrite:hasPrimaryMaxspeed,
        piirrite:hasPrimaryMinspeed,
        piirrite:hasPrimaryMotorroad,
        piirrite:hasPrimaryName,
        piirrite:hasPrimaryOldRef,
        piirrite:hasPrimaryOneway,
        piirrite:hasPrimaryOperator,
        piirrite:hasPrimaryRef,
        piirrite:hasPrimarySurface,
        piirrite:hasPrimaryTo,
        piirrite:hasPrimaryTunnel ;
    piirrite:osmId "primary" ;
    rdfs:subClassOf piirrite:OsmEntity ;
    skos:definition "A major highway linking large towns. In cities, a major arterial road. osmcarto-rendering=File:Rendering-highway primary carto.png osmcarto-rendering-size=125px"@en ;
    skos:inScheme piirritev:Highway ;
    skos:prefLabel "Primary"@en .

piirritev:HighwayPrimaryLink a skos:Concept ;
    piirrite:hasRelatedOsmTag piirrite:hasPrimaryLinkDestination,
        piirrite:hasPrimaryLinkMaxspeed,
        piirrite:hasPrimaryLinkOneway ;
    piirrite:osmId "primary_link" ;
    rdfs:subClassOf piirrite:OsmEntity ;
    skos:definition "Connecting slip roads/ramps of primary highways osmcarto-rendering=File:Rendering-highway primary link.png osmcarto-rendering-size=125px"@en ;
    skos:inScheme piirritev:Highway ;
    skos:prefLabel "Primary link"@en .

piirritev:HighwayProposed a skos:Concept ;
    piirrite:hasRelatedOsmTag piirrite:hasProposedType ;
    piirrite:osmId "proposed" ;
    rdfs:subClassOf piirrite:OsmEntity ;
    skos:definition "A road that is about to be built, but where any construction work hasn't yet been started."@en ;
    skos:inScheme piirritev:Highway ;
    skos:prefLabel "Proposed"@en .

piirritev:HighwayRaceway a skos:Concept ;
    piirrite:hasRelatedOsmTag piirrite:hasRacewaySport ;
    piirrite:osmId "raceway" ;
    rdfs:subClassOf piirrite:OsmEntity ;
    skos:definition "A racetrack for motorised racing, e.g. cars, motorbikes and karts. osmcarto-rendering=File:Rendering-highway-raceway-mapnik.png osmcarto-rendering-size=125px"@en ;
    skos:inScheme piirritev:Highway ;
    skos:prefLabel "Raceway"@en .

piirritev:HighwayResidential a skos:Concept ;
    piirrite:hasRelatedOsmTag piirrite:hasResidentialAccess,
        piirrite:hasResidentialName,
        piirrite:hasResidentialOneway,
        piirrite:hasResidentialSurface ;
    piirrite:osmId "residential" ;
    rdfs:subClassOf piirrite:OsmEntity ;
    skos:definition "Road in a residential area osmcarto-rendering=File:Rendering-highway residential.png osmcarto-rendering-size=125px"@en ;
    skos:inScheme piirritev:Highway ;
    skos:prefLabel "Residential"@en .

piirritev:HighwayRestArea a skos:Concept ;
    piirrite:hasRelatedOsmTag piirrite:hasRestAreaName,
        piirrite:hasRestAreaOperator,
        piirrite:hasRestAreaToilets ;
    piirrite:osmId "rest_area" ;
    rdfs:subClassOf piirrite:OsmEntity ;
    skos:definition "Place where drivers can leave the road to rest, but not refuel. osmcarto-rendering=File:Rendering-highway services.png osmcarto-rendering-size=100px"@en ;
    skos:inScheme piirritev:Highway ;
    skos:prefLabel "Rest area"@en .

piirritev:HighwayRoad a skos:Concept ;
    piirrite:hasRelatedOsmTag piirrite:hasRoadName,
        piirrite:hasRoadOneway ;
    piirrite:osmId "road" ;
    rdfs:subClassOf piirrite:OsmEntity ;
    skos:definition "Road with unknown classification. osmcarto-rendering=File:Rendering-highway-road-mapnik.png osmcarto-rendering-size=125px"@en ;
    skos:inScheme piirritev:Highway ;
    skos:prefLabel "Road"@en .

piirritev:HighwaySecondary a skos:Concept ;
    piirrite:hasRelatedOsmTag piirrite:hasSecondaryName,
        piirrite:hasSecondaryRef ;
    piirrite:osmId "secondary" ;
    rdfs:subClassOf piirrite:OsmEntity ;
    skos:definition "A highway linking large towns. In cities, an arterial road of lesser importance. osmcarto-rendering=File:Rendering-highway secondary carto.png osmcarto-rendering-size=125px"@en ;
    skos:inScheme piirritev:Highway ;
    skos:prefLabel "Secondary"@en .

piirritev:HighwaySecondaryLink a skos:Concept ;
    piirrite:hasRelatedOsmTag piirrite:hasSecondaryLinkOneway ;
    piirrite:osmId "secondary_link" ;
    rdfs:subClassOf piirrite:OsmEntity ;
    skos:definition "Connecting slip roads/ramps of secondary highways osmcarto-rendering = File:Rendering-highway secondary link.png osmcarto-rendering-size = 125px"@en ;
    skos:inScheme piirritev:Highway ;
    skos:prefLabel "Secondary link"@en .

piirritev:HighwayService a skos:Concept ;
    piirrite:hasRelatedOsmTag piirrite:hasServiceAccess,
        piirrite:hasServiceCovered,
        piirrite:hasServiceLit,
        piirrite:hasServiceLivingStreet,
        piirrite:hasServiceMaxspeed,
        piirrite:hasServiceName,
        piirrite:hasServiceOneway,
        piirrite:hasServiceSurface,
        piirrite:hasServiceTunnel,
        piirrite:hasServiceType ;
    piirrite:osmId "service" ;
    rdfs:subClassOf piirrite:OsmEntity ;
    skos:definition "Provides access to a building, service station, beach, campsite, industrial estate, business park, etc. osmcarto-rendering=File:Rendering-highway service.png osmcarto-rendering-size=125px"@en ;
    skos:inScheme piirritev:Highway ;
    skos:prefLabel "Service"@en .

piirritev:HighwayServices a skos:Concept ;
    piirrite:hasRelatedOsmTag piirrite:hasServicesName,
        piirrite:hasServicesOperator ;
    piirrite:osmId "services" ;
    rdfs:subClassOf piirrite:OsmEntity ;
    skos:definition "Place where drivers can leave a road to refuel, rest, or take refreshments. osmcarto-rendering=File:Rendering-highway services.png osmcarto-rendering-size=100px"@en ;
    skos:inScheme piirritev:Highway ;
    skos:prefLabel "Services"@en .

piirritev:HighwaySpeedCamera a skos:Concept ;
    piirrite:hasRelatedOsmTag piirrite:hasSpeedCameraColour,
        piirrite:hasSpeedCameraDirection,
        piirrite:hasSpeedCameraMaxspeed,
        piirrite:hasSpeedCameraOperator,
        piirrite:hasSpeedCameraRef ;
    piirrite:osmId "speed_camera" ;
    rdfs:subClassOf piirrite:OsmEntity ;
    skos:definition "A fixed road-side or overhead speed camera."@en ;
    skos:inScheme piirritev:Highway ;
    skos:prefLabel "Speed camera"@en .

piirritev:HighwaySteps a skos:Concept ;
    piirrite:hasRelatedOsmTag piirrite:hasStepsConveying,
        piirrite:hasStepsIncline,
        piirrite:hasStepsRamp,
        piirrite:hasStepsStepCount ;
    piirrite:osmId "steps" ;
    rdfs:subClassOf piirrite:OsmEntity ;
    skos:definition "For flights of steps on footways and paths. osmcarto-rendering=File:Rendering-highway steps.png osmcarto-rendering-size=125px"@en ;
    skos:inScheme piirritev:Highway ;
    skos:prefLabel "Steps"@en .

piirritev:HighwayStop a skos:Concept ;
    piirrite:hasRelatedOsmTag piirrite:hasStopDirection,
        piirrite:hasStopType ;
    piirrite:osmId "stop" ;
    rdfs:subClassOf piirrite:OsmEntity ;
    skos:definition "A point at which a vehicle must come to a complete stop."@en ;
    skos:inScheme piirritev:Highway ;
    skos:prefLabel "Stop"@en .

piirritev:HighwayStreetLamp a skos:Concept ;
    piirrite:hasRelatedOsmTag piirrite:hasStreetLampLampModel,
        piirrite:hasStreetLampLampMount,
        piirrite:hasStreetLampLampType ;
    piirrite:osmId "street_lamp" ;
    rdfs:subClassOf piirrite:OsmEntity ;
    skos:definition "A single pole with one or more lights to illuminate the street."@en ;
    skos:inScheme piirritev:Highway ;
    skos:prefLabel "Street lamp"@en .

piirritev:HighwayTertiary a skos:Concept ;
    piirrite:hasRelatedOsmTag piirrite:hasTertiaryCycleway,
        piirrite:hasTertiaryEmbeddedRails,
        piirrite:hasTertiaryEstWidth,
        piirrite:hasTertiaryLaneMarkings,
        piirrite:hasTertiaryLanes,
        piirrite:hasTertiaryLit,
        piirrite:hasTertiaryLocName,
        piirrite:hasTertiaryMaxspeed,
        piirrite:hasTertiaryMaxweight,
        piirrite:hasTertiaryName,
        piirrite:hasTertiaryOldName,
        piirrite:hasTertiaryOneway,
        piirrite:hasTertiaryRef,
        piirrite:hasTertiarySidewalk,
        piirrite:hasTertiarySurface,
        piirrite:hasTertiaryWidth,
        piirrite:hasTertiaryWinterService ;
    piirrite:osmId "tertiary" ;
    rdfs:subClassOf piirrite:OsmEntity ;
    skos:definition "A road linking small settlements, or the local centres of a large town or city. osmcarto-rendering=File:Rendering-highway tertiary carto.png osmcarto-rendering-size=125px"@en ;
    skos:inScheme piirritev:Highway ;
    skos:prefLabel "Tertiary"@en .

piirritev:HighwayTertiaryLink a skos:Concept ;
    piirrite:hasRelatedOsmTag piirrite:hasTertiaryLinkOneway ;
    piirrite:osmId "tertiary_link" ;
    rdfs:subClassOf piirrite:OsmEntity ;
    skos:definition "Connecting slip road/ramp of a tertiary highway. osmcarto-rendering=File:Rendering-highway tertiary link.png osmcarto-rendering-size=125px"@en ;
    skos:inScheme piirritev:Highway ;
    skos:prefLabel "Tertiary link"@en .

piirritev:HighwayTrack a skos:Concept ;
    piirrite:hasRelatedOsmTag piirrite:hasTrackAccess,
        piirrite:hasTrackName,
        piirrite:hasTrackRef,
        piirrite:hasTrackSmoothness,
        piirrite:hasTrackSurface,
        piirrite:hasTrackTracktype,
        piirrite:hasTrackWidth ;
    piirrite:osmId "track" ;
    rdfs:subClassOf piirrite:OsmEntity ;
    skos:definition "A minor land-access road like a farm or forest track. osmcarto-rendering=File:Mapnik-tracktype-not-set.png osmcarto-rendering-size=125px"@en ;
    skos:inScheme piirritev:Highway ;
    skos:prefLabel "Track"@en .

piirritev:HighwayTrafficMirror a skos:Concept ;
    piirrite:osmId "traffic_mirror" ;
    rdfs:subClassOf piirrite:OsmEntity ;
    skos:definition "Mirror that reflects the traffic on one road when direct view is blocked."@en ;
    skos:inScheme piirritev:Highway ;
    skos:prefLabel "Traffic mirror"@en .

piirritev:HighwayTrafficSignals a skos:Concept ;
    piirrite:hasRelatedOsmTag piirrite:hasTrafficSignalsName,
        piirrite:hasTrafficSignalsRef ;
    piirrite:osmId "traffic_signals" ;
    rdfs:subClassOf piirrite:OsmEntity ;
    skos:definition "A traffic signal (or a set of those) for regulating circulation. osmcarto-rendering=File:Traffic light-16.svg osmcarto-rendering-size=28px"@en ;
    skos:inScheme piirritev:Highway ;
    skos:prefLabel "Traffic signals"@en .

piirritev:HighwayTrailhead a skos:Concept ;
    piirrite:hasRelatedOsmTag piirrite:hasTrailheadName,
        piirrite:hasTrailheadOperator ;
    piirrite:osmId "trailhead" ;
    rdfs:subClassOf piirrite:OsmEntity ;
    skos:definition "A trailhead is a designated or customary place where a trip on a trail begins or ends."@en ;
    skos:inScheme piirritev:Highway ;
    skos:prefLabel "Trailhead"@en .

piirritev:HighwayTrunk a skos:Concept ;
    piirrite:hasRelatedOsmTag piirrite:hasTrunkDestination,
        piirrite:hasTrunkExpressway,
        piirrite:hasTrunkLanes,
        piirrite:hasTrunkMotorroad,
        piirrite:hasTrunkName,
        piirrite:hasTrunkOneway,
        piirrite:hasTrunkRef ;
    piirrite:osmId "trunk" ;
    rdfs:subClassOf piirrite:OsmEntity ;
    skos:definition "An important road that is not a motorway. osmcarto-rendering=File:Rendering-highway trunk carto.png osmcarto-rendering-size=125px"@en ;
    skos:inScheme piirritev:Highway ;
    skos:prefLabel "Trunk"@en .

piirritev:HighwayTrunkLink a skos:Concept ;
    piirrite:hasRelatedOsmTag piirrite:hasTrunkLinkOneway,
        piirrite:hasTrunkLinkRef ;
    piirrite:osmId "trunk_link" ;
    rdfs:subClassOf piirrite:OsmEntity ;
    skos:definition "The link road (sliproad / ramp) leading to and from a trunk highway. osmcarto-rendering=File:Rendering-highway trunk link.png osmcarto-rendering-size=125px"@en ;
    skos:inScheme piirritev:Highway ;
    skos:prefLabel "Trunk link"@en .

piirritev:HighwayTurningCircle a skos:Concept ;
    piirrite:hasRelatedOsmTag piirrite:hasTurningCircleDiameter,
        piirrite:hasTurningCircleName ;
    piirrite:osmId "turning_circle" ;
    rdfs:subClassOf piirrite:OsmEntity ;
    skos:definition "A widened area of road that allows vehicles to turn more easily. osmcarto-rendering=File:Mapping-Features-Turning-Circle.png osmcarto-rendering-size=100px"@en ;
    skos:inScheme piirritev:Highway ;
    skos:prefLabel "Turning circle"@en .

piirritev:HighwayTurningLoop a skos:Concept ;
    piirrite:osmId "turning_loop" ;
    rdfs:subClassOf piirrite:OsmEntity ;
    skos:definition "A widened area of a highway with a non-traversable island for turning around, often circular and at the end of a road."@en ;
    skos:inScheme piirritev:Highway ;
    skos:prefLabel "Turning loop"@en .

piirritev:HighwayUnclassified a skos:Concept ;
    piirrite:hasRelatedOsmTag piirrite:hasUnclassifiedAbutters,
        piirrite:hasUnclassifiedLanes,
        piirrite:hasUnclassifiedLit,
        piirrite:hasUnclassifiedName,
        piirrite:hasUnclassifiedOneway,
        piirrite:hasUnclassifiedSidewalk,
        piirrite:hasUnclassifiedSurface ;
    piirrite:osmId "unclassified" ;
    rdfs:subClassOf piirrite:OsmEntity ;
    skos:definition "Public access road, non-residential. osmcarto-rendering=File:Rendering-highway unclassified.png osmcarto-rendering-size=125px"@en ;
    skos:inScheme piirritev:Highway ;
    skos:prefLabel "Unclassified"@en .

piirritev:Hiking a skos:ConceptScheme ;
    piirrite:osmId "hiking" ;
    skos:definition "Information for hikers here."@en ;
    skos:prefLabel "Hiking, types"@en .

piirritev:Horse a skos:ConceptScheme ;
    piirrite:osmId "horse" ;
    skos:definition "Access permission for equestrians."@en ;
    skos:prefLabel "Horse, types"@en .

piirritev:HouseBungalow a skos:Concept ;
    piirrite:osmId "bungalow" ;
    rdfs:subClassOf piirrite:OsmEntity ;
    skos:definition "Simple single-storey house, sometimes with a second storey built into a sloped roof."@en ;
    skos:inScheme piirritev:House ;
    skos:prefLabel "Bungalow"@en .

piirritev:HouseDetached a skos:Concept ;
    piirrite:osmId "detached" ;
    rdfs:subClassOf piirrite:OsmEntity ;
    skos:definition "A detached house is a freestanding residential building usually housing a single family."@en ;
    skos:inScheme piirritev:House ;
    skos:prefLabel "Detached"@en .

piirritev:HouseResidential a skos:Concept ;
    piirrite:osmId "residential" ;
    rdfs:subClassOf piirrite:OsmEntity ;
    skos:definition ""@en ;
    skos:inScheme piirritev:House ;
    skos:prefLabel "Residential"@en .

piirritev:HouseSemi-Detached a skos:Concept ;
    piirrite:osmId "semi-detached" ;
    rdfs:subClassOf piirrite:OsmEntity ;
    skos:definition "A house that is attached to another house on one side."@en ;
    skos:inScheme piirritev:House ;
    skos:prefLabel "Semi-detached"@en .

piirritev:HouseTerrace a skos:Concept ;
    piirrite:hasRelatedOsmTag piirrite:hasTerraceBuilding ;
    piirrite:osmId "terrace" ;
    rdfs:subClassOf piirrite:OsmEntity ;
    skos:definition "Used in addition to tag:building=house on the outline of a linear row of residential dwellings, each of which normally has its own entrance, which form a terrace (\"row-house\" or \"townhouse\" in North American English)."@en ;
    skos:inScheme piirritev:House ;
    skos:prefLabel "Terrace"@en .

piirritev:HouseTerraced a skos:Concept ;
    piirrite:osmId "terraced" ;
    rdfs:subClassOf piirrite:OsmEntity ;
    skos:definition "Used in addition to tag:building=house to map the individual units in a terrace. Preferred over mapping the whole terrace as one building."@en ;
    skos:inScheme piirritev:House ;
    skos:prefLabel "Terraced"@en .

piirritev:Image a skos:ConceptScheme ;
    piirrite:osmId "image" ;
    skos:definition "Reference to an image of the object."@en ;
    skos:prefLabel "Image, types"@en .

piirritev:ImportBudovy201004 a skos:Concept ;
    piirrite:osmId "budovy201004" ;
    rdfs:subClassOf piirrite:OsmEntity ;
    skos:definition ""@en ;
    skos:inScheme piirritev:Import ;
    skos:prefLabel "Budovy201004"@en .

piirritev:ImportBudovy201004Drev a skos:Concept ;
    piirrite:osmId "budovy201004drev" ;
    rdfs:subClassOf piirrite:OsmEntity ;
    skos:definition ""@en ;
    skos:inScheme piirritev:Import ;
    skos:prefLabel "Budovy201004drev"@en .

piirritev:ImportFreemapkapor a skos:Concept ;
    piirrite:osmId "freemapkapor" ;
    rdfs:subClassOf piirrite:OsmEntity ;
    skos:definition ""@en ;
    skos:inScheme piirritev:Import ;
    skos:prefLabel "Freemapkapor"@en .

piirritev:ImportGrabremote a skos:Concept ;
    piirrite:osmId "grabremote" ;
    rdfs:subClassOf piirrite:OsmEntity ;
    skos:definition ""@en ;
    skos:inScheme piirritev:Import ;
    skos:prefLabel "Grabremote"@en .

piirritev:Incline a skos:ConceptScheme ;
    piirrite:osmId "incline" ;
    skos:definition "Incline steepness"@en ;
    skos:prefLabel "Incline, types"@en .

piirritev:IndoorArea a skos:Concept ;
    piirrite:hasRelatedOsmTag piirrite:hasAreaAccess,
        piirrite:hasAreaName,
        piirrite:hasAreaRef,
        piirrite:hasAreaWheelchair ;
    piirrite:osmId "area" ;
    rdfs:subClassOf piirrite:OsmEntity ;
    skos:definition "An indoor area without walls along at least some of its edges."@en ;
    skos:inScheme piirritev:Indoor ;
    skos:prefLabel "Area"@en .

piirritev:IndoorColumn a skos:Concept ;
    piirrite:hasRelatedOsmTag piirrite:hasColumnLevel ;
    piirrite:osmId "column" ;
    rdfs:subClassOf piirrite:OsmEntity ;
    skos:definition "A column that is part of the structure of the building."@en ;
    skos:inScheme piirritev:Indoor ;
    skos:prefLabel "Column"@en .

piirritev:IndoorCorridor a skos:Concept ;
    piirrite:hasRelatedOsmTag piirrite:hasCorridorName,
        piirrite:hasCorridorRef ;
    piirrite:osmId "corridor" ;
    rdfs:subClassOf piirrite:OsmEntity ;
    skos:definition "Enclosed walkway area that connects rooms."@en ;
    skos:inScheme piirritev:Indoor ;
    skos:prefLabel "Corridor"@en .

piirritev:IndoorDoor a skos:Concept ;
    piirrite:hasRelatedOsmTag piirrite:hasDoorAccess,
        piirrite:hasDoorLevel,
        piirrite:hasDoorOpen,
        piirrite:hasDoorOpening,
        piirrite:hasDoorRef,
        piirrite:hasDoorType,
        piirrite:hasDoorWheelchair ;
    piirrite:osmId "door" ;
    rdfs:subClassOf piirrite:OsmEntity ;
    skos:definition "A swinging or sliding barrier that closes off rooms within a building"@en ;
    skos:inScheme piirritev:Indoor ;
    skos:prefLabel "Door"@en .

piirritev:IndoorRoom a skos:Concept ;
    piirrite:hasRelatedOsmTag piirrite:hasRoomAccess,
        piirrite:hasRoomName,
        piirrite:hasRoomRef,
        piirrite:hasRoomType,
        piirrite:hasRoomWheelchair ;
    piirrite:osmId "room" ;
    rdfs:subClassOf piirrite:OsmEntity ;
    skos:definition "Conventional room with walls"@en ;
    skos:inScheme piirritev:Indoor ;
    skos:prefLabel "Room"@en .

piirritev:IndoorSeating a skos:ConceptScheme ;
    piirrite:osmId "indoor_seating" ;
    skos:definition "To indicate if a restaurant offers indoor seating."@en ;
    skos:prefLabel "Indoor seating, types"@en .

piirritev:IndoorWall a skos:Concept ;
    piirrite:osmId "wall" ;
    rdfs:subClassOf piirrite:OsmEntity ;
    skos:definition "Individual (non-passable) wall element"@en ;
    skos:inScheme piirritev:Indoor ;
    skos:prefLabel "Wall"@en .

piirritev:Industrial a skos:ConceptScheme ;
    piirrite:osmId "industrial" ;
    skos:definition "Type of industry or type of industrial object."@en ;
    skos:prefLabel "Industrial, types"@en .

piirritev:Informal a skos:ConceptScheme ;
    piirrite:osmId "informal" ;
    skos:definition "Indicates whether the feature was intentionally planned or formally set up."@en ;
    skos:prefLabel "Informal, types"@en .

piirritev:InformationBoard a skos:Concept ;
    piirrite:hasRelatedOsmTag piirrite:hasBoardBoardType,
        piirrite:hasBoardName,
        piirrite:hasBoardNetwork ;
    piirrite:osmId "board" ;
    rdfs:subClassOf piirrite:OsmEntity ;
    skos:definition "An information board."@en ;
    skos:inScheme piirritev:Information ;
    skos:prefLabel "Board"@en .

piirritev:InformationGuidepost a skos:Concept ;
    piirrite:hasRelatedOsmTag piirrite:hasGuidepostEle,
        piirrite:hasGuidepostName,
        piirrite:hasGuidepostRef ;
    piirrite:osmId "guidepost" ;
    rdfs:subClassOf piirrite:OsmEntity ;
    skos:definition "Used to mark a guidepost/signpost osmcarto-rendering=File:Guidepost-14.svg osmcarto-rendering-size=24px"@en ;
    skos:inScheme piirritev:Information ;
    skos:prefLabel "Guidepost"@en .

piirritev:InformationMap a skos:Concept ;
    piirrite:hasRelatedOsmTag piirrite:hasMapBicycle,
        piirrite:hasMapHiking,
        piirrite:hasMapHorse,
        piirrite:hasMapMapSize,
        piirrite:hasMapMapSource,
        piirrite:hasMapMapType,
        piirrite:hasMapMtb,
        piirrite:hasMapSki,
        piirrite:hasMapTourism ;
    piirrite:osmId "map" ;
    rdfs:subClassOf piirrite:OsmEntity ;
    skos:definition "A board with a map. osmcarto-rendering=File:Map-14.svg osmcarto-rendering-size=28px"@en ;
    skos:inScheme piirritev:Information ;
    skos:prefLabel "Map"@en .

piirritev:InformationOffice a skos:Concept ;
    piirrite:hasRelatedOsmTag piirrite:hasOfficeName,
        piirrite:hasOfficeOpeningHours,
        piirrite:hasOfficeOperator,
        piirrite:hasOfficeWebsite,
        piirrite:hasOfficeWheelchair ;
    piirrite:osmId "office" ;
    rdfs:subClassOf piirrite:OsmEntity ;
    skos:definition "An office where you can get information about a town or region. osmcarto-rendering=File:Office-14.svg osmcarto-rendering-size=28px"@en ;
    skos:inScheme piirritev:Information ;
    skos:prefLabel "Office"@en .

piirritev:InformationRouteMarker a skos:Concept ;
    piirrite:osmId "route_marker" ;
    rdfs:subClassOf piirrite:OsmEntity ;
    skos:definition "A marker that shows the position of the way of a route. Could be a symbol, a short pole or a painted marking."@en ;
    skos:inScheme piirritev:Information ;
    skos:prefLabel "Route marker"@en .

piirritev:InformationTerminal a skos:Concept ;
    piirrite:hasRelatedOsmTag piirrite:hasTerminalSupport ;
    piirrite:osmId "terminal" ;
    rdfs:subClassOf piirrite:OsmEntity ;
    skos:definition "A information terminal osmcarto-rendering=File:Terminal-14.svg osmcarto-rendering-size=28px"@en ;
    skos:inScheme piirritev:Information ;
    skos:prefLabel "Terminal"@en .

piirritev:InformationTrailBlaze a skos:Concept ;
    piirrite:osmId "trail_blaze" ;
    rdfs:subClassOf piirrite:OsmEntity ;
    skos:definition "A marker that shows the position of the way of a route. Could be a symbol, a short pole or a painted marking."@en ;
    skos:inScheme piirritev:Information ;
    skos:prefLabel "Trail blaze"@en .

piirritev:Inscription a skos:ConceptScheme ;
    piirrite:osmId "inscription" ;
    skos:definition "Text which is written on an object."@en ;
    skos:prefLabel "Inscription, types"@en .

piirritev:IntName a skos:ConceptScheme ;
    piirrite:osmId "int_name" ;
    skos:definition ""@en ;
    skos:prefLabel "Int name, types"@en .

piirritev:IntRefAh1 a skos:Concept ;
    piirrite:osmId "AH1" ;
    rdfs:subClassOf piirrite:OsmEntity ;
    skos:definition ""@en ;
    skos:inScheme piirritev:IntRef ;
    skos:prefLabel "Ah1"@en .

piirritev:IntRefAh2 a skos:Concept ;
    piirrite:osmId "AH2" ;
    rdfs:subClassOf piirrite:OsmEntity ;
    skos:definition ""@en ;
    skos:inScheme piirritev:IntRef ;
    skos:prefLabel "Ah2"@en .

piirritev:IntRefE22 a skos:Concept ;
    piirrite:osmId "E_22" ;
    rdfs:subClassOf piirrite:OsmEntity ;
    skos:definition ""@en ;
    skos:inScheme piirritev:IntRef ;
    skos:prefLabel "E 22"@en .

piirritev:IntRefE30 a skos:Concept ;
    piirrite:osmId "E_30" ;
    rdfs:subClassOf piirrite:OsmEntity ;
    skos:definition ""@en ;
    skos:inScheme piirritev:IntRef ;
    skos:prefLabel "E 30"@en .

piirritev:IntRefE40 a skos:Concept ;
    piirrite:osmId "E_40" ;
    rdfs:subClassOf piirrite:OsmEntity ;
    skos:definition ""@en ;
    skos:inScheme piirritev:IntRef ;
    skos:prefLabel "E 40"@en .

piirritev:IntRefE45 a skos:Concept ;
    piirrite:osmId "E_45" ;
    rdfs:subClassOf piirrite:OsmEntity ;
    skos:definition ""@en ;
    skos:inScheme piirritev:IntRef ;
    skos:prefLabel "E 45"@en .

piirritev:IntRefE70 a skos:Concept ;
    piirrite:osmId "E_70" ;
    rdfs:subClassOf piirrite:OsmEntity ;
    skos:definition ""@en ;
    skos:inScheme piirritev:IntRef ;
    skos:prefLabel "E 70"@en .

piirritev:IntRefE75 a skos:Concept ;
    piirrite:osmId "E_75" ;
    rdfs:subClassOf piirrite:OsmEntity ;
    skos:definition ""@en ;
    skos:inScheme piirritev:IntRef ;
    skos:prefLabel "E 75"@en .

piirritev:Intermittent a skos:ConceptScheme ;
    piirrite:osmId "intermittent" ;
    skos:definition "Used to indicate whether or not a waterway or water body does not permanently contain water. osmcarto-rendering-way=File:Rendering-waterway_river_intermittent.png osmcarto-rendering-way-size=100px osmcarto-rendering-area=File:Water_intermittent_100.png osmcarto-rendering-area-size=100px"@en ;
    skos:prefLabel "Intermittent, types"@en .

piirritev:InternetAccessWlan a skos:Concept ;
    piirrite:hasRelatedOsmTag piirrite:hasWlanInternetAccess ;
    piirrite:osmId "wlan" ;
    rdfs:subClassOf piirrite:OsmEntity ;
    skos:definition "Specifies that a feature offers a WLAN wireless internet Hotspot (Wi-Fi)"@en ;
    skos:inScheme piirritev:InternetAccess ;
    skos:prefLabel "Wlan"@en .

piirritev:JunctionCircular a skos:Concept ;
    piirrite:osmId "circular" ;
    rdfs:subClassOf piirrite:OsmEntity ;
    skos:definition "A road junction where the traffic goes around a non-traversable island but does not always have right of way."@en ;
    skos:inScheme piirritev:Junction ;
    skos:prefLabel "Circular"@en .

piirritev:JunctionRoundabout a skos:Concept ;
    piirrite:hasRelatedOsmTag piirrite:hasRoundaboutHighway ;
    piirrite:osmId "roundabout" ;
    rdfs:subClassOf piirrite:OsmEntity ;
    skos:definition "A road junction where the traffic goes around a non-traversable island and has right of way."@en ;
    skos:inScheme piirritev:Junction ;
    skos:prefLabel "Roundabout"@en .

piirritev:Kerb a skos:ConceptScheme ;
    piirrite:osmId "kerb" ;
    skos:definition "Used to indicate height and thus accessibility of a kerb."@en ;
    skos:prefLabel "Kerb, types"@en .

piirritev:LampMountAngledMast a skos:Concept ;
    piirrite:osmId "angled_mast" ;
    rdfs:subClassOf piirrite:OsmEntity ;
    skos:definition ""@en ;
    skos:inScheme piirritev:LampMount ;
    skos:prefLabel "Angled mast"@en .

piirritev:LampMountBentMast a skos:Concept ;
    piirrite:osmId "bent_mast" ;
    rdfs:subClassOf piirrite:OsmEntity ;
    skos:definition ""@en ;
    skos:inScheme piirritev:LampMount ;
    skos:prefLabel "Bent mast"@en .

piirritev:LampMountHighMast a skos:Concept ;
    piirrite:osmId "high_mast" ;
    rdfs:subClassOf piirrite:OsmEntity ;
    skos:definition ""@en ;
    skos:inScheme piirritev:LampMount ;
    skos:prefLabel "High mast"@en .

piirritev:LampMountPole a skos:Concept ;
    piirrite:osmId "pole" ;
    rdfs:subClassOf piirrite:OsmEntity ;
    skos:definition ""@en ;
    skos:inScheme piirritev:LampMount ;
    skos:prefLabel "Pole"@en .

piirritev:LampMountStraightMast a skos:Concept ;
    piirrite:osmId "straight_mast" ;
    rdfs:subClassOf piirrite:OsmEntity ;
    skos:definition ""@en ;
    skos:inScheme piirritev:LampMount ;
    skos:prefLabel "Straight mast"@en .

piirritev:LampMountWall a skos:Concept ;
    piirrite:osmId "wall" ;
    rdfs:subClassOf piirrite:OsmEntity ;
    skos:definition ""@en ;
    skos:inScheme piirritev:LampMount ;
    skos:prefLabel "Wall"@en .

piirritev:LampTypeElectric a skos:Concept ;
    piirrite:osmId "electric" ;
    rdfs:subClassOf piirrite:OsmEntity ;
    skos:definition ""@en ;
    skos:inScheme piirritev:LampType ;
    skos:prefLabel "Electric"@en .

piirritev:LampTypeFluorescent a skos:Concept ;
    piirrite:osmId "fluorescent" ;
    rdfs:subClassOf piirrite:OsmEntity ;
    skos:definition ""@en ;
    skos:inScheme piirritev:LampType ;
    skos:prefLabel "Fluorescent"@en .

piirritev:LampTypeGaslight a skos:Concept ;
    piirrite:osmId "gaslight" ;
    rdfs:subClassOf piirrite:OsmEntity ;
    skos:definition ""@en ;
    skos:inScheme piirritev:LampType ;
    skos:prefLabel "Gaslight"@en .

piirritev:LampTypeLed a skos:Concept ;
    piirrite:osmId "LED",
        "led" ;
    rdfs:subClassOf piirrite:OsmEntity ;
    skos:definition ""@en ;
    skos:inScheme piirritev:LampType ;
    skos:prefLabel "Led"@en .

piirritev:LampTypeMetal-Halogenide a skos:Concept ;
    piirrite:osmId "metal-halogenide" ;
    rdfs:subClassOf piirrite:OsmEntity ;
    skos:definition ""@en ;
    skos:inScheme piirritev:LampType ;
    skos:prefLabel "Metal-halogenide"@en .

piirritev:LampTypeSodium a skos:Concept ;
    piirrite:osmId "sodium" ;
    rdfs:subClassOf piirrite:OsmEntity ;
    skos:definition ""@en ;
    skos:inScheme piirritev:LampType ;
    skos:prefLabel "Sodium"@en .

piirritev:LandcoverGrass a skos:Concept ;
    piirrite:osmId "grass" ;
    rdfs:subClassOf piirrite:OsmEntity ;
    skos:definition "An area covered with grass."@en ;
    skos:inScheme piirritev:Landcover ;
    skos:prefLabel "Grass"@en .

piirritev:LandcoverMostlyRock a skos:Concept ;
    piirrite:osmId "mostly_rock" ;
    rdfs:subClassOf piirrite:OsmEntity ;
    skos:definition "Indicates that a land is physically covered with rocks."@en ;
    skos:inScheme piirritev:Landcover ;
    skos:prefLabel "Mostly rock"@en .

piirritev:LandcoverScrub a skos:Concept ;
    piirrite:osmId "scrub" ;
    rdfs:subClassOf piirrite:OsmEntity ;
    skos:definition ""@en ;
    skos:inScheme piirritev:Landcover ;
    skos:prefLabel "Scrub"@en .

piirritev:LandcoverTrees a skos:Concept ;
    piirrite:osmId "trees" ;
    rdfs:subClassOf piirrite:OsmEntity ;
    skos:definition "An area covered with trees."@en ;
    skos:inScheme piirritev:Landcover ;
    skos:prefLabel "Trees"@en .

piirritev:LanduseAllotments a skos:Concept ;
    piirrite:hasRelatedOsmTag piirrite:hasAllotmentsName,
        piirrite:hasAllotmentsOperator ;
    piirrite:osmId "allotments" ;
    rdfs:subClassOf piirrite:OsmEntity ;
    skos:definition "allotment gardens with multiple land parcels assigned to individuals or families for gardening. osmcarto-rendering=File:Landuse-allotments.png osmcarto-rendering-size=125px onNode=no onWay=no onArea=yes onRelation=no seeAlso = * landuse=farmland * leisure=garden combination= * name * operator status=de facto"@en ;
    skos:inScheme piirritev:Landuse ;
    skos:prefLabel "Allotments"@en .

piirritev:LanduseAnimalKeeping a skos:Concept ;
    piirrite:hasRelatedOsmTag piirrite:hasAnimalKeepingBarrier,
        piirrite:hasAnimalKeepingType ;
    piirrite:osmId "animal_keeping" ;
    rdfs:subClassOf piirrite:OsmEntity ;
    skos:definition "An area of land that is used to keep animals"@en ;
    skos:inScheme piirritev:Landuse ;
    skos:prefLabel "Animal keeping"@en .

piirritev:LanduseAquaculture a skos:Concept ;
    piirrite:hasRelatedOsmTag piirrite:hasAquacultureNatural,
        piirrite:hasAquacultureType ;
    piirrite:osmId "aquaculture" ;
    rdfs:subClassOf piirrite:OsmEntity ;
    skos:definition "An area on land or water that is used to farm aquatic organisms."@en ;
    skos:inScheme piirritev:Landuse ;
    skos:prefLabel "Aquaculture"@en .

piirritev:LanduseBasin a skos:Concept ;
    piirrite:hasRelatedOsmTag piirrite:hasBasinIntermittent,
        piirrite:hasBasinName,
        piirrite:hasBasinType ;
    piirrite:osmId "basin" ;
    rdfs:subClassOf piirrite:OsmEntity ;
    skos:definition "An area of land artificially graded to hold water. Includes also structures typically without water."@en ;
    skos:inScheme piirritev:Landuse ;
    skos:prefLabel "Basin"@en .

piirritev:LanduseBrownfield a skos:Concept ;
    piirrite:osmId "brownfield" ;
    rdfs:subClassOf piirrite:OsmEntity ;
    skos:definition "Land which was developed which is no longer in use. osmcarto-rendering=File:Rendering-landuse-construction-mapnik.png osmcarto-rendering-size=100px"@en ;
    skos:inScheme piirritev:Landuse ;
    skos:prefLabel "Brownfield"@en .

piirritev:LanduseCemetery a skos:Concept ;
    piirrite:hasRelatedOsmTag piirrite:hasCemeteryName,
        piirrite:hasCemeteryReligion ;
    piirrite:osmId "cemetery" ;
    rdfs:subClassOf piirrite:OsmEntity ;
    skos:definition "A place where people, or sometimes animals are buried that isn't part of a place of worship osmcarto-rendering=File:Landuse-cemetery.png osmcarto-rendering-size=125px"@en ;
    skos:inScheme piirritev:Landuse ;
    skos:prefLabel "Cemetery"@en .

piirritev:LanduseCommercial a skos:Concept ;
    piirrite:hasRelatedOsmTag piirrite:hasCommercialName ;
    piirrite:osmId "commercial" ;
    rdfs:subClassOf piirrite:OsmEntity ;
    skos:definition "A commercial zone, predominantly offices or services.  osmcarto-rendering=File:Landuse-commercial.png  osmcarto-rendering-size=100px"@en ;
    skos:inScheme piirritev:Landuse ;
    skos:prefLabel "Commercial"@en .

piirritev:LanduseConstruction a skos:Concept ;
    piirrite:hasRelatedOsmTag piirrite:hasConstructionCheckDate,
        piirrite:hasConstructionName,
        piirrite:hasConstructionType ;
    piirrite:osmId "construction" ;
    rdfs:subClassOf piirrite:OsmEntity ;
    skos:definition "An area being built on. osmcarto-rendering=File:Rendering-landuse-construction-mapnik.png osmcarto-rendering-size=100px"@en ;
    skos:inScheme piirritev:Landuse ;
    skos:prefLabel "Construction"@en .

piirritev:LanduseEducation a skos:Concept ;
    piirrite:hasRelatedOsmTag piirrite:hasEducationAmenity ;
    piirrite:osmId "education" ;
    rdfs:subClassOf piirrite:OsmEntity ;
    skos:definition "An area used by educational facilities."@en ;
    skos:inScheme piirritev:Landuse ;
    skos:prefLabel "Education"@en .

piirritev:LanduseFarmland a skos:Concept ;
    piirrite:hasRelatedOsmTag piirrite:hasFarmlandBarrier,
        piirrite:hasFarmlandCrop,
        piirrite:hasFarmlandName ;
    piirrite:osmId "farmland" ;
    rdfs:subClassOf piirrite:OsmEntity ;
    skos:definition "Area of farmland used mainly for tillage (annual crops). osmcarto-rendering=File:Rendering-landuse-farm-mapnik.png osmcarto-rendering-size=125px"@en ;
    skos:inScheme piirritev:Landuse ;
    skos:prefLabel "Farmland"@en .

piirritev:LanduseFarmyard a skos:Concept ;
    piirrite:hasRelatedOsmTag piirrite:hasFarmyardName,
        piirrite:hasFarmyardOperator,
        piirrite:hasFarmyardType ;
    piirrite:osmId "farmyard" ;
    rdfs:subClassOf piirrite:OsmEntity ;
    skos:definition "Area of land with farm buildings (farmhouse, sheds, stables, barns, etc.). osmcarto-rendering=File:Rendering-area-landuse farmyard-mapnik.png osmcarto-rendering-size=125px"@en ;
    skos:inScheme piirritev:Landuse ;
    skos:prefLabel "Farmyard"@en .

piirritev:LanduseFlowerbed a skos:Concept ;
    piirrite:hasRelatedOsmTag piirrite:hasFlowerbedGenus,
        piirrite:hasFlowerbedOperator,
        piirrite:hasFlowerbedSpecies,
        piirrite:hasFlowerbedSurface,
        piirrite:hasFlowerbedTaxon ;
    piirrite:osmId "flowerbed" ;
    rdfs:subClassOf piirrite:OsmEntity ;
    skos:definition "An area designated for flowers.  osmcarto-rendering = File:Landuse-flowerbed.png  osmcarto-rendering-size = 125px"@en ;
    skos:inScheme piirritev:Landuse ;
    skos:prefLabel "Flowerbed"@en .

piirritev:LanduseGarages a skos:Concept ;
    piirrite:hasRelatedOsmTag piirrite:hasGaragesBuilding,
        piirrite:hasGaragesHighway ;
    piirrite:osmId "garages" ;
    rdfs:subClassOf piirrite:OsmEntity ;
    skos:definition "An area occupied by multiple private garage buildings. osmcarto-rendering=File:Rendering-area-landuse garages-mapnik.png osmcarto-rendering-size=100px"@en ;
    skos:inScheme piirritev:Landuse ;
    skos:prefLabel "Garages"@en .

piirritev:LanduseGrass a skos:Concept ;
    piirrite:osmId "grass" ;
    rdfs:subClassOf piirrite:OsmEntity ;
    skos:definition "A smaller area of grass, usually mown and managed. osmcarto-rendering=File:Landuse grass.png osmcarto-rendering-size=125px"@en ;
    skos:inScheme piirritev:Landuse ;
    skos:prefLabel "Grass"@en .

piirritev:LanduseGreenery a skos:Concept ;
    piirrite:hasRelatedOsmTag piirrite:hasGreeneryBarrier,
        piirrite:hasGreeneryLanduse,
        piirrite:hasGreeneryLeisure,
        piirrite:hasGreeneryNatural ;
    piirrite:osmId "greenery" ;
    rdfs:subClassOf piirrite:OsmEntity ;
    skos:definition "An area covered in unspecified or various types of decorative vegetation. Consider using a more specific tag instead"@en ;
    skos:inScheme piirritev:Landuse ;
    skos:prefLabel "Greenery"@en .

piirritev:LanduseGreenfield a skos:Concept ;
    piirrite:hasRelatedOsmTag piirrite:hasGreenfieldLanduse ;
    piirrite:osmId "greenfield" ;
    rdfs:subClassOf piirrite:OsmEntity ;
    skos:definition "Undeveloped land scheduled to turn into a construction site"@en ;
    skos:inScheme piirritev:Landuse ;
    skos:prefLabel "Greenfield"@en .

piirritev:LanduseGreenhouseHorticulture a skos:Concept ;
    piirrite:hasRelatedOsmTag piirrite:hasGreenhouseHorticultureCrop ;
    piirrite:osmId "greenhouse_horticulture" ;
    rdfs:subClassOf piirrite:OsmEntity ;
    skos:definition "Land area used for growing plants in greenhouses. osmcarto-rendering=File:Rendering-landuse-farm-mapnik.png osmcarto-rendering-size=125px"@en ;
    skos:inScheme piirritev:Landuse ;
    skos:prefLabel "Greenhouse horticulture"@en .

piirritev:LanduseHighway a skos:Concept ;
    piirrite:osmId "highway" ;
    rdfs:subClassOf piirrite:OsmEntity ;
    skos:definition "A land used for a highway, including all auxiliary areas like associated footways and verges, ditches, etc."@en ;
    skos:inScheme piirritev:Landuse ;
    skos:prefLabel "Highway"@en .

piirritev:LanduseIndustrial a skos:Concept ;
    piirrite:hasRelatedOsmTag piirrite:hasIndustrialLanduse,
        piirrite:hasIndustrialManMade,
        piirrite:hasIndustrialName,
        piirrite:hasIndustrialPipeline,
        piirrite:hasIndustrialPower,
        piirrite:hasIndustrialType,
        piirrite:hasIndustrialUtility ;
    piirrite:osmId "industrial" ;
    rdfs:subClassOf piirrite:OsmEntity ;
    skos:definition "An area with predominantly workshops, factories or warehouses. osmcarto-rendering=File:Landuse-industrial.png osmcarto-rendering-size=100px"@en ;
    skos:inScheme piirritev:Landuse ;
    skos:prefLabel "Industrial"@en .

piirritev:LanduseLandfill a skos:Concept ;
    piirrite:hasRelatedOsmTag piirrite:hasLandfillInformal,
        piirrite:hasLandfillName,
        piirrite:hasLandfillOperator ;
    piirrite:osmId "landfill" ;
    rdfs:subClassOf piirrite:OsmEntity ;
    skos:definition "A site for permanent or long term storage of waste materials. osmcarto-rendering=File:Rendering-landuse-landfill-mapnik.png osmcarto-rendering-size=100px"@en ;
    skos:inScheme piirritev:Landuse ;
    skos:prefLabel "Landfill"@en .

piirritev:LanduseLogging a skos:Concept ;
    piirrite:hasRelatedOsmTag piirrite:hasLoggingLanduse,
        piirrite:hasLoggingNatural ;
    piirrite:osmId "logging" ;
    rdfs:subClassOf piirrite:OsmEntity ;
    skos:definition "An area where some or all trees have been cut down."@en ;
    skos:inScheme piirritev:Landuse ;
    skos:prefLabel "Logging"@en .

piirritev:LanduseMeadow a skos:Concept ;
    piirrite:hasRelatedOsmTag piirrite:hasMeadowCrop,
        piirrite:hasMeadowName,
        piirrite:hasMeadowType ;
    piirrite:osmId "meadow" ;
    rdfs:subClassOf piirrite:OsmEntity ;
    skos:definition "An area of meadow or pasture: land primarily vegetated by grass and other non-woody plants, mainly used for hay or grazing. osmcarto-rendering=File:Landuse Meadow.png osmcarto-rendering-size=125px"@en ;
    skos:inScheme piirritev:Landuse ;
    skos:prefLabel "Meadow"@en .

piirritev:LanduseMilitary a skos:Concept ;
    piirrite:hasRelatedOsmTag piirrite:hasMilitaryMilitaryService,
        piirrite:hasMilitaryType ;
    piirrite:osmId "military" ;
    rdfs:subClassOf piirrite:OsmEntity ;
    skos:definition "Area used for military purposes. osmcarto-rendering=File:Landuse-military 100.png osmcarto-rendering-size=100px"@en ;
    skos:inScheme piirritev:Landuse ;
    skos:prefLabel "Military"@en .

piirritev:LanduseOrchard a skos:Concept ;
    piirrite:hasRelatedOsmTag piirrite:hasOrchardCrop,
        piirrite:hasOrchardProduce,
        piirrite:hasOrchardSelfHarvesting,
        piirrite:hasOrchardTrees,
        piirrite:hasOrchardType ;
    piirrite:osmId "orchard" ;
    rdfs:subClassOf piirrite:OsmEntity ;
    skos:definition "Used to mark intentional planting of trees or shrubs maintained for food production"@en ;
    skos:inScheme piirritev:Landuse ;
    skos:prefLabel "Orchard"@en .

piirritev:LandusePlantNursery a skos:Concept ;
    piirrite:hasRelatedOsmTag piirrite:hasPlantNurseryGenus,
        piirrite:hasPlantNurseryName,
        piirrite:hasPlantNurseryOperator,
        piirrite:hasPlantNurseryPlant,
        piirrite:hasPlantNurserySpecies ;
    piirrite:osmId "plant_nursery" ;
    rdfs:subClassOf piirrite:OsmEntity ;
    skos:definition "Represents land that is used solely for plant nurseries, which grow live plants."@en ;
    skos:inScheme piirritev:Landuse ;
    skos:prefLabel "Plant nursery"@en .

piirritev:LanduseQuarry a skos:Concept ;
    piirrite:hasRelatedOsmTag piirrite:hasQuarryName,
        piirrite:hasQuarryOperator,
        piirrite:hasQuarryResource ;
    piirrite:osmId "quarry" ;
    rdfs:subClassOf piirrite:OsmEntity ;
    skos:definition "An area of land used for surface extraction (open-pit mining). osmcarto-rendering=File:Rendering-landuse-quarry-mapnik.png osmcarto-rendering-size=125px"@en ;
    skos:inScheme piirritev:Landuse ;
    skos:prefLabel "Quarry"@en .

piirritev:LanduseRailway a skos:Concept ;
    piirrite:hasRelatedOsmTag piirrite:hasRailwayName ;
    piirrite:osmId "railway" ;
    rdfs:subClassOf piirrite:OsmEntity ;
    skos:definition "An area of land dedicated to train operation or support, including areas around tracks, rail corridors, yards, sidings, station complexes, and ancillary man-made objects along the tracks."@en ;
    skos:inScheme piirritev:Landuse ;
    skos:prefLabel "Railway"@en .

piirritev:LanduseRecreationGround a skos:Concept ;
    piirrite:hasRelatedOsmTag piirrite:hasRecreationGroundName ;
    piirrite:osmId "recreation_ground" ;
    rdfs:subClassOf piirrite:OsmEntity ;
    skos:definition "An open green space for general recreation, which often includes formal or informal pitches, nets and so on. Often municipally owned, sometimes part of colleges / companies or commercially operated. osmcarto-rendering=File:Landuse-recreation ground.png osmcarto-rendering-size=125px"@en ;
    skos:inScheme piirritev:Landuse ;
    skos:prefLabel "Recreation ground"@en .

piirritev:LanduseReligious a skos:Concept ;
    piirrite:hasRelatedOsmTag piirrite:hasReligiousBarrier,
        piirrite:hasReligiousReligion ;
    piirrite:osmId "religious" ;
    rdfs:subClassOf piirrite:OsmEntity ;
    skos:definition "An area used for religious purposes. osmcarto-rendering=File:Place of worship area.png osmcarto-rendering-size=125px"@en ;
    skos:inScheme piirritev:Landuse ;
    skos:prefLabel "Religious"@en .

piirritev:LanduseReservoir a skos:Concept ;
    piirrite:osmId "reservoir" ;
    rdfs:subClassOf piirrite:OsmEntity ;
    skos:definition "Using this tag is discouraged; use tag:natural=water + tag:water=reservoir instead. osmcarto-rendering=File:Base layer water.png osmcarto-rendering-size=100px"@en ;
    skos:inScheme piirritev:Landuse ;
    skos:prefLabel "Reservoir"@en .

piirritev:LanduseResidential a skos:Concept ;
    piirrite:hasRelatedOsmTag piirrite:hasResidentialType ;
    piirrite:osmId "residential" ;
    rdfs:subClassOf piirrite:OsmEntity ;
    skos:definition "A portion of land predominantly used for residential purposes.  osmcarto-rendering = File:Rendering-area-landuse-residential.png  osmcarto-rendering-size = 100px"@en ;
    skos:inScheme piirritev:Landuse ;
    skos:prefLabel "Residential"@en .

piirritev:LanduseRetail a skos:Concept ;
    piirrite:hasRelatedOsmTag piirrite:hasRetailName,
        piirrite:hasRetailOperator ;
    piirrite:osmId "retail" ;
    rdfs:subClassOf piirrite:OsmEntity ;
    skos:definition "An area that encloses predominantly shops. osmcarto-rendering=File:Landuse-retail.png osmcarto-rendering-size=100px"@en ;
    skos:inScheme piirritev:Landuse ;
    skos:prefLabel "Retail"@en .

piirritev:LanduseSaltPond a skos:Concept ;
    piirrite:hasRelatedOsmTag piirrite:hasSaltPondName,
        piirrite:hasSaltPondOperator ;
    piirrite:osmId "salt_pond" ;
    rdfs:subClassOf piirrite:OsmEntity ;
    skos:definition "A place where sea water is evaporated to extract its salt osmcarto-rendering=File:Rendering-landuse-salt-pond.png osmcarto-rendering-size=125px"@en ;
    skos:inScheme piirritev:Landuse ;
    skos:prefLabel "Salt pond"@en .

piirritev:LanduseStaticCaravan a skos:Concept ;
    piirrite:osmId "static_caravan" ;
    rdfs:subClassOf piirrite:OsmEntity ;
    skos:definition "A plot for static caravans."@en ;
    skos:inScheme piirritev:Landuse ;
    skos:prefLabel "Static caravan"@en .

piirritev:LanduseVillageGreen a skos:Concept ;
    piirrite:hasRelatedOsmTag piirrite:hasVillageGreenName ;
    piirrite:osmId "village_green" ;
    rdfs:subClassOf piirrite:OsmEntity ;
    skos:definition "A village green is a distinctive area of grassy public land in a village centre. Not a generic tag for urban greenery.  osmcarto-rendering = File:Landuse-village green.png  osmcarto-rendering-size = 125px"@en ;
    skos:inScheme piirritev:Landuse ;
    skos:prefLabel "Village green"@en .

piirritev:LanduseVineyard a skos:Concept ;
    piirrite:hasRelatedOsmTag piirrite:hasVineyardGrapeVariety,
        piirrite:hasVineyardName,
        piirrite:hasVineyardOrganic ;
    piirrite:osmId "vineyard" ;
    rdfs:subClassOf piirrite:OsmEntity ;
    skos:definition "Used to tag vineyards, a piece of land where grapes are grown.  osmcarto-rendering = File:Landuse-vineyard.png  osmcarto-rendering-size = 125px"@en ;
    skos:inScheme piirritev:Landuse ;
    skos:prefLabel "Vineyard"@en .

piirritev:LaneMarkings a skos:ConceptScheme ;
    piirrite:osmId "lane_markings" ;
    skos:definition "Specifies if a highway has painted markings to indicate the position of the lanes"@en ;
    skos:prefLabel "Lane markings, types"@en .

piirritev:Lanes a skos:ConceptScheme ;
    piirrite:osmId "lanes" ;
    skos:definition "Total number of traffic lanes available for motorised traffic."@en ;
    skos:prefLabel "Lanes, types"@en .

piirritev:Layer a skos:ConceptScheme ;
    piirrite:osmId "layer" ;
    skos:definition "Used to mark the vertical relationship between two intersecting features."@en ;
    skos:prefLabel "Layer, types"@en .

piirritev:LcnProposed a skos:Concept ;
    piirrite:osmId "proposed" ;
    rdfs:subClassOf piirrite:OsmEntity ;
    skos:definition ""@en ;
    skos:inScheme piirritev:Lcn ;
    skos:prefLabel "Proposed"@en .

piirritev:LeafCycleDeciduous a skos:Concept ;
    piirrite:osmId "deciduous" ;
    rdfs:subClassOf piirrite:OsmEntity ;
    skos:definition "Deciduous woody vegetation"@en ;
    skos:inScheme piirritev:LeafCycle ;
    skos:prefLabel "Deciduous"@en .

piirritev:LeafCycleEvergreen a skos:Concept ;
    piirrite:osmId "evergreen" ;
    rdfs:subClassOf piirrite:OsmEntity ;
    skos:definition "Evergreen woody vegetation"@en ;
    skos:inScheme piirritev:LeafCycle ;
    skos:prefLabel "Evergreen"@en .

piirritev:LeafCycleMixed a skos:Concept ;
    piirrite:osmId "mixed" ;
    rdfs:subClassOf piirrite:OsmEntity ;
    skos:definition "Habitat with evergreen and deciduous vegetation."@en ;
    skos:inScheme piirritev:LeafCycle ;
    skos:prefLabel "Mixed"@en .

piirritev:LeafCycleSemiDeciduous a skos:Concept ;
    piirrite:osmId "semi_deciduous" ;
    rdfs:subClassOf piirrite:OsmEntity ;
    skos:definition "Semi-deciduous woody vegetation"@en ;
    skos:inScheme piirritev:LeafCycle ;
    skos:prefLabel "Semi deciduous"@en .

piirritev:LeafCycleSemiEvergreen a skos:Concept ;
    piirrite:osmId "semi_evergreen" ;
    rdfs:subClassOf piirrite:OsmEntity ;
    skos:definition "Semi-evergreen woody vegetation"@en ;
    skos:inScheme piirritev:LeafCycle ;
    skos:prefLabel "Semi evergreen"@en .

piirritev:LeafTypeBroadleaved a skos:Concept ;
    piirrite:osmId "broadleaved" ;
    rdfs:subClassOf piirrite:OsmEntity ;
    skos:definition "Indicates that the trees or tree is broadleaved as opposed to needleleaved or leafless.  osmcarto-rendering=File:Leaftype_broadleaved_100.png  osmcarto-rendering-size=100px"@en ;
    skos:inScheme piirritev:LeafType ;
    skos:prefLabel "Broadleaved"@en .

piirritev:LeafTypeMixed a skos:Concept ;
    piirrite:osmId "mixed" ;
    rdfs:subClassOf piirrite:OsmEntity ;
    skos:definition "Habitat with broadleaved and needleleaved woody vegetation  osmcarto-rendering=File:Leaftype_mixed.png  osmcarto-rendering-size=125px"@en ;
    skos:inScheme piirritev:LeafType ;
    skos:prefLabel "Mixed"@en .

piirritev:LeafTypeNeedleleaved a skos:Concept ;
    piirrite:osmId "needleleaved" ;
    rdfs:subClassOf piirrite:OsmEntity ;
    skos:definition "Needleleaved woody vegetation  osmcarto-rendering=File:Leaftype_needleleaved.png  osmcarto-rendering-size=125px"@en ;
    skos:inScheme piirritev:LeafType ;
    skos:prefLabel "Needleleaved"@en .

piirritev:LeafTypePalm a skos:Concept ;
    piirrite:osmId "palm" ;
    rdfs:subClassOf piirrite:OsmEntity ;
    skos:definition "Used for palm-shaped trees."@en ;
    skos:inScheme piirritev:LeafType ;
    skos:prefLabel "Palm"@en .

piirritev:Length a skos:ConceptScheme ;
    piirrite:osmId "length" ;
    skos:definition "The length of a feature. Values are interpreted as meters by default."@en ;
    skos:prefLabel "Length, types"@en .

piirritev:Level a skos:ConceptScheme ;
    piirrite:osmId "level" ;
    skos:definition "Zero-based floor number of a feature (where 0 is the ground level and -1 is the basement)."@en ;
    skos:prefLabel "Level, types"@en .

piirritev:LightSource a skos:ConceptScheme ;
    piirrite:osmId "light_source" ;
    skos:definition ""@en ;
    skos:prefLabel "Light source, types"@en .

piirritev:LitAutomatic a skos:Concept ;
    piirrite:osmId "automatic" ;
    rdfs:subClassOf piirrite:OsmEntity ;
    skos:definition ""@en ;
    skos:inScheme piirritev:Lit ;
    skos:prefLabel "Automatic"@en .

piirritev:LivingStreet a skos:ConceptScheme ;
    piirrite:osmId "living_street" ;
    skos:definition "Used to mark that pedestrians are superior to vehicles as defined in road rules."@en ;
    skos:prefLabel "Living street, types"@en .

piirritev:LoadingGaugeTsiGa a skos:Concept ;
    piirrite:osmId "TSI_GA" ;
    rdfs:subClassOf piirrite:OsmEntity ;
    skos:definition ""@en ;
    skos:inScheme piirritev:LoadingGauge ;
    skos:prefLabel "Tsi ga"@en .

piirritev:LoadingGaugeTsiGb a skos:Concept ;
    piirrite:osmId "TSI_GB" ;
    rdfs:subClassOf piirrite:OsmEntity ;
    skos:definition ""@en ;
    skos:inScheme piirritev:LoadingGauge ;
    skos:prefLabel "Tsi gb"@en .

piirritev:LoadingGaugeTsiGb1 a skos:Concept ;
    piirrite:osmId "TSI_GB1" ;
    rdfs:subClassOf piirrite:OsmEntity ;
    skos:definition ""@en ;
    skos:inScheme piirritev:LoadingGauge ;
    skos:prefLabel "Tsi gb1"@en .

piirritev:LoadingGaugeTsiGc a skos:Concept ;
    piirrite:osmId "TSI_GC" ;
    rdfs:subClassOf piirrite:OsmEntity ;
    skos:definition ""@en ;
    skos:inScheme piirritev:LoadingGauge ;
    skos:prefLabel "Tsi gc"@en .

piirritev:LocName a skos:ConceptScheme ;
    piirrite:osmId "loc_name" ;
    skos:definition ""@en ;
    skos:prefLabel "Loc name, types"@en .

piirritev:LocRef a skos:ConceptScheme ;
    piirrite:osmId "loc_ref" ;
    skos:definition "Local reference number or code."@en ;
    skos:prefLabel "Loc ref, types"@en .

piirritev:LocalRefA a skos:Concept ;
    piirrite:osmId "A" ;
    rdfs:subClassOf piirrite:OsmEntity ;
    skos:definition ""@en ;
    skos:inScheme piirritev:LocalRef ;
    skos:prefLabel "A"@en .

piirritev:LocalRefB a skos:Concept ;
    piirrite:osmId "B" ;
    rdfs:subClassOf piirrite:OsmEntity ;
    skos:definition ""@en ;
    skos:inScheme piirritev:LocalRef ;
    skos:prefLabel "B"@en .

piirritev:LocationAboveground a skos:Concept ;
    piirrite:osmId "aboveground" ;
    rdfs:subClassOf piirrite:OsmEntity ;
    skos:definition ""@en ;
    skos:inScheme piirritev:Location ;
    skos:prefLabel "Aboveground"@en .

piirritev:LocationGround a skos:Concept ;
    piirrite:osmId "ground" ;
    rdfs:subClassOf piirrite:OsmEntity ;
    skos:definition ""@en ;
    skos:inScheme piirritev:Location ;
    skos:prefLabel "Ground"@en .

piirritev:LocationIndoor a skos:Concept ;
    piirrite:osmId "indoor" ;
    rdfs:subClassOf piirrite:OsmEntity ;
    skos:definition "Indicate a given feature is indoor"@en ;
    skos:inScheme piirritev:Location ;
    skos:prefLabel "Indoor"@en .

piirritev:LocationOutdoor a skos:Concept ;
    piirrite:osmId "outdoor" ;
    rdfs:subClassOf piirrite:OsmEntity ;
    skos:definition "Indicate a given feature is outdoor"@en ;
    skos:inScheme piirritev:Location ;
    skos:prefLabel "Outdoor"@en .

piirritev:LocationOverground a skos:Concept ;
    piirrite:osmId "overground" ;
    rdfs:subClassOf piirrite:OsmEntity ;
    skos:definition "Indicate a given feature is installed on the ground surface and can be touched"@en ;
    skos:inScheme piirritev:Location ;
    skos:prefLabel "Overground"@en .

piirritev:LocationOverhead a skos:Concept ;
    piirrite:osmId "overhead" ;
    rdfs:subClassOf piirrite:OsmEntity ;
    skos:definition "Indicate a given feature is installed over the ground at a height allowing persons or vehicles to pass underneath."@en ;
    skos:inScheme piirritev:Location ;
    skos:prefLabel "Overhead"@en .

piirritev:LocationPole a skos:Concept ;
    piirrite:osmId "pole" ;
    rdfs:subClassOf piirrite:OsmEntity ;
    skos:definition ""@en ;
    skos:inScheme piirritev:Location ;
    skos:prefLabel "Pole"@en .

piirritev:LocationRoof a skos:Concept ;
    piirrite:osmId "roof" ;
    rdfs:subClassOf piirrite:OsmEntity ;
    skos:definition "Indicates that a given feature is located on top of the roof."@en ;
    skos:inScheme piirritev:Location ;
    skos:prefLabel "Roof"@en .

piirritev:LocationSurface a skos:Concept ;
    piirrite:hasRelatedOsmTag piirrite:hasSurfaceBuilding ;
    piirrite:osmId "surface" ;
    rdfs:subClassOf piirrite:OsmEntity ;
    skos:definition "Feature is on the surface of the ground"@en ;
    skos:inScheme piirritev:Location ;
    skos:prefLabel "Surface"@en .

piirritev:LocationUnderground a skos:Concept ;
    piirrite:hasRelatedOsmTag piirrite:hasUndergroundManMade,
        piirrite:hasUndergroundPower,
        piirrite:hasUndergroundTunnel ;
    piirrite:osmId "underground" ;
    rdfs:subClassOf piirrite:OsmEntity ;
    skos:definition "Indicate a given feature is buried or dug under the surface of the ground."@en ;
    skos:inScheme piirritev:Location ;
    skos:prefLabel "Underground"@en .

piirritev:LocationUnderwater a skos:Concept ;
    piirrite:hasRelatedOsmTag piirrite:hasUnderwaterLocation ;
    piirrite:osmId "underwater" ;
    rdfs:subClassOf piirrite:OsmEntity ;
    skos:definition "Indicate a given feature is underwater."@en ;
    skos:inScheme piirritev:Location ;
    skos:prefLabel "Underwater"@en .

piirritev:Marker a skos:ConceptScheme ;
    piirrite:osmId "marker" ;
    skos:definition "Shape and function of a physical spot indicating underground utility infrastructure, highway milestones or private property limits"@en ;
    skos:prefLabel "Marker, types"@en .

piirritev:MaxheightBelowDefault a skos:Concept ;
    piirrite:osmId "below_default" ;
    rdfs:subClassOf piirrite:OsmEntity ;
    skos:definition ""@en ;
    skos:inScheme piirritev:Maxheight ;
    skos:prefLabel "Below default"@en .

piirritev:MaxheightDefault a skos:Concept ;
    piirrite:hasRelatedOsmTag piirrite:hasDefaultHighway ;
    piirrite:osmId "default" ;
    rdfs:subClassOf piirrite:OsmEntity ;
    skos:definition "No specific legal height limit (no sign), default height rules apply here"@en ;
    skos:inScheme piirritev:Maxheight ;
    skos:prefLabel "Default"@en .

piirritev:Maxspeed a skos:ConceptScheme ;
    piirrite:osmId "maxspeed" ;
    skos:definition "Specifies the maximum legal speed limit on a road, railway or waterway."@en ;
    skos:prefLabel "Maxspeed, types"@en .

piirritev:MinHeight a skos:ConceptScheme ;
    piirrite:osmId "min_height" ;
    skos:definition "Height of location of bottom part of building, part of building or another objects."@en ;
    skos:prefLabel "Min height, types"@en .

piirritev:Minspeed a skos:ConceptScheme ;
    piirrite:osmId "minspeed" ;
    skos:definition "Specifies the minimum speed limit on a road, railway or waterway. Note that may refer to minimum achievable speed by vehicle or to minimum movement speed at given moment."@en ;
    skos:prefLabel "Minspeed, types"@en .

piirritev:MopedDesignated a skos:Concept ;
    piirrite:osmId "designated" ;
    rdfs:subClassOf piirrite:OsmEntity ;
    skos:definition ""@en ;
    skos:inScheme piirritev:Moped ;
    skos:prefLabel "Designated"@en .

piirritev:MopedUseSidepath a skos:Concept ;
    piirrite:hasRelatedOsmTag piirrite:hasUseSidepathHighway ;
    piirrite:osmId "use_sidepath" ;
    rdfs:subClassOf piirrite:OsmEntity ;
    skos:definition "Use compulsory parallel way instead"@en ;
    skos:inScheme piirritev:Moped ;
    skos:prefLabel "Use sidepath"@en .

piirritev:Name a skos:ConceptScheme ;
    piirrite:osmId "name" ;
    skos:definition "The primary name: in general, the most prominent signposted name or the most common name in the local language(s)."@en ;
    skos:prefLabel "Name, types"@en .

piirritev:NavigationaidAls a skos:Concept ;
    piirrite:osmId "als" ;
    rdfs:subClassOf piirrite:OsmEntity ;
    skos:definition "Approach Lighting System"@en ;
    skos:inScheme piirritev:Navigationaid ;
    skos:prefLabel "Als"@en .

piirritev:NavigationaidRwc a skos:Concept ;
    piirrite:osmId "rwc" ;
    rdfs:subClassOf piirrite:OsmEntity ;
    skos:definition "Beaconing runway centerline"@en ;
    skos:inScheme piirritev:Navigationaid ;
    skos:prefLabel "Rwc"@en .

piirritev:NavigationaidRwe a skos:Concept ;
    piirrite:osmId "rwe" ;
    rdfs:subClassOf piirrite:OsmEntity ;
    skos:definition "Beaconing runway edge"@en ;
    skos:inScheme piirritev:Navigationaid ;
    skos:prefLabel "Rwe"@en .

piirritev:NavigationaidTdz a skos:Concept ;
    piirrite:osmId "tdz" ;
    rdfs:subClassOf piirrite:OsmEntity ;
    skos:definition "Touchdown zone lighting"@en ;
    skos:inScheme piirritev:Navigationaid ;
    skos:prefLabel "Tdz"@en .

piirritev:NavigationaidTxc a skos:Concept ;
    piirrite:osmId "txc" ;
    rdfs:subClassOf piirrite:OsmEntity ;
    skos:definition "Beaconing taxiway centreline"@en ;
    skos:inScheme piirritev:Navigationaid ;
    skos:prefLabel "Txc"@en .

piirritev:NavigationaidTxe a skos:Concept ;
    piirrite:osmId "txe" ;
    rdfs:subClassOf piirrite:OsmEntity ;
    skos:definition "Beaconing taxiway edge"@en ;
    skos:inScheme piirritev:Navigationaid ;
    skos:prefLabel "Txe"@en .

piirritev:Nhs a skos:ConceptScheme ;
    piirrite:osmId "NHS" ;
    skos:definition "Specifies, if the road is part of a National Highway System."@en ;
    skos:prefLabel "Nhs, types"@en .

piirritev:NoteA13-0603Xml a skos:Concept ;
    piirrite:osmId "A13-06_03_xml" ;
    rdfs:subClassOf piirrite:OsmEntity ;
    skos:definition ""@en ;
    skos:inScheme piirritev:Note ;
    skos:prefLabel "A13-06 03 xml"@en .

piirritev:NoteA13-0612Xml a skos:Concept ;
    piirrite:osmId "A13-06_12_xml" ;
    rdfs:subClassOf piirrite:OsmEntity ;
    skos:definition ""@en ;
    skos:inScheme piirritev:Note ;
    skos:prefLabel "A13-06 12 xml"@en .

piirritev:NoteC a skos:Concept ;
    piirrite:osmId "C" ;
    rdfs:subClassOf piirrite:OsmEntity ;
    skos:definition ""@en ;
    skos:inScheme piirritev:Note ;
    skos:prefLabel "C"@en .

piirritev:NoteIstniejcy a skos:Concept ;
    piirrite:osmId "istniejcy" ;
    rdfs:subClassOf piirrite:OsmEntity ;
    skos:definition ""@en ;
    skos:inScheme piirritev:Note ;
    skos:prefLabel "Istniejcy"@en .

piirritev:NoteSemiDur a skos:Concept ;
    piirrite:osmId "semi_dur" ;
    rdfs:subClassOf piirrite:OsmEntity ;
    skos:definition ""@en ;
    skos:inScheme piirritev:Note ;
    skos:prefLabel "Semi dur"@en .

piirritev:Note a skos:Concept ;
    piirrite:osmId "" ;
    rdfs:subClassOf piirrite:OsmEntity ;
    skos:definition ""@en ;
    skos:inScheme piirritev:Note ;
    skos:prefLabel ""@en .

piirritev:Note a skos:Concept ;
    piirrite:osmId "" ;
    rdfs:subClassOf piirrite:OsmEntity ;
    skos:definition ""@en ;
    skos:inScheme piirritev:Note ;
    skos:prefLabel ""@en .

piirritev:OfficialNameStarbucksCoffee a skos:Concept ;
    piirrite:osmId "Starbucks_Coffee" ;
    rdfs:subClassOf piirrite:OsmEntity ;
    skos:definition ""@en ;
    skos:inScheme piirritev:OfficialName ;
    skos:prefLabel "Starbucks coffee"@en .

piirritev:OfficialStatus a skos:ConceptScheme ;
    piirrite:osmId "official_status" ;
    skos:definition ""@en ;
    skos:prefLabel "Official status, types"@en .

piirritev:OldName a skos:ConceptScheme ;
    piirrite:osmId "old_name" ;
    skos:definition "Old / previous / historic name for an element."@en ;
    skos:prefLabel "Old name, types"@en .

piirritev:OperatorAdif a skos:Concept ;
    piirrite:osmId "Adif" ;
    rdfs:subClassOf piirrite:OsmEntity ;
    skos:definition ""@en ;
    skos:inScheme piirritev:Operator ;
    skos:prefLabel "Adif"@en .

piirritev:OperatorAtac a skos:Concept ;
    piirrite:osmId "ATAC" ;
    rdfs:subClassOf piirrite:OsmEntity ;
    skos:definition ""@en ;
    skos:inScheme piirritev:Operator ;
    skos:prefLabel "Atac"@en .

piirritev:OperatorBnsfRailway a skos:Concept ;
    piirrite:osmId "BNSF_Railway" ;
    rdfs:subClassOf piirrite:OsmEntity ;
    skos:definition ""@en ;
    skos:inScheme piirritev:Operator ;
    skos:prefLabel "Bnsf railway"@en .

piirritev:OperatorCanadaPost a skos:Concept ;
    piirrite:osmId "Canada_Post" ;
    rdfs:subClassOf piirrite:OsmEntity ;
    skos:definition ""@en ;
    skos:inScheme piirritev:Operator ;
    skos:prefLabel "Canada post"@en .

piirritev:OperatorCfr a skos:Concept ;
    piirrite:osmId "CFR" ;
    rdfs:subClassOf piirrite:OsmEntity ;
    skos:definition ""@en ;
    skos:inScheme piirritev:Operator ;
    skos:prefLabel "Cfr"@en .

piirritev:OperatorCsxTransportation a skos:Concept ;
    piirrite:osmId "CSX_Transportation" ;
    rdfs:subClassOf piirrite:OsmEntity ;
    skos:definition ""@en ;
    skos:inScheme piirritev:Operator ;
    skos:prefLabel "Csx transportation"@en .

piirritev:OperatorDbInfrago a skos:Concept ;
    piirrite:osmId "DB_InfraGO" ;
    rdfs:subClassOf piirrite:OsmEntity ;
    skos:definition ""@en ;
    skos:inScheme piirritev:Operator ;
    skos:prefLabel "Db infrago"@en .

piirritev:OperatorDbNetz a skos:Concept ;
    piirrite:osmId "DB_Netz" ;
    rdfs:subClassOf piirrite:OsmEntity ;
    skos:definition ""@en ;
    skos:inScheme piirritev:Operator ;
    skos:prefLabel "Db netz"@en .

piirritev:OperatorDeLijn a skos:Concept ;
    piirrite:osmId "De_Lijn" ;
    rdfs:subClassOf piirrite:OsmEntity ;
    skos:definition ""@en ;
    skos:inScheme piirritev:Operator ;
    skos:prefLabel "De lijn"@en .

piirritev:OperatorDeutschePost a skos:Concept ;
    piirrite:osmId "Deutsche_Post" ;
    rdfs:subClassOf piirrite:OsmEntity ;
    skos:definition ""@en ;
    skos:inScheme piirritev:Operator ;
    skos:prefLabel "Deutsche post"@en .

piirritev:OperatorDhl a skos:Concept ;
    piirrite:osmId "DHL" ;
    rdfs:subClassOf piirrite:OsmEntity ;
    skos:definition ""@en ;
    skos:inScheme piirritev:Operator ;
    skos:prefLabel "Dhl"@en .

piirritev:OperatorE-Redes a skos:Concept ;
    piirrite:osmId "E-REDES" ;
    rdfs:subClassOf piirrite:OsmEntity ;
    skos:definition ""@en ;
    skos:inScheme piirritev:Operator ;
    skos:prefLabel "E-redes"@en .

piirritev:OperatorEamNetz a skos:Concept ;
    piirrite:osmId "EAM_Netz" ;
    rdfs:subClassOf piirrite:OsmEntity ;
    skos:definition ""@en ;
    skos:inScheme piirritev:Operator ;
    skos:prefLabel "Eam netz"@en .

piirritev:OperatorEnedis a skos:Concept ;
    piirrite:hasRelatedOsmTag piirrite:hasEnedisPower ;
    piirrite:osmId "Enedis" ;
    rdfs:subClassOf piirrite:OsmEntity ;
    skos:definition "French network operator for electricity distribution in metropolitan France."@en ;
    skos:inScheme piirritev:Operator ;
    skos:prefLabel "Enedis"@en .

piirritev:OperatorEnergieAg a skos:Concept ;
    piirrite:osmId "Energie_AG" ;
    rdfs:subClassOf piirrite:OsmEntity ;
    skos:definition ""@en ;
    skos:inScheme piirritev:Operator ;
    skos:prefLabel "Energie ag"@en .

piirritev:OperatorEsbNetworks a skos:Concept ;
    piirrite:osmId "ESB_Networks" ;
    rdfs:subClassOf piirrite:OsmEntity ;
    skos:definition ""@en ;
    skos:inScheme piirritev:Operator ;
    skos:prefLabel "Esb networks"@en .

piirritev:OperatorFederalTransferido a skos:Concept ;
    piirrite:osmId "Federal_Transferido" ;
    rdfs:subClassOf piirrite:OsmEntity ;
    skos:definition ""@en ;
    skos:inScheme piirritev:Operator ;
    skos:prefLabel "Federal transferido"@en .

piirritev:OperatorGrdis a skos:Concept ;
    piirrite:osmId "Grdis" ;
    rdfs:subClassOf piirrite:OsmEntity ;
    skos:definition ""@en ;
    skos:inScheme piirritev:Operator ;
    skos:prefLabel "Grdis"@en .

piirritev:OperatorHelpbidea a skos:Concept ;
    piirrite:osmId "helpbidea" ;
    rdfs:subClassOf piirrite:OsmEntity ;
    skos:definition ""@en ;
    skos:inScheme piirritev:Operator ;
    skos:prefLabel "Helpbidea"@en .

piirritev:OperatorHydro-Qubec a skos:Concept ;
    piirrite:osmId "Hydro-Qubec" ;
    rdfs:subClassOf piirrite:OsmEntity ;
    skos:definition ""@en ;
    skos:inScheme piirritev:Operator ;
    skos:prefLabel "Hydro-qubec"@en .

piirritev:OperatorHydroOne a skos:Concept ;
    piirrite:osmId "Hydro_One" ;
    rdfs:subClassOf piirrite:OsmEntity ;
    skos:definition ""@en ;
    skos:inScheme piirritev:Operator ;
    skos:prefLabel "Hydro one"@en .

piirritev:OperatorInfrabel a skos:Concept ;
    piirrite:osmId "Infrabel" ;
    rdfs:subClassOf piirrite:OsmEntity ;
    skos:definition ""@en ;
    skos:inScheme piirritev:Operator ;
    skos:prefLabel "Infrabel"@en .

piirritev:OperatorInpost a skos:Concept ;
    piirrite:osmId "InPost" ;
    rdfs:subClassOf piirrite:OsmEntity ;
    skos:definition ""@en ;
    skos:inScheme piirritev:Operator ;
    skos:prefLabel "Inpost"@en .

piirritev:OperatorJcdecaux a skos:Concept ;
    piirrite:osmId "JCDecaux" ;
    rdfs:subClassOf piirrite:OsmEntity ;
    skos:definition ""@en ;
    skos:inScheme piirritev:Operator ;
    skos:prefLabel "Jcdecaux"@en .

piirritev:OperatorLaPoste a skos:Concept ;
    piirrite:osmId "La_Poste" ;
    rdfs:subClassOf piirrite:OsmEntity ;
    skos:definition "La Poste is the postal operator of France."@en ;
    skos:inScheme piirritev:Operator ;
    skos:prefLabel "La poste"@en .

piirritev:OperatorLimasam a skos:Concept ;
    piirrite:osmId "Limasam" ;
    rdfs:subClassOf piirrite:OsmEntity ;
    skos:definition ""@en ;
    skos:inScheme piirritev:Operator ;
    skos:prefLabel "Limasam"@en .

piirritev:OperatorLisea a skos:Concept ;
    piirrite:osmId "LISEA" ;
    rdfs:subClassOf piirrite:OsmEntity ;
    skos:definition ""@en ;
    skos:inScheme piirritev:Operator ;
    skos:prefLabel "Lisea"@en .

piirritev:OperatorMeralco a skos:Concept ;
    piirrite:osmId "Meralco" ;
    rdfs:subClassOf piirrite:OsmEntity ;
    skos:definition ""@en ;
    skos:inScheme piirritev:Operator ;
    skos:prefLabel "Meralco"@en .

piirritev:OperatorMetroTransit a skos:Concept ;
    piirrite:osmId "Metro_Transit" ;
    rdfs:subClassOf piirrite:OsmEntity ;
    skos:definition ""@en ;
    skos:inScheme piirritev:Operator ;
    skos:prefLabel "Metro transit"@en .

piirritev:OperatorMiami-DadeTransit a skos:Concept ;
    piirrite:osmId "Miami-Dade_Transit" ;
    rdfs:subClassOf piirrite:OsmEntity ;
    skos:definition ""@en ;
    skos:inScheme piirritev:Operator ;
    skos:prefLabel "Miami-dade transit"@en .

piirritev:OperatorMv a skos:Concept ;
    piirrite:osmId "MV" ;
    rdfs:subClassOf piirrite:OsmEntity ;
    skos:definition ""@en ;
    skos:inScheme piirritev:Operator ;
    skos:prefLabel "Mv"@en .

piirritev:OperatorNationalGrid a skos:Concept ;
    piirrite:osmId "National_Grid" ;
    rdfs:subClassOf piirrite:OsmEntity ;
    skos:definition ""@en ;
    skos:inScheme piirritev:Operator ;
    skos:prefLabel "National grid"@en .

piirritev:OperatorNationalHighways a skos:Concept ;
    piirrite:osmId "National_Highways" ;
    rdfs:subClassOf piirrite:OsmEntity ;
    skos:definition ""@en ;
    skos:inScheme piirritev:Operator ;
    skos:prefLabel "National highways"@en .

piirritev:OperatorNatran a skos:Concept ;
    piirrite:hasRelatedOsmTag piirrite:hasNatranManMade,
        piirrite:hasNatranMarker,
        piirrite:hasNatranPipeline ;
    piirrite:osmId "NaTran" ;
    rdfs:subClassOf piirrite:OsmEntity ;
    skos:definition "Main French gas transmission network operator."@en ;
    skos:inScheme piirritev:Operator ;
    skos:prefLabel "Natran"@en .

piirritev:OperatorNetworkRail a skos:Concept ;
    piirrite:osmId "Network_Rail" ;
    rdfs:subClassOf piirrite:OsmEntity ;
    skos:definition ""@en ;
    skos:inScheme piirritev:Operator ;
    skos:prefLabel "Network rail"@en .

piirritev:OperatorNieNetworks a skos:Concept ;
    piirrite:osmId "NIE_Networks" ;
    rdfs:subClassOf piirrite:OsmEntity ;
    skos:definition ""@en ;
    skos:inScheme piirritev:Operator ;
    skos:prefLabel "Nie networks"@en .

piirritev:OperatorOrange a skos:Concept ;
    piirrite:hasRelatedOsmTag piirrite:hasOrangeTelecom ;
    piirrite:osmId "Orange" ;
    rdfs:subClassOf piirrite:OsmEntity ;
    skos:definition "Global telecommunication network operator based in France."@en ;
    skos:inScheme piirritev:Operator ;
    skos:prefLabel "Orange"@en .

piirritev:OperatorPag a skos:Concept ;
    piirrite:osmId "PAG" ;
    rdfs:subClassOf piirrite:OsmEntity ;
    skos:definition ""@en ;
    skos:inScheme piirritev:Operator ;
    skos:prefLabel "Pag"@en .

piirritev:OperatorPgeDystrybucja a skos:Concept ;
    piirrite:osmId "PGE_Dystrybucja" ;
    rdfs:subClassOf piirrite:OsmEntity ;
    skos:definition ""@en ;
    skos:inScheme piirritev:Operator ;
    skos:prefLabel "Pge dystrybucja"@en .

piirritev:OperatorPglLp a skos:Concept ;
    piirrite:osmId "PGL_LP" ;
    rdfs:subClassOf piirrite:OsmEntity ;
    skos:definition ""@en ;
    skos:inScheme piirritev:Operator ;
    skos:prefLabel "Pgl lp"@en .

piirritev:OperatorPosteItaliane a skos:Concept ;
    piirrite:osmId "Poste_Italiane" ;
    rdfs:subClassOf piirrite:OsmEntity ;
    skos:definition ""@en ;
    skos:inScheme piirritev:Operator ;
    skos:prefLabel "Poste italiane"@en .

piirritev:OperatorProrail a skos:Concept ;
    piirrite:hasRelatedOsmTag piirrite:hasProrailRailway ;
    piirrite:osmId "ProRail" ;
    rdfs:subClassOf piirrite:OsmEntity ;
    skos:definition "Operated by ProRail B.V., The Netherlands"@en ;
    skos:inScheme piirritev:Operator ;
    skos:prefLabel "Prorail"@en .

piirritev:OperatorRfi a skos:Concept ;
    piirrite:osmId "RFI" ;
    rdfs:subClassOf piirrite:OsmEntity ;
    skos:definition ""@en ;
    skos:inScheme piirritev:Operator ;
    skos:prefLabel "Rfi"@en .

piirritev:OperatorRijkswaterstaat a skos:Concept ;
    piirrite:hasRelatedOsmTag piirrite:hasRijkswaterstaatHighway,
        piirrite:hasRijkswaterstaatManMade,
        piirrite:hasRijkswaterstaatOwner,
        piirrite:hasRijkswaterstaatWaterway ;
    piirrite:osmId "Rijkswaterstaat" ;
    rdfs:subClassOf piirrite:OsmEntity ;
    skos:definition "Operated by the Dutch Rijkswaterstaat"@en ;
    skos:inScheme piirritev:Operator ;
    skos:prefLabel "Rijkswaterstaat"@en .

piirritev:OperatorRoyalMail a skos:Concept ;
    piirrite:osmId "Royal_Mail" ;
    rdfs:subClassOf piirrite:OsmEntity ;
    skos:definition ""@en ;
    skos:inScheme piirritev:Operator ;
    skos:prefLabel "Royal mail"@en .

piirritev:OperatorRte a skos:Concept ;
    piirrite:hasRelatedOsmTag piirrite:hasRtePower ;
    piirrite:osmId "RTE" ;
    rdfs:subClassOf piirrite:OsmEntity ;
    skos:definition "Company responsible of French power transmission network operation."@en ;
    skos:inScheme piirritev:Operator ;
    skos:prefLabel "Rte"@en .

piirritev:OperatorSadalesTkls a skos:Concept ;
    piirrite:osmId "Sadales_tkls" ;
    rdfs:subClassOf piirrite:OsmEntity ;
    skos:definition ""@en ;
    skos:inScheme piirritev:Operator ;
    skos:prefLabel "Sadales tkls"@en .

piirritev:OperatorSbb a skos:Concept ;
    piirrite:osmId "SBB" ;
    rdfs:subClassOf piirrite:OsmEntity ;
    skos:definition ""@en ;
    skos:inScheme piirritev:Operator ;
    skos:prefLabel "Sbb"@en .

piirritev:OperatorSchwarzwaldverein a skos:Concept ;
    piirrite:osmId "Schwarzwaldverein" ;
    rdfs:subClassOf piirrite:OsmEntity ;
    skos:definition ""@en ;
    skos:inScheme piirritev:Operator ;
    skos:prefLabel "Schwarzwaldverein"@en .

piirritev:OperatorSncf a skos:Concept ;
    piirrite:osmId "SNCF" ;
    rdfs:subClassOf piirrite:OsmEntity ;
    skos:definition ""@en ;
    skos:inScheme piirritev:Operator ;
    skos:prefLabel "Sncf"@en .

piirritev:OperatorSncfRseau a skos:Concept ;
    piirrite:osmId "SNCF_Rseau" ;
    rdfs:subClassOf piirrite:OsmEntity ;
    skos:definition ""@en ;
    skos:inScheme piirritev:Operator ;
    skos:prefLabel "Sncf rseau"@en .

piirritev:OperatorSrd a skos:Concept ;
    piirrite:osmId "SRD" ;
    rdfs:subClassOf piirrite:OsmEntity ;
    skos:definition ""@en ;
    skos:inScheme piirritev:Operator ;
    skos:prefLabel "Srd"@en .

piirritev:OperatorStadtWitten a skos:Concept ;
    piirrite:osmId "Stadt_Witten" ;
    rdfs:subClassOf piirrite:OsmEntity ;
    skos:definition ""@en ;
    skos:inScheme piirritev:Operator ;
    skos:prefLabel "Stadt witten"@en .

piirritev:OperatorTauron a skos:Concept ;
    piirrite:osmId "Tauron" ;
    rdfs:subClassOf piirrite:OsmEntity ;
    skos:definition ""@en ;
    skos:inScheme piirritev:Operator ;
    skos:prefLabel "Tauron"@en .

piirritev:OperatorTcdd a skos:Concept ;
    piirrite:osmId "TCDD" ;
    rdfs:subClassOf piirrite:OsmEntity ;
    skos:definition ""@en ;
    skos:inScheme piirritev:Operator ;
    skos:prefLabel "Tcdd"@en .

piirritev:OperatorTec a skos:Concept ;
    piirrite:hasRelatedOsmTag piirrite:hasTecHighway,
        piirrite:hasTecPublicTransport,
        piirrite:hasTecRoute ;
    piirrite:osmId "TEC" ;
    rdfs:subClassOf piirrite:OsmEntity ;
    skos:definition "Operated by Transport en Commun (TEC)"@en ;
    skos:inScheme piirritev:Operator ;
    skos:prefLabel "Tec"@en .

piirritev:OperatorTeia a skos:Concept ;
    piirrite:osmId "TEA" ;
    rdfs:subClassOf piirrite:OsmEntity ;
    skos:definition ""@en ;
    skos:inScheme piirritev:Operator ;
    skos:prefLabel "Teia"@en .

piirritev:OperatorTrafikverket a skos:Concept ;
    piirrite:osmId "Trafikverket" ;
    rdfs:subClassOf piirrite:OsmEntity ;
    skos:definition ""@en ;
    skos:inScheme piirritev:Operator ;
    skos:prefLabel "Trafikverket"@en .

piirritev:OperatorTreda a skos:Concept ;
    piirrite:osmId "TREDA" ;
    rdfs:subClassOf piirrite:OsmEntity ;
    skos:definition ""@en ;
    skos:inScheme piirritev:Operator ;
    skos:prefLabel "Treda"@en .

piirritev:OperatorVejdirektoratet a skos:Concept ;
    piirrite:osmId "Vejdirektoratet" ;
    rdfs:subClassOf piirrite:OsmEntity ;
    skos:definition ""@en ;
    skos:inScheme piirritev:Operator ;
    skos:prefLabel "Vejdirektoratet"@en .

piirritev:OperatorVolnbusz a skos:Concept ;
    piirrite:osmId "Volnbusz" ;
    rdfs:subClassOf piirrite:OsmEntity ;
    skos:definition ""@en ;
    skos:inScheme piirritev:Operator ;
    skos:prefLabel "Volnbusz"@en .

piirritev:OperatorVylvirasto a skos:Concept ;
    piirrite:osmId "Vylvirasto" ;
    rdfs:subClassOf piirrite:OsmEntity ;
    skos:definition ""@en ;
    skos:inScheme piirritev:Operator ;
    skos:prefLabel "Vylvirasto"@en .

piirritev:OperatorYpfSA a skos:Concept ;
    piirrite:osmId "YPF_S_A_" ;
    rdfs:subClassOf piirrite:OsmEntity ;
    skos:definition ""@en ;
    skos:inScheme piirritev:Operator ;
    skos:prefLabel "Ypf s a "@en .

piirritev:Operatorbb-InfrastrukturAg a skos:Concept ;
    piirrite:osmId "BB-Infrastruktur_AG" ;
    rdfs:subClassOf piirrite:OsmEntity ;
    skos:definition ""@en ;
    skos:inScheme piirritev:Operator ;
    skos:prefLabel "bb-infrastruktur ag"@en .

piirritev:OperatorezDistribuce a skos:Concept ;
    piirrite:osmId "EZ_Distribuce" ;
    rdfs:subClassOf piirrite:OsmEntity ;
    skos:definition ""@en ;
    skos:inScheme piirritev:Operator ;
    skos:prefLabel "ez distribuce"@en .

piirritev:Operatorett a skos:Concept ;
    piirrite:osmId "ETT" ;
    rdfs:subClassOf piirrite:OsmEntity ;
    skos:definition ""@en ;
    skos:inScheme piirritev:Operator ;
    skos:prefLabel "ett"@en .

piirritev:Operatorsr a skos:Concept ;
    piirrite:osmId "SR" ;
    rdfs:subClassOf piirrite:OsmEntity ;
    skos:definition ""@en ;
    skos:inScheme piirritev:Operator ;
    skos:prefLabel "sr"@en .

piirritev:Operator a skos:Concept ;
    piirrite:osmId "_" ;
    rdfs:subClassOf piirrite:OsmEntity ;
    skos:definition ""@en ;
    skos:inScheme piirritev:Operator ;
    skos:prefLabel " "@en .

piirritev:Operator a skos:Concept ;
    piirrite:osmId "" ;
    rdfs:subClassOf piirrite:OsmEntity ;
    skos:definition ""@en ;
    skos:inScheme piirritev:Operator ;
    skos:prefLabel ""@en .

piirritev:Operator a skos:Concept ;
    piirrite:osmId "" ;
    rdfs:subClassOf piirrite:OsmEntity ;
    skos:definition ""@en ;
    skos:inScheme piirritev:Operator ;
    skos:prefLabel ""@en .

piirritev:Operator a skos:Concept ;
    piirrite:osmId "" ;
    rdfs:subClassOf piirrite:OsmEntity ;
    skos:definition ""@en ;
    skos:inScheme piirritev:Operator ;
    skos:prefLabel ""@en .

piirritev:Operator a skos:Concept ;
    piirrite:osmId "" ;
    rdfs:subClassOf piirrite:OsmEntity ;
    skos:definition ""@en ;
    skos:inScheme piirritev:Operator ;
    skos:prefLabel ""@en .

piirritev:Operator a skos:Concept ;
    piirrite:osmId "" ;
    rdfs:subClassOf piirrite:OsmEntity ;
    skos:definition ""@en ;
    skos:inScheme piirritev:Operator ;
    skos:prefLabel ""@en .

piirritev:Operator a skos:Concept ;
    piirrite:osmId "_" ;
    rdfs:subClassOf piirrite:OsmEntity ;
    skos:definition ""@en ;
    skos:inScheme piirritev:Operator ;
    skos:prefLabel " "@en .

piirritev:Operator a skos:Concept ;
    piirrite:osmId "" ;
    rdfs:subClassOf piirrite:OsmEntity ;
    skos:definition ""@en ;
    skos:inScheme piirritev:Operator ;
    skos:prefLabel ""@en .

piirritev:Operator a skos:Concept ;
    piirrite:osmId "" ;
    rdfs:subClassOf piirrite:OsmEntity ;
    skos:definition ""@en ;
    skos:inScheme piirritev:Operator ;
    skos:prefLabel ""@en .

piirritev:Overtaking a skos:ConceptScheme ;
    piirrite:osmId "overtaking" ;
    skos:definition "Overtaking restrictions as signposted or painted on the ground"@en ;
    skos:prefLabel "Overtaking, types"@en .

piirritev:OwnerRgionWallonne a skos:Concept ;
    piirrite:osmId "Rgion_wallonne" ;
    rdfs:subClassOf piirrite:OsmEntity ;
    skos:definition ""@en ;
    skos:inScheme piirritev:Owner ;
    skos:prefLabel "Rgion wallonne"@en .

piirritev:ParkingSpaceCharging a skos:Concept ;
    piirrite:osmId "charging" ;
    rdfs:subClassOf piirrite:OsmEntity ;
    skos:definition "A parking space designated for use while charging electric vehicles. osmcarto-rendering=File:Rendering-parking space.png osmcarto-rendering-size=125px"@en ;
    skos:inScheme piirritev:ParkingSpace ;
    skos:prefLabel "Charging"@en .

piirritev:ParkingSpaceDisabled a skos:Concept ;
    piirrite:osmId "disabled" ;
    rdfs:subClassOf piirrite:OsmEntity ;
    skos:definition "A parking space specifically designated for use by people with disabilities."@en ;
    skos:inScheme piirritev:ParkingSpace ;
    skos:prefLabel "Disabled"@en .

piirritev:PassengerInformationDisplay a skos:ConceptScheme ;
    piirrite:osmId "passenger_information_display" ;
    skos:definition "A passenger information system."@en ;
    skos:prefLabel "Passenger information display, types"@en .

piirritev:PassengerLines a skos:ConceptScheme ;
    piirrite:osmId "passenger_lines" ;
    skos:definition "Used to describe number of tracks of the railway line a certain track segment belongs to."@en ;
    skos:prefLabel "Passenger lines, types"@en .

piirritev:Phone a skos:ConceptScheme ;
    piirrite:osmId "phone" ;
    skos:definition "A telephone number associated with the object. Use +CC XXX XXX XXX format, where CC is a country code."@en ;
    skos:prefLabel "Phone, types"@en .

piirritev:PlacementTransition a skos:Concept ;
    piirrite:hasRelatedOsmTag piirrite:hasTransitionHighway ;
    piirrite:osmId "transition" ;
    rdfs:subClassOf piirrite:OsmEntity ;
    skos:definition "Used to indicate that the shape of the OSM way follows neither the middle nor the left/right side of any lane."@en ;
    skos:inScheme piirritev:Placement ;
    skos:prefLabel "Transition"@en .

piirritev:Population a skos:ConceptScheme ;
    piirrite:osmId "population" ;
    skos:definition "Indicates a rough number of citizens in a given place."@en ;
    skos:prefLabel "Population, types"@en .

piirritev:Power a skos:ConceptScheme ;
    piirrite:osmId "power" ;
    skos:definition "Facilities for generation and distribution of electrical power."@en ;
    skos:prefLabel "Power, types"@en .

piirritev:PriorityRoadDesignated a skos:Concept ;
    piirrite:osmId "designated" ;
    rdfs:subClassOf piirrite:OsmEntity ;
    skos:definition ""@en ;
    skos:inScheme piirritev:PriorityRoad ;
    skos:prefLabel "Designated"@en .

piirritev:ProposedMotorway a skos:Concept ;
    piirrite:osmId "motorway" ;
    rdfs:subClassOf piirrite:OsmEntity ;
    skos:definition ""@en ;
    skos:inScheme piirritev:Proposed ;
    skos:prefLabel "Motorway"@en .

piirritev:ProposedRail a skos:Concept ;
    piirrite:osmId "rail" ;
    rdfs:subClassOf piirrite:OsmEntity ;
    skos:definition ""@en ;
    skos:inScheme piirritev:Proposed ;
    skos:prefLabel "Rail"@en .

piirritev:ProposedResidential a skos:Concept ;
    piirrite:osmId "residential" ;
    rdfs:subClassOf piirrite:OsmEntity ;
    skos:definition ""@en ;
    skos:inScheme piirritev:Proposed ;
    skos:prefLabel "Residential"@en .

piirritev:Pump a skos:ConceptScheme ;
    piirrite:osmId "pump" ;
    skos:definition "Presence and technology of a pump on a source of water."@en ;
    skos:prefLabel "Pump, types"@en .

piirritev:RoomOffice a skos:Concept ;
    piirrite:osmId "office" ;
    rdfs:subClassOf piirrite:OsmEntity ;
    skos:definition ""@en ;
    skos:inScheme piirritev:Room ;
    skos:prefLabel "Office"@en .

piirritev:RoomShop a skos:Concept ;
    piirrite:osmId "shop" ;
    rdfs:subClassOf piirrite:OsmEntity ;
    skos:definition ""@en ;
    skos:inScheme piirritev:Room ;
    skos:prefLabel "Shop"@en .

piirritev:RouteMasterBus a skos:Concept ;
    piirrite:osmId "bus" ;
    rdfs:subClassOf piirrite:OsmEntity ;
    skos:definition ""@en ;
    skos:inScheme piirritev:RouteMaster ;
    skos:prefLabel "Bus"@en .

piirritev:ServiceAlley a skos:Concept ;
    piirrite:osmId "alley" ;
    rdfs:subClassOf piirrite:OsmEntity ;
    skos:definition "An alley is a service road usually located between properties for access to utilities."@en ;
    skos:inScheme piirritev:Service ;
    skos:prefLabel "Alley"@en .

piirritev:ServiceCrossover a skos:Concept ;
    piirrite:hasRelatedOsmTag piirrite:hasCrossoverElectrified,
        piirrite:hasCrossoverGauge,
        piirrite:hasCrossoverOperator ;
    piirrite:osmId "crossover" ;
    rdfs:subClassOf piirrite:OsmEntity ;
    skos:definition "A railway crossover"@en ;
    skos:inScheme piirritev:Service ;
    skos:prefLabel "Crossover"@en .

piirritev:ServiceDrive-Through a skos:Concept ;
    piirrite:hasRelatedOsmTag piirrite:hasDrive-ThroughOneway ;
    piirrite:osmId "drive-through" ;
    rdfs:subClassOf piirrite:OsmEntity ;
    skos:definition "A drive-through way where customers can visit a business without leaving their cars. osmcarto-rendering=File:Rendering-highway service minor.png osmcarto-rendering-size=125px"@en ;
    skos:inScheme piirritev:Service ;
    skos:prefLabel "Drive-through"@en .

piirritev:ServiceDriveway a skos:Concept ;
    piirrite:hasRelatedOsmTag piirrite:hasDrivewayAccess,
        piirrite:hasDrivewayOneway ;
    piirrite:osmId "driveway" ;
    rdfs:subClassOf piirrite:OsmEntity ;
    skos:definition "Specifies that a road is a driveway, typically leading to a residence or business. osmcarto-rendering=File:Rendering-highway service minor.png osmcarto-rendering-size=125px"@en ;
    skos:inScheme piirritev:Service ;
    skos:prefLabel "Driveway"@en .

piirritev:ServiceEmergencyAccess a skos:Concept ;
    piirrite:hasRelatedOsmTag piirrite:hasEmergencyAccessEmergency,
        piirrite:hasEmergencyAccessSurface ;
    piirrite:osmId "emergency_access" ;
    rdfs:subClassOf piirrite:OsmEntity ;
    skos:definition "A way that is an emergency access road."@en ;
    skos:inScheme piirritev:Service ;
    skos:prefLabel "Emergency access"@en .

piirritev:ServiceIrrigation a skos:Concept ;
    piirrite:hasRelatedOsmTag piirrite:hasIrrigationLocation,
        piirrite:hasIrrigationWaterway ;
    piirrite:osmId "irrigation" ;
    rdfs:subClassOf piirrite:OsmEntity ;
    skos:definition "Specifies a waterway which carries water to be used for agriculture"@en ;
    skos:inScheme piirritev:Service ;
    skos:prefLabel "Irrigation"@en .

piirritev:ServiceParkingAisle a skos:Concept ;
    piirrite:hasRelatedOsmTag piirrite:hasParkingAisleOneway ;
    piirrite:osmId "parking_aisle" ;
    rdfs:subClassOf piirrite:OsmEntity ;
    skos:definition "a subordinated way in a parking lot between rows of parking spaces that vehicles use to drive into and out of the spaces.  osmcarto-rendering=File:Rendering-highway service minor.png  osmcarto-rendering-size=125px"@en ;
    skos:inScheme piirritev:Service ;
    skos:prefLabel "Parking aisle"@en .

piirritev:ServiceRegional a skos:Concept ;
    piirrite:osmId "regional" ;
    rdfs:subClassOf piirrite:OsmEntity ;
    skos:definition ""@en ;
    skos:inScheme piirritev:Service ;
    skos:prefLabel "Regional"@en .

piirritev:ServiceSiding a skos:Concept ;
    piirrite:hasRelatedOsmTag piirrite:hasSidingOperator,
        piirrite:hasSidingRef ;
    piirrite:osmId "siding" ;
    rdfs:subClassOf piirrite:OsmEntity ;
    skos:definition "Relatively short lengths of track, running parallel to (and connected to) a main route. osmcarto-rendering=File:Rendering-railway rail service.png osmcarto-rendering-size=125px"@en ;
    skos:inScheme piirritev:Service ;
    skos:prefLabel "Siding"@en .

piirritev:ServiceSlipway a skos:Concept ;
    piirrite:osmId "slipway" ;
    rdfs:subClassOf piirrite:OsmEntity ;
    skos:definition "A ramp for launching a boat that leads into the water."@en ;
    skos:inScheme piirritev:Service ;
    skos:prefLabel "Slipway"@en .

piirritev:ServiceSpur a skos:Concept ;
    piirrite:hasRelatedOsmTag piirrite:hasSpurOperator,
        piirrite:hasSpurRef ;
    piirrite:osmId "spur" ;
    rdfs:subClassOf piirrite:OsmEntity ;
    skos:definition "Relatively short lengths of track, built to give one company or entity access to the main line, normally for freight-only use. osmcarto-rendering=File:Rendering-railway rail service.png osmcarto-rendering-size=125px"@en ;
    skos:inScheme piirritev:Service ;
    skos:prefLabel "Spur"@en .

piirritev:ServiceUtility a skos:Concept ;
    piirrite:osmId "utility" ;
    rdfs:subClassOf piirrite:OsmEntity ;
    skos:definition ""@en ;
    skos:inScheme piirritev:Service ;
    skos:prefLabel "Utility"@en .

piirritev:ServiceYard a skos:Concept ;
    piirrite:hasRelatedOsmTag piirrite:hasYardOperator,
        piirrite:hasYardRef ;
    piirrite:osmId "yard" ;
    rdfs:subClassOf piirrite:OsmEntity ;
    skos:definition "Tracks within rail yards operated by the same company as one operating main line. osmcarto-rendering=File:Rendering-railway rail service.png osmcarto-rendering-size=125px"@en ;
    skos:inScheme piirritev:Service ;
    skos:prefLabel "Yard"@en .

piirritev:Shelter a skos:ConceptScheme ;
    piirrite:osmId "shelter" ;
    skos:definition "Indicates the presence of an associated shelter."@en ;
    skos:prefLabel "Shelter, types"@en .

piirritev:ShoulderBoth a skos:Concept ;
    piirrite:osmId "both" ;
    rdfs:subClassOf piirrite:OsmEntity ;
    skos:definition ""@en ;
    skos:inScheme piirritev:Shoulder ;
    skos:prefLabel "Both"@en .

piirritev:ShoulderRight a skos:Concept ;
    piirrite:osmId "right" ;
    rdfs:subClassOf piirrite:OsmEntity ;
    skos:definition ""@en ;
    skos:inScheme piirritev:Shoulder ;
    skos:prefLabel "Right"@en .

piirritev:SideLeft a skos:Concept ;
    piirrite:osmId "left" ;
    rdfs:subClassOf piirrite:OsmEntity ;
    skos:definition ""@en ;
    skos:inScheme piirritev:Side ;
    skos:prefLabel "Left"@en .

piirritev:SideRight a skos:Concept ;
    piirrite:osmId "right" ;
    rdfs:subClassOf piirrite:OsmEntity ;
    skos:definition ""@en ;
    skos:inScheme piirritev:Side ;
    skos:prefLabel "Right"@en .

piirritev:SmokingOutside a skos:Concept ;
    piirrite:osmId "outside" ;
    rdfs:subClassOf piirrite:OsmEntity ;
    skos:definition ""@en ;
    skos:inScheme piirritev:Smoking ;
    skos:prefLabel "Outside"@en .

piirritev:SocialFacilityAssistedLiving a skos:Concept ;
    piirrite:hasRelatedOsmTag piirrite:hasAssistedLivingName,
        piirrite:hasAssistedLivingOpeningHours,
        piirrite:hasAssistedLivingOperator,
        piirrite:hasAssistedLivingPhone,
        piirrite:hasAssistedLivingWebsite,
        piirrite:hasAssistedLivingWheelchair ;
    piirrite:osmId "assisted_living" ;
    rdfs:subClassOf piirrite:OsmEntity ;
    skos:definition "A residential facility like group_home, but the occupants are more independent. Usually conceived for people with minor disabilities."@en ;
    skos:inScheme piirritev:SocialFacility ;
    skos:prefLabel "Assisted living"@en .

piirritev:SocialFacilityGroupHome a skos:Concept ;
    piirrite:hasRelatedOsmTag piirrite:hasGroupHomeCapacity,
        piirrite:hasGroupHomeName,
        piirrite:hasGroupHomeOperator,
        piirrite:hasGroupHomePhone,
        piirrite:hasGroupHomeWebsite,
        piirrite:hasGroupHomeWheelchair ;
    piirrite:osmId "group_home" ;
    rdfs:subClassOf piirrite:OsmEntity ;
    skos:definition "A group home is a residence for a certain demographic, providing social and medical services, leisure activities, meals, and supervision."@en ;
    skos:inScheme piirritev:SocialFacility ;
    skos:prefLabel "Group home"@en .

piirritev:SocialFacilityNursingHome a skos:Concept ;
    piirrite:hasRelatedOsmTag piirrite:hasNursingHomeName ;
    piirrite:osmId "nursing_home" ;
    rdfs:subClassOf piirrite:OsmEntity ;
    skos:definition "A nursing home provides permanent care to elderly, ill, or disabled people."@en ;
    skos:inScheme piirritev:SocialFacility ;
    skos:prefLabel "Nursing home"@en .

piirritev:SocialFacilityOutreach a skos:Concept ;
    piirrite:osmId "outreach" ;
    rdfs:subClassOf piirrite:OsmEntity ;
    skos:definition "A non-residential facility that provides social welfare services such as advocacy, counseling, job placement, veterans services, housing placement, wellness programs or leisure activities."@en ;
    skos:inScheme piirritev:SocialFacility ;
    skos:prefLabel "Outreach"@en .

piirritev:StartDate19761991 a skos:Concept ;
    piirrite:osmId "1976__1991" ;
    rdfs:subClassOf piirrite:OsmEntity ;
    skos:definition ""@en ;
    skos:inScheme piirritev:StartDate ;
    skos:prefLabel "1976  1991"@en .

piirritev:StatusAbandoned a skos:Concept ;
    piirrite:osmId "abandoned" ;
    rdfs:subClassOf piirrite:OsmEntity ;
    skos:definition ""@en ;
    skos:inScheme piirritev:Status ;
    skos:prefLabel "Abandoned"@en .

piirritev:Status a skos:Concept ;
    piirrite:osmId "" ;
    rdfs:subClassOf piirrite:OsmEntity ;
    skos:definition ""@en ;
    skos:inScheme piirritev:Status ;
    skos:prefLabel ""@en .

piirritev:Supervised a skos:ConceptScheme ;
    piirrite:osmId "supervised" ;
    skos:definition "Indicates whether there is a person who supervises the place"@en ;
    skos:prefLabel "Supervised, types"@en .

piirritev:SurfaceSurvey a skos:ConceptScheme ;
    piirrite:osmId "surface_survey" ;
    skos:definition "Used to indicate the date when the surface feature of a highway was surveyed and tagged, mainly in Romania."@en ;
    skos:prefLabel "Surface survey, types"@en .

piirritev:Switch a skos:ConceptScheme ;
    piirrite:osmId "switch" ;
    skos:definition "Specifies switch function in a network"@en ;
    skos:prefLabel "Switch, types"@en .

piirritev:Toilets a skos:ConceptScheme ;
    piirrite:osmId "toilets" ;
    skos:definition "Indicates if a feature has a toilet."@en ;
    skos:prefLabel "Toilets, types"@en .

piirritev:TrailblazedSymbols a skos:Concept ;
    piirrite:osmId "symbols" ;
    rdfs:subClassOf piirrite:OsmEntity ;
    skos:definition ""@en ;
    skos:inScheme piirritev:Trailblazed ;
    skos:prefLabel "Symbols"@en .

piirritev:Tram a skos:ConceptScheme ;
    piirrite:osmId "tram" ;
    skos:definition "Specifies whether trams stop at a feature"@en ;
    skos:prefLabel "Tram, types"@en .

piirritev:TunnelBuildingPassage a skos:Concept ;
    piirrite:hasRelatedOsmTag piirrite:hasBuildingPassageHighway ;
    piirrite:osmId "building_passage" ;
    rdfs:subClassOf piirrite:OsmEntity ;
    skos:definition "A tunnel passage that goes through/under a building, but is not inside the building itself."@en ;
    skos:inScheme piirritev:Tunnel ;
    skos:prefLabel "Building passage"@en .

piirritev:TunnelCulvert a skos:Concept ;
    piirrite:hasRelatedOsmTag piirrite:hasCulvertDiameter,
        piirrite:hasCulvertLayer,
        piirrite:hasCulvertWaterway ;
    piirrite:osmId "culvert" ;
    rdfs:subClassOf piirrite:OsmEntity ;
    skos:definition "For a stream/drain/ditch/river passing under a road. Use it on the section of waterway passing under the road. osmcarto-rendering=File:Rendering-waterway river tunnel.png osmcarto-rendering-size=125px"@en ;
    skos:inScheme piirritev:Tunnel ;
    skos:prefLabel "Culvert"@en .

piirritev:TunnelFlooded a skos:Concept ;
    piirrite:hasRelatedOsmTag piirrite:hasFloodedUsage,
        piirrite:hasFloodedWaterway ;
    piirrite:osmId "flooded" ;
    rdfs:subClassOf piirrite:OsmEntity ;
    skos:definition "A long (over 100 meters) tunnel where flowing water or other fluid prevent humans from safely walking inside."@en ;
    skos:inScheme piirritev:Tunnel ;
    skos:prefLabel "Flooded"@en .

piirritev:UicRef a skos:ConceptScheme ;
    piirrite:osmId "uic_ref" ;
    skos:definition "The UIC reference is used to identify railway stations."@en ;
    skos:prefLabel "Uic ref, types"@en .

piirritev:UtilityGas a skos:Concept ;
    piirrite:hasRelatedOsmTag piirrite:hasGasBuilding,
        piirrite:hasGasLanduse,
        piirrite:hasGasManMade,
        piirrite:hasGasMarker,
        piirrite:hasGasOperator,
        piirrite:hasGasSubstance ;
    piirrite:osmId "gas" ;
    rdfs:subClassOf piirrite:OsmEntity ;
    skos:definition "Infrastructure related to gas transmission and distribution towards industries and domestic consumers."@en ;
    skos:inScheme piirritev:Utility ;
    skos:prefLabel "Gas"@en .

piirritev:UtilityPower a skos:Concept ;
    piirrite:hasRelatedOsmTag piirrite:hasPowerBuilding,
        piirrite:hasPowerLanduse,
        piirrite:hasPowerManMade,
        piirrite:hasPowerMarker,
        piirrite:hasPowerOperator,
        piirrite:hasPowerType ;
    piirrite:osmId "power" ;
    rdfs:subClassOf piirrite:OsmEntity ;
    skos:definition "Infrastructure related to electricity transmission and distribution towards industries and domestic consumers."@en ;
    skos:inScheme piirritev:Utility ;
    skos:prefLabel "Power"@en .

piirritev:UtilityStreetLighting a skos:Concept ;
    piirrite:hasRelatedOsmTag piirrite:hasStreetLightingOperator,
        piirrite:hasStreetLightingUsage ;
    piirrite:osmId "street_lighting" ;
    rdfs:subClassOf piirrite:OsmEntity ;
    skos:definition "Activity related to street, roads and cities lighting"@en ;
    skos:inScheme piirritev:Utility ;
    skos:prefLabel "Street lighting"@en .

piirritev:UtilityTelecom a skos:Concept ;
    piirrite:hasRelatedOsmTag piirrite:hasTelecomBuilding,
        piirrite:hasTelecomLanduse,
        piirrite:hasTelecomManMade,
        piirrite:hasTelecomMarker,
        piirrite:hasTelecomOperator,
        piirrite:hasTelecomType ;
    piirrite:osmId "telecom" ;
    rdfs:subClassOf piirrite:OsmEntity ;
    skos:definition "Infrastructure related to telecommunications networks providing phone and internet service towards industries and domestic subscribers."@en ;
    skos:inScheme piirritev:Utility ;
    skos:prefLabel "Telecom"@en .

piirritev:VehicleAgricultural a skos:Concept ;
    piirrite:osmId "agricultural" ;
    rdfs:subClassOf piirrite:OsmEntity ;
    skos:definition "The use of the road is authorized exclusively for all types of vehicles which use it for agricultural purposes"@en ;
    skos:inScheme piirritev:Vehicle ;
    skos:prefLabel "Agricultural"@en .

piirritev:VehicleDestination a skos:Concept ;
    piirrite:osmId "destination" ;
    rdfs:subClassOf piirrite:OsmEntity ;
    skos:definition "Indicates that transit traffic using vehicle is not allowed."@en ;
    skos:inScheme piirritev:Vehicle ;
    skos:prefLabel "Destination"@en .

piirritev:VehicleForestry a skos:Concept ;
    piirrite:osmId "forestry" ;
    rdfs:subClassOf piirrite:OsmEntity ;
    skos:definition "The use of the road is authorized exclusively for all types of vehicles which use it for agricultural purposes"@en ;
    skos:inScheme piirritev:Vehicle ;
    skos:prefLabel "Forestry"@en .

piirritev:VehiclePrivate a skos:Concept ;
    piirrite:osmId "private" ;
    rdfs:subClassOf piirrite:OsmEntity ;
    skos:definition ""@en ;
    skos:inScheme piirritev:Vehicle ;
    skos:prefLabel "Private"@en .

piirritev:Wall a skos:ConceptScheme ;
    piirrite:osmId "wall" ;
    skos:definition "Used to provide more detailed information about a tag:barrier=wall. The value should indicate the principle feature of the wall, which might be the type, purpose, or building material of the wall."@en ;
    skos:prefLabel "Wall, types"@en .

piirritev:Ward a skos:ConceptScheme ;
    piirrite:osmId "ward" ;
    skos:definition "Used differently around the world."@en ;
    skos:prefLabel "Ward, types"@en .

piirritev:WasteDogExcrement a skos:Concept ;
    piirrite:hasRelatedOsmTag piirrite:hasDogExcrementVending ;
    piirrite:osmId "dog_excrement" ;
    rdfs:subClassOf piirrite:OsmEntity ;
    skos:definition "A bin made for the disposal of dog excrement."@en ;
    skos:inScheme piirritev:Waste ;
    skos:prefLabel "Dog excrement"@en .

piirritev:WasteMixed a skos:Concept ;
    piirrite:osmId "mixed" ;
    rdfs:subClassOf piirrite:OsmEntity ;
    skos:definition ""@en ;
    skos:inScheme piirritev:Waste ;
    skos:prefLabel "Mixed"@en .

piirritev:WasteTrash a skos:Concept ;
    piirrite:osmId "trash" ;
    rdfs:subClassOf piirrite:OsmEntity ;
    skos:definition "A bin made for the disposal of trash/rubbish."@en ;
    skos:inScheme piirritev:Waste ;
    skos:prefLabel "Trash"@en .

piirritev:Website a skos:ConceptScheme ;
    piirrite:osmId "website" ;
    skos:definition "Specifies the link to the official website for a feature."@en ;
    skos:prefLabel "Website, types"@en .

piirritev:WetlandBog a skos:Concept ;
    piirrite:osmId "bog" ;
    rdfs:subClassOf piirrite:OsmEntity ;
    skos:definition "Acidic peat producing wetland. osmcarto-rendering-area=File:Natural_wetland_bog.png osmcarto-rendering-area-size=100px"@en ;
    skos:inScheme piirritev:Wetland ;
    skos:prefLabel "Bog"@en .

piirritev:WetlandFen a skos:Concept ;
    piirrite:osmId "fen" ;
    rdfs:subClassOf piirrite:OsmEntity ;
    skos:definition "Groundwater-fed peatforming wetland covered by mosses, grasses, sedges, reeds, and wildflowers. osmcarto-rendering=File:Natural_wetland_marsh.png osmcarto-rendering-size=100px"@en ;
    skos:inScheme piirritev:Wetland ;
    skos:prefLabel "Fen"@en .

piirritev:WetlandMangrove a skos:Concept ;
    piirrite:osmId "mangrove" ;
    rdfs:subClassOf piirrite:OsmEntity ;
    skos:definition "Mangrove ecosystem is formed by forests of salt tolerant mangrove trees in the tidal zone of tropical coasts with water temperatures above 20 C. osmcarto-rendering=File:Natural wetland mangrove.png osmcarto-rendering-size=100px"@en ;
    skos:inScheme piirritev:Wetland ;
    skos:prefLabel "Mangrove"@en .

piirritev:WetlandMarsh a skos:Concept ;
    piirrite:osmId "marsh" ;
    rdfs:subClassOf piirrite:OsmEntity ;
    skos:definition "Marsh is periodically saturated, flooded, or ponded with water and characterized by herbaceous (non-woody) vegetation adapted to wet soil conditions. osmcarto-rendering-area=File:Natural_wetland_marsh.png osmcarto-rendering-area-size=100px"@en ;
    skos:inScheme piirritev:Wetland ;
    skos:prefLabel "Marsh"@en .

piirritev:WetlandReedbed a skos:Concept ;
    piirrite:osmId "reedbed" ;
    rdfs:subClassOf piirrite:OsmEntity ;
    skos:definition "An inundated area dominated by certain tall non-woody plants (reeds, bulrushes, cattail). osmcarto-rendering-area=File:Natural_wetland_reed.png osmcarto-rendering-area-size=100px"@en ;
    skos:inScheme piirritev:Wetland ;
    skos:prefLabel "Reedbed"@en .

piirritev:WetlandSaltmarsh a skos:Concept ;
    piirrite:osmId "saltmarsh" ;
    rdfs:subClassOf piirrite:OsmEntity ;
    skos:definition "Either a coastal or dry inland marsh, therefore characterized by herbaceous plants with special adaptations to saline environments. osmcarto-rendering-area=File:Natural_wetland_saltmarsh_100.png osmcarto-rendering-area-size=100px"@en ;
    skos:inScheme piirritev:Wetland ;
    skos:prefLabel "Saltmarsh"@en .

piirritev:WetlandStringBog a skos:Concept ;
    piirrite:osmId "string_bog" ;
    rdfs:subClassOf piirrite:OsmEntity ;
    skos:definition "Bog consisting of slightly elevated ridges and islands, with woody plants, alternating with flat, wet sedge mat areas. osmcarto-rendering-area=File:Natural_wetland_bog.png osmcarto-rendering-area-size=100px"@en ;
    skos:inScheme piirritev:Wetland ;
    skos:prefLabel "String bog"@en .

piirritev:WetlandSwamp a skos:Concept ;
    piirrite:osmId "swamp" ;
    rdfs:subClassOf piirrite:OsmEntity ;
    skos:definition "An area of waterlogged forest, with dense vegetation. osmcarto-rendering-area=File:Natural_wetland_swamp.png osmcarto-rendering-area-size=100px"@en ;
    skos:inScheme piirritev:Wetland ;
    skos:prefLabel "Swamp"@en .

piirritev:WetlandTidalflat a skos:Concept ;
    piirrite:osmId "tidalflat" ;
    rdfs:subClassOf piirrite:OsmEntity ;
    skos:definition "Tidally inundated areas of bare mud or similar sediments. osmcarto-rendering-area=File:Wetland_tidalflat_100.png osmcarto-rendering-area-size=100px"@en ;
    skos:inScheme piirritev:Wetland ;
    skos:prefLabel "Tidalflat"@en .

piirritev:WetlandWetMeadow a skos:Concept ;
    piirrite:osmId "wet_meadow" ;
    rdfs:subClassOf piirrite:OsmEntity ;
    skos:definition "Semi-wetland meadow osmcarto-rendering-area=File:Natural_wetland_marsh.png osmcarto-rendering-area-size=100px"@en ;
    skos:inScheme piirritev:Wetland ;
    skos:prefLabel "Wet meadow"@en .

piirritev:WikimediaCommons a skos:ConceptScheme ;
    piirrite:osmId "wikimedia_commons" ;
    skos:definition "Links to related Wikimedia Commons' media of the feature (syntax File:xxxxxx.xxx / Category:xxxxx)."@en ;
    skos:prefLabel "Wikimedia commons, types"@en .

piirritev:Workrules a skos:ConceptScheme ;
    piirrite:osmId "workrules" ;
    skos:definition "Describes which workrules (law) applies for a piece of railway."@en ;
    skos:prefLabel "Workrules, types"@en .

piirritev:Bus a skos:ConceptScheme ;
    piirrite:osmId "bus" ;
    skos:definition "Legal access permissions for public transport buses, OR the type of public transport vehicle."@en ;
    skos:prefLabel "Bus, types"@en .

piirritev:Colour a skos:ConceptScheme ;
    piirrite:osmId "colour" ;
    skos:definition "The colour associated with the object"@en ;
    skos:prefLabel "Colour, types"@en .

piirritev:Covered a skos:ConceptScheme ;
    piirrite:osmId "covered" ;
    skos:definition "A property to denote if an object is covered by something."@en ;
    skos:prefLabel "Covered, types"@en .

piirritev:Ford a skos:ConceptScheme ;
    piirrite:osmId "ford" ;
    skos:definition "A small part of a highway where a waterway runs over it. osmcarto-rendering=File:Ford.16.svg osmcarto-rendering-size=28px"@en ;
    skos:prefLabel "Ford, types"@en .

piirritev:GolfCart a skos:ConceptScheme ;
    piirrite:osmId "golf_cart" ;
    skos:definition "Access restrictions for golf carts"@en ;
    skos:prefLabel "Golf cart, types"@en .

piirritev:Hazmat a skos:ConceptScheme ;
    piirrite:osmId "hazmat" ;
    skos:definition "Restrictions on vehicles transporting hazardous materials."@en ;
    skos:prefLabel "Hazmat, types"@en .

piirritev:InternetAccess a skos:ConceptScheme ;
    piirrite:osmId "internet_access" ;
    skos:definition "Indicates if an object offers internet access. The access can be with given computers or WLAN access. The only limitation is that the internet access has to be public."@en ;
    skos:prefLabel "Internet access, types"@en .

piirritev:Lcn a skos:ConceptScheme ;
    piirrite:osmId "lcn" ;
    skos:definition ""@en ;
    skos:prefLabel "Lcn, types"@en .

piirritev:Lit a skos:ConceptScheme ;
    piirrite:osmId "lit" ;
    skos:definition "Indicates whether a feature is lit."@en ;
    skos:prefLabel "Lit, types"@en .

piirritev:OfficialName a skos:ConceptScheme ;
    piirrite:osmId "official_name" ;
    skos:definition "The official name of the feature, or the name as used by governments and other official organizations. Usually tagged when object has unwieldy and typically not used name that was officially assigned."@en ;
    skos:prefLabel "Official name, types"@en .

piirritev:Owner a skos:ConceptScheme ;
    piirrite:osmId "owner" ;
    skos:definition "The name of the owner of a given map feature"@en ;
    skos:prefLabel "Owner, types"@en .

piirritev:Placement a skos:ConceptScheme ;
    piirrite:osmId "placement" ;
    skos:definition "Used to specify the placement of the OSM-way relative to the road it represents."@en ;
    skos:prefLabel "Placement, types"@en .

piirritev:PriorityRoad a skos:ConceptScheme ;
    piirrite:osmId "priority_road" ;
    skos:definition "A signposted priority road."@en ;
    skos:prefLabel "Priority road, types"@en .

piirritev:RouteMaster a skos:ConceptScheme ;
    piirrite:osmId "route_master" ;
    skos:definition "Defines the type of vehicle operated on a public transport route_master relation"@en ;
    skos:prefLabel "Route master, types"@en .

piirritev:Smoking a skos:ConceptScheme ;
    piirrite:osmId "smoking" ;
    skos:definition "For marking applicable smoking rules. However, if a law mandates a given smoking rule, that need not be mapped."@en ;
    skos:prefLabel "Smoking, types"@en .

piirritev:StartDate a skos:ConceptScheme ;
    piirrite:osmId "start_date" ;
    skos:definition "Date when feature opened or the construction of the feature finished."@en ;
    skos:prefLabel "Start date, types"@en .

piirritev:Trailblazed a skos:ConceptScheme ;
    piirrite:osmId "trailblazed" ;
    skos:definition "Markings on outdoor paths and trails by signs, markers, poles, cairns or in another way."@en ;
    skos:prefLabel "Trailblazed, types"@en .

piirritev:Aerialway a skos:ConceptScheme ;
    piirrite:osmId "aerialway" ;
    skos:definition "Used for various forms of transport for passengers and goods that use wires, including cable-cars, chair-lifts and drag-lifts."@en ;
    skos:prefLabel "Aerialway, types"@en .

piirritev:Education a skos:ConceptScheme ;
    piirrite:osmId "education" ;
    skos:definition "Sometimes used to map schools, kindergartens, universities, and other educational features."@en ;
    skos:prefLabel "Education, types"@en .

piirritev:Electrified a skos:ConceptScheme ;
    piirrite:osmId "electrified" ;
    skos:definition "Indicates infrastructure to supply vehicles with electricity, on rail tracks or highways."@en ;
    skos:prefLabel "Electrified, types"@en .

piirritev:Junction a skos:ConceptScheme ;
    piirrite:osmId "junction" ;
    skos:definition "Describing the kind of a junction."@en ;
    skos:prefLabel "Junction, types"@en .

piirritev:LocalRef a skos:ConceptScheme ;
    piirrite:osmId "local_ref" ;
    skos:definition "Letters and/or numbers identifying a public transport stop within a larger stop group"@en ;
    skos:prefLabel "Local ref, types"@en .

piirritev:Maxheight a skos:ConceptScheme ;
    piirrite:osmId "maxheight" ;
    skos:definition "The legal maximum height."@en ;
    skos:prefLabel "Maxheight, types"@en .

piirritev:Moped a skos:ConceptScheme ;
    piirrite:osmId "moped" ;
    skos:definition "Access permission for mopeds"@en ;
    skos:prefLabel "Moped, types"@en .

piirritev:ParkingSpace a skos:ConceptScheme ;
    piirrite:osmId "parking_space" ;
    skos:definition "Indicates the type of the parking space."@en ;
    skos:prefLabel "Parking space, types"@en .

piirritev:Room a skos:ConceptScheme ;
    piirrite:osmId "room" ;
    skos:definition "Defines the function of a given room."@en ;
    skos:prefLabel "Room, types"@en .

piirritev:Shoulder a skos:ConceptScheme ;
    piirrite:osmId "shoulder" ;
    skos:definition "Presence of shoulder in highway"@en ;
    skos:prefLabel "Shoulder, types"@en .

piirritev:Side a skos:ConceptScheme ;
    piirrite:osmId "side" ;
    skos:definition "Specifies which side of a way an associated feature is located."@en ;
    skos:prefLabel "Side, types"@en .

piirritev:Status a skos:ConceptScheme ;
    piirrite:osmId "status" ;
    skos:definition "group="@en ;
    skos:prefLabel "Status, types"@en .

piirritev:Age a skos:ConceptScheme ;
    piirrite:osmId "age" ;
    skos:definition "Describes the maturity of a tree."@en ;
    skos:prefLabel "Age, types"@en .

piirritev:Bridge a skos:ConceptScheme ;
    piirrite:osmId "bridge" ;
    skos:definition "A bridge is an artificial construction that spans features such as roads, railways, paths, waterways or valleys and carries a road, railway or other feature."@en ;
    skos:prefLabel "Bridge, types"@en .

piirritev:Condition a skos:ConceptScheme ;
    piirrite:osmId "condition" ;
    skos:definition "Describes the physical condition of an object (good, bad)"@en ;
    skos:prefLabel "Condition, types"@en .

piirritev:CrossingRef a skos:ConceptScheme ;
    piirrite:osmId "crossing_ref" ;
    skos:definition "Used to reference a specific type of crossing."@en ;
    skos:prefLabel "Crossing ref, types"@en .

piirritev:Designation a skos:ConceptScheme ;
    piirrite:osmId "designation" ;
    skos:definition "The legal classification of an object, usually used on key:highway features."@en ;
    skos:prefLabel "Designation, types"@en .

piirritev:Hfcs a skos:ConceptScheme ;
    piirrite:osmId "HFCS" ;
    skos:definition "The highway functional classification of a road in the United States as designated by a state department of transportation."@en ;
    skos:prefLabel "Hfcs, types"@en .

piirritev:Proposed a skos:ConceptScheme ;
    piirrite:osmId "proposed" ;
    skos:definition "The proposed tag may be used for any road, railway or route that is in planning phase."@en ;
    skos:prefLabel "Proposed, types"@en .

piirritev:Tunnel a skos:ConceptScheme ;
    piirrite:osmId "tunnel" ;
    skos:definition "A tunnel is an underground passageway built for a road or similar."@en ;
    skos:prefLabel "Tunnel, types"@en .

piirritev:Waste a skos:ConceptScheme ;
    piirrite:osmId "waste" ;
    skos:definition "The type of waste in waste disposal."@en ;
    skos:prefLabel "Waste, types"@en .

piirritev:Bollard a skos:ConceptScheme ;
    piirrite:osmId "bollard" ;
    skos:definition "Finer-grained classification of a bollard."@en ;
    skos:prefLabel "Bollard, types"@en .

piirritev:Description a skos:ConceptScheme ;
    piirrite:osmId "description" ;
    skos:definition "To provide additional information about the related element to the end map user."@en ;
    skos:prefLabel "Description, types"@en .

piirritev:Hgv a skos:ConceptScheme ;
    piirrite:osmId "hgv" ;
    skos:definition "Access permission for heavy goods vehicle; in most countries goods vehicles with a permissible maximum mass over 3.5 tonnes"@en ;
    skos:prefLabel "Hgv, types"@en .

piirritev:Import a skos:ConceptScheme ;
    piirrite:osmId "import" ;
    skos:definition "Unnecessary duplicate of key:source."@en ;
    skos:prefLabel "Import, types"@en .

piirritev:Landcover a skos:ConceptScheme ;
    piirrite:osmId "landcover" ;
    skos:definition "A key to describe the physical coverage of an area."@en ;
    skos:prefLabel "Landcover, types"@en .

piirritev:LeafType a skos:ConceptScheme ;
    piirrite:osmId "leaf_type" ;
    skos:definition "Describes the type of leaves"@en ;
    skos:prefLabel "Leaf type, types"@en .

piirritev:LoadingGauge a skos:ConceptScheme ;
    piirrite:osmId "loading_gauge" ;
    skos:definition "Used to show what freight wagons can go on a track."@en ;
    skos:prefLabel "Loading gauge, types"@en .

piirritev:SocialFacility a skos:ConceptScheme ;
    piirrite:osmId "social_facility" ;
    skos:definition "Specifies the type of a facility that provides social services."@en ;
    skos:prefLabel "Social facility, types"@en .

piirritev:Utility a skos:ConceptScheme ;
    piirrite:osmId "utility" ;
    skos:definition "Specifies the type of utility infrastructure which a feature represents."@en ;
    skos:prefLabel "Utility, types"@en .

piirritev:Vehicle a skos:ConceptScheme ;
    piirrite:osmId "vehicle" ;
    skos:definition "Access permission for all vehicles"@en ;
    skos:prefLabel "Vehicle, types"@en .

piirritev:BicycleParking a skos:ConceptScheme ;
    piirrite:osmId "bicycle_parking" ;
    skos:definition "For describing the type of bicycle parking."@en ;
    skos:prefLabel "Bicycle parking, types"@en .

piirritev:LeafCycle a skos:ConceptScheme ;
    piirrite:osmId "leaf_cycle" ;
    skos:definition "Describes the phenology of leaves"@en ;
    skos:prefLabel "Leaf cycle, types"@en .

piirritev:BoardType a skos:ConceptScheme ;
    piirrite:osmId "board_type" ;
    skos:definition "Specifies the details of an tag:information=board"@en ;
    skos:prefLabel "Board type, types"@en .

piirritev:Foot a skos:ConceptScheme ;
    piirrite:osmId "foot" ;
    skos:definition "Access permission for pedestrians"@en ;
    skos:prefLabel "Foot, types"@en .

piirritev:House a skos:ConceptScheme ;
    piirrite:osmId "house" ;
    skos:definition "The type of a house. Used in combination with tag:building=house."@en ;
    skos:prefLabel "House, types"@en .

piirritev:Indoor a skos:ConceptScheme ;
    piirrite:osmId "indoor" ;
    skos:definition "Key used with the Simple Indoor Tagging scheme."@en ;
    skos:prefLabel "Indoor, types"@en .

piirritev:LampMount a skos:ConceptScheme ;
    piirrite:osmId "lamp_mount" ;
    skos:definition "Lamp holder of a street lamp"@en ;
    skos:prefLabel "Lamp mount, types"@en .

piirritev:LampType a skos:ConceptScheme ;
    piirrite:osmId "lamp_type" ;
    skos:definition "Type of lamp."@en ;
    skos:prefLabel "Lamp type, types"@en .

piirritev:Navigationaid a skos:ConceptScheme ;
    piirrite:osmId "navigationaid" ;
    skos:definition "A type of facility that supports navigation for aircraft"@en ;
    skos:prefLabel "Navigationaid, types"@en .

piirritev:Attribution a skos:ConceptScheme ;
    piirrite:osmId "attribution" ;
    skos:definition "The data source of the information used to tag and/or place this element (often considered deprecated)"@en ;
    skos:prefLabel "Attribution, types"@en .

piirritev:Fixme a skos:ConceptScheme ;
    piirrite:osmId "fixme" ;
    skos:definition "Description of a (possible) error in the map."@en ;
    skos:prefLabel "Fixme, types"@en .

piirritev:Footway a skos:ConceptScheme ;
    piirrite:osmId "footway" ;
    skos:definition "Further refinement of footways"@en ;
    skos:prefLabel "Footway, types"@en .

piirritev:Information a skos:ConceptScheme ;
    piirrite:osmId "information" ;
    skos:definition "Refines detail for tag:tourism=information."@en ;
    skos:prefLabel "Information, types"@en .

piirritev:Note a skos:ConceptScheme ;
    piirrite:osmId "note" ;
    skos:definition "A note to yourself or to other mappers."@en ;
    skos:prefLabel "Note, types"@en .

piirritev:IntRef a skos:ConceptScheme ;
    piirrite:osmId "int_ref" ;
    skos:definition "International reference number or code on roads, highway exits, routes, etc."@en ;
    skos:prefLabel "Int ref, types"@en .

piirritev:Golf a skos:ConceptScheme ;
    piirrite:osmId "golf" ;
    skos:definition "To map the details on a golf course"@en ;
    skos:prefLabel "Golf, types"@en .

piirritev:Crop a skos:ConceptScheme ;
    piirrite:osmId "crop" ;
    skos:definition "The crop produced by cultivated land."@en ;
    skos:prefLabel "Crop, types"@en .

piirritev:Denotation a skos:ConceptScheme ;
    piirrite:osmId "denotation" ;
    skos:definition "Defines the denotation of a tree"@en ;
    skos:prefLabel "Denotation, types"@en .

piirritev:FenceType a skos:ConceptScheme ;
    piirrite:osmId "fence_type" ;
    skos:definition "Describes the type of a fence."@en ;
    skos:prefLabel "Fence type, types"@en .

piirritev:Wetland a skos:ConceptScheme ;
    piirrite:osmId "wetland" ;
    skos:definition "Type of wetland."@en ;
    skos:prefLabel "Wetland, types"@en .

piirritev:Direction a skos:ConceptScheme ;
    piirrite:osmId "direction" ;
    skos:definition "Specifies the direction of a feature."@en ;
    skos:prefLabel "Direction, types"@en .

piirritev:Location a skos:ConceptScheme ;
    piirrite:osmId "location" ;
    skos:definition "To define the location of a feature which may be above or under ground or in relation to objects such as roofs, bridges or buildings."@en ;
    skos:prefLabel "Location, types"@en .

piirritev:Boundary a skos:ConceptScheme ;
    piirrite:osmId "boundary" ;
    skos:definition "Used to mark the borders of areas, mostly political, but possibly also of other administrative areas."@en ;
    skos:prefLabel "Boundary, types"@en .

piirritev:Emergency a skos:ConceptScheme ;
    piirrite:osmId "emergency" ;
    skos:definition "Describes various emergency services, facilities, amenities or the possibility of access for emergency services"@en ;
    skos:prefLabel "Emergency, types"@en .

piirritev:Service a skos:ConceptScheme ;
    piirrite:osmId "service" ;
    skos:definition "Additional information about a service highway/railway/waterway, or about services offered at a business."@en ;
    skos:prefLabel "Service, types"@en .

piirritev:Aeroway a skos:ConceptScheme ;
    piirrite:osmId "aeroway" ;
    skos:definition "For physical infrastructure used to support aircraft, air travel, spacecraft and space flight."@en ;
    skos:prefLabel "Aeroway, types"@en .

piirritev:Construction a skos:ConceptScheme ;
    piirrite:osmId "construction" ;
    skos:definition "Used together with the top-level tags like tag:highway=construction or tag:building=construction to describe the type of feature which is currently under construction."@en ;
    skos:prefLabel "Construction, types"@en .

piirritev:Denomination a skos:ConceptScheme ;
    piirrite:osmId "denomination" ;
    skos:definition "Defines the subgroup of a specific religion."@en ;
    skos:prefLabel "Denomination, types"@en .

piirritev:CreatedBy a skos:ConceptScheme ;
    piirrite:osmId "created_by" ;
    skos:definition "The editor or script that created the changeset, node, way or relation. Used before 2009, now only on changesets."@en ;
    skos:prefLabel "Created by, types"@en .

piirritev:Barrier a skos:ConceptScheme ;
    piirrite:osmId "barrier" ;
    skos:definition "A barrier is a physical structure which blocks or impedes movement."@en ;
    skos:prefLabel "Barrier, types"@en .

piirritev:Landuse a skos:ConceptScheme ;
    piirrite:osmId "landuse" ;
    skos:definition "Mainly used for describing the primary use of areas of land."@en ;
    skos:prefLabel "Landuse, types"@en .

piirritev:Highway a skos:ConceptScheme ;
    piirrite:osmId "highway" ;
    skos:definition "Used for roads and road-related facilities."@en ;
    skos:prefLabel "Highway, types"@en .

piirritev:Operator a skos:ConceptScheme ;
    piirrite:osmId "operator" ;
    skos:definition "ompany, corporation, person or any other entity who is directly in charge of the current operation of a map object"@en ;
    skos:prefLabel "Operator, types"@en .

piirritev:Building a skos:ConceptScheme ;
    piirrite:osmId "building" ;
    skos:definition "To mark the outline of a building, a man-made structure with a roof, standing more or less permanently in one place.  osmcarto-rendering = File:Area building=yes.png  osmcarto-rendering-size = 28px"@en ;
    skos:prefLabel "Building, types"@en .

piirritev:Amenity a skos:ConceptScheme ;
    piirrite:osmId "amenity" ;
    skos:definition "For describing useful and important facilities for visitors and residents."@en ;
    skos:prefLabel "Amenity, types"@en .

